<?xml version="1.0"?>
<rdf:RDF xmlns="http://data.ign.fr/def/geometrie#"
     xml:base="http://data.ign.fr/def/geometrie"
     xmlns:ns="http://creativecommons.org/ns#"
     xmlns:org="http://www.w3.org/ns/org#"
     xmlns:owl="http://www.w3.org/2002/07/owl#"
     xmlns:rdf="http://www.w3.org/1999/02/22-rdf-syntax-ns#"
     xmlns:xml="http://www.w3.org/XML/1998/namespace"
     xmlns:xsd="http://www.w3.org/2001/XMLSchema#"
     xmlns:foaf="http://xmlns.com/foaf/0.1/"
     xmlns:rdfs="http://www.w3.org/2000/01/rdf-schema#"
     xmlns:time="http://www.w3.org/2006/time#"
     xmlns:vann="http://purl.org/vocab/vann/"
     xmlns:terms="http://purl.org/dc/terms/">
    <owl:Ontology rdf:about="http://data.ign.fr/def/geometrie">
        <ns:license rdf:resource="http://creativecommons.org/licenses/by/2.0/"/>
        <ns:license rdf:resource="http://opendatacommons.org/licenses/by/"/>
        <ns:license rdf:resource="http://www.data.gouv.fr/Licence-Ouverte-Open-Licence"/>
        <terms:contributor rdf:resource="_:genid-nodeid-node1d3jq8du2x108"/>
        <terms:contributor rdf:resource="http://data.semanticweb.org/person/bernard-vatant"/>
        <terms:contributor rdf:resource="http://recherche.ign.fr/labos/cogit/cv.php?prenom=Bénédicte&amp;nom=Bucher"/>
        <terms:contributor rdf:resource="http://www.eurecom.fr/~troncy/"/>
        <terms:creator rdf:resource="_:genid-nodeid-node1d3jq8du2x103"/>
        <terms:creator rdf:resource="http://www.eurecom.fr/~atemezin/"/>
        <terms:description xml:lang="fr">Ontologie des primitives géométriques représentant la forme et la localisation d&apos;entités topographiques.</terms:description>
        <terms:description xml:lang="en">Ontology of geometric primitives representing the shape and location of topographic features.</terms:description>
        <terms:issued rdf:datatype="http://www.w3.org/2001/XMLSchema#date">2013-06-11</terms:issued>
        <terms:modified rdf:datatype="http://www.w3.org/2001/XMLSchema#date">2014-08-22</terms:modified>
        <terms:modified rdf:datatype="http://www.w3.org/2001/XMLSchema#date">2016-06-28</terms:modified>
        <terms:modified rdf:datatype="http://www.w3.org/2001/XMLSchema#date">2019-02-12</terms:modified>
        <terms:publisher rdf:resource="http://fr.dbpedia.org/resource/Institut_national_de_l%27information_g%C3%A9ographique_et_foresti%C3%A8re"/>
        <terms:rights>Copyright 2019, IGN</terms:rights>
        <terms:title xml:lang="fr">Ontologie des primitives géométriques</terms:title>
        <terms:title xml:lang="en">Ontology of geometric primitives</terms:title>
        <vann:preferredNamespacePrefix>geom</vann:preferredNamespacePrefix>
        <vann:preferredNamespaceUri rdf:resource="http://data.ign.fr/def/geometrie#"/>
        <owl:priorVersion rdf:resource="http://data.ign.fr/def/geometrie/20160628.ttl"/>
        <owl:versionInfo>Version 1.2 - 2019-02-12</owl:versionInfo>
    </owl:Ontology>
    


    <!-- 
    ///////////////////////////////////////////////////////////////////////////////////////
    //
    // Annotation properties
    //
    ///////////////////////////////////////////////////////////////////////////////////////
     -->


    


    <!-- http://creativecommons.org/ns#license -->


    <owl:AnnotationProperty rdf:about="http://creativecommons.org/ns#license"/>
    


    <!-- http://purl.org/dc/terms/contributor -->


    <owl:AnnotationProperty rdf:about="http://purl.org/dc/terms/contributor"/>
    


    <!-- http://purl.org/dc/terms/creator -->


    <owl:AnnotationProperty rdf:about="http://purl.org/dc/terms/creator"/>
    


    <!-- http://purl.org/dc/terms/description -->


    <owl:AnnotationProperty rdf:about="http://purl.org/dc/terms/description"/>
    


    <!-- http://purl.org/dc/terms/issued -->


    <owl:AnnotationProperty rdf:about="http://purl.org/dc/terms/issued"/>
    


    <!-- http://purl.org/dc/terms/modified -->


    <owl:AnnotationProperty rdf:about="http://purl.org/dc/terms/modified"/>
    


    <!-- http://purl.org/dc/terms/publisher -->


    <owl:AnnotationProperty rdf:about="http://purl.org/dc/terms/publisher"/>
    


    <!-- http://purl.org/dc/terms/rights -->


    <owl:AnnotationProperty rdf:about="http://purl.org/dc/terms/rights"/>
    


    <!-- http://purl.org/dc/terms/title -->


    <owl:AnnotationProperty rdf:about="http://purl.org/dc/terms/title"/>
    


    <!-- http://purl.org/vocab/vann/preferredNamespacePrefix -->


    <owl:AnnotationProperty rdf:about="http://purl.org/vocab/vann/preferredNamespacePrefix"/>
    


    <!-- http://purl.org/vocab/vann/preferredNamespaceUri -->


    <owl:AnnotationProperty rdf:about="http://purl.org/vocab/vann/preferredNamespaceUri"/>
    


    <!-- http://www.w3.org/2006/time#hasBeginning -->


    <owl:AnnotationProperty rdf:about="http://www.w3.org/2006/time#hasBeginning"/>
    


    <!-- http://www.w3.org/2006/time#inXSDDateTimeStamp -->


    <owl:AnnotationProperty rdf:about="http://www.w3.org/2006/time#inXSDDateTimeStamp"/>
    


    <!-- http://www.w3.org/ns/org#hasMembership -->


    <owl:AnnotationProperty rdf:about="http://www.w3.org/ns/org#hasMembership"/>
    


    <!-- http://www.w3.org/ns/org#memberDuring -->


    <owl:AnnotationProperty rdf:about="http://www.w3.org/ns/org#memberDuring"/>
    


    <!-- http://www.w3.org/ns/org#organization -->


    <owl:AnnotationProperty rdf:about="http://www.w3.org/ns/org#organization"/>
    


    <!-- http://www.w3.org/ns/org#role -->


    <owl:AnnotationProperty rdf:about="http://www.w3.org/ns/org#role"/>
    


    <!-- http://xmlns.com/foaf/0.1/family_name -->


    <owl:AnnotationProperty rdf:about="http://xmlns.com/foaf/0.1/family_name"/>
    


    <!-- http://xmlns.com/foaf/0.1/firstName -->


    <owl:AnnotationProperty rdf:about="http://xmlns.com/foaf/0.1/firstName"/>
    


    <!-- http://xmlns.com/foaf/0.1/mbox -->


    <owl:AnnotationProperty rdf:about="http://xmlns.com/foaf/0.1/mbox"/>
    


    <!-- http://xmlns.com/foaf/0.1/name -->


    <owl:AnnotationProperty rdf:about="http://xmlns.com/foaf/0.1/name"/>
    


    <!-- http://xmlns.com/foaf/0.1/workInfoHomepage -->


    <owl:AnnotationProperty rdf:about="http://xmlns.com/foaf/0.1/workInfoHomepage"/>
    


    <!-- 
    ///////////////////////////////////////////////////////////////////////////////////////
    //
    // Object Properties
    //
    ///////////////////////////////////////////////////////////////////////////////////////
     -->


    


    <!-- http://data.ign.fr/def/geometrie#boundary -->


    <owl:ObjectProperty rdf:about="http://data.ign.fr/def/geometrie#boundary">
        <rdfs:domain rdf:resource="http://data.ign.fr/def/geometrie#Polygon"/>
        <rdfs:range rdf:resource="http://data.ign.fr/def/geometrie#LinearRing"/>
        <rdfs:comment xml:lang="en">Connect a polygon to a ring describing its boundary.</rdfs:comment>
        <rdfs:comment xml:lang="fr">Relie un polygone à un anneau décrivant sa frontière.</rdfs:comment>
        <rdfs:label xml:lang="en">boundary</rdfs:label>
        <rdfs:label xml:lang="fr">frontière</rdfs:label>
    </owl:ObjectProperty>
    


    <!-- http://data.ign.fr/def/geometrie#centroid -->


    <owl:ObjectProperty rdf:about="http://data.ign.fr/def/geometrie#centroid">
        <rdfs:domain rdf:resource="http://data.ign.fr/def/geometrie#Surface"/>
        <rdfs:range rdf:resource="http://data.ign.fr/def/geometrie#Point"/>
        <rdfs:comment xml:lang="en">Centroid of a geometry</rdfs:comment>
        <rdfs:comment xml:lang="fr">Centroide d&apos;une géométrie</rdfs:comment>
        <rdfs:label xml:lang="en">centroid</rdfs:label>
        <rdfs:label xml:lang="fr">centroïde</rdfs:label>
    </owl:ObjectProperty>
    


    <!-- http://data.ign.fr/def/geometrie#crs -->


    <owl:ObjectProperty rdf:about="http://data.ign.fr/def/geometrie#crs">
        <rdfs:domain rdf:resource="http://data.ign.fr/def/geometrie#Geometry"/>
        <rdfs:range rdf:resource="http://data.ign.fr/def/ignf#CRS"/>
        <rdfs:comment xml:lang="en">Coordinate system associated with a geometric primitive.</rdfs:comment>
        <rdfs:comment xml:lang="fr">Système de coordonnées associé à une primitive géométrique.</rdfs:comment>
        <rdfs:label xml:lang="en">coordinate reference system</rdfs:label>
        <rdfs:label xml:lang="fr">système de coordonnées</rdfs:label>
    </owl:ObjectProperty>
    


    <!-- http://data.ign.fr/def/geometrie#envelope -->


    <owl:ObjectProperty rdf:about="http://data.ign.fr/def/geometrie#envelope">
        <rdfs:domain rdf:resource="http://data.ign.fr/def/geometrie#Geometry"/>
        <rdfs:range rdf:resource="http://data.ign.fr/def/geometrie#Envelope"/>
        <rdfs:comment xml:lang="en">Minimal enclosing rectangle of a geometry</rdfs:comment>
        <rdfs:comment xml:lang="fr">Rectangle englobant minimal d&apos;une géométrie</rdfs:comment>
        <rdfs:label xml:lang="en">envelope</rdfs:label>
        <rdfs:label xml:lang="fr">enveloppe</rdfs:label>
    </owl:ObjectProperty>
    


    <!-- http://data.ign.fr/def/geometrie#exterior -->


    <owl:ObjectProperty rdf:about="http://data.ign.fr/def/geometrie#exterior">
        <rdfs:subPropertyOf rdf:resource="http://data.ign.fr/def/geometrie#boundary"/>
        <rdfs:domain rdf:resource="http://data.ign.fr/def/geometrie#Polygon"/>
        <rdfs:range rdf:resource="http://data.ign.fr/def/geometrie#LinearRing"/>
        <rdfs:comment xml:lang="en">Connect a polygon to a ring describing the outer contour of its surface.</rdfs:comment>
        <rdfs:comment xml:lang="fr">Relie un polygone à un anneau décrivant le contour extérieur de sa surface.</rdfs:comment>
        <rdfs:label xml:lang="en">exterior</rdfs:label>
        <rdfs:label xml:lang="fr">extérieur</rdfs:label>
    </owl:ObjectProperty>
    


    <!-- http://data.ign.fr/def/geometrie#firstAndLast -->


    <owl:ObjectProperty rdf:about="http://data.ign.fr/def/geometrie#firstAndLast">
        <rdfs:subPropertyOf rdf:resource="http://www.w3.org/1999/02/22-rdf-syntax-ns#first"/>
        <rdfs:domain rdf:resource="http://data.ign.fr/def/geometrie#PointsList"/>
        <rdfs:range rdf:resource="http://data.ign.fr/def/geometrie#Point"/>
        <rdfs:comment xml:lang="fr">Désigne le point servant de point initial et de point final à une liste circulaire de points.</rdfs:comment>
        <rdfs:comment xml:lang="en">Refers to the point that serves as the start and end point for a circular list of points.</rdfs:comment>
        <rdfs:label xml:lang="en">first and last</rdfs:label>
        <rdfs:label xml:lang="fr">premier et dernier</rdfs:label>
    </owl:ObjectProperty>
    


    <!-- http://data.ign.fr/def/geometrie#geometry -->


    <owl:ObjectProperty rdf:about="http://data.ign.fr/def/geometrie#geometry">
        <rdfs:range rdf:resource="http://data.ign.fr/def/geometrie#Geometry"/>
        <rdfs:comment xml:lang="en">Geometric primitive associated with an object to represent its location and possibly its shape.</rdfs:comment>
        <rdfs:comment xml:lang="fr">Primitive géométrique associée à un objet pour représenter sa localisation et éventuellement sa forme.</rdfs:comment>
        <rdfs:label xml:lang="fr">a pour géométrie</rdfs:label>
        <rdfs:label xml:lang="en">has geometry</rdfs:label>
    </owl:ObjectProperty>
    


    <!-- http://data.ign.fr/def/geometrie#interior -->


    <owl:ObjectProperty rdf:about="http://data.ign.fr/def/geometrie#interior">
        <rdfs:subPropertyOf rdf:resource="http://data.ign.fr/def/geometrie#boundary"/>
        <rdfs:domain rdf:resource="http://data.ign.fr/def/geometrie#Polygon"/>
        <rdfs:range rdf:resource="http://data.ign.fr/def/geometrie#LinearRing"/>
        <rdfs:comment xml:lang="en">Connect a polygon to a ring describing a hole in its surface.</rdfs:comment>
        <rdfs:comment xml:lang="fr">Relie un polygone à un anneau décrivant un trou dans sa surface.</rdfs:comment>
        <rdfs:label xml:lang="en">interior</rdfs:label>
        <rdfs:label xml:lang="fr">intérieur</rdfs:label>
    </owl:ObjectProperty>
    


    <!-- http://data.ign.fr/def/geometrie#lineStringMember -->


    <owl:ObjectProperty rdf:about="http://data.ign.fr/def/geometrie#lineStringMember">
        <rdfs:domain rdf:resource="http://data.ign.fr/def/geometrie#MultiLineString"/>
        <rdfs:range rdf:resource="http://data.ign.fr/def/geometrie#LineString"/>
        <rdfs:comment xml:lang="en">Links a MultiLineString geometry to the linestrings that compose it.</rdfs:comment>
        <rdfs:comment xml:lang="fr">Relie une géométrie de type MultiLineString aux linestrings qui la composent.</rdfs:comment>
        <rdfs:label xml:lang="en">line string member</rdfs:label>
        <rdfs:label xml:lang="fr">polyligne membre</rdfs:label>
    </owl:ObjectProperty>
    


    <!-- http://data.ign.fr/def/geometrie#lowerCorner -->


    <owl:ObjectProperty rdf:about="http://data.ign.fr/def/geometrie#lowerCorner">
        <rdfs:domain rdf:resource="http://data.ign.fr/def/geometrie#Envelope"/>
        <rdfs:range rdf:resource="http://data.ign.fr/def/geometrie#Point"/>
        <rdfs:comment xml:lang="fr">Coin d&apos;une enveloppe correspondant aux valeurs de X et Y les moins élevées.</rdfs:comment>
        <rdfs:comment xml:lang="en">The corner of an envelope corresponding to the lowest values of X and Y.</rdfs:comment>
        <rdfs:label xml:lang="fr">coin inférieur</rdfs:label>
        <rdfs:label xml:lang="en">lower corner</rdfs:label>
    </owl:ObjectProperty>
    


    <!-- http://data.ign.fr/def/geometrie#pointMember -->


    <owl:ObjectProperty rdf:about="http://data.ign.fr/def/geometrie#pointMember">
        <rdfs:domain rdf:resource="http://data.ign.fr/def/geometrie#MultiPoint"/>
        <rdfs:range rdf:resource="http://data.ign.fr/def/geometrie#Point"/>
        <rdfs:comment xml:lang="en">Connect a MultiPoint geometry to the points that compose it.</rdfs:comment>
        <rdfs:comment xml:lang="fr">Relie une géométrie de type MultiPoint aux points qui la composent.</rdfs:comment>
        <rdfs:label xml:lang="en">point member</rdfs:label>
        <rdfs:label xml:lang="fr">point membre</rdfs:label>
    </owl:ObjectProperty>
    


    <!-- http://data.ign.fr/def/geometrie#points -->


    <owl:ObjectProperty rdf:about="http://data.ign.fr/def/geometrie#points">
        <rdfs:domain rdf:resource="http://data.ign.fr/def/geometrie#Curve"/>
        <rdfs:range rdf:resource="http://data.ign.fr/def/geometrie#PointsList"/>
        <rdfs:comment xml:lang="fr">La liste ordonnée des points consitutant une géométrie de type Curve.</rdfs:comment>
        <rdfs:comment xml:lang="en">The ordered list of points constituting a Curve geometry.</rdfs:comment>
        <rdfs:label xml:lang="en">points</rdfs:label>
        <rdfs:label xml:lang="fr">points</rdfs:label>
    </owl:ObjectProperty>
    


    <!-- http://data.ign.fr/def/geometrie#polygonMember -->


    <owl:ObjectProperty rdf:about="http://data.ign.fr/def/geometrie#polygonMember">
        <rdfs:domain rdf:resource="http://data.ign.fr/def/geometrie#MultiPolygon"/>
        <rdfs:range rdf:resource="http://data.ign.fr/def/geometrie#Polygon"/>
        <rdfs:comment xml:lang="en">Connects a MultiPolygon geometry to the polygons that compose it.</rdfs:comment>
        <rdfs:comment xml:lang="fr">Relie une géométrie de type MultiPolygon aux polygones qui la composent.</rdfs:comment>
        <rdfs:label xml:lang="en">polygon member</rdfs:label>
        <rdfs:label xml:lang="fr">polygone membre</rdfs:label>
    </owl:ObjectProperty>
    


    <!-- http://data.ign.fr/def/geometrie#upperCorner -->


    <owl:ObjectProperty rdf:about="http://data.ign.fr/def/geometrie#upperCorner">
        <rdfs:domain rdf:resource="http://data.ign.fr/def/geometrie#Envelope"/>
        <rdfs:range rdf:resource="http://data.ign.fr/def/geometrie#Point"/>
        <rdfs:comment xml:lang="fr">Coin d&apos;une enveloppe correspondant aux valeurs de X et Y les plus élevées.</rdfs:comment>
        <rdfs:comment xml:lang="en">Corner of an envelope corresponding to the highest values of X and Y.</rdfs:comment>
        <rdfs:label xml:lang="fr">coin supérieur</rdfs:label>
        <rdfs:label xml:lang="en">upper corner</rdfs:label>
    </owl:ObjectProperty>
    


    <!-- http://www.w3.org/1999/02/22-rdf-syntax-ns#first -->


    <owl:ObjectProperty rdf:about="http://www.w3.org/1999/02/22-rdf-syntax-ns#first"/>
    


    <!-- http://www.w3.org/1999/02/22-rdf-syntax-ns#rest -->


    <owl:ObjectProperty rdf:about="http://www.w3.org/1999/02/22-rdf-syntax-ns#rest"/>
    


    <!-- 
    ///////////////////////////////////////////////////////////////////////////////////////
    //
    // Data properties
    //
    ///////////////////////////////////////////////////////////////////////////////////////
     -->


    


    <!-- http://data.ign.fr/def/geometrie#coordM -->


    <owl:DatatypeProperty rdf:about="http://data.ign.fr/def/geometrie#coordM">
        <rdfs:domain rdf:resource="http://data.ign.fr/def/geometrie#Point"/>
        <rdfs:range rdf:resource="http://www.w3.org/2001/XMLSchema#double"/>
        <rdfs:comment xml:lang="fr">L&apos;interprétation des coordonnées d&apos;un point dépend du système de coordonnées de référence associé à ce point. La coordonnées M d&apos;un point représente une mesure.</rdfs:comment>
        <rdfs:comment xml:lang="en">The interpretation of the coordinates of a point depends on the reference coordinate system associated with that point. The coordinate M of a point represents a measurement.</rdfs:comment>
        <rdfs:label xml:lang="en">m</rdfs:label>
        <rdfs:label xml:lang="fr">m</rdfs:label>
    </owl:DatatypeProperty>
    


    <!-- http://data.ign.fr/def/geometrie#coordX -->


    <owl:DatatypeProperty rdf:about="http://data.ign.fr/def/geometrie#coordX">
        <rdfs:domain rdf:resource="http://data.ign.fr/def/geometrie#Point"/>
        <rdfs:range rdf:resource="http://www.w3.org/2001/XMLSchema#double"/>
        <rdfs:comment xml:lang="fr">L&apos;interprétation des coordonnées d&apos;un point dépend du système de coordonnées de référence associé à ce point. La propriété coordX désigne la coordonnée définie par rapport au premier axe du système de coordonnées.</rdfs:comment>
        <rdfs:comment xml:lang="en">The interpretation of the coordinates of a point depends on the reference coordinate system associated with that point. The coordX property is the coordinate defined relative to the first axis of the coordinate system.</rdfs:comment>
        <rdfs:label xml:lang="en">x</rdfs:label>
        <rdfs:label xml:lang="fr">x</rdfs:label>
    </owl:DatatypeProperty>
    


    <!-- http://data.ign.fr/def/geometrie#coordY -->


    <owl:DatatypeProperty rdf:about="http://data.ign.fr/def/geometrie#coordY">
        <rdfs:domain rdf:resource="http://data.ign.fr/def/geometrie#Point"/>
        <rdfs:range rdf:resource="http://www.w3.org/2001/XMLSchema#double"/>
        <rdfs:comment xml:lang="fr">L&apos;interprétation des coordonnées d&apos;un point dépend du système de coordonnées de référence associé à ce point. La propriété coordY désigne la coordonnée définie par rapport au deuxième axe du système de coordonnées.</rdfs:comment>
        <rdfs:comment xml:lang="en">The interpretation of the coordinates of a point depends on the reference coordinate system associated with that point. The coordY property is the coordinate defined relative to the second axis of the coordinate system.</rdfs:comment>
        <rdfs:label xml:lang="en">y</rdfs:label>
        <rdfs:label xml:lang="fr">y</rdfs:label>
    </owl:DatatypeProperty>
    


    <!-- http://data.ign.fr/def/geometrie#coordZ -->


    <owl:DatatypeProperty rdf:about="http://data.ign.fr/def/geometrie#coordZ">
        <rdfs:domain rdf:resource="http://data.ign.fr/def/geometrie#Point"/>
        <rdfs:range rdf:resource="http://www.w3.org/2001/XMLSchema#double"/>
        <rdfs:comment xml:lang="fr">L&apos;interprétation des coordonnées d&apos;un point dépend du système de coordonnées de référence associé à ce point. La propriété coordZ désigne la coordonnée définie par rapport au troisième axe du système de coordonnées. La coordonnées Z d&apos;un point représente typiquement, mais pas nécessairement, l&apos;altitude ou la hauteur de ce point.</rdfs:comment>
        <rdfs:comment xml:lang="en">The interpretation of the coordinates of a point depends on the reference coordinate system associated with that point. The coordZ property is the coordinate defined relative to the third axis of the coordinate system. The Z coordinate of a point typically, but not necessarily, represents the altitude or height of that point.</rdfs:comment>
        <rdfs:label xml:lang="en">z</rdfs:label>
        <rdfs:label xml:lang="fr">z</rdfs:label>
    </owl:DatatypeProperty>
    


    <!-- 
    ///////////////////////////////////////////////////////////////////////////////////////
    //
    // Classes
    //
    ///////////////////////////////////////////////////////////////////////////////////////
     -->


    


    <!-- http://data.ign.fr/def/geometrie#Curve -->


    <owl:Class rdf:about="http://data.ign.fr/def/geometrie#Curve">
        <rdfs:subClassOf rdf:resource="http://data.ign.fr/def/geometrie#Geometry"/>
        <rdfs:subClassOf rdf:resource="http://www.opengis.net/ont/sf#Curve"/>
        <rdfs:comment xml:lang="en">Geometric primitive representing a curve. It is not instantiable. It&apos;s specializations are instantiated as an ordered list of points associated with an interpolation function.</rdfs:comment>
        <rdfs:comment xml:lang="fr">Primitive géométrique représentant une courbe. Elle n&apos;est pas instanciable. Ses spécialisations sont instanciées sous la forme d&apos;une liste ordonnée de points associée à une fonction d&apos;interpolation.</rdfs:comment>
        <rdfs:label xml:lang="fr">Courbe</rdfs:label>
        <rdfs:label xml:lang="en">Curve</rdfs:label>
    </owl:Class>
    


    <!-- http://data.ign.fr/def/geometrie#Envelope -->


    <owl:Class rdf:about="http://data.ign.fr/def/geometrie#Envelope">
        <owl:equivalentClass>
            <owl:Class>
                <owl:intersectionOf rdf:parseType="Collection">
                    <owl:Restriction>
                        <owl:onProperty rdf:resource="http://data.ign.fr/def/geometrie#lowerCorner"/>
                        <owl:qualifiedCardinality rdf:datatype="http://www.w3.org/2001/XMLSchema#nonNegativeInteger">1</owl:qualifiedCardinality>
                        <owl:onClass rdf:resource="http://data.ign.fr/def/geometrie#Point"/>
                    </owl:Restriction>
                    <owl:Restriction>
                        <owl:onProperty rdf:resource="http://data.ign.fr/def/geometrie#upperCorner"/>
                        <owl:qualifiedCardinality rdf:datatype="http://www.w3.org/2001/XMLSchema#nonNegativeInteger">1</owl:qualifiedCardinality>
                        <owl:onClass rdf:resource="http://data.ign.fr/def/geometrie#Point"/>
                    </owl:Restriction>
                </owl:intersectionOf>
            </owl:Class>
        </owl:equivalentClass>
        <rdfs:subClassOf rdf:resource="http://data.ign.fr/def/geometrie#Geometry"/>
        <rdfs:comment xml:lang="en">Geometric primitive representing the minimal envelope of a geometry. An envelope is represented by two points: its maximum coordinate corner and its minimal coordinate corner.</rdfs:comment>
        <rdfs:comment xml:lang="fr">Primitive géométrique représentant l&apos;enveloppe minimale d&apos;une géométrie. Une enveloppe est représentée par deux points: son coin de coordonnées maximales et son coin de coordonnées minimales.</rdfs:comment>
        <rdfs:label xml:lang="en">Envelope</rdfs:label>
        <rdfs:label xml:lang="fr">Enveloppe</rdfs:label>
    </owl:Class>
    


    <!-- http://data.ign.fr/def/geometrie#Geometry -->


    <owl:Class rdf:about="http://data.ign.fr/def/geometrie#Geometry">
        <owl:equivalentClass>
            <owl:Restriction>
                <owl:onProperty rdf:resource="http://data.ign.fr/def/geometrie#crs"/>
                <owl:qualifiedCardinality rdf:datatype="http://www.w3.org/2001/XMLSchema#nonNegativeInteger">1</owl:qualifiedCardinality>
                <owl:onClass rdf:resource="http://data.ign.fr/def/ignf#CoordinatesSystem"/>
            </owl:Restriction>
        </owl:equivalentClass>
        <rdfs:subClassOf rdf:resource="http://geovocab.org/geometry#Geometry"/>
        <rdfs:subClassOf rdf:resource="http://www.opengis.net/ont/sf#Geometry"/>
        <rdfs:comment xml:lang="en">Non-instantiable geometric primitive, root of the ontology of geometric primitives. Geometry is associated with a coordinate system and only one.</rdfs:comment>
        <rdfs:comment xml:lang="fr">Primitive géométrique non instanciable, racine de l&apos;ontologie des primitives géométriques. Une géométrie est associée à un système de coordonnées et un seul.</rdfs:comment>
        <rdfs:label xml:lang="en">Geometry</rdfs:label>
        <rdfs:label xml:lang="fr">Géométrie</rdfs:label>
    </owl:Class>
    


    <!-- http://data.ign.fr/def/geometrie#GeometryCollection -->


    <owl:Class rdf:about="http://data.ign.fr/def/geometrie#GeometryCollection">
        <rdfs:subClassOf rdf:resource="http://data.ign.fr/def/geometrie#Geometry"/>
        <rdfs:subClassOf rdf:resource="http://www.opengis.net/ont/sf#GeometryCollection"/>
        <rdfs:comment xml:lang="fr">Collection comprenant un ou plusieurs objets géométriques, sans structure interne. Tous les éléments d&apos;une collection de géométries sont définis dans le même système de coordonnées.</rdfs:comment>
        <rdfs:comment xml:lang="en">Collection comprising one or more geometric objects, without internal structure. All elements of a collection of geometries are defined in the same coordinate system.</rdfs:comment>
        <rdfs:label xml:lang="fr">Collection de géométries</rdfs:label>
        <rdfs:label xml:lang="en">Geometry collection</rdfs:label>
    </owl:Class>
    


    <!-- http://data.ign.fr/def/geometrie#Line -->


    <owl:Class rdf:about="http://data.ign.fr/def/geometrie#Line">
        <owl:equivalentClass>
            <owl:Restriction>
                <owl:onProperty rdf:resource="http://data.ign.fr/def/geometrie#points"/>
                <owl:someValuesFrom>
                    <owl:Class>
                        <owl:intersectionOf rdf:parseType="Collection">
                            <rdf:Description rdf:about="http://data.ign.fr/def/geometrie#PointsList"/>
                            <owl:Restriction>
                                <owl:onProperty rdf:resource="http://www.w3.org/1999/02/22-rdf-syntax-ns#rest"/>
                                <owl:someValuesFrom>
                                    <owl:Class>
                                        <owl:intersectionOf rdf:parseType="Collection">
                                            <rdf:Description rdf:about="http://data.ign.fr/def/geometrie#PointsList"/>
                                            <owl:Restriction>
                                                <owl:onProperty rdf:resource="http://www.w3.org/1999/02/22-rdf-syntax-ns#rest"/>
                                                <owl:hasValue rdf:resource="http://www.w3.org/1999/02/22-rdf-syntax-ns#nil"/>
                                            </owl:Restriction>
                                        </owl:intersectionOf>
                                    </owl:Class>
                                </owl:someValuesFrom>
                            </owl:Restriction>
                        </owl:intersectionOf>
                    </owl:Class>
                </owl:someValuesFrom>
            </owl:Restriction>
        </owl:equivalentClass>
        <rdfs:subClassOf rdf:resource="http://data.ign.fr/def/geometrie#LineString"/>
        <rdfs:subClassOf rdf:resource="http://www.opengis.net/ont/sf#Line"/>
        <rdfs:comment xml:lang="en">Geometric primitive specializing the primitive Polyline and consisting of only two points.</rdfs:comment>
        <rdfs:comment xml:lang="fr">Primitive géométrique spécialisant la primitive Polyligne et composée de seulement deux points.</rdfs:comment>
        <rdfs:label xml:lang="fr">Ligne</rdfs:label>
        <rdfs:label xml:lang="en">Line</rdfs:label>
    </owl:Class>
    


    <!-- http://data.ign.fr/def/geometrie#LineString -->


    <owl:Class rdf:about="http://data.ign.fr/def/geometrie#LineString">
        <owl:equivalentClass>
            <owl:Restriction>
                <owl:onProperty rdf:resource="http://data.ign.fr/def/geometrie#points"/>
                <owl:someValuesFrom rdf:resource="http://data.ign.fr/def/geometrie#PointsList"/>
            </owl:Restriction>
        </owl:equivalentClass>
        <rdfs:subClassOf rdf:resource="http://data.ign.fr/def/geometrie#Curve"/>
        <rdfs:subClassOf rdf:resource="http://www.opengis.net/ont/sf#LineString"/>
        <rdfs:subClassOf>
            <owl:Restriction>
                <owl:onProperty rdf:resource="http://data.ign.fr/def/geometrie#points"/>
                <owl:qualifiedCardinality rdf:datatype="http://www.w3.org/2001/XMLSchema#nonNegativeInteger">1</owl:qualifiedCardinality>
                <owl:onClass rdf:resource="http://data.ign.fr/def/geometrie#PointsList"/>
            </owl:Restriction>
        </rdfs:subClassOf>
        <rdfs:comment xml:lang="en">Geometric primitive specializing the abstract primitive curve. Its points are linked by a linear interpolation function. Each pair of successive points therefore constitutes a straight line segment.</rdfs:comment>
        <rdfs:comment xml:lang="fr">Primitive géométrique spécialisant la primitive abstraite curve. Ses points sont reliés par une fonction d&apos;interpolation linéaire. Chaque paire de points successifs constitue donc un segment de ligne droite.</rdfs:comment>
        <rdfs:label xml:lang="en">Line string</rdfs:label>
        <rdfs:label xml:lang="fr">Polyligne</rdfs:label>
    </owl:Class>
    


    <!-- http://data.ign.fr/def/geometrie#LinearRing -->


    <owl:Class rdf:about="http://data.ign.fr/def/geometrie#LinearRing">
        <owl:equivalentClass>
            <owl:Restriction>
                <owl:onProperty rdf:resource="http://data.ign.fr/def/geometrie#points"/>
                <owl:someValuesFrom>
                    <owl:Class>
                        <owl:intersectionOf rdf:parseType="Collection">
                            <rdf:Description rdf:about="http://data.ign.fr/def/geometrie#PointsList"/>
                            <owl:Restriction>
                                <owl:onProperty rdf:resource="http://data.ign.fr/def/geometrie#firstAndLast"/>
                                <owl:qualifiedCardinality rdf:datatype="http://www.w3.org/2001/XMLSchema#nonNegativeInteger">1</owl:qualifiedCardinality>
                                <owl:onClass rdf:resource="http://data.ign.fr/def/geometrie#Point"/>
                            </owl:Restriction>
                        </owl:intersectionOf>
                    </owl:Class>
                </owl:someValuesFrom>
            </owl:Restriction>
        </owl:equivalentClass>
        <rdfs:subClassOf rdf:resource="http://data.ign.fr/def/geometrie#LineString"/>
        <rdfs:subClassOf rdf:resource="http://www.opengis.net/ont/sf#LinearRing"/>
        <rdfs:comment xml:lang="en">Geometric primitive specializing the primitive Polyline. It is a simple, closed curve.</rdfs:comment>
        <rdfs:comment xml:lang="fr">Primitive géométrique spécialisant la primitive Polyligne. C&apos;est une courbe simple et fermée.</rdfs:comment>
        <rdfs:label xml:lang="fr">Anneau</rdfs:label>
        <rdfs:label xml:lang="en">Linear ring</rdfs:label>
    </owl:Class>
    


    <!-- http://data.ign.fr/def/geometrie#MultiCurve -->


    <owl:Class rdf:about="http://data.ign.fr/def/geometrie#MultiCurve">
        <rdfs:subClassOf rdf:resource="http://data.ign.fr/def/geometrie#GeometryCollection"/>
        <rdfs:subClassOf rdf:resource="http://www.opengis.net/ont/sf#MultiCurve"/>
        <rdfs:comment xml:lang="fr">Collection d&apos;objets géométriques de type Courbe. Cette primitive n&apos;est pas instanciable: elle définit des propriétés pour ses sous-classes.</rdfs:comment>
        <rdfs:comment xml:lang="en">Collection of geometric objects of type Curve. This primitive is not instantiable: it defines properties for its subclasses.</rdfs:comment>
        <rdfs:label xml:lang="en">Multi curve</rdfs:label>
        <rdfs:label xml:lang="fr">Multicourbe</rdfs:label>
    </owl:Class>
    


    <!-- http://data.ign.fr/def/geometrie#MultiLineString -->


    <owl:Class rdf:about="http://data.ign.fr/def/geometrie#MultiLineString">
        <owl:equivalentClass>
            <owl:Restriction>
                <owl:onProperty rdf:resource="http://data.ign.fr/def/geometrie#lineStringMember"/>
                <owl:someValuesFrom rdf:resource="http://data.ign.fr/def/geometrie#LineString"/>
            </owl:Restriction>
        </owl:equivalentClass>
        <rdfs:subClassOf rdf:resource="http://data.ign.fr/def/geometrie#MultiCurve"/>
        <rdfs:subClassOf rdf:resource="http://www.opengis.net/ont/sf#MultiLineString"/>
        <rdfs:comment xml:lang="fr">Collection d&apos;objets géométriques de type Polyligne. C&apos;est une MultiCourbe dont tous les éléments sont des Polylignes.</rdfs:comment>
        <rdfs:comment xml:lang="en">Collection of geometric objects of type Polyline. It&apos;s a MultiCurve whose elements are all Polylines.</rdfs:comment>
        <rdfs:label xml:lang="en">Multi line string</rdfs:label>
        <rdfs:label xml:lang="fr">Multipolyligne</rdfs:label>
    </owl:Class>
    


    <!-- http://data.ign.fr/def/geometrie#MultiPoint -->


    <owl:Class rdf:about="http://data.ign.fr/def/geometrie#MultiPoint">
        <owl:equivalentClass>
            <owl:Restriction>
                <owl:onProperty rdf:resource="http://data.ign.fr/def/geometrie#pointMember"/>
                <owl:someValuesFrom rdf:resource="http://data.ign.fr/def/geometrie#Point"/>
            </owl:Restriction>
        </owl:equivalentClass>
        <rdfs:subClassOf rdf:resource="http://data.ign.fr/def/geometrie#GeometryCollection"/>
        <rdfs:subClassOf rdf:resource="http://www.opengis.net/ont/sf#MultiPoint"/>
        <rdfs:comment xml:lang="fr">Collection d&apos;objets géométriques de type Point, non connectés et non ordonnés. Un multipoint est dit simple si tous ses points sont différents (i.e. ont des coordonnées différentes).</rdfs:comment>
        <rdfs:comment xml:lang="en">Collection of Point geometric objects, unconnected and unordered. A multipoint is said to be simple if all its points are different (i.e. have different coordinates).</rdfs:comment>
        <rdfs:label xml:lang="en">Multi point</rdfs:label>
        <rdfs:label xml:lang="fr">Multipoint</rdfs:label>
    </owl:Class>
    


    <!-- http://data.ign.fr/def/geometrie#MultiPolygon -->


    <owl:Class rdf:about="http://data.ign.fr/def/geometrie#MultiPolygon">
        <owl:equivalentClass>
            <owl:Restriction>
                <owl:onProperty rdf:resource="http://data.ign.fr/def/geometrie#polygonMember"/>
                <owl:someValuesFrom rdf:resource="http://data.ign.fr/def/geometrie#Polygon"/>
            </owl:Restriction>
        </owl:equivalentClass>
        <rdfs:subClassOf rdf:resource="http://data.ign.fr/def/geometrie#MultiSurface"/>
        <rdfs:subClassOf rdf:resource="http://www.opengis.net/ont/sf#MultiPolygon"/>
        <rdfs:comment xml:lang="fr">Collection d&apos;objets géométriques de type Polygone. C&apos;est une MultiSurface dont tous les éléments sont des Polygones.</rdfs:comment>
        <rdfs:comment xml:lang="en">Collection of geometric objects of type Polygon. It is a MultiSurface whose elements are all Polygons.</rdfs:comment>
        <rdfs:label xml:lang="en">Multi polygon</rdfs:label>
        <rdfs:label xml:lang="fr">Multipolygone</rdfs:label>
    </owl:Class>
    


    <!-- http://data.ign.fr/def/geometrie#MultiSurface -->


    <owl:Class rdf:about="http://data.ign.fr/def/geometrie#MultiSurface">
        <rdfs:subClassOf rdf:resource="http://data.ign.fr/def/geometrie#GeometryCollection"/>
        <rdfs:subClassOf rdf:resource="http://www.opengis.net/ont/sf#MultiSurface"/>
        <rdfs:comment xml:lang="fr">Collection d&apos;objets géométriques de type Surface. Cette primitive n&apos;est pas instanciable: elle définit des propriétés pour ses sous classes.</rdfs:comment>
        <rdfs:comment xml:lang="en">Collection of geometric objects of Surface type. This primitive is not instantiable: it defines properties for its subclasses.</rdfs:comment>
        <rdfs:label xml:lang="en">Multi surface</rdfs:label>
        <rdfs:label xml:lang="fr">Multisurface</rdfs:label>
    </owl:Class>
    


    <!-- http://data.ign.fr/def/geometrie#Point -->


    <owl:Class rdf:about="http://data.ign.fr/def/geometrie#Point">
        <owl:equivalentClass>
            <owl:Class>
                <owl:intersectionOf rdf:parseType="Collection">
                    <owl:Restriction>
                        <owl:onProperty rdf:resource="http://data.ign.fr/def/geometrie#coordX"/>
                        <owl:qualifiedCardinality rdf:datatype="http://www.w3.org/2001/XMLSchema#nonNegativeInteger">1</owl:qualifiedCardinality>
                        <owl:onDataRange rdf:resource="http://www.w3.org/2001/XMLSchema#double"/>
                    </owl:Restriction>
                    <owl:Restriction>
                        <owl:onProperty rdf:resource="http://data.ign.fr/def/geometrie#coordY"/>
                        <owl:qualifiedCardinality rdf:datatype="http://www.w3.org/2001/XMLSchema#nonNegativeInteger">1</owl:qualifiedCardinality>
                        <owl:onDataRange rdf:resource="http://www.w3.org/2001/XMLSchema#double"/>
                    </owl:Restriction>
                    <owl:Restriction>
                        <owl:onProperty rdf:resource="http://data.ign.fr/def/geometrie#coordM"/>
                        <owl:maxQualifiedCardinality rdf:datatype="http://www.w3.org/2001/XMLSchema#nonNegativeInteger">1</owl:maxQualifiedCardinality>
                        <owl:onDataRange rdf:resource="http://www.w3.org/2001/XMLSchema#double"/>
                    </owl:Restriction>
                    <owl:Restriction>
                        <owl:onProperty rdf:resource="http://data.ign.fr/def/geometrie#coordZ"/>
                        <owl:maxQualifiedCardinality rdf:datatype="http://www.w3.org/2001/XMLSchema#nonNegativeInteger">1</owl:maxQualifiedCardinality>
                        <owl:onDataRange rdf:resource="http://www.w3.org/2001/XMLSchema#double"/>
                    </owl:Restriction>
                </owl:intersectionOf>
            </owl:Class>
        </owl:equivalentClass>
        <rdfs:subClassOf rdf:resource="http://data.ign.fr/def/geometrie#Geometry"/>
        <rdfs:subClassOf rdf:resource="http://www.opengis.net/ont/sf#Point"/>
        <rdfs:comment xml:lang="en">Geometric primitive to represent a geographical position. This position is represented via X and Y coordinates expressed in a given coordinate system. If the coordinate system associated with the point allows it, the point may also have Z and M coordinates.</rdfs:comment>
        <rdfs:comment xml:lang="fr">Primitive géométrique permettant de représenter une position géographique. Cette position est représentée via des coordonnées X et Y exprimées dans un système de coordonnées donné. Si le système de coordonnées associé au point le permet, ce dernier peut également avoir des coordonnées Z et M.</rdfs:comment>
        <rdfs:label xml:lang="en">Point</rdfs:label>
        <rdfs:label xml:lang="fr">Point</rdfs:label>
    </owl:Class>
    


    <!-- http://data.ign.fr/def/geometrie#PointsList -->


    <owl:Class rdf:about="http://data.ign.fr/def/geometrie#PointsList">
        <rdfs:subClassOf>
            <owl:Class>
                <owl:intersectionOf rdf:parseType="Collection">
                    <rdf:Description rdf:about="http://www.w3.org/1999/02/22-rdf-syntax-ns#List"/>
                    <owl:Restriction>
                        <owl:onProperty rdf:resource="http://www.w3.org/1999/02/22-rdf-syntax-ns#first"/>
                        <owl:allValuesFrom rdf:resource="http://data.ign.fr/def/geometrie#Point"/>
                    </owl:Restriction>
                    <owl:Restriction>
                        <owl:onProperty rdf:resource="http://www.w3.org/1999/02/22-rdf-syntax-ns#rest"/>
                        <owl:allValuesFrom rdf:resource="http://data.ign.fr/def/geometrie#PointsList"/>
                    </owl:Restriction>
                </owl:intersectionOf>
            </owl:Class>
        </rdfs:subClassOf>
        <rdfs:comment xml:lang="en">List of points</rdfs:comment>
        <rdfs:comment xml:lang="fr">Liste de points.</rdfs:comment>
        <rdfs:label xml:lang="en">List of points</rdfs:label>
        <rdfs:label xml:lang="fr">Liste de points</rdfs:label>
    </owl:Class>
    


    <!-- http://data.ign.fr/def/geometrie#Polygon -->


    <owl:Class rdf:about="http://data.ign.fr/def/geometrie#Polygon">
        <owl:equivalentClass>
            <owl:Restriction>
                <owl:onProperty rdf:resource="http://data.ign.fr/def/geometrie#exterior"/>
                <owl:someValuesFrom rdf:resource="http://data.ign.fr/def/geometrie#LinearRing"/>
            </owl:Restriction>
        </owl:equivalentClass>
        <rdfs:subClassOf rdf:resource="http://data.ign.fr/def/geometrie#Surface"/>
        <rdfs:subClassOf rdf:resource="http://www.opengis.net/ont/sf#Polygon"/>
        <rdfs:subClassOf>
            <owl:Class>
                <owl:intersectionOf rdf:parseType="Collection">
                    <owl:Restriction>
                        <owl:onProperty rdf:resource="http://data.ign.fr/def/geometrie#interior"/>
                        <owl:someValuesFrom rdf:resource="http://data.ign.fr/def/geometrie#LinearRing"/>
                    </owl:Restriction>
                    <owl:Restriction>
                        <owl:onProperty rdf:resource="http://data.ign.fr/def/geometrie#exterior"/>
                        <owl:qualifiedCardinality rdf:datatype="http://www.w3.org/2001/XMLSchema#nonNegativeInteger">1</owl:qualifiedCardinality>
                        <owl:onClass rdf:resource="http://data.ign.fr/def/geometrie#LinearRing"/>
                    </owl:Restriction>
                </owl:intersectionOf>
            </owl:Class>
        </rdfs:subClassOf>
        <rdfs:comment xml:lang="en">Geometric primitive specializing Surface primitive. It is a flat surface defined by an outer boundary and zero or more interior boundaries. Each inner boundary defines a hole in the polygon.</rdfs:comment>
        <rdfs:comment xml:lang="fr">Primitive géométrique spécialisant la primitive Surface. C&apos;est une surface plane définie par une frontière extérieure et zéro ou plusieurs frontières intérieures. Chaque frontière intérieure définit un trou dans le polygone.</rdfs:comment>
        <rdfs:label xml:lang="en">Polygon</rdfs:label>
        <rdfs:label xml:lang="fr">Polygone</rdfs:label>
    </owl:Class>
    


    <!-- http://data.ign.fr/def/geometrie#Surface -->


    <owl:Class rdf:about="http://data.ign.fr/def/geometrie#Surface">
        <rdfs:subClassOf rdf:resource="http://data.ign.fr/def/geometrie#Geometry"/>
        <rdfs:subClassOf rdf:resource="http://www.opengis.net/ont/sf#Surface"/>
        <rdfs:comment xml:lang="en">Geometric primitive locally representing a continuous image of a region of a plane. It is not instantiable. The outline of a surface is a set of closed curves corresponding to its boundaries.</rdfs:comment>
        <rdfs:comment xml:lang="fr">Primitive géométrique représentant localement une image continue d&apos;une région d&apos;un plan. Elle n&apos;est pas instanciable. Le contour d&apos;une surface est un ensemble de courbes fermées correspondant à ses frontières.</rdfs:comment>
        <rdfs:label xml:lang="en">Surface</rdfs:label>
        <rdfs:label xml:lang="fr">Surface</rdfs:label>
    </owl:Class>
    


    <!-- http://data.ign.fr/def/ignf#CRS -->


    <owl:Class rdf:about="http://data.ign.fr/def/ignf#CRS"/>
    


    <!-- http://data.ign.fr/def/ignf#CoordinatesSystem -->


    <owl:Class rdf:about="http://data.ign.fr/def/ignf#CoordinatesSystem"/>
    


    <!-- http://geovocab.org/geometry#Geometry -->


    <owl:Class rdf:about="http://geovocab.org/geometry#Geometry"/>
    


    <!-- http://www.opengis.net/ont/sf#Curve -->


    <owl:Class rdf:about="http://www.opengis.net/ont/sf#Curve"/>
    


    <!-- http://www.opengis.net/ont/sf#Geometry -->


    <owl:Class rdf:about="http://www.opengis.net/ont/sf#Geometry"/>
    


    <!-- http://www.opengis.net/ont/sf#GeometryCollection -->


    <owl:Class rdf:about="http://www.opengis.net/ont/sf#GeometryCollection"/>
    


    <!-- http://www.opengis.net/ont/sf#Line -->


    <owl:Class rdf:about="http://www.opengis.net/ont/sf#Line"/>
    


    <!-- http://www.opengis.net/ont/sf#LineString -->


    <owl:Class rdf:about="http://www.opengis.net/ont/sf#LineString"/>
    


    <!-- http://www.opengis.net/ont/sf#LinearRing -->


    <owl:Class rdf:about="http://www.opengis.net/ont/sf#LinearRing"/>
    


    <!-- http://www.opengis.net/ont/sf#MultiCurve -->


    <owl:Class rdf:about="http://www.opengis.net/ont/sf#MultiCurve"/>
    


    <!-- http://www.opengis.net/ont/sf#MultiLineString -->


    <owl:Class rdf:about="http://www.opengis.net/ont/sf#MultiLineString"/>
    


    <!-- http://www.opengis.net/ont/sf#MultiPoint -->


    <owl:Class rdf:about="http://www.opengis.net/ont/sf#MultiPoint"/>
    


    <!-- http://www.opengis.net/ont/sf#MultiPolygon -->


    <owl:Class rdf:about="http://www.opengis.net/ont/sf#MultiPolygon"/>
    


    <!-- http://www.opengis.net/ont/sf#MultiSurface -->


    <owl:Class rdf:about="http://www.opengis.net/ont/sf#MultiSurface"/>
    


    <!-- http://www.opengis.net/ont/sf#Point -->


    <owl:Class rdf:about="http://www.opengis.net/ont/sf#Point"/>
    


    <!-- http://www.opengis.net/ont/sf#Polygon -->


    <owl:Class rdf:about="http://www.opengis.net/ont/sf#Polygon"/>
    


    <!-- http://www.opengis.net/ont/sf#Surface -->


    <owl:Class rdf:about="http://www.opengis.net/ont/sf#Surface"/>
    


    <!-- http://www.w3.org/1999/02/22-rdf-syntax-ns#List -->


    <owl:Class rdf:about="http://www.w3.org/1999/02/22-rdf-syntax-ns#List"/>
    


    <!-- http://www.w3.org/2006/time#Instant -->


    <owl:Class rdf:about="http://www.w3.org/2006/time#Instant"/>
    


    <!-- http://www.w3.org/2006/time#Interval -->


    <owl:Class rdf:about="http://www.w3.org/2006/time#Interval"/>
    


    <!-- http://www.w3.org/ns/org#Membership -->


    <owl:Class rdf:about="http://www.w3.org/ns/org#Membership"/>
    


    <!-- http://www.w3.org/ns/org#Role -->


    <owl:Class rdf:about="http://www.w3.org/ns/org#Role"/>
    


    <!-- http://xmlns.com/foaf/0.1/Person -->


    <owl:Class rdf:about="http://xmlns.com/foaf/0.1/Person"/>
    


    <!-- 
    ///////////////////////////////////////////////////////////////////////////////////////
    //
    // Individuals
    //
    ///////////////////////////////////////////////////////////////////////////////////////
     -->


    


    <!-- http://data.semanticweb.org/person/bernard-vatant -->


    <owl:NamedIndividual rdf:about="http://data.semanticweb.org/person/bernard-vatant">
        <rdf:type rdf:resource="http://xmlns.com/foaf/0.1/Person"/>
    </owl:NamedIndividual>
    


    <!-- http://recherche.ign.fr/labos/cogit/cv.php?prenom=Bénédicte&amp;nom=Bucher -->


    <owl:NamedIndividual rdf:about="http://recherche.ign.fr/labos/cogit/cv.php?prenom=Bénédicte&amp;nom=Bucher">
        <rdf:type rdf:resource="http://xmlns.com/foaf/0.1/Person"/>
    </owl:NamedIndividual>
    


    <!-- http://www.eurecom.fr/~atemezin/ -->


    <owl:NamedIndividual rdf:about="http://www.eurecom.fr/~atemezin/">
        <rdf:type rdf:resource="http://xmlns.com/foaf/0.1/Person"/>
    </owl:NamedIndividual>
    


    <!-- http://www.eurecom.fr/~troncy/ -->


    <owl:NamedIndividual rdf:about="http://www.eurecom.fr/~troncy/">
        <rdf:type rdf:resource="http://xmlns.com/foaf/0.1/Person"/>
    </owl:NamedIndividual>
    


    <!-- http://www.w3.org/1999/02/22-rdf-syntax-ns#nil -->


    <owl:NamedIndividual rdf:about="http://www.w3.org/1999/02/22-rdf-syntax-ns#nil"/>
    <rdf:Description rdf:nodeID="genid47">
        <rdf:type rdf:resource="http://xmlns.com/foaf/0.1/Person"/>
        <org:hasMembership>
            <rdf:Description rdf:nodeID="genid48">
                <rdf:type rdf:resource="http://www.w3.org/ns/org#Membership"/>
                <org:memberDuring>
                    <rdf:Description rdf:nodeID="genid49">
                        <rdf:type rdf:resource="http://www.w3.org/2006/time#Interval"/>
                        <time:hasBeginning>
                            <rdf:Description rdf:nodeID="genid50">
                                <rdf:type rdf:resource="http://www.w3.org/2006/time#Instant"/>
                                <time:inXSDDateTimeStamp rdf:datatype="http://www.w3.org/2001/XMLSchema#dateTimeStamp">2005-09-09</time:inXSDDateTimeStamp>
                            </rdf:Description>
                        </time:hasBeginning>
                    </rdf:Description>
                </org:memberDuring>
                <org:organization rdf:resource="http://recherche.ign.fr/"/>
                <org:organization rdf:resource="http://www.ign.fr/"/>
                <org:role>
                    <rdf:Description rdf:nodeID="genid51">
                        <rdf:type rdf:resource="http://www.w3.org/ns/org#Role"/>
                        <rdfs:label xml:lang="fr">Chargée de recherche</rdfs:label>
                        <rdfs:label xml:lang="en">Survey engineer and Scientist</rdfs:label>
                    </rdf:Description>
                </org:role>
            </rdf:Description>
        </org:hasMembership>
        <foaf:family_name>Abadie</foaf:family_name>
        <foaf:firstName>Nathalie</foaf:firstName>
        <foaf:mbox rdf:resource="mailto:nathalie-f.abadie@ign.fr"/>
        <foaf:name>Nathalie Abadie</foaf:name>
        <foaf:workInfoHomepage rdf:resource="http://recherche.ign.fr/labos/cogit/cv.php?prenom=Nathalie&amp;nom=Abadie"/>
    </rdf:Description>
    <rdf:Description rdf:nodeID="genid52">
        <rdf:type rdf:resource="http://xmlns.com/foaf/0.1/Person"/>
        <org:hasMembership>
            <rdf:Description rdf:nodeID="genid53">
                <rdf:type rdf:resource="http://www.w3.org/ns/org#Membership"/>
                <org:memberDuring>
                    <rdf:Description rdf:nodeID="genid54">
                        <rdf:type rdf:resource="http://www.w3.org/2006/time#Interval"/>
                        <time:hasBeginning>
                            <rdf:Description rdf:nodeID="genid55">
                                <rdf:type rdf:resource="http://www.w3.org/2006/time#Instant"/>
                                <time:inXSDDateTimeStamp rdf:datatype="http://www.w3.org/2001/XMLSchema#dateTimeStamp">2014-04-01T00:00:00+08:00</time:inXSDDateTimeStamp>
                            </rdf:Description>
                        </time:hasBeginning>
                    </rdf:Description>
                </org:memberDuring>
                <org:organization rdf:resource="http://dbpedia.org/resource/JPL"/>
                <org:organization rdf:resource="https://www.jpl.nasa.gov"/>
                <org:role>
                    <rdf:Description rdf:nodeID="genid56">
                        <rdf:type rdf:resource="http://www.w3.org/ns/org#Role"/>
                        <rdfs:label>Data Scientist</rdfs:label>
                    </rdf:Description>
                </org:role>
            </rdf:Description>
        </org:hasMembership>
        <foaf:family_name>McGibbney</foaf:family_name>
        <foaf:firstName>Lewis J</foaf:firstName>
        <foaf:mbox rdf:resource="mailto:lewis.j.mcgibbney@jpl.nasa.gov"/>
        <foaf:name>Lewis John McGibbney</foaf:name>
    </rdf:Description>
</rdf:RDF>



<!-- Generated by the OWL API (version 5.1.9) https://github.com/owlcs/owlapi/ -->


