<?xml version="1.0"?>
<rdf:RDF xmlns="https://www.gleif.org/ontology/Base/"
     xml:base="https://www.gleif.org/ontology/Base/"
     xmlns:owl="http://www.w3.org/2002/07/owl#"
     xmlns:rdf="http://www.w3.org/1999/02/22-rdf-syntax-ns#"
     xmlns:xml="http://www.w3.org/XML/1998/namespace"
     xmlns:xsd="http://www.w3.org/2001/XMLSchema#"
     xmlns:Base="https://www.gleif.org/ontology/Base/"
     xmlns:rdfs="http://www.w3.org/2000/01/rdf-schema#"
     xmlns:skos="http://www.w3.org/2004/02/skos/core#"
     xmlns:vann="http://purl.org/vocab/vann/"
     xmlns:terms="http://purl.org/dc/terms/"
     xmlns:SpecificationMetadata="http://www.omg.org/techprocess/ab/SpecificationMetadata/">
    <owl:Ontology rdf:about="https://www.gleif.org/ontology/Base/">
        <owl:versionIRI rdf:resource="https://www.gleif.org/ontology/Base-v1.0/Base/"/>
        <owl:imports rdf:resource="https://www.omg.org/spec/LCC/Countries/CountryRepresentation/"/>
        <terms:abstract xml:lang="en">Ontology defining generic concepts for reuse by other Global Legal Entity Identifier Foundation (GLEIF) ontologies. It defines generic classes for (legal) Entities and their relationships and statuses; and generic properties for different types of name and address. It makes use of the OMG Languages Countries and Codes (LCC) ontology (based on the ISO 3166 standard) for country and region information.</terms:abstract>
        <terms:contributor rdf:resource="http://www.workingontologist.com"/>
        <terms:contributor rdf:resource="http://purl.org/bryon"/>
        <terms:contributor rdf:resource="https://www.linkedin.com/in/peterivett/"/>
        <terms:creator rdf:resource="https://www.gleif.org/ontology/Base/GLEIF"/>
        <terms:issued rdf:datatype="http://www.w3.org/2001/XMLSchema#dateTime">2019-02-01T00:00:00+00:00</terms:issued>
        <terms:license rdf:datatype="http://www.w3.org/2001/XMLSchema#anyURI">https://www.gleif.org/en/meta/lei-data-terms-of-use/</terms:license>
        <terms:rights>Copyright (c) 2019 Global Legal Entity Identifier Foundation (GLEIF)</terms:rights>
        <terms:rightsHolder rdf:resource="https://www.gleif.org/ontology/Base/GLEIF"/>
        <terms:source rdf:datatype="http://www.w3.org/2001/XMLSchema#anyURI">https://www.gleif.org/en/about-lei/common-data-file-format/lei-cdf-format/lei-cdf-format-version-2-1</terms:source>
        <terms:title xml:lang="en">Global Legal Entity Identifier Foundation Base Ontology</terms:title>
        <vann:preferredNamespacePrefix>gleif-base</vann:preferredNamespacePrefix>
        <vann:preferredNamespaceUri>https://www.gleif.org/ontology/Base/</vann:preferredNamespaceUri>
        <rdfs:label xml:lang="en">GLEIF Base Ontology</rdfs:label>
    </owl:Ontology>
    


    <!-- 
    ///////////////////////////////////////////////////////////////////////////////////////
    //
    // Annotation properties
    //
    ///////////////////////////////////////////////////////////////////////////////////////
     -->


    


    <!-- http://purl.org/dc/terms/rightsHolder -->


    <owl:AnnotationProperty rdf:about="http://purl.org/dc/terms/rightsHolder"/>
    


    <!-- http://purl.org/vocab/vann/preferredNamespacePrefix -->


    <owl:AnnotationProperty rdf:about="http://purl.org/vocab/vann/preferredNamespacePrefix"/>
    


    <!-- http://purl.org/vocab/vann/preferredNamespaceUri -->


    <owl:AnnotationProperty rdf:about="http://purl.org/vocab/vann/preferredNamespaceUri"/>
    


    <!-- https://www.gleif.org/ontology/Base/hasAbbreviation -->


    <owl:AnnotationProperty rdf:about="https://www.gleif.org/ontology/Base/hasAbbreviation">
        <rdfs:subPropertyOf rdf:resource="http://www.w3.org/2004/02/skos/core#altLabel"/>
    </owl:AnnotationProperty>
    


    <!-- https://www.gleif.org/ontology/Base/hasLegalName -->


    <owl:AnnotationProperty rdf:about="https://www.gleif.org/ontology/Base/hasLegalName"/>
    


    <!-- https://www.gleif.org/ontology/Base/hasName -->


    <owl:AnnotationProperty rdf:about="https://www.gleif.org/ontology/Base/hasName">
        <rdfs:subPropertyOf rdf:resource="http://www.w3.org/2000/01/rdf-schema#label"/>
    </owl:AnnotationProperty>
    


    <!-- https://www.gleif.org/ontology/Base/hasNameAdditional -->


    <owl:AnnotationProperty rdf:about="https://www.gleif.org/ontology/Base/hasNameAdditional">
        <rdfs:subPropertyOf rdf:resource="http://www.w3.org/2004/02/skos/core#altLabel"/>
    </owl:AnnotationProperty>
    


    <!-- https://www.gleif.org/ontology/Base/hasNameLegalLocal -->


    <owl:AnnotationProperty rdf:about="https://www.gleif.org/ontology/Base/hasNameLegalLocal">
        <rdfs:subPropertyOf rdf:resource="http://www.w3.org/2004/02/skos/core#prefLabel"/>
    </owl:AnnotationProperty>
    


    <!-- https://www.gleif.org/ontology/Base/hasNameTransliterated -->


    <owl:AnnotationProperty rdf:about="https://www.gleif.org/ontology/Base/hasNameTransliterated">
        <rdfs:subPropertyOf rdf:resource="http://www.w3.org/2004/02/skos/core#altLabel"/>
    </owl:AnnotationProperty>
    


    <!-- 
    ///////////////////////////////////////////////////////////////////////////////////////
    //
    // Object Properties
    //
    ///////////////////////////////////////////////////////////////////////////////////////
     -->


    


    <!-- https://www.gleif.org/ontology/Base/hasAddress -->


    <owl:ObjectProperty rdf:about="https://www.gleif.org/ontology/Base/hasAddress">
        <rdfs:domain rdf:resource="https://www.gleif.org/ontology/Base/Entity"/>
        <rdfs:range rdf:resource="https://www.gleif.org/ontology/Base/PhysicalAddress"/>
        <rdfs:isDefinedBy rdf:resource="https://www.gleif.org/ontology/Base/"/>
        <rdfs:label>has address</rdfs:label>
        <skos:definition>Has a means by which the entity may be located or contacted or may receive correspondence.</skos:definition>
    </owl:ObjectProperty>
    


    <!-- https://www.gleif.org/ontology/Base/hasAddressHeadquarters -->


    <owl:ObjectProperty rdf:about="https://www.gleif.org/ontology/Base/hasAddressHeadquarters">
        <rdfs:subPropertyOf rdf:resource="https://www.gleif.org/ontology/Base/hasAddress"/>
        <rdfs:isDefinedBy rdf:resource="https://www.gleif.org/ontology/Base/"/>
        <rdfs:label>has address headquarters</rdfs:label>
        <skos:definition>An address of the headquarters of the Entity.</skos:definition>
    </owl:ObjectProperty>
    


    <!-- https://www.gleif.org/ontology/Base/hasAddressLegal -->


    <owl:ObjectProperty rdf:about="https://www.gleif.org/ontology/Base/hasAddressLegal">
        <rdfs:subPropertyOf rdf:resource="https://www.gleif.org/ontology/Base/hasAddress"/>
        <rdfs:isDefinedBy rdf:resource="https://www.gleif.org/ontology/Base/"/>
        <rdfs:label>has address legal</rdfs:label>
        <skos:definition>An address of the entity as recorded in the registration of the entity in its legal jurisdiction.</skos:definition>
    </owl:ObjectProperty>
    


    <!-- https://www.gleif.org/ontology/Base/hasAddressTransliterated -->


    <owl:ObjectProperty rdf:about="https://www.gleif.org/ontology/Base/hasAddressTransliterated">
        <rdfs:subPropertyOf rdf:resource="https://www.gleif.org/ontology/Base/hasAddress"/>
        <rdfs:range rdf:resource="https://www.gleif.org/ontology/Base/PhysicalAddressASCII"/>
        <rdfs:isDefinedBy rdf:resource="https://www.gleif.org/ontology/Base/"/>
        <rdfs:label>has address transliterated</rdfs:label>
        <skos:definition>An address which has been converted from original to western text.</skos:definition>
    </owl:ObjectProperty>
    


    <!-- https://www.gleif.org/ontology/Base/hasCountry -->


    <owl:ObjectProperty rdf:about="https://www.gleif.org/ontology/Base/hasCountry">
        <rdfs:subPropertyOf rdf:resource="https://www.gleif.org/ontology/Base/hasGeographicRegion"/>
        <rdfs:domain rdf:resource="https://www.gleif.org/ontology/Base/PhysicalAddress"/>
        <rdfs:range rdf:resource="https://www.omg.org/spec/LCC/Countries/CountryRepresentation/Country"/>
        <rdfs:isDefinedBy rdf:resource="https://www.gleif.org/ontology/Base/"/>
        <rdfs:label>has country</rdfs:label>
        <skos:definition>The country, based on the 2-character ISO 3166-1 country code.</skos:definition>
    </owl:ObjectProperty>
    


    <!-- https://www.gleif.org/ontology/Base/hasCoverageArea -->


    <owl:ObjectProperty rdf:about="https://www.gleif.org/ontology/Base/hasCoverageArea">
        <rdfs:range rdf:resource="https://www.omg.org/spec/LCC/Countries/CountryRepresentation/GeographicRegion"/>
        <rdfs:isDefinedBy rdf:resource="https://www.gleif.org/ontology/Base/"/>
        <rdfs:label>has coverage area</rdfs:label>
        <skos:definition>Indicates a geographic region in which some service is provided, or to which some policy applies, or in which something is available.</skos:definition>
    </owl:ObjectProperty>
    


    <!-- https://www.gleif.org/ontology/Base/hasEntityExpirationReason -->


    <owl:ObjectProperty rdf:about="https://www.gleif.org/ontology/Base/hasEntityExpirationReason">
        <rdfs:domain rdf:resource="https://www.gleif.org/ontology/Base/Entity"/>
        <rdfs:range rdf:resource="https://www.gleif.org/ontology/Base/EntityExpirationReason"/>
        <rdfs:isDefinedBy rdf:resource="https://www.gleif.org/ontology/Base/"/>
        <rdfs:label>has entity expiration reason</rdfs:label>
        <skos:definition>The reason that an entity ceased to exist and/or operate.</skos:definition>
    </owl:ObjectProperty>
    


    <!-- https://www.gleif.org/ontology/Base/hasEntityStatus -->


    <owl:ObjectProperty rdf:about="https://www.gleif.org/ontology/Base/hasEntityStatus">
        <rdf:type rdf:resource="http://www.w3.org/2002/07/owl#FunctionalProperty"/>
        <rdfs:domain rdf:resource="https://www.gleif.org/ontology/Base/Entity"/>
        <rdfs:range rdf:resource="https://www.gleif.org/ontology/Base/EntityStatus"/>
        <rdfs:isDefinedBy rdf:resource="https://www.gleif.org/ontology/Base/"/>
        <rdfs:label>has entity status</rdfs:label>
        <skos:definition>Indicates the status of the entity (i.e., active, inactive).</skos:definition>
    </owl:ObjectProperty>
    


    <!-- https://www.gleif.org/ontology/Base/hasGeographicRegion -->


    <owl:ObjectProperty rdf:about="https://www.gleif.org/ontology/Base/hasGeographicRegion">
        <rdfs:range rdf:resource="https://www.omg.org/spec/LCC/Countries/CountryRepresentation/GeographicRegion"/>
        <rdfs:isDefinedBy rdf:resource="https://www.gleif.org/ontology/Base/"/>
        <rdfs:label>has geographic region</rdfs:label>
        <skos:definition>The country or region where something is located.</skos:definition>
    </owl:ObjectProperty>
    


    <!-- https://www.gleif.org/ontology/Base/hasLegalJurisdiction -->


    <owl:ObjectProperty rdf:about="https://www.gleif.org/ontology/Base/hasLegalJurisdiction">
        <rdfs:domain rdf:resource="https://www.gleif.org/ontology/Base/Entity"/>
        <rdfs:range rdf:resource="https://www.omg.org/spec/LCC/Countries/CountryRepresentation/GeographicRegion"/>
        <rdfs:isDefinedBy rdf:resource="https://www.gleif.org/ontology/Base/"/>
        <rdfs:label>has legal jurisdiction</rdfs:label>
        <skos:definition>The jurisdiction of legal formation and registration of the entity (and upon which the LegalForm data element is also dependent). </skos:definition>
    </owl:ObjectProperty>
    


    <!-- https://www.gleif.org/ontology/Base/hasRegion -->


    <owl:ObjectProperty rdf:about="https://www.gleif.org/ontology/Base/hasRegion">
        <rdfs:subPropertyOf rdf:resource="https://www.gleif.org/ontology/Base/hasGeographicRegion"/>
        <rdfs:range rdf:resource="https://www.omg.org/spec/LCC/Countries/CountryRepresentation/CountrySubdivision"/>
        <rdfs:isDefinedBy rdf:resource="https://www.gleif.org/ontology/Base/"/>
        <rdfs:label>has region</rdfs:label>
        <skos:altLabel>has state</skos:altLabel>
        <skos:altLabel>has subdivision</skos:altLabel>
        <skos:definition>The (optional) region or subdivision (state, province, region, etc.) based on the 4- to 6-character ISO 3166-2 region code</skos:definition>
        <skos:prefLabel>has region</skos:prefLabel>
    </owl:ObjectProperty>
    


    <!-- https://www.gleif.org/ontology/Base/hasRegistrationStatus -->


    <owl:ObjectProperty rdf:about="https://www.gleif.org/ontology/Base/hasRegistrationStatus">
        <rdf:type rdf:resource="http://www.w3.org/2002/07/owl#FunctionalProperty"/>
        <rdfs:range rdf:resource="https://www.gleif.org/ontology/Base/RegistrationStatus"/>
        <rdfs:isDefinedBy rdf:resource="https://www.gleif.org/ontology/Base/"/>
        <rdfs:label>has registration status</rdfs:label>
        <skos:definition>indicates the status of a specific registration, such as for an identifier or license</skos:definition>
    </owl:ObjectProperty>
    


    <!-- https://www.gleif.org/ontology/Base/hasSource -->


    <owl:ObjectProperty rdf:about="https://www.gleif.org/ontology/Base/hasSource">
        <rdf:type rdf:resource="http://www.w3.org/2002/07/owl#FunctionalProperty"/>
        <rdfs:domain rdf:resource="https://www.gleif.org/ontology/Base/LegalEntityRelationship"/>
        <rdfs:range rdf:resource="https://www.gleif.org/ontology/Base/Entity"/>
        <rdfs:isDefinedBy rdf:resource="https://www.gleif.org/ontology/Base/"/>
        <rdfs:label>has source</rdfs:label>
        <skos:definition>The entity that is the source of the directed relationship.</skos:definition>
    </owl:ObjectProperty>
    


    <!-- https://www.gleif.org/ontology/Base/hasSuccessor -->


    <owl:ObjectProperty rdf:about="https://www.gleif.org/ontology/Base/hasSuccessor">
        <rdfs:domain rdf:resource="https://www.gleif.org/ontology/Base/Entity"/>
        <rdfs:range rdf:resource="https://www.gleif.org/ontology/Base/Entity"/>
        <rdfs:isDefinedBy rdf:resource="https://www.gleif.org/ontology/Base/"/>
        <rdfs:label>has successor</rdfs:label>
        <skos:definition>The surviving/new entity which continues/replaces this registration.</skos:definition>
    </owl:ObjectProperty>
    


    <!-- https://www.gleif.org/ontology/Base/hasTarget -->


    <owl:ObjectProperty rdf:about="https://www.gleif.org/ontology/Base/hasTarget">
        <rdf:type rdf:resource="http://www.w3.org/2002/07/owl#FunctionalProperty"/>
        <rdfs:domain rdf:resource="https://www.gleif.org/ontology/Base/LegalEntityRelationship"/>
        <rdfs:range rdf:resource="https://www.gleif.org/ontology/Base/Entity"/>
        <rdfs:isDefinedBy rdf:resource="https://www.gleif.org/ontology/Base/"/>
        <rdfs:label>has target</rdfs:label>
        <skos:definition>The entity that plays the target of the directed relationship.</skos:definition>
    </owl:ObjectProperty>
    


    <!-- https://www.gleif.org/ontology/Base/identifies -->


    <owl:ObjectProperty rdf:about="https://www.gleif.org/ontology/Base/identifies">
        <rdf:type rdf:resource="http://www.w3.org/2002/07/owl#FunctionalProperty"/>
        <rdfs:isDefinedBy rdf:resource="https://www.gleif.org/ontology/Base/"/>
        <rdfs:label>identifies</rdfs:label>
        <skos:definition>The relationship between an identifier and the thing it uniquely identifies.</skos:definition>
    </owl:ObjectProperty>
    


    <!-- https://www.gleif.org/ontology/Base/isManagedBy -->


    <owl:ObjectProperty rdf:about="https://www.gleif.org/ontology/Base/isManagedBy">
        <rdfs:isDefinedBy rdf:resource="https://www.gleif.org/ontology/Base/"/>
        <rdfs:label>is managed by</rdfs:label>
        <skos:definition>Relates something to another thing that has some role in directing its affairs.</skos:definition>
    </owl:ObjectProperty>
    


    <!-- https://www.gleif.org/ontology/Base/isQualifiedBy -->


    <owl:ObjectProperty rdf:about="https://www.gleif.org/ontology/Base/isQualifiedBy">
        <rdfs:domain rdf:resource="https://www.gleif.org/ontology/Base/LegalEntityRelationship"/>
        <rdfs:isDefinedBy rdf:resource="https://www.gleif.org/ontology/Base/"/>
        <rdfs:label>is qualified by</rdfs:label>
        <skos:definition>Any additional qualitative properties that help to categorize the relationship.</skos:definition>
    </owl:ObjectProperty>
    


    <!-- https://www.gleif.org/ontology/Base/isRegisteredIn -->


    <owl:ObjectProperty rdf:about="https://www.gleif.org/ontology/Base/isRegisteredIn">
        <rdfs:range rdf:resource="https://www.gleif.org/ontology/Base/Registry"/>
        <rdfs:isDefinedBy rdf:resource="https://www.gleif.org/ontology/Base/"/>
        <rdfs:label>is registered in</rdfs:label>
        <skos:definition>indicates the registry that something is registered in</skos:definition>
    </owl:ObjectProperty>
    


    <!-- https://www.gleif.org/ontology/Base/records -->


    <owl:ObjectProperty rdf:about="https://www.gleif.org/ontology/Base/records">
        <rdf:type rdf:resource="http://www.w3.org/2002/07/owl#FunctionalProperty"/>
        <rdfs:domain rdf:resource="https://www.gleif.org/ontology/Base/RegistryEntry"/>
        <rdfs:isDefinedBy rdf:resource="https://www.gleif.org/ontology/Base/"/>
        <rdfs:label>records</rdfs:label>
        <skos:definition>The thing which the registry entry is a record of.</skos:definition>
    </owl:ObjectProperty>
    


    <!-- 
    ///////////////////////////////////////////////////////////////////////////////////////
    //
    // Data properties
    //
    ///////////////////////////////////////////////////////////////////////////////////////
     -->


    


    <!-- http://purl.org/dc/terms/created -->


    <owl:DatatypeProperty rdf:about="http://purl.org/dc/terms/created"/>
    


    <!-- http://purl.org/dc/terms/modified -->


    <owl:DatatypeProperty rdf:about="http://purl.org/dc/terms/modified"/>
    


    <!-- https://www.gleif.org/ontology/Base/hasAbbreviation -->


    <owl:DatatypeProperty rdf:about="https://www.gleif.org/ontology/Base/hasAbbreviation"/>
    


    <!-- https://www.gleif.org/ontology/Base/hasAbbreviationLocal -->


    <owl:DatatypeProperty rdf:about="https://www.gleif.org/ontology/Base/hasAbbreviationLocal">
        <rdfs:subPropertyOf rdf:resource="https://www.gleif.org/ontology/Base/hasAbbreviation"/>
        <rdfs:isDefinedBy rdf:resource="https://www.gleif.org/ontology/Base/"/>
        <rdfs:label>has abbreviation local</rdfs:label>
        <skos:definition>An abbreviation using a language local to the entity identified; may be English.</skos:definition>
    </owl:DatatypeProperty>
    


    <!-- https://www.gleif.org/ontology/Base/hasAbbreviationTransliterated -->


    <owl:DatatypeProperty rdf:about="https://www.gleif.org/ontology/Base/hasAbbreviationTransliterated">
        <rdfs:subPropertyOf rdf:resource="https://www.gleif.org/ontology/Base/hasAbbreviation"/>
        <rdfs:isDefinedBy rdf:resource="https://www.gleif.org/ontology/Base/"/>
        <rdfs:label>has abbreviation transliterated</rdfs:label>
        <skos:definition>An abbreviation transliterated into a Western alphabet.</skos:definition>
    </owl:DatatypeProperty>
    


    <!-- https://www.gleif.org/ontology/Base/hasAdditionalAddressLine -->


    <owl:DatatypeProperty rdf:about="https://www.gleif.org/ontology/Base/hasAdditionalAddressLine">
        <rdfs:domain rdf:resource="https://www.gleif.org/ontology/Base/PhysicalAddress"/>
        <rdfs:isDefinedBy rdf:resource="https://www.gleif.org/ontology/Base/"/>
        <rdfs:label>has additional address line</rdfs:label>
        <skos:definition>Means to collect the one to three specifically-named optional additional address line elements.</skos:definition>
    </owl:DatatypeProperty>
    


    <!-- https://www.gleif.org/ontology/Base/hasAddressLine1 -->


    <owl:DatatypeProperty rdf:about="https://www.gleif.org/ontology/Base/hasAddressLine1">
        <owl:equivalentProperty rdf:resource="https://www.gleif.org/ontology/Base/hasFirstAddressLine"/>
        <rdfs:domain rdf:resource="https://www.gleif.org/ontology/Base/PhysicalAddress"/>
        <rdfs:isDefinedBy rdf:resource="https://www.gleif.org/ontology/Base/"/>
        <rdfs:label>has address line 1</rdfs:label>
        <skos:definition>The mandatory first address line element.</skos:definition>
    </owl:DatatypeProperty>
    


    <!-- https://www.gleif.org/ontology/Base/hasAddressLine2 -->


    <owl:DatatypeProperty rdf:about="https://www.gleif.org/ontology/Base/hasAddressLine2">
        <rdfs:subPropertyOf rdf:resource="https://www.gleif.org/ontology/Base/hasAdditionalAddressLine"/>
        <rdfs:domain rdf:resource="https://www.gleif.org/ontology/Base/PhysicalAddress"/>
        <rdfs:isDefinedBy rdf:resource="https://www.gleif.org/ontology/Base/"/>
        <rdfs:label>has address line 2</rdfs:label>
        <skos:definition>The second line of the one to three optional additional address line elements.</skos:definition>
    </owl:DatatypeProperty>
    


    <!-- https://www.gleif.org/ontology/Base/hasAddressLine3 -->


    <owl:DatatypeProperty rdf:about="https://www.gleif.org/ontology/Base/hasAddressLine3">
        <rdfs:subPropertyOf rdf:resource="https://www.gleif.org/ontology/Base/hasAdditionalAddressLine"/>
        <rdfs:domain rdf:resource="https://www.gleif.org/ontology/Base/PhysicalAddress"/>
        <rdfs:isDefinedBy rdf:resource="https://www.gleif.org/ontology/Base/"/>
        <rdfs:label>has address line 3</rdfs:label>
        <skos:definition>The third line of the one to three optional additional address line elements.</skos:definition>
        <skos:note>This element SHALL be omitted if address line 2 is omitted.</skos:note>
    </owl:DatatypeProperty>
    


    <!-- https://www.gleif.org/ontology/Base/hasAddressLine4 -->


    <owl:DatatypeProperty rdf:about="https://www.gleif.org/ontology/Base/hasAddressLine4">
        <rdfs:subPropertyOf rdf:resource="https://www.gleif.org/ontology/Base/hasAdditionalAddressLine"/>
        <rdfs:domain rdf:resource="https://www.gleif.org/ontology/Base/PhysicalAddress"/>
        <rdfs:isDefinedBy rdf:resource="https://www.gleif.org/ontology/Base/"/>
        <rdfs:label>has address line 4</rdfs:label>
        <skos:definition>The fourth line of the one to three optional additional address line elements.</skos:definition>
        <skos:note>This element SHALL be omitted if address line 3 is omitted.</skos:note>
    </owl:DatatypeProperty>
    


    <!-- https://www.gleif.org/ontology/Base/hasAddressNumber -->


    <owl:DatatypeProperty rdf:about="https://www.gleif.org/ontology/Base/hasAddressNumber">
        <rdfs:domain rdf:resource="https://www.gleif.org/ontology/Base/PhysicalAddress"/>
        <rdfs:isDefinedBy rdf:resource="https://www.gleif.org/ontology/Base/"/>
        <rdfs:label>has address number</rdfs:label>
        <skos:definition>Optional, additional structured version of an external house number, or range of numbers, contained in one of the address line elements.</skos:definition>
    </owl:DatatypeProperty>
    


    <!-- https://www.gleif.org/ontology/Base/hasAddressNumberWithinBuilding -->


    <owl:DatatypeProperty rdf:about="https://www.gleif.org/ontology/Base/hasAddressNumberWithinBuilding">
        <rdfs:domain rdf:resource="https://www.gleif.org/ontology/Base/PhysicalAddress"/>
        <rdfs:isDefinedBy rdf:resource="https://www.gleif.org/ontology/Base/"/>
        <rdfs:label>has address number within building</rdfs:label>
        <skos:definition>Optional, additional structured version of an internal location number, or range of numbers, contained in one of the address line elements.</skos:definition>
    </owl:DatatypeProperty>
    


    <!-- https://www.gleif.org/ontology/Base/hasCity -->


    <owl:DatatypeProperty rdf:about="https://www.gleif.org/ontology/Base/hasCity">
        <rdfs:domain rdf:resource="https://www.gleif.org/ontology/Base/PhysicalAddress"/>
        <rdfs:isDefinedBy rdf:resource="https://www.gleif.org/ontology/Base/"/>
        <rdfs:label>has city</rdfs:label>
        <skos:definition>The mandatory name of the city.</skos:definition>
    </owl:DatatypeProperty>
    


    <!-- https://www.gleif.org/ontology/Base/hasEnd -->


    <owl:DatatypeProperty rdf:about="https://www.gleif.org/ontology/Base/hasEnd">
        <rdfs:domain rdf:resource="https://www.gleif.org/ontology/Base/Period"/>
        <rdfs:range rdf:resource="http://www.w3.org/2001/XMLSchema#dateTime"/>
        <rdfs:isDefinedBy rdf:resource="https://www.gleif.org/ontology/Base/"/>
        <rdfs:label xml:lang="en">has end</rdfs:label>
        <skos:definition>The end time of a period.</skos:definition>
    </owl:DatatypeProperty>
    


    <!-- https://www.gleif.org/ontology/Base/hasEntityExpirationDate -->


    <owl:DatatypeProperty rdf:about="https://www.gleif.org/ontology/Base/hasEntityExpirationDate">
        <rdfs:domain rdf:resource="https://www.gleif.org/ontology/Base/Entity"/>
        <rdfs:range rdf:resource="http://www.w3.org/2001/XMLSchema#dateTime"/>
        <rdfs:isDefinedBy rdf:resource="https://www.gleif.org/ontology/Base/"/>
        <rdfs:label>has entity expiration date</rdfs:label>
        <skos:definition>The date that the entity ceased to operate, whether due to dissolution, merger or acquisition.</skos:definition>
    </owl:DatatypeProperty>
    


    <!-- https://www.gleif.org/ontology/Base/hasFirstAddressLine -->


    <owl:DatatypeProperty rdf:about="https://www.gleif.org/ontology/Base/hasFirstAddressLine">
        <rdfs:domain rdf:resource="https://www.gleif.org/ontology/Base/PhysicalAddress"/>
        <rdfs:isDefinedBy rdf:resource="https://www.gleif.org/ontology/Base/"/>
        <rdfs:label>has first address line</rdfs:label>
        <skos:definition>The mandatory first address line element.</skos:definition>
    </owl:DatatypeProperty>
    


    <!-- https://www.gleif.org/ontology/Base/hasInitialRegistrationDate -->


    <owl:DatatypeProperty rdf:about="https://www.gleif.org/ontology/Base/hasInitialRegistrationDate">
        <rdfs:subPropertyOf rdf:resource="http://purl.org/dc/terms/created"/>
        <rdfs:range rdf:resource="http://www.w3.org/2001/XMLSchema#dateTime"/>
        <rdfs:isDefinedBy rdf:resource="https://www.gleif.org/ontology/Base/"/>
        <rdfs:label>has initial registration date</rdfs:label>
        <skos:definition>The date on which an identifier or other registered item was first registered.</skos:definition>
    </owl:DatatypeProperty>
    


    <!-- https://www.gleif.org/ontology/Base/hasLastUpdateDate -->


    <owl:DatatypeProperty rdf:about="https://www.gleif.org/ontology/Base/hasLastUpdateDate">
        <rdfs:subPropertyOf rdf:resource="http://purl.org/dc/terms/modified"/>
        <rdfs:range rdf:resource="http://www.w3.org/2001/XMLSchema#dateTime"/>
        <rdfs:isDefinedBy rdf:resource="https://www.gleif.org/ontology/Base/"/>
        <rdfs:label>has last modification date</rdfs:label>
        <skos:definition>The date that the detail of a specific registration in the registry was last revised.</skos:definition>
    </owl:DatatypeProperty>
    


    <!-- https://www.gleif.org/ontology/Base/hasMailRouting -->


    <owl:DatatypeProperty rdf:about="https://www.gleif.org/ontology/Base/hasMailRouting">
        <rdfs:domain rdf:resource="https://www.gleif.org/ontology/Base/PhysicalAddress"/>
        <rdfs:isDefinedBy rdf:resource="https://www.gleif.org/ontology/Base/"/>
        <rdfs:label>mail routing</rdfs:label>
        <skos:definition>Optional free text address line to hold content from other address lines containing explicit routing information (this element&apos;s presence indicates that this address is a routing / &apos;care of&apos; address).</skos:definition>
    </owl:DatatypeProperty>
    


    <!-- https://www.gleif.org/ontology/Base/hasName -->


    <owl:DatatypeProperty rdf:about="https://www.gleif.org/ontology/Base/hasName"/>
    


    <!-- https://www.gleif.org/ontology/Base/hasNameASCII -->


    <owl:DatatypeProperty rdf:about="https://www.gleif.org/ontology/Base/hasNameASCII">
        <rdfs:subPropertyOf rdf:resource="https://www.gleif.org/ontology/Base/hasNameTransliterated"/>
        <rdfs:isDefinedBy rdf:resource="https://www.gleif.org/ontology/Base/"/>
        <rdfs:label>has name ASCII</rdfs:label>
        <skos:altLabel>has ASCII name</skos:altLabel>
        <skos:definition>The name used to refer to a person or organization in 7 bit ASCII text (ISO 646); also valid UNICODE (ISO 10646).</skos:definition>
        <skos:prefLabel>has name ASCII</skos:prefLabel>
    </owl:DatatypeProperty>
    


    <!-- https://www.gleif.org/ontology/Base/hasNameASCIIAutomatic -->


    <owl:DatatypeProperty rdf:about="https://www.gleif.org/ontology/Base/hasNameASCIIAutomatic">
        <rdfs:subPropertyOf rdf:resource="https://www.gleif.org/ontology/Base/hasNameASCII"/>
        <rdfs:subPropertyOf rdf:resource="https://www.gleif.org/ontology/Base/hasNameLegal"/>
        <rdfs:isDefinedBy rdf:resource="https://www.gleif.org/ontology/Base/"/>
        <rdfs:label>has name ASCII automatic</rdfs:label>
        <skos:altLabel>has auto ASCII transliterated legal name</skos:altLabel>
        <skos:definition>Legal name of the entity transliterated to ASCII characters, auto-transliterated by the managing LOU.</skos:definition>
        <skos:prefLabel>has name ASCII automatic</skos:prefLabel>
    </owl:DatatypeProperty>
    


    <!-- https://www.gleif.org/ontology/Base/hasNameASCIIPreferred -->


    <owl:DatatypeProperty rdf:about="https://www.gleif.org/ontology/Base/hasNameASCIIPreferred">
        <rdfs:subPropertyOf rdf:resource="https://www.gleif.org/ontology/Base/hasNameASCII"/>
        <rdfs:subPropertyOf rdf:resource="https://www.gleif.org/ontology/Base/hasNameLegal"/>
        <rdfs:isDefinedBy rdf:resource="https://www.gleif.org/ontology/Base/"/>
        <rdfs:label>has name ASCII preferred</rdfs:label>
        <skos:altLabel>has preferred transliterated legal name</skos:altLabel>
        <skos:definition>Legal name of the entity transliterated to ASCII characters, provided by the entity for this purpose.</skos:definition>
        <skos:prefLabel>has name ASCII preferred</skos:prefLabel>
    </owl:DatatypeProperty>
    


    <!-- https://www.gleif.org/ontology/Base/hasNameAdditional -->


    <owl:DatatypeProperty rdf:about="https://www.gleif.org/ontology/Base/hasNameAdditional">
        <rdfs:subPropertyOf rdf:resource="https://www.gleif.org/ontology/Base/hasName"/>
    </owl:DatatypeProperty>
    


    <!-- https://www.gleif.org/ontology/Base/hasNameAdditionalLocal -->


    <owl:DatatypeProperty rdf:about="https://www.gleif.org/ontology/Base/hasNameAdditionalLocal">
        <rdfs:subPropertyOf rdf:resource="https://www.gleif.org/ontology/Base/hasNameAdditional"/>
        <rdfs:subPropertyOf rdf:resource="https://www.gleif.org/ontology/Base/hasNameLocal"/>
        <rdfs:isDefinedBy rdf:resource="https://www.gleif.org/ontology/Base/"/>
        <rdfs:label>has name additional local</rdfs:label>
        <skos:definition>Registered name of the entity in an alternative language in the legal jurisdiction in which the entity is registered.</skos:definition>
    </owl:DatatypeProperty>
    


    <!-- https://www.gleif.org/ontology/Base/hasNameLegal -->


    <owl:DatatypeProperty rdf:about="https://www.gleif.org/ontology/Base/hasNameLegal">
        <rdfs:subPropertyOf rdf:resource="https://www.gleif.org/ontology/Base/hasName"/>
        <rdfs:isDefinedBy rdf:resource="https://www.gleif.org/ontology/Base/"/>
        <rdfs:label>has name legal</rdfs:label>
        <skos:altLabel>has legal name</skos:altLabel>
        <skos:definition>The name used to refer to an person or organization in legal communications.</skos:definition>
        <skos:prefLabel>has name legal</skos:prefLabel>
    </owl:DatatypeProperty>
    


    <!-- https://www.gleif.org/ontology/Base/hasNameLegalLocal -->


    <owl:DatatypeProperty rdf:about="https://www.gleif.org/ontology/Base/hasNameLegalLocal">
        <rdfs:subPropertyOf rdf:resource="https://www.gleif.org/ontology/Base/hasNameLegal"/>
        <rdfs:subPropertyOf rdf:resource="https://www.gleif.org/ontology/Base/hasNameLocal"/>
    </owl:DatatypeProperty>
    


    <!-- https://www.gleif.org/ontology/Base/hasNameLocal -->


    <owl:DatatypeProperty rdf:about="https://www.gleif.org/ontology/Base/hasNameLocal">
        <rdfs:subPropertyOf rdf:resource="https://www.gleif.org/ontology/Base/hasName"/>
        <rdfs:isDefinedBy rdf:resource="https://www.gleif.org/ontology/Base/"/>
        <rdfs:label>has name local</rdfs:label>
        <skos:altLabel>has local name</skos:altLabel>
        <skos:definition>A name in a language local to the entity identified; may be English.</skos:definition>
        <skos:prefLabel>has name local</skos:prefLabel>
    </owl:DatatypeProperty>
    


    <!-- https://www.gleif.org/ontology/Base/hasNamePreviousLegal -->


    <owl:DatatypeProperty rdf:about="https://www.gleif.org/ontology/Base/hasNamePreviousLegal">
        <rdfs:subPropertyOf rdf:resource="https://www.gleif.org/ontology/Base/hasNameAdditional"/>
        <rdfs:isDefinedBy rdf:resource="https://www.gleif.org/ontology/base/"/>
        <rdfs:label>has name previous legal</rdfs:label>
        <skos:definition>A primary legal name previously used by this entity.</skos:definition>
    </owl:DatatypeProperty>
    


    <!-- https://www.gleif.org/ontology/Base/hasNameTradingOrOperating -->


    <owl:DatatypeProperty rdf:about="https://www.gleif.org/ontology/Base/hasNameTradingOrOperating">
        <rdfs:subPropertyOf rdf:resource="https://www.gleif.org/ontology/Base/hasNameAdditional"/>
        <rdfs:isDefinedBy rdf:resource="https://www.gleif.org/ontology/base/"/>
        <rdfs:label>has name trading or operating</rdfs:label>
        <skos:altLabel>brand name</skos:altLabel>
        <skos:altLabel>doing business as</skos:altLabel>
        <skos:altLabel>has trading or operating name</skos:altLabel>
        <skos:altLabel>operating under</skos:altLabel>
        <skos:altLabel>trading as</skos:altLabel>
        <skos:definition>A &apos;trading as&apos;, &apos;brand name&apos; or &apos;operating under&apos; name currently used by this entity in addition to, but not replacing, the (primary) legal, official registered name</skos:definition>
        <skos:prefLabel>has name trading or operating</skos:prefLabel>
    </owl:DatatypeProperty>
    


    <!-- https://www.gleif.org/ontology/Base/hasNameTranslatedEnglish -->


    <owl:DatatypeProperty rdf:about="https://www.gleif.org/ontology/Base/hasNameTranslatedEnglish">
        <rdfs:subPropertyOf rdf:resource="https://www.gleif.org/ontology/Base/hasNameASCII"/>
        <rdfs:isDefinedBy rdf:resource="https://www.gleif.org/ontology/Base/"/>
        <rdfs:label>has name translated English</rdfs:label>
        <skos:altLabel>has English name</skos:altLabel>
        <skos:altLabel>has international name</skos:altLabel>
        <skos:definition>The name used to refer to a person or organization, translated into English. Transliterated to ASCII by definition.</skos:definition>
        <skos:prefLabel>has name translated English</skos:prefLabel>
    </owl:DatatypeProperty>
    


    <!-- https://www.gleif.org/ontology/Base/hasNameTransliterated -->


    <owl:DatatypeProperty rdf:about="https://www.gleif.org/ontology/Base/hasNameTransliterated">
        <rdfs:subPropertyOf rdf:resource="https://www.gleif.org/ontology/Base/hasName"/>
    </owl:DatatypeProperty>
    


    <!-- https://www.gleif.org/ontology/Base/hasNextRenewalDate -->


    <owl:DatatypeProperty rdf:about="https://www.gleif.org/ontology/Base/hasNextRenewalDate">
        <rdfs:range rdf:resource="http://www.w3.org/2001/XMLSchema#dateTime"/>
        <rdfs:isDefinedBy rdf:resource="https://www.gleif.org/ontology/Base/"/>
        <rdfs:label>has next renewal date</rdfs:label>
        <skos:definition>The date by which a specific registration in the registry must be renewed or updated.</skos:definition>
    </owl:DatatypeProperty>
    


    <!-- https://www.gleif.org/ontology/Base/hasPostalCode -->


    <owl:DatatypeProperty rdf:about="https://www.gleif.org/ontology/Base/hasPostalCode">
        <rdfs:domain rdf:resource="https://www.gleif.org/ontology/Base/PhysicalAddress"/>
        <rdfs:isDefinedBy rdf:resource="https://www.gleif.org/ontology/Base/"/>
        <rdfs:label>has postal code</rdfs:label>
        <skos:definition>The (optional) postal code of this address as specified by the local postal service.</skos:definition>
    </owl:DatatypeProperty>
    


    <!-- https://www.gleif.org/ontology/Base/hasStart -->


    <owl:DatatypeProperty rdf:about="https://www.gleif.org/ontology/Base/hasStart">
        <rdfs:domain rdf:resource="https://www.gleif.org/ontology/Base/Period"/>
        <rdfs:range rdf:resource="http://www.w3.org/2001/XMLSchema#dateTime"/>
        <rdfs:isDefinedBy rdf:resource="https://www.gleif.org/ontology/Base/"/>
        <rdfs:label xml:lang="en">has start</rdfs:label>
        <skos:definition>The start time of a period.</skos:definition>
    </owl:DatatypeProperty>
    


    <!-- https://www.gleif.org/ontology/Base/hasSuccessorName -->


    <owl:DatatypeProperty rdf:about="https://www.gleif.org/ontology/Base/hasSuccessorName">
        <rdfs:domain rdf:resource="https://www.gleif.org/ontology/Base/Entity"/>
        <rdfs:isDefinedBy rdf:resource="https://www.gleif.org/ontology/Base/"/>
        <rdfs:label>has successor name</rdfs:label>
        <skos:definition>The name of the successor entity.</skos:definition>
    </owl:DatatypeProperty>
    


    <!-- https://www.gleif.org/ontology/Base/hasTag -->


    <owl:DatatypeProperty rdf:about="https://www.gleif.org/ontology/Base/hasTag">
        <rdfs:subPropertyOf rdf:resource="http://www.w3.org/2004/02/skos/core#notation"/>
        <rdf:type rdf:resource="http://www.w3.org/2002/07/owl#FunctionalProperty"/>
        <rdfs:range rdf:resource="http://www.w3.org/2001/XMLSchema#string"/>
        <rdfs:isDefinedBy rdf:resource="https://www.gleif.org/ontology/Base/"/>
        <rdfs:label>has tag</rdfs:label>
        <skos:definition>Has a unique combination of alphanumeric characters or binary representation corresponding to the identifier, code, or other element to which it applies.</skos:definition>
    </owl:DatatypeProperty>
    


    <!-- https://www.gleif.org/ontology/Base/hasWebsite -->


    <owl:DatatypeProperty rdf:about="https://www.gleif.org/ontology/Base/hasWebsite">
        <rdfs:range rdf:resource="http://www.w3.org/2001/XMLSchema#anyURI"/>
        <rdfs:isDefinedBy rdf:resource="https://www.gleif.org/ontology/Base/"/>
        <rdfs:label>has website</rdfs:label>
        <skos:definition>A website associated with something, including but not limited to an organization.</skos:definition>
    </owl:DatatypeProperty>
    


    <!-- https://www.gleif.org/ontology/Base/isQuantifiedBy -->


    <owl:DatatypeProperty rdf:about="https://www.gleif.org/ontology/Base/isQuantifiedBy">
        <rdfs:domain rdf:resource="https://www.gleif.org/ontology/Base/LegalEntityRelationship"/>
        <rdfs:range rdf:resource="http://www.w3.org/2001/XMLSchema#decimal"/>
        <rdfs:isDefinedBy rdf:resource="https://www.gleif.org/ontology/Base/"/>
        <rdfs:label>is quantified by</rdfs:label>
        <skos:definition>Any additional quantitative properties that help to categorize the relationship.</skos:definition>
    </owl:DatatypeProperty>
    


    <!-- 
    ///////////////////////////////////////////////////////////////////////////////////////
    //
    // Classes
    //
    ///////////////////////////////////////////////////////////////////////////////////////
     -->


    


    <!-- http://purl.org/vocommons/voaf#Vocabulary -->


    <owl:Class rdf:about="http://purl.org/vocommons/voaf#Vocabulary"/>
    


    <!-- https://www.gleif.org/ontology/Base/Entity -->


    <owl:Class rdf:about="https://www.gleif.org/ontology/Base/Entity">
        <rdfs:subClassOf>
            <owl:Restriction>
                <owl:onProperty rdf:resource="https://www.gleif.org/ontology/Base/hasLegalJurisdiction"/>
                <owl:minQualifiedCardinality rdf:datatype="http://www.w3.org/2001/XMLSchema#nonNegativeInteger">0</owl:minQualifiedCardinality>
                <owl:onClass rdf:resource="https://www.omg.org/spec/LCC/Countries/CountryRepresentation/GeographicRegion"/>
            </owl:Restriction>
        </rdfs:subClassOf>
        <rdfs:subClassOf>
            <owl:Restriction>
                <owl:onProperty rdf:resource="https://www.gleif.org/ontology/Base/hasSuccessor"/>
                <owl:minQualifiedCardinality rdf:datatype="http://www.w3.org/2001/XMLSchema#nonNegativeInteger">0</owl:minQualifiedCardinality>
                <owl:onClass rdf:resource="https://www.gleif.org/ontology/Base/Entity"/>
            </owl:Restriction>
        </rdfs:subClassOf>
        <rdfs:subClassOf>
            <owl:Restriction>
                <owl:onProperty rdf:resource="https://www.gleif.org/ontology/Base/hasEntityStatus"/>
                <owl:qualifiedCardinality rdf:datatype="http://www.w3.org/2001/XMLSchema#nonNegativeInteger">1</owl:qualifiedCardinality>
                <owl:onClass rdf:resource="https://www.gleif.org/ontology/Base/EntityStatus"/>
            </owl:Restriction>
        </rdfs:subClassOf>
        <rdfs:subClassOf>
            <owl:Restriction>
                <owl:onProperty rdf:resource="https://www.gleif.org/ontology/Base/hasEntityExpirationReason"/>
                <owl:maxQualifiedCardinality rdf:datatype="http://www.w3.org/2001/XMLSchema#nonNegativeInteger">1</owl:maxQualifiedCardinality>
                <owl:onClass rdf:resource="https://www.gleif.org/ontology/Base/EntityExpirationReason"/>
            </owl:Restriction>
        </rdfs:subClassOf>
        <rdfs:subClassOf>
            <owl:Restriction>
                <owl:onProperty rdf:resource="https://www.gleif.org/ontology/Base/hasNameLegalLocal"/>
                <owl:cardinality rdf:datatype="http://www.w3.org/2001/XMLSchema#nonNegativeInteger">1</owl:cardinality>
            </owl:Restriction>
        </rdfs:subClassOf>
        <rdfs:subClassOf>
            <owl:Restriction>
                <owl:onProperty rdf:resource="https://www.gleif.org/ontology/Base/hasEntityExpirationDate"/>
                <owl:maxQualifiedCardinality rdf:datatype="http://www.w3.org/2001/XMLSchema#nonNegativeInteger">1</owl:maxQualifiedCardinality>
                <owl:onDataRange rdf:resource="http://www.w3.org/2001/XMLSchema#dateTime"/>
            </owl:Restriction>
        </rdfs:subClassOf>
        <rdfs:isDefinedBy rdf:resource="https://www.gleif.org/ontology/Base/"/>
        <rdfs:label>entity</rdfs:label>
        <skos:definition>A partnership, corporation, or other organization having the capacity to negotiate contracts, assume financial obligations, and pay off debts, organized under the laws of some jurisdiction.</skos:definition>
    </owl:Class>
    


    <!-- https://www.gleif.org/ontology/Base/EntityExpirationReason -->


    <owl:Class rdf:about="https://www.gleif.org/ontology/Base/EntityExpirationReason">
        <owl:equivalentClass>
            <owl:Class>
                <owl:oneOf rdf:parseType="Collection">
                    <rdf:Description rdf:about="https://www.gleif.org/ontology/Base/EntityExpirationReasonCorporateAction"/>
                    <rdf:Description rdf:about="https://www.gleif.org/ontology/Base/EntityExpirationReasonDissolved"/>
                    <rdf:Description rdf:about="https://www.gleif.org/ontology/Base/EntityExpirationReasonOther"/>
                </owl:oneOf>
            </owl:Class>
        </owl:equivalentClass>
        <rdfs:isDefinedBy rdf:resource="https://www.gleif.org/ontology/Base/"/>
        <rdfs:label>entity expiration reason</rdfs:label>
        <skos:definition>The reason that an entity ceased to exist and/or operate.</skos:definition>
    </owl:Class>
    


    <!-- https://www.gleif.org/ontology/Base/EntityStatus -->


    <owl:Class rdf:about="https://www.gleif.org/ontology/Base/EntityStatus">
        <owl:equivalentClass>
            <owl:Class>
                <owl:oneOf rdf:parseType="Collection">
                    <rdf:Description rdf:about="https://www.gleif.org/ontology/Base/EntityStatusActive"/>
                    <rdf:Description rdf:about="https://www.gleif.org/ontology/Base/EntityStatusInactive"/>
                </owl:oneOf>
            </owl:Class>
        </owl:equivalentClass>
        <rdfs:isDefinedBy rdf:resource="https://www.gleif.org/ontology/Base/"/>
        <rdfs:label>entity status</rdfs:label>
        <skos:definition>The operational and/or legal registration status of the entity (may be ACTIVE or INACTIVE)</skos:definition>
    </owl:Class>
    


    <!-- https://www.gleif.org/ontology/Base/Identifier -->


    <owl:Class rdf:about="https://www.gleif.org/ontology/Base/Identifier">
        <rdfs:subClassOf>
            <owl:Restriction>
                <owl:onProperty rdf:resource="https://www.gleif.org/ontology/Base/identifies"/>
                <owl:cardinality rdf:datatype="http://www.w3.org/2001/XMLSchema#nonNegativeInteger">1</owl:cardinality>
            </owl:Restriction>
        </rdfs:subClassOf>
        <rdfs:subClassOf>
            <owl:Restriction>
                <owl:onProperty rdf:resource="https://www.gleif.org/ontology/Base/hasTag"/>
                <owl:qualifiedCardinality rdf:datatype="http://www.w3.org/2001/XMLSchema#nonNegativeInteger">1</owl:qualifiedCardinality>
                <owl:onDataRange rdf:resource="http://www.w3.org/2001/XMLSchema#string"/>
            </owl:Restriction>
        </rdfs:subClassOf>
        <rdfs:isDefinedBy rdf:resource="https://www.gleif.org/ontology/Base/"/>
        <rdfs:label>identifier</rdfs:label>
        <skos:definition>Sequence of characters, capable of uniquely identifying that with which it is associated, within a specified context.</skos:definition>
    </owl:Class>
    


    <!-- https://www.gleif.org/ontology/Base/LegalEntityRelationship -->


    <owl:Class rdf:about="https://www.gleif.org/ontology/Base/LegalEntityRelationship">
        <rdfs:subClassOf>
            <owl:Restriction>
                <owl:onProperty rdf:resource="https://www.gleif.org/ontology/Base/hasSource"/>
                <owl:qualifiedCardinality rdf:datatype="http://www.w3.org/2001/XMLSchema#nonNegativeInteger">1</owl:qualifiedCardinality>
                <owl:onClass rdf:resource="https://www.gleif.org/ontology/Base/Entity"/>
            </owl:Restriction>
        </rdfs:subClassOf>
        <rdfs:subClassOf>
            <owl:Restriction>
                <owl:onProperty rdf:resource="https://www.gleif.org/ontology/Base/hasTarget"/>
                <owl:qualifiedCardinality rdf:datatype="http://www.w3.org/2001/XMLSchema#nonNegativeInteger">1</owl:qualifiedCardinality>
                <owl:onClass rdf:resource="https://www.gleif.org/ontology/Base/Entity"/>
            </owl:Restriction>
        </rdfs:subClassOf>
        <rdfs:isDefinedBy rdf:resource="https://www.gleif.org/ontology/Base/"/>
        <rdfs:label>legal entity relationship</rdfs:label>
        <skos:definition>abstract superclass to represent a reified directed relationship</skos:definition>
    </owl:Class>
    


    <!-- https://www.gleif.org/ontology/Base/LegalPerson -->


    <owl:Class rdf:about="https://www.gleif.org/ontology/Base/LegalPerson">
        <rdfs:subClassOf rdf:resource="https://www.gleif.org/ontology/Base/Entity"/>
        <rdfs:isDefinedBy rdf:resource="https://www.gleif.org/ontology/Base/"/>
        <rdfs:label>legal person</rdfs:label>
        <skos:definition>Any entity which can incur legal obligation and can be sued at law.</skos:definition>
    </owl:Class>
    


    <!-- https://www.gleif.org/ontology/Base/Period -->


    <owl:Class rdf:about="https://www.gleif.org/ontology/Base/Period">
        <rdfs:subClassOf>
            <owl:Restriction>
                <owl:onProperty rdf:resource="https://www.gleif.org/ontology/Base/hasStart"/>
                <owl:qualifiedCardinality rdf:datatype="http://www.w3.org/2001/XMLSchema#nonNegativeInteger">1</owl:qualifiedCardinality>
                <owl:onDataRange rdf:resource="http://www.w3.org/2001/XMLSchema#dateTime"/>
            </owl:Restriction>
        </rdfs:subClassOf>
        <rdfs:subClassOf>
            <owl:Restriction>
                <owl:onProperty rdf:resource="https://www.gleif.org/ontology/Base/hasEnd"/>
                <owl:maxQualifiedCardinality rdf:datatype="http://www.w3.org/2001/XMLSchema#nonNegativeInteger">1</owl:maxQualifiedCardinality>
                <owl:onDataRange rdf:resource="http://www.w3.org/2001/XMLSchema#dateTime"/>
            </owl:Restriction>
        </rdfs:subClassOf>
        <rdfs:isDefinedBy rdf:resource="https://www.gleif.org/ontology/Base/"/>
        <rdfs:label xml:lang="en">period</rdfs:label>
        <skos:definition>A period of time, with at least a start time, and possibly an end.</skos:definition>
    </owl:Class>
    


    <!-- https://www.gleif.org/ontology/Base/PhysicalAddress -->


    <owl:Class rdf:about="https://www.gleif.org/ontology/Base/PhysicalAddress">
        <rdfs:subClassOf>
            <owl:Restriction>
                <owl:onProperty rdf:resource="https://www.gleif.org/ontology/Base/hasCountry"/>
                <owl:qualifiedCardinality rdf:datatype="http://www.w3.org/2001/XMLSchema#nonNegativeInteger">1</owl:qualifiedCardinality>
                <owl:onClass rdf:resource="https://www.omg.org/spec/LCC/Countries/CountryRepresentation/Country"/>
            </owl:Restriction>
        </rdfs:subClassOf>
        <rdfs:subClassOf>
            <owl:Restriction>
                <owl:onProperty rdf:resource="https://www.gleif.org/ontology/Base/hasRegion"/>
                <owl:maxQualifiedCardinality rdf:datatype="http://www.w3.org/2001/XMLSchema#nonNegativeInteger">1</owl:maxQualifiedCardinality>
                <owl:onClass rdf:resource="https://www.omg.org/spec/LCC/Countries/CountryRepresentation/Region"/>
            </owl:Restriction>
        </rdfs:subClassOf>
        <rdfs:subClassOf>
            <owl:Restriction>
                <owl:onProperty rdf:resource="https://www.gleif.org/ontology/Base/hasAddressLine1"/>
                <owl:cardinality rdf:datatype="http://www.w3.org/2001/XMLSchema#nonNegativeInteger">1</owl:cardinality>
            </owl:Restriction>
        </rdfs:subClassOf>
        <rdfs:subClassOf>
            <owl:Restriction>
                <owl:onProperty rdf:resource="https://www.gleif.org/ontology/Base/hasCity"/>
                <owl:cardinality rdf:datatype="http://www.w3.org/2001/XMLSchema#nonNegativeInteger">1</owl:cardinality>
            </owl:Restriction>
        </rdfs:subClassOf>
        <rdfs:subClassOf>
            <owl:Restriction>
                <owl:onProperty rdf:resource="https://www.gleif.org/ontology/Base/hasAddressLine2"/>
                <owl:maxCardinality rdf:datatype="http://www.w3.org/2001/XMLSchema#nonNegativeInteger">1</owl:maxCardinality>
            </owl:Restriction>
        </rdfs:subClassOf>
        <rdfs:subClassOf>
            <owl:Restriction>
                <owl:onProperty rdf:resource="https://www.gleif.org/ontology/Base/hasAddressLine3"/>
                <owl:maxCardinality rdf:datatype="http://www.w3.org/2001/XMLSchema#nonNegativeInteger">1</owl:maxCardinality>
            </owl:Restriction>
        </rdfs:subClassOf>
        <rdfs:subClassOf>
            <owl:Restriction>
                <owl:onProperty rdf:resource="https://www.gleif.org/ontology/Base/hasAddressLine4"/>
                <owl:maxCardinality rdf:datatype="http://www.w3.org/2001/XMLSchema#nonNegativeInteger">1</owl:maxCardinality>
            </owl:Restriction>
        </rdfs:subClassOf>
        <rdfs:subClassOf>
            <owl:Restriction>
                <owl:onProperty rdf:resource="https://www.gleif.org/ontology/Base/hasAddressNumber"/>
                <owl:maxCardinality rdf:datatype="http://www.w3.org/2001/XMLSchema#nonNegativeInteger">1</owl:maxCardinality>
            </owl:Restriction>
        </rdfs:subClassOf>
        <rdfs:subClassOf>
            <owl:Restriction>
                <owl:onProperty rdf:resource="https://www.gleif.org/ontology/Base/hasAddressNumberWithinBuilding"/>
                <owl:maxCardinality rdf:datatype="http://www.w3.org/2001/XMLSchema#nonNegativeInteger">1</owl:maxCardinality>
            </owl:Restriction>
        </rdfs:subClassOf>
        <rdfs:subClassOf>
            <owl:Restriction>
                <owl:onProperty rdf:resource="https://www.gleif.org/ontology/Base/hasMailRouting"/>
                <owl:maxCardinality rdf:datatype="http://www.w3.org/2001/XMLSchema#nonNegativeInteger">1</owl:maxCardinality>
            </owl:Restriction>
        </rdfs:subClassOf>
        <rdfs:subClassOf>
            <owl:Restriction>
                <owl:onProperty rdf:resource="https://www.gleif.org/ontology/Base/hasPostalCode"/>
                <owl:maxCardinality rdf:datatype="http://www.w3.org/2001/XMLSchema#nonNegativeInteger">1</owl:maxCardinality>
            </owl:Restriction>
        </rdfs:subClassOf>
        <rdfs:isDefinedBy rdf:resource="https://www.gleif.org/ontology/Base/"/>
        <rdfs:label xml:lang="en">physical address</rdfs:label>
        <skos:definition>a physical address where communications can be addressed, papers served or representatives located for any kind of organization or person</skos:definition>
        <skos:note>An address is a collection of information, presented in a mostly fixed format, used for describing the location of a building, apartment, or other structure or a plot of land, generally using political boundaries and street names as references, along with other identifiers such as house or apartment numbers.  Some addresses also contain special codes to aid routing of mail and packages, such as a ZIP code or post code. (Wikipedia)</skos:note>
    </owl:Class>
    


    <!-- https://www.gleif.org/ontology/Base/PhysicalAddressASCII -->


    <owl:Class rdf:about="https://www.gleif.org/ontology/Base/PhysicalAddressASCII">
        <rdfs:subClassOf rdf:resource="https://www.gleif.org/ontology/Base/PhysicalAddress"/>
        <rdfs:isDefinedBy rdf:resource="https://www.gleif.org/ontology/Base/"/>
        <rdfs:label>physical address ASCII</rdfs:label>
        <skos:definition>An address transliterated to ASCII characters.</skos:definition>
    </owl:Class>
    


    <!-- https://www.gleif.org/ontology/Base/RegistrationAuthority -->


    <owl:Class rdf:about="https://www.gleif.org/ontology/Base/RegistrationAuthority">
        <rdfs:subClassOf rdf:resource="https://www.gleif.org/ontology/Base/Entity"/>
        <rdfs:isDefinedBy rdf:resource="https://www.gleif.org/ontology/Base/"/>
        <rdfs:label>registration authority</rdfs:label>
        <skos:altLabel>RA</skos:altLabel>
        <skos:definition>An organization that is responsible for maintaining a registry and provides registration services.</skos:definition>
        <skos:prefLabel>registration authority</skos:prefLabel>
    </owl:Class>
    


    <!-- https://www.gleif.org/ontology/Base/RegistrationStatus -->


    <owl:Class rdf:about="https://www.gleif.org/ontology/Base/RegistrationStatus">
        <rdfs:isDefinedBy rdf:resource="https://www.gleif.org/ontology/Base/"/>
        <rdfs:label>registration status</rdfs:label>
        <skos:definition>A lifecycle stage indicating the status of a given registration of something, such as a business or legal entity.</skos:definition>
    </owl:Class>
    


    <!-- https://www.gleif.org/ontology/Base/Registry -->


    <owl:Class rdf:about="https://www.gleif.org/ontology/Base/Registry">
        <rdfs:subClassOf>
            <owl:Restriction>
                <owl:onProperty rdf:resource="https://www.gleif.org/ontology/Base/isManagedBy"/>
                <owl:qualifiedCardinality rdf:datatype="http://www.w3.org/2001/XMLSchema#nonNegativeInteger">1</owl:qualifiedCardinality>
                <owl:onClass rdf:resource="https://www.gleif.org/ontology/Base/Entity"/>
            </owl:Restriction>
        </rdfs:subClassOf>
        <rdfs:isDefinedBy rdf:resource="https://www.gleif.org/ontology/Base/"/>
        <rdfs:label>registry</rdfs:label>
        <skos:definition>A system, typically an information system, that records the registration of items.</skos:definition>
    </owl:Class>
    


    <!-- https://www.gleif.org/ontology/Base/RegistryEntry -->


    <owl:Class rdf:about="https://www.gleif.org/ontology/Base/RegistryEntry">
        <rdfs:isDefinedBy rdf:resource="https://www.gleif.org/ontology/Base/"/>
        <rdfs:label>registry entry</rdfs:label>
        <skos:definition>An entry in a registry that specifies something about the thing that is recorded.</skos:definition>
    </owl:Class>
    


    <!-- https://www.gleif.org/ontology/Base/RegistryIdentifier -->


    <owl:Class rdf:about="https://www.gleif.org/ontology/Base/RegistryIdentifier">
        <rdfs:subClassOf rdf:resource="https://www.gleif.org/ontology/Base/Identifier"/>
        <rdfs:subClassOf>
            <owl:Restriction>
                <owl:onProperty rdf:resource="https://www.gleif.org/ontology/Base/isRegisteredIn"/>
                <owl:someValuesFrom rdf:resource="https://www.gleif.org/ontology/Base/Registry"/>
            </owl:Restriction>
        </rdfs:subClassOf>
        <rdfs:isDefinedBy rdf:resource="https://www.gleif.org/ontology/Base/"/>
        <rdfs:label>registry identifier</rdfs:label>
        <skos:definition>An identifier associated with an entry in a registry, i.e., one that provides an index to the registry for the recorded item.</skos:definition>
    </owl:Class>
    


    <!-- https://www.omg.org/spec/LCC/Countries/CountryRepresentation/Region -->


    <owl:Class rdf:about="https://www.omg.org/spec/LCC/Countries/CountryRepresentation/Region"/>
    


    <!-- 
    ///////////////////////////////////////////////////////////////////////////////////////
    //
    // Individuals
    //
    ///////////////////////////////////////////////////////////////////////////////////////
     -->


    


    <!-- https://www.gleif.org/ontology/Base/ -->


    <owl:NamedIndividual rdf:about="https://www.gleif.org/ontology/Base/">
        <rdf:type rdf:resource="http://purl.org/vocommons/voaf#Vocabulary"/>
    </owl:NamedIndividual>
    


    <!-- https://www.gleif.org/ontology/Base/EntityExpirationReasonCorporateAction -->


    <owl:NamedIndividual rdf:about="https://www.gleif.org/ontology/Base/EntityExpirationReasonCorporateAction">
        <rdf:type rdf:resource="https://www.gleif.org/ontology/Base/EntityExpirationReason"/>
        <hasTag>CORPORATE_ACTION</hasTag>
        <rdfs:isDefinedBy rdf:resource="https://www.gleif.org/ontology/Base/"/>
        <rdfs:label>corporate action</rdfs:label>
        <skos:definition>The entity was acquired or merged with another entity.</skos:definition>
    </owl:NamedIndividual>
    


    <!-- https://www.gleif.org/ontology/Base/EntityExpirationReasonDissolved -->


    <owl:NamedIndividual rdf:about="https://www.gleif.org/ontology/Base/EntityExpirationReasonDissolved">
        <rdf:type rdf:resource="https://www.gleif.org/ontology/Base/EntityExpirationReason"/>
        <hasTag>DISSOLVED</hasTag>
        <rdfs:isDefinedBy rdf:resource="https://www.gleif.org/ontology/Base/"/>
        <rdfs:label>dissolved</rdfs:label>
        <skos:definition>The entity ceased to operate.</skos:definition>
    </owl:NamedIndividual>
    


    <!-- https://www.gleif.org/ontology/Base/EntityExpirationReasonOther -->


    <owl:NamedIndividual rdf:about="https://www.gleif.org/ontology/Base/EntityExpirationReasonOther">
        <rdf:type rdf:resource="https://www.gleif.org/ontology/Base/EntityExpirationReason"/>
        <hasTag>OTHER</hasTag>
        <rdfs:isDefinedBy rdf:resource="https://www.gleif.org/ontology/Base/"/>
        <rdfs:label>other</rdfs:label>
        <skos:definition>The reason for expiry is neither of dissolved nor corporate action.</skos:definition>
    </owl:NamedIndividual>
    


    <!-- https://www.gleif.org/ontology/Base/EntityStatusActive -->


    <owl:NamedIndividual rdf:about="https://www.gleif.org/ontology/Base/EntityStatusActive">
        <rdf:type rdf:resource="https://www.gleif.org/ontology/Base/EntityStatus"/>
        <hasTag>ACTIVE</hasTag>
        <rdfs:isDefinedBy rdf:resource="https://www.gleif.org/ontology/Base/"/>
        <rdfs:label>active</rdfs:label>
        <skos:definition>As of the last report or update, the entity reported that it was legally registered and operating.</skos:definition>
    </owl:NamedIndividual>
    


    <!-- https://www.gleif.org/ontology/Base/EntityStatusInactive -->


    <owl:NamedIndividual rdf:about="https://www.gleif.org/ontology/Base/EntityStatusInactive">
        <rdf:type rdf:resource="https://www.gleif.org/ontology/Base/EntityStatus"/>
        <hasTag>INACTIVE</hasTag>
        <rdfs:isDefinedBy rdf:resource="https://www.gleif.org/ontology/Base/"/>
        <rdfs:label>inactive</rdfs:label>
        <skos:definition>It has been determined that the entity that was assigned the LEI is no longer legally registered and/or operating, whether as a result of business closure, acquisition by or merger with another (or new) entity, or determination of illegitimacy.</skos:definition>
    </owl:NamedIndividual>
    


    <!-- https://www.gleif.org/ontology/Base/GLEIF -->


    <owl:NamedIndividual rdf:about="https://www.gleif.org/ontology/Base/GLEIF">
        <rdf:type rdf:resource="https://www.gleif.org/ontology/Base/RegistrationAuthority"/>
        <hasNameLegalLocal xml:lang="en">Global Legal Entity Identifier Foundation</hasNameLegalLocal>
        <rdfs:isDefinedBy rdf:resource="https://www.gleif.org/ontology/Base/"/>
        <hasLegalName>Global Legal Entity Identifier Foundation</hasLegalName>
    </owl:NamedIndividual>
    


    <!-- 
    ///////////////////////////////////////////////////////////////////////////////////////
    //
    // Annotations
    //
    ///////////////////////////////////////////////////////////////////////////////////////
     -->


    <rdf:Description rdf:about="https://www.gleif.org/ontology/Base/hasAbbreviation">
        <rdfs:isDefinedBy rdf:resource="https://www.gleif.org/ontology/Base/"/>
        <rdfs:label>has abbreviation</rdfs:label>
        <skos:definition>An abbreviation for the entity identified.</skos:definition>
    </rdf:Description>
    <rdf:Description rdf:about="https://www.gleif.org/ontology/Base/hasName">
        <rdfs:isDefinedBy rdf:resource="https://www.gleif.org/ontology/Base/"/>
        <rdfs:label>has name</rdfs:label>
        <skos:definition>Associates a name, reference name, or appellation with an individual resource.</skos:definition>
    </rdf:Description>
    <rdf:Description rdf:about="https://www.gleif.org/ontology/Base/hasNameAdditional">
        <rdfs:isDefinedBy rdf:resource="https://www.gleif.org/ontology/Base/"/>
        <rdfs:label>has name additional</rdfs:label>
        <skos:altLabel>has other name</skos:altLabel>
        <skos:definition>The name used to refer to an person or organization informally.</skos:definition>
        <skos:prefLabel>has name additional</skos:prefLabel>
    </rdf:Description>
    <rdf:Description rdf:about="https://www.gleif.org/ontology/Base/hasNameLegalLocal">
        <rdfs:isDefinedBy rdf:resource="https://www.gleif.org/ontology/Base/"/>
        <rdfs:label>has name legal local</rdfs:label>
        <skos:altLabel>has local legal name</skos:altLabel>
        <skos:definition>The name used to refer to an person or organization in legal communications in local alphabet, which may be English.</skos:definition>
        <skos:prefLabel>has name legal local</skos:prefLabel>
    </rdf:Description>
    <rdf:Description rdf:about="https://www.gleif.org/ontology/Base/hasNameTransliterated">
        <rdfs:isDefinedBy rdf:resource="https://www.gleif.org/ontology/Base/"/>
        <rdfs:label>has name transliterated</rdfs:label>
        <skos:altLabel>has transliterated name</skos:altLabel>
        <skos:altLabel>has transliterated other names</skos:altLabel>
        <skos:definition>The name used to refer to a person or organization, converted from original to western text. Not generally the legal name.</skos:definition>
        <skos:prefLabel>has name transliterated</skos:prefLabel>
    </rdf:Description>
    


    <!-- 
    ///////////////////////////////////////////////////////////////////////////////////////
    //
    // General axioms
    //
    ///////////////////////////////////////////////////////////////////////////////////////
     -->


    <rdf:Description>
        <rdf:type rdf:resource="http://www.w3.org/2002/07/owl#AllDifferent"/>
        <owl:distinctMembers rdf:parseType="Collection">
            <rdf:Description rdf:about="https://www.gleif.org/ontology/Base/EntityExpirationReasonCorporateAction"/>
            <rdf:Description rdf:about="https://www.gleif.org/ontology/Base/EntityExpirationReasonDissolved"/>
            <rdf:Description rdf:about="https://www.gleif.org/ontology/Base/EntityExpirationReasonOther"/>
        </owl:distinctMembers>
    </rdf:Description>
    <rdf:Description>
        <rdf:type rdf:resource="http://www.w3.org/2002/07/owl#AllDifferent"/>
        <owl:distinctMembers rdf:parseType="Collection">
            <rdf:Description rdf:about="https://www.gleif.org/ontology/Base/EntityStatusActive"/>
            <rdf:Description rdf:about="https://www.gleif.org/ontology/Base/EntityStatusInactive"/>
        </owl:distinctMembers>
    </rdf:Description>
</rdf:RDF>



<!-- Generated by the OWL API (version 5.1.9) https://github.com/owlcs/owlapi/ -->


