<?xml version="1.0"?>
<rdf:RDF xmlns="http://data.ign.fr/def/ignf#"
     xml:base="http://data.ign.fr/def/ignf"
     xmlns:ns="http://creativecommons.org/ns#"
     xmlns:org="http://www.w3.org/ns/org#"
     xmlns:owl="http://www.w3.org/2002/07/owl#"
     xmlns:rdf="http://www.w3.org/1999/02/22-rdf-syntax-ns#"
     xmlns:xml="http://www.w3.org/XML/1998/namespace"
     xmlns:xsd="http://www.w3.org/2001/XMLSchema#"
     xmlns:foaf="http://xmlns.com/foaf/0.1/"
     xmlns:rdfs="http://www.w3.org/2000/01/rdf-schema#"
     xmlns:time="http://www.w3.org/2006/time#"
     xmlns:vann="http://purl.org/vocab/vann/"
     xmlns:terms="http://purl.org/dc/terms/">
    <owl:Ontology rdf:about="http://data.ign.fr/def/ignf">
        <ns:license rdf:resource="http://creativecommons.org/licenses/by/2.0/"/>
        <ns:license rdf:resource="http://opendatacommons.org/licenses/by/"/>
        <ns:license rdf:resource="http://www.data.gouv.fr/Licence-Ouverte-Open-Licence"/>
        <terms:contributor rdf:resource="http://www.eurecom.fr/~troncy/"/>
        <terms:creator rdf:resource="_:genid-nodeid-node1d3jrsfu2x156"/>
        <terms:creator rdf:resource="http://www.eurecom.fr/~atemezin/"/>
        <terms:description xml:lang="en">Codes for describing coordinates reference systems consistently with ISO TC/211. French translations of terms and definitions are mainly taken from the multilingual glossary of ISO/TC 211 available online: http://www.isotc211.org/Terminology.htm</terms:description>
        <terms:description xml:lang="fr">Codes pour la description de systèmes de coordonnées de référence conforme ISO TC/211. Les traductions françaises des termes et leurs définitions sont pour la plupart issues du glossaire multilingue ISO/TC 211 disponible ici: http://www.isotc211.org/Terminology.htm</terms:description>
        <terms:issued rdf:datatype="http://www.w3.org/2001/XMLSchema#date">2013-06-11</terms:issued>
        <terms:modified rdf:datatype="http://www.w3.org/2001/XMLSchema#date">2014-04-09</terms:modified>
        <terms:modified rdf:datatype="http://www.w3.org/2001/XMLSchema#date">2015-05-05</terms:modified>
        <terms:modified rdf:datatype="http://www.w3.org/2001/XMLSchema#date">2016-06-28</terms:modified>
        <terms:modified rdf:datatype="http://www.w3.org/2001/XMLSchema#date">2019-02-13</terms:modified>
        <terms:publisher rdf:resource="http://fr.dbpedia.org/resource/Institut_national_de_l%27information_g%C3%A9ographique_et_foresti%C3%A8re"/>
        <terms:rights>Copyright 2019, IGN</terms:rights>
        <terms:title xml:lang="fr">Ontologie des systèmes de coordonnées de référence</terms:title>
        <terms:title xml:lang="en">Ontology of coordinates reference systems</terms:title>
        <vann:preferredNamespacePrefix>ignf</vann:preferredNamespacePrefix>
        <vann:preferredNamespaceUri rdf:resource="http://data.ign.fr/def/ignf#"/>
        <rdfs:seeAlso rdf:resource="http://librairies.ignf.fr/geoportail/resources/IGNF.xml"/>
        <owl:priorVersion rdf:resource="http://data.ign.fr/def/ignf/20160628.ttl"/>
        <owl:versionInfo>Version 3.1 - 2019-02-13</owl:versionInfo>
    </owl:Ontology>
    


    <!-- 
    ///////////////////////////////////////////////////////////////////////////////////////
    //
    // Annotation properties
    //
    ///////////////////////////////////////////////////////////////////////////////////////
     -->


    


    <!-- http://creativecommons.org/ns#license -->


    <owl:AnnotationProperty rdf:about="http://creativecommons.org/ns#license"/>
    


    <!-- http://purl.org/dc/terms/contributor -->


    <owl:AnnotationProperty rdf:about="http://purl.org/dc/terms/contributor"/>
    


    <!-- http://purl.org/dc/terms/creator -->


    <owl:AnnotationProperty rdf:about="http://purl.org/dc/terms/creator"/>
    


    <!-- http://purl.org/dc/terms/description -->


    <owl:AnnotationProperty rdf:about="http://purl.org/dc/terms/description"/>
    


    <!-- http://purl.org/dc/terms/issued -->


    <owl:AnnotationProperty rdf:about="http://purl.org/dc/terms/issued"/>
    


    <!-- http://purl.org/dc/terms/modified -->


    <owl:AnnotationProperty rdf:about="http://purl.org/dc/terms/modified"/>
    


    <!-- http://purl.org/dc/terms/publisher -->


    <owl:AnnotationProperty rdf:about="http://purl.org/dc/terms/publisher"/>
    


    <!-- http://purl.org/dc/terms/rights -->


    <owl:AnnotationProperty rdf:about="http://purl.org/dc/terms/rights"/>
    


    <!-- http://purl.org/dc/terms/title -->


    <owl:AnnotationProperty rdf:about="http://purl.org/dc/terms/title"/>
    


    <!-- http://purl.org/vocab/vann/preferredNamespacePrefix -->


    <owl:AnnotationProperty rdf:about="http://purl.org/vocab/vann/preferredNamespacePrefix"/>
    


    <!-- http://purl.org/vocab/vann/preferredNamespaceUri -->


    <owl:AnnotationProperty rdf:about="http://purl.org/vocab/vann/preferredNamespaceUri"/>
    


    <!-- http://www.w3.org/2006/time#hasBeginning -->


    <owl:AnnotationProperty rdf:about="http://www.w3.org/2006/time#hasBeginning"/>
    


    <!-- http://www.w3.org/2006/time#inXSDDateTimeStamp -->


    <owl:AnnotationProperty rdf:about="http://www.w3.org/2006/time#inXSDDateTimeStamp"/>
    


    <!-- http://www.w3.org/ns/org#hasMembership -->


    <owl:AnnotationProperty rdf:about="http://www.w3.org/ns/org#hasMembership"/>
    


    <!-- http://www.w3.org/ns/org#memberDuring -->


    <owl:AnnotationProperty rdf:about="http://www.w3.org/ns/org#memberDuring"/>
    


    <!-- http://www.w3.org/ns/org#organization -->


    <owl:AnnotationProperty rdf:about="http://www.w3.org/ns/org#organization"/>
    


    <!-- http://www.w3.org/ns/org#role -->


    <owl:AnnotationProperty rdf:about="http://www.w3.org/ns/org#role"/>
    


    <!-- http://xmlns.com/foaf/0.1/family_name -->


    <owl:AnnotationProperty rdf:about="http://xmlns.com/foaf/0.1/family_name"/>
    


    <!-- http://xmlns.com/foaf/0.1/firstName -->


    <owl:AnnotationProperty rdf:about="http://xmlns.com/foaf/0.1/firstName"/>
    


    <!-- http://xmlns.com/foaf/0.1/mbox -->


    <owl:AnnotationProperty rdf:about="http://xmlns.com/foaf/0.1/mbox"/>
    


    <!-- http://xmlns.com/foaf/0.1/name -->


    <owl:AnnotationProperty rdf:about="http://xmlns.com/foaf/0.1/name"/>
    


    <!-- http://xmlns.com/foaf/0.1/workInfoHomepage -->


    <owl:AnnotationProperty rdf:about="http://xmlns.com/foaf/0.1/workInfoHomepage"/>
    


    <!-- 
    ///////////////////////////////////////////////////////////////////////////////////////
    //
    // Object Properties
    //
    ///////////////////////////////////////////////////////////////////////////////////////
     -->


    


    <!-- http://data.ign.fr/def/ignf#axis -->


    <owl:ObjectProperty rdf:about="http://data.ign.fr/def/ignf#axis">
        <rdfs:domain rdf:resource="http://data.ign.fr/def/ignf#CoordinateSystem"/>
        <rdfs:range rdf:resource="http://data.ign.fr/def/ignf#AxesList"/>
        <rdfs:comment xml:lang="en">An axis used by some ellipsoidal or cartesian coordinate system. Cf. ISO 19111:2007:2007-07, table 17, association role axis.</rdfs:comment>
        <rdfs:comment xml:lang="fr">Désigne un axe utilisé par un système de coordonnées ellipsoïdal ou cartésien. Cf. ISO 19111:2007:2007-07, tableau 17, rôle d&apos;association axis.</rdfs:comment>
        <rdfs:isDefinedBy rdf:resource="http://data.ign.fr/def/ignf"/>
        <rdfs:label xml:lang="en">uses axis</rdfs:label>
        <rdfs:label xml:lang="fr">utilise l&apos;axe</rdfs:label>
    </owl:ObjectProperty>
    


    <!-- http://data.ign.fr/def/ignf#baseCRS -->


    <owl:ObjectProperty rdf:about="http://data.ign.fr/def/ignf#baseCRS">
        <rdfs:domain rdf:resource="http://data.ign.fr/def/ignf#ProjectedCRS"/>
        <rdfs:range rdf:resource="http://data.ign.fr/def/ignf#GeodeticCRS"/>
        <rdfs:comment xml:lang="fr">Désigne le système de coordonnées de référence géodésique sur lequel repose un système de coordonnées de référence projeté. Cf. ISO 19111:2007:2007-07, tableau 11, rôle d&apos;association baseCRS.</rdfs:comment>
        <rdfs:comment xml:lang="en">The geodetic coordinate reference system on which a projected coordinate reference system is based. Cf. ISO 19111:2007:2007-07, table 11, association role baseCRS.</rdfs:comment>
        <rdfs:isDefinedBy rdf:resource="http://data.ign.fr/def/ignf"/>
        <rdfs:label xml:lang="en">base coordinate reference system</rdfs:label>
        <rdfs:label xml:lang="fr">système de coordonnées de référence de base</rdfs:label>
    </owl:ObjectProperty>
    


    <!-- http://data.ign.fr/def/ignf#cartesianCS -->


    <owl:ObjectProperty rdf:about="http://data.ign.fr/def/ignf#cartesianCS">
        <rdfs:subPropertyOf rdf:resource="http://data.ign.fr/def/ignf#coordinateSystem"/>
        <rdfs:domain>
            <owl:Class>
                <owl:unionOf rdf:parseType="Collection">
                    <rdf:Description rdf:about="http://data.ign.fr/def/ignf#GeodeticCRS"/>
                    <rdf:Description rdf:about="http://data.ign.fr/def/ignf#ProjectedCRS"/>
                </owl:unionOf>
            </owl:Class>
        </rdfs:domain>
        <rdfs:range rdf:resource="http://data.ign.fr/def/ignf#CartesianCS"/>
        <rdfs:comment xml:lang="fr">Désigne le système de coordonnées cartésien utilisé par un système de coordonnées de référence géodésique ou projeté. Cf. ISO 19111:2007:2007-07, tableaux 10 et 11, association nommée CoordinateSystem.</rdfs:comment>
        <rdfs:comment xml:lang="en">The cartesian coordinate system used by some geodetic or projected coordinate reference system. Cf. ISO 19111:2007:2007-07, tables 10 et 11, association roles coordinateSystem.</rdfs:comment>
        <rdfs:isDefinedBy rdf:resource="http://data.ign.fr/def/ignf"/>
        <rdfs:label xml:lang="en">uses cartesian coordinate system</rdfs:label>
        <rdfs:label xml:lang="fr">utilise le système de coordonnées cartesien</rdfs:label>
    </owl:ObjectProperty>
    


    <!-- http://data.ign.fr/def/ignf#conversion -->


    <owl:ObjectProperty rdf:about="http://data.ign.fr/def/ignf#conversion">
        <rdfs:domain rdf:resource="http://data.ign.fr/def/ignf#ProjectedCRS"/>
        <rdfs:range rdf:resource="http://data.ign.fr/def/ignf#Conversion"/>
        <rdfs:comment xml:lang="fr">Désigne la conversion utilisée pour définir un système de coordonnées de référence projeté. Cf. ISO 19111:2007:2007-07, tableau 7, association nommée Definition.</rdfs:comment>
        <rdfs:comment xml:lang="en">The conversion used to define a projected coordinate reference system. Cf. ISO 19111:2007:2007-07, table 7, named association Definition.</rdfs:comment>
        <rdfs:isDefinedBy rdf:resource="http://data.ign.fr/def/ignf"/>
        <rdfs:label xml:lang="en">defined by conversion</rdfs:label>
        <rdfs:label xml:lang="fr">défini par conversion</rdfs:label>
    </owl:ObjectProperty>
    


    <!-- http://data.ign.fr/def/ignf#coordinateSystem -->


    <owl:ObjectProperty rdf:about="http://data.ign.fr/def/ignf#coordinateSystem">
        <rdfs:domain rdf:resource="http://data.ign.fr/def/ignf#SingleCRS"/>
        <rdfs:range rdf:resource="http://data.ign.fr/def/ignf#CoordinateSystem"/>
        <rdfs:comment xml:lang="fr">Désigne le système de coordonnées utilisé par un système de coordonnées de référence. Cf. ISO 19111:2007:2007-07, tableau 5, association nommée CoordinateSystem.</rdfs:comment>
        <rdfs:comment xml:lang="en">The coordinate system used by a coordinate reference system. Cf. ISO 19111:2007:2007-07, table 5, named association CoordinateSystem.</rdfs:comment>
        <rdfs:isDefinedBy rdf:resource="http://data.ign.fr/def/ignf"/>
        <rdfs:label xml:lang="en">uses coordinate system</rdfs:label>
        <rdfs:label xml:lang="fr">utilise le système de coordonnées</rdfs:label>
    </owl:ObjectProperty>
    


    <!-- http://data.ign.fr/def/ignf#datum -->


    <owl:ObjectProperty rdf:about="http://data.ign.fr/def/ignf#datum">
        <rdfs:domain rdf:resource="http://data.ign.fr/def/ignf#SingleCRS"/>
        <rdfs:range rdf:resource="http://data.ign.fr/def/ignf#Datum"/>
        <rdfs:comment xml:lang="fr">Désigne le référentiel utilisé par un système de coordonnées de référence simple. Cf. ISO 19111:2007:2007-07, tableau 5, association nommée DefiningDatum.</rdfs:comment>
        <rdfs:comment xml:lang="en">The datum used by a single coordinate reference system. Cf. ISO 19111:2007:2007-07, table 5, named association DefiningDatum.</rdfs:comment>
        <rdfs:isDefinedBy rdf:resource="http://data.ign.fr/def/ignf"/>
        <rdfs:label xml:lang="en">uses datum</rdfs:label>
        <rdfs:label xml:lang="fr">utilise le référentiel</rdfs:label>
    </owl:ObjectProperty>
    


    <!-- http://data.ign.fr/def/ignf#domainOfValidity -->


    <owl:ObjectProperty rdf:about="http://data.ign.fr/def/ignf#domainOfValidity">
        <rdfs:range rdf:resource="http://data.ign.fr/def/ignf#Extent"/>
        <rdfs:comment xml:lang="en">Geographic area or time interval in which the referring object is valid. Cf. ISO 19111:2007:2007-07, tables 4, 33 and 42, attribute domainOfValidity.</rdfs:comment>
        <rdfs:comment xml:lang="fr">Zone ou intervalle de temps dans lequel l&apos;objet de référence est valide. Cf. ISO 19111:2007:2007-07, tableaux 4, 33 et 42, attribut domainOfValidity.</rdfs:comment>
        <rdfs:isDefinedBy rdf:resource="http://data.ign.fr/def/ignf"/>
        <rdfs:label xml:lang="en">domain of validity</rdfs:label>
        <rdfs:label xml:lang="fr">domaine de validité</rdfs:label>
    </owl:ObjectProperty>
    


    <!-- http://data.ign.fr/def/ignf#ellipsoid -->


    <owl:ObjectProperty rdf:about="http://data.ign.fr/def/ignf#ellipsoid">
        <rdfs:domain rdf:resource="http://data.ign.fr/def/ignf#GeodeticDatum"/>
        <rdfs:range rdf:resource="http://data.ign.fr/def/ignf#Ellipsoid"/>
        <rdfs:comment xml:lang="fr">Désigne l&apos;ellipsoïde utilisé par un référentiel géodésique. Cf. ISO 19111:2007:2007-07, tableau 34, rôle d&apos;association ellipsoid.</rdfs:comment>
        <rdfs:comment xml:lang="en">The ellipsoid used by a geodetic datum. Cf. ISO 19111:2007:2007-07, table 34, association role ellipsoid.</rdfs:comment>
        <rdfs:isDefinedBy rdf:resource="http://data.ign.fr/def/ignf"/>
        <rdfs:label xml:lang="en">uses ellipsoid</rdfs:label>
        <rdfs:label xml:lang="fr">utilise l&apos;ellipsoïde</rdfs:label>
    </owl:ObjectProperty>
    


    <!-- http://data.ign.fr/def/ignf#ellipsoidalCS -->


    <owl:ObjectProperty rdf:about="http://data.ign.fr/def/ignf#ellipsoidalCS">
        <rdfs:subPropertyOf rdf:resource="http://data.ign.fr/def/ignf#coordinateSystem"/>
        <rdfs:domain rdf:resource="http://data.ign.fr/def/ignf#GeodeticCRS"/>
        <rdfs:range rdf:resource="http://data.ign.fr/def/ignf#EllipsoidalCS"/>
        <rdfs:comment xml:lang="fr">Désigne le système de coordonnées ellipsoïdal utilisé par un système de coordonnées de référence géodésique. Cf. ISO 19111:2007:2007-07, tableau 10, association nommée CoordinateSystem.</rdfs:comment>
        <rdfs:comment xml:lang="en">The ellipsoidal coordinate system used by a geodetic coordinate reference system. Cf. ISO 19111:2007:2007-07, table 10, named association CoordinateSystem.</rdfs:comment>
        <rdfs:isDefinedBy rdf:resource="http://data.ign.fr/def/ignf"/>
        <rdfs:label xml:lang="en">uses ellipsoidal coordinate system</rdfs:label>
        <rdfs:label xml:lang="fr">utilise le système de coordonnées ellipsoïdal</rdfs:label>
    </owl:ObjectProperty>
    


    <!-- http://data.ign.fr/def/ignf#geodeticDatum -->


    <owl:ObjectProperty rdf:about="http://data.ign.fr/def/ignf#geodeticDatum">
        <rdfs:subPropertyOf rdf:resource="http://data.ign.fr/def/ignf#datum"/>
        <rdfs:domain rdf:resource="http://data.ign.fr/def/ignf#GeodeticCRS"/>
        <rdfs:range rdf:resource="http://data.ign.fr/def/ignf#GeodeticDatum"/>
        <rdfs:comment xml:lang="fr">Désigne le référentiel géodésique utilisé par un système de coordonnées de référence géodésique. Cf. ISO 19111:2007:2007-07, tableau 10, association nommée DefiningDatum.</rdfs:comment>
        <rdfs:comment xml:lang="en">The geodetic datum used by a geodetic coordinate reference system. Cf. ISO 19111:2007:2007-07, table 10, named association DefiningDatum.</rdfs:comment>
        <rdfs:isDefinedBy rdf:resource="http://data.ign.fr/def/ignf"/>
        <rdfs:label xml:lang="en">uses geodetic datum</rdfs:label>
        <rdfs:label xml:lang="fr">utilise le référentiel géodésique</rdfs:label>
    </owl:ObjectProperty>
    


    <!-- http://data.ign.fr/def/ignf#geographicElement -->


    <owl:ObjectProperty rdf:about="http://data.ign.fr/def/ignf#geographicElement">
        <rdfs:domain rdf:resource="http://data.ign.fr/def/ignf#Extent"/>
        <rdfs:range rdf:resource="http://data.ign.fr/def/ignf#GeographicBoundingBox"/>
        <rdfs:comment xml:lang="fr">Désigne le cadre englobant géographique d&apos;une région de validité. Cf. ISO 19115-1:2014:2014-04, partie 6.6.1 et tableau B.15 ligne 337.</rdfs:comment>
        <rdfs:comment xml:lang="en">The geographic bounding box used for defining a domain of validity. Cf. ISO 19115-1:2014:2014-04, part 6.6.1 and table B.15 line 337.</rdfs:comment>
        <rdfs:isDefinedBy rdf:resource="http://data.ign.fr/def/ignf"/>
        <rdfs:label xml:lang="en">geographic element</rdfs:label>
        <rdfs:label xml:lang="fr">élément géographique</rdfs:label>
    </owl:ObjectProperty>
    


    <!-- http://data.ign.fr/def/ignf#greenwichLongitude -->


    <owl:ObjectProperty rdf:about="http://data.ign.fr/def/ignf#greenwichLongitude">
        <rdfs:domain rdf:resource="http://data.ign.fr/def/ignf#PrimeMeridian"/>
        <rdfs:range>
            <owl:Class>
                <owl:intersectionOf rdf:parseType="Collection">
                    <rdf:Description rdf:about="http://qudt.org/1.1/schema/qudt#QuantityValue"/>
                    <owl:Restriction>
                        <owl:onProperty rdf:resource="http://qudt.org/1.1/schema/qudt#unit"/>
                        <owl:allValuesFrom rdf:resource="http://qudt.org/1.1/schema/qudt#AngleUnit"/>
                    </owl:Restriction>
                </owl:intersectionOf>
            </owl:Class>
        </rdfs:range>
        <rdfs:comment xml:lang="fr">Désigne la longitude par rapport au méridien de Greenwich. Cf. ISO 19111:2007:2007-07, tableau 35, attribut longitude du méridien d&apos;origine.</rdfs:comment>
        <rdfs:comment xml:lang="en">Indicates the longitude from Greenwich meridian. Cf. ISO 19111:2007:2007-07, table 35, attribute prime meridian Greenwich longitude.</rdfs:comment>
        <rdfs:isDefinedBy rdf:resource="http://data.ign.fr/def/ignf"/>
        <rdfs:label xml:lang="en">greenwich longitude</rdfs:label>
        <rdfs:label xml:lang="fr">longitude par rapport à Greenwich</rdfs:label>
    </owl:ObjectProperty>
    


    <!-- http://data.ign.fr/def/ignf#includesSingleCRS -->


    <owl:ObjectProperty rdf:about="http://data.ign.fr/def/ignf#includesSingleCRS">
        <rdfs:domain rdf:resource="http://data.ign.fr/def/ignf#CompoundCRS"/>
        <rdfs:range rdf:resource="http://data.ign.fr/def/ignf#SingleCRSList"/>
        <rdfs:comment xml:lang="fr">Désigne les systèmes de coordonnées de référence simples qui composent un système de coordonnées de référence composé. Cf. ISO 19111:2007:2007-07, tableau 6, rôle d&apos;association componentReferenceSystem.</rdfs:comment>
        <rdfs:comment xml:lang="en">Indicates the single coordinate reference systems used by a compound coordinate reference system. Cf. ISO 19111:2007:2007-07, table 6, association role componentReferenceSystem.</rdfs:comment>
        <rdfs:isDefinedBy rdf:resource="http://data.ign.fr/def/ignf"/>
        <rdfs:label xml:lang="en">includes some single coordinate reference systems</rdfs:label>
        <rdfs:label xml:lang="fr">inclut des systèmes de coordonnées de référence simples</rdfs:label>
    </owl:ObjectProperty>
    


    <!-- http://data.ign.fr/def/ignf#inverseFlattening -->


    <owl:ObjectProperty rdf:about="http://data.ign.fr/def/ignf#inverseFlattening">
        <rdfs:domain rdf:resource="http://data.ign.fr/def/ignf#Ellipsoid"/>
        <rdfs:range>
            <owl:Class>
                <owl:intersectionOf rdf:parseType="Collection">
                    <rdf:Description rdf:about="http://qudt.org/1.1/schema/qudt#QuantityValue"/>
                    <owl:Restriction>
                        <owl:onProperty rdf:resource="http://qudt.org/1.1/schema/qudt#unit"/>
                        <owl:allValuesFrom rdf:resource="http://qudt.org/1.1/schema/qudt#CountingUnit"/>
                    </owl:Restriction>
                </owl:intersectionOf>
            </owl:Class>
        </rdfs:range>
        <rdfs:comment xml:lang="fr">Désigne la valeur d&apos;aplatissement inverse d&apos;un ellipsoïde, exprimée sous la forme d&apos;un nombre ou d&apos;un ratio (pourcentage, parties par million, etc.). Cf. ISO 19111:2007:2007-07, tableau 37, attribut aplatissement inverse.</rdfs:comment>
        <rdfs:comment xml:lang="en">Indicates the inverse flattening value of an ellipsoid, expressed as a number or a ratio (percentage rate, parts per million, etc.). Cf. ISO 19111:2007:2007-07, table 37, attribute inverse flattening</rdfs:comment>
        <rdfs:isDefinedBy rdf:resource="http://data.ign.fr/def/ignf"/>
        <rdfs:label xml:lang="fr">aplatissement inverse</rdfs:label>
        <rdfs:label xml:lang="en">inverse flattening</rdfs:label>
    </owl:ObjectProperty>
    


    <!-- http://data.ign.fr/def/ignf#parameter -->


    <owl:ObjectProperty rdf:about="http://data.ign.fr/def/ignf#parameter">
        <rdfs:domain rdf:resource="http://data.ign.fr/def/ignf#OperationParameterValue"/>
        <rdfs:range rdf:resource="http://data.ign.fr/def/ignf#OperationParameter"/>
        <rdfs:comment xml:lang="fr">Désigne le paramètre auquel est associée une valeur. Cf. ISO 19111:2007:2007-07, tableau 55, rôle d&apos;association parameter.</rdfs:comment>
        <rdfs:comment xml:lang="en">The parameter associated to a given value. Cf. ISO 19111:2007:2007-07, table 55, association role parameter.</rdfs:comment>
        <rdfs:isDefinedBy rdf:resource="http://data.ign.fr/def/ignf"/>
        <rdfs:label xml:lang="en">parameter</rdfs:label>
        <rdfs:label xml:lang="fr">paramètre</rdfs:label>
    </owl:ObjectProperty>
    


    <!-- http://data.ign.fr/def/ignf#primeMeridian -->


    <owl:ObjectProperty rdf:about="http://data.ign.fr/def/ignf#primeMeridian">
        <rdfs:domain rdf:resource="http://data.ign.fr/def/ignf#GeodeticDatum"/>
        <rdfs:range rdf:resource="http://data.ign.fr/def/ignf#PrimeMeridian"/>
        <rdfs:comment xml:lang="fr">Désigne le méridien origine d&apos;un référentiel géodésique. Cf. ISO 19111:2007:2007-07, tableau 34, rôle d&apos;association primeMeridian.</rdfs:comment>
        <rdfs:comment xml:lang="en">The prime meridian used by a geodetic datum. Cf. ISO 19111:2007:2007-07, table 34, association role primeMeridian.</rdfs:comment>
        <rdfs:isDefinedBy rdf:resource="http://data.ign.fr/def/ignf"/>
        <rdfs:label xml:lang="en">uses prime meridian</rdfs:label>
        <rdfs:label xml:lang="fr">utilise le méridien origine</rdfs:label>
    </owl:ObjectProperty>
    


    <!-- http://data.ign.fr/def/ignf#semiMajorAxis -->


    <owl:ObjectProperty rdf:about="http://data.ign.fr/def/ignf#semiMajorAxis">
        <rdfs:domain rdf:resource="http://data.ign.fr/def/ignf#Ellipsoid"/>
        <rdfs:range>
            <owl:Class>
                <owl:intersectionOf rdf:parseType="Collection">
                    <rdf:Description rdf:about="http://qudt.org/1.1/schema/qudt#QuantityValue"/>
                    <owl:Restriction>
                        <owl:onProperty rdf:resource="http://qudt.org/1.1/schema/qudt#unit"/>
                        <owl:allValuesFrom rdf:resource="http://qudt.org/1.1/schema/qudt#LengthUnit"/>
                    </owl:Restriction>
                </owl:intersectionOf>
            </owl:Class>
        </rdfs:range>
        <rdfs:comment xml:lang="fr">Désigne la longueur du demi grand axe d&apos;un ellipsoïde. Cf. ISO 19111:2007:2007-07, tableau 36, attribut longueur du demi-grand axe.</rdfs:comment>
        <rdfs:comment xml:lang="en">Indicates the length of the semi major axis of an ellipsoid. Cf. ISO 19111:2007:2007-07, table 36, attribute length of semi-major axis.</rdfs:comment>
        <rdfs:isDefinedBy rdf:resource="http://data.ign.fr/def/ignf"/>
        <rdfs:label xml:lang="fr">demi grand axe</rdfs:label>
        <rdfs:label xml:lang="en">semi major axis</rdfs:label>
    </owl:ObjectProperty>
    


    <!-- http://data.ign.fr/def/ignf#semiMinorAxis -->


    <owl:ObjectProperty rdf:about="http://data.ign.fr/def/ignf#semiMinorAxis">
        <rdfs:domain rdf:resource="http://data.ign.fr/def/ignf#Ellipsoid"/>
        <rdfs:range>
            <owl:Class>
                <owl:intersectionOf rdf:parseType="Collection">
                    <rdf:Description rdf:about="http://qudt.org/1.1/schema/qudt#QuantityValue"/>
                    <owl:Restriction>
                        <owl:onProperty rdf:resource="http://qudt.org/1.1/schema/qudt#unit"/>
                        <owl:allValuesFrom rdf:resource="http://qudt.org/1.1/schema/qudt#LengthUnit"/>
                    </owl:Restriction>
                </owl:intersectionOf>
            </owl:Class>
        </rdfs:range>
        <rdfs:comment xml:lang="fr">Désigne la longueur du demi petit axe d&apos;un ellipsoïde. Cf. ISO 19111:2007:2007-07, tableau 37, attribut longueur du demi-petit axe.</rdfs:comment>
        <rdfs:comment xml:lang="en">Indicates the length of the semi minor axis of an ellipsoid. Cf. ISO 19111:2007:2007-07, table 37, attribute length of semi-minor axis.</rdfs:comment>
        <rdfs:isDefinedBy rdf:resource="http://data.ign.fr/def/ignf"/>
        <rdfs:label xml:lang="fr">demi petit axe</rdfs:label>
        <rdfs:label xml:lang="en">semi minor axis</rdfs:label>
    </owl:ObjectProperty>
    


    <!-- http://data.ign.fr/def/ignf#sourceCRS -->


    <owl:ObjectProperty rdf:about="http://data.ign.fr/def/ignf#sourceCRS">
        <rdfs:domain rdf:resource="http://data.ign.fr/def/ignf#CoordinateOperation"/>
        <rdfs:range rdf:resource="http://data.ign.fr/def/ignf#CRS"/>
        <rdfs:comment xml:lang="fr">Désigne le système de coordonnées de référence des données en entrée d&apos;une opération. Cf. ISO 19111:2007:2007-07, tableau 42, association nommée Source.</rdfs:comment>
        <rdfs:comment xml:lang="en">The coordinate reference system associated to the data used as input of a given operation. Cf. ISO 19111:2007:2007-07, table 42, named association Source.</rdfs:comment>
        <rdfs:isDefinedBy rdf:resource="http://data.ign.fr/def/ignf"/>
        <rdfs:label xml:lang="en">source coordinate reference system</rdfs:label>
        <rdfs:label xml:lang="fr">système de coordonnées de référence source</rdfs:label>
    </owl:ObjectProperty>
    


    <!-- http://data.ign.fr/def/ignf#targetCRS -->


    <owl:ObjectProperty rdf:about="http://data.ign.fr/def/ignf#targetCRS">
        <rdfs:domain rdf:resource="http://data.ign.fr/def/ignf#CoordinateOperation"/>
        <rdfs:range rdf:resource="http://data.ign.fr/def/ignf#CRS"/>
        <rdfs:comment xml:lang="fr">Désigne le système de coordonnées de référence des données en sortie d&apos;une opération. Cf. ISO 19111:2007:2007-07, tableau 42, association nommée Target.</rdfs:comment>
        <rdfs:comment xml:lang="en">The coordinate reference system associated to the data obtained as output of a given operation. Cf. ISO 19111:2007:2007-07, table 42, named association Target.</rdfs:comment>
        <rdfs:isDefinedBy rdf:resource="http://data.ign.fr/def/ignf"/>
        <rdfs:label xml:lang="fr">système de coordonnées de référence cible</rdfs:label>
        <rdfs:label xml:lang="en">target coordinate reference system</rdfs:label>
    </owl:ObjectProperty>
    


    <!-- http://data.ign.fr/def/ignf#usesMethod -->


    <owl:ObjectProperty rdf:about="http://data.ign.fr/def/ignf#usesMethod">
        <rdfs:domain rdf:resource="http://data.ign.fr/def/ignf#CoordinateOperation"/>
        <rdfs:range rdf:resource="http://data.ign.fr/def/ignf#OperationMethod"/>
        <rdfs:comment xml:lang="fr">Désigne la méthode utilisée par une opération sur des coordonnées. Cf. ISO 19111:2007:2007-07, tableau 43, rôle d&apos;association method.</rdfs:comment>
        <rdfs:comment xml:lang="en">The method used by an operation on coordinates. Cf. ISO 19111:2007:2007-07, table 43, association role method.</rdfs:comment>
        <rdfs:isDefinedBy rdf:resource="http://data.ign.fr/def/ignf"/>
        <rdfs:label xml:lang="en">uses method</rdfs:label>
        <rdfs:label xml:lang="fr">utilise la méthode</rdfs:label>
    </owl:ObjectProperty>
    


    <!-- http://data.ign.fr/def/ignf#usesParameter -->


    <owl:ObjectProperty rdf:about="http://data.ign.fr/def/ignf#usesParameter">
        <rdfs:domain rdf:resource="http://data.ign.fr/def/ignf#OperationMethod"/>
        <rdfs:range rdf:resource="http://data.ign.fr/def/ignf#OperationParameter"/>
        <rdfs:comment xml:lang="en">A parameter used by a method to perform an operation on coordinates. Cf. ISO 19111:2007:2007-07, table 48, association role parameter.</rdfs:comment>
        <rdfs:comment xml:lang="fr">Désigne un paramètre utilisé par une méthode pour faire une opération sur des coordonnées. Cf. ISO 19111:2007:2007-07, tableau 48, rôle d&apos;association parameter.</rdfs:comment>
        <rdfs:isDefinedBy rdf:resource="http://data.ign.fr/def/ignf"/>
        <rdfs:label xml:lang="en">uses parameter</rdfs:label>
        <rdfs:label xml:lang="fr">utilise le paramètre</rdfs:label>
    </owl:ObjectProperty>
    


    <!-- http://data.ign.fr/def/ignf#usesValue -->


    <owl:ObjectProperty rdf:about="http://data.ign.fr/def/ignf#usesValue">
        <rdfs:domain rdf:resource="http://data.ign.fr/def/ignf#CoordinateOperation"/>
        <rdfs:range rdf:resource="http://data.ign.fr/def/ignf#OperationParameterValue"/>
        <rdfs:comment xml:lang="en">A value used by an operation on coordinates. Cf. ISO 19111:2007:2007-07, table 43, association role parameterValue.</rdfs:comment>
        <rdfs:comment xml:lang="fr">Désigne une valeur utilisée par une opération sur des coordonnées. Cf. ISO 19111:2007:2007-07, tableau 43, rôle d&apos;association parameterValue.</rdfs:comment>
        <rdfs:isDefinedBy rdf:resource="http://data.ign.fr/def/ignf"/>
        <rdfs:label xml:lang="en">uses value</rdfs:label>
        <rdfs:label xml:lang="fr">utilise la valeur</rdfs:label>
    </owl:ObjectProperty>
    


    <!-- http://data.ign.fr/def/ignf#verticalCS -->


    <owl:ObjectProperty rdf:about="http://data.ign.fr/def/ignf#verticalCS">
        <rdfs:subPropertyOf rdf:resource="http://data.ign.fr/def/ignf#coordinateSystem"/>
        <rdfs:domain rdf:resource="http://data.ign.fr/def/ignf#VerticalCRS"/>
        <rdfs:range rdf:resource="http://data.ign.fr/def/ignf#VerticalCS"/>
        <rdfs:comment xml:lang="fr">Désigne le système de coordonnées vertical utilisé par un système de coordonnées de référence vertical. Cf. ISO 19111:2007:2007-07, tableau 14, association nommée CoordinateSystem.</rdfs:comment>
        <rdfs:comment xml:lang="en">The vertical coordinate system used by a vertical coordinate reference system. Cf. ISO 19111:2007:2007-07, table 14, named association CoordinateSystem.</rdfs:comment>
        <rdfs:isDefinedBy rdf:resource="http://data.ign.fr/def/ignf"/>
        <rdfs:label xml:lang="en">uses vertical coordinate system</rdfs:label>
        <rdfs:label xml:lang="fr">utilise le système vertical de coordonnées</rdfs:label>
    </owl:ObjectProperty>
    


    <!-- http://data.ign.fr/def/ignf#verticalDatum -->


    <owl:ObjectProperty rdf:about="http://data.ign.fr/def/ignf#verticalDatum">
        <rdfs:subPropertyOf rdf:resource="http://data.ign.fr/def/ignf#datum"/>
        <rdfs:domain rdf:resource="http://data.ign.fr/def/ignf#VerticalCRS"/>
        <rdfs:range rdf:resource="http://data.ign.fr/def/ignf#VerticalDatum"/>
        <rdfs:comment xml:lang="fr">Désigne le référentiel vertical utilisé par un système de coordonnées de référence vertical. Cf. ISO 19111:2007:2007-07, tableau 14, association nommée DefiningDatum.</rdfs:comment>
        <rdfs:comment xml:lang="en">The vertical datum used by a vertical coordinate reference system. Cf. ISO 19111:2007:2007-07, table 14, named association DefiningDatum.</rdfs:comment>
        <rdfs:isDefinedBy rdf:resource="http://data.ign.fr/def/ignf"/>
        <rdfs:label xml:lang="en">uses vertical datum</rdfs:label>
        <rdfs:label xml:lang="fr">utilise le référentiel vertical</rdfs:label>
    </owl:ObjectProperty>
    


    <!-- http://qudt.org/1.1/schema/qudt#unit -->


    <owl:ObjectProperty rdf:about="http://qudt.org/1.1/schema/qudt#unit"/>
    


    <!-- http://www.w3.org/1999/02/22-rdf-syntax-ns#first -->


    <owl:ObjectProperty rdf:about="http://www.w3.org/1999/02/22-rdf-syntax-ns#first"/>
    


    <!-- http://www.w3.org/1999/02/22-rdf-syntax-ns#rest -->


    <owl:ObjectProperty rdf:about="http://www.w3.org/1999/02/22-rdf-syntax-ns#rest"/>
    


    <!-- 
    ///////////////////////////////////////////////////////////////////////////////////////
    //
    // Data properties
    //
    ///////////////////////////////////////////////////////////////////////////////////////
     -->


    


    <!-- http://data.ign.fr/def/ignf#axisAbbrev -->


    <owl:DatatypeProperty rdf:about="http://data.ign.fr/def/ignf#axisAbbrev">
        <rdfs:domain rdf:resource="http://data.ign.fr/def/ignf#CoordinateSystemAxis"/>
        <rdfs:range rdf:resource="http://www.w3.org/2001/XMLSchema#string"/>
        <rdfs:comment xml:lang="fr">Désigne l&apos;abréviation utilisée pour désigner l&apos;axe. Cf. ISO 19111:2007:2007-07, tableau 27, attribut abréviation de l&apos;axe du système de coordonnées.</rdfs:comment>
        <rdfs:comment xml:lang="en">The abbreviation used to identify an axis. Cf. ISO 19111:2007:2007-07, table 27, attribute coordinate system axis abbreviation.</rdfs:comment>
        <rdfs:isDefinedBy rdf:resource="http://data.ign.fr/def/ignf"/>
        <rdfs:label xml:lang="fr">abréviation utilisée pour désigner l&apos;axe</rdfs:label>
        <rdfs:label xml:lang="en">axis abbreviation</rdfs:label>
    </owl:DatatypeProperty>
    


    <!-- http://data.ign.fr/def/ignf#axisDirection -->


    <owl:DatatypeProperty rdf:about="http://data.ign.fr/def/ignf#axisDirection">
        <rdfs:domain rdf:resource="http://data.ign.fr/def/ignf#CoordinateSystemAxis"/>
        <rdfs:range rdf:resource="http://www.w3.org/2001/XMLSchema#string"/>
        <rdfs:comment xml:lang="fr">Désigne la direction de l&apos;axe. Cf. ISO 19111:2007:2007-07, tableau 27, attribut direction de l&apos;axe du système de coordonnées.</rdfs:comment>
        <rdfs:comment xml:lang="en">The direction of an axis. Cf. ISO 19111:2007:2007-07, table 27, attribute coordinate system axis direction.</rdfs:comment>
        <rdfs:isDefinedBy rdf:resource="http://data.ign.fr/def/ignf"/>
        <rdfs:label xml:lang="en">axis direction</rdfs:label>
        <rdfs:label xml:lang="fr">direction de l&apos;axe</rdfs:label>
    </owl:DatatypeProperty>
    


    <!-- http://data.ign.fr/def/ignf#codeSpace -->


    <owl:DatatypeProperty rdf:about="http://data.ign.fr/def/ignf#codeSpace">
        <rdfs:range rdf:resource="http://www.w3.org/2001/XMLSchema#string"/>
        <rdfs:comment xml:lang="fr">Désigne la règle ou l&apos;autorité dont résulte la valeur de la référence.</rdfs:comment>
        <rdfs:comment xml:lang="en">Rule or authority for a code, name, term or category.</rdfs:comment>
        <rdfs:isDefinedBy rdf:resource="http://data.ign.fr/def/ignf"/>
        <rdfs:label xml:lang="en">code space</rdfs:label>
        <rdfs:label xml:lang="fr">espace de codage</rdfs:label>
    </owl:DatatypeProperty>
    


    <!-- http://data.ign.fr/def/ignf#eastBoundLongitude -->


    <owl:DatatypeProperty rdf:about="http://data.ign.fr/def/ignf#eastBoundLongitude">
        <rdfs:domain rdf:resource="http://data.ign.fr/def/ignf#GeographicBoundingBox"/>
        <rdfs:range rdf:resource="http://www.w3.org/2001/XMLSchema#double"/>
        <rdfs:comment xml:lang="fr">Désigne la longitude est maximale du cadre englobant. Cf. ISO 19115-1:2014:2014-04, partie 6.6.1 et tableau B.15.1 ligne 346.</rdfs:comment>
        <rdfs:comment xml:lang="en">Indicates the east bound longitude of a bounding box. Cf. ISO 19115-1:2014:2014-04, part 6.6.1 and table B.15.1 line 346.</rdfs:comment>
        <rdfs:isDefinedBy rdf:resource="http://data.ign.fr/def/ignf"/>
        <rdfs:label xml:lang="en">east bound longitude</rdfs:label>
        <rdfs:label xml:lang="fr">longitude est maximale</rdfs:label>
    </owl:DatatypeProperty>
    


    <!-- http://data.ign.fr/def/ignf#epsgID -->


    <owl:DatatypeProperty rdf:about="http://data.ign.fr/def/ignf#epsgID">
        <rdfs:range rdf:resource="http://www.w3.org/2001/XMLSchema#string"/>
        <rdfs:comment xml:lang="fr">Indique l&apos;identifiant EPSG de la ressource.</rdfs:comment>
        <rdfs:comment xml:lang="en">The EPSG identifier of the resource.</rdfs:comment>
        <rdfs:isDefinedBy rdf:resource="http://data.ign.fr/def/ignf"/>
        <rdfs:label xml:lang="en">espg identifier</rdfs:label>
        <rdfs:label xml:lang="fr">identifiant epsg</rdfs:label>
    </owl:DatatypeProperty>
    


    <!-- http://data.ign.fr/def/ignf#isSphere -->


    <owl:DatatypeProperty rdf:about="http://data.ign.fr/def/ignf#isSphere">
        <rdfs:domain rdf:resource="http://data.ign.fr/def/ignf#Ellipsoid"/>
        <rdfs:range rdf:resource="http://www.w3.org/2001/XMLSchema#boolean"/>
        <rdfs:comment xml:lang="en">Indicates whether the ellipsoid is a sphere. Cf. ISO 19111:2007:2007-07, table 37, attribute ellipsoid=sphere indicator.</rdfs:comment>
        <rdfs:comment xml:lang="fr">Indique si l&apos;ellipsoïde est une sphère. Cf. ISO 19111:2007:2007-07, tableau 37, attribut indicateur ellipsoïde=sphère.</rdfs:comment>
        <rdfs:isDefinedBy rdf:resource="http://data.ign.fr/def/ignf"/>
        <rdfs:label xml:lang="fr">est une sphère</rdfs:label>
        <rdfs:label xml:lang="en">is sphere</rdfs:label>
    </owl:DatatypeProperty>
    


    <!-- http://data.ign.fr/def/ignf#methodFormula -->


    <owl:DatatypeProperty rdf:about="http://data.ign.fr/def/ignf#methodFormula">
        <rdfs:domain rdf:resource="http://data.ign.fr/def/ignf#OperationMethod"/>
        <rdfs:range rdf:resource="http://www.w3.org/2001/XMLSchema#string"/>
        <rdfs:comment xml:lang="fr">Indique la formule utilisée par une méthode pour faire opération sur des coordonnées. Cf. ISO 19111:2007:2007-07, tableau 48, attribut référence de formule de la méthode d&apos;opération sur les coordonnées.</rdfs:comment>
        <rdfs:comment xml:lang="en">The formula used by a method to perform an operation on coordinates. Cf. ISO 19111:2007:2007-07, table 48, attribute coordinate operation method formula reference.</rdfs:comment>
        <rdfs:isDefinedBy rdf:resource="http://data.ign.fr/def/ignf"/>
        <rdfs:label xml:lang="fr">formule de la méthode</rdfs:label>
        <rdfs:label xml:lang="en">method formula</rdfs:label>
    </owl:DatatypeProperty>
    


    <!-- http://data.ign.fr/def/ignf#northBoundLatitude -->


    <owl:DatatypeProperty rdf:about="http://data.ign.fr/def/ignf#northBoundLatitude">
        <rdfs:domain rdf:resource="http://data.ign.fr/def/ignf#GeographicBoundingBox"/>
        <rdfs:range rdf:resource="http://www.w3.org/2001/XMLSchema#double"/>
        <rdfs:comment xml:lang="fr">Désigne la latitude nord maximale du cadre englobant. Cf. ISO 19115-1:2014:2014-04, partie 6.6.1 et tableau B.15.1 ligne 348.</rdfs:comment>
        <rdfs:comment xml:lang="en">Indicates the north bound longitude of a bounding box. Cf. ISO 19115-1:2014:2014-04, part 6.6.1 and table B.15.1 line 348.</rdfs:comment>
        <rdfs:isDefinedBy rdf:resource="http://data.ign.fr/def/ignf"/>
        <rdfs:label xml:lang="fr">latitude nord maximale</rdfs:label>
        <rdfs:label xml:lang="en">north bound longitude</rdfs:label>
    </owl:DatatypeProperty>
    


    <!-- http://data.ign.fr/def/ignf#operationVersion -->


    <owl:DatatypeProperty rdf:about="http://data.ign.fr/def/ignf#operationVersion">
        <rdfs:domain rdf:resource="http://data.ign.fr/def/ignf#CoordinateOperation"/>
        <rdfs:range rdf:resource="http://www.w3.org/2001/XMLSchema#string"/>
        <rdfs:comment xml:lang="fr">Indique la version d&apos;une opération appliquée sur des coordonnées. Cf. ISO 19111:2007:2007-07, tableau 42, attribut version de l&apos;opération sur les coordonnées.</rdfs:comment>
        <rdfs:comment xml:lang="en">The version of an operation performed on coordinates. Cf. ISO 19111:2007:2007-07, table 42, attribute coordinate operation version.</rdfs:comment>
        <rdfs:isDefinedBy rdf:resource="http://data.ign.fr/def/ignf"/>
        <rdfs:label xml:lang="en">operation version</rdfs:label>
        <rdfs:label xml:lang="fr">version de l&apos;opération</rdfs:label>
    </owl:DatatypeProperty>
    


    <!-- http://data.ign.fr/def/ignf#scope -->


    <owl:DatatypeProperty rdf:about="http://data.ign.fr/def/ignf#scope">
        <rdfs:range rdf:resource="http://www.w3.org/2001/XMLSchema#string"/>
        <rdfs:comment xml:lang="fr">Désigne la portée de la référence. Cf. ISO 19111:2007:2007-07, tableaux 4, 33 et 42, attribut scope.</rdfs:comment>
        <rdfs:comment xml:lang="en">The scope of the referring object. Cf. ISO 19111:2007:2007-07, tables 4, 33 et 42, attribute scope.</rdfs:comment>
        <rdfs:isDefinedBy rdf:resource="http://data.ign.fr/def/ignf"/>
        <rdfs:label xml:lang="fr">portée</rdfs:label>
        <rdfs:label xml:lang="en">scope</rdfs:label>
    </owl:DatatypeProperty>
    


    <!-- http://data.ign.fr/def/ignf#sourceDimension -->


    <owl:DatatypeProperty rdf:about="http://data.ign.fr/def/ignf#sourceDimension">
        <rdfs:domain rdf:resource="http://data.ign.fr/def/ignf#OperationMethod"/>
        <rdfs:range rdf:resource="http://www.w3.org/2001/XMLSchema#integer"/>
        <rdfs:comment xml:lang="fr">Indique la dimension du système de coordonnées de référence des données en entrée d&apos;une opération. Cf. ISO 19111:2007:2007-07, tableau 48, attribut dimension du système de coordonnées de référence source.</rdfs:comment>
        <rdfs:comment xml:lang="en">The dimension of the coordinate reference system associated with the data used as input of an operation. Cf. ISO 19111:2007:2007-07, table 48, attribute dimension of source CRS.</rdfs:comment>
        <rdfs:isDefinedBy rdf:resource="http://data.ign.fr/def/ignf"/>
        <rdfs:label xml:lang="fr">dimension du système de coordonnées de référence source</rdfs:label>
        <rdfs:label xml:lang="en">source coordinate reference system dimension</rdfs:label>
    </owl:DatatypeProperty>
    


    <!-- http://data.ign.fr/def/ignf#southBoundLatitude -->


    <owl:DatatypeProperty rdf:about="http://data.ign.fr/def/ignf#southBoundLatitude">
        <rdfs:domain rdf:resource="http://data.ign.fr/def/ignf#GeographicBoundingBox"/>
        <rdfs:range rdf:resource="http://www.w3.org/2001/XMLSchema#double"/>
        <rdfs:comment xml:lang="fr">Désigne la latitude sud minimale du cadre englobant. Cf. ISO 19115-1:2014:2014-04, partie 6.6.1 et tableau B.15.1 ligne 347.</rdfs:comment>
        <rdfs:comment xml:lang="en">Indicates the south bound latitude of a bounding box. Cf. ISO 19115-1:2014:2014-04, part 6.6.1 and table B.15.1 line 347.</rdfs:comment>
        <rdfs:isDefinedBy rdf:resource="http://data.ign.fr/def/ignf"/>
        <rdfs:label xml:lang="fr">latitude sud minimale</rdfs:label>
        <rdfs:label xml:lang="en">south bound latitude</rdfs:label>
    </owl:DatatypeProperty>
    


    <!-- http://data.ign.fr/def/ignf#targetDimension -->


    <owl:DatatypeProperty rdf:about="http://data.ign.fr/def/ignf#targetDimension">
        <rdfs:domain rdf:resource="http://data.ign.fr/def/ignf#OperationMethod"/>
        <rdfs:range rdf:resource="http://www.w3.org/2001/XMLSchema#integer"/>
        <rdfs:comment xml:lang="fr">Indique la dimension du système de coordonnées de référence des données en sortie d&apos;une opération. Cf. ISO 19111:2007:2007-07, tableau 48, attribut dimension du système de coordonnées de référence cible.</rdfs:comment>
        <rdfs:comment xml:lang="en">The dimension of the coordinate reference system associated with the data obtained as output of an operation. Cf. ISO 19111:2007:2007-07, table 48, attribute dimension of target CRS.</rdfs:comment>
        <rdfs:isDefinedBy rdf:resource="http://data.ign.fr/def/ignf"/>
        <rdfs:label xml:lang="fr">dimension du système de coordonnées de référence cible</rdfs:label>
        <rdfs:label xml:lang="en">target coordinate reference system dimension</rdfs:label>
    </owl:DatatypeProperty>
    


    <!-- http://data.ign.fr/def/ignf#westBoundLongitude -->


    <owl:DatatypeProperty rdf:about="http://data.ign.fr/def/ignf#westBoundLongitude">
        <rdfs:domain rdf:resource="http://data.ign.fr/def/ignf#GeographicBoundingBox"/>
        <rdfs:range rdf:resource="http://www.w3.org/2001/XMLSchema#double"/>
        <rdfs:comment xml:lang="fr">Désigne la longitude ouest minimale du cadre englobant. Cf. ISO 19115-1:2014:2014-04, partie 6.6.1 et tableau B.15.1 ligne 345.</rdfs:comment>
        <rdfs:comment xml:lang="en">Indicates the west bound longitude of a bounding box. Cf. ISO 19115-1:2014:2014-04, part 6.6.1 and table B.15.1 line 345.</rdfs:comment>
        <rdfs:isDefinedBy rdf:resource="http://data.ign.fr/def/ignf"/>
        <rdfs:label xml:lang="fr">longitude ouest minimale</rdfs:label>
        <rdfs:label xml:lang="en">west bound longitude</rdfs:label>
    </owl:DatatypeProperty>
    


    <!-- 
    ///////////////////////////////////////////////////////////////////////////////////////
    //
    // Classes
    //
    ///////////////////////////////////////////////////////////////////////////////////////
     -->


    


    <!-- http://data.ign.fr/def/ignf#AxesList -->


    <owl:Class rdf:about="http://data.ign.fr/def/ignf#AxesList">
        <rdfs:subClassOf>
            <owl:Class>
                <owl:intersectionOf rdf:parseType="Collection">
                    <rdf:Description rdf:about="http://www.w3.org/1999/02/22-rdf-syntax-ns#List"/>
                    <owl:Restriction>
                        <owl:onProperty rdf:resource="http://www.w3.org/1999/02/22-rdf-syntax-ns#first"/>
                        <owl:allValuesFrom rdf:resource="http://data.ign.fr/def/ignf#CoordinateSystemAxis"/>
                    </owl:Restriction>
                    <owl:Restriction>
                        <owl:onProperty rdf:resource="http://www.w3.org/1999/02/22-rdf-syntax-ns#rest"/>
                        <owl:allValuesFrom rdf:resource="http://data.ign.fr/def/ignf#AxesList"/>
                    </owl:Restriction>
                </owl:intersectionOf>
            </owl:Class>
        </rdfs:subClassOf>
        <rdfs:comment xml:lang="fr">Liste ordonnée d&apos;axes de systèmes de coordonnées.</rdfs:comment>
        <rdfs:comment xml:lang="en">Ordered list of coordinates system axes.</rdfs:comment>
        <rdfs:isDefinedBy rdf:resource="http://data.ign.fr/def/ignf"/>
        <rdfs:label xml:lang="en">List of axes</rdfs:label>
        <rdfs:label xml:lang="fr">Liste d&apos;axes</rdfs:label>
    </owl:Class>
    


    <!-- http://data.ign.fr/def/ignf#CRS -->


    <owl:Class rdf:about="http://data.ign.fr/def/ignf#CRS">
        <rdfs:subClassOf>
            <owl:Restriction>
                <owl:onProperty rdf:resource="http://data.ign.fr/def/ignf#domainOfValidity"/>
                <owl:someValuesFrom rdf:resource="http://data.ign.fr/def/ignf#Extent"/>
            </owl:Restriction>
        </rdfs:subClassOf>
        <owl:disjointWith rdf:resource="http://data.ign.fr/def/ignf#CoordinateSystem"/>
        <rdfs:comment xml:lang="en">Depending on the spatial dimension of coordinates (1D, 2D, 3D), this piece of metadata is used for specifying the elements of definition associated to a given set of coordinates: its datum, its ellipsoid, its prime meridian, the type of coordinates (geocentric, geographic, projected,...), the coordinates units of measure, when appropriate the cartographic projection used, the vertical coordinate reference system. Definition translated from: http://geodesie.ign.fr/index.php?page=glossaire. Cf. ISO 19111:2007:2007-07, part 8.2, table 4 and annex B.1.</rdfs:comment>
        <rdfs:comment xml:lang="fr">Métadonnées permettant de préciser, selon la dimension spatiale des coordonnées 1D, 2D ou 3D, les éléments de définition associés au jeu de coordonnées: le système de référence terrestre, l&apos;ellipsoïde géodésique, le méridien origine, le type de coordonnées (cartésiennes géocentriques, planes, géographiques,...), les unités dans lesquelles sont exprimées les coordonnées, la projection cartographique, le référentiel altimétrique(http://geodesie.ign.fr/index.php?page=glossaire). Cf. ISO 19111:2007:2007-07, partie 8.2, tableau 4 et annexe B.1.</rdfs:comment>
        <rdfs:isDefinedBy rdf:resource="http://data.ign.fr/def/ignf"/>
        <rdfs:label xml:lang="en">Coordinate reference system (CRS)</rdfs:label>
        <rdfs:label xml:lang="fr">Système de coordonnées de référence</rdfs:label>
    </owl:Class>
    


    <!-- http://data.ign.fr/def/ignf#CartesianCS -->


    <owl:Class rdf:about="http://data.ign.fr/def/ignf#CartesianCS">
        <rdfs:subClassOf rdf:resource="http://data.ign.fr/def/ignf#CoordinateSystem"/>
        <owl:disjointWith rdf:resource="http://data.ign.fr/def/ignf#GeodeticCRS"/>
        <rdfs:comment xml:lang="en">Coordinate system which gives the position of points relative to n mutually perpendicular axes. Cf. ISO 19111:2007:2007-07, tables 15 and 18.</rdfs:comment>
        <rdfs:comment xml:lang="fr">Système de coordonnées donnant la position des points relativement à n axes perpendiculaires deux à deux. Cf. ISO 19111:2007:2007-07, tableaux 15 et 18.</rdfs:comment>
        <rdfs:isDefinedBy rdf:resource="http://data.ign.fr/def/ignf"/>
        <rdfs:label xml:lang="en">Cartesian coordinate system</rdfs:label>
        <rdfs:label xml:lang="fr">Système cartésien de coordonnées</rdfs:label>
    </owl:Class>
    


    <!-- http://data.ign.fr/def/ignf#CompoundCRS -->


    <owl:Class rdf:about="http://data.ign.fr/def/ignf#CompoundCRS">
        <rdfs:subClassOf rdf:resource="http://data.ign.fr/def/ignf#CRS"/>
        <rdfs:subClassOf>
            <owl:Restriction>
                <owl:onProperty rdf:resource="http://data.ign.fr/def/ignf#includesSingleCRS"/>
                <owl:someValuesFrom>
                    <owl:Class>
                        <owl:intersectionOf rdf:parseType="Collection">
                            <rdf:Description rdf:about="http://data.ign.fr/def/ignf#SingleCRSList"/>
                            <owl:Restriction>
                                <owl:onProperty rdf:resource="http://www.w3.org/1999/02/22-rdf-syntax-ns#rest"/>
                                <owl:qualifiedCardinality rdf:datatype="http://www.w3.org/2001/XMLSchema#nonNegativeInteger">1</owl:qualifiedCardinality>
                                <owl:onClass rdf:resource="http://data.ign.fr/def/ignf#SingleCRSList"/>
                            </owl:Restriction>
                        </owl:intersectionOf>
                    </owl:Class>
                </owl:someValuesFrom>
            </owl:Restriction>
        </rdfs:subClassOf>
        <owl:disjointWith rdf:resource="http://data.ign.fr/def/ignf#GeodeticCRS"/>
        <rdfs:comment xml:lang="en">Coordinate reference system using at least two independent single coordinate reference systems. Cf. ISO 19111:2007:2007-07, parts 8.2.3.c, 8.2.4, table 6 and annex B.1.2.4.</rdfs:comment>
        <rdfs:comment xml:lang="fr">Système de coordonnées de référence utilisant au moins deux systèmes de coordonnées de référence simples indépendants. Cf. ISO 19111:2007:2007-07, parties 8.2.3.c, 8.2.4, tableau 6 et annexe B.1.2.4.</rdfs:comment>
        <rdfs:isDefinedBy rdf:resource="http://data.ign.fr/def/ignf"/>
        <rdfs:label xml:lang="en">Compound coordinate reference system</rdfs:label>
        <rdfs:label xml:lang="fr">Système de coordonnées de référence combiné</rdfs:label>
    </owl:Class>
    


    <!-- http://data.ign.fr/def/ignf#Conversion -->


    <owl:Class rdf:about="http://data.ign.fr/def/ignf#Conversion">
        <rdfs:subClassOf rdf:resource="http://data.ign.fr/def/ignf#SingleOperation"/>
        <rdfs:comment xml:lang="en">Coordinate operation in which both coordinate reference systems are based on the same datum. Cf. ISO 19111:2007:2007-07, table 45 and annex B.4.2.</rdfs:comment>
        <rdfs:comment xml:lang="fr">Opération sur les coordonnées dans laquelle les deux systèmes de coordonnées de référence sont basés sur le même référentiel (ex: projection cartographique). Cf. ISO 19111:2007:2007-07, tableau 45 et annexe B.4.2.</rdfs:comment>
        <rdfs:isDefinedBy rdf:resource="http://data.ign.fr/def/ignf"/>
        <rdfs:label xml:lang="en">Conversion</rdfs:label>
        <rdfs:label xml:lang="fr">Conversion</rdfs:label>
    </owl:Class>
    


    <!-- http://data.ign.fr/def/ignf#CoordinateOperation -->


    <owl:Class rdf:about="http://data.ign.fr/def/ignf#CoordinateOperation">
        <rdfs:comment xml:lang="en">Mathematical operation on coordinates, based on one-to-one relationship, that changes coordinates from one coordinate reference system to another. Cf. ISO 19111:2007:2007-07, part 11.1, table 42 and annex B.4.</rdfs:comment>
        <rdfs:comment xml:lang="fr">Opération mathématique sur des coordonnées, basée sur une relation 1:1, qui change ces coordonnées d&apos;une système de coordonnées de référence à un autre. Cf. ISO 19111:2007:2007-07, partie 11.1, tableau 42 et annexe B.4.</rdfs:comment>
        <rdfs:isDefinedBy rdf:resource="http://data.ign.fr/def/ignf"/>
        <rdfs:label xml:lang="en">Coordinate operation</rdfs:label>
        <rdfs:label xml:lang="fr">Opération sur les coordonnées</rdfs:label>
    </owl:Class>
    


    <!-- http://data.ign.fr/def/ignf#CoordinateSystem -->


    <owl:Class rdf:about="http://data.ign.fr/def/ignf#CoordinateSystem">
        <rdfs:subClassOf>
            <owl:Restriction>
                <owl:onProperty rdf:resource="http://data.ign.fr/def/ignf#axis"/>
                <owl:minQualifiedCardinality rdf:datatype="http://www.w3.org/2001/XMLSchema#nonNegativeInteger">1</owl:minQualifiedCardinality>
                <owl:onClass rdf:resource="http://data.ign.fr/def/ignf#AxesList"/>
            </owl:Restriction>
        </rdfs:subClassOf>
        <rdfs:comment xml:lang="fr">Ensemble d&apos;axes couvrant un espace de coordonnées, et de règles mathématiques permettant l&apos;affectation de coordonnées à un point. Cf. ISO 19111:2007:2007-07, partie 9.2, tableau 17 et annexe B.2.</rdfs:comment>
        <rdfs:comment xml:lang="en">Set of axes that spans a given coordinate space and of mathematical rules for specifying how coordinates are to be assigned to points. Cf. ISO 19111:2007:2007-07, part 9.2, table 17 and annex B.2.</rdfs:comment>
        <rdfs:isDefinedBy rdf:resource="http://data.ign.fr/def/ignf"/>
        <rdfs:label xml:lang="en">Coordinate system</rdfs:label>
        <rdfs:label xml:lang="fr">Système de coordonnées</rdfs:label>
    </owl:Class>
    


    <!-- http://data.ign.fr/def/ignf#CoordinateSystemAxis -->


    <owl:Class rdf:about="http://data.ign.fr/def/ignf#CoordinateSystemAxis">
        <rdfs:comment xml:lang="fr">Axe par rapport auquel une coordonnée d&apos;un point est spécifiée dans un système de coordonnées. Cf. ISO 19111:2007:2007-07, partie 9.3, tableau 27 et annexe B.2.2.</rdfs:comment>
        <rdfs:comment xml:lang="en">Axis composing a coordinate system and used to specify one given coordinate in a coordinate tuple describing the position of a point. Cf. ISO 19111:2007:2007-07, part 9.3, table 27 and annex B.2.2.</rdfs:comment>
        <rdfs:isDefinedBy rdf:resource="http://data.ign.fr/def/ignf"/>
        <rdfs:label xml:lang="fr">Axe</rdfs:label>
        <rdfs:label xml:lang="en">Axis</rdfs:label>
    </owl:Class>
    


    <!-- http://data.ign.fr/def/ignf#Datum -->


    <owl:Class rdf:about="http://data.ign.fr/def/ignf#Datum">
        <rdfs:comment xml:lang="en">Parameter or set of parameters that define the position of the origin, the scale and the orientation of a coordinate system. Cf. ISO 19111:2007:2007-07, part 10.1, table 33 and annex B.3.</rdfs:comment>
        <rdfs:comment xml:lang="fr">Paramètre ou ensemble de paramètres définissant la position de l&apos;origine, l&apos;échelle et l&apos;orientation d&apos;un système de coordonnées. Cf. ISO 19111:2007:2007-07, partie 10.1, tableau 33 et annexe B.3.</rdfs:comment>
        <rdfs:isDefinedBy rdf:resource="http://data.ign.fr/def/ignf"/>
        <rdfs:label xml:lang="en">Datum</rdfs:label>
        <rdfs:label xml:lang="fr">Référentiel</rdfs:label>
    </owl:Class>
    


    <!-- http://data.ign.fr/def/ignf#Ellipsoid -->


    <owl:Class rdf:about="http://data.ign.fr/def/ignf#Ellipsoid">
        <rdfs:subClassOf>
            <owl:Class>
                <owl:intersectionOf rdf:parseType="Collection">
                    <owl:Class>
                        <owl:unionOf rdf:parseType="Collection">
                            <owl:Restriction>
                                <owl:onProperty rdf:resource="http://data.ign.fr/def/ignf#inverseFlattening"/>
                                <owl:qualifiedCardinality rdf:datatype="http://www.w3.org/2001/XMLSchema#nonNegativeInteger">1</owl:qualifiedCardinality>
                                <owl:onClass rdf:resource="http://qudt.org/1.1/schema/qudt#QuantityValue"/>
                            </owl:Restriction>
                            <owl:Restriction>
                                <owl:onProperty rdf:resource="http://data.ign.fr/def/ignf#semiMinorAxis"/>
                                <owl:qualifiedCardinality rdf:datatype="http://www.w3.org/2001/XMLSchema#nonNegativeInteger">1</owl:qualifiedCardinality>
                                <owl:onClass rdf:resource="http://qudt.org/1.1/schema/qudt#QuantityValue"/>
                            </owl:Restriction>
                            <owl:Restriction>
                                <owl:onProperty rdf:resource="http://data.ign.fr/def/ignf#isSphere"/>
                                <owl:qualifiedCardinality rdf:datatype="http://www.w3.org/2001/XMLSchema#nonNegativeInteger">1</owl:qualifiedCardinality>
                                <owl:onDataRange rdf:resource="http://www.w3.org/2001/XMLSchema#boolean"/>
                            </owl:Restriction>
                        </owl:unionOf>
                    </owl:Class>
                    <owl:Restriction>
                        <owl:onProperty rdf:resource="http://data.ign.fr/def/ignf#semiMajorAxis"/>
                        <owl:qualifiedCardinality rdf:datatype="http://www.w3.org/2001/XMLSchema#nonNegativeInteger">1</owl:qualifiedCardinality>
                        <owl:onClass rdf:resource="http://qudt.org/1.1/schema/qudt#QuantityValue"/>
                    </owl:Restriction>
                </owl:intersectionOf>
            </owl:Class>
        </rdfs:subClassOf>
        <owl:disjointWith rdf:resource="http://data.ign.fr/def/ignf#PrimeMeridian"/>
        <rdfs:comment xml:lang="fr">Surface de révolution engendrée par une ellipse tournant autour de son petit axe, définie par le rayon équatorial et un paramètre d&apos;aplatissement, et sensiblement géocentrique. Note : Il s&apos;agit d&apos;un modèle mathématique du géoïde, c&apos;est-à-dire de la Terre débarrassée de son relief. Il existe de nombreux ellipsoïdes géodésiques. Cf. ISO 19111:2007:2007-07, partie 10.2.2, tableau 36 et annexe B.3.2.3.</rdfs:comment>
        <rdfs:comment xml:lang="en">Surface formed by the rotation of an ellipse about its minor axis, defined by a semi-major axis and a flattening parameter and fairly geocentric. NB : It is a mathematical model of the geoid, i.e. the Earth without its relief. Many geodetic ellipsoids exist. Cf. ISO 19111:2007:2007-07, part 10.2.2, table 36 and annex B.3.2.3.</rdfs:comment>
        <rdfs:isDefinedBy rdf:resource="http://data.ign.fr/def/ignf"/>
        <rdfs:label xml:lang="en">Ellipsoid</rdfs:label>
        <rdfs:label xml:lang="fr">Ellipsoïde</rdfs:label>
    </owl:Class>
    


    <!-- http://data.ign.fr/def/ignf#EllipsoidalCS -->


    <owl:Class rdf:about="http://data.ign.fr/def/ignf#EllipsoidalCS">
        <rdfs:subClassOf rdf:resource="http://data.ign.fr/def/ignf#CoordinateSystem"/>
        <owl:disjointWith rdf:resource="http://data.ign.fr/def/ignf#GeodeticCRS"/>
        <rdfs:comment xml:lang="en">Coordinate system which gives the position is specified by geodetic latitude, geodetic longitude and (in the three-dimensional case) ellipsoidal height. Cf. ISO 19111:2007:2007-07, tables 15 and 20.</rdfs:comment>
        <rdfs:comment xml:lang="fr">Système de coordonnées dans lequel la position est spécifiée par la latitude géodésique, la longitude géodésique et (dans le cas tridimensionnel) la hauteur ellipsoïdale. Cf. ISO 19111:2007:2007-07, tableaux 15 et 20.</rdfs:comment>
        <rdfs:isDefinedBy rdf:resource="http://data.ign.fr/def/ignf"/>
        <rdfs:label xml:lang="en">Ellipsoidal coordinate system</rdfs:label>
        <rdfs:label xml:lang="fr">Système de coordonnées ellipsoïdal</rdfs:label>
    </owl:Class>
    


    <!-- http://data.ign.fr/def/ignf#Extent -->


    <owl:Class rdf:about="http://data.ign.fr/def/ignf#Extent">
        <rdfs:comment xml:lang="en">Geographic area or time interval in which the referring object is valid. Cf. ISO 19115-1:2014:2014-04, part 6.6.1 and table B.15 line 335.</rdfs:comment>
        <rdfs:comment xml:lang="fr">Zone géographique ou intervalle de temps dans lequel la référence est valide. Cf. ISO 19115-1:2014:2014-04, partie 6.6.1 et tableau B.15 ligne 335.</rdfs:comment>
        <rdfs:isDefinedBy rdf:resource="http://data.ign.fr/def/ignf"/>
        <rdfs:label xml:lang="en">Extent</rdfs:label>
        <rdfs:label xml:lang="fr">Étendue</rdfs:label>
    </owl:Class>
    


    <!-- http://data.ign.fr/def/ignf#GeodeticCRS -->


    <owl:Class rdf:about="http://data.ign.fr/def/ignf#GeodeticCRS">
        <rdfs:subClassOf rdf:resource="http://data.ign.fr/def/ignf#SingleCRS"/>
        <rdfs:subClassOf>
            <owl:Restriction>
                <owl:onProperty rdf:resource="http://data.ign.fr/def/ignf#datum"/>
                <owl:allValuesFrom rdf:resource="http://data.ign.fr/def/ignf#GeodeticDatum"/>
            </owl:Restriction>
        </rdfs:subClassOf>
        <rdfs:comment xml:lang="en">Coordinate reference system associated with a geodetic datum. Cf. ISO 19111:2007:2007-07, part 8.2.2.a, table 10 and annex B.1.2.1.a.</rdfs:comment>
        <rdfs:comment xml:lang="fr">Système de coordonnées de référence associé à un référentiel géodésique. Cf. ISO 19111:2007:2007-07, partie 8.2.2.a, tableau 10 et annexe B.1.2.1.a.</rdfs:comment>
        <rdfs:isDefinedBy rdf:resource="http://data.ign.fr/def/ignf"/>
        <rdfs:label xml:lang="en">Geodetic coordinate reference system</rdfs:label>
        <rdfs:label xml:lang="fr">Système de coordonnées de référence geodésique</rdfs:label>
    </owl:Class>
    


    <!-- http://data.ign.fr/def/ignf#GeodeticDatum -->


    <owl:Class rdf:about="http://data.ign.fr/def/ignf#GeodeticDatum">
        <rdfs:subClassOf rdf:resource="http://data.ign.fr/def/ignf#Datum"/>
        <rdfs:subClassOf>
            <owl:Class>
                <owl:intersectionOf rdf:parseType="Collection">
                    <owl:Restriction>
                        <owl:onProperty rdf:resource="http://data.ign.fr/def/ignf#ellipsoid"/>
                        <owl:qualifiedCardinality rdf:datatype="http://www.w3.org/2001/XMLSchema#nonNegativeInteger">1</owl:qualifiedCardinality>
                        <owl:onClass rdf:resource="http://data.ign.fr/def/ignf#Ellipsoid"/>
                    </owl:Restriction>
                    <owl:Restriction>
                        <owl:onProperty rdf:resource="http://data.ign.fr/def/ignf#primeMeridian"/>
                        <owl:qualifiedCardinality rdf:datatype="http://www.w3.org/2001/XMLSchema#nonNegativeInteger">1</owl:qualifiedCardinality>
                        <owl:onClass rdf:resource="http://data.ign.fr/def/ignf#PrimeMeridian"/>
                    </owl:Restriction>
                </owl:intersectionOf>
            </owl:Class>
        </rdfs:subClassOf>
        <rdfs:comment xml:lang="en">Datum describing the relation of a two- or three-dimensional coordinate system to the Earth. Cf. ISO 19111:2007:2007-07, part 10.2, table 34 and annex B.3.2.</rdfs:comment>
        <rdfs:comment xml:lang="fr">Référentiel décrivant la relation entre un système de coordonnées à deux ou trois dimensions et la Terre. Cf. ISO 19111:2007:2007-07, partie 10.2, tableau 34 et annexe B.3.2.</rdfs:comment>
        <rdfs:isDefinedBy rdf:resource="http://data.ign.fr/def/ignf"/>
        <rdfs:label xml:lang="en">Geodetic datum</rdfs:label>
        <rdfs:label xml:lang="fr">Référentiel géodésique</rdfs:label>
    </owl:Class>
    


    <!-- http://data.ign.fr/def/ignf#GeographicBoundingBox -->


    <owl:Class rdf:about="http://data.ign.fr/def/ignf#GeographicBoundingBox">
        <rdfs:subClassOf>
            <owl:Class>
                <owl:intersectionOf rdf:parseType="Collection">
                    <owl:Restriction>
                        <owl:onProperty rdf:resource="http://data.ign.fr/def/ignf#eastBoundLongitude"/>
                        <owl:qualifiedCardinality rdf:datatype="http://www.w3.org/2001/XMLSchema#nonNegativeInteger">1</owl:qualifiedCardinality>
                        <owl:onDataRange rdf:resource="http://www.w3.org/2001/XMLSchema#double"/>
                    </owl:Restriction>
                    <owl:Restriction>
                        <owl:onProperty rdf:resource="http://data.ign.fr/def/ignf#northBoundLatitude"/>
                        <owl:qualifiedCardinality rdf:datatype="http://www.w3.org/2001/XMLSchema#nonNegativeInteger">1</owl:qualifiedCardinality>
                        <owl:onDataRange rdf:resource="http://www.w3.org/2001/XMLSchema#double"/>
                    </owl:Restriction>
                    <owl:Restriction>
                        <owl:onProperty rdf:resource="http://data.ign.fr/def/ignf#southBoundLatitude"/>
                        <owl:qualifiedCardinality rdf:datatype="http://www.w3.org/2001/XMLSchema#nonNegativeInteger">1</owl:qualifiedCardinality>
                        <owl:onDataRange rdf:resource="http://www.w3.org/2001/XMLSchema#double"/>
                    </owl:Restriction>
                    <owl:Restriction>
                        <owl:onProperty rdf:resource="http://data.ign.fr/def/ignf#westBoundLongitude"/>
                        <owl:qualifiedCardinality rdf:datatype="http://www.w3.org/2001/XMLSchema#nonNegativeInteger">1</owl:qualifiedCardinality>
                        <owl:onDataRange rdf:resource="http://www.w3.org/2001/XMLSchema#double"/>
                    </owl:Restriction>
                </owl:intersectionOf>
            </owl:Class>
        </rdfs:subClassOf>
        <rdfs:comment xml:lang="en">Box bounding an area of interest. Cf. ISO 19115-1:2014:2014-04, part 6.6.1 and table B.15.1 line 344.</rdfs:comment>
        <rdfs:comment xml:lang="fr">Cadre délimitant une zone d&apos;intérêt. Cf. ISO 19115-1:2014:2014-04, partie 6.6.1 et tableau B.15.1 ligne 344.</rdfs:comment>
        <rdfs:isDefinedBy rdf:resource="http://data.ign.fr/def/ignf"/>
        <rdfs:label xml:lang="fr">Cadre englobant géographique</rdfs:label>
        <rdfs:label xml:lang="en">Geographic bounding box</rdfs:label>
    </owl:Class>
    


    <!-- http://data.ign.fr/def/ignf#OperationMethod -->


    <owl:Class rdf:about="http://data.ign.fr/def/ignf#OperationMethod">
        <rdfs:comment xml:lang="fr">Méthode utilisée pour faire une opération sur des coordonnées. Cf. ISO 19111:2007:2007-07, tableau 48 et annexe B.4.5.</rdfs:comment>
        <rdfs:comment xml:lang="en">The method (algorithm or procedure) used to perform the coordinate operation. Cf. ISO 19111:2007:2007-07, table 48 and annex B.4.5.</rdfs:comment>
        <rdfs:isDefinedBy rdf:resource="http://data.ign.fr/def/ignf"/>
        <rdfs:label xml:lang="fr">Méthode</rdfs:label>
        <rdfs:label xml:lang="en">Operation method</rdfs:label>
    </owl:Class>
    


    <!-- http://data.ign.fr/def/ignf#OperationParameter -->


    <owl:Class rdf:about="http://data.ign.fr/def/ignf#OperationParameter">
        <rdfs:comment xml:lang="en">Parameter used by a method to perform some coordinate operation. Cf. ISO 19111:2007:2007-07, table 52 and annex B.4.5.</rdfs:comment>
        <rdfs:comment xml:lang="fr">Paramètre utilisé par une méthode pour faire une opération sur des coordonnées. Cf. ISO 19111:2007:2007-07, tableau 52 et annexe B.4.5.</rdfs:comment>
        <rdfs:isDefinedBy rdf:resource="http://data.ign.fr/def/ignf"/>
        <rdfs:label xml:lang="en">Operation parameter</rdfs:label>
        <rdfs:label xml:lang="fr">Paramètre</rdfs:label>
    </owl:Class>
    


    <!-- http://data.ign.fr/def/ignf#OperationParameterValue -->


    <owl:Class rdf:about="http://data.ign.fr/def/ignf#OperationParameterValue">
        <rdfs:comment xml:lang="fr">Valeur d&apos;un paramètre utilisé par une méthode pour faire une opération sur des coordonnées. Cf. ISO 19111:2007:2007-07, tableau 55.</rdfs:comment>
        <rdfs:comment xml:lang="en">Value of a parameter used by a method to perform some coordinate operation. Cf. ISO 19111:2007:2007-07, table 55.</rdfs:comment>
        <rdfs:isDefinedBy rdf:resource="http://data.ign.fr/def/ignf"/>
        <rdfs:label xml:lang="en">Operation parameter value</rdfs:label>
        <rdfs:label xml:lang="fr">Valeur de paramètre</rdfs:label>
    </owl:Class>
    


    <!-- http://data.ign.fr/def/ignf#PrimeMeridian -->


    <owl:Class rdf:about="http://data.ign.fr/def/ignf#PrimeMeridian">
        <rdfs:comment xml:lang="en">Meridian from which the longitudes of other meridians are quantified. Cf. ISO 19111:2007:2007-07, part 10.2.1, table 35 and annex B.3.2.2.</rdfs:comment>
        <rdfs:comment xml:lang="fr">Méridien à partir duquel les longitudes d&apos;autres méridiens sont mesurées. Cf. ISO 19111:2007:2007-07, partie 10.2.1, tableau 35 et annexe B.3.2.2.</rdfs:comment>
        <rdfs:isDefinedBy rdf:resource="http://data.ign.fr/def/ignf"/>
        <rdfs:label xml:lang="fr">Méridien origine</rdfs:label>
        <rdfs:label xml:lang="en">Prime meridian</rdfs:label>
    </owl:Class>
    


    <!-- http://data.ign.fr/def/ignf#ProjectedCRS -->


    <owl:Class rdf:about="http://data.ign.fr/def/ignf#ProjectedCRS">
        <rdfs:subClassOf rdf:resource="http://data.ign.fr/def/ignf#SingleCRS"/>
        <rdfs:subClassOf>
            <owl:Restriction>
                <owl:onProperty rdf:resource="http://data.ign.fr/def/ignf#baseCRS"/>
                <owl:allValuesFrom rdf:resource="http://data.ign.fr/def/ignf#GeodeticCRS"/>
            </owl:Restriction>
        </rdfs:subClassOf>
        <rdfs:comment xml:lang="en">Coordinate reference system derived from a two-dimensional geodetic coordinate reference system by applying a map projection. Cf. ISO 19111:2007:2007-07, part 8.2.3.b, table 11 and annex B.1.2.3.</rdfs:comment>
        <rdfs:comment xml:lang="fr">Système de coordonnées de référence dérivé par projection cartographique d&apos;un système de coordonnées de référence bidimentionnel. Cf. ISO 19111:2007:2007-07, partie 8.2.3.b, tableau 11 et annexe B.1.2.3.</rdfs:comment>
        <rdfs:isDefinedBy rdf:resource="http://data.ign.fr/def/ignf"/>
        <rdfs:label xml:lang="en">Projected coordinate reference system</rdfs:label>
        <rdfs:label xml:lang="fr">Système de coordonnées de référence projeté</rdfs:label>
    </owl:Class>
    


    <!-- http://data.ign.fr/def/ignf#SingleCRS -->


    <owl:Class rdf:about="http://data.ign.fr/def/ignf#SingleCRS">
        <rdfs:subClassOf rdf:resource="http://data.ign.fr/def/ignf#CRS"/>
        <rdfs:subClassOf>
            <owl:Class>
                <owl:intersectionOf rdf:parseType="Collection">
                    <owl:Restriction>
                        <owl:onProperty rdf:resource="http://data.ign.fr/def/ignf#coordinateSystem"/>
                        <owl:qualifiedCardinality rdf:datatype="http://www.w3.org/2001/XMLSchema#nonNegativeInteger">1</owl:qualifiedCardinality>
                        <owl:onClass rdf:resource="http://data.ign.fr/def/ignf#CoordinateSystem"/>
                    </owl:Restriction>
                    <owl:Restriction>
                        <owl:onProperty rdf:resource="http://data.ign.fr/def/ignf#datum"/>
                        <owl:qualifiedCardinality rdf:datatype="http://www.w3.org/2001/XMLSchema#nonNegativeInteger">1</owl:qualifiedCardinality>
                        <owl:onClass rdf:resource="http://data.ign.fr/def/ignf#Datum"/>
                    </owl:Restriction>
                </owl:intersectionOf>
            </owl:Class>
        </rdfs:subClassOf>
        <rdfs:comment xml:lang="en">Coordinate reference system consisting of one coordinate system and one datum. Cf. ISO 19111:2007:2007-07, table 5.</rdfs:comment>
        <rdfs:comment xml:lang="fr">Système de coordonnées de référence composé d&apos;un système de coordonnées et d&apos;un référentiel. Cf. ISO 19111:2007:2007-07 tableau 5.</rdfs:comment>
        <rdfs:isDefinedBy rdf:resource="http://data.ign.fr/def/ignf"/>
        <rdfs:label xml:lang="en">Single coordinate reference system</rdfs:label>
        <rdfs:label xml:lang="fr">Système de coordonnées de référence simple</rdfs:label>
    </owl:Class>
    


    <!-- http://data.ign.fr/def/ignf#SingleCRSList -->


    <owl:Class rdf:about="http://data.ign.fr/def/ignf#SingleCRSList">
        <rdfs:subClassOf>
            <owl:Class>
                <owl:intersectionOf rdf:parseType="Collection">
                    <rdf:Description rdf:about="http://www.w3.org/1999/02/22-rdf-syntax-ns#List"/>
                    <owl:Restriction>
                        <owl:onProperty rdf:resource="http://www.w3.org/1999/02/22-rdf-syntax-ns#first"/>
                        <owl:allValuesFrom rdf:resource="http://data.ign.fr/def/ignf#SingleCRS"/>
                    </owl:Restriction>
                    <owl:Restriction>
                        <owl:onProperty rdf:resource="http://www.w3.org/1999/02/22-rdf-syntax-ns#rest"/>
                        <owl:allValuesFrom rdf:resource="http://data.ign.fr/def/ignf#SingleCRSList"/>
                    </owl:Restriction>
                </owl:intersectionOf>
            </owl:Class>
        </rdfs:subClassOf>
        <rdfs:comment xml:lang="fr">Liste ordonnée de systèmes de coordonnées de référence simples.</rdfs:comment>
        <rdfs:comment xml:lang="en">Ordered list of single coordinate reference systems.</rdfs:comment>
        <rdfs:isDefinedBy rdf:resource="http://data.ign.fr/def/ignf"/>
        <rdfs:label xml:lang="en">List of single coordinate reference systems</rdfs:label>
        <rdfs:label xml:lang="fr">Liste de systèmes de coordonnées de référence simples</rdfs:label>
    </owl:Class>
    


    <!-- http://data.ign.fr/def/ignf#SingleOperation -->


    <owl:Class rdf:about="http://data.ign.fr/def/ignf#SingleOperation">
        <rdfs:subClassOf rdf:resource="http://data.ign.fr/def/ignf#CoordinateOperation"/>
        <rdfs:comment xml:lang="en">A non concatenated coordinate operation. Cf. ISO 19111:2007:2007-07, table 43.</rdfs:comment>
        <rdfs:comment xml:lang="fr">Opération non concaténée sur des coordonnées. Cf. ISO 19111:2007:2007-07, tableau 43.</rdfs:comment>
        <rdfs:isDefinedBy rdf:resource="http://data.ign.fr/def/ignf"/>
        <rdfs:label xml:lang="fr">Opération simple sur les coordonnées</rdfs:label>
        <rdfs:label xml:lang="en">Single coordinate operation</rdfs:label>
    </owl:Class>
    


    <!-- http://data.ign.fr/def/ignf#Transformation -->


    <owl:Class rdf:about="http://data.ign.fr/def/ignf#Transformation">
        <rdfs:subClassOf rdf:resource="http://data.ign.fr/def/ignf#SingleOperation"/>
        <rdfs:comment xml:lang="en">Coordinate operation in which the two coordinate reference systems are based on different datums. Cf. ISO 19111:2007:2007-07, table 44.</rdfs:comment>
        <rdfs:comment xml:lang="fr">Opération sur les coordonnées dans laquelle les deux systèmes de coordonnées de référence sont basés sur des référentiels distincts. Cf. ISO 19111:2007:2007-07, tableau 44.</rdfs:comment>
        <rdfs:isDefinedBy rdf:resource="http://data.ign.fr/def/ignf"/>
        <rdfs:label xml:lang="en">Transformation</rdfs:label>
        <rdfs:label xml:lang="fr">Transformation</rdfs:label>
    </owl:Class>
    


    <!-- http://data.ign.fr/def/ignf#VerticalCRS -->


    <owl:Class rdf:about="http://data.ign.fr/def/ignf#VerticalCRS">
        <rdfs:subClassOf rdf:resource="http://data.ign.fr/def/ignf#SingleCRS"/>
        <rdfs:subClassOf>
            <owl:Class>
                <owl:intersectionOf rdf:parseType="Collection">
                    <owl:Restriction>
                        <owl:onProperty rdf:resource="http://data.ign.fr/def/ignf#coordinateSystem"/>
                        <owl:allValuesFrom rdf:resource="http://data.ign.fr/def/ignf#VerticalCS"/>
                    </owl:Restriction>
                    <owl:Restriction>
                        <owl:onProperty rdf:resource="http://data.ign.fr/def/ignf#datum"/>
                        <owl:allValuesFrom rdf:resource="http://data.ign.fr/def/ignf#VerticalDatum"/>
                    </owl:Restriction>
                </owl:intersectionOf>
            </owl:Class>
        </rdfs:subClassOf>
        <owl:disjointWith rdf:resource="http://data.ign.fr/def/ignf#VerticalCS"/>
        <rdfs:comment xml:lang="en">One-dimensional coordinate reference system associated with a vertical datum and used for recording heights or depths.Ellipsoidal heights are not captured in a vertical coordinate reference system but as part of a 3D coordinates tuple defined in a geodetic 3D coordinate reference system. Cf. ISO 19111:2007:2007-07, parts 8.2.2.b, table 14 and annex B.1.2.1.b.</rdfs:comment>
        <rdfs:comment xml:lang="fr">Système de coordonnées de référence à une dimension, associé à un référentiel vertical, et utilisé pour enregistrer des hauteurs ou des profondeurs. Les hauteurs ellipsoïdales ne sont pas enregistrées à l&apos;aide d&apos;un système de coordonnées de référence vertical, mais au sein d&apos;un tuple de coordonnées 3D défini dans un système de coordonnées de référence géodésique 3D. Cf. ISO 19111:2007:2007-07, parties 8.2.2.b, tableau 14 et annexe B.1.2.1.b.</rdfs:comment>
        <rdfs:isDefinedBy rdf:resource="http://data.ign.fr/def/ignf"/>
        <rdfs:label xml:lang="fr">Système de coordonnées de référence vertical</rdfs:label>
        <rdfs:label xml:lang="en">Vertical coordinate reference system</rdfs:label>
    </owl:Class>
    


    <!-- http://data.ign.fr/def/ignf#VerticalCS -->


    <owl:Class rdf:about="http://data.ign.fr/def/ignf#VerticalCS">
        <rdfs:subClassOf rdf:resource="http://data.ign.fr/def/ignf#CoordinateSystem"/>
        <rdfs:comment xml:lang="en">One-dimensional coordinate system used for gravity related height or depth measurements. Cf. ISO 19111:2007:2007-07, tables 15 and 25.</rdfs:comment>
        <rdfs:comment xml:lang="fr">Système de coordonnées à une dimension utilisé pour les mesures de hauteur ou de profondeur relatives à la gravité. Cf. ISO 19111:2007:2007-07, tableaux 15 et 25.</rdfs:comment>
        <rdfs:isDefinedBy rdf:resource="http://data.ign.fr/def/ignf"/>
        <rdfs:label xml:lang="fr">Système de coordonnées vertical</rdfs:label>
        <rdfs:label xml:lang="en">Vertical coordinate system</rdfs:label>
    </owl:Class>
    


    <!-- http://data.ign.fr/def/ignf#VerticalDatum -->


    <owl:Class rdf:about="http://data.ign.fr/def/ignf#VerticalDatum">
        <rdfs:subClassOf rdf:resource="http://data.ign.fr/def/ignf#Datum"/>
        <rdfs:comment xml:lang="en">Datum describing the relation of gravity-related heights or depths to the Earth. Cf. ISO 19111:2007:2007-07, table 41 and annex B.3.3.</rdfs:comment>
        <rdfs:comment xml:lang="fr">Référentiel décrivant la relation entre les hauteurs ou les profondeurs relatives à la gravité et la Terre. Cf. ISO 19111:2007:2007-07, tableau 41 et annexe B.3.3.</rdfs:comment>
        <rdfs:isDefinedBy rdf:resource="http://data.ign.fr/def/ignf"/>
        <rdfs:label xml:lang="fr">Référentiel vertical</rdfs:label>
        <rdfs:label xml:lang="en">Vertical datum</rdfs:label>
    </owl:Class>
    


    <!-- http://purl.org/vocommons/voaf#Vocabulary -->


    <owl:Class rdf:about="http://purl.org/vocommons/voaf#Vocabulary"/>
    


    <!-- http://qudt.org/1.1/schema/qudt#AngleUnit -->


    <owl:Class rdf:about="http://qudt.org/1.1/schema/qudt#AngleUnit"/>
    


    <!-- http://qudt.org/1.1/schema/qudt#CountingUnit -->


    <owl:Class rdf:about="http://qudt.org/1.1/schema/qudt#CountingUnit"/>
    


    <!-- http://qudt.org/1.1/schema/qudt#LengthUnit -->


    <owl:Class rdf:about="http://qudt.org/1.1/schema/qudt#LengthUnit"/>
    


    <!-- http://qudt.org/1.1/schema/qudt#QuantityValue -->


    <owl:Class rdf:about="http://qudt.org/1.1/schema/qudt#QuantityValue"/>
    


    <!-- http://www.w3.org/1999/02/22-rdf-syntax-ns#List -->


    <owl:Class rdf:about="http://www.w3.org/1999/02/22-rdf-syntax-ns#List"/>
    


    <!-- http://www.w3.org/2006/time#Instant -->


    <owl:Class rdf:about="http://www.w3.org/2006/time#Instant"/>
    


    <!-- http://www.w3.org/2006/time#Interval -->


    <owl:Class rdf:about="http://www.w3.org/2006/time#Interval"/>
    


    <!-- http://www.w3.org/ns/org#Membership -->


    <owl:Class rdf:about="http://www.w3.org/ns/org#Membership"/>
    


    <!-- http://www.w3.org/ns/org#Role -->


    <owl:Class rdf:about="http://www.w3.org/ns/org#Role"/>
    


    <!-- http://xmlns.com/foaf/0.1/Person -->


    <owl:Class rdf:about="http://xmlns.com/foaf/0.1/Person"/>
    


    <!-- 
    ///////////////////////////////////////////////////////////////////////////////////////
    //
    // Individuals
    //
    ///////////////////////////////////////////////////////////////////////////////////////
     -->


    


    <!-- http://data.ign.fr/def/ignf -->


    <owl:NamedIndividual rdf:about="http://data.ign.fr/def/ignf">
        <rdf:type rdf:resource="http://purl.org/vocommons/voaf#Vocabulary"/>
    </owl:NamedIndividual>
    


    <!-- http://www.eurecom.fr/~atemezin/ -->


    <owl:NamedIndividual rdf:about="http://www.eurecom.fr/~atemezin/">
        <rdf:type rdf:resource="http://xmlns.com/foaf/0.1/Person"/>
    </owl:NamedIndividual>
    


    <!-- http://www.eurecom.fr/~troncy/ -->


    <owl:NamedIndividual rdf:about="http://www.eurecom.fr/~troncy/">
        <rdf:type rdf:resource="http://xmlns.com/foaf/0.1/Person"/>
    </owl:NamedIndividual>
    <rdf:Description rdf:nodeID="genid76">
        <rdf:type rdf:resource="http://xmlns.com/foaf/0.1/Person"/>
        <org:hasMembership>
            <rdf:Description rdf:nodeID="genid77">
                <rdf:type rdf:resource="http://www.w3.org/ns/org#Membership"/>
                <org:memberDuring>
                    <rdf:Description rdf:nodeID="genid78">
                        <rdf:type rdf:resource="http://www.w3.org/2006/time#Interval"/>
                        <time:hasBeginning>
                            <rdf:Description rdf:nodeID="genid79">
                                <rdf:type rdf:resource="http://www.w3.org/2006/time#Instant"/>
                                <time:inXSDDateTimeStamp rdf:datatype="http://www.w3.org/2001/XMLSchema#dateTimeStamp">2005-09-09</time:inXSDDateTimeStamp>
                            </rdf:Description>
                        </time:hasBeginning>
                    </rdf:Description>
                </org:memberDuring>
                <org:organization rdf:resource="http://recherche.ign.fr/"/>
                <org:organization rdf:resource="http://www.ign.fr/"/>
                <org:role>
                    <rdf:Description rdf:nodeID="genid80">
                        <rdf:type rdf:resource="http://www.w3.org/ns/org#Role"/>
                        <rdfs:label xml:lang="fr">Chargée de recherche</rdfs:label>
                        <rdfs:label xml:lang="en">Survey engineer and Scientist</rdfs:label>
                    </rdf:Description>
                </org:role>
            </rdf:Description>
        </org:hasMembership>
        <foaf:family_name>Abadie</foaf:family_name>
        <foaf:firstName>Nathalie</foaf:firstName>
        <foaf:mbox rdf:resource="mailto:nathalie-f.abadie@ign.fr"/>
        <foaf:name>Nathalie Abadie</foaf:name>
        <foaf:workInfoHomepage rdf:resource="http://recherche.ign.fr/labos/cogit/cv.php?prenom=Nathalie&amp;nom=Abadie"/>
    </rdf:Description>
</rdf:RDF>



<!-- Generated by the OWL API (version 5.1.9) https://github.com/owlcs/owlapi/ -->


