<?xml version="1.0"?>
<rdf:RDF xmlns="http://w3id.org/nfdi4ing/metadata4ing#"
     xml:base="http://w3id.org/nfdi4ing/metadata4ing"
     xmlns:owl="http://www.w3.org/2002/07/owl#"
     xmlns:rdf="http://www.w3.org/1999/02/22-rdf-syntax-ns#"
     xmlns:xml="http://www.w3.org/XML/1998/namespace"
     xmlns:xsd="http://www.w3.org/2001/XMLSchema#"
     xmlns:bibo="http://purl.org/ontology/bibo/"
     xmlns:rdfs="http://www.w3.org/2000/01/rdf-schema#"
     xmlns:skos="http://www.w3.org/2004/02/skos/core#"
     xmlns:vann="http://purl.org/vocab/vann/"
     xmlns:terms="http://purl.org/dc/terms/"
     xmlns:schema="https://schema.org/">
    <owl:Ontology rdf:about="http://w3id.org/nfdi4ing/metadata4ing#">
        <owl:versionIRI rdf:resource="http://w3id.org/nfdi4ing/metadata4ing/1.2.1"/>
        <terms:abstract>The ontology Metadata4Ing is developed within the NFDI Consortium NFDI4Ing with the aim of providing a thorough framework for the semantic description of research data, with a particular focus on engineering sciences and neighbouring disciplines. This ontology allows a thorough description of the whole data generation process (experiment, observation, simulation), embracing the object of investigation, all sample and data manipulation procedures, a summary of the data files and the information contained, and all personal and institutional roles. The subordinate classes and relations can be built according to the two principles of _inheritance_ and _modularity_. _Inheritance_ means that a subclass inherits all properties of its superordinate class, possibly adding some new ones. _Modularity_ means that all expansions are independent of each other; this makes possible for instance to generate expanded ontologies for any possible combinations of method × object of research.</terms:abstract>
        <terms:contributor>Ashish Karmacharya (https://orcid.org/0000-0003-2822-7648), Technische Universität Darmstadt (https://ror.org/05n911h24, https://isni.org/isni/0000000109401669)</terms:contributor>
        <terms:contributor>Benjamin Farnbacher (https://orcid.org/0000-0002-1489-6501), Technische Universität München (TUM) (https://ror.org/02kkvpp62, https://isni.org/isni/0000000123222966)</terms:contributor>
        <terms:contributor>Cord Wiljes (https://orcid.org/0000-0003-2528-5391), Universität Bielefeld (https://ror.org/02hpadn98, https://isni.org/isni/0000000109449128)</terms:contributor>
        <terms:contributor>Dorothea Iglezakis (https://orcid.org/0000-0002-8524-0569), Universität Stuttgart (https://ror.org/04vnq7t77, https://isni.org/isni/0000000419369713)</terms:contributor>
        <terms:contributor>Džulia Terzijska (https://orcid.org/0000-0002-1698-6826), Technische Universität Braunschweig (TUBS) (https://ror.org/010nsgg66, https://isni.org/isni/0000000110900254)</terms:contributor>
        <terms:contributor>Giacomo Lanza (https://orcid.org/0000-0002-2239-3955), Physikalisch-Technische Bundesanstalt (PTB) (https://ror.org/05r3f7h03, https://isni.org/isni/0000000121861887)</terms:contributor>
        <terms:contributor>Johanna Hickmann (https://orcid.org/0000-0002-7535-8344), Physikalisch-Technische Bundesanstalt (PTB) (https://ror.org/05r3f7h03, https://isni.org/isni/0000000121861887)</terms:contributor>
        <terms:contributor>Johannes Munke (https://orcid.org/0000-0002-5031-9170), Leibniz Supercomputing Centre (LRZ) (https://ror.org/05558nw16, https://isni.org/isni/0000000123369749)</terms:contributor>
        <terms:contributor>Johannes Theissen-Lipp (https://orcid.org/0000-0002-2639-1949), RWTH Aachen University (https://ror.org/04xfq0f34, https://isni.org/isni/0000000121811804)</terms:contributor>
        <terms:contributor>Jürgen Windeck (https://orcid.org/0000-0003-1909-4353), Technische Universität Darmstadt (https://ror.org/05n911h24, https://isni.org/isni/0000000109401669)</terms:contributor>
        <terms:contributor>Martin Thomas Horsch (https://orcid.org/0000-0002-9464-6739), Norges miljø- og biovitenskapelige universitet (NMBU) (https://ror.org/04a1mvv97, https://isni.org/isni/000000040607975X)</terms:contributor>
        <terms:contributor>Nils Hoppe (https://orcid.org/0000-0003-0580-9717), Technische Universität München (TUM) (https://ror.org/02kkvpp62, https://isni.org/isni/0000000123222966)</terms:contributor>
        <terms:contributor>Sophia Leimer (https://orcid.org/0000-0001-6272-204X), Universität Duisburg-Essen (https://ror.org/04mz5ra38, https://isni.org/isni/0000000121875445)</terms:contributor>
        <terms:contributor>Stephan Hachinger (https://orcid.org/0000-0001-8341-1478), Leibniz Supercomputing Centre (LRZ) (https://ror.org/05558nw16, https://isni.org/isni/0000000123369749)</terms:contributor>
        <terms:contributor>Susanne Arndt (https://orcid.org/0000-0002-1019-9151), Technische Informationsbibliothek (TIB) (https://ror.org/04aj4c181, https://isni.org/isni/0000000121746694)</terms:contributor>
        <terms:created>2022-02-22</terms:created>
        <terms:creator>Metadata4Ing Workgroup</terms:creator>
        <terms:issued>2022-02-22</terms:issued>
        <terms:license rdf:resource="https://creativecommons.org/licenses/by/4.0/"/>
        <terms:modified>2023-10-20</terms:modified>
        <terms:publisher>NFDI4Ing (https://www.nfdi4ing.de/)</terms:publisher>
        <terms:references rdf:resource="https://doi.org/10.14454/3w3z-sa82"/>
        <terms:references rdf:resource="https://doi.org/10.1504/IJMSO.2020.107792"/>
        <terms:references rdf:resource="https://doi.org/10.5281/zenodo.3816686"/>
        <terms:references rdf:resource="https://doi.org/10.5281/zenodo.3982367"/>
        <terms:references rdf:resource="https://doi.org/10.5281/zenodo.4846313"/>
        <terms:replaces rdf:resource="http://w3id.org/nfdi4ing/metadata4ing/1.2.0"/>
        <terms:rights rdf:resource="https://creativecommons.org/licenses/by/4.0/"/>
        <terms:title xml:lang="en">Metadata4Ing: An ontology for describing the generation of research data within a scientific activity.</terms:title>
        <bibo:doi rdf:resource="https://doi.org/10.5281/zenodo.5957104"/>
        <bibo:status xml:lang="en">active</bibo:status>
        <vann:preferredNamespacePrefix>m4i</vann:preferredNamespacePrefix>
        <vann:preferredNamespaceUri rdf:resource="http://w3id.org/nfdi4ing/metadata4ing#"/>
        <rdfs:comment xml:lang="en">
Metadata4Ing defines classes and properties or reuses such classes and properties from other ontologies to describe research processes and research data management in NFDI4Ing. 
New concepts and properties are located in the namespace of Metadata4Ing.
Metadata4Ing does not import complete ontologies for the sake of relevance, readability, understandability and usability by and for engineers.
Instead, it tries to make re-use of existing identifiers for classes and properties by re-using all or a relevant subset of the axioms from the original ontology.
These statements have been extracted in different ways, e.g. by using Protégé tools importing an ontology and copying axioms of relevant items to Metadata4Ing or by download from data services or raw files of ontologies and manual copypasting.
In some cases there was a need to extend or modify the original set of statements about an entity, e.g. because labels and definitions were expressed with a different owl:AnnotationProperty than the rest of Metadata4Ing, or because a skos:preflabel or a skos:definition in any of the languages we would like to support was missing.
Any editorial changes on elements from external ontologies are declared in Metadata4Ing by an annotation with skos:editorialNote at item-level.
To get the original set of statements we encourage to visit the original namespace of the respective item.
Metadata4Ing reuses elements from the following ontologies:
- BIBO = Bibliographic Ontology  
- BIRO = Bibliographic Reference Ontology  
- DCAT = Data Catalog  
- DCC = Digital Calibration Certificate  
- DCTERMS = Dublin Core Terms  
- EMMO = European Materials and Modelling Ontology  
- FOAF = Friend of a Friend  
- OBO = Open Biological and Biomedical Ontologies:
  - BFO = Basic Formal Ontology  
  - RO = Relation Ontology  
- OWL = Web Ontology Language  
- PIMS-II = PIMS Interoperability Infrastructure  
- PROV = Provenance Namespace  
- QUDT = Quantities, Units, Dimensions and Types  
- RDF = Resource Description Framework  
- RDFS = RDF Schema  
- SCHEMA = schema.org  
- D-SI = Digital System of Units  
- SKOS = Simple Knowledge Organization System  
- SSN = Semantic Sensor Network Ontology  
- VANN = Vocabulary for Annotating vocabulary descriptions  
- XSD = XML Schema Definition  
</rdfs:comment>
        <rdfs:label>Metadata4Ing</rdfs:label>
        <owl:versionInfo>v1.2.1</owl:versionInfo>
        <schema:citation xml:lang="en">Metadata4Ing Workgroup (2022). Metadata4Ing: An ontology for describing the generation of research data within a scientific activity.</schema:citation>
    </owl:Ontology>
    


    <!-- 
    ///////////////////////////////////////////////////////////////////////////////////////
    //
    // Annotation properties
    //
    ///////////////////////////////////////////////////////////////////////////////////////
     -->


    


    <!-- http://purl.org/dc/terms/abstract -->


    <owl:AnnotationProperty rdf:about="http://purl.org/dc/terms/abstract"/>
    


    <!-- http://purl.org/dc/terms/contributor -->


    <owl:AnnotationProperty rdf:about="http://purl.org/dc/terms/contributor"/>
    


    <!-- http://purl.org/dc/terms/created -->


    <owl:AnnotationProperty rdf:about="http://purl.org/dc/terms/created"/>
    


    <!-- http://purl.org/dc/terms/creator -->


    <owl:AnnotationProperty rdf:about="http://purl.org/dc/terms/creator"/>
    


    <!-- http://purl.org/dc/terms/description -->


    <owl:AnnotationProperty rdf:about="http://purl.org/dc/terms/description">
        <skos:definition xml:lang="en">An account of the resource.</skos:definition>
        <skos:editorialNote xml:lang="en">changed by m4i: added skos:prefLabel</skos:editorialNote>
        <skos:prefLabel xml:lang="de">Beschreibung</skos:prefLabel>
        <skos:prefLabel xml:lang="en">description</skos:prefLabel>
    </owl:AnnotationProperty>
    


    <!-- http://purl.org/dc/terms/isReferencedBy -->


    <owl:AnnotationProperty rdf:about="http://purl.org/dc/terms/isReferencedBy">
        <terms:description xml:lang="en">This property is intended to be used with non-literal values. This property is an inverse property of References.</terms:description>
        <rdfs:comment xml:lang="en">A related resource that references, cites, or otherwise points to the described resource.</rdfs:comment>
        <skos:editorialNote xml:lang="en">changed by m4i: added german labels, added skos:prefLabel</skos:editorialNote>
        <skos:prefLabel xml:lang="en">is referenced by</skos:prefLabel>
        <skos:prefLabel xml:lang="de">ist referenziert von</skos:prefLabel>
    </owl:AnnotationProperty>
    


    <!-- http://purl.org/dc/terms/issued -->


    <owl:AnnotationProperty rdf:about="http://purl.org/dc/terms/issued"/>
    


    <!-- http://purl.org/dc/terms/license -->


    <owl:AnnotationProperty rdf:about="http://purl.org/dc/terms/license"/>
    


    <!-- http://purl.org/dc/terms/modified -->


    <owl:AnnotationProperty rdf:about="http://purl.org/dc/terms/modified"/>
    


    <!-- http://purl.org/dc/terms/publisher -->


    <owl:AnnotationProperty rdf:about="http://purl.org/dc/terms/publisher"/>
    


    <!-- http://purl.org/dc/terms/references -->


    <owl:AnnotationProperty rdf:about="http://purl.org/dc/terms/references"/>
    


    <!-- http://purl.org/dc/terms/replaces -->


    <owl:AnnotationProperty rdf:about="http://purl.org/dc/terms/replaces"/>
    


    <!-- http://purl.org/dc/terms/rights -->


    <owl:AnnotationProperty rdf:about="http://purl.org/dc/terms/rights"/>
    


    <!-- http://purl.org/dc/terms/title -->


    <owl:AnnotationProperty rdf:about="http://purl.org/dc/terms/title"/>
    


    <!-- http://purl.org/ontology/bibo/doi -->


    <owl:AnnotationProperty rdf:about="http://purl.org/ontology/bibo/doi"/>
    


    <!-- http://purl.org/ontology/bibo/status -->


    <owl:AnnotationProperty rdf:about="http://purl.org/ontology/bibo/status"/>
    


    <!-- http://purl.org/vocab/vann/preferredNamespacePrefix -->


    <owl:AnnotationProperty rdf:about="http://purl.org/vocab/vann/preferredNamespacePrefix"/>
    


    <!-- http://purl.org/vocab/vann/preferredNamespaceUri -->


    <owl:AnnotationProperty rdf:about="http://purl.org/vocab/vann/preferredNamespaceUri"/>
    


    <!-- http://www.w3.org/2004/02/skos/core#altLabel -->


    <owl:AnnotationProperty rdf:about="http://www.w3.org/2004/02/skos/core#altLabel"/>
    


    <!-- http://www.w3.org/2004/02/skos/core#broader -->


    <owl:AnnotationProperty rdf:about="http://www.w3.org/2004/02/skos/core#broader"/>
    


    <!-- http://www.w3.org/2004/02/skos/core#closeMatch -->


    <owl:AnnotationProperty rdf:about="http://www.w3.org/2004/02/skos/core#closeMatch"/>
    


    <!-- http://www.w3.org/2004/02/skos/core#definition -->


    <owl:AnnotationProperty rdf:about="http://www.w3.org/2004/02/skos/core#definition"/>
    


    <!-- http://www.w3.org/2004/02/skos/core#editorialNote -->


    <owl:AnnotationProperty rdf:about="http://www.w3.org/2004/02/skos/core#editorialNote"/>
    


    <!-- http://www.w3.org/2004/02/skos/core#example -->


    <owl:AnnotationProperty rdf:about="http://www.w3.org/2004/02/skos/core#example"/>
    


    <!-- http://www.w3.org/2004/02/skos/core#narrower -->


    <owl:AnnotationProperty rdf:about="http://www.w3.org/2004/02/skos/core#narrower"/>
    


    <!-- http://www.w3.org/2004/02/skos/core#note -->


    <owl:AnnotationProperty rdf:about="http://www.w3.org/2004/02/skos/core#note"/>
    


    <!-- http://www.w3.org/2004/02/skos/core#prefLabel -->


    <owl:AnnotationProperty rdf:about="http://www.w3.org/2004/02/skos/core#prefLabel"/>
    


    <!-- http://www.w3.org/2004/02/skos/core#scopeNote -->


    <owl:AnnotationProperty rdf:about="http://www.w3.org/2004/02/skos/core#scopeNote"/>
    


    <!-- https://schema.org/affiliation -->


    <owl:AnnotationProperty rdf:about="https://schema.org/affiliation">
        <rdfs:comment xml:lang="en">An organization that this person is affiliated with. For example, a school/university, a club, or a team.</rdfs:comment>
        <rdfs:comment xml:lang="de">Eine Organisation, der eine Person angehört</rdfs:comment>
        <skos:editorialNote xml:lang="en">changed by m4i: added German definition, added language tag to English definition</skos:editorialNote>
        <skos:editorialNote xml:lang="en">changed by m4i: added application example</skos:editorialNote>
        <skos:editorialNote xml:lang="en">changed by m4i: use of skos:prefLabel instead of rdfs:label, added German label, added language tag to English label</skos:editorialNote>
        <skos:example xml:lang="en">:Person schema:affiliation :Organization .</skos:example>
        <skos:prefLabel xml:lang="de">Organisationszugehörigkeit</skos:prefLabel>
        <skos:prefLabel xml:lang="en">affiliation</skos:prefLabel>
    </owl:AnnotationProperty>
    


    <!-- https://schema.org/citation -->


    <owl:AnnotationProperty rdf:about="https://schema.org/citation"/>
    


    <!-- https://schema.org/funder -->


    <owl:AnnotationProperty rdf:about="https://schema.org/funder">
        <rdfs:comment xml:lang="en">A person or organization that supports (sponsors) something through some kind of financial contribution.</rdfs:comment>
        <rdfs:comment xml:lang="de">Eine Person oder Organisation, die etwas finanziell unterstützt</rdfs:comment>
        <skos:editorialNote xml:lang="en">changed by m4i: added German definition, added language tag to English definition</skos:editorialNote>
        <skos:editorialNote xml:lang="en">changed by m4i: added application example</skos:editorialNote>
        <skos:editorialNote xml:lang="en">changed by m4i: use of skos:prefLabel instead of rdfs:label, added German label, added language tag to English label</skos:editorialNote>
        <skos:example xml:lang="en">:Project schema:funder :DFG</skos:example>
        <skos:prefLabel xml:lang="de">Förderer</skos:prefLabel>
        <skos:prefLabel xml:lang="en">funder</skos:prefLabel>
    </owl:AnnotationProperty>
    


    <!-- 
    ///////////////////////////////////////////////////////////////////////////////////////
    //
    // Datatypes
    //
    ///////////////////////////////////////////////////////////////////////////////////////
     -->


    


    <!-- http://www.w3.org/2001/XMLSchema#date -->


    <rdfs:Datatype rdf:about="http://www.w3.org/2001/XMLSchema#date"/>
    


    <!-- http://www.w3.org/2001/XMLSchema#duration -->


    <rdfs:Datatype rdf:about="http://www.w3.org/2001/XMLSchema#duration"/>
    


    <!-- https://ptb.de/dcc/formulaType -->


    <rdfs:Datatype rdf:about="https://ptb.de/dcc/formulaType">
        <skos:definition xml:lang="en">A data type to express formulae in a markup language such as MathML or LaTeX. The preferred syntax is Semantic MathML.</skos:definition>
        <skos:editorialNote xml:lang="en">harmonized spelling to OBO naming conventions (lower case, space separated)</skos:editorialNote>
        <skos:prefLabel xml:lang="de">Formel</skos:prefLabel>
        <skos:prefLabel xml:lang="en">formula</skos:prefLabel>
    </rdfs:Datatype>
    


    <!-- https://schema.org/DateTime -->


    <rdfs:Datatype rdf:about="https://schema.org/DateTime">
        <skos:definition xml:lang="en">A combination of date and time of day in the form [-]CCYY-MM-DDThh:mm:ss[Z|(+|-)hh:mm] (see Chapter 5.4 of ISO 8601)</skos:definition>
        <skos:editorialNote xml:lang="en">changed by m4i: added skos:prefLabel, added german label, harmonized spelling to OBO naming conventions (lower case, space separated)</skos:editorialNote>
        <skos:prefLabel xml:lang="de">Datum mit Zeit</skos:prefLabel>
        <skos:prefLabel xml:lang="en">date with time</skos:prefLabel>
    </rdfs:Datatype>
    


    <!-- 
    ///////////////////////////////////////////////////////////////////////////////////////
    //
    // Object Properties
    //
    ///////////////////////////////////////////////////////////////////////////////////////
     -->


    


    <!-- http://purl.obolibrary.org/obo/BFO_0000050 -->


    <owl:ObjectProperty rdf:about="http://purl.obolibrary.org/obo/BFO_0000050">
        <owl:inverseOf rdf:resource="http://purl.obolibrary.org/obo/BFO_0000051"/>
        <rdf:type rdf:resource="http://www.w3.org/2002/07/owl#TransitiveProperty"/>
        <skos:definition xml:lang="en">a core relation that holds between a part and its whole</skos:definition>
        <skos:editorialNote xml:lang="en">changed by m4i: added german labels, added skos:prefLabel</skos:editorialNote>
        <skos:editorialNote xml:lang="en">changed by m4i: copied obo:IAO_0000115 to a skos:definition</skos:editorialNote>
        <skos:prefLabel xml:lang="de">Teil von</skos:prefLabel>
        <skos:prefLabel xml:lang="en">part of</skos:prefLabel>
    </owl:ObjectProperty>
    


    <!-- http://purl.obolibrary.org/obo/BFO_0000051 -->


    <owl:ObjectProperty rdf:about="http://purl.obolibrary.org/obo/BFO_0000051">
        <rdf:type rdf:resource="http://www.w3.org/2002/07/owl#TransitiveProperty"/>
        <skos:definition xml:lang="en">a core relation that holds between a whole and its part</skos:definition>
        <skos:editorialNote xml:lang="en">changed by m4i: added german labels, added skos:prefLabel</skos:editorialNote>
        <skos:editorialNote xml:lang="en">changed by m4i: copied obo:IAO_0000115 to a skos:definition</skos:editorialNote>
        <skos:prefLabel xml:lang="en">has part</skos:prefLabel>
        <skos:prefLabel xml:lang="de">hat Teil</skos:prefLabel>
    </owl:ObjectProperty>
    


    <!-- http://purl.obolibrary.org/obo/BFO_0000054 -->


    <owl:ObjectProperty rdf:about="http://purl.obolibrary.org/obo/BFO_0000054">
        <owl:inverseOf rdf:resource="http://purl.obolibrary.org/obo/BFO_0000055"/>
        <rdfs:domain rdf:resource="http://purl.obolibrary.org/obo/BFO_0000017"/>
        <rdfs:range rdf:resource="http://purl.obolibrary.org/obo/BFO_0000015"/>
        <rdfs:comment>Paraphrase of elucidation: a relation between a realizable entity and a process, where there is some material entity that is bearer of the realizable entity and participates in the process, and the realizable entity comes to be realized in the course of the process</rdfs:comment>
        <rdfs:isDefinedBy rdf:resource="http://purl.obolibrary.org/obo/"/>
        <skos:editorialNote xml:lang="en">changed by m4i: added german labels, added skos:prefLabel</skos:editorialNote>
        <skos:prefLabel xml:lang="de">realisiert in</skos:prefLabel>
        <skos:prefLabel xml:lang="en">realized in</skos:prefLabel>
    </owl:ObjectProperty>
    


    <!-- http://purl.obolibrary.org/obo/BFO_0000055 -->


    <owl:ObjectProperty rdf:about="http://purl.obolibrary.org/obo/BFO_0000055">
        <rdfs:domain rdf:resource="http://purl.obolibrary.org/obo/BFO_0000015"/>
        <rdfs:range rdf:resource="http://purl.obolibrary.org/obo/BFO_0000017"/>
        <rdfs:comment>Paraphrase of elucidation: a relation between a process and a realizable entity, where there is some material entity that is bearer of the realizable entity and participates in the process, and the realizable entity comes to be realized in the course of the process</rdfs:comment>
        <rdfs:isDefinedBy rdf:resource="http://purl.obolibrary.org/obo/"/>
        <skos:editorialNote xml:lang="en">changed by m4i: added german labels, added skos:prefLabel</skos:editorialNote>
        <skos:prefLabel xml:lang="de">realisiert</skos:prefLabel>
        <skos:prefLabel xml:lang="en">realizes</skos:prefLabel>
    </owl:ObjectProperty>
    


    <!-- http://purl.obolibrary.org/obo/BFO_0000063 -->


    <owl:ObjectProperty rdf:about="http://purl.obolibrary.org/obo/BFO_0000063">
        <rdf:type rdf:resource="http://www.w3.org/2002/07/owl#TransitiveProperty"/>
        <rdfs:domain rdf:resource="http://purl.obolibrary.org/obo/BFO_0000015"/>
        <rdfs:range rdf:resource="http://purl.obolibrary.org/obo/BFO_0000015"/>
        <skos:definition xml:lang="en">x precedes y if and only if the time point at which x ends is before or equivalent to the time point at which y starts. Formally: x precedes y iff ω(x) &lt;= α(y), where α is a function that maps a process to a start point, and ω is a function that maps a process to an end point.</skos:definition>
        <skos:prefLabel xml:lang="de">ist Voraussetzung für Schritt</skos:prefLabel>
        <skos:prefLabel xml:lang="en">precedes</skos:prefLabel>
    </owl:ObjectProperty>
    


    <!-- http://purl.obolibrary.org/obo/RO_0000056 -->


    <owl:ObjectProperty rdf:about="http://purl.obolibrary.org/obo/RO_0000056">
        <owl:inverseOf rdf:resource="http://purl.obolibrary.org/obo/RO_0000057"/>
        <skos:definition xml:lang="en">a relation between a continuant and a process, in which the continuant is somehow involved in the process</skos:definition>
        <skos:editorialNote xml:lang="en">changed by m4i: added german labels, added skos:prefLabel</skos:editorialNote>
        <skos:editorialNote xml:lang="en">changed by m4i: copied obo:IAO_0000115 to a skos:definition</skos:editorialNote>
        <skos:prefLabel xml:lang="de">ist beteiligt an</skos:prefLabel>
        <skos:prefLabel xml:lang="en">participates in</skos:prefLabel>
    </owl:ObjectProperty>
    


    <!-- http://purl.obolibrary.org/obo/RO_0000057 -->


    <owl:ObjectProperty rdf:about="http://purl.obolibrary.org/obo/RO_0000057">
        <owl:propertyChainAxiom rdf:parseType="Collection">
            <rdf:Description rdf:about="http://www.w3.org/ns/prov#qualifiedAssociation"/>
            <rdf:Description rdf:about="http://www.w3.org/ns/prov#agent"/>
        </owl:propertyChainAxiom>
        <skos:definition xml:lang="en">a relation between a process and a continuant, in which the continuant is somehow involved in the process</skos:definition>
        <skos:editorialNote xml:lang="en">changed by m4i: added a property chain axiom for use with prov:qualifiedAssociation</skos:editorialNote>
        <skos:editorialNote xml:lang="en">changed by m4i: added german labels, added skos:prefLabel</skos:editorialNote>
        <skos:editorialNote xml:lang="en">changed by m4i: copied obo:IAO_0000115 to a skos:definition</skos:editorialNote>
        <skos:prefLabel xml:lang="en">has participant</skos:prefLabel>
        <skos:prefLabel xml:lang="de">hat Teilnehmer</skos:prefLabel>
    </owl:ObjectProperty>
    


    <!-- http://purl.obolibrary.org/obo/RO_0002090 -->


    <owl:ObjectProperty rdf:about="http://purl.obolibrary.org/obo/RO_0002090">
        <rdfs:subPropertyOf rdf:resource="http://purl.obolibrary.org/obo/BFO_0000063"/>
        <rdfs:domain rdf:resource="http://purl.obolibrary.org/obo/BFO_0000015"/>
        <rdfs:range rdf:resource="http://purl.obolibrary.org/obo/BFO_0000015"/>
        <skos:definition>X immediately precedes_Y iff: end(X) simultaneous_with start(Y)</skos:definition>
        <skos:editorialNote xml:lang="en">changed by m4i: added skos:prefLabel</skos:editorialNote>
        <skos:prefLabel xml:lang="en">immediately precedes</skos:prefLabel>
        <skos:prefLabel xml:lang="de">ist unmittelbare Voraussetzung für Schritt</skos:prefLabel>
    </owl:ObjectProperty>
    


    <!-- http://purl.obolibrary.org/obo/RO_0002224 -->


    <owl:ObjectProperty rdf:about="http://purl.obolibrary.org/obo/RO_0002224">
        <rdfs:subPropertyOf rdf:resource="http://purl.obolibrary.org/obo/BFO_0000051"/>
        <rdf:type rdf:resource="http://www.w3.org/2002/07/owl#TransitiveProperty"/>
        <rdfs:domain rdf:resource="http://w3id.org/nfdi4ing/metadata4ing#ProcessingStep"/>
        <rdfs:range rdf:resource="http://w3id.org/nfdi4ing/metadata4ing#ProcessingStep"/>
        <rdfs:seeAlso rdf:resource="http://ontologydesignpatterns.org/wiki/Submissions:Componency"/>
        <skos:altLabel xml:lang="en">started by</skos:altLabel>
        <skos:definition xml:lang="en">x starts with y if and only if x has part y and the time point at which x starts is equivalent to the time point at which y starts. Formally: α(y) = α(x) ∧ ω(y) &lt; ω(x), where α is a function that maps a process to a start point, and ω is a function that maps a process to an end point.</skos:definition>
        <skos:editorialNote xml:lang="en">changed by m4i: added german labels, added skos:prefLabel</skos:editorialNote>
        <skos:prefLabel xml:lang="de">beginnt mit</skos:prefLabel>
        <skos:prefLabel xml:lang="en">starts with</skos:prefLabel>
    </owl:ObjectProperty>
    


    <!-- http://purl.obolibrary.org/obo/RO_0002230 -->


    <owl:ObjectProperty rdf:about="http://purl.obolibrary.org/obo/RO_0002230">
        <rdfs:subPropertyOf rdf:resource="http://purl.obolibrary.org/obo/BFO_0000051"/>
        <rdf:type rdf:resource="http://www.w3.org/2002/07/owl#TransitiveProperty"/>
        <rdfs:domain rdf:resource="http://w3id.org/nfdi4ing/metadata4ing#ProcessingStep"/>
        <rdfs:range rdf:resource="http://w3id.org/nfdi4ing/metadata4ing#ProcessingStep"/>
        <skos:altLabel xml:lang="en">finished by</skos:altLabel>
        <skos:definition xml:lang="en">x ends with y if and only if x has part y and the time point at which x ends is equivalent to the time point at which y ends. Formally: α(y) &gt; α(x) ∧ ω(y) = ω(x), where α is a function that maps a process to a start point, and ω is a function that maps a process to an end point.</skos:definition>
        <skos:editorialNote xml:lang="en">changed by m4i: added german labels, added skos:prefLabel</skos:editorialNote>
        <skos:prefLabel xml:lang="de">endet mit</skos:prefLabel>
        <skos:prefLabel xml:lang="en">ends with</skos:prefLabel>
    </owl:ObjectProperty>
    


    <!-- http://purl.obolibrary.org/obo/RO_0002233 -->


    <owl:ObjectProperty rdf:about="http://purl.obolibrary.org/obo/RO_0002233">
        <rdfs:subPropertyOf rdf:resource="http://purl.obolibrary.org/obo/RO_0000057"/>
        <owl:inverseOf rdf:resource="http://purl.obolibrary.org/obo/RO_0002352"/>
        <skos:definition xml:lang="en">(x has input y) means x takes specific input as y for further processes</skos:definition>
        <skos:editorialNote xml:lang="en">changed by m4i: added skos:prefLabel</skos:editorialNote>
        <skos:prefLabel xml:lang="en">has input</skos:prefLabel>
        <skos:prefLabel xml:lang="de">hat Input</skos:prefLabel>
    </owl:ObjectProperty>
    


    <!-- http://purl.obolibrary.org/obo/RO_0002234 -->


    <owl:ObjectProperty rdf:about="http://purl.obolibrary.org/obo/RO_0002234">
        <rdfs:subPropertyOf rdf:resource="http://purl.obolibrary.org/obo/RO_0000057"/>
        <owl:inverseOf rdf:resource="http://purl.obolibrary.org/obo/RO_0002353"/>
        <skos:definition xml:lang="en">(x has output y) means x provides specific output y for the result or further processes</skos:definition>
        <skos:editorialNote xml:lang="en">changed by m4i: added skos:prefLabel</skos:editorialNote>
        <skos:prefLabel xml:lang="en">has output</skos:prefLabel>
        <skos:prefLabel xml:lang="de">hat Output</skos:prefLabel>
    </owl:ObjectProperty>
    


    <!-- http://purl.obolibrary.org/obo/RO_0002352 -->


    <owl:ObjectProperty rdf:about="http://purl.obolibrary.org/obo/RO_0002352">
        <rdfs:subPropertyOf rdf:resource="http://purl.obolibrary.org/obo/RO_0000056"/>
        <skos:definition xml:lang="en">(x input of y) means x is a specific input of y to carry out further processes</skos:definition>
        <skos:editorialNote xml:lang="en">changed by m4i: added skos:prefLabel</skos:editorialNote>
        <skos:prefLabel xml:lang="de">Input von</skos:prefLabel>
        <skos:prefLabel xml:lang="en">input of</skos:prefLabel>
    </owl:ObjectProperty>
    


    <!-- http://purl.obolibrary.org/obo/RO_0002353 -->


    <owl:ObjectProperty rdf:about="http://purl.obolibrary.org/obo/RO_0002353">
        <rdfs:subPropertyOf rdf:resource="http://purl.obolibrary.org/obo/RO_0000056"/>
        <skos:definition xml:lang="en">(x output of y) means x is the specific output of y as the result or further processes</skos:definition>
        <skos:editorialNote xml:lang="en">changed by m4i: added skos:prefLabel</skos:editorialNote>
        <skos:prefLabel xml:lang="de">Output von</skos:prefLabel>
        <skos:prefLabel xml:lang="en">output of</skos:prefLabel>
    </owl:ObjectProperty>
    


    <!-- http://w3id.org/nfdi4ing/metadata4ing#hasAdmissibleUnit -->


    <owl:ObjectProperty rdf:about="http://w3id.org/nfdi4ing/metadata4ing#hasAdmissibleUnit">
        <owl:inverseOf rdf:resource="http://www.molmod.info/semantics/pims-ii.ttl#isAdmissibleUnitFor"/>
        <rdfs:domain>
            <owl:Class>
                <owl:unionOf rdf:parseType="Collection">
                    <rdf:Description rdf:about="http://qudt.org/schema/qudt/QuantityKind"/>
                    <rdf:Description rdf:about="http://w3id.org/nfdi4ing/metadata4ing#NumericalVariable"/>
                </owl:unionOf>
            </owl:Class>
        </rdfs:domain>
        <rdfs:range rdf:resource="http://qudt.org/schema/qudt/Unit"/>
        <rdfs:comment>redundant information: applicable unit can be deduced from quantity kind. If one wants to enforce the use of a specific unit, use a SHACL constraint.</rdfs:comment>
        <owl:deprecated rdf:datatype="http://www.w3.org/2001/XMLSchema#boolean">true</owl:deprecated>
        <skos:definition xml:lang="en">DEPRECATED (x hasAdmissibleUnit y) means that y is a unit that can be associated with the variable x</skos:definition>
        <skos:prefLabel xml:lang="en">has admissible unit</skos:prefLabel>
        <skos:prefLabel xml:lang="de">hat als zulässige Einheit</skos:prefLabel>
    </owl:ObjectProperty>
    


    <!-- http://w3id.org/nfdi4ing/metadata4ing#hasAdmissibleValue -->


    <owl:ObjectProperty rdf:about="http://w3id.org/nfdi4ing/metadata4ing#hasAdmissibleValue">
        <owl:inverseOf rdf:resource="http://www.molmod.info/semantics/pims-ii.ttl#isAdmissibleValueFor"/>
        <rdfs:domain rdf:resource="http://www.molmod.info/semantics/pims-ii.ttl#Variable"/>
        <rdfs:range rdf:resource="http://www.molmod.info/semantics/pims-ii.ttl#Value"/>
        <skos:definition xml:lang="en">(x hasAdmissibleValue y) means that y is a value that can be assigned to the variable x</skos:definition>
        <skos:prefLabel xml:lang="en">has admissible value</skos:prefLabel>
        <skos:prefLabel xml:lang="de">hat als zulässigen Wert</skos:prefLabel>
    </owl:ObjectProperty>
    


    <!-- http://w3id.org/nfdi4ing/metadata4ing#hasAssignedValue -->


    <owl:ObjectProperty rdf:about="http://w3id.org/nfdi4ing/metadata4ing#hasAssignedValue">
        <owl:inverseOf rdf:resource="http://www.molmod.info/semantics/pims-ii.ttl#isValueInAssignment"/>
        <rdfs:domain rdf:resource="http://www.molmod.info/semantics/pims-ii.ttl#Assignment"/>
        <rdfs:range rdf:resource="http://www.molmod.info/semantics/pims-ii.ttl#Value"/>
        <skos:definition xml:lang="en">(a hasAssignedValue y) means that a: x = y is an assignment where the value y is assigned to a variable x</skos:definition>
        <skos:prefLabel xml:lang="en">has assigned value</skos:prefLabel>
        <skos:prefLabel xml:lang="de">hat zugewiesenen Wert</skos:prefLabel>
    </owl:ObjectProperty>
    


    <!-- http://w3id.org/nfdi4ing/metadata4ing#hasCoverageInterval -->


    <owl:ObjectProperty rdf:about="http://w3id.org/nfdi4ing/metadata4ing#hasCoverageInterval">
        <rdfs:subPropertyOf rdf:resource="http://w3id.org/nfdi4ing/metadata4ing#hasUncertaintyDeclaration"/>
        <rdfs:domain rdf:resource="https://ptb.de/si/Real"/>
        <rdfs:range rdf:resource="https://ptb.de/si/CoverageInterval"/>
        <skos:definition xml:lang="en">Associates an si:Real quantity value with an si:CoverageInterval</skos:definition>
        <skos:prefLabel xml:lang="en">has coverage interval</skos:prefLabel>
        <skos:prefLabel xml:lang="de">hat Überdeckungsintervall</skos:prefLabel>
    </owl:ObjectProperty>
    


    <!-- http://w3id.org/nfdi4ing/metadata4ing#hasEmployedTool -->


    <owl:ObjectProperty rdf:about="http://w3id.org/nfdi4ing/metadata4ing#hasEmployedTool">
        <rdfs:subPropertyOf rdf:resource="https://schema.org/instrument"/>
        <owl:inverseOf rdf:resource="http://w3id.org/nfdi4ing/metadata4ing#isEmployedToolIn"/>
        <rdfs:domain rdf:resource="http://w3id.org/nfdi4ing/metadata4ing#ProcessingStep"/>
        <rdfs:range rdf:resource="http://w3id.org/nfdi4ing/metadata4ing#Tool"/>
        <skos:definition xml:lang="en">Points to a tool that is used within a given processing step</skos:definition>
        <skos:definition xml:lang="de">verweist auf ein Werkzeug, das in einem Arbeitsschritt verwendet wurde</skos:definition>
        <skos:prefLabel xml:lang="en">has employed tool</skos:prefLabel>
        <skos:prefLabel xml:lang="de">hat eingesetztes Werkzeug</skos:prefLabel>
    </owl:ObjectProperty>
    


    <!-- http://w3id.org/nfdi4ing/metadata4ing#hasExpandedUnc -->


    <owl:ObjectProperty rdf:about="http://w3id.org/nfdi4ing/metadata4ing#hasExpandedUnc">
        <rdfs:subPropertyOf rdf:resource="http://w3id.org/nfdi4ing/metadata4ing#hasUncertaintyDeclaration"/>
        <rdfs:domain rdf:resource="https://ptb.de/si/Real"/>
        <rdfs:range rdf:resource="https://ptb.de/si/ExpandedUnc"/>
        <skos:definition xml:lang="en">Relates an si:Real to its expanded uncertainty</skos:definition>
        <skos:prefLabel xml:lang="en">has expanded uncertainty</skos:prefLabel>
        <skos:prefLabel xml:lang="de">hat erweiterte Unsicherheit</skos:prefLabel>
    </owl:ObjectProperty>
    


    <!-- http://w3id.org/nfdi4ing/metadata4ing#hasKindOfQuantity -->


    <owl:ObjectProperty rdf:about="http://w3id.org/nfdi4ing/metadata4ing#hasKindOfQuantity">
        <rdfs:domain rdf:resource="http://w3id.org/nfdi4ing/metadata4ing#NumericalVariable"/>
        <rdfs:range rdf:resource="http://qudt.org/schema/qudt/QuantityKind"/>
        <skos:definition xml:lang="en">Points to the property characterization (i.e., to the kind of quantity) from a controlled vocabulary</skos:definition>
        <skos:note xml:lang="en">we recommend using a persistent identifier resolving to a persistent URL</skos:note>
        <skos:prefLabel xml:lang="en">has kind of quantity</skos:prefLabel>
        <skos:prefLabel xml:lang="de">hat Größenart</skos:prefLabel>
    </owl:ObjectProperty>
    


    <!-- http://w3id.org/nfdi4ing/metadata4ing#hasParameter -->


    <owl:ObjectProperty rdf:about="http://w3id.org/nfdi4ing/metadata4ing#hasParameter">
        <rdfs:domain>
            <owl:Class>
                <owl:unionOf rdf:parseType="Collection">
                    <rdf:Description rdf:about="http://w3id.org/nfdi4ing/metadata4ing#Method"/>
                    <rdf:Description rdf:about="http://w3id.org/nfdi4ing/metadata4ing#Tool"/>
                </owl:unionOf>
            </owl:Class>
        </rdfs:domain>
        <rdfs:range rdf:resource="http://www.molmod.info/semantics/pims-ii.ttl#Variable"/>
        <skos:definition xml:lang="en">Points to a parameter of a given method or tool.</skos:definition>
        <skos:prefLabel xml:lang="en">has parameter</skos:prefLabel>
        <skos:prefLabel xml:lang="de">hat Parameter</skos:prefLabel>
    </owl:ObjectProperty>
    


    <!-- http://w3id.org/nfdi4ing/metadata4ing#hasRuntimeAssignment -->


    <owl:ObjectProperty rdf:about="http://w3id.org/nfdi4ing/metadata4ing#hasRuntimeAssignment">
        <rdfs:subPropertyOf rdf:resource="http://purl.obolibrary.org/obo/RO_0000057"/>
        <rdfs:subPropertyOf>
            <rdf:Description>
                <owl:inverseOf rdf:resource="http://www.molmod.info/semantics/pims-ii.ttl#isAssignmentFor"/>
            </rdf:Description>
        </rdfs:subPropertyOf>
        <rdfs:domain rdf:resource="http://w3id.org/nfdi4ing/metadata4ing#ProcessingStep"/>
        <rdfs:range rdf:resource="http://www.molmod.info/semantics/pims-ii.ttl#Assignment"/>
        <skos:definition xml:lang="en">Points to an assignment that is neither input nor output</skos:definition>
        <skos:prefLabel xml:lang="en">has runtime assignment</skos:prefLabel>
        <skos:prefLabel xml:lang="de">hat Laufzeitzuweisung</skos:prefLabel>
    </owl:ObjectProperty>
    


    <!-- http://w3id.org/nfdi4ing/metadata4ing#hasUncertaintyDeclaration -->


    <owl:ObjectProperty rdf:about="http://w3id.org/nfdi4ing/metadata4ing#hasUncertaintyDeclaration">
        <rdfs:domain rdf:resource="https://ptb.de/si/Real"/>
        <rdfs:range rdf:resource="http://w3id.org/nfdi4ing/metadata4ing#UncertaintyDeclaration"/>
        <skos:definition xml:lang="en">Associates an si:Real quantity value with its mandatory uncertainty declaration (i.e., with an expanded uncertainty or a coverage interval)</skos:definition>
        <skos:prefLabel xml:lang="en">has uncertainty declaration</skos:prefLabel>
        <skos:prefLabel xml:lang="de">hat Unsicherheitsdeklaration</skos:prefLabel>
    </owl:ObjectProperty>
    


    <!-- http://w3id.org/nfdi4ing/metadata4ing#hasUnit -->


    <owl:ObjectProperty rdf:about="http://w3id.org/nfdi4ing/metadata4ing#hasUnit">
        <rdfs:domain rdf:resource="https://ptb.de/si/Real"/>
        <rdfs:range rdf:resource="http://qudt.org/schema/qudt/Unit"/>
        <skos:closeMatch rdf:resource="http://qudt.org/schema/qudt/unit"/>
        <skos:closeMatch rdf:resource="https://ptb.de/si/hasUnit"/>
        <skos:definition xml:lang="en">Represents the unit of a numerical (real) value</skos:definition>
        <skos:definition xml:lang="de">Repräsentiert die Einheit eines numerischen (reelen) Wertes</skos:definition>
        <skos:note xml:lang="de">Kardinalität dieser Property bei der Beschreibung eines si:Real: 0-1</skos:note>
        <skos:note xml:lang="de">Obligation dieser Property bei der Beschreibung eines si:Real: recommended</skos:note>
        <skos:note xml:lang="en">We recommend using a resolvable PID from a controlled vocabulary, such as ISO 80000, IEC or QUDT</skos:note>
        <skos:note xml:lang="en">cardinality of this property for the description of a si:Real: 0-1</skos:note>
        <skos:note xml:lang="en">obligation of this property for the description of a si:Real: recommended</skos:note>
        <skos:prefLabel xml:lang="en">has unit</skos:prefLabel>
        <skos:prefLabel xml:lang="de">hat Einheit</skos:prefLabel>
    </owl:ObjectProperty>
    


    <!-- http://w3id.org/nfdi4ing/metadata4ing#hasVariable -->


    <owl:ObjectProperty rdf:about="http://w3id.org/nfdi4ing/metadata4ing#hasVariable">
        <owl:inverseOf rdf:resource="http://www.molmod.info/semantics/pims-ii.ttl#isVariableInAssignment"/>
        <rdfs:domain rdf:resource="http://www.molmod.info/semantics/pims-ii.ttl#Assignment"/>
        <rdfs:range rdf:resource="http://www.molmod.info/semantics/pims-ii.ttl#Variable"/>
        <skos:definition xml:lang="de">( a hasVariable x ) bedeutet, dass a: x = y eine Variablenzuordnung ist, in der der Variablen x ein Wert zugeordnet wird.</skos:definition>
        <skos:definition xml:lang="en">( a hasVariable x ) means that a: x = y is an assignment where the value y is assigned to a variable x</skos:definition>
        <skos:prefLabel xml:lang="en">has variable</skos:prefLabel>
        <skos:prefLabel xml:lang="de">hat Variable</skos:prefLabel>
    </owl:ObjectProperty>
    


    <!-- http://w3id.org/nfdi4ing/metadata4ing#implementedByTool -->


    <owl:ObjectProperty rdf:about="http://w3id.org/nfdi4ing/metadata4ing#implementedByTool">
        <rdfs:subPropertyOf rdf:resource="http://www.w3.org/ns/ssn/implementedBy"/>
        <owl:inverseOf rdf:resource="http://w3id.org/nfdi4ing/metadata4ing#implementsMethod"/>
        <rdfs:domain rdf:resource="http://w3id.org/nfdi4ing/metadata4ing#Method"/>
        <rdfs:range rdf:resource="http://w3id.org/nfdi4ing/metadata4ing#Tool"/>
        <skos:definition xml:lang="en">Points to a tool that implements a given method</skos:definition>
        <skos:prefLabel xml:lang="en">implemented by</skos:prefLabel>
        <skos:prefLabel xml:lang="de">wird implementiert durch</skos:prefLabel>
    </owl:ObjectProperty>
    


    <!-- http://w3id.org/nfdi4ing/metadata4ing#implementsMethod -->


    <owl:ObjectProperty rdf:about="http://w3id.org/nfdi4ing/metadata4ing#implementsMethod">
        <rdfs:subPropertyOf rdf:resource="http://www.w3.org/ns/ssn/implements"/>
        <rdfs:domain rdf:resource="http://w3id.org/nfdi4ing/metadata4ing#Tool"/>
        <rdfs:range rdf:resource="http://w3id.org/nfdi4ing/metadata4ing#Method"/>
        <skos:definition xml:lang="en">Points to a method that is implemented by a given tool</skos:definition>
        <skos:prefLabel xml:lang="de">implementiert</skos:prefLabel>
        <skos:prefLabel xml:lang="en">implements</skos:prefLabel>
    </owl:ObjectProperty>
    


    <!-- http://w3id.org/nfdi4ing/metadata4ing#inProject -->


    <owl:ObjectProperty rdf:about="http://w3id.org/nfdi4ing/metadata4ing#inProject">
        <owl:inverseOf rdf:resource="http://w3id.org/nfdi4ing/metadata4ing#projectParticipant"/>
        <rdfs:domain>
            <owl:Class>
                <owl:unionOf rdf:parseType="Collection">
                    <rdf:Description rdf:about="http://www.w3.org/ns/prov#Organization"/>
                    <rdf:Description rdf:about="http://www.w3.org/ns/prov#Person"/>
                </owl:unionOf>
            </owl:Class>
        </rdfs:domain>
        <rdfs:range rdf:resource="https://schema.org/Project"/>
        <skos:definition xml:lang="en">A property that connects a person or an organization with a project.</skos:definition>
        <skos:prefLabel xml:lang="en">associated to project</skos:prefLabel>
        <skos:prefLabel xml:lang="de">gehört zu Projekt</skos:prefLabel>
    </owl:ObjectProperty>
    


    <!-- http://w3id.org/nfdi4ing/metadata4ing#investigates -->


    <owl:ObjectProperty rdf:about="http://w3id.org/nfdi4ing/metadata4ing#investigates">
        <rdfs:domain rdf:resource="http://w3id.org/nfdi4ing/metadata4ing#ProcessingStep"/>
        <rdfs:range rdf:resource="http://www.w3.org/2002/07/owl#Thing"/>
        <skos:definition xml:lang="en">(x investigates y) means that x is about y, in the context of scientific research and development</skos:definition>
        <skos:prefLabel xml:lang="en">investigates</skos:prefLabel>
        <skos:prefLabel xml:lang="de">untersucht</skos:prefLabel>
    </owl:ObjectProperty>
    


    <!-- http://w3id.org/nfdi4ing/metadata4ing#investigatesProperty -->


    <owl:ObjectProperty rdf:about="http://w3id.org/nfdi4ing/metadata4ing#investigatesProperty">
        <rdfs:subPropertyOf rdf:resource="http://w3id.org/nfdi4ing/metadata4ing#investigates"/>
        <rdfs:range rdf:resource="http://www.molmod.info/semantics/pims-ii.ttl#Property"/>
        <skos:broader rdf:resource="http://emmo.info/emmo#EMMO_60577dea_9019_4537_ac41_80b0fb563d41"/>
        <skos:broader rdf:resource="http://www.molmod.info/semantics/pims-ii.ttl#hasRepresentamen"/>
        <skos:definition xml:lang="en">(x investigatesProperty y) means that x is about target property y, in the context of scientific research and development</skos:definition>
        <skos:prefLabel xml:lang="en">investigates property</skos:prefLabel>
        <skos:prefLabel xml:lang="de">untersucht Eigenschaft</skos:prefLabel>
    </owl:ObjectProperty>
    


    <!-- http://w3id.org/nfdi4ing/metadata4ing#isEmployedToolIn -->


    <owl:ObjectProperty rdf:about="http://w3id.org/nfdi4ing/metadata4ing#isEmployedToolIn">
        <rdfs:domain rdf:resource="http://w3id.org/nfdi4ing/metadata4ing#Tool"/>
        <rdfs:range rdf:resource="http://w3id.org/nfdi4ing/metadata4ing#ProcessingStep"/>
        <skos:definition xml:lang="en">Points to a processing step the tool has been used in</skos:definition>
        <skos:definition xml:lang="de">verweist auf einen Arbeitsschritt, in dem das Werkzeug eingesetzt wurde</skos:definition>
        <skos:prefLabel xml:lang="en">is employed tool</skos:prefLabel>
        <skos:prefLabel xml:lang="de">ist eingesetztes Werkzeug</skos:prefLabel>
    </owl:ObjectProperty>
    


    <!-- http://w3id.org/nfdi4ing/metadata4ing#projectParticipant -->


    <owl:ObjectProperty rdf:about="http://w3id.org/nfdi4ing/metadata4ing#projectParticipant">
        <rdfs:domain rdf:resource="https://schema.org/Project"/>
        <rdfs:range>
            <owl:Class>
                <owl:unionOf rdf:parseType="Collection">
                    <rdf:Description rdf:about="http://www.w3.org/ns/prov#Organization"/>
                    <rdf:Description rdf:about="http://www.w3.org/ns/prov#Person"/>
                </owl:unionOf>
            </owl:Class>
        </rdfs:range>
        <skos:definition xml:lang="en">A property that connects a project with a person or an organisation.</skos:definition>
        <skos:prefLabel xml:lang="de">hat Projektmitglied</skos:prefLabel>
        <skos:prefLabel xml:lang="en">project participant</skos:prefLabel>
    </owl:ObjectProperty>
    


    <!-- http://w3id.org/nfdi4ing/metadata4ing#realizesMethod -->


    <owl:ObjectProperty rdf:about="http://w3id.org/nfdi4ing/metadata4ing#realizesMethod">
        <rdfs:subPropertyOf rdf:resource="http://purl.obolibrary.org/obo/BFO_0000055"/>
        <rdfs:domain rdf:resource="http://w3id.org/nfdi4ing/metadata4ing#ProcessingStep"/>
        <rdfs:range rdf:resource="http://w3id.org/nfdi4ing/metadata4ing#Method"/>
        <skos:definition xml:lang="en">Points to a method that is used within a given processing step</skos:definition>
        <skos:prefLabel xml:lang="de">realisiert Methode</skos:prefLabel>
        <skos:prefLabel xml:lang="en">realizes method</skos:prefLabel>
    </owl:ObjectProperty>
    


    <!-- http://www.molmod.info/semantics/pims-ii.ttl#isAdmissibleUnitFor -->


    <owl:ObjectProperty rdf:about="http://www.molmod.info/semantics/pims-ii.ttl#isAdmissibleUnitFor">
        <rdfs:domain rdf:resource="http://qudt.org/schema/qudt/Unit"/>
        <rdfs:range>
            <owl:Class>
                <owl:unionOf rdf:parseType="Collection">
                    <rdf:Description rdf:about="http://qudt.org/schema/qudt/QuantityKind"/>
                    <rdf:Description rdf:about="http://w3id.org/nfdi4ing/metadata4ing#NumericalVariable"/>
                </owl:unionOf>
            </owl:Class>
        </rdfs:range>
        <rdfs:comment>redundant information: admissible unit can be deduced from quantity kind. If one wants to enforce the use of a specific unit, use a SHACL contraint.</rdfs:comment>
        <owl:deprecated rdf:datatype="http://www.w3.org/2001/XMLSchema#boolean">true</owl:deprecated>
        <skos:definition xml:lang="en">DEPRECATED (x isAdmissibleUnitFor y) means that x is a unit that can be associated with the variable y; subsumption under msHPIPIR is explained as follows: There is a sign z for the variable y (where z is a description of admissible values of y) of which x is constitutive (and with which x hence overlaps)</skos:definition>
        <skos:editorialNote>changed by m4i: added skos:prefLabel, adjusted german labels, harmonized spelling to OBO naming conventions (lower case, space separated)</skos:editorialNote>
        <skos:prefLabel xml:lang="en">is admissible unit for</skos:prefLabel>
        <skos:prefLabel xml:lang="de">ist zulässige Einheit für</skos:prefLabel>
    </owl:ObjectProperty>
    


    <!-- http://www.molmod.info/semantics/pims-ii.ttl#isAdmissibleValueFor -->


    <owl:ObjectProperty rdf:about="http://www.molmod.info/semantics/pims-ii.ttl#isAdmissibleValueFor">
        <rdfs:domain rdf:resource="http://www.molmod.info/semantics/pims-ii.ttl#Value"/>
        <rdfs:range rdf:resource="http://www.molmod.info/semantics/pims-ii.ttl#Variable"/>
        <skos:definition xml:lang="en">(x isAdmissibleValueFor y) means that x is a value that can be assigned to the variable y; subsumption under msIPIRIR is explained as follows: There is a sign z for the variable y (where z is the range of admissible values of y), for which in turn there is another sign z&apos; (where z&apos; lists members of z, explicitly including x) of which x is a part</skos:definition>
        <skos:editorialNote>changed by m4i: added skos:prefLabel, adjusted german labels, harmonized spelling to OBO naming conventions (lower case, space separated)</skos:editorialNote>
        <skos:prefLabel xml:lang="en">is admissible value for</skos:prefLabel>
        <skos:prefLabel xml:lang="de">ist zulässiger Wert für</skos:prefLabel>
    </owl:ObjectProperty>
    


    <!-- http://www.molmod.info/semantics/pims-ii.ttl#isAssignmentFor -->


    <owl:ObjectProperty rdf:about="http://www.molmod.info/semantics/pims-ii.ttl#isAssignmentFor">
        <rdfs:domain rdf:resource="http://www.molmod.info/semantics/pims-ii.ttl#Assignment"/>
        <skos:broader rdf:resource="http://www.molmod.info/semantics/pims-ii.ttl#isRepresentamenFor"/>
        <skos:definition xml:lang="en">(o isAssignment for d) means that d: x = y is an assignment that refers to o; e.g., x may be temperature, y may be a temperature value, and o may be an object of which the temperature has been measured or some other context to which the assignment refers</skos:definition>
        <skos:editorialNote>changed by m4i: added skos:prefLabel, adjusted german labels, harmonized spelling to OBO naming conventions (lower case, space separated)</skos:editorialNote>
        <skos:prefLabel xml:lang="en">is assignment for</skos:prefLabel>
        <skos:prefLabel xml:lang="de">ist Zuweisung in Bezug auf</skos:prefLabel>
    </owl:ObjectProperty>
    


    <!-- http://www.molmod.info/semantics/pims-ii.ttl#isValueInAssignment -->


    <owl:ObjectProperty rdf:about="http://www.molmod.info/semantics/pims-ii.ttl#isValueInAssignment">
        <rdfs:domain rdf:resource="http://www.molmod.info/semantics/pims-ii.ttl#Value"/>
        <rdfs:range rdf:resource="http://www.molmod.info/semantics/pims-ii.ttl#Assignment"/>
        <skos:broader rdf:resource="http://www.molmod.info/semantics/pims-ii.ttl#isSemioticallyConstitutiveOf"/>
        <skos:definition xml:lang="en">(y isValueInAssignment a) means that a: x = y is an assignment where the value y is assigned to a variable x</skos:definition>
        <skos:editorialNote>changed by m4i: added skos:prefLabel, adjusted german labels, harmonized spelling to OBO naming conventions (lower case, space separated)</skos:editorialNote>
        <skos:prefLabel xml:lang="en">is value in assignment</skos:prefLabel>
        <skos:prefLabel xml:lang="de">ist Wert in Zuweisung</skos:prefLabel>
    </owl:ObjectProperty>
    


    <!-- http://www.molmod.info/semantics/pims-ii.ttl#isVariableInAssignment -->


    <owl:ObjectProperty rdf:about="http://www.molmod.info/semantics/pims-ii.ttl#isVariableInAssignment">
        <rdfs:domain rdf:resource="http://www.molmod.info/semantics/pims-ii.ttl#Variable"/>
        <rdfs:range rdf:resource="http://www.molmod.info/semantics/pims-ii.ttl#Assignment"/>
        <skos:broader rdf:resource="http://www.molmod.info/semantics/pims-ii.ttl#isSemioticallyConstitutiveOf"/>
        <skos:definition xml:lang="en">(x isVariableInAssignment a) means that a: x = y is an assignment where a value y is assigned to the variable x</skos:definition>
        <skos:editorialNote>changed by m4i: added skos:prefLabel, adjusted german labels, harmonized spelling to OBO naming conventions (lower case, space separated)</skos:editorialNote>
        <skos:prefLabel xml:lang="en">is variable in assignment</skos:prefLabel>
        <skos:prefLabel xml:lang="de">ist Variable in Zuweisung</skos:prefLabel>
    </owl:ObjectProperty>
    


    <!-- http://www.w3.org/ns/dcat#compressFormat -->


    <owl:ObjectProperty rdf:about="http://www.w3.org/ns/dcat#compressFormat">
        <rdfs:domain rdf:resource="http://www.w3.org/ns/dcat#Distribution"/>
        <rdfs:isDefinedBy rdf:resource="http://www.w3.org/ns/dcat#"/>
        <skos:definition xml:lang="en">The compression format of the distribution in which the data is contained in a compressed form, e.g. to reduce the size of the downloadable file.</skos:definition>
        <skos:editorialNote xml:lang="en">changed by m4i: added skos:prefLabel, added german labels, removed redundant notes, removed other languages than english in comment, label, changeNote and definition</skos:editorialNote>
        <skos:prefLabel xml:lang="de">Kompressionsformat</skos:prefLabel>
        <skos:prefLabel xml:lang="en">compression format</skos:prefLabel>
        <skos:scopeNote xml:lang="en">This property is to be used when the files in the distribution are compressed, e.g. in a ZIP file. The format SHOULD be expressed using a media type as defined by IANA media types registry https://www.iana.org/assignments/media-types/, if available.</skos:scopeNote>
    </owl:ObjectProperty>
    


    <!-- http://www.w3.org/ns/dcat#distribution -->


    <owl:ObjectProperty rdf:about="http://www.w3.org/ns/dcat#distribution">
        <rdfs:domain rdf:resource="http://www.w3.org/ns/dcat#Dataset"/>
        <rdfs:isDefinedBy rdf:resource="http://www.w3.org/ns/dcat#"/>
        <skos:definition xml:lang="en">An available distribution of the dataset.</skos:definition>
        <skos:editorialNote xml:lang="en">changed by m4i: added skos:prefLabel, added german labels, removed redundant notes, removed other languages than english in comment, label, changeNote and definition</skos:editorialNote>
        <skos:prefLabel xml:lang="en">has distribution</skos:prefLabel>
        <skos:prefLabel xml:lang="de">hat Verteilung</skos:prefLabel>
    </owl:ObjectProperty>
    


    <!-- http://www.w3.org/ns/dcat#downloadURL -->


    <owl:ObjectProperty rdf:about="http://www.w3.org/ns/dcat#downloadURL">
        <rdfs:domain rdf:resource="http://www.w3.org/ns/dcat#Distribution"/>
        <rdfs:isDefinedBy rdf:resource="http://purl.org/dc/terms/"/>
        <skos:definition xml:lang="en">The URL of the downloadable file in a given format. E.g. CSV file or RDF file. The format is indicated by the distribution&apos;s dcterms:format and/or dcat:mediaType.</skos:definition>
        <skos:editorialNote xml:lang="en">changed by m4i: added skos:prefLabel, added german labels, removed redundant notes, removed other languages than english in comment, label, changeNote and definition</skos:editorialNote>
        <skos:prefLabel xml:lang="de">Downloadlink</skos:prefLabel>
        <skos:prefLabel xml:lang="en">download URL</skos:prefLabel>
        <skos:scopeNote xml:lang="en">dcat:downloadURL SHOULD be used for the address at which this distribution is available directly, typically through a HTTP Get request.</skos:scopeNote>
    </owl:ObjectProperty>
    


    <!-- http://www.w3.org/ns/dcat#inSeries -->


    <owl:ObjectProperty rdf:about="http://www.w3.org/ns/dcat#inSeries">
        <rdfs:subPropertyOf rdf:resource="http://purl.obolibrary.org/obo/BFO_0000050"/>
        <rdfs:domain rdf:resource="http://www.w3.org/ns/dcat#Dataset"/>
        <rdfs:range rdf:resource="http://www.w3.org/ns/dcat#DatasetSeries"/>
        <rdfs:comment xml:lang="en">Normally, child datasets in dataset series are represented as dcat:Dataset. The use of dcat:Distribution for typing child datasets is however recognized as a possible alternative, whenever it addresses more effectively the requirements of a given application scenario.</rdfs:comment>
        <rdfs:isDefinedBy rdf:resource="http://www.w3.org/ns/dcat#"/>
        <skos:definition xml:lang="en">A dataset series of which the dataset is part.</skos:definition>
        <skos:editorialNote xml:lang="en">changed by m4i: changed subproperty relation from DCTerms to OBO_000050 added skos:prefLabel, added german labels,  removed redundant notes, extracted from DCAT3-Documentation https://www.w3.org/TR/vocab-dcat-3/#Class:Dataset_Series</skos:editorialNote>
        <skos:prefLabel xml:lang="de">in Serie</skos:prefLabel>
        <skos:prefLabel xml:lang="en">in series</skos:prefLabel>
    </owl:ObjectProperty>
    


    <!-- http://www.w3.org/ns/dcat#mediaType -->


    <owl:ObjectProperty rdf:about="http://www.w3.org/ns/dcat#mediaType">
        <rdfs:domain rdf:resource="http://www.w3.org/ns/dcat#Distribution"/>
        <rdfs:isDefinedBy rdf:resource="http://www.w3.org/ns/dcat#"/>
        <skos:definition xml:lang="en">The media type of the distribution as defined by IANA.</skos:definition>
        <skos:editorialNote xml:lang="en">changed by m4i: added skos:prefLabel, added german labels, removed redundant notes, removed other languages than english in comment, label, changeNote and definition</skos:editorialNote>
        <skos:prefLabel xml:lang="de">Medientyp</skos:prefLabel>
        <skos:prefLabel xml:lang="en">media type</skos:prefLabel>
        <skos:scopeNote xml:lang="en">This property SHOULD be used when the media type of the distribution is defined in the IANA media types registry https://www.iana.org/assignments/media-types/, otherwise dcterms:format MAY be used with different values.</skos:scopeNote>
    </owl:ObjectProperty>
    


    <!-- http://www.w3.org/ns/dcat#packageFormat -->


    <owl:ObjectProperty rdf:about="http://www.w3.org/ns/dcat#packageFormat">
        <rdfs:domain rdf:resource="http://www.w3.org/ns/dcat#Distribution"/>
        <rdfs:isDefinedBy rdf:resource="http://www.w3.org/ns/dcat#"/>
        <skos:definition xml:lang="en">The package format of the distribution in which one or more data files are grouped together, e.g. to enable a set of related files to be downloaded together.</skos:definition>
        <skos:editorialNote xml:lang="en">changed by m4i: added skos:prefLabel, added german labels, removed redundant notes, removed other languages than english in comment, label, changeNote and definition</skos:editorialNote>
        <skos:prefLabel xml:lang="de">Packformat</skos:prefLabel>
        <skos:prefLabel xml:lang="en">packaging format</skos:prefLabel>
        <skos:scopeNote xml:lang="en">This property to be used when the files in the distribution are packaged, e.g. in a TAR file, a Frictionless Data Package or a Bagit file. The format SHOULD be expressed using a media type as defined by IANA media types registry https://www.iana.org/assignments/media-types/, if available.</skos:scopeNote>
    </owl:ObjectProperty>
    


    <!-- http://www.w3.org/ns/prov#agent -->


    <owl:ObjectProperty rdf:about="http://www.w3.org/ns/prov#agent">
        <rdfs:range rdf:resource="http://www.w3.org/ns/prov#Agent"/>
        <skos:definition xml:lang="en">The prov:agent property is used to reference an agent that had a role in an activity.</skos:definition>
        <skos:editorialNote xml:lang="en">changed by m4i: added german label, added skos:prefLabel</skos:editorialNote>
        <skos:editorialNote xml:lang="en">changed by m4i: simplified definition</skos:editorialNote>
        <skos:prefLabel xml:lang="en">has agent</skos:prefLabel>
        <skos:prefLabel xml:lang="de">ist Akteur in</skos:prefLabel>
    </owl:ObjectProperty>
    


    <!-- http://www.w3.org/ns/prov#hadRole -->


    <owl:ObjectProperty rdf:about="http://www.w3.org/ns/prov#hadRole">
        <owl:inverseOf rdf:resource="http://www.w3.org/ns/prov#wasRoleIn"/>
        <rdfs:domain rdf:resource="http://www.w3.org/ns/prov#Association"/>
        <rdfs:label xml:lang="en">had role</rdfs:label>
        <rdfs:label xml:lang="de">hatte Rolle</rdfs:label>
        <skos:definition xml:lang="en">prov:hadRole references the Role (i.e. the function of an entity with respect to an activity)</skos:definition>
        <skos:editorialNote xml:lang="en">changed by m4i: added german label</skos:editorialNote>
        <skos:editorialNote xml:lang="en">changed by m4i: simplified definition</skos:editorialNote>
        <skos:editorialNote xml:lang="en">changed by m4i: simplified rdfs:domain to prov:Association</skos:editorialNote>
    </owl:ObjectProperty>
    


    <!-- http://www.w3.org/ns/prov#qualifiedAssociation -->


    <owl:ObjectProperty rdf:about="http://www.w3.org/ns/prov#qualifiedAssociation">
        <rdfs:domain rdf:resource="http://www.w3.org/ns/prov#Activity"/>
        <rdfs:range rdf:resource="http://www.w3.org/ns/prov#Association"/>
        <rdfs:isDefinedBy rdf:resource="http://www.w3.org/ns/prov#"/>
        <skos:definition xml:lang="en">Allows to specify more information (e.g. a role) about an association between an agent (e.g. a person) and an Activity (e.g. a processing step).</skos:definition>
        <skos:definition xml:lang="de">Ermöglicht die Angabe weiterer Informationen (z.B. einer Rolle) zu einer Verknüpfung zwischen einem Agenten (z.B. einer Person) und einer Aktivität (z.B. einem Prozessschritt).</skos:definition>
        <skos:editorialNote xml:lang="en">changed by m4i: added german label, added skos:prefLabel, added skos:definition, skos:example and skos:note</skos:editorialNote>
        <skos:example xml:lang="en">Example application in m4i:
:SomeProcess
    a m4i:ProcessingStep; 
    obo:RO_0000057 :SomePerson;
    prov:qualifiedAssociation [
        a prov:Association;
        prov:agent   :SomePerson;
        prov:hadRole :SomeRole;
        rdfs:comment &quot;:SomePerson had the :SomeRole in this :SomeProcess&quot;@en
    ].

The direct relation between an activity and an agent expressed with &apos;has participant&apos; (http://purl.obolibrary.org/obo/RO_0000057) does not give details about the agent&apos;s role in that activity. Using the property prov:qualifiedAssociation one can point to a blank node (cf. https://en.wikipedia.org/w/index.php?title=Blank_node&amp;oldid=1015446558) containing additional information about the participation relation.
</skos:example>
        <skos:note xml:lang="en">In metadata4ing use obo:RO_0000057 as unqualified form for the relation between an activity and an agent.</skos:note>
        <skos:prefLabel xml:lang="de">näher beschriebene Verbindung</skos:prefLabel>
        <skos:prefLabel xml:lang="en">qualified association</skos:prefLabel>
    </owl:ObjectProperty>
    


    <!-- http://www.w3.org/ns/prov#wasRoleIn -->


    <owl:ObjectProperty rdf:about="http://www.w3.org/ns/prov#wasRoleIn">
        <rdfs:label xml:lang="de">war Rolle in</rdfs:label>
        <rdfs:label xml:lang="en">was role in</rdfs:label>
        <skos:definition>prov:wasRoleIn references the association (e.g. between an agent and an activity) in which a role shall be defined. Inverse property of prov:hadRole.</skos:definition>
        <skos:editorialNote xml:lang="en">changed by m4i: added german label, added skos:definition, harmonized spelling to OBO naming conventions (lower case, space separated)</skos:editorialNote>
    </owl:ObjectProperty>
    


    <!-- http://www.w3.org/ns/ssn/hasProperty -->


    <owl:ObjectProperty rdf:about="http://www.w3.org/ns/ssn/hasProperty">
        <owl:inverseOf rdf:resource="http://www.w3.org/ns/ssn/isPropertyOf"/>
        <rdfs:isDefinedBy rdf:resource="http://www.w3.org/ns/ssn/"/>
        <skos:definition xml:lang="en">Relation between an entity and a Property of that entity.</skos:definition>
        <skos:editorialNote xml:lang="en">changed by m4i: added skos:prefLabel, added german labels</skos:editorialNote>
        <skos:prefLabel xml:lang="en">has property</skos:prefLabel>
        <skos:prefLabel xml:lang="de">hat Eigenschaft</skos:prefLabel>
    </owl:ObjectProperty>
    


    <!-- http://www.w3.org/ns/ssn/implementedBy -->


    <owl:ObjectProperty rdf:about="http://www.w3.org/ns/ssn/implementedBy">
        <skos:prefLabel xml:lang="en">implemented by</skos:prefLabel>
        <skos:prefLabel xml:lang="de">wird implementiert durch</skos:prefLabel>
    </owl:ObjectProperty>
    


    <!-- http://www.w3.org/ns/ssn/implements -->


    <owl:ObjectProperty rdf:about="http://www.w3.org/ns/ssn/implements">
        <skos:prefLabel xml:lang="de">implementiert</skos:prefLabel>
        <skos:prefLabel xml:lang="en">implements</skos:prefLabel>
    </owl:ObjectProperty>
    


    <!-- http://www.w3.org/ns/ssn/isPropertyOf -->


    <owl:ObjectProperty rdf:about="http://www.w3.org/ns/ssn/isPropertyOf">
        <skos:definition xml:lang="en">Relation between a Property and the entity it belongs to.</skos:definition>
        <skos:editorialNote xml:lang="en">changed by m4i: added skos:prefLabel, added german labels</skos:editorialNote>
        <skos:prefLabel xml:lang="en">is property of</skos:prefLabel>
        <skos:prefLabel xml:lang="de">ist Eigenschaft von</skos:prefLabel>
    </owl:ObjectProperty>
    


    <!-- http://xmlns.com/foaf/0.1/mbox -->


    <owl:ObjectProperty rdf:about="http://xmlns.com/foaf/0.1/mbox">
        <rdf:type rdf:resource="http://www.w3.org/2002/07/owl#InverseFunctionalProperty"/>
        <rdfs:range rdf:resource="http://www.w3.org/2002/07/owl#Thing"/>
        <rdfs:comment>A personal mailbox, ie. an Internet mailbox associated with exactly one owner, the first owner of this mailbox. This is a &apos;static inverse functional property&apos;, in that   there is (across time and change) at most one individual that ever has any particular value for foaf:mbox.</rdfs:comment>
        <rdfs:isDefinedBy rdf:resource="http://xmlns.com/foaf/0.1/"/>
        <skos:editorialNote xml:lang="en">changed by m4i: added german labels, added skos:prefLabel</skos:editorialNote>
        <skos:prefLabel xml:lang="de">E-Mail-Adresse</skos:prefLabel>
        <skos:prefLabel xml:lang="en">personal mailbox</skos:prefLabel>
    </owl:ObjectProperty>
    


    <!-- https://schema.org/instrument -->


    <owl:ObjectProperty rdf:about="https://schema.org/instrument">
        <rdfs:subPropertyOf rdf:resource="http://purl.obolibrary.org/obo/RO_0000057"/>
        <rdfs:domain rdf:resource="http://www.w3.org/ns/prov#Activity"/>
        <skos:definition xml:lang="en">points to an object that helped the agent perform the action (e.g., John wrote a book with a pen)</skos:definition>
        <skos:editorialNote xml:lang="en">changed by m4i: added different skos:prefLabel, added german label</skos:editorialNote>
        <skos:editorialNote xml:lang="en">changed by m4i: domain changed to prov:Activity from schema:Action</skos:editorialNote>
        <skos:prefLabel xml:lang="de">nutzt Instrument</skos:prefLabel>
        <skos:prefLabel xml:lang="en">uses instrument</skos:prefLabel>
    </owl:ObjectProperty>
    


    <!-- 
    ///////////////////////////////////////////////////////////////////////////////////////
    //
    // Data properties
    //
    ///////////////////////////////////////////////////////////////////////////////////////
     -->


    


    <!-- http://w3id.org/nfdi4ing/metadata4ing#UsageInstruction -->


    <owl:DatatypeProperty rdf:about="http://w3id.org/nfdi4ing/metadata4ing#UsageInstruction">
        <rdfs:domain rdf:resource="http://w3id.org/nfdi4ing/metadata4ing#ProcessingStep"/>
        <rdfs:range>
            <rdfs:Datatype>
                <owl:unionOf rdf:parseType="Collection">
                    <rdf:Description rdf:about="http://www.w3.org/2000/01/rdf-schema#Literal"/>
                    <rdf:Description rdf:about="http://www.w3.org/2001/XMLSchema#string"/>
                </owl:unionOf>
            </rdfs:Datatype>
        </rdfs:range>
        <skos:definition xml:lang="en">Textual description of a processing step within a research process to enable or facilitate its reproducibility</skos:definition>
        <skos:definition xml:lang="de">Textuelle Beschreibung eines Verarbeitungsschritts innerhalb eines Forschungsprozesses, um dessen Reproduzierbarkeit zu erleichtern oder zu ermöglichen</skos:definition>
        <skos:prefLabel xml:lang="de">Verwendungshinweis</skos:prefLabel>
        <skos:prefLabel xml:lang="en">usage instruction</skos:prefLabel>
    </owl:DatatypeProperty>
    


    <!-- http://w3id.org/nfdi4ing/metadata4ing#endOfProject -->


    <owl:DatatypeProperty rdf:about="http://w3id.org/nfdi4ing/metadata4ing#endOfProject">
        <rdfs:domain rdf:resource="https://schema.org/Project"/>
        <rdfs:range rdf:resource="http://www.w3.org/2001/XMLSchema#date"/>
        <skos:definition xml:lang="de">Projektenddatum</skos:definition>
        <skos:definition xml:lang="en">end date of a project</skos:definition>
        <skos:prefLabel xml:lang="de">Projektenddatum</skos:prefLabel>
        <skos:prefLabel xml:lang="en">project end date</skos:prefLabel>
    </owl:DatatypeProperty>
    


    <!-- http://w3id.org/nfdi4ing/metadata4ing#hasAssignmentTimestamp -->


    <owl:DatatypeProperty rdf:about="http://w3id.org/nfdi4ing/metadata4ing#hasAssignmentTimestamp">
        <rdfs:subPropertyOf rdf:resource="https://schema.org/temporal"/>
        <rdfs:domain rdf:resource="http://www.molmod.info/semantics/pims-ii.ttl#Assignment"/>
        <rdfs:range rdf:resource="https://schema.org/DateTime"/>
        <skos:definition xml:lang="en">Points to a timestamp associated with an assignment; there are multiple kinds of timestamp datatype properties, which are included here from schema.org</skos:definition>
        <skos:prefLabel xml:lang="en">has assignment timestamp</skos:prefLabel>
        <skos:prefLabel xml:lang="de">hat Zuweisungszeitstempel</skos:prefLabel>
    </owl:DatatypeProperty>
    


    <!-- http://w3id.org/nfdi4ing/metadata4ing#hasDateAssignmentCreated -->


    <owl:DatatypeProperty rdf:about="http://w3id.org/nfdi4ing/metadata4ing#hasDateAssignmentCreated">
        <rdfs:subPropertyOf rdf:resource="http://w3id.org/nfdi4ing/metadata4ing#hasAssignmentTimestamp"/>
        <rdfs:domain rdf:resource="http://www.molmod.info/semantics/pims-ii.ttl#Assignment"/>
        <rdfs:range rdf:resource="https://schema.org/DateTime"/>
        <skos:broader rdf:resource="https://schema.org/dateCreated"/>
        <skos:definition xml:lang="en">Points to a date(time) of creation of an assignment</skos:definition>
        <skos:prefLabel xml:lang="en">has date assignment created</skos:prefLabel>
        <skos:prefLabel xml:lang="de">hat Datumszuweisung erzeugt</skos:prefLabel>
    </owl:DatatypeProperty>
    


    <!-- http://w3id.org/nfdi4ing/metadata4ing#hasDateAssignmentDeleted -->


    <owl:DatatypeProperty rdf:about="http://w3id.org/nfdi4ing/metadata4ing#hasDateAssignmentDeleted">
        <rdfs:subPropertyOf rdf:resource="http://w3id.org/nfdi4ing/metadata4ing#hasAssignmentTimestamp"/>
        <rdfs:domain rdf:resource="http://www.molmod.info/semantics/pims-ii.ttl#Assignment"/>
        <rdfs:range rdf:resource="https://schema.org/DateTime"/>
        <skos:broader rdf:resource="https://schema.org/dateDeleted"/>
        <skos:definition xml:lang="en">Points to a date(time) of deletion of an assignment</skos:definition>
        <skos:prefLabel xml:lang="en">has date assignment deleted</skos:prefLabel>
        <skos:prefLabel xml:lang="de">hat Datumszuweisung gelöscht</skos:prefLabel>
    </owl:DatatypeProperty>
    


    <!-- http://w3id.org/nfdi4ing/metadata4ing#hasDateAssignmentModified -->


    <owl:DatatypeProperty rdf:about="http://w3id.org/nfdi4ing/metadata4ing#hasDateAssignmentModified">
        <rdfs:subPropertyOf rdf:resource="http://w3id.org/nfdi4ing/metadata4ing#hasAssignmentTimestamp"/>
        <rdfs:domain rdf:resource="http://www.molmod.info/semantics/pims-ii.ttl#Assignment"/>
        <rdfs:range rdf:resource="https://schema.org/DateTime"/>
        <skos:broader rdf:resource="https://schema.org/dateModified"/>
        <skos:definition xml:lang="en">Points to a date(time) of modification of an assignment</skos:definition>
        <skos:prefLabel xml:lang="en">has date assignment modified</skos:prefLabel>
        <skos:prefLabel xml:lang="de">hat Datumszuweisung bearbeitet</skos:prefLabel>
    </owl:DatatypeProperty>
    


    <!-- http://w3id.org/nfdi4ing/metadata4ing#hasDateAssignmentValidFrom -->


    <owl:DatatypeProperty rdf:about="http://w3id.org/nfdi4ing/metadata4ing#hasDateAssignmentValidFrom">
        <rdfs:subPropertyOf rdf:resource="http://w3id.org/nfdi4ing/metadata4ing#hasAssignmentTimestamp"/>
        <rdfs:domain rdf:resource="http://www.molmod.info/semantics/pims-ii.ttl#Assignment"/>
        <rdfs:range rdf:resource="https://schema.org/DateTime"/>
        <skos:broader rdf:resource="https://schema.org/validFrom"/>
        <skos:definition xml:lang="en">Points to a date(time) at which the validity of an assignment begins</skos:definition>
        <skos:prefLabel xml:lang="en">has date assignment valid from</skos:prefLabel>
        <skos:prefLabel xml:lang="de">hat Datumszuweisung gültig ab</skos:prefLabel>
    </owl:DatatypeProperty>
    


    <!-- http://w3id.org/nfdi4ing/metadata4ing#hasDateAssignmentValidUntil -->


    <owl:DatatypeProperty rdf:about="http://w3id.org/nfdi4ing/metadata4ing#hasDateAssignmentValidUntil">
        <rdfs:subPropertyOf rdf:resource="http://w3id.org/nfdi4ing/metadata4ing#hasAssignmentTimestamp"/>
        <rdfs:domain rdf:resource="http://www.molmod.info/semantics/pims-ii.ttl#Assignment"/>
        <rdfs:range rdf:resource="https://schema.org/DateTime"/>
        <skos:broader rdf:resource="https://schema.org/validThrough"/>
        <skos:definition xml:lang="en">Points to a date(time) at which the validity of an assignment ends</skos:definition>
        <skos:prefLabel xml:lang="en">has date assignment valid until</skos:prefLabel>
        <skos:prefLabel xml:lang="de">hat Datumszuweisung gültig bis</skos:prefLabel>
    </owl:DatatypeProperty>
    


    <!-- http://w3id.org/nfdi4ing/metadata4ing#hasMaximumValue -->


    <owl:DatatypeProperty rdf:about="http://w3id.org/nfdi4ing/metadata4ing#hasMaximumValue">
        <rdfs:subPropertyOf rdf:resource="http://w3id.org/nfdi4ing/metadata4ing#hasValue"/>
        <rdfs:domain rdf:resource="https://ptb.de/si/Real"/>
        <rdfs:range>
            <rdfs:Datatype>
                <owl:unionOf rdf:parseType="Collection">
                    <rdf:Description rdf:about="http://www.w3.org/2001/XMLSchema#decimal"/>
                    <rdf:Description rdf:about="https://ptb.de/dcc/formulaType"/>
                </owl:unionOf>
            </rdfs:Datatype>
        </rdfs:range>
        <skos:broader rdf:resource="http://qudt.org/schema/qudt/value"/>
        <skos:broader rdf:resource="http://www.molmod.info/semantics/pims-ii.ttl#isLiterally"/>
        <skos:broader rdf:resource="https://ptb.de/si/hasValue"/>
        <skos:definition xml:lang="en">Represents the highest value of a multi-valued variable</skos:definition>
        <skos:prefLabel xml:lang="en">has maximum value</skos:prefLabel>
        <skos:prefLabel xml:lang="de">hat Maximalwert</skos:prefLabel>
    </owl:DatatypeProperty>
    


    <!-- http://w3id.org/nfdi4ing/metadata4ing#hasMinimumValue -->


    <owl:DatatypeProperty rdf:about="http://w3id.org/nfdi4ing/metadata4ing#hasMinimumValue">
        <rdfs:subPropertyOf rdf:resource="http://w3id.org/nfdi4ing/metadata4ing#hasValue"/>
        <rdfs:domain rdf:resource="https://ptb.de/si/Real"/>
        <rdfs:range>
            <rdfs:Datatype>
                <owl:unionOf rdf:parseType="Collection">
                    <rdf:Description rdf:about="http://www.w3.org/2001/XMLSchema#decimal"/>
                    <rdf:Description rdf:about="https://ptb.de/dcc/formulaType"/>
                </owl:unionOf>
            </rdfs:Datatype>
        </rdfs:range>
        <skos:broader rdf:resource="http://qudt.org/schema/qudt/value"/>
        <skos:broader rdf:resource="http://www.molmod.info/semantics/pims-ii.ttl#isLiterally"/>
        <skos:broader rdf:resource="https://ptb.de/si/hasValue"/>
        <skos:definition xml:lang="en">Represents the lowest value of a multi-valued variable</skos:definition>
        <skos:prefLabel xml:lang="en">has minimum value</skos:prefLabel>
        <skos:prefLabel xml:lang="de">hat Minimalwert</skos:prefLabel>
    </owl:DatatypeProperty>
    


    <!-- http://w3id.org/nfdi4ing/metadata4ing#hasNumericalValue -->


    <owl:DatatypeProperty rdf:about="http://w3id.org/nfdi4ing/metadata4ing#hasNumericalValue">
        <rdfs:subPropertyOf rdf:resource="http://w3id.org/nfdi4ing/metadata4ing#hasValue"/>
        <rdfs:domain rdf:resource="https://ptb.de/si/Real"/>
        <rdfs:range>
            <rdfs:Datatype>
                <owl:unionOf rdf:parseType="Collection">
                    <rdf:Description rdf:about="http://www.w3.org/2001/XMLSchema#decimal"/>
                    <rdf:Description rdf:about="https://ptb.de/dcc/formulaType"/>
                </owl:unionOf>
            </rdfs:Datatype>
        </rdfs:range>
        <skos:broader rdf:resource="http://qudt.org/schema/qudt/value"/>
        <skos:broader rdf:resource="http://www.molmod.info/semantics/pims-ii.ttl#isLiterally"/>
        <skos:broader rdf:resource="https://ptb.de/si/hasValue"/>
        <skos:closeMatch rdf:resource="https://ptb.de/si/hasNumericalValue"/>
        <skos:definition xml:lang="en">Represents the numerical value of a real</skos:definition>
        <skos:prefLabel xml:lang="en">has numerical value</skos:prefLabel>
        <skos:prefLabel xml:lang="de">hat Zahlenwert</skos:prefLabel>
    </owl:DatatypeProperty>
    


    <!-- http://w3id.org/nfdi4ing/metadata4ing#hasRorId -->


    <owl:DatatypeProperty rdf:about="http://w3id.org/nfdi4ing/metadata4ing#hasRorId">
        <rdfs:subPropertyOf rdf:resource="http://w3id.org/nfdi4ing/metadata4ing#identifier"/>
        <rdfs:domain rdf:resource="http://www.w3.org/ns/prov#Organization"/>
        <rdfs:range>
            <rdfs:Datatype>
                <owl:onDatatype rdf:resource="http://www.w3.org/2001/XMLSchema#string"/>
                <owl:withRestrictions rdf:parseType="Collection">
                    <rdf:Description>
                        <xsd:pattern>https://ror.org/[0-9][0-9][a-z0-9][a-z0-9][a-z0-9][a-z0-9][a-z0-9][0-9][0-9]</xsd:pattern>
                    </rdf:Description>
                </owl:withRestrictions>
            </rdfs:Datatype>
        </rdfs:range>
        <skos:altLabel xml:lang="en">has research organization registry id</skos:altLabel>
        <skos:altLabel xml:lang="de">hat Forschungsorganisationsid</skos:altLabel>
        <skos:definition xml:lang="en">A Research Organization Registry identifier, that points to a research organization</skos:definition>
        <skos:definition xml:lang="de">Eine Identifier für Organisationen der Research Organization Registry, die eine Forschungseinrichtung eindeutig identifiziert.</skos:definition>
        <skos:prefLabel xml:lang="en">has ROR ID</skos:prefLabel>
        <skos:prefLabel xml:lang="de">hat ROR ID</skos:prefLabel>
    </owl:DatatypeProperty>
    


    <!-- http://w3id.org/nfdi4ing/metadata4ing#hasStepSize -->


    <owl:DatatypeProperty rdf:about="http://w3id.org/nfdi4ing/metadata4ing#hasStepSize">
        <rdfs:subPropertyOf rdf:resource="http://w3id.org/nfdi4ing/metadata4ing#hasValue"/>
        <rdfs:domain rdf:resource="https://ptb.de/si/Real"/>
        <rdfs:range>
            <rdfs:Datatype>
                <owl:unionOf rdf:parseType="Collection">
                    <rdf:Description rdf:about="http://www.w3.org/2001/XMLSchema#decimal"/>
                    <rdf:Description rdf:about="https://ptb.de/dcc/formulaType"/>
                </owl:unionOf>
            </rdfs:Datatype>
        </rdfs:range>
        <skos:broader rdf:resource="http://qudt.org/schema/qudt/value"/>
        <skos:broader rdf:resource="http://www.molmod.info/semantics/pims-ii.ttl#isLiterally"/>
        <skos:broader rdf:resource="https://ptb.de/si/hasValue"/>
        <skos:definition xml:lang="en">Describes the spacing of a multi-valued variable</skos:definition>
        <skos:prefLabel xml:lang="en">has step size</skos:prefLabel>
        <skos:prefLabel xml:lang="de">hat Schrittweite</skos:prefLabel>
    </owl:DatatypeProperty>
    


    <!-- http://w3id.org/nfdi4ing/metadata4ing#hasStringValue -->


    <owl:DatatypeProperty rdf:about="http://w3id.org/nfdi4ing/metadata4ing#hasStringValue">
        <rdfs:subPropertyOf rdf:resource="http://w3id.org/nfdi4ing/metadata4ing#hasValue"/>
        <rdfs:domain rdf:resource="http://w3id.org/nfdi4ing/metadata4ing#TextVariable"/>
        <rdfs:range rdf:resource="http://www.w3.org/2001/XMLSchema#string"/>
        <skos:definition xml:lang="en">A character string of any length</skos:definition>
        <skos:definition xml:lang="de">Eine Zeichenkette (Text) beliebiger Länge.</skos:definition>
        <skos:prefLabel xml:lang="en">has string value</skos:prefLabel>
        <skos:prefLabel xml:lang="de">hat Zeichenwert</skos:prefLabel>
    </owl:DatatypeProperty>
    


    <!-- http://w3id.org/nfdi4ing/metadata4ing#hasSymbol -->


    <owl:DatatypeProperty rdf:about="http://w3id.org/nfdi4ing/metadata4ing#hasSymbol">
        <rdfs:domain rdf:resource="http://www.molmod.info/semantics/pims-ii.ttl#Variable"/>
        <rdfs:range rdf:resource="http://www.w3.org/2001/XMLSchema#string"/>
        <skos:broader rdf:resource="http://qudt.org/schema/qudt/symbol"/>
        <skos:definition xml:lang="de">Buchstabe oder Zeichenkette, die eine Variable repräsentiert</skos:definition>
        <skos:definition xml:lang="en">Letter or string that denotes a variable</skos:definition>
        <skos:prefLabel xml:lang="en">has symbol</skos:prefLabel>
        <skos:prefLabel xml:lang="de">hat Symbol</skos:prefLabel>
    </owl:DatatypeProperty>
    


    <!-- http://w3id.org/nfdi4ing/metadata4ing#hasValue -->


    <owl:DatatypeProperty rdf:about="http://w3id.org/nfdi4ing/metadata4ing#hasValue">
        <rdfs:domain rdf:resource="http://www.molmod.info/semantics/pims-ii.ttl#Variable"/>
        <skos:definition xml:lang="en">A value of any type</skos:definition>
        <skos:definition xml:lang="de">Ein beliebiger Wert</skos:definition>
        <skos:prefLabel xml:lang="en">has value</skos:prefLabel>
        <skos:prefLabel xml:lang="de">hat Wert</skos:prefLabel>
    </owl:DatatypeProperty>
    


    <!-- http://w3id.org/nfdi4ing/metadata4ing#hasVariableDescription -->


    <owl:DatatypeProperty rdf:about="http://w3id.org/nfdi4ing/metadata4ing#hasVariableDescription">
        <rdfs:domain rdf:resource="http://www.molmod.info/semantics/pims-ii.ttl#Variable"/>
        <rdfs:range rdf:resource="http://www.w3.org/2001/XMLSchema#string"/>
        <skos:definition xml:lang="en">Textual and human readable description of a variable in a research context</skos:definition>
        <skos:definition xml:lang="de">Textuelle und menschenlesbare Beschreibung einer Variablen im Forschungskontext</skos:definition>
        <skos:prefLabel xml:lang="en">has variable description</skos:prefLabel>
        <skos:prefLabel xml:lang="de">hat Variablenbeschreibung</skos:prefLabel>
    </owl:DatatypeProperty>
    


    <!-- http://w3id.org/nfdi4ing/metadata4ing#identifier -->


    <owl:DatatypeProperty rdf:about="http://w3id.org/nfdi4ing/metadata4ing#identifier">
        <rdfs:domain rdf:resource="http://www.w3.org/2002/07/owl#Thing"/>
        <rdfs:range rdf:resource="http://www.w3.org/2001/XMLSchema#string"/>
        <skos:altLabel xml:lang="de">besitzt eindeutigen Identifikator</skos:altLabel>
        <skos:altLabel xml:lang="en">has unique identifier</skos:altLabel>
        <skos:altLabel xml:lang="en">is represented through identifier</skos:altLabel>
        <skos:altLabel xml:lang="de">wird durch Identifikator repräsentiert</skos:altLabel>
        <skos:definition xml:lang="en">A systematically built alphanumeric string that identifies a unique object (e.g. a person, a publication, an organisation, a research activity, a sample, etc.) or a unique class of objects.</skos:definition>
        <skos:prefLabel xml:lang="en">has identifier</skos:prefLabel>
        <skos:prefLabel xml:lang="de">hat Identifikator</skos:prefLabel>
    </owl:DatatypeProperty>
    


    <!-- http://w3id.org/nfdi4ing/metadata4ing#orcidId -->


    <owl:DatatypeProperty rdf:about="http://w3id.org/nfdi4ing/metadata4ing#orcidId">
        <rdfs:subPropertyOf rdf:resource="http://w3id.org/nfdi4ing/metadata4ing#identifier"/>
        <rdfs:domain rdf:resource="http://www.w3.org/ns/prov#Person"/>
        <rdfs:range rdf:resource="http://www.w3.org/2001/XMLSchema#string"/>
        <skos:prefLabel xml:lang="en">has ORCID ID</skos:prefLabel>
        <skos:prefLabel xml:lang="de">hat ORCID ID</skos:prefLabel>
    </owl:DatatypeProperty>
    


    <!-- http://w3id.org/nfdi4ing/metadata4ing#projectReferenceID -->


    <owl:DatatypeProperty rdf:about="http://w3id.org/nfdi4ing/metadata4ing#projectReferenceID">
        <rdfs:subPropertyOf rdf:resource="http://w3id.org/nfdi4ing/metadata4ing#identifier"/>
        <rdfs:domain rdf:resource="https://schema.org/Project"/>
        <rdfs:range rdf:resource="http://www.w3.org/2001/XMLSchema#string"/>
        <skos:definition xml:lang="en">An alphanumeric identifier for a project.</skos:definition>
        <skos:definition xml:lang="de">Eine alphanumerische ID zur Referenzierung eines Projekts.</skos:definition>
        <skos:prefLabel xml:lang="en">has project ID</skos:prefLabel>
        <skos:prefLabel xml:lang="de">hat Projekt-ID</skos:prefLabel>
    </owl:DatatypeProperty>
    


    <!-- http://w3id.org/nfdi4ing/metadata4ing#startOfProject -->


    <owl:DatatypeProperty rdf:about="http://w3id.org/nfdi4ing/metadata4ing#startOfProject">
        <rdfs:domain rdf:resource="https://schema.org/Project"/>
        <rdfs:range rdf:resource="http://www.w3.org/2001/XMLSchema#date"/>
        <skos:definition xml:lang="de">Startdatum eines Projekts</skos:definition>
        <skos:definition xml:lang="en">start date of a project</skos:definition>
        <skos:prefLabel xml:lang="de">Projektstartdatum</skos:prefLabel>
        <skos:prefLabel xml:lang="en">project start date</skos:prefLabel>
    </owl:DatatypeProperty>
    


    <!-- http://www.w3.org/ns/dcat#byteSize -->


    <owl:DatatypeProperty rdf:about="http://www.w3.org/ns/dcat#byteSize">
        <rdfs:domain rdf:resource="http://www.w3.org/ns/dcat#Distribution"/>
        <rdfs:isDefinedBy rdf:resource="http://www.w3.org/ns/dcat#"/>
        <skos:definition xml:lang="en">The size of a distribution in bytes.</skos:definition>
        <skos:editorialNote xml:lang="en">changed by m4i: added skos:prefLabel, added german labels, removed redundant notes, removed other languages than english in comment, label, changeNote and definition</skos:editorialNote>
        <skos:prefLabel xml:lang="de">Dateigröße (in Byte)</skos:prefLabel>
        <skos:prefLabel xml:lang="en">file size (in bytes)</skos:prefLabel>
        <skos:scopeNote xml:lang="en">The size in bytes can be approximated when the precise size is not known. The literal value of dcat:byteSize should by typed as xsd:decimal.</skos:scopeNote>
    </owl:DatatypeProperty>
    


    <!-- http://www.w3.org/ns/dcat#spatialResolutionInMeters -->


    <owl:DatatypeProperty rdf:about="http://www.w3.org/ns/dcat#spatialResolutionInMeters">
        <rdfs:range rdf:resource="http://www.w3.org/2001/XMLSchema#decimal"/>
        <skos:definition xml:lang="en">Minimum spatial separation resolvable in a dataset, measured in metres.</skos:definition>
        <skos:editorialNote xml:lang="en">changed by m4i: added skos:prefLabel, added german labels, removed redundant notes, removed other languages than english in comment, label, changeNote and definition, adjusted spelling conform to SI</skos:editorialNote>
        <skos:prefLabel xml:lang="de">räumliche Auflösung (in Metern)</skos:prefLabel>
        <skos:prefLabel xml:lang="en">spatial resolution (in metres)</skos:prefLabel>
        <skos:scopeNote xml:lang="en">Alternative spatial resolutions might be provided as different dataset distributions.</skos:scopeNote>
        <skos:scopeNote xml:lang="en">If the dataset is an image or grid this should correspond to the spacing of items. For other kinds of spatial dataset, this property will usually indicate the smallest distance between items in the dataset.</skos:scopeNote>
    </owl:DatatypeProperty>
    


    <!-- http://www.w3.org/ns/dcat#temporalResolution -->


    <owl:DatatypeProperty rdf:about="http://www.w3.org/ns/dcat#temporalResolution">
        <rdfs:range rdf:resource="http://www.w3.org/2001/XMLSchema#duration"/>
        <skos:definition xml:lang="en">Minimum time period resolvable in a dataset.</skos:definition>
        <skos:editorialNote xml:lang="en">changed by m4i: added skos:prefLabel, added german labels, removed redundant notes, removed other languages than english in comment, label, changeNote and definition, harmonized spelling to OBO naming conventions (lower case, space separated)</skos:editorialNote>
        <skos:prefLabel xml:lang="en">temporal resolution</skos:prefLabel>
        <skos:prefLabel xml:lang="de">zeitliche Auflösung</skos:prefLabel>
        <skos:scopeNote xml:lang="en">Alternative temporal resolutions might be provided as different dataset distributions.</skos:scopeNote>
        <skos:scopeNote xml:lang="en">If the dataset is a time-series this should correspond to the spacing of items in the series. For other kinds of dataset, this property will usually indicate the smallest time difference between items in the dataset.</skos:scopeNote>
    </owl:DatatypeProperty>
    


    <!-- http://xmlns.com/foaf/0.1/firstName -->


    <owl:DatatypeProperty rdf:about="http://xmlns.com/foaf/0.1/firstName">
        <rdfs:range rdf:resource="http://www.w3.org/2000/01/rdf-schema#Literal"/>
        <rdfs:comment>The first name of a person.</rdfs:comment>
        <skos:editorialNote xml:lang="en">changed by m4i: added german labels, added skos:prefLabel</skos:editorialNote>
        <skos:prefLabel xml:lang="de">Vorname</skos:prefLabel>
        <skos:prefLabel xml:lang="en">first name</skos:prefLabel>
    </owl:DatatypeProperty>
    


    <!-- http://xmlns.com/foaf/0.1/lastName -->


    <owl:DatatypeProperty rdf:about="http://xmlns.com/foaf/0.1/lastName">
        <rdfs:range rdf:resource="http://www.w3.org/2000/01/rdf-schema#Literal"/>
        <rdfs:comment>The last name of a person.</rdfs:comment>
        <skos:editorialNote xml:lang="en">changed by m4i: added german labels, added skos:prefLabel</skos:editorialNote>
        <skos:prefLabel xml:lang="de">Nachname</skos:prefLabel>
        <skos:prefLabel xml:lang="en">last name</skos:prefLabel>
    </owl:DatatypeProperty>
    


    <!-- http://xmlns.com/foaf/0.1/title -->


    <owl:DatatypeProperty rdf:about="http://xmlns.com/foaf/0.1/title">
        <rdfs:range rdf:resource="http://www.w3.org/2000/01/rdf-schema#Literal"/>
        <rdfs:comment>Title (Mr, Mrs, Ms, Dr. etc)</rdfs:comment>
        <skos:editorialNote xml:lang="en">changed by m4i: added german labels, added skos:prefLabel, defined rdfs:domain and rdfs:range</skos:editorialNote>
        <skos:prefLabel xml:lang="de">Anrede</skos:prefLabel>
        <skos:prefLabel xml:lang="en">salutation</skos:prefLabel>
    </owl:DatatypeProperty>
    


    <!-- https://ptb.de/si/hasCoverageFactor -->


    <owl:DatatypeProperty rdf:about="https://ptb.de/si/hasCoverageFactor">
        <rdfs:domain rdf:resource="https://ptb.de/si/ExpandedUnc"/>
        <rdfs:range>
            <rdfs:Datatype>
                <owl:onDatatype rdf:resource="http://www.w3.org/2001/XMLSchema#decimal"/>
                <owl:withRestrictions rdf:parseType="Collection">
                    <rdf:Description>
                        <xsd:minInclusive rdf:datatype="http://www.w3.org/2001/XMLSchema#decimal">1.0</xsd:minInclusive>
                    </rdf:Description>
                </owl:withRestrictions>
            </rdfs:Datatype>
        </rdfs:range>
        <skos:definition xml:lang="en">points to the coverage factor, i.e., to a factor (greater than or equal to unity) by which the expanded uncertainty relates to the standard uncertainty</skos:definition>
        <skos:editorialNote>changed by m4i: harmonized spelling to OBO naming conventions (lower case, space separated), added skos:prefLabel</skos:editorialNote>
        <skos:prefLabel xml:lang="en">has coverage factor</skos:prefLabel>
        <skos:prefLabel xml:lang="de">hat Überdeckungsfaktor</skos:prefLabel>
    </owl:DatatypeProperty>
    


    <!-- https://ptb.de/si/hasCoverageProbability -->


    <owl:DatatypeProperty rdf:about="https://ptb.de/si/hasCoverageProbability">
        <rdfs:domain rdf:resource="http://w3id.org/nfdi4ing/metadata4ing#UncertaintyDeclaration"/>
        <rdfs:range>
            <rdfs:Datatype>
                <owl:onDatatype rdf:resource="http://www.w3.org/2001/XMLSchema#decimal"/>
                <owl:withRestrictions rdf:parseType="Collection">
                    <rdf:Description>
                        <xsd:minInclusive rdf:datatype="http://www.w3.org/2001/XMLSchema#decimal">0.0</xsd:minInclusive>
                    </rdf:Description>
                    <rdf:Description>
                        <xsd:maxInclusive rdf:datatype="http://www.w3.org/2001/XMLSchema#decimal">1.0</xsd:maxInclusive>
                    </rdf:Description>
                </owl:withRestrictions>
            </rdfs:Datatype>
        </rdfs:range>
        <skos:definition xml:lang="en">points to the probability (between 0 and 1) ascribed to the event of the actual value falling within the range asserted by the given uncertainty declaration</skos:definition>
        <skos:editorialNote>changed by m4i: harmonized spelling to OBO naming conventions (lower case, space separated), added skos:prefLabel</skos:editorialNote>
        <skos:prefLabel xml:lang="en">has coverage probability</skos:prefLabel>
        <skos:prefLabel xml:lang="de">hat Deckungswahrscheinlichkeit</skos:prefLabel>
    </owl:DatatypeProperty>
    


    <!-- https://ptb.de/si/hasDistribution -->


    <owl:DatatypeProperty rdf:about="https://ptb.de/si/hasDistribution">
        <rdfs:domain rdf:resource="http://w3id.org/nfdi4ing/metadata4ing#UncertaintyDeclaration"/>
        <rdfs:range rdf:resource="http://www.w3.org/2001/XMLSchema#string"/>
        <skos:definition xml:lang="en">points to a descriptor/label of the assumed underlying distribution</skos:definition>
        <skos:editorialNote>changed by m4i: harmonized spelling to OBO naming conventions (lower case, space separated), added skos:prefLabel</skos:editorialNote>
        <skos:prefLabel xml:lang="en">has statistical distribution</skos:prefLabel>
        <skos:prefLabel xml:lang="de">hat statistische Verteilung</skos:prefLabel>
    </owl:DatatypeProperty>
    


    <!-- https://ptb.de/si/hasIntervalMax -->


    <owl:DatatypeProperty rdf:about="https://ptb.de/si/hasIntervalMax">
        <rdfs:domain rdf:resource="https://ptb.de/si/CoverageInterval"/>
        <rdfs:range rdf:resource="http://www.w3.org/2001/XMLSchema#decimal"/>
        <skos:definition xml:lang="en">upper boundary of the coverage interval</skos:definition>
        <skos:editorialNote>changed by m4i: harmonized spelling to OBO naming conventions (lower case, space separated), added skos:prefLabel</skos:editorialNote>
        <skos:prefLabel xml:lang="en">has interval maximum</skos:prefLabel>
        <skos:prefLabel xml:lang="de">hat Intervallmaximum</skos:prefLabel>
    </owl:DatatypeProperty>
    


    <!-- https://ptb.de/si/hasIntervalMin -->


    <owl:DatatypeProperty rdf:about="https://ptb.de/si/hasIntervalMin">
        <rdfs:domain rdf:resource="https://ptb.de/si/CoverageInterval"/>
        <rdfs:range rdf:resource="http://www.w3.org/2001/XMLSchema#decimal"/>
        <skos:definition xml:lang="en">lower boundary of the coverage interval</skos:definition>
        <skos:editorialNote>changed by m4i: harmonized spelling to OBO naming conventions (lower case, space separated), added skos:prefLabel</skos:editorialNote>
        <skos:prefLabel xml:lang="en">has interval minimum</skos:prefLabel>
        <skos:prefLabel xml:lang="de">hat Intervallminimum</skos:prefLabel>
    </owl:DatatypeProperty>
    


    <!-- https://ptb.de/si/hasStandardUnc -->


    <owl:DatatypeProperty rdf:about="https://ptb.de/si/hasStandardUnc">
        <rdfs:domain rdf:resource="https://ptb.de/si/CoverageInterval"/>
        <rdfs:range>
            <rdfs:Datatype>
                <owl:onDatatype rdf:resource="http://www.w3.org/2001/XMLSchema#decimal"/>
                <owl:withRestrictions rdf:parseType="Collection">
                    <rdf:Description>
                        <xsd:minInclusive rdf:datatype="http://www.w3.org/2001/XMLSchema#decimal">0.0</xsd:minInclusive>
                    </rdf:Description>
                </owl:withRestrictions>
            </rdfs:Datatype>
        </rdfs:range>
        <skos:definition xml:lang="en">The standard measurement uncertainty is the measurement uncertainty expressed as a standard deviation</skos:definition>
        <skos:editorialNote>changed by m4i: harmonized spelling to OBO naming conventions (lower case, space separated), added skos:prefLabel</skos:editorialNote>
        <skos:prefLabel xml:lang="en">has standard uncertainty</skos:prefLabel>
        <skos:prefLabel xml:lang="de">hat Standardunsicherheit</skos:prefLabel>
    </owl:DatatypeProperty>
    


    <!-- https://ptb.de/si/hasUncertainty -->


    <owl:DatatypeProperty rdf:about="https://ptb.de/si/hasUncertainty">
        <rdfs:domain rdf:resource="https://ptb.de/si/ExpandedUnc"/>
        <rdfs:range>
            <rdfs:Datatype>
                <owl:onDatatype rdf:resource="http://www.w3.org/2001/XMLSchema#decimal"/>
                <owl:withRestrictions rdf:parseType="Collection">
                    <rdf:Description>
                        <xsd:minInclusive rdf:datatype="http://www.w3.org/2001/XMLSchema#decimal">0.0</xsd:minInclusive>
                    </rdf:Description>
                </owl:withRestrictions>
            </rdfs:Datatype>
        </rdfs:range>
        <skos:definition xml:lang="en">absolute magnitude of the indicated uncertainty</skos:definition>
        <skos:editorialNote>changed by m4i: harmonized spelling to OBO naming conventions (lower case, space separated), added skos:prefLabel</skos:editorialNote>
        <skos:prefLabel xml:lang="en">has uncertainty</skos:prefLabel>
        <skos:prefLabel xml:lang="de">hat Unsicherheit</skos:prefLabel>
    </owl:DatatypeProperty>
    


    <!-- https://schema.org/endTime -->


    <owl:DatatypeProperty rdf:about="https://schema.org/endTime">
        <rdfs:domain rdf:resource="http://w3id.org/nfdi4ing/metadata4ing#ProcessingStep"/>
        <rdfs:range rdf:resource="https://schema.org/DateTime"/>
        <rdfs:comment xml:lang="en">The endTime of something. For a reserved event or service (e.g. FoodEstablishmentReservation), the time that it is expected to end. For actions that span a period of time, when the action was performed. e.g. John wrote a book from January to &lt;em&gt;December&lt;/em&gt;. For media, including audio and video, it&apos;s the time offset of the end of a clip within a larger file.&lt;br/&gt;&lt;br/&gt;

Note that Event uses startDate/endDate instead of startTime/endTime, even when describing dates with times. This situation may be clarified in future revisions.</rdfs:comment>
        <rdfs:isDefinedBy rdf:resource="https://schema.org/"/>
        <skos:editorialNote xml:lang="en">changed by m4i: added skos:prefLabel, added german label</skos:editorialNote>
        <skos:prefLabel xml:lang="de">Endzeit</skos:prefLabel>
        <skos:prefLabel xml:lang="en">end time</skos:prefLabel>
    </owl:DatatypeProperty>
    


    <!-- https://schema.org/startTime -->


    <owl:DatatypeProperty rdf:about="https://schema.org/startTime">
        <rdfs:domain rdf:resource="http://w3id.org/nfdi4ing/metadata4ing#ProcessingStep"/>
        <rdfs:range rdf:resource="https://schema.org/DateTime"/>
        <rdfs:comment xml:lang="en">The startTime of something. For a reserved event or service (e.g. FoodEstablishmentReservation), the time that it is expected to start. For actions that span a period of time, when the action was performed. e.g. John wrote a book from &lt;em&gt;January&lt;/em&gt; to December. For media, including audio and video, it&apos;s the time offset of the start of a clip within a larger file.&lt;br/&gt;&lt;br/&gt;

Note that Event uses startDate/endDate instead of startTime/endTime, even when describing dates with times. This situation may be clarified in future revisions.</rdfs:comment>
        <rdfs:isDefinedBy rdf:resource="https://schema.org/"/>
        <skos:editorialNote xml:lang="en">changed by m4i: added skos:prefLabel, added german label</skos:editorialNote>
        <skos:prefLabel xml:lang="de">Startzeit</skos:prefLabel>
        <skos:prefLabel xml:lang="en">start time</skos:prefLabel>
    </owl:DatatypeProperty>
    


    <!-- https://schema.org/temporal -->


    <owl:DatatypeProperty rdf:about="https://schema.org/temporal">
        <rdfs:range rdf:resource="https://schema.org/DateTime"/>
        <skos:definition xml:lang="en">The &apos;temporal&apos; property can be used in cases where more specific properties (e.g., dateCreated, dateModified, datePublished) are not known to be appropriate</skos:definition>
        <skos:editorialNote xml:lang="en">changed by m4i: added different skos:prefLabel, added german label</skos:editorialNote>
        <skos:prefLabel xml:lang="en">has timestamp</skos:prefLabel>
        <skos:prefLabel xml:lang="de">hat Zeitstempel</skos:prefLabel>
    </owl:DatatypeProperty>
    


    <!-- 
    ///////////////////////////////////////////////////////////////////////////////////////
    //
    // Classes
    //
    ///////////////////////////////////////////////////////////////////////////////////////
     -->


    


    <!-- http://purl.obolibrary.org/obo/BFO_0000015 -->


    <owl:Class rdf:about="http://purl.obolibrary.org/obo/BFO_0000015">
        <skos:closeMatch rdf:resource="http://www.molmod.info/semantics/pims-ii.ttl#Process"/>
        <skos:definition xml:lang="en">Process, i.e., a physical entity with a temporal evolution that &apos;has a meaning for the ontologist&apos;</skos:definition>
        <skos:editorialNote xml:lang="en">changed by m4i: added german labels, added skos:prefLabel</skos:editorialNote>
        <skos:prefLabel xml:lang="de">Prozess</skos:prefLabel>
        <skos:prefLabel xml:lang="en">process</skos:prefLabel>
    </owl:Class>
    


    <!-- http://purl.obolibrary.org/obo/BFO_0000017 -->


    <owl:Class rdf:about="http://purl.obolibrary.org/obo/BFO_0000017">
        <skos:definition>To say that b is a realizable entity is to say that b is a specifically dependent continuant that inheres in some independent continuant which is not a spatial region and is of a type instances of which are realized in processes of a correlated type. (axiom label in BFO2 Reference: [058-002])</skos:definition>
        <skos:editorialNote xml:lang="en">changed by m4i: added german labels, added skos:prefLabel</skos:editorialNote>
        <skos:prefLabel xml:lang="de">realisierbare Entität</skos:prefLabel>
        <skos:prefLabel xml:lang="en">realizable entity</skos:prefLabel>
    </owl:Class>
    


    <!-- http://purl.org/spar/biro/BibliographicRecord -->


    <owl:Class rdf:about="http://purl.org/spar/biro/BibliographicRecord">
        <rdfs:comment xml:lang="en">A record that uniquely describes a particular textual or data publication (or a work in preparation for publication). Each bibliographic record is a set of entities describing aspects of the referenced work, including, for example, but not restricted to: authors, title, journal, publication year, DOI, ISSN, publisher and copyright information, or, in the case of a data publication: creators, title, version, archive, publication year, DOI or other identifier). The FRBR expression of a bibliographic record is a bibliographic reference, which usually contains only a sub-set of these entities, ordered in a particular way that corresponds to the house style of the publication in which it occurs.</rdfs:comment>
        <skos:editorialNote xml:lang="en">changed by m4i: added german labels, added skos:prefLabel</skos:editorialNote>
        <skos:prefLabel xml:lang="de">bibliografischer Eintrag</skos:prefLabel>
        <skos:prefLabel xml:lang="en">bibliographic record</skos:prefLabel>
    </owl:Class>
    


    <!-- http://qudt.org/schema/qudt/QuantityKind -->


    <owl:Class rdf:about="http://qudt.org/schema/qudt/QuantityKind">
        <rdfs:subClassOf rdf:resource="https://schema.org/Intangible"/>
        <rdfs:comment xml:lang="en">A &lt;b&gt;Quantity Kind&lt;/b&gt; is any observable property that can be  measured and quantified numerically. Familiar examples include physical properties such as length, mass, time, force, energy, power, electric charge, etc. Less familiar examples include currency, interest rate, price to earning ratio, and information capacity.</rdfs:comment>
        <skos:definition xml:lang="en">Kind of quantity, i.e., a physical/chemical quantity from a controlled vocabulary, such as QUDT, IEC, or EMMO</skos:definition>
        <skos:editorialNote xml:lang="en">changed by m4i: added german labels, added skos:prefLabel, harmonized spelling to OBO naming conventions (lower case, space separated)</skos:editorialNote>
        <skos:note xml:lang="en">we recommend using a persistent identifier resolving to a persistent URL</skos:note>
        <skos:prefLabel xml:lang="de">Größenart</skos:prefLabel>
        <skos:prefLabel xml:lang="en">quantity kind</skos:prefLabel>
    </owl:Class>
    


    <!-- http://qudt.org/schema/qudt/Unit -->


    <owl:Class rdf:about="http://qudt.org/schema/qudt/Unit">
        <rdfs:subClassOf rdf:resource="https://schema.org/Intangible"/>
        <skos:closeMatch rdf:resource="http://emmo.info/emmo#EMMO_b081b346_7279_46ef_9a3d_2c088fcd79f4"/>
        <skos:closeMatch rdf:resource="http://www.molmod.info/semantics/pims-ii.ttl#MeasurementUnit"/>
        <skos:definition xml:lang="en">A unit of measure, or unit is a particular quantity value that has been chosen as a scale for measuring other quantities the same kind (more generally of equivalent dimension). For example, the meter is a quantity of length that has been rigorously defined and standardized by the BIPM (International Board of Weights and Measures). Any measurement of the length can be expressed as a number multiplied by the unit meter. More formally, the value of physical quanitity Q with respect to a unit (U) is expressed as the scalar multiple of a real number (n) and U, as Q = nU.</skos:definition>
        <skos:editorialNote xml:lang="en">changed by m4i: added skos:prefLabel, added German label, harmonized spelling to OBO naming conventions (lower case, space separated)</skos:editorialNote>
        <skos:prefLabel xml:lang="de">Einheit</skos:prefLabel>
        <skos:prefLabel xml:lang="en">unit</skos:prefLabel>
    </owl:Class>
    


    <!-- http://w3id.org/nfdi4ing/metadata4ing#Method -->


    <owl:Class rdf:about="http://w3id.org/nfdi4ing/metadata4ing#Method">
        <rdfs:subClassOf rdf:resource="http://purl.obolibrary.org/obo/BFO_0000017"/>
        <skos:definition xml:lang="en">Abstract description of a method for analysis, generation and transformation of data and material objects like, e.g., &apos;Fourier Transform Infrared Spectroscopy&apos; or &apos;Molecular Dynamics Simulation&apos;. Note that while values for relevant parameters should be provided, m4i:Method does not refer to the actual execution of the process that is described (use m4i:ProcessingStep for that), but rather a description of the underlying principle.</skos:definition>
        <skos:prefLabel xml:lang="de">Methode</skos:prefLabel>
        <skos:prefLabel xml:lang="en">method</skos:prefLabel>
    </owl:Class>
    


    <!-- http://w3id.org/nfdi4ing/metadata4ing#NumericalAssignment -->


    <owl:Class rdf:about="http://w3id.org/nfdi4ing/metadata4ing#NumericalAssignment">
        <rdfs:subClassOf rdf:resource="http://www.molmod.info/semantics/pims-ii.ttl#Assignment"/>
        <rdfs:subClassOf>
            <owl:Restriction>
                <owl:onProperty>
                    <rdf:Description>
                        <owl:inverseOf rdf:resource="http://www.molmod.info/semantics/pims-ii.ttl#isValueInAssignment"/>
                    </rdf:Description>
                </owl:onProperty>
                <owl:someValuesFrom rdf:resource="https://ptb.de/si/Real"/>
            </owl:Restriction>
        </rdfs:subClassOf>
        <rdfs:subClassOf>
            <owl:Restriction>
                <owl:onProperty>
                    <rdf:Description>
                        <owl:inverseOf rdf:resource="http://www.molmod.info/semantics/pims-ii.ttl#isVariableInAssignment"/>
                    </rdf:Description>
                </owl:onProperty>
                <owl:minCardinality rdf:datatype="http://www.w3.org/2001/XMLSchema#nonNegativeInteger">1</owl:minCardinality>
            </owl:Restriction>
        </rdfs:subClassOf>
        <skos:definition xml:lang="en">Assignment by which a variable (e.g., a physical property) is assigned an si:Real quantity value (scalar x measurement unit) in some context (e.g., applied to some object of research)</skos:definition>
        <skos:prefLabel xml:lang="en">numerical assignment</skos:prefLabel>
        <skos:prefLabel xml:lang="de">numerische Zuweisung</skos:prefLabel>
    </owl:Class>
    


    <!-- http://w3id.org/nfdi4ing/metadata4ing#NumericalVariable -->


    <owl:Class rdf:about="http://w3id.org/nfdi4ing/metadata4ing#NumericalVariable">
        <rdfs:subClassOf rdf:resource="http://www.molmod.info/semantics/pims-ii.ttl#Variable"/>
        <skos:closeMatch rdf:resource="http://qudt.org/schema/qudt/Quantity"/>
        <skos:closeMatch rdf:resource="https://ptb.de/si/Real"/>
        <skos:definition xml:lang="en">A variable that expects a float or integer as a value</skos:definition>
        <skos:definition xml:lang="de">Eine Variable, die eine Zahl als Wert erwartet</skos:definition>
        <skos:prefLabel xml:lang="en">numerical variable</skos:prefLabel>
        <skos:prefLabel xml:lang="de">numerische Variable</skos:prefLabel>
    </owl:Class>
    


    <!-- http://w3id.org/nfdi4ing/metadata4ing#ProcessingStep -->


    <owl:Class rdf:about="http://w3id.org/nfdi4ing/metadata4ing#ProcessingStep">
        <rdfs:subClassOf rdf:resource="http://www.w3.org/ns/prov#Activity"/>
        <skos:definition xml:lang="en">Specific action undertaken during research</skos:definition>
        <skos:prefLabel xml:lang="de">Arbeitsschritt</skos:prefLabel>
        <skos:prefLabel xml:lang="en">processing step</skos:prefLabel>
    </owl:Class>
    


    <!-- http://w3id.org/nfdi4ing/metadata4ing#TextVariable -->


    <owl:Class rdf:about="http://w3id.org/nfdi4ing/metadata4ing#TextVariable">
        <rdfs:subClassOf rdf:resource="http://www.molmod.info/semantics/pims-ii.ttl#Variable"/>
        <skos:definition xml:lang="en">A variable that expects a string of characters as a value</skos:definition>
        <skos:definition xml:lang="de">Eine Variable, die eine Zeichenkette als Wert erwartet</skos:definition>
        <skos:prefLabel xml:lang="en">text variable</skos:prefLabel>
        <skos:prefLabel xml:lang="de">textbasierte Variable</skos:prefLabel>
    </owl:Class>
    


    <!-- http://w3id.org/nfdi4ing/metadata4ing#Tool -->


    <owl:Class rdf:about="http://w3id.org/nfdi4ing/metadata4ing#Tool">
        <skos:definition xml:lang="en">Object that helps an agent perform an action (e.g., John wrote a book with a pen), i.e., an object of the relation schema:instrument or m4i:hasTool</skos:definition>
        <skos:prefLabel xml:lang="de">Werkzeug</skos:prefLabel>
        <skos:prefLabel xml:lang="en">tool</skos:prefLabel>
    </owl:Class>
    


    <!-- http://w3id.org/nfdi4ing/metadata4ing#UncertaintyDeclaration -->


    <owl:Class rdf:about="http://w3id.org/nfdi4ing/metadata4ing#UncertaintyDeclaration">
        <rdfs:subClassOf rdf:resource="https://schema.org/Intangible"/>
        <skos:definition xml:lang="en">Declaration that can be applied to an si:Real quantity value to give an assessment of uncertainty</skos:definition>
        <skos:prefLabel xml:lang="de">Unsicherheitsdeklaration</skos:prefLabel>
        <skos:prefLabel xml:lang="en">uncertainty declaration</skos:prefLabel>
    </owl:Class>
    


    <!-- http://www.molmod.info/semantics/pims-ii.ttl#Assignment -->


    <owl:Class rdf:about="http://www.molmod.info/semantics/pims-ii.ttl#Assignment">
        <rdfs:subClassOf rdf:resource="https://schema.org/Intangible"/>
        <rdfs:subClassOf>
            <owl:Restriction>
                <owl:onProperty>
                    <rdf:Description>
                        <owl:inverseOf rdf:resource="http://www.molmod.info/semantics/pims-ii.ttl#isValueInAssignment"/>
                    </rdf:Description>
                </owl:onProperty>
                <owl:someValuesFrom rdf:resource="http://www.molmod.info/semantics/pims-ii.ttl#Value"/>
            </owl:Restriction>
        </rdfs:subClassOf>
        <rdfs:subClassOf>
            <owl:Restriction>
                <owl:onProperty>
                    <rdf:Description>
                        <owl:inverseOf rdf:resource="http://www.molmod.info/semantics/pims-ii.ttl#isVariableInAssignment"/>
                    </rdf:Description>
                </owl:onProperty>
                <owl:someValuesFrom rdf:resource="http://www.molmod.info/semantics/pims-ii.ttl#Variable"/>
            </owl:Restriction>
        </rdfs:subClassOf>
        <rdfs:subClassOf>
            <owl:Restriction>
                <owl:onProperty rdf:resource="http://www.molmod.info/semantics/pims-ii.ttl#isAssignmentFor"/>
                <owl:minCardinality rdf:datatype="http://www.w3.org/2001/XMLSchema#nonNegativeInteger">1</owl:minCardinality>
            </owl:Restriction>
        </rdfs:subClassOf>
        <rdfs:comment xml:lang="en">Assignment, i.e., a data item by which a value is assigned to a variable with respect to a particular referent (e.g., T = 200 K for substance o as it was measured in a particular cognitive step); therein, T is the variable, related to the assignment by m4i:hasVariable, 200 K is the value, related to the assignment by m4i:hasValue, and o is the referent, related to the assignment by isAssignmentFor</rdfs:comment>
        <skos:editorialNote>changed by m4i: added skos:prefLabel, adjusted german labels,  harmonized spelling to OBO naming conventions (lower case, space separated)</skos:editorialNote>
        <skos:prefLabel xml:lang="de">Zuweisung</skos:prefLabel>
        <skos:prefLabel xml:lang="en">assignment</skos:prefLabel>
    </owl:Class>
    


    <!-- http://www.molmod.info/semantics/pims-ii.ttl#Property -->


    <owl:Class rdf:about="http://www.molmod.info/semantics/pims-ii.ttl#Property">
        <rdfs:subClassOf rdf:resource="http://www.molmod.info/semantics/pims-ii.ttl#Variable"/>
        <skos:broader rdf:resource="http://purl.obolibrary.org/obo/BFO_0000020"/>
        <skos:closeMatch rdf:resource="http://emmo.info/emmo#EMMO_b7bcff25_ffc3_474e_9ab5_01b1664bd4ba"/>
        <skos:definition xml:lang="en">Property, i.e., a variable that can be considered (as an investigated property, i.e., target property) within a processing step</skos:definition>
        <skos:editorialNote>changed by m4i: added skos:prefLabel, adjusted german labels, harmonized spelling to OBO naming conventions (lower case, space separated)</skos:editorialNote>
        <skos:prefLabel xml:lang="de">Eigenschaft</skos:prefLabel>
        <skos:prefLabel xml:lang="en">property</skos:prefLabel>
    </owl:Class>
    


    <!-- http://www.molmod.info/semantics/pims-ii.ttl#QuantityValue -->


    <owl:Class rdf:about="http://www.molmod.info/semantics/pims-ii.ttl#QuantityValue">
        <rdfs:subClassOf rdf:resource="http://www.molmod.info/semantics/pims-ii.ttl#Value"/>
        <skos:definition xml:lang="en">Quantity value, i.e., a value that has a numerical magnitude and a physical unit</skos:definition>
        <skos:editorialNote>changed by m4i: added skos:prefLabel, adjusted german labels, harmonized spelling to OBO naming conventions (lower case, space separated)</skos:editorialNote>
        <skos:prefLabel xml:lang="de">Größenwert</skos:prefLabel>
        <skos:prefLabel xml:lang="en">quantity value</skos:prefLabel>
    </owl:Class>
    


    <!-- http://www.molmod.info/semantics/pims-ii.ttl#Value -->


    <owl:Class rdf:about="http://www.molmod.info/semantics/pims-ii.ttl#Value">
        <rdfs:subClassOf rdf:resource="https://schema.org/Intangible"/>
        <rdfs:subClassOf>
            <owl:Restriction>
                <owl:onProperty rdf:resource="http://www.molmod.info/semantics/pims-ii.ttl#isAdmissibleValueFor"/>
                <owl:minCardinality rdf:datatype="http://www.w3.org/2001/XMLSchema#nonNegativeInteger">1</owl:minCardinality>
            </owl:Restriction>
        </rdfs:subClassOf>
        <skos:definition xml:lang="en">Value, i.e., an articulation that is by social convention understood to be potentially assignable to a variable</skos:definition>
        <skos:editorialNote>changed by m4i: added skos:prefLabel, adjusted german labels, harmonized spelling to OBO naming conventions (lower case, space separated)</skos:editorialNote>
        <skos:prefLabel xml:lang="de">Wert</skos:prefLabel>
        <skos:prefLabel xml:lang="en">value</skos:prefLabel>
    </owl:Class>
    


    <!-- http://www.molmod.info/semantics/pims-ii.ttl#Variable -->


    <owl:Class rdf:about="http://www.molmod.info/semantics/pims-ii.ttl#Variable">
        <owl:equivalentClass>
            <owl:Restriction>
                <owl:onProperty>
                    <rdf:Description>
                        <owl:inverseOf rdf:resource="http://www.molmod.info/semantics/pims-ii.ttl#isAdmissibleValueFor"/>
                    </rdf:Description>
                </owl:onProperty>
                <owl:someValuesFrom rdf:resource="http://www.molmod.info/semantics/pims-ii.ttl#Value"/>
            </owl:Restriction>
        </owl:equivalentClass>
        <rdfs:subClassOf rdf:resource="https://schema.org/Intangible"/>
        <skos:closeMatch rdf:resource="http://emmo.info/emmo#EMMO_1eed0732_e3f1_4b2c_a9c4_b4e75eeb5895"/>
        <skos:definition xml:lang="en">Variable, i.e., a conventional that is employed for something to which values can be assigned (this may include different notations for the same variable including, e.g., computational representations); this is to be understood very generally, e.g., a variable may be an array or set of elements or have another kind of internal structure</skos:definition>
        <skos:editorialNote>changed by m4i: added skos:prefLabel, adjusted german labels, harmonized spelling to OBO naming conventions (lower case, space separated)</skos:editorialNote>
        <skos:prefLabel xml:lang="de">Variable</skos:prefLabel>
        <skos:prefLabel xml:lang="en">variable</skos:prefLabel>
    </owl:Class>
    


    <!-- http://www.w3.org/ns/dcat#Dataset -->


    <owl:Class rdf:about="http://www.w3.org/ns/dcat#Dataset">
        <rdfs:comment xml:lang="en">A collection of data, published or curated by a single source, and available for access or download in one or more representations.</rdfs:comment>
        <rdfs:isDefinedBy rdf:resource="http://www.w3.org/ns/dcat#"/>
        <skos:editorialNote xml:lang="en">changed by m4i: added skos:prefLabel, added german labels, removed redundant notes, removed other languages than english in comment, label, changeNote and definition</skos:editorialNote>
        <skos:prefLabel xml:lang="de">Datensatz</skos:prefLabel>
        <skos:prefLabel xml:lang="en">dataset</skos:prefLabel>
        <skos:scopeNote xml:lang="en">The notion of dataset in DCAT is broad and inclusive, with the intention of accommodating resource types arising from all communities. Data comes in many forms including numbers, text, pixels, imagery, sound and other multi-media, and potentially other types, any of which might be collected into a dataset.</skos:scopeNote>
        <skos:scopeNote xml:lang="en">This class describes the conceptual dataset. One or more representations might be available, with differing schematic layouts and formats or serializations.</skos:scopeNote>
    </owl:Class>
    


    <!-- http://www.w3.org/ns/dcat#DatasetSeries -->


    <owl:Class rdf:about="http://www.w3.org/ns/dcat#DatasetSeries">
        <rdfs:subClassOf rdf:resource="http://www.w3.org/ns/dcat#Dataset"/>
        <rdfs:isDefinedBy rdf:resource="http://www.w3.org/ns/dcat#"/>
        <skos:definition xml:lang="en">A collection of datasets that are published separately, but share some common characteristics that groups them.</skos:definition>
        <skos:editorialNote xml:lang="en">changed by m4i: added skos:prefLabel, added german labels, removed redundant notes, extracted from DCAT3-Documentation https://www.w3.org/TR/vocab-dcat-3/#Class:Dataset_Series</skos:editorialNote>
        <skos:prefLabel xml:lang="de">Datensatzserie</skos:prefLabel>
        <skos:prefLabel xml:lang="en">dataset series</skos:prefLabel>
    </owl:Class>
    


    <!-- http://www.w3.org/ns/dcat#Distribution -->


    <owl:Class rdf:about="http://www.w3.org/ns/dcat#Distribution">
        <rdfs:isDefinedBy rdf:resource="http://www.w3.org/ns/dcat#"/>
        <skos:definition xml:lang="en">A specific representation of a dataset. A dataset might be available in multiple serializations that may differ in various ways, including natural language, media-type or format, schematic organization, temporal and spatial resolution, level of detail or profiles (which might specify any or all of the above).</skos:definition>
        <skos:editorialNote xml:lang="en">changed by m4i: added skos:prefLabel, added german labels, removed redundant notes, removed other languages than english in comment, label, changeNote and definition</skos:editorialNote>
        <skos:prefLabel xml:lang="de">Verteilung</skos:prefLabel>
        <skos:prefLabel xml:lang="en">distribution</skos:prefLabel>
    </owl:Class>
    


    <!-- http://www.w3.org/ns/prov#Activity -->


    <owl:Class rdf:about="http://www.w3.org/ns/prov#Activity">
        <rdfs:subClassOf rdf:resource="http://purl.obolibrary.org/obo/BFO_0000015"/>
        <skos:closeMatch rdf:resource="http://www.molmod.info/semantics/pims-ii.ttl#Action"/>
        <skos:definition xml:lang="en">An activity is something that occurs over a period of time and acts upon or with entities; it may include consuming, processing, transforming, modifying, relocating, using, or generating entities.</skos:definition>
        <skos:definition xml:lang="de">Eine Aktivität ist etwas, das über einen Zeitraum und mit oder an Entitäten erfolgt; dazu kann das Verbrauchen, Verarbeiten, Transformieren, Modifizieren, Relokalisieren, Verwenden, oder die Genese von Entitäten gehören.</skos:definition>
        <skos:editorialNote xml:lang="en">changed by m4i: added skos:prefLabel, added german label, harmonized spelling to OBO naming conventions (lower case, space separated)</skos:editorialNote>
        <skos:prefLabel xml:lang="de">Aktivität</skos:prefLabel>
        <skos:prefLabel xml:lang="en">activity</skos:prefLabel>
    </owl:Class>
    


    <!-- http://www.w3.org/ns/prov#Agent -->


    <owl:Class rdf:about="http://www.w3.org/ns/prov#Agent">
        <rdfs:isDefinedBy rdf:resource="http://www.w3.org/ns/prov#"/>
        <skos:definition xml:lang="en">An agent is something that bears some form of responsibility for an activity taking place, for the existence of an entity, or for another agent&apos;s activity.</skos:definition>
        <skos:editorialNote xml:lang="en">changed by m4i: added german labels, added skos:prefLabel, added skos:definition, added german definition, added instances</skos:editorialNote>
        <skos:prefLabel xml:lang="de">Akteur</skos:prefLabel>
        <skos:prefLabel xml:lang="en">agent</skos:prefLabel>
    </owl:Class>
    


    <!-- http://www.w3.org/ns/prov#Association -->


    <owl:Class rdf:about="http://www.w3.org/ns/prov#Association">
        <rdfs:comment xml:lang="en">An instance of prov:Association provides additional descriptions about the binary prov:wasAssociatedWith relation from an prov:Activity to some prov:Agent that had some responsiblity for it. For example, :baking prov:wasAssociatedWith :baker; prov:qualifiedssociation [ a prov:Association; prov:agent :baker; :foo :bar ].</rdfs:comment>
        <skos:editorialNote xml:lang="en">changed by m4i: harmonized spelling to OBO naming conventions (lower case, space separated)</skos:editorialNote>
        <skos:prefLabel xml:lang="de">Verknüpfung</skos:prefLabel>
        <skos:prefLabel xml:lang="en">association</skos:prefLabel>
    </owl:Class>
    


    <!-- http://www.w3.org/ns/prov#Organization -->


    <owl:Class rdf:about="http://www.w3.org/ns/prov#Organization">
        <rdfs:subClassOf rdf:resource="http://www.w3.org/ns/prov#Agent"/>
        <rdfs:isDefinedBy rdf:resource="http://www.w3.org/ns/prov#"/>
        <skos:definition xml:lang="en">An organization is a social or legal institution such as a company, society, etc.</skos:definition>
        <skos:definition xml:lang="de">Eine Organisation ist eine soziale oder rechtliche Institution wie ein Unternehmen, ein Verein usw.</skos:definition>
        <skos:editorialNote xml:lang="en">changed by m4i: added german labels, added skos:prefLabel, added skos:definition, added german definition, added instances</skos:editorialNote>
        <skos:prefLabel xml:lang="de">Organisation</skos:prefLabel>
        <skos:prefLabel xml:lang="en">organization</skos:prefLabel>
    </owl:Class>
    


    <!-- http://www.w3.org/ns/prov#Person -->


    <owl:Class rdf:about="http://www.w3.org/ns/prov#Person">
        <rdfs:subClassOf rdf:resource="http://www.w3.org/ns/prov#Agent"/>
        <rdfs:isDefinedBy rdf:resource="http://www.w3.org/ns/prov#"/>
        <skos:definition xml:lang="de">Eine Person als Akteur ist eine natürliche Person, also ein handelnder Mensch.</skos:definition>
        <skos:definition xml:lang="en">Person agents are people.</skos:definition>
        <skos:editorialNote xml:lang="en">changed by m4i: added german labels, added skos:prefLabel, added skos:definition, added german definition, added instances</skos:editorialNote>
        <skos:prefLabel xml:lang="de">Person</skos:prefLabel>
        <skos:prefLabel xml:lang="en">person</skos:prefLabel>
    </owl:Class>
    


    <!-- http://www.w3.org/ns/prov#Role -->


    <owl:Class rdf:about="http://www.w3.org/ns/prov#Role">
        <rdfs:isDefinedBy rdf:resource="http://www.w3.org/ns/prov#"/>
        <skos:definition xml:lang="en">A role is the function of an entity or agent with respect to an activity, in the context of a usage, generation, invalidation, association, start, and end.</skos:definition>
        <skos:editorialNote xml:lang="en">changed by m4i: added german labels, added skos:prefLabel, added skos:definition, added german definition, added instances, harmonized spelling to OBO naming conventions (lower case, space separated)</skos:editorialNote>
        <skos:prefLabel xml:lang="de">Rolle des Akteurs</skos:prefLabel>
        <skos:prefLabel xml:lang="en">role</skos:prefLabel>
    </owl:Class>
    


    <!-- http://www.w3.org/ns/prov#SoftwareAgent -->


    <owl:Class rdf:about="http://www.w3.org/ns/prov#SoftwareAgent">
        <rdfs:subClassOf rdf:resource="http://www.w3.org/ns/prov#Agent"/>
        <rdfs:isDefinedBy rdf:resource="http://www.w3.org/ns/prov#"/>
        <skos:definition xml:lang="en">A software agent is running software.</skos:definition>
        <skos:definition xml:lang="de">Ein Software als Akteur ist ein Stück laufender Programmcode, der eine Aufgabe in einem Prozess übernimmt.</skos:definition>
        <skos:editorialNote xml:lang="en">changed by m4i: added german labels, added skos:prefLabel, added skos:definition, added german definition, added instances</skos:editorialNote>
        <skos:prefLabel xml:lang="de">Software-Akteur</skos:prefLabel>
        <skos:prefLabel xml:lang="en">software agent</skos:prefLabel>
    </owl:Class>
    


    <!-- http://xmlns.com/foaf/0.1/Agent -->


    <owl:Class rdf:about="http://xmlns.com/foaf/0.1/Agent">
        <rdfs:comment>DEPRECATED An agent (eg. person, group, software or physical artifact).</rdfs:comment>
        <rdfs:comment>exchanged foaf:Agent by prov:Agent to fulfill range definition of prov:agent property</rdfs:comment>
        <rdfs:seeAlso rdf:resource="http://www.w3.org/ns/prov#Agent"/>
        <owl:deprecated rdf:datatype="http://www.w3.org/2001/XMLSchema#boolean">true</owl:deprecated>
    </owl:Class>
    


    <!-- http://xmlns.com/foaf/0.1/Group -->


    <owl:Class rdf:about="http://xmlns.com/foaf/0.1/Group">
        <rdfs:subClassOf rdf:resource="http://xmlns.com/foaf/0.1/Agent"/>
        <rdfs:comment>DEPRECATED A class of Agents.</rdfs:comment>
        <rdfs:comment>Remove foaf:Group, use prov:Organization instead</rdfs:comment>
        <rdfs:seeAlso rdf:resource="http://www.w3.org/ns/prov#Organization"/>
        <owl:deprecated rdf:datatype="http://www.w3.org/2001/XMLSchema#boolean">true</owl:deprecated>
    </owl:Class>
    


    <!-- http://xmlns.com/foaf/0.1/Organization -->


    <owl:Class rdf:about="http://xmlns.com/foaf/0.1/Organization">
        <rdfs:subClassOf rdf:resource="http://xmlns.com/foaf/0.1/Agent"/>
        <rdfs:comment>DEPRECATED An organization.</rdfs:comment>
        <rdfs:comment>Replace foaf:Organization by prov:Organization</rdfs:comment>
        <rdfs:seeAlso rdf:resource="http://www.w3.org/ns/prov#Organization"/>
        <owl:deprecated rdf:datatype="http://www.w3.org/2001/XMLSchema#boolean">true</owl:deprecated>
    </owl:Class>
    


    <!-- http://xmlns.com/foaf/0.1/Person -->


    <owl:Class rdf:about="http://xmlns.com/foaf/0.1/Person">
        <rdfs:subClassOf rdf:resource="http://xmlns.com/foaf/0.1/Agent"/>
        <rdfs:comment>DEPRECATED A person.</rdfs:comment>
        <rdfs:comment>Replace foaf:Person by prov:Person</rdfs:comment>
        <rdfs:seeAlso rdf:resource="http://www.w3.org/ns/prov#Person"/>
        <owl:deprecated rdf:datatype="http://www.w3.org/2001/XMLSchema#boolean">true</owl:deprecated>
    </owl:Class>
    


    <!-- https://ptb.de/si/CoverageInterval -->


    <owl:Class rdf:about="https://ptb.de/si/CoverageInterval">
        <rdfs:subClassOf rdf:resource="http://w3id.org/nfdi4ing/metadata4ing#UncertaintyDeclaration"/>
        <rdfs:subClassOf>
            <owl:Restriction>
                <owl:onProperty rdf:resource="https://ptb.de/si/hasCoverageProbability"/>
                <owl:cardinality rdf:datatype="http://www.w3.org/2001/XMLSchema#nonNegativeInteger">1</owl:cardinality>
            </owl:Restriction>
        </rdfs:subClassOf>
        <rdfs:subClassOf>
            <owl:Restriction>
                <owl:onProperty rdf:resource="https://ptb.de/si/hasIntervalMax"/>
                <owl:cardinality rdf:datatype="http://www.w3.org/2001/XMLSchema#nonNegativeInteger">1</owl:cardinality>
            </owl:Restriction>
        </rdfs:subClassOf>
        <rdfs:subClassOf>
            <owl:Restriction>
                <owl:onProperty rdf:resource="https://ptb.de/si/hasIntervalMin"/>
                <owl:cardinality rdf:datatype="http://www.w3.org/2001/XMLSchema#nonNegativeInteger">1</owl:cardinality>
            </owl:Restriction>
        </rdfs:subClassOf>
        <rdfs:subClassOf>
            <owl:Restriction>
                <owl:onProperty rdf:resource="https://ptb.de/si/hasStandardUnc"/>
                <owl:cardinality rdf:datatype="http://www.w3.org/2001/XMLSchema#nonNegativeInteger">1</owl:cardinality>
            </owl:Restriction>
        </rdfs:subClassOf>
        <rdfs:subClassOf>
            <owl:Restriction>
                <owl:onProperty rdf:resource="https://ptb.de/si/hasDistribution"/>
                <owl:maxCardinality rdf:datatype="http://www.w3.org/2001/XMLSchema#nonNegativeInteger">1</owl:maxCardinality>
            </owl:Restriction>
        </rdfs:subClassOf>
        <skos:definition xml:lang="en">Structure for stating a probabilistic-symmetric coverage interval for a real uncertainty, to be applied to an si:Real quantity value</skos:definition>
        <skos:editorialNote>changed by m4i: harmonized spelling to OBO naming conventions (lower case, space separated), added skos:prefLabel</skos:editorialNote>
        <skos:prefLabel xml:lang="en">coverage interval</skos:prefLabel>
        <skos:prefLabel xml:lang="de">Überdeckungsintervall</skos:prefLabel>
    </owl:Class>
    


    <!-- https://ptb.de/si/ExpandedUnc -->


    <owl:Class rdf:about="https://ptb.de/si/ExpandedUnc">
        <rdfs:subClassOf rdf:resource="http://w3id.org/nfdi4ing/metadata4ing#UncertaintyDeclaration"/>
        <rdfs:subClassOf>
            <owl:Restriction>
                <owl:onProperty rdf:resource="https://ptb.de/si/hasCoverageFactor"/>
                <owl:cardinality rdf:datatype="http://www.w3.org/2001/XMLSchema#nonNegativeInteger">1</owl:cardinality>
            </owl:Restriction>
        </rdfs:subClassOf>
        <rdfs:subClassOf>
            <owl:Restriction>
                <owl:onProperty rdf:resource="https://ptb.de/si/hasCoverageProbability"/>
                <owl:cardinality rdf:datatype="http://www.w3.org/2001/XMLSchema#nonNegativeInteger">1</owl:cardinality>
            </owl:Restriction>
        </rdfs:subClassOf>
        <rdfs:subClassOf>
            <owl:Restriction>
                <owl:onProperty rdf:resource="https://ptb.de/si/hasUncertainty"/>
                <owl:cardinality rdf:datatype="http://www.w3.org/2001/XMLSchema#nonNegativeInteger">1</owl:cardinality>
            </owl:Restriction>
        </rdfs:subClassOf>
        <rdfs:subClassOf>
            <owl:Restriction>
                <owl:onProperty rdf:resource="https://ptb.de/si/hasDistribution"/>
                <owl:maxCardinality rdf:datatype="http://www.w3.org/2001/XMLSchema#nonNegativeInteger">1</owl:maxCardinality>
            </owl:Restriction>
        </rdfs:subClassOf>
        <skos:definition xml:lang="en">Structure for stating an expanded measurement, model, or simulation uncertainty, e.g., to be applied to an si:Real quantity value</skos:definition>
        <skos:editorialNote>changed by m4i: harmonized spelling to OBO naming conventions (lower case, space separated), added skos:prefLabel</skos:editorialNote>
        <skos:prefLabel xml:lang="de">erweiterte Unsicherheit</skos:prefLabel>
        <skos:prefLabel xml:lang="en">expanded uncertainty</skos:prefLabel>
    </owl:Class>
    


    <!-- https://ptb.de/si/Real -->


    <owl:Class rdf:about="https://ptb.de/si/Real">
        <rdfs:subClassOf rdf:resource="http://www.molmod.info/semantics/pims-ii.ttl#QuantityValue"/>
        <rdfs:subClassOf>
            <owl:Restriction>
                <owl:onProperty rdf:resource="http://w3id.org/nfdi4ing/metadata4ing#hasUncertaintyDeclaration"/>
                <owl:cardinality rdf:datatype="http://www.w3.org/2001/XMLSchema#nonNegativeInteger">1</owl:cardinality>
            </owl:Restriction>
        </rdfs:subClassOf>
        <rdfs:subClassOf>
            <owl:Restriction>
                <owl:onProperty rdf:resource="http://w3id.org/nfdi4ing/metadata4ing#hasNumericalValue"/>
                <owl:cardinality rdf:datatype="http://www.w3.org/2001/XMLSchema#nonNegativeInteger">1</owl:cardinality>
            </owl:Restriction>
        </rdfs:subClassOf>
        <skos:definition xml:lang="en">(Real value +- uncertainty) x measurement unit, i.e., a scalar value with a measurement unit and an uncertainty indication</skos:definition>
        <skos:editorialNote>changed by m4i: harmonized spelling to OBO naming conventions (lower case, space separated), added skos:prefLabel</skos:editorialNote>
        <skos:prefLabel xml:lang="de">Reell</skos:prefLabel>
        <skos:prefLabel xml:lang="en">real</skos:prefLabel>
    </owl:Class>
    


    <!-- https://schema.org/Intangible -->


    <owl:Class rdf:about="https://schema.org/Intangible">
        <skos:definition xml:lang="en">A utility class that serves as the umbrella for a number of &apos;intangible&apos; things such as quantities, structured values, etc.</skos:definition>
        <skos:editorialNote xml:lang="en">changed by m4i: added skos:prefLabel, added german label, harmonized spelling to OBO naming conventions (lower case, space separated)</skos:editorialNote>
        <skos:prefLabel xml:lang="de">Ungreifbares</skos:prefLabel>
        <skos:prefLabel xml:lang="en">intangible</skos:prefLabel>
    </owl:Class>
    


    <!-- https://schema.org/Project -->


    <owl:Class rdf:about="https://schema.org/Project">
        <rdfs:comment xml:lang="en">An enterprise (potentially individual but typically collaborative), planned to achieve a particular aim</rdfs:comment>
        <rdfs:comment xml:lang="de">Ein typischerweise kollektives Unterfangen zum Erreichen eines vorab geplanten Ziels</rdfs:comment>
        <skos:editorialNote xml:lang="en">changed by m4i: added German definition, added language tag to English definition, shortened definition</skos:editorialNote>
        <skos:editorialNote xml:lang="en">changed by m4i: use of skos:prefLabel instead of rdfs:label, added German label, added language tag to English label, harmonized spelling to OBO naming conventions (lower case, space separated)</skos:editorialNote>
        <skos:prefLabel xml:lang="de">Projekt</skos:prefLabel>
        <skos:prefLabel xml:lang="en">project</skos:prefLabel>
    </owl:Class>
    


    <!-- https://schema.org/ResearchProject -->


    <owl:Class rdf:about="https://schema.org/ResearchProject">
        <rdfs:subClassOf rdf:resource="https://schema.org/Project"/>
        <rdfs:comment xml:lang="en">A research project</rdfs:comment>
        <rdfs:comment xml:lang="de">ein Forschungsprojekt</rdfs:comment>
        <skos:editorialNote xml:lang="en">changed by m4i: added German definition, added language tag to English definition</skos:editorialNote>
        <skos:editorialNote xml:lang="en">changed by m4i: changed label to &quot;research project&quot; (no CamelCase)</skos:editorialNote>
        <skos:editorialNote xml:lang="en">changed by m4i: use of skos:prefLabel instead of rdfs:label, added German label, added language tag to English label</skos:editorialNote>
        <skos:prefLabel xml:lang="de">Forschungsprojekt</skos:prefLabel>
        <skos:prefLabel xml:lang="en">research project</skos:prefLabel>
    </owl:Class>
    


    <!-- 
    ///////////////////////////////////////////////////////////////////////////////////////
    //
    // Individuals
    //
    ///////////////////////////////////////////////////////////////////////////////////////
     -->


    


    <!-- http://w3id.org/nfdi4ing/metadata4ing#ContactPerson -->


    <owl:NamedIndividual rdf:about="http://w3id.org/nfdi4ing/metadata4ing#ContactPerson">
        <rdf:type rdf:resource="http://www.w3.org/ns/prov#Role"/>
        <rdfs:seeAlso rdf:datatype="http://www.w3.org/2001/XMLSchema#anyURI">https://schema.datacite.org/meta/kernel-4.4/doc/DataCite-MetadataKernel_v4.4.pdf#page=40</rdfs:seeAlso>
        <skos:definition xml:lang="en">Person with knowledge of how to access, troubleshoot, or otherwise field issues related to the resource</skos:definition>
        <skos:prefLabel xml:lang="de">Kontaktperson</skos:prefLabel>
        <skos:prefLabel xml:lang="en">contact person</skos:prefLabel>
        <skos:scopeNote xml:lang="en">May also be the &quot;Point of Contact&quot; in an organisation that controls access to the resource, if that organisation is different from the Publisher, Distributor, and Data Manager.</skos:scopeNote>
    </owl:NamedIndividual>
    


    <!-- http://w3id.org/nfdi4ing/metadata4ing#DataCollector -->


    <owl:NamedIndividual rdf:about="http://w3id.org/nfdi4ing/metadata4ing#DataCollector">
        <rdf:type rdf:resource="http://www.w3.org/ns/prov#Role"/>
        <rdfs:seeAlso rdf:datatype="http://www.w3.org/2001/XMLSchema#anyURI">https://schema.datacite.org/meta/kernel-4.4/doc/DataCite-MetadataKernel_v4.4.pdf#page=40</rdfs:seeAlso>
        <skos:definition xml:lang="en">Person/institution responsible for finding or gathering/collecting data under the guidelines of the author(s) or Principal Investigator (PI)</skos:definition>
        <skos:prefLabel xml:lang="de">Datenerfasser*in</skos:prefLabel>
        <skos:prefLabel xml:lang="en">data collector</skos:prefLabel>
        <skos:scopeNote xml:lang="en">May also be used when crediting survey conductors, interviewers, event or condition observers, or persons responsible for monitoring key instrument data.</skos:scopeNote>
    </owl:NamedIndividual>
    


    <!-- http://w3id.org/nfdi4ing/metadata4ing#DataCurator -->


    <owl:NamedIndividual rdf:about="http://w3id.org/nfdi4ing/metadata4ing#DataCurator">
        <rdf:type rdf:resource="http://www.w3.org/ns/prov#Role"/>
        <rdfs:seeAlso rdf:datatype="http://www.w3.org/2001/XMLSchema#anyURI">https://schema.datacite.org/meta/kernel-4.4/doc/DataCite-MetadataKernel_v4.4.pdf#page=40</rdfs:seeAlso>
        <skos:definition xml:lang="en">Person tasked with reviewing, enhancing, cleaning, or standardizing metadata and the associated data submitted for storage, use, and maintenance within a data centre or repository</skos:definition>
        <skos:prefLabel xml:lang="de">Datenkurator*in</skos:prefLabel>
        <skos:prefLabel xml:lang="en">data curator</skos:prefLabel>
        <skos:scopeNote xml:lang="en">While the DataManager is concerned with digital maintenance, the DataCurator&apos;s role encompasses quality assurance focused on content and metadata. DataCurator responsibilities include: checking completeness of the submitted dataset against the content as described by the submitter; verifying standard metadata according to the applicable system or schema; adding or verifying specialized metadata to add value and ensure access across disciplines; and determining how the metadata might map to search engines, database products, and automated feeds. Repository managers as well as data librarians working in the repository fall within this category. 

Example: https://doi.org/10.20375/0000-000D-1D1F-2</skos:scopeNote>
    </owl:NamedIndividual>
    


    <!-- http://w3id.org/nfdi4ing/metadata4ing#DataManager -->


    <owl:NamedIndividual rdf:about="http://w3id.org/nfdi4ing/metadata4ing#DataManager">
        <rdf:type rdf:resource="http://www.w3.org/ns/prov#Role"/>
        <rdfs:seeAlso rdf:datatype="http://www.w3.org/2001/XMLSchema#anyURI">https://schema.datacite.org/meta/kernel-4.4/doc/DataCite-MetadataKernel_v4.4.pdf#page=40</rdfs:seeAlso>
        <skos:definition xml:lang="en">Person (or organisation with a staff of data managers, such as a data centre) responsible for maintaining the finished resource</skos:definition>
        <skos:prefLabel xml:lang="de">Datenverwalter*in</skos:prefLabel>
        <skos:prefLabel xml:lang="en">data manager</skos:prefLabel>
        <skos:scopeNote xml:lang="en">The work done by this person or organisation ensures that the resource is periodically &quot;refreshed&quot; in terms of software/hardware support, is kept available or is protected from unauthorized access, is stored in accordance with industry standards, and is handled in accordance with the records management requirements applicable to it.

Example: https://doi.org/10.6073/pasta/41b3ed2e152e1e4c3846e646118208e7</skos:scopeNote>
    </owl:NamedIndividual>
    


    <!-- http://w3id.org/nfdi4ing/metadata4ing#Distributor -->


    <owl:NamedIndividual rdf:about="http://w3id.org/nfdi4ing/metadata4ing#Distributor">
        <rdf:type rdf:resource="http://www.w3.org/ns/prov#Role"/>
        <rdfs:seeAlso rdf:datatype="http://www.w3.org/2001/XMLSchema#anyURI">https://schema.datacite.org/meta/kernel-4.4/doc/DataCite-MetadataKernel_v4.4.pdf#page=40</rdfs:seeAlso>
        <skos:definition xml:lang="en">Institution tasked with responsibility to generate/disseminate copies of the resource in either electronic or print form</skos:definition>
        <skos:prefLabel xml:lang="de">Anbieter*in</skos:prefLabel>
        <skos:prefLabel xml:lang="en">distributor</skos:prefLabel>
        <skos:scopeNote xml:lang="en">Works stored in more than one archive/repository may credit each as a distributor.</skos:scopeNote>
    </owl:NamedIndividual>
    


    <!-- http://w3id.org/nfdi4ing/metadata4ing#Editor -->


    <owl:NamedIndividual rdf:about="http://w3id.org/nfdi4ing/metadata4ing#Editor">
        <rdf:type rdf:resource="http://www.w3.org/ns/prov#Role"/>
        <rdfs:seeAlso rdf:datatype="http://www.w3.org/2001/XMLSchema#anyURI">https://schema.datacite.org/meta/kernel-4.4/doc/DataCite-MetadataKernel_v4.4.pdf#page=40</rdfs:seeAlso>
        <skos:definition xml:lang="en">A person who oversees the details related to the publication format of the resource</skos:definition>
        <skos:prefLabel xml:lang="de">Herausgeber*in</skos:prefLabel>
        <skos:prefLabel xml:lang="en">editor</skos:prefLabel>
        <skos:scopeNote xml:lang="en">Note: if the Editor is to be credited in place of multiple creators, the Editor&apos;s name may be supplied as Creator, with &quot;(Ed.)&quot; appended to the name.</skos:scopeNote>
    </owl:NamedIndividual>
    


    <!-- http://w3id.org/nfdi4ing/metadata4ing#HostingInstitution -->


    <owl:NamedIndividual rdf:about="http://w3id.org/nfdi4ing/metadata4ing#HostingInstitution">
        <rdf:type rdf:resource="http://www.w3.org/ns/prov#Role"/>
        <rdfs:seeAlso rdf:datatype="http://www.w3.org/2001/XMLSchema#anyURI">https://schema.datacite.org/meta/kernel-4.4/doc/DataCite-MetadataKernel_v4.4.pdf#page=40</rdfs:seeAlso>
        <skos:definition xml:lang="en">Typically, the organisation allowing the resource to be available on the internet through the provision of its hardware/software/operating support</skos:definition>
        <skos:prefLabel xml:lang="de">bereitstellende Institution</skos:prefLabel>
        <skos:prefLabel xml:lang="en">hosting institution</skos:prefLabel>
        <skos:scopeNote xml:lang="en">This role normally falls on the University, research center or organization where the data center/data repository belongs.

EXAMPLE: Université Grenoble Alpes (UGA)

May also be used for an organisation that stores the data offline-often a data centre if that data centre is not the &quot;publisher&quot; of the resource.</skos:scopeNote>
    </owl:NamedIndividual>
    


    <!-- http://w3id.org/nfdi4ing/metadata4ing#Other -->


    <owl:NamedIndividual rdf:about="http://w3id.org/nfdi4ing/metadata4ing#Other">
        <rdf:type rdf:resource="http://www.w3.org/ns/prov#Role"/>
        <rdfs:seeAlso rdf:datatype="http://www.w3.org/2001/XMLSchema#anyURI">https://schema.datacite.org/meta/kernel-4.4/doc/DataCite-MetadataKernel_v4.4.pdf#page=40</rdfs:seeAlso>
        <skos:definition xml:lang="en">Any person or institution making a significant contribution to the development and/or maintenance of the resource, but whose contribution is notadequately described by any of the other values for contributorType</skos:definition>
        <skos:editorialNote>Label adjusted. Do we really need to define all these person roles in our ontology? (GIACOMO)</skos:editorialNote>
        <skos:prefLabel xml:lang="en">other person</skos:prefLabel>
        <skos:prefLabel xml:lang="de">weitere Person</skos:prefLabel>
        <skos:scopeNote xml:lang="en">Could be a photographer, artist, or writer whose contribution helped to publicize the resource (as opposed to creating it), a reviewer of the resource, someone providing administrative services to the author (such as depositing updates into an online repository, analysing usage, etc.), or one of many other roles.</skos:scopeNote>
    </owl:NamedIndividual>
    


    <!-- http://w3id.org/nfdi4ing/metadata4ing#Producer -->


    <owl:NamedIndividual rdf:about="http://w3id.org/nfdi4ing/metadata4ing#Producer">
        <rdf:type rdf:resource="http://www.w3.org/ns/prov#Role"/>
        <rdfs:seeAlso rdf:datatype="http://www.w3.org/2001/XMLSchema#anyURI">https://schema.datacite.org/meta/kernel-4.4/doc/DataCite-MetadataKernel_v4.4.pdf#page=40</rdfs:seeAlso>
        <skos:definition xml:lang="en">Typically,a person or organisation responsible for the artistry and form of a media product</skos:definition>
        <skos:prefLabel xml:lang="de">Produzent*in</skos:prefLabel>
        <skos:prefLabel xml:lang="en">producer</skos:prefLabel>
        <skos:scopeNote xml:lang="en">In the data industry, this may be a company &quot;producing&quot; DVDs that package data for future dissemination by a distributor.</skos:scopeNote>
    </owl:NamedIndividual>
    


    <!-- http://w3id.org/nfdi4ing/metadata4ing#ProjectLeader -->


    <owl:NamedIndividual rdf:about="http://w3id.org/nfdi4ing/metadata4ing#ProjectLeader">
        <rdf:type rdf:resource="http://www.w3.org/ns/prov#Role"/>
        <rdfs:seeAlso rdf:datatype="http://www.w3.org/2001/XMLSchema#anyURI">https://schema.datacite.org/meta/kernel-4.4/doc/DataCite-MetadataKernel_v4.4.pdf#page=40</rdfs:seeAlso>
        <skos:definition xml:lang="en">Person officially designated as head of project team or sub-project team instrumental in the work necessary to development of the resource</skos:definition>
        <skos:prefLabel xml:lang="de">Projektleiter*in</skos:prefLabel>
        <skos:prefLabel xml:lang="en">project leader</skos:prefLabel>
        <skos:scopeNote xml:lang="en">The Project Leader is not &quot;removed&quot; from the work that resulted in the resource; he or she remains intimately involved</skos:scopeNote>
    </owl:NamedIndividual>
    


    <!-- http://w3id.org/nfdi4ing/metadata4ing#ProjectManager -->


    <owl:NamedIndividual rdf:about="http://w3id.org/nfdi4ing/metadata4ing#ProjectManager">
        <rdf:type rdf:resource="http://www.w3.org/ns/prov#Role"/>
        <rdfs:seeAlso rdf:datatype="http://www.w3.org/2001/XMLSchema#anyURI">https://schema.datacite.org/meta/kernel-4.4/doc/DataCite-MetadataKernel_v4.4.pdf#page=40</rdfs:seeAlso>
        <skos:definition xml:lang="en">Person officially designated as manager of a project. Project may consist of one or many project teams and sub-teams.</skos:definition>
        <skos:prefLabel xml:lang="de">Projektmanager*in</skos:prefLabel>
        <skos:prefLabel xml:lang="en">project manager</skos:prefLabel>
        <skos:scopeNote xml:lang="en">The manager of a project normally has more administrative responsibility than actual work involvement.</skos:scopeNote>
    </owl:NamedIndividual>
    


    <!-- http://w3id.org/nfdi4ing/metadata4ing#ProjectMember -->


    <owl:NamedIndividual rdf:about="http://w3id.org/nfdi4ing/metadata4ing#ProjectMember">
        <rdf:type rdf:resource="http://www.w3.org/ns/prov#Role"/>
        <rdfs:seeAlso rdf:datatype="http://www.w3.org/2001/XMLSchema#anyURI">https://schema.datacite.org/meta/kernel-4.4/doc/DataCite-MetadataKernel_v4.4.pdf#page=40</rdfs:seeAlso>
        <skos:definition xml:lang="en">Person on the membership list of a designated project/project team</skos:definition>
        <skos:prefLabel xml:lang="de">Projektmitglied</skos:prefLabel>
        <skos:prefLabel xml:lang="en">project member</skos:prefLabel>
        <skos:scopeNote xml:lang="en">This vocabulary may or may not indicate the quality, quantity, or substance of the person&apos;s involvement.</skos:scopeNote>
    </owl:NamedIndividual>
    


    <!-- http://w3id.org/nfdi4ing/metadata4ing#RegistrationAgency -->


    <owl:NamedIndividual rdf:about="http://w3id.org/nfdi4ing/metadata4ing#RegistrationAgency">
        <rdf:type rdf:resource="http://www.w3.org/ns/prov#Role"/>
        <rdfs:seeAlso rdf:datatype="http://www.w3.org/2001/XMLSchema#anyURI">https://schema.datacite.org/meta/kernel-4.4/doc/DataCite-MetadataKernel_v4.4.pdf#page=40</rdfs:seeAlso>
        <skos:definition xml:lang="en">Institution/organisation officially appointed by a Registration Authority to handle specific tasks within a defined area of responsibility</skos:definition>
        <skos:prefLabel xml:lang="de">Registrierungsstelle</skos:prefLabel>
        <skos:prefLabel xml:lang="en">registration agency</skos:prefLabel>
        <skos:scopeNote xml:lang="en">DataCite is a Registration Agency for the International DOI Foundation (IDF). One of DataCite’s tasks is to assign DOI prefixes to the allocating agents who then assign the full, specific character string to data clients, provide metadata back to the DataCite registry, etc.</skos:scopeNote>
    </owl:NamedIndividual>
    


    <!-- http://w3id.org/nfdi4ing/metadata4ing#RegistrationAuthority -->


    <owl:NamedIndividual rdf:about="http://w3id.org/nfdi4ing/metadata4ing#RegistrationAuthority">
        <rdf:type rdf:resource="http://www.w3.org/ns/prov#Role"/>
        <rdfs:seeAlso rdf:datatype="http://www.w3.org/2001/XMLSchema#anyURI">https://schema.datacite.org/meta/kernel-4.4/doc/DataCite-MetadataKernel_v4.4.pdf#page=40</rdfs:seeAlso>
        <skos:definition xml:lang="en">A standards-setting body from which Registration Agencies obtain official recognition and guidance</skos:definition>
        <skos:prefLabel xml:lang="de">Registrierungsbehörde</skos:prefLabel>
        <skos:prefLabel xml:lang="en">registration authority</skos:prefLabel>
        <skos:scopeNote xml:lang="en">The IDF serves as the Registration Authority for the International Standards Organisation (ISO) in the area/domain of Digital Object Identifiers.</skos:scopeNote>
    </owl:NamedIndividual>
    


    <!-- http://w3id.org/nfdi4ing/metadata4ing#RelatedPerson -->


    <owl:NamedIndividual rdf:about="http://w3id.org/nfdi4ing/metadata4ing#RelatedPerson">
        <rdf:type rdf:resource="http://www.w3.org/ns/prov#Role"/>
        <rdfs:seeAlso rdf:datatype="http://www.w3.org/2001/XMLSchema#anyURI">https://schema.datacite.org/meta/kernel-4.4/doc/DataCite-MetadataKernel_v4.4.pdf#page=40</rdfs:seeAlso>
        <skos:definition xml:lang="en">A person without a specifically defined role in the development of the resource, but who is someone the author wishes to recognize</skos:definition>
        <skos:prefLabel xml:lang="en">related person</skos:prefLabel>
        <skos:prefLabel xml:lang="de">zugehörige Person</skos:prefLabel>
        <skos:scopeNote xml:lang="en">This person could be an author&apos;s intellectual mentor, a person providing intellectual leadership in the discipline or subject domain, etc.</skos:scopeNote>
    </owl:NamedIndividual>
    


    <!-- http://w3id.org/nfdi4ing/metadata4ing#ResearchGroup -->


    <owl:NamedIndividual rdf:about="http://w3id.org/nfdi4ing/metadata4ing#ResearchGroup">
        <rdf:type rdf:resource="http://www.w3.org/ns/prov#Role"/>
        <rdfs:seeAlso rdf:datatype="http://www.w3.org/2001/XMLSchema#anyURI">https://schema.datacite.org/meta/kernel-4.4/doc/DataCite-MetadataKernel_v4.4.pdf#page=40</rdfs:seeAlso>
        <skos:definition xml:lang="en">Typically refers to a group of individuals with a lab, department, or divisionthathas a specifically defined focus of activity.</skos:definition>
        <skos:prefLabel xml:lang="de">Forschungsgruppe</skos:prefLabel>
        <skos:prefLabel xml:lang="en">research group</skos:prefLabel>
        <skos:scopeNote xml:lang="en">May operate at a narrower level of scope; may or may not hold less administrative responsibility than a project team.

Example: Space Research &amp; Planetary Sciences Division of the University of Bern (WP Unibe)

Source: https://doi.org/10.26302/SSHADE/EXPERIMENT_OP_20201104_001</skos:scopeNote>
    </owl:NamedIndividual>
    


    <!-- http://w3id.org/nfdi4ing/metadata4ing#Researcher -->


    <owl:NamedIndividual rdf:about="http://w3id.org/nfdi4ing/metadata4ing#Researcher">
        <rdf:type rdf:resource="http://www.w3.org/ns/prov#Role"/>
        <rdfs:seeAlso rdf:datatype="http://www.w3.org/2001/XMLSchema#anyURI">https://schema.datacite.org/meta/kernel-4.4/doc/DataCite-MetadataKernel_v4.4.pdf#page=40</rdfs:seeAlso>
        <skos:definition xml:lang="en">A person involved in analysing data or the results of an experiment or formal study. May indicate an intern or assistant to one of the authors who helped with research but who was not so “key” as to be listed as an author.</skos:definition>
        <skos:prefLabel xml:lang="de">Rechercheur*in</skos:prefLabel>
        <skos:prefLabel xml:lang="en">researcher</skos:prefLabel>
        <skos:scopeNote xml:lang="en">Should be a person, not an institution. Note that a person involved in the gathering of data would fall under the contributorType &quot;DataCollector.&quot; The researcher may find additional data online and correlate it to the data collected for the experiment or study, for example.</skos:scopeNote>
    </owl:NamedIndividual>
    


    <!-- http://w3id.org/nfdi4ing/metadata4ing#RightsHolder -->


    <owl:NamedIndividual rdf:about="http://w3id.org/nfdi4ing/metadata4ing#RightsHolder">
        <rdf:type rdf:resource="http://www.w3.org/ns/prov#Role"/>
        <rdfs:seeAlso rdf:datatype="http://www.w3.org/2001/XMLSchema#anyURI">https://schema.datacite.org/meta/kernel-4.4/doc/DataCite-MetadataKernel_v4.4.pdf#page=40</rdfs:seeAlso>
        <skos:definition xml:lang="en">Person or institution owning or managing property rights, including intellectual property rights over the resource</skos:definition>
        <skos:prefLabel xml:lang="de">Rechteinhaber*in</skos:prefLabel>
        <skos:prefLabel xml:lang="en">rights holder</skos:prefLabel>
    </owl:NamedIndividual>
    


    <!-- http://w3id.org/nfdi4ing/metadata4ing#Sponsor -->


    <owl:NamedIndividual rdf:about="http://w3id.org/nfdi4ing/metadata4ing#Sponsor">
        <rdf:type rdf:resource="http://www.w3.org/ns/prov#Role"/>
        <rdfs:seeAlso rdf:datatype="http://www.w3.org/2001/XMLSchema#anyURI">https://schema.datacite.org/meta/kernel-4.4/doc/DataCite-MetadataKernel_v4.4.pdf#page=40</rdfs:seeAlso>
        <skos:definition xml:lang="en">Person or organisation that issued a contract or under the auspices of which a work has been written, printed, published, developed, etc.</skos:definition>
        <skos:prefLabel xml:lang="de">Sponsor*in</skos:prefLabel>
        <skos:prefLabel xml:lang="en">sponsor</skos:prefLabel>
        <skos:scopeNote xml:lang="en">Includes organisations that provide in-kind support, through donation, provision of people or a facility or instrumentation necessary for the development of the resource, etc.</skos:scopeNote>
    </owl:NamedIndividual>
    


    <!-- http://w3id.org/nfdi4ing/metadata4ing#Supervisor -->


    <owl:NamedIndividual rdf:about="http://w3id.org/nfdi4ing/metadata4ing#Supervisor">
        <rdf:type rdf:resource="http://www.w3.org/ns/prov#Role"/>
        <rdfs:seeAlso rdf:datatype="http://www.w3.org/2001/XMLSchema#anyURI">https://schema.datacite.org/meta/kernel-4.4/doc/DataCite-MetadataKernel_v4.4.pdf#page=40</rdfs:seeAlso>
        <skos:definition xml:lang="en">Designated administrator over one or more groups/teams working to produce a resource, or over one or more steps of a development process</skos:definition>
        <skos:prefLabel xml:lang="de">Betreuer*in</skos:prefLabel>
        <skos:prefLabel xml:lang="en">supervisor</skos:prefLabel>
    </owl:NamedIndividual>
    


    <!-- http://w3id.org/nfdi4ing/metadata4ing#WorkPackageLeader -->


    <owl:NamedIndividual rdf:about="http://w3id.org/nfdi4ing/metadata4ing#WorkPackageLeader">
        <rdf:type rdf:resource="http://www.w3.org/ns/prov#Role"/>
        <rdfs:seeAlso rdf:datatype="http://www.w3.org/2001/XMLSchema#anyURI">https://schema.datacite.org/meta/kernel-4.4/doc/DataCite-MetadataKernel_v4.4.pdf#page=40</rdfs:seeAlso>
        <skos:definition xml:lang="en">A Work Package is a recognized data product, not all of which is included in publication. The package, instead, may include notes, discarded documents, etc. The Work Package Leader is responsible for ensuring the comprehensive contents, versioning, and availability of the Work Package during the development of the resource.</skos:definition>
        <skos:prefLabel xml:lang="de">Arbeitspaketleiter*in</skos:prefLabel>
        <skos:prefLabel xml:lang="en">work package leader</skos:prefLabel>
    </owl:NamedIndividual>
    


    <!-- 
    ///////////////////////////////////////////////////////////////////////////////////////
    //
    // Annotations
    //
    ///////////////////////////////////////////////////////////////////////////////////////
     -->


    <rdf:Description rdf:about="http://purl.org/dc/terms/references">
        <terms:description xml:lang="en">This property is intended to be used with non-literal values. This property is an inverse property of Is Referenced By.</terms:description>
        <rdfs:comment xml:lang="en">A related resource that is referenced, cited, or otherwise pointed to by the described resource.</rdfs:comment>
        <skos:editorialNote xml:lang="en">changed by m4i: added german labels, added skos:prefLabel</skos:editorialNote>
        <skos:prefLabel xml:lang="en">references</skos:prefLabel>
        <skos:prefLabel xml:lang="de">referenziert</skos:prefLabel>
    </rdf:Description>
    <rdf:Description rdf:about="http://purl.org/dc/terms/title">
        <skos:definition xml:lang="en">A name given to the resource.</skos:definition>
        <skos:editorialNote xml:lang="en">changed by m4i: added skos:prefLabel</skos:editorialNote>
        <skos:prefLabel xml:lang="de">Titel</skos:prefLabel>
        <skos:prefLabel xml:lang="en">title</skos:prefLabel>
    </rdf:Description>
</rdf:RDF>



<!-- Generated by the OWL API (version 5.1.18) https://github.com/owlcs/owlapi/ -->


