<?xml version="1.0" encoding="utf-8" ?>
<rdf:RDF xmlns:rdf="http://www.w3.org/1999/02/22-rdf-syntax-ns#"
         xmlns:owl="http://www.w3.org/2002/07/owl#"
         xmlns:ns0="http://purl.org/vocab/vann/"
         xmlns:dc="http://purl.org/dc/terms/"
         xmlns:foaf="http://xmlns.com/foaf/0.1/"
         xmlns:rdfs="http://www.w3.org/2000/01/rdf-schema#"
         xmlns:ns1="http://www.w3.org/2003/06/sw-vocab-status/ns#">

  <owl:Ontology rdf:about="http://semanticturkey.uniroma2.it/ns/mdr">
    <ns0:preferredNamespacePrefix>mdr</ns0:preferredNamespacePrefix>
    <ns0:preferredNamespaceUri>http://semanticturkey.uniroma2.it/ns/mdr#</ns0:preferredNamespaceUri>
    <dc:title xml:lang="en">The Semantic Turkey metadata registry ontology</dc:title>
    <dc:description xml:lang="en">An application profile of DCAT combining it with other metadata vocabularies (e.g. VoID, DCTERMS, LIME)
 to meet requirements elicited in various use cases of the Semantic Web platform Semantic Turkey</dc:description>
    <owl:versionInfo>2.0.1</owl:versionInfo>
    <owl:versionIRI rdf:resource="http://semanticturkey.uniroma2.it/ns/mdr-2.0.1"/>
    <owl:priorVersion rdf:resource="http://semanticturkey.uniroma2.it/ns/mdr-2.0"/>
    <dc:issued rdf:datatype="http://www.w3.org/2001/XMLSchema#date">2020-01-23</dc:issued>
    <dc:modified rdf:datatype="http://www.w3.org/2001/XMLSchema#date">2023-02-11</dc:modified>
    <dc:rights>Copyright Â© 2020 ART Group @ University of Rome Tor Vergata. All rights reserved.</dc:rights>
    <dc:license rdf:resource="https://creativecommons.org/licenses/by/4.0/"/>
    <dc:creator>
      <foaf:Person>
        <foaf:name>Manuel Fiorelli</foaf:name>
        <foaf:homepage rdf:resource="https://art.uniroma2.it/fiorelli"/>
      </foaf:Person>
    </dc:creator>

    <dc:creator>
      <foaf:Person>
        <foaf:name>Armando stellato</foaf:name>
        <foaf:homepage rdf:resource="https://art.uniroma2.it/stellato"/>
      </foaf:Person>
    </dc:creator>

    <owl:imports rdf:resource="http://www.w3.org/ns/dcat"/>
    <owl:imports rdf:resource="http://purl.org/dc/terms/"/>
    <owl:imports rdf:resource="http://xmlns.com/foaf/0.1/"/>
    <owl:imports rdf:resource="http://rdfs.org/ns/void"/>
    <owl:imports rdf:resource="http://www.w3.org/ns/lemon/lime"/>
  </owl:Ontology>

  <owl:Class rdf:about="http://semanticturkey.uniroma2.it/ns/mdr#DereferenciationSystem">
    <rdfs:label xml:lang="en">Dereferenciation System</rdfs:label>
    <rdfs:comment xml:lang="en">a method to dereference the identifiers defined by a dataset</rdfs:comment>
    <rdfs:isDefinedBy rdf:resource="http://semanticturkey.uniroma2.it/ns/mdr"/>
    <ns1:term_status>stable</ns1:term_status>
  </owl:Class>

  <owl:Class rdf:about="http://semanticturkey.uniroma2.it/ns/mdr#HTTPSPARQLProvider">
    <rdfs:label xml:lang="en">HTTP SPARQL Provider</rdfs:label>
    <rdfs:comment xml:lang="en">a dataset deployment that supports the SPARQL HTTP Protocol</rdfs:comment>
    <rdfs:subClassOf>
      <owl:Class rdf:about="http://semanticturkey.uniroma2.it/ns/mdr#RDFRepository">
        <rdfs:label xml:lang="en">RDF Repository</rdfs:label>
        <rdfs:comment xml:lang="en">a deployment of a dataset on an RDF store technology</rdfs:comment>
        <rdfs:subClassOf rdf:resource="http://www.w3.org/ns/dcat#Distribution"/>
        <rdfs:subClassOf rdf:resource="http://rdfs.org/ns/void#Dataset"/>
        <rdfs:isDefinedBy rdf:resource="http://semanticturkey.uniroma2.it/ns/mdr"/>
        <ns1:term_status>stable</ns1:term_status>
      </owl:Class>
    </rdfs:subClassOf>

    <rdfs:isDefinedBy rdf:resource="http://semanticturkey.uniroma2.it/ns/mdr"/>
    <ns1:term_status>stable</ns1:term_status>
  </owl:Class>

  <owl:Class rdf:about="http://semanticturkey.uniroma2.it/ns/mdr#SPARQLEndpoint">
    <rdfs:label xml:lang="en">SPARQL Endpoint</rdfs:label>
    <rdfs:comment xml:lang="en">a data service enabling SPARQL queries over a dataset</rdfs:comment>
    <rdfs:subClassOf rdf:resource="http://www.w3.org/ns/dcat#DataService"/>
    <rdfs:isDefinedBy rdf:resource="http://semanticturkey.uniroma2.it/ns/mdr"/>
    <ns1:term_status>stable</ns1:term_status>
  </owl:Class>

  <owl:Class rdf:about="http://semanticturkey.uniroma2.it/ns/mdr#SparqlEndpointLimitation">
    <owl:deprecated rdf:datatype="http://www.w3.org/2001/XMLSchema#boolean">true</owl:deprecated>
    <rdfs:label xml:lang="en">SPARQL Endpoint Limitation</rdfs:label>
    <rdfs:comment xml:lang="en">a limitation of some SPARQL endpoint. This class is an extension point for recording and subsequently reacting in an application-specific manner to any perceived limitation of an endpoint. The focus is on limitations that cannot objectively be defined a-priori, as they rather depend on a number of boundary conditions, such as the task, the underlying access technology and even the specific queries run to perform the task. Such limitations can then be defined in application-specific ontologies reusing this vocabulary</rdfs:comment>
    <owl:equivalentClass rdf:resource="http://semanticturkey.uniroma2.it/ns/mdr#SPARQLEndpointLimitation"/>
    <rdfs:isDefinedBy rdf:resource="http://semanticturkey.uniroma2.it/ns/mdr"/>
    <ns1:term_status>archaic</ns1:term_status>
  </owl:Class>

  <owl:Class rdf:about="http://semanticturkey.uniroma2.it/ns/mdr#SPARQLEndpointLimitation">
    <rdfs:label xml:lang="en">SPARQL Endpoint Limitation</rdfs:label>
    <rdfs:comment xml:lang="en">a limitation of some SPARQL endpoint. This class is an extension point for recording and subsequently reacting in an application-specific manner to any perceived limitation of an endpoint. The focus is on limitations that cannot objectively be defined a-priori, as they rather depend on a number of boundary conditions, such as the task, the underlying access technology and even the specific queries run to perform the task. Such limitations can then be defined in application-specific ontologies reusing this vocabulary</rdfs:comment>
    <rdfs:isDefinedBy rdf:resource="http://semanticturkey.uniroma2.it/ns/mdr"/>
    <ns1:term_status>stable</ns1:term_status>
  </owl:Class>

  <owl:ObjectProperty rdf:about="http://semanticturkey.uniroma2.it/ns/mdr#dereferenciationSystem">
    <rdfs:label xml:lang="en">dereferenciation system</rdfs:label>
    <rdfs:comment xml:lang="en">relates a void:Dataset to a resource describing a method to dereference the identifiers defined by that dataset. Currently only two instances: :standardDereferenciation and :noDereferenciation are available, however this will be extended soon to account for versioning and other URI-transformation needs</rdfs:comment>
    <rdfs:domain rdf:resource="http://rdfs.org/ns/void#Dataset"/>
    <rdfs:range rdf:resource="http://semanticturkey.uniroma2.it/ns/mdr#DereferenciationSystem"/>
    <rdfs:isDefinedBy rdf:resource="http://semanticturkey.uniroma2.it/ns/mdr"/>
    <ns1:term_status>stable</ns1:term_status>
  </owl:ObjectProperty>

  <owl:ObjectProperty rdf:about="http://semanticturkey.uniroma2.it/ns/mdr#lod">
    <rdfs:label xml:lang="en">lod</rdfs:label>
    <rdfs:comment xml:lang="en">relates an abstract dcat:Dataset to a concrete one that represents whatever is published as linked data at the dataset namespace</rdfs:comment>
    <rdfs:domain rdf:resource="http://www.w3.org/ns/dcat#Dataset"/>
    <rdfs:range rdf:resource="http://www.w3.org/ns/dcat#Dataset"/>
    <rdfs:isDefinedBy rdf:resource="http://semanticturkey.uniroma2.it/ns/mdr"/>
    <ns1:term_status>stable</ns1:term_status>
  </owl:ObjectProperty>

  <owl:ObjectProperty rdf:about="http://semanticturkey.uniroma2.it/ns/mdr#master">
    <rdfs:label xml:lang="en">master</rdfs:label>
    <rdfs:comment xml:lang="en">relates an abstract dcat:Dataset to a concrete one that plays the role of master for the dataset development</rdfs:comment>
    <rdfs:domain rdf:resource="http://www.w3.org/ns/dcat#Dataset"/>
    <rdfs:range rdf:resource="http://www.w3.org/ns/dcat#Dataset"/>
    <rdfs:isDefinedBy rdf:resource="http://semanticturkey.uniroma2.it/ns/mdr"/>
    <ns1:term_status>stable</ns1:term_status>
  </owl:ObjectProperty>

  <owl:ObjectProperty rdf:about="http://semanticturkey.uniroma2.it/ns/mdr#sparqlEndpointLimitation">
    <rdfs:label xml:lang="en">SPARQL endpoint limitation</rdfs:label>
    <rdfs:comment xml:lang="en">relates a SPARQL endpoint to a resource describing some limitation of that endpoint</rdfs:comment>
    <rdfs:domain rdf:resource="http://semanticturkey.uniroma2.it/ns/mdr#SPARQLEndpoint"/>
    <rdfs:range rdf:resource="http://semanticturkey.uniroma2.it/ns/mdr#SPARQLEndpointLimitation"/>
    <rdfs:isDefinedBy rdf:resource="http://semanticturkey.uniroma2.it/ns/mdr"/>
    <ns1:term_status>stable</ns1:term_status>
  </owl:ObjectProperty>

  <rdf:Description rdf:about="http://semanticturkey.uniroma2.it/ns/mdr#standardDereferenciation">
    <rdf:type rdf:resource="http://semanticturkey.uniroma2.it/ns/mdr#DereferenciationSystem"/>
    <rdfs:label xml:lang="en">standard dereferenciation</rdfs:label>
    <rdfs:comment xml:lang="en">the method to dereference identifiers by means of HTTP resolution</rdfs:comment>
    <rdfs:isDefinedBy rdf:resource="http://semanticturkey.uniroma2.it/ns/mdr"/>
    <ns1:term_status>stable</ns1:term_status>
  </rdf:Description>

  <rdf:Description rdf:about="http://semanticturkey.uniroma2.it/ns/mdr#noDereferenciation">
    <rdf:type rdf:resource="http://semanticturkey.uniroma2.it/ns/mdr#DereferenciationSystem"/>
    <rdfs:label xml:lang="en">no dereferenciation</rdfs:label>
    <rdfs:comment xml:lang="en">missing support for any dereferenciation method</rdfs:comment>
    <rdfs:isDefinedBy rdf:resource="http://semanticturkey.uniroma2.it/ns/mdr"/>
    <ns1:term_status>stable</ns1:term_status>
  </rdf:Description>

</rdf:RDF>
