<?xml version="1.0"?>
<rdf:RDF xmlns="http://data.ign.fr/def/topo#"
     xml:base="http://data.ign.fr/def/topo"
     xmlns:ns="http://creativecommons.org/ns#"
     xmlns:org="http://www.w3.org/ns/org#"
     xmlns:owl="http://www.w3.org/2002/07/owl#"
     xmlns:rdf="http://www.w3.org/1999/02/22-rdf-syntax-ns#"
     xmlns:xml="http://www.w3.org/XML/1998/namespace"
     xmlns:xsd="http://www.w3.org/2001/XMLSchema#"
     xmlns:foaf="http://xmlns.com/foaf/0.1/"
     xmlns:rdfs="http://www.w3.org/2000/01/rdf-schema#"
     xmlns:skos="http://www.w3.org/2004/02/skos/core#"
     xmlns:time="http://www.w3.org/2006/time#"
     xmlns:vann="http://purl.org/vocab/vann/"
     xmlns:terms="http://purl.org/dc/terms/">
    <owl:Ontology rdf:about="http://data.ign.fr/def/topo#">
        <ns:license rdf:resource="http://creativecommons.org/licenses/by/2.0/"/>
        <ns:license rdf:resource="http://opendatacommons.org/licenses/by/"/>
        <ns:license rdf:resource="http://www.data.gouv.fr/Licence-Ouverte-Open-Licence"/>
        <terms:contributor rdf:resource="_:genid-nodeid-node1d3jspeb3x174"/>
        <terms:contributor rdf:resource="http://www.eurecom.fr/~atemezin/"/>
        <terms:creator rdf:resource="_:genid-nodeid-node1d3jspeb3x169"/>
        <terms:description xml:lang="fr">Ontologie décrivant les éléments du territoire et ses infrastructures. Elle reprend l&apos;essentiel du vocabulaire de la BDTOPO(IGN) et vise à couvrir l&apos;ensemble des entités topographiques et administratives du territoire national. Les thèmes couverts sont: le réseau routier, le réseau ferroviaire, le réseau de transport d&apos;énergie, le réseau hydrographique, les bâtiments, la végétation arborée, l&apos;orographie, les communes, les points d&apos;activité ou d&apos;intérêt.</terms:description>
        <terms:description xml:lang="en">Ontology describing the elements of the territory and its infrastructures. It covers most of the vocabulary of the BDTOPO (IGN) and aims to cover all the topographic and administrative entities of the national territory. The topics covered are: the road network, the railway network, the energy transport network, the hydrographic network, the buildings, the wooded vegetation, the orography, the communes, the points of activity or interest.</terms:description>
        <terms:issued rdf:datatype="http://www.w3.org/2001/XMLSchema#date">2014-04-16</terms:issued>
        <terms:modified rdf:datatype="http://www.w3.org/2001/XMLSchema#date">2019-02-12</terms:modified>
        <terms:publisher rdf:resource="http://fr.dbpedia.org/resource/Institut_national_de_l%27information_g%C3%A9ographique_et_foresti%C3%A8re"/>
        <terms:rights>Copyright 2019, IGN</terms:rights>
        <terms:title xml:lang="fr">Ontologie des éléments du territoire et de ses infrastructures de l&apos;IGN</terms:title>
        <terms:title xml:lang="en">Ontology of the elements of the territory and its infrastructures of the IGN</terms:title>
        <vann:preferredNamespacePrefix>topo</vann:preferredNamespacePrefix>
        <vann:preferredNamespaceUri rdf:resource="http://data.ign.fr/def/topo#"/>
        <owl:priorVersion rdf:resource="http://data.ign.fr/def/topo/20140416.ttl"/>
        <owl:versionInfo>Version 1.1 - 2019-02-12</owl:versionInfo>
    </owl:Ontology>
    


    <!-- 
    ///////////////////////////////////////////////////////////////////////////////////////
    //
    // Annotation properties
    //
    ///////////////////////////////////////////////////////////////////////////////////////
     -->


    


    <!-- http://creativecommons.org/ns#license -->


    <owl:AnnotationProperty rdf:about="http://creativecommons.org/ns#license"/>
    


    <!-- http://purl.org/dc/terms/contributor -->


    <owl:AnnotationProperty rdf:about="http://purl.org/dc/terms/contributor"/>
    


    <!-- http://purl.org/dc/terms/creator -->


    <owl:AnnotationProperty rdf:about="http://purl.org/dc/terms/creator"/>
    


    <!-- http://purl.org/dc/terms/description -->


    <owl:AnnotationProperty rdf:about="http://purl.org/dc/terms/description"/>
    


    <!-- http://purl.org/dc/terms/issued -->


    <owl:AnnotationProperty rdf:about="http://purl.org/dc/terms/issued"/>
    


    <!-- http://purl.org/dc/terms/modified -->


    <owl:AnnotationProperty rdf:about="http://purl.org/dc/terms/modified"/>
    


    <!-- http://purl.org/dc/terms/publisher -->


    <owl:AnnotationProperty rdf:about="http://purl.org/dc/terms/publisher"/>
    


    <!-- http://purl.org/dc/terms/rights -->


    <owl:AnnotationProperty rdf:about="http://purl.org/dc/terms/rights"/>
    


    <!-- http://purl.org/dc/terms/title -->


    <owl:AnnotationProperty rdf:about="http://purl.org/dc/terms/title"/>
    


    <!-- http://purl.org/vocab/vann/preferredNamespacePrefix -->


    <owl:AnnotationProperty rdf:about="http://purl.org/vocab/vann/preferredNamespacePrefix"/>
    


    <!-- http://purl.org/vocab/vann/preferredNamespaceUri -->


    <owl:AnnotationProperty rdf:about="http://purl.org/vocab/vann/preferredNamespaceUri"/>
    


    <!-- http://www.w3.org/2004/02/skos/core#altLabel -->


    <owl:AnnotationProperty rdf:about="http://www.w3.org/2004/02/skos/core#altLabel"/>
    


    <!-- http://www.w3.org/2004/02/skos/core#broadMatch -->


    <owl:AnnotationProperty rdf:about="http://www.w3.org/2004/02/skos/core#broadMatch"/>
    


    <!-- http://www.w3.org/2004/02/skos/core#broader -->


    <owl:AnnotationProperty rdf:about="http://www.w3.org/2004/02/skos/core#broader"/>
    


    <!-- http://www.w3.org/2004/02/skos/core#definition -->


    <owl:AnnotationProperty rdf:about="http://www.w3.org/2004/02/skos/core#definition"/>
    


    <!-- http://www.w3.org/2004/02/skos/core#hasTopConcept -->


    <owl:AnnotationProperty rdf:about="http://www.w3.org/2004/02/skos/core#hasTopConcept"/>
    


    <!-- http://www.w3.org/2004/02/skos/core#narrowMatch -->


    <owl:AnnotationProperty rdf:about="http://www.w3.org/2004/02/skos/core#narrowMatch"/>
    


    <!-- http://www.w3.org/2004/02/skos/core#prefLabel -->


    <owl:AnnotationProperty rdf:about="http://www.w3.org/2004/02/skos/core#prefLabel"/>
    


    <!-- http://www.w3.org/2004/02/skos/core#relatedMatch -->


    <owl:AnnotationProperty rdf:about="http://www.w3.org/2004/02/skos/core#relatedMatch"/>
    


    <!-- http://www.w3.org/2006/time#hasBeginning -->


    <owl:AnnotationProperty rdf:about="http://www.w3.org/2006/time#hasBeginning"/>
    


    <!-- http://www.w3.org/2006/time#inXSDDateTimeStamp -->


    <owl:AnnotationProperty rdf:about="http://www.w3.org/2006/time#inXSDDateTimeStamp"/>
    


    <!-- http://www.w3.org/ns/org#hasMembership -->


    <owl:AnnotationProperty rdf:about="http://www.w3.org/ns/org#hasMembership"/>
    


    <!-- http://www.w3.org/ns/org#memberDuring -->


    <owl:AnnotationProperty rdf:about="http://www.w3.org/ns/org#memberDuring"/>
    


    <!-- http://www.w3.org/ns/org#organization -->


    <owl:AnnotationProperty rdf:about="http://www.w3.org/ns/org#organization"/>
    


    <!-- http://www.w3.org/ns/org#role -->


    <owl:AnnotationProperty rdf:about="http://www.w3.org/ns/org#role"/>
    


    <!-- http://xmlns.com/foaf/0.1/family_name -->


    <owl:AnnotationProperty rdf:about="http://xmlns.com/foaf/0.1/family_name"/>
    


    <!-- http://xmlns.com/foaf/0.1/firstName -->


    <owl:AnnotationProperty rdf:about="http://xmlns.com/foaf/0.1/firstName"/>
    


    <!-- http://xmlns.com/foaf/0.1/homepage -->


    <owl:AnnotationProperty rdf:about="http://xmlns.com/foaf/0.1/homepage"/>
    


    <!-- http://xmlns.com/foaf/0.1/mbox -->


    <owl:AnnotationProperty rdf:about="http://xmlns.com/foaf/0.1/mbox"/>
    


    <!-- http://xmlns.com/foaf/0.1/name -->


    <owl:AnnotationProperty rdf:about="http://xmlns.com/foaf/0.1/name"/>
    


    <!-- http://xmlns.com/foaf/0.1/workInfoHomepage -->


    <owl:AnnotationProperty rdf:about="http://xmlns.com/foaf/0.1/workInfoHomepage"/>
    


    <!-- 
    ///////////////////////////////////////////////////////////////////////////////////////
    //
    // Object Properties
    //
    ///////////////////////////////////////////////////////////////////////////////////////
     -->


    


    <!-- http://data.ign.fr/def/geometrie#geometry -->


    <owl:ObjectProperty rdf:about="http://data.ign.fr/def/geometrie#geometry"/>
    


    <!-- http://data.ign.fr/def/topo#borneFin -->


    <owl:ObjectProperty rdf:about="http://data.ign.fr/def/topo#borneFin">
        <rdfs:domain rdf:resource="http://data.ign.fr/def/topo#Route"/>
        <rdfs:range rdf:resource="http://data.ign.fr/def/topo#BornePostale"/>
        <rdfs:comment xml:lang="fr">Relation entre un tronçon de route et la borne postale correspondant à son point final.</rdfs:comment>
        <rdfs:comment xml:lang="en">Relationship between a section of road and the post office terminal corresponding to its end point.</rdfs:comment>
        <rdfs:isDefinedBy rdf:resource="http://data.ign.fr/def/topo"/>
        <rdfs:label xml:lang="fr">borne finale</rdfs:label>
        <rdfs:label xml:lang="en">final civic number marker</rdfs:label>
    </owl:ObjectProperty>
    


    <!-- http://data.ign.fr/def/topo#borneIni -->


    <owl:ObjectProperty rdf:about="http://data.ign.fr/def/topo#borneIni">
        <rdfs:domain rdf:resource="http://data.ign.fr/def/topo#Route"/>
        <rdfs:range rdf:resource="http://data.ign.fr/def/topo#BornePostale"/>
        <rdfs:comment xml:lang="fr">Relation entre un tronçon de route et la borne postale correspondant à son point initial.</rdfs:comment>
        <rdfs:comment xml:lang="en">Relationship between a section of road and the post office terminal corresponding to its initial point.</rdfs:comment>
        <rdfs:isDefinedBy rdf:resource="http://data.ign.fr/def/topo"/>
        <rdfs:label xml:lang="fr">borne initiale</rdfs:label>
        <rdfs:label xml:lang="en">initial civic number marker</rdfs:label>
    </owl:ObjectProperty>
    


    <!-- http://data.ign.fr/def/topo#clAdmin -->


    <owl:ObjectProperty rdf:about="http://data.ign.fr/def/topo#clAdmin">
        <rdfs:domain rdf:resource="http://data.ign.fr/def/topo#Route"/>
        <rdfs:range>
            <owl:Restriction>
                <owl:onProperty rdf:resource="http://www.w3.org/2004/02/skos/core#inScheme"/>
                <owl:hasValue rdf:resource="http://data.ign.fr/id/codes/topo/typederoute/liste"/>
            </owl:Restriction>
        </rdfs:range>
        <rdfs:comment xml:lang="en">Administrative classification. Status of a numbered or named road.</rdfs:comment>
        <rdfs:comment xml:lang="fr">Classement administratif. Statut d’une route numérotée ou nommée.</rdfs:comment>
        <rdfs:isDefinedBy rdf:resource="http://data.ign.fr/def/topo"/>
        <rdfs:label xml:lang="en">administrative status</rdfs:label>
        <rdfs:label xml:lang="fr">classement administratif</rdfs:label>
    </owl:ObjectProperty>
    


    <!-- http://data.ign.fr/def/topo#concerne -->


    <owl:ObjectProperty rdf:about="http://data.ign.fr/def/topo#concerne">
        <rdfs:domain rdf:resource="http://data.ign.fr/def/topo#BornePostale"/>
        <rdfs:range rdf:resource="http://data.ign.fr/def/topo#Voie"/>
        <rdfs:comment xml:lang="fr">Relation entre une borne postale et la voie à laquelle elle se rapporte.</rdfs:comment>
        <rdfs:comment xml:lang="en">Relationship between a postal station and the route to which it relates.</rdfs:comment>
        <rdfs:isDefinedBy rdf:resource="http://data.ign.fr/def/topo"/>
        <rdfs:label xml:lang="fr">concerne</rdfs:label>
        <rdfs:label xml:lang="en">related to</rdfs:label>
    </owl:ObjectProperty>
    


    <!-- http://data.ign.fr/def/topo#gestionVoie -->


    <owl:ObjectProperty rdf:about="http://data.ign.fr/def/topo#gestionVoie">
        <rdfs:domain rdf:resource="http://data.ign.fr/def/topo#Voie"/>
        <rdfs:range rdf:resource="http://data.ign.fr/def/geofla#Commune"/>
        <rdfs:comment xml:lang="fr">Relation entre une voie nommée et la commune dont elle dépend.</rdfs:comment>
        <rdfs:comment xml:lang="en">Relationship between a named path and the municipality on which it depends.</rdfs:comment>
        <rdfs:isDefinedBy rdf:resource="http://data.ign.fr/def/topo"/>
        <rdfs:label xml:lang="fr">commune gestionnaire de la voie nommée</rdfs:label>
        <rdfs:label xml:lang="en">manager of the nammed street</rdfs:label>
    </owl:ObjectProperty>
    


    <!-- http://data.ign.fr/def/topo#nature -->


    <owl:ObjectProperty rdf:about="http://data.ign.fr/def/topo#nature">
        <rdfs:domain rdf:resource="http://data.ign.fr/def/topo#EntiteTopographique"/>
        <rdfs:range rdf:resource="http://www.w3.org/2004/02/skos/core#Concept"/>
        <rdfs:comment xml:lang="en">Link a topographic entity to the concept that specifies its nature.</rdfs:comment>
        <rdfs:comment xml:lang="fr">Relie une entité topographique au concept qui précise sa nature.</rdfs:comment>
        <rdfs:isDefinedBy rdf:resource="http://data.ign.fr/def/topo"/>
        <rdfs:label xml:lang="en">nature</rdfs:label>
        <rdfs:label xml:lang="fr">nature</rdfs:label>
    </owl:ObjectProperty>
    


    <!-- http://data.ign.fr/def/topo#origine -->


    <owl:ObjectProperty rdf:about="http://data.ign.fr/def/topo#origine">
        <rdfs:subPropertyOf rdf:resource="http://www.w3.org/ns/prov#wasDerivedFrom"/>
        <rdfs:domain rdf:resource="http://data.ign.fr/def/topo#EntiteTopographique"/>
        <rdfs:range rdf:resource="http://www.w3.org/ns/prov#Entity"/>
        <rdfs:comment xml:lang="fr">Source de l&apos;information.</rdfs:comment>
        <rdfs:comment xml:lang="en">Source of information.</rdfs:comment>
        <rdfs:isDefinedBy rdf:resource="http://data.ign.fr/def/topo"/>
        <rdfs:label xml:lang="en">origine</rdfs:label>
        <rdfs:label xml:lang="fr">origine</rdfs:label>
    </owl:ObjectProperty>
    


    <!-- http://data.ign.fr/def/topo#typeDeBatiment -->


    <owl:ObjectProperty rdf:about="http://data.ign.fr/def/topo#typeDeBatiment">
        <rdfs:subPropertyOf rdf:resource="http://data.ign.fr/def/topo#nature"/>
        <rdfs:domain rdf:resource="http://data.ign.fr/def/topo#Batiment"/>
        <rdfs:range>
            <owl:Restriction>
                <owl:onProperty rdf:resource="http://www.w3.org/2004/02/skos/core#inScheme"/>
                <owl:hasValue rdf:resource="http://data.ign.fr/id/codes/topo/typedebatiment/liste"/>
            </owl:Restriction>
        </rdfs:range>
        <rdfs:comment xml:lang="en">Links a building instance to an instance of skos: Concept defined in the list &apos;building&apos; which specifies its nature.</rdfs:comment>
        <rdfs:comment xml:lang="fr">Relie une instance de bâtiment à une instance de skos:Concept définie dans la liste &apos;bati&apos; qui précise sa nature.</rdfs:comment>
        <rdfs:isDefinedBy rdf:resource="http://data.ign.fr/def/topo"/>
        <rdfs:label xml:lang="fr">type de bâtiment</rdfs:label>
        <rdfs:label xml:lang="en">type of building </rdfs:label>
    </owl:ObjectProperty>
    


    <!-- http://data.ign.fr/def/topo#typeDeConstruction -->


    <owl:ObjectProperty rdf:about="http://data.ign.fr/def/topo#typeDeConstruction">
        <rdfs:subPropertyOf rdf:resource="http://data.ign.fr/def/topo#nature"/>
        <rdfs:domain rdf:resource="http://data.ign.fr/def/topo#Construction"/>
        <rdfs:range>
            <owl:Restriction>
                <owl:onProperty rdf:resource="http://www.w3.org/2004/02/skos/core#inScheme"/>
                <owl:hasValue rdf:resource="http://data.ign.fr/id/codes/topo/typedeconstruction/liste"/>
            </owl:Restriction>
        </rdfs:range>
        <rdfs:comment xml:lang="en">Links a build instance to an instance of skos: Concept defined in the list &apos;cnstr&apos; which specifies its nature.</rdfs:comment>
        <rdfs:comment xml:lang="fr">Relie une instance de construction à une instance de skos:Concept définie dans la liste &apos;cnstr&apos; qui précise sa nature.</rdfs:comment>
        <rdfs:isDefinedBy rdf:resource="http://data.ign.fr/def/topo"/>
        <rdfs:label xml:lang="fr">type de construction</rdfs:label>
        <rdfs:label xml:lang="en">type of structure</rdfs:label>
    </owl:ObjectProperty>
    


    <!-- http://data.ign.fr/def/topo#typeDeFranchissement -->


    <owl:ObjectProperty rdf:about="http://data.ign.fr/def/topo#typeDeFranchissement">
        <rdfs:domain>
            <owl:Class>
                <owl:unionOf rdf:parseType="Collection">
                    <rdf:Description rdf:about="http://data.ign.fr/def/topo#Route"/>
                    <rdf:Description rdf:about="http://data.ign.fr/def/topo#VoieFerree"/>
                </owl:unionOf>
            </owl:Class>
        </rdfs:domain>
        <rdfs:range>
            <owl:Restriction>
                <owl:onProperty rdf:resource="http://www.w3.org/2004/02/skos/core#inScheme"/>
                <owl:hasValue rdf:resource="http://data.ign.fr/id/codes/topo/typedefranchissement/liste"/>
            </owl:Restriction>
        </rdfs:range>
        <rdfs:comment xml:lang="en">Links the elements of the transport networks to the type of crossing structure to which they correspond.</rdfs:comment>
        <rdfs:comment xml:lang="fr">Relie les éléments de réseaux de transport au type d&apos;ouvrage de franchissement auquel ils correspondent.</rdfs:comment>
        <rdfs:isDefinedBy rdf:resource="http://data.ign.fr/def/topo"/>
        <rdfs:label xml:lang="fr">type de franchissement</rdfs:label>
        <rdfs:label xml:lang="en">type of crossing</rdfs:label>
    </owl:ObjectProperty>
    


    <!-- http://data.ign.fr/def/topo#typeDeLaisse -->


    <owl:ObjectProperty rdf:about="http://data.ign.fr/def/topo#typeDeLaisse">
        <rdfs:subPropertyOf rdf:resource="http://data.ign.fr/def/topo#nature"/>
        <rdfs:domain rdf:resource="http://data.ign.fr/def/topo#Laisse"/>
        <rdfs:range>
            <owl:Restriction>
                <owl:onProperty rdf:resource="http://www.w3.org/2004/02/skos/core#inScheme"/>
                <owl:hasValue rdf:resource="http://data.ign.fr/id/codes/topo/typedelaisse/liste"/>
            </owl:Restriction>
        </rdfs:range>
        <rdfs:comment xml:lang="en">Links an instance of leash to an instance of skos: Concept defined in the list &apos;tdl&apos; which specifies its nature.</rdfs:comment>
        <rdfs:comment xml:lang="fr">Relie une instance de laisse à une instance de skos:Concept définie dans la liste &apos;tdl&apos; qui précise sa nature.</rdfs:comment>
        <rdfs:isDefinedBy rdf:resource="http://data.ign.fr/def/topo"/>
        <rdfs:label xml:lang="fr">type de laisse</rdfs:label>
        <rdfs:label xml:lang="en">type of tide line</rdfs:label>
    </owl:ObjectProperty>
    


    <!-- http://data.ign.fr/def/topo#typeDePointDEau -->


    <owl:ObjectProperty rdf:about="http://data.ign.fr/def/topo#typeDePointDEau">
        <rdfs:subPropertyOf rdf:resource="http://data.ign.fr/def/topo#nature"/>
        <rdfs:domain rdf:resource="http://data.ign.fr/def/topo#PointDEau"/>
        <rdfs:range>
            <owl:Restriction>
                <owl:onProperty rdf:resource="http://www.w3.org/2004/02/skos/core#inScheme"/>
                <owl:hasValue rdf:resource="http://data.ign.fr/id/codes/topo/typedepointdeau/liste"/>
            </owl:Restriction>
        </rdfs:range>
        <rdfs:comment xml:lang="en">Links an instance of water point to an instance of skos: Concept defined in the list &apos;pte&apos; which specifies its nature.</rdfs:comment>
        <rdfs:comment xml:lang="fr">Relie une instance de point d&apos;eau à une instance de skos:Concept définie dans la liste &apos;pte&apos; qui précise sa nature.</rdfs:comment>
        <rdfs:isDefinedBy rdf:resource="http://data.ign.fr/def/topo"/>
        <rdfs:label xml:lang="fr">type de point d&apos;eau</rdfs:label>
        <rdfs:label xml:lang="en">type of waterhole</rdfs:label>
    </owl:ObjectProperty>
    


    <!-- http://data.ign.fr/def/topo#typeDeRelief -->


    <owl:ObjectProperty rdf:about="http://data.ign.fr/def/topo#typeDeRelief">
        <rdfs:subPropertyOf rdf:resource="http://data.ign.fr/def/topo#nature"/>
        <rdfs:domain rdf:resource="http://data.ign.fr/def/topo#ElementDuRelief"/>
        <rdfs:range>
            <owl:Restriction>
                <owl:onProperty rdf:resource="http://www.w3.org/2004/02/skos/core#inScheme"/>
                <owl:hasValue rdf:resource="http://data.ign.fr/id/codes/topo/typederelief/liste"/>
            </owl:Restriction>
        </rdfs:range>
        <rdfs:comment xml:lang="en">Links a terrain element instance to an instance of skos: Concept defined in the &apos;rel&apos; list that specifies its nature.</rdfs:comment>
        <rdfs:comment xml:lang="fr">Relie une instance d&apos;élément du relief à une instance de skos:Concept définie dans la liste &apos;rel&apos; qui précise sa nature.</rdfs:comment>
        <rdfs:isDefinedBy rdf:resource="http://data.ign.fr/def/topo"/>
        <rdfs:label xml:lang="fr">type d&apos;élément du relief</rdfs:label>
        <rdfs:label xml:lang="en">type of relief feature</rdfs:label>
    </owl:ObjectProperty>
    


    <!-- http://data.ign.fr/def/topo#typeDeReservoir -->


    <owl:ObjectProperty rdf:about="http://data.ign.fr/def/topo#typeDeReservoir">
        <rdfs:subPropertyOf rdf:resource="http://data.ign.fr/def/topo#nature"/>
        <rdfs:domain rdf:resource="http://data.ign.fr/def/topo#Reservoir"/>
        <rdfs:range>
            <owl:Restriction>
                <owl:onProperty rdf:resource="http://www.w3.org/2004/02/skos/core#inScheme"/>
                <owl:hasValue rdf:resource="http://data.ign.fr/id/codes/topo/typedereservoir/liste"/>
            </owl:Restriction>
        </rdfs:range>
        <rdfs:comment xml:lang="en">Links a tank instance to an instance of skos: Concept defined in the &apos;rsv&apos; list which specifies its nature.</rdfs:comment>
        <rdfs:comment xml:lang="fr">Relie une instance de réservoir à une instance de skos:Concept définie dans la liste &apos;rsv&apos; qui précise sa nature.</rdfs:comment>
        <rdfs:isDefinedBy rdf:resource="http://data.ign.fr/def/topo"/>
        <rdfs:label xml:lang="fr">type de réservoir</rdfs:label>
        <rdfs:label xml:lang="en">type of tank</rdfs:label>
    </owl:ObjectProperty>
    


    <!-- http://data.ign.fr/def/topo#typeDeRoute -->


    <owl:ObjectProperty rdf:about="http://data.ign.fr/def/topo#typeDeRoute">
        <rdfs:subPropertyOf rdf:resource="http://data.ign.fr/def/topo#nature"/>
        <rdfs:domain rdf:resource="http://data.ign.fr/def/topo#Route"/>
        <rdfs:range>
            <owl:Restriction>
                <owl:onProperty rdf:resource="http://www.w3.org/2004/02/skos/core#inScheme"/>
                <owl:hasValue rdf:resource="http://data.ign.fr/id/codes/topo/typederoute/liste"/>
            </owl:Restriction>
        </rdfs:range>
        <rdfs:comment xml:lang="en">Links a route instance to an instance of skos: Concept defined in the list &apos;rte&apos; which specifies its nature.</rdfs:comment>
        <rdfs:comment xml:lang="fr">Relie une instance de route à une instance de skos:Concept définie dans la liste &apos;rte&apos; qui précise sa nature.</rdfs:comment>
        <rdfs:isDefinedBy rdf:resource="http://data.ign.fr/def/topo"/>
        <rdfs:label xml:lang="fr">type de route</rdfs:label>
        <rdfs:label xml:lang="en">type of road</rdfs:label>
    </owl:ObjectProperty>
    


    <!-- http://data.ign.fr/def/topo#typeDeTerrainDeSport -->


    <owl:ObjectProperty rdf:about="http://data.ign.fr/def/topo#typeDeTerrainDeSport">
        <rdfs:subPropertyOf rdf:resource="http://data.ign.fr/def/topo#nature"/>
        <rdfs:domain rdf:resource="http://data.ign.fr/def/topo#TerrainDeSport"/>
        <rdfs:range>
            <owl:Restriction>
                <owl:onProperty rdf:resource="http://www.w3.org/2004/02/skos/core#inScheme"/>
                <owl:hasValue rdf:resource="http://data.ign.fr/id/codes/topo/typedeterraindesport/liste"/>
            </owl:Restriction>
        </rdfs:range>
        <rdfs:comment xml:lang="en">Links a sport field instance to an instance of skos: Concept defined in the &apos;tds&apos; list which specifies its nature.</rdfs:comment>
        <rdfs:comment xml:lang="fr">Relie une instance de terrain de sport à une instance de skos:Concept définie dans la liste &apos;tds&apos; qui précise sa nature.</rdfs:comment>
        <rdfs:isDefinedBy rdf:resource="http://data.ign.fr/def/topo"/>
        <rdfs:label xml:lang="fr">type de terrain de sport</rdfs:label>
        <rdfs:label xml:lang="en">type of sports ground</rdfs:label>
    </owl:ObjectProperty>
    


    <!-- http://data.ign.fr/def/topo#typeDeTransportCable -->


    <owl:ObjectProperty rdf:about="http://data.ign.fr/def/topo#typeDeTransportCable">
        <rdfs:subPropertyOf rdf:resource="http://data.ign.fr/def/topo#nature"/>
        <rdfs:domain rdf:resource="http://data.ign.fr/def/topo#LigneTransportCable"/>
        <rdfs:range>
            <owl:Restriction>
                <owl:onProperty rdf:resource="http://www.w3.org/2004/02/skos/core#inScheme"/>
                <owl:hasValue rdf:resource="http://data.ign.fr/id/codes/topo/typedetransportcable/liste"/>
            </owl:Restriction>
        </rdfs:range>
        <rdfs:comment xml:lang="en">Links a cable transport infrastructure instance to an instance of skos: Concept defined in the &apos;tpc&apos; list which specifies its nature.</rdfs:comment>
        <rdfs:comment xml:lang="fr">Relie une instance d&apos;infrastructure de transport par câble à une instance de skos:Concept définie dans la liste &apos;tpc&apos; qui précise sa nature.</rdfs:comment>
        <rdfs:isDefinedBy rdf:resource="http://data.ign.fr/def/topo"/>
        <rdfs:label xml:lang="fr">type de ligne de transport par câble</rdfs:label>
        <rdfs:label xml:lang="en">type of cableway transport line</rdfs:label>
    </owl:ObjectProperty>
    


    <!-- http://data.ign.fr/def/topo#typeDeVegetation -->


    <owl:ObjectProperty rdf:about="http://data.ign.fr/def/topo#typeDeVegetation">
        <rdfs:subPropertyOf rdf:resource="http://data.ign.fr/def/topo#nature"/>
        <rdfs:domain rdf:resource="http://data.ign.fr/def/topo#ZoneDeVegetation"/>
        <rdfs:range>
            <owl:Restriction>
                <owl:onProperty rdf:resource="http://www.w3.org/2004/02/skos/core#inScheme"/>
                <owl:hasValue rdf:resource="http://data.ign.fr/id/codes/topo/typedevegetation/liste"/>
            </owl:Restriction>
        </rdfs:range>
        <rdfs:comment xml:lang="en">Links an instance of a vegetation zone to an instance of skos: Concept defined in the &apos;veg&apos; list which specifies its nature.</rdfs:comment>
        <rdfs:comment xml:lang="fr">Relie une instance de zone de végétation à une instance de skos:Concept définie dans la liste &apos;veg&apos; qui précise sa nature.</rdfs:comment>
        <rdfs:isDefinedBy rdf:resource="http://data.ign.fr/def/topo"/>
        <rdfs:label xml:lang="fr">type de végétation</rdfs:label>
        <rdfs:label xml:lang="en">type of vegetation </rdfs:label>
    </owl:ObjectProperty>
    


    <!-- http://data.ign.fr/def/topo#typeDeVoieFerree -->


    <owl:ObjectProperty rdf:about="http://data.ign.fr/def/topo#typeDeVoieFerree">
        <rdfs:subPropertyOf rdf:resource="http://data.ign.fr/def/topo#nature"/>
        <rdfs:domain rdf:resource="http://data.ign.fr/def/topo#VoieFerree"/>
        <rdfs:range>
            <owl:Restriction>
                <owl:onProperty rdf:resource="http://www.w3.org/2004/02/skos/core#inScheme"/>
                <owl:hasValue rdf:resource="http://data.ign.fr/id/codes/topo/typedevoieferree/liste"/>
            </owl:Restriction>
        </rdfs:range>
        <rdfs:comment xml:lang="en">Links a railroad instance to an instance of skos: Concept defined in the &apos;vfr&apos; list which specifies its nature.</rdfs:comment>
        <rdfs:comment xml:lang="fr">Relie une instance de voie ferrée à une instance de skos:Concept définie dans la liste &apos;vfr&apos; qui précise sa nature.</rdfs:comment>
        <rdfs:isDefinedBy rdf:resource="http://data.ign.fr/def/topo"/>
        <rdfs:label xml:lang="fr">type de voie ferrée</rdfs:label>
        <rdfs:label xml:lang="en">type of railway track</rdfs:label>
    </owl:ObjectProperty>
    


    <!-- http://data.ign.fr/def/topo#typeDeZAI -->


    <owl:ObjectProperty rdf:about="http://data.ign.fr/def/topo#typeDeZAI">
        <rdfs:subPropertyOf rdf:resource="http://data.ign.fr/def/topo#nature"/>
        <rdfs:domain rdf:resource="http://data.ign.fr/def/topo#ZoneActiviteInteret"/>
        <rdfs:range>
            <owl:Restriction>
                <owl:onProperty rdf:resource="http://www.w3.org/2004/02/skos/core#inScheme"/>
                <owl:hasValue rdf:resource="http://data.ign.fr/id/codes/topo/typedezai/liste"/>
            </owl:Restriction>
        </rdfs:range>
        <rdfs:comment xml:lang="en">Links an instance of activity and interest zone to an instance of skos: Concept defined in the list &apos;zai&apos; which specifies its nature.</rdfs:comment>
        <rdfs:comment xml:lang="fr">Relie une instance de zone d&apos;activité et d&apos;intérêt à une instance de skos:Concept définie dans la liste &apos;zai&apos; qui précise sa nature.</rdfs:comment>
        <rdfs:isDefinedBy rdf:resource="http://data.ign.fr/def/topo"/>
        <rdfs:label xml:lang="fr">type de ZAI</rdfs:label>
        <rdfs:label xml:lang="en">type of Area Of Interest (AOI)</rdfs:label>
    </owl:ObjectProperty>
    


    <!-- http://purl.org/dc/terms/isPartOf -->


    <owl:ObjectProperty rdf:about="http://purl.org/dc/terms/isPartOf"/>
    


    <!-- http://www.w3.org/ns/prov#wasDerivedFrom -->


    <owl:ObjectProperty rdf:about="http://www.w3.org/ns/prov#wasDerivedFrom"/>
    


    <!-- 
    ///////////////////////////////////////////////////////////////////////////////////////
    //
    // Data properties
    //
    ///////////////////////////////////////////////////////////////////////////////////////
     -->


    


    <!-- http://data.ign.fr/def/topo#artif -->


    <owl:DatatypeProperty rdf:about="http://data.ign.fr/def/topo#artif">
        <rdfs:domain rdf:resource="http://data.ign.fr/def/topo#CoursDEau"/>
        <rdfs:range rdf:resource="http://www.w3.org/2001/XMLSchema#boolean"/>
        <rdfs:comment xml:lang="en">Allows natural streams to be distinguished from artificial or artificialized streams.</rdfs:comment>
        <rdfs:comment xml:lang="fr">Permet de distinguer les cours d&apos;eau naturels des cours d&apos;eau artificiels ou artificialisés.</rdfs:comment>
        <rdfs:isDefinedBy rdf:resource="http://data.ign.fr/def/topo"/>
        <rdfs:label xml:lang="en">artificial</rdfs:label>
        <rdfs:label xml:lang="fr">artificiel</rdfs:label>
    </owl:DatatypeProperty>
    


    <!-- http://data.ign.fr/def/topo#codePostal -->


    <owl:DatatypeProperty rdf:about="http://data.ign.fr/def/topo#codePostal">
        <rdfs:domain rdf:resource="http://data.ign.fr/def/geofla#Commune"/>
        <rdfs:range rdf:resource="http://www.w3.org/2001/XMLSchema#integer"/>
        <rdfs:comment xml:lang="fr">Numéro de code postal.</rdfs:comment>
        <rdfs:comment xml:lang="en">Postal Code Number.</rdfs:comment>
        <rdfs:isDefinedBy rdf:resource="http://data.ign.fr/def/topo"/>
        <rdfs:label xml:lang="fr">code postal</rdfs:label>
        <rdfs:label xml:lang="en">postal code</rdfs:label>
    </owl:DatatypeProperty>
    


    <!-- http://data.ign.fr/def/topo#electrifie -->


    <owl:DatatypeProperty rdf:about="http://data.ign.fr/def/topo#electrifie">
        <rdfs:domain rdf:resource="http://data.ign.fr/def/topo#VoieFerree"/>
        <rdfs:range rdf:resource="http://www.w3.org/2001/XMLSchema#boolean"/>
        <rdfs:comment xml:lang="fr">Désigne le type d&apos;énergie servant à la propulsion des locomotives. Prends la valeur &apos;vrai&apos; s&apos;il s&apos;agit d&apos;une ligne électrifiée.</rdfs:comment>
        <rdfs:comment xml:lang="en">Refers to the type of energy used to propel locomotives. Take the value &apos;true&apos; if it is an electrified line.</rdfs:comment>
        <rdfs:isDefinedBy rdf:resource="http://data.ign.fr/def/topo"/>
        <rdfs:label xml:lang="en">electrified</rdfs:label>
        <rdfs:label xml:lang="fr">électrifié</rdfs:label>
    </owl:DatatypeProperty>
    


    <!-- http://data.ign.fr/def/topo#enConstruction -->


    <owl:DatatypeProperty rdf:about="http://data.ign.fr/def/topo#enConstruction">
        <rdfs:domain>
            <owl:Class>
                <owl:unionOf rdf:parseType="Collection">
                    <rdf:Description rdf:about="http://data.ign.fr/def/topo#Route"/>
                    <rdf:Description rdf:about="http://data.ign.fr/def/topo#VoieFerree"/>
                </owl:unionOf>
            </owl:Class>
        </rdfs:domain>
        <rdfs:range rdf:resource="http://www.w3.org/2001/XMLSchema#boolean"/>
        <rdfs:comment xml:lang="en">Indicates the state of an artificial topographic feature. Returns &apos;true&apos; if this entity is being built.</rdfs:comment>
        <rdfs:comment xml:lang="fr">Indique l&apos;état d&apos;une entité topographique artificielle. Renvoie &apos;vrai&apos; si cette entité est en cours de construction.</rdfs:comment>
        <rdfs:isDefinedBy rdf:resource="http://data.ign.fr/def/topo"/>
        <rdfs:label xml:lang="fr">en construction</rdfs:label>
        <rdfs:label xml:lang="en">under construction</rdfs:label>
    </owl:DatatypeProperty>
    


    <!-- http://data.ign.fr/def/topo#fictif -->


    <owl:DatatypeProperty rdf:about="http://data.ign.fr/def/topo#fictif">
        <rdfs:domain>
            <owl:Class>
                <owl:unionOf rdf:parseType="Collection">
                    <rdf:Description rdf:about="http://data.ign.fr/def/topo#CoursDEau"/>
                    <rdf:Description rdf:about="http://data.ign.fr/def/topo#Route"/>
                </owl:unionOf>
            </owl:Class>
        </rdfs:domain>
        <rdfs:range rdf:resource="http://www.w3.org/2001/XMLSchema#boolean"/>
        <rdfs:comment xml:lang="fr">La valeur &apos;oui&apos; indique que la géométrie du tronçon de réseau n&apos;est pas significative.</rdfs:comment>
        <rdfs:comment xml:lang="en">The value &apos;yes&apos; indicates that the geometry of the network section is not significant.</rdfs:comment>
        <rdfs:isDefinedBy rdf:resource="http://data.ign.fr/def/topo"/>
        <rdfs:label xml:lang="en">dummy</rdfs:label>
        <rdfs:label xml:lang="fr">fictif</rdfs:label>
    </owl:DatatypeProperty>
    


    <!-- http://data.ign.fr/def/topo#gestion -->


    <owl:DatatypeProperty rdf:about="http://data.ign.fr/def/topo#gestion">
        <rdfs:domain rdf:resource="http://data.ign.fr/def/topo#Route"/>
        <rdfs:range rdf:resource="http://www.w3.org/2001/XMLSchema#string"/>
        <rdfs:comment xml:lang="en">Defines the administrative manager of a route. All classified routes have a &apos;Manager&apos;.</rdfs:comment>
        <rdfs:comment xml:lang="fr">Définit le gestionnaire administratif d’une route. Toutes les routes classées possèdent un ‘Gestionnaire’.</rdfs:comment>
        <rdfs:isDefinedBy rdf:resource="http://data.ign.fr/def/topo"/>
        <rdfs:label xml:lang="fr">gestionnaire</rdfs:label>
        <rdfs:label xml:lang="en">manager</rdfs:label>
    </owl:DatatypeProperty>
    


    <!-- http://data.ign.fr/def/topo#hauteur -->


    <owl:DatatypeProperty rdf:about="http://data.ign.fr/def/topo#hauteur">
        <rdfs:domain rdf:resource="http://data.ign.fr/def/topo#Batiment"/>
        <rdfs:range rdf:resource="http://www.w3.org/2001/XMLSchema#integer"/>
        <rdfs:comment xml:lang="fr">Hauteur du bâtiment correspondant à la différence entre le Z le plus élevé du pourtour du bâtiment et un point situé au pied du bâtiment.</rdfs:comment>
        <rdfs:comment xml:lang="en">The height of the building corresponding to the difference between the highest Z around the building and a point at the foot of the building.</rdfs:comment>
        <rdfs:isDefinedBy rdf:resource="http://data.ign.fr/def/topo"/>
        <rdfs:label xml:lang="fr">hauteur</rdfs:label>
        <rdfs:label xml:lang="en">height</rdfs:label>
    </owl:DatatypeProperty>
    


    <!-- http://data.ign.fr/def/topo#importance -->


    <owl:DatatypeProperty rdf:about="http://data.ign.fr/def/topo#importance">
        <rdfs:domain rdf:resource="http://data.ign.fr/def/topo#EntiteTopographique"/>
        <rdfs:range>
            <rdfs:Datatype>
                <owl:oneOf>
                    <rdf:Description>
                        <rdf:type rdf:resource="http://www.w3.org/1999/02/22-rdf-syntax-ns#List"/>
                        <rdf:first>1</rdf:first>
                        <rdf:rest>
                            <rdf:Description>
                                <rdf:type rdf:resource="http://www.w3.org/1999/02/22-rdf-syntax-ns#List"/>
                                <rdf:first>2</rdf:first>
                                <rdf:rest>
                                    <rdf:Description>
                                        <rdf:type rdf:resource="http://www.w3.org/1999/02/22-rdf-syntax-ns#List"/>
                                        <rdf:first>3</rdf:first>
                                        <rdf:rest>
                                            <rdf:Description>
                                                <rdf:type rdf:resource="http://www.w3.org/1999/02/22-rdf-syntax-ns#List"/>
                                                <rdf:first>4</rdf:first>
                                                <rdf:rest>
                                                    <rdf:Description>
                                                        <rdf:type rdf:resource="http://www.w3.org/1999/02/22-rdf-syntax-ns#List"/>
                                                        <rdf:first>5</rdf:first>
                                                        <rdf:rest>
                                                            <rdf:Description>
                                                                <rdf:type rdf:resource="http://www.w3.org/1999/02/22-rdf-syntax-ns#List"/>
                                                                <rdf:first>6</rdf:first>
                                                                <rdf:rest>
                                                                    <rdf:Description>
                                                                        <rdf:type rdf:resource="http://www.w3.org/1999/02/22-rdf-syntax-ns#List"/>
                                                                        <rdf:first>7</rdf:first>
                                                                        <rdf:rest>
                                                                            <rdf:Description>
                                                                                <rdf:type rdf:resource="http://www.w3.org/1999/02/22-rdf-syntax-ns#List"/>
                                                                                <rdf:first>8</rdf:first>
                                                                                <rdf:rest>
                                                                                    <rdf:Description>
                                                                                        <rdf:type rdf:resource="http://www.w3.org/1999/02/22-rdf-syntax-ns#List"/>
                                                                                        <rdf:first>NC</rdf:first>
                                                                                        <rdf:rest>
                                                                                            <rdf:Description>
                                                                                                <rdf:type rdf:resource="http://www.w3.org/1999/02/22-rdf-syntax-ns#List"/>
                                                                                                <rdf:first>NR</rdf:first>
                                                                                                <rdf:rest rdf:resource="http://www.w3.org/1999/02/22-rdf-syntax-ns#nil"/>
                                                                                            </rdf:Description>
                                                                                        </rdf:rest>
                                                                                    </rdf:Description>
                                                                                </rdf:rest>
                                                                            </rdf:Description>
                                                                        </rdf:rest>
                                                                    </rdf:Description>
                                                                </rdf:rest>
                                                            </rdf:Description>
                                                        </rdf:rest>
                                                    </rdf:Description>
                                                </rdf:rest>
                                            </rdf:Description>
                                        </rdf:rest>
                                    </rdf:Description>
                                </rdf:rest>
                            </rdf:Description>
                        </rdf:rest>
                    </rdf:Description>
                </owl:oneOf>
            </rdfs:Datatype>
        </rdfs:range>
        <rdfs:comment xml:lang="fr">Importance du toponyme dans son environnement. Le toponyme de valeur 1 est plus important que le toponyme de valeur 2, lui-même plus important que le toponyme de valeur 3, etc.</rdfs:comment>
        <rdfs:comment xml:lang="en">Importance of the place name in its environment. The toponym of value 1 is more important than the toponym of value 2, itself more important than the toponym of value 3, etc.</rdfs:comment>
        <rdfs:isDefinedBy rdf:resource="http://data.ign.fr/def/topo"/>
        <rdfs:label xml:lang="en">importance</rdfs:label>
        <rdfs:label xml:lang="fr">importance</rdfs:label>
    </owl:DatatypeProperty>
    


    <!-- http://data.ign.fr/def/topo#itEurop -->


    <owl:DatatypeProperty rdf:about="http://data.ign.fr/def/topo#itEurop">
        <rdfs:domain rdf:resource="http://data.ign.fr/def/topo#Route"/>
        <rdfs:range rdf:resource="http://www.w3.org/2001/XMLSchema#string"/>
        <rdfs:comment xml:lang="en">European road number: a European road generally uses the motorway or national network (exceptionally departmental or unclassified).</rdfs:comment>
        <rdfs:comment xml:lang="fr">Numéro de route européenne : une route européenne emprunte en général le réseau autoroutier ou national (exceptionnellement départemental ou non classé).</rdfs:comment>
        <rdfs:isDefinedBy rdf:resource="http://data.ign.fr/def/topo"/>
        <rdfs:label xml:lang="en">european itinerary</rdfs:label>
        <rdfs:label xml:lang="fr">itinéraire européen</rdfs:label>
    </owl:DatatypeProperty>
    


    <!-- http://data.ign.fr/def/topo#itVert -->


    <owl:DatatypeProperty rdf:about="http://data.ign.fr/def/topo#itVert">
        <rdfs:domain rdf:resource="http://data.ign.fr/def/topo#Route"/>
        <rdfs:range rdf:resource="http://www.w3.org/2001/XMLSchema#boolean"/>
        <rdfs:comment xml:lang="en">Indicates whether or not a road segment belongs to the green network. The green network, made up of green poles and green links, covers the entire French territory. The green poles are made up of communes of more than 23,000 inhabitants in the province and 39,000 inhabitants in Ile-de-France, as well as certain poles of administrative, economic, tourist or industrial activities. We only remember the green transit network between green poles. The green network of drawdown, inside the cities, and the green network recommended to the trucks are not retained.</rdfs:comment>
        <rdfs:comment xml:lang="fr">Indique l’appartenance ou non d’un tronçon routier au réseau vert. Le réseau vert, composé de pôles verts et de liaisons vertes, couvre l’ensemble du territoire français. Les pôles verts sont composés de communes de plus de 23.000 habitants en province et de 39.000 habitants en Ile-de-France, ainsi que certains pôles d’activités administratifs, économiques, touristiques ou industriels. On retient seulement le réseau vert de transit entre pôles verts. Le réseau vert de rabattement, à l’intérieur des villes, et le réseau vert conseillé aux poids lourds ne sont pas retenus.</rdfs:comment>
        <rdfs:isDefinedBy rdf:resource="http://data.ign.fr/def/topo"/>
        <rdfs:label xml:lang="en">green itinerary</rdfs:label>
        <rdfs:label xml:lang="fr">itinéraire vert</rdfs:label>
    </owl:DatatypeProperty>
    


    <!-- http://data.ign.fr/def/topo#largeurChaussee -->


    <owl:DatatypeProperty rdf:about="http://data.ign.fr/def/topo#largeurChaussee">
        <rdfs:domain rdf:resource="http://data.ign.fr/def/topo#Route"/>
        <rdfs:range rdf:resource="http://www.w3.org/2001/XMLSchema#double"/>
        <rdfs:comment xml:lang="fr">Largeur de chaussée (d’accotement à accotement) exprimée en mètres.</rdfs:comment>
        <rdfs:comment xml:lang="en">Width of road (shoulder shoulders) expressed in meters.</rdfs:comment>
        <rdfs:isDefinedBy rdf:resource="http://data.ign.fr/def/topo"/>
        <rdfs:label xml:lang="en">carriageway width</rdfs:label>
        <rdfs:label xml:lang="fr">largeur de chaussée</rdfs:label>
    </owl:DatatypeProperty>
    


    <!-- http://data.ign.fr/def/topo#largeurVF -->


    <owl:DatatypeProperty rdf:about="http://data.ign.fr/def/topo#largeurVF">
        <rdfs:domain rdf:resource="http://data.ign.fr/def/topo#VoieFerree"/>
        <rdfs:range>
            <rdfs:Datatype>
                <owl:oneOf>
                    <rdf:Description>
                        <rdf:type rdf:resource="http://www.w3.org/1999/02/22-rdf-syntax-ns#List"/>
                        <rdf:first>large</rdf:first>
                        <rdf:rest>
                            <rdf:Description>
                                <rdf:type rdf:resource="http://www.w3.org/1999/02/22-rdf-syntax-ns#List"/>
                                <rdf:first>narrow</rdf:first>
                                <rdf:rest>
                                    <rdf:Description>
                                        <rdf:type rdf:resource="http://www.w3.org/1999/02/22-rdf-syntax-ns#List"/>
                                        <rdf:first>normal</rdf:first>
                                        <rdf:rest>
                                            <rdf:Description>
                                                <rdf:type rdf:resource="http://www.w3.org/1999/02/22-rdf-syntax-ns#List"/>
                                                <rdf:first>normale</rdf:first>
                                                <rdf:rest>
                                                    <rdf:Description>
                                                        <rdf:type rdf:resource="http://www.w3.org/1999/02/22-rdf-syntax-ns#List"/>
                                                        <rdf:first>étroite</rdf:first>
                                                        <rdf:rest rdf:resource="http://www.w3.org/1999/02/22-rdf-syntax-ns#nil"/>
                                                    </rdf:Description>
                                                </rdf:rest>
                                            </rdf:Description>
                                        </rdf:rest>
                                    </rdf:Description>
                                </rdf:rest>
                            </rdf:Description>
                        </rdf:rest>
                    </rdf:Description>
                </owl:oneOf>
            </rdfs:Datatype>
        </rdfs:range>
        <rdfs:comment xml:lang="fr">Attribut permettant de distinguer les voies ferrées de largeur standard (normale) pour la France (1,435 m), des voies ferrées plus larges ou plus étroites.</rdfs:comment>
        <rdfs:comment xml:lang="en">Attribute distinguishing between standard width (normal) railways for France (1.435 m), wider or narrower railways.</rdfs:comment>
        <rdfs:isDefinedBy rdf:resource="http://data.ign.fr/def/topo"/>
        <rdfs:label xml:lang="fr">largeur de la voie ferrée</rdfs:label>
        <rdfs:label xml:lang="en">railway track width</rdfs:label>
    </owl:DatatypeProperty>
    


    <!-- http://data.ign.fr/def/topo#militaire -->


    <owl:DatatypeProperty rdf:about="http://data.ign.fr/def/topo#militaire">
        <rdfs:domain>
            <owl:Class>
                <owl:unionOf rdf:parseType="Collection">
                    <rdf:Description rdf:about="http://data.ign.fr/def/topo#Cimetiere"/>
                    <owl:Restriction>
                        <owl:onProperty rdf:resource="http://data.ign.fr/def/topo#nature"/>
                        <owl:hasValue rdf:resource="http://data.ign.fr/id/codes/topo/typedezai/Aerodrome"/>
                    </owl:Restriction>
                </owl:unionOf>
            </owl:Class>
        </rdfs:domain>
        <rdfs:range rdf:resource="http://www.w3.org/2001/XMLSchema#boolean"/>
        <rdfs:comment xml:lang="fr">Attribut permettant de distinguer une entité topographique à vocation militaire ou simplement gérée par le ministère de la défense d&apos;une entité civile. La valeur « vrai » est également affectée aux cimetières militaires gérés par le Ministère des Anciens Combattants ou par des états étrangers.</rdfs:comment>
        <rdfs:comment xml:lang="en">Attribute to distinguish a topographic entity with a military purpose or simply managed by the Ministry of Defense of a civil entity. The true value is also assigned to military cemeteries operated by the Department of Veterans Affairs or foreign states.</rdfs:comment>
        <rdfs:isDefinedBy rdf:resource="http://data.ign.fr/def/topo"/>
        <rdfs:label xml:lang="fr">entité à vocation militaire</rdfs:label>
        <rdfs:label xml:lang="en">military feature</rdfs:label>
    </owl:DatatypeProperty>
    


    <!-- http://data.ign.fr/def/topo#miseEnService -->


    <owl:DatatypeProperty rdf:about="http://data.ign.fr/def/topo#miseEnService">
        <rdfs:domain rdf:resource="http://data.ign.fr/def/topo#Route"/>
        <rdfs:range rdf:resource="http://www.w3.org/2001/XMLSchema#string"/>
        <rdfs:comment xml:lang="en">Defines the planned date or effective date of bringing a section of road into service. This attribute is only filled for sections under construction, it is at &quot;NR&quot; in other cases. Sections with a date of commissioning are completely closed to vehicles before that date.</rdfs:comment>
        <rdfs:comment xml:lang="fr">Définit la date prévue ou la date effective de mise en service d’un tronçon de route. Cet attribut n&apos;est rempli que pour les tronçons en construction, il est à “NR“ dans les autres cas. Les tronçons qui possèdent une date de mise en service sont complètement fermés aux véhicules avant cette date.</rdfs:comment>
        <rdfs:isDefinedBy rdf:resource="http://data.ign.fr/def/topo"/>
        <rdfs:label xml:lang="fr">date de mise en service</rdfs:label>
        <rdfs:label xml:lang="en">in service date</rdfs:label>
    </owl:DatatypeProperty>
    


    <!-- http://data.ign.fr/def/topo#nbVoiesCirculation -->


    <owl:DatatypeProperty rdf:about="http://data.ign.fr/def/topo#nbVoiesCirculation">
        <rdfs:domain rdf:resource="http://data.ign.fr/def/topo#Route"/>
        <rdfs:range rdf:resource="http://www.w3.org/2001/XMLSchema#integer"/>
        <rdfs:comment xml:lang="fr">Nombre total de voies d’une route, d’une rue ou d’une chaussée de route à chaussées séparées.</rdfs:comment>
        <rdfs:comment xml:lang="en">Total number of lanes on a road, street or pavement with separate carriageways.</rdfs:comment>
        <rdfs:isDefinedBy rdf:resource="http://data.ign.fr/def/topo"/>
        <rdfs:label xml:lang="fr">nombre de voies de circulation</rdfs:label>
        <rdfs:label xml:lang="en">number of traffic lanes</rdfs:label>
    </owl:DatatypeProperty>
    


    <!-- http://data.ign.fr/def/topo#nbVoiesFerrees -->


    <owl:DatatypeProperty rdf:about="http://data.ign.fr/def/topo#nbVoiesFerrees">
        <rdfs:domain rdf:resource="http://data.ign.fr/def/topo#VoieFerree"/>
        <rdfs:range rdf:resource="http://www.w3.org/2001/XMLSchema#integer"/>
        <rdfs:comment xml:lang="fr">Nombre de voies constituant cette portion de ligne de chemin de fer. La valeur 0 indique que le nombre de voies est inconnu.</rdfs:comment>
        <rdfs:comment xml:lang="en">Number of lanes constituting this portion of a railway line. A value of 0 indicates that the number of channels is unknown.</rdfs:comment>
        <rdfs:isDefinedBy rdf:resource="http://data.ign.fr/def/topo"/>
        <rdfs:label xml:lang="fr">nombre de voies ferrées</rdfs:label>
        <rdfs:label xml:lang="en">number of tracks</rdfs:label>
    </owl:DatatypeProperty>
    


    <!-- http://data.ign.fr/def/topo#nomIti -->


    <owl:DatatypeProperty rdf:about="http://data.ign.fr/def/topo#nomIti">
        <rdfs:domain rdf:resource="http://data.ign.fr/def/topo#Route"/>
        <rdfs:range rdf:resource="http://www.w3.org/2001/XMLSchema#string"/>
        <rdfs:comment xml:lang="en">Define a named route.</rdfs:comment>
        <rdfs:comment xml:lang="fr">Définit un parcours routier nommé.</rdfs:comment>
        <rdfs:isDefinedBy rdf:resource="http://data.ign.fr/def/topo"/>
        <rdfs:label xml:lang="en">name of itinerary</rdfs:label>
        <rdfs:label xml:lang="fr">nom d&apos;itinéraire</rdfs:label>
    </owl:DatatypeProperty>
    


    <!-- http://data.ign.fr/def/topo#numero -->


    <owl:DatatypeProperty rdf:about="http://data.ign.fr/def/topo#numero">
        <rdfs:domain rdf:resource="http://data.ign.fr/def/topo#Route"/>
        <rdfs:range rdf:resource="http://www.w3.org/2001/XMLSchema#string"/>
        <rdfs:comment xml:lang="fr">Désigne le classement administratif d&apos;un tronçon routier.</rdfs:comment>
        <rdfs:comment xml:lang="en">Refers to the administrative classification of a road section.</rdfs:comment>
        <rdfs:isDefinedBy rdf:resource="http://data.ign.fr/def/topo"/>
        <rdfs:label xml:lang="en">number</rdfs:label>
        <rdfs:label xml:lang="fr">numéro</rdfs:label>
    </owl:DatatypeProperty>
    


    <!-- http://data.ign.fr/def/topo#numeroBorne -->


    <owl:DatatypeProperty rdf:about="http://data.ign.fr/def/topo#numeroBorne">
        <rdfs:domain rdf:resource="http://data.ign.fr/def/topo#BornePostale"/>
        <rdfs:range rdf:resource="http://www.w3.org/2001/XMLSchema#integer"/>
        <rdfs:comment xml:lang="fr">Numéro de borne postale.</rdfs:comment>
        <rdfs:comment xml:lang="en">Postal code number.</rdfs:comment>
        <rdfs:isDefinedBy rdf:resource="http://data.ign.fr/def/topo"/>
        <rdfs:label xml:lang="en">civic number</rdfs:label>
        <rdfs:label xml:lang="fr">numéro de borne postale</rdfs:label>
    </owl:DatatypeProperty>
    


    <!-- http://data.ign.fr/def/topo#posSol -->


    <owl:DatatypeProperty rdf:about="http://data.ign.fr/def/topo#posSol">
        <rdfs:domain rdf:resource="http://data.ign.fr/def/topo#Conduite"/>
        <rdfs:range rdf:resource="http://www.w3.org/2001/XMLSchema#integer"/>
        <rdfs:comment xml:lang="fr">Position par rapport au sol. Donne le niveau de l’objet par rapport à la surface du sol (valeur nulle pour un objet au sol, négative pour un objet situé au-dessous du niveau du sol et positive pour un objet en sursol).</rdfs:comment>
        <rdfs:comment xml:lang="en">Position relative to the ground. Gives the level of the object relative to the ground surface (zero value for a ground object, negative for an object below ground level and positive for an object on the ground).</rdfs:comment>
        <rdfs:isDefinedBy rdf:resource="http://data.ign.fr/def/topo"/>
        <rdfs:label xml:lang="en">position in relation to the ground</rdfs:label>
        <rdfs:label xml:lang="fr">position par rapport au sol</rdfs:label>
    </owl:DatatypeProperty>
    


    <!-- http://data.ign.fr/def/topo#precAlti -->


    <owl:DatatypeProperty rdf:about="http://data.ign.fr/def/topo#precAlti">
        <rdfs:domain rdf:resource="http://data.ign.fr/def/topo#EntiteTopographique"/>
        <rdfs:range rdf:resource="http://www.w3.org/2001/XMLSchema#double"/>
        <rdfs:comment xml:lang="en">Geometric altimetric accuracy.</rdfs:comment>
        <rdfs:comment xml:lang="fr">Précision géométrique altimétrique.</rdfs:comment>
        <rdfs:isDefinedBy rdf:resource="http://data.ign.fr/def/topo"/>
        <rdfs:label xml:lang="en">altimetric accuracy</rdfs:label>
        <rdfs:label xml:lang="fr">précision altimétrique</rdfs:label>
    </owl:DatatypeProperty>
    


    <!-- http://data.ign.fr/def/topo#precPlani -->


    <owl:DatatypeProperty rdf:about="http://data.ign.fr/def/topo#precPlani">
        <rdfs:domain rdf:resource="http://data.ign.fr/def/topo#EntiteTopographique"/>
        <rdfs:range rdf:resource="http://www.w3.org/2001/XMLSchema#double"/>
        <rdfs:comment xml:lang="en">Planimetric geometric precision.</rdfs:comment>
        <rdfs:comment xml:lang="fr">Précision géométrique planimétrique.</rdfs:comment>
        <rdfs:isDefinedBy rdf:resource="http://data.ign.fr/def/topo"/>
        <rdfs:label xml:lang="en">planimetric accuracy</rdfs:label>
        <rdfs:label xml:lang="fr">précision planimétrique</rdfs:label>
    </owl:DatatypeProperty>
    


    <!-- http://data.ign.fr/def/topo#regime -->


    <owl:DatatypeProperty rdf:about="http://data.ign.fr/def/topo#regime">
        <rdfs:domain rdf:resource="http://data.ign.fr/def/topo#CoursDEau"/>
        <rdfs:range>
            <rdfs:Datatype>
                <owl:oneOf>
                    <rdf:Description>
                        <rdf:type rdf:resource="http://www.w3.org/1999/02/22-rdf-syntax-ns#List"/>
                        <rdf:first>intermittent</rdf:first>
                        <rdf:rest>
                            <rdf:Description>
                                <rdf:type rdf:resource="http://www.w3.org/1999/02/22-rdf-syntax-ns#List"/>
                                <rdf:first>permanent</rdf:first>
                                <rdf:rest rdf:resource="http://www.w3.org/1999/02/22-rdf-syntax-ns#nil"/>
                            </rdf:Description>
                        </rdf:rest>
                    </rdf:Description>
                </owl:oneOf>
            </rdfs:Datatype>
        </rdfs:range>
        <rdfs:comment xml:lang="fr">Attribut permettant de caractériser un objet hydrographique en fonction du régime des eaux.</rdfs:comment>
        <rdfs:comment xml:lang="en">Attribute to characterize a hydrographic object according to the water regime.</rdfs:comment>
        <rdfs:isDefinedBy rdf:resource="http://data.ign.fr/def/topo"/>
        <rdfs:label xml:lang="fr">régime des eaux</rdfs:label>
        <rdfs:label xml:lang="en">water regime</rdfs:label>
    </owl:DatatypeProperty>
    


    <!-- http://data.ign.fr/def/topo#sens -->


    <owl:DatatypeProperty rdf:about="http://data.ign.fr/def/topo#sens">
        <rdfs:domain rdf:resource="http://data.ign.fr/def/topo#Route"/>
        <rdfs:range>
            <rdfs:Datatype>
                <owl:oneOf>
                    <rdf:Description>
                        <rdf:type rdf:resource="http://www.w3.org/1999/02/22-rdf-syntax-ns#List"/>
                        <rdf:first>NC</rdf:first>
                        <rdf:rest>
                            <rdf:Description>
                                <rdf:type rdf:resource="http://www.w3.org/1999/02/22-rdf-syntax-ns#List"/>
                                <rdf:first>NR</rdf:first>
                                <rdf:rest>
                                    <rdf:Description>
                                        <rdf:type rdf:resource="http://www.w3.org/1999/02/22-rdf-syntax-ns#List"/>
                                        <rdf:first>direct</rdf:first>
                                        <rdf:rest>
                                            <rdf:Description>
                                                <rdf:type rdf:resource="http://www.w3.org/1999/02/22-rdf-syntax-ns#List"/>
                                                <rdf:first>double</rdf:first>
                                                <rdf:rest>
                                                    <rdf:Description>
                                                        <rdf:type rdf:resource="http://www.w3.org/1999/02/22-rdf-syntax-ns#List"/>
                                                        <rdf:first>inverse</rdf:first>
                                                        <rdf:rest rdf:resource="http://www.w3.org/1999/02/22-rdf-syntax-ns#nil"/>
                                                    </rdf:Description>
                                                </rdf:rest>
                                            </rdf:Description>
                                        </rdf:rest>
                                    </rdf:Description>
                                </rdf:rest>
                            </rdf:Description>
                        </rdf:rest>
                    </rdf:Description>
                </owl:oneOf>
            </rdfs:Datatype>
        </rdfs:range>
        <rdfs:comment xml:lang="en">Permitted traffic direction for cars on tracks.</rdfs:comment>
        <rdfs:comment xml:lang="fr">Sens de circulation autorisée pour les automobiles sur les voies.</rdfs:comment>
        <rdfs:isDefinedBy rdf:resource="http://data.ign.fr/def/topo"/>
        <rdfs:label xml:lang="en">direction of traffic</rdfs:label>
        <rdfs:label xml:lang="fr">sens de circulation</rdfs:label>
    </owl:DatatypeProperty>
    


    <!-- http://data.ign.fr/def/topo#typAdres -->


    <owl:DatatypeProperty rdf:about="http://data.ign.fr/def/topo#typAdres">
        <rdfs:domain rdf:resource="http://data.ign.fr/def/topo#Route"/>
        <rdfs:range>
            <rdfs:Datatype>
                <owl:oneOf>
                    <rdf:Description>
                        <rdf:type rdf:resource="http://www.w3.org/1999/02/22-rdf-syntax-ns#List"/>
                        <rdf:first>NC</rdf:first>
                        <rdf:rest>
                            <rdf:Description>
                                <rdf:type rdf:resource="http://www.w3.org/1999/02/22-rdf-syntax-ns#List"/>
                                <rdf:first>NR</rdf:first>
                                <rdf:rest>
                                    <rdf:Description>
                                        <rdf:type rdf:resource="http://www.w3.org/1999/02/22-rdf-syntax-ns#List"/>
                                        <rdf:first>autre</rdf:first>
                                        <rdf:rest>
                                            <rdf:Description>
                                                <rdf:type rdf:resource="http://www.w3.org/1999/02/22-rdf-syntax-ns#List"/>
                                                <rdf:first>classique</rdf:first>
                                                <rdf:rest>
                                                    <rdf:Description>
                                                        <rdf:type rdf:resource="http://www.w3.org/1999/02/22-rdf-syntax-ns#List"/>
                                                        <rdf:first>linéaire</rdf:first>
                                                        <rdf:rest>
                                                            <rdf:Description>
                                                                <rdf:type rdf:resource="http://www.w3.org/1999/02/22-rdf-syntax-ns#List"/>
                                                                <rdf:first>métrique</rdf:first>
                                                                <rdf:rest rdf:resource="http://www.w3.org/1999/02/22-rdf-syntax-ns#nil"/>
                                                            </rdf:Description>
                                                        </rdf:rest>
                                                    </rdf:Description>
                                                </rdf:rest>
                                            </rdf:Description>
                                        </rdf:rest>
                                    </rdf:Description>
                                </rdf:rest>
                            </rdf:Description>
                        </rdf:rest>
                    </rdf:Description>
                </owl:oneOf>
            </rdfs:Datatype>
        </rdfs:range>
        <rdfs:comment xml:lang="en">Provides information on the type of addressing of the section.</rdfs:comment>
        <rdfs:comment xml:lang="fr">Renseigne sur le type d’adressage du tronçon.</rdfs:comment>
        <rdfs:isDefinedBy rdf:resource="http://data.ign.fr/def/topo"/>
        <rdfs:label xml:lang="fr">type d’adressage</rdfs:label>
        <rdfs:label xml:lang="en">type of addressing</rdfs:label>
    </owl:DatatypeProperty>
    


    <!-- http://data.ign.fr/def/topo#typeDePiste -->


    <owl:DatatypeProperty rdf:about="http://data.ign.fr/def/topo#typeDePiste">
        <rdfs:domain rdf:resource="http://data.ign.fr/def/topo#PisteAerodrome"/>
        <rdfs:range>
            <rdfs:Datatype>
                <owl:oneOf>
                    <rdf:Description>
                        <rdf:type rdf:resource="http://www.w3.org/1999/02/22-rdf-syntax-ns#List"/>
                        <rdf:first>Piste aménagée sur de l&apos;herbe</rdf:first>
                        <rdf:rest>
                            <rdf:Description>
                                <rdf:type rdf:resource="http://www.w3.org/1999/02/22-rdf-syntax-ns#List"/>
                                <rdf:first>Piste aménagée sur une surface dure</rdf:first>
                                <rdf:rest>
                                    <rdf:Description>
                                        <rdf:type rdf:resource="http://www.w3.org/1999/02/22-rdf-syntax-ns#List"/>
                                        <rdf:first>Track arranged on grass</rdf:first>
                                        <rdf:rest>
                                            <rdf:Description>
                                                <rdf:type rdf:resource="http://www.w3.org/1999/02/22-rdf-syntax-ns#List"/>
                                                <rdf:first>Track laid out on a hard surface</rdf:first>
                                                <rdf:rest rdf:resource="http://www.w3.org/1999/02/22-rdf-syntax-ns#nil"/>
                                            </rdf:Description>
                                        </rdf:rest>
                                    </rdf:Description>
                                </rdf:rest>
                            </rdf:Description>
                        </rdf:rest>
                    </rdf:Description>
                </owl:oneOf>
            </rdfs:Datatype>
        </rdfs:range>
        <rdfs:comment xml:lang="fr">Attribut permettant de distinguer différentes natures d&apos;aérodrome.</rdfs:comment>
        <rdfs:comment xml:lang="en">Attribute to distinguish different types of aerodrome.</rdfs:comment>
        <rdfs:isDefinedBy rdf:resource="http://data.ign.fr/def/topo"/>
        <rdfs:label xml:lang="fr">type de piste</rdfs:label>
        <rdfs:label xml:lang="en">type of taxiway</rdfs:label>
    </owl:DatatypeProperty>
    


    <!-- http://data.ign.fr/def/topo#voltage -->


    <owl:DatatypeProperty rdf:about="http://data.ign.fr/def/topo#voltage">
        <rdfs:domain rdf:resource="http://data.ign.fr/def/topo#LigneElectrique"/>
        <rdfs:range>
            <rdfs:Datatype>
                <owl:oneOf>
                    <rdf:Description>
                        <rdf:type rdf:resource="http://www.w3.org/1999/02/22-rdf-syntax-ns#List"/>
                        <rdf:first>150</rdf:first>
                        <rdf:rest>
                            <rdf:Description>
                                <rdf:type rdf:resource="http://www.w3.org/1999/02/22-rdf-syntax-ns#List"/>
                                <rdf:first>225</rdf:first>
                                <rdf:rest>
                                    <rdf:Description>
                                        <rdf:type rdf:resource="http://www.w3.org/1999/02/22-rdf-syntax-ns#List"/>
                                        <rdf:first>400</rdf:first>
                                        <rdf:rest>
                                            <rdf:Description>
                                                <rdf:type rdf:resource="http://www.w3.org/1999/02/22-rdf-syntax-ns#List"/>
                                                <rdf:first>63</rdf:first>
                                                <rdf:rest>
                                                    <rdf:Description>
                                                        <rdf:type rdf:resource="http://www.w3.org/1999/02/22-rdf-syntax-ns#List"/>
                                                        <rdf:first>90</rdf:first>
                                                        <rdf:rest>
                                                            <rdf:Description>
                                                                <rdf:type rdf:resource="http://www.w3.org/1999/02/22-rdf-syntax-ns#List"/>
                                                                <rdf:first>NR</rdf:first>
                                                                <rdf:rest rdf:resource="http://www.w3.org/1999/02/22-rdf-syntax-ns#nil"/>
                                                            </rdf:Description>
                                                        </rdf:rest>
                                                    </rdf:Description>
                                                </rdf:rest>
                                            </rdf:Description>
                                        </rdf:rest>
                                    </rdf:Description>
                                </rdf:rest>
                            </rdf:Description>
                        </rdf:rest>
                    </rdf:Description>
                </owl:oneOf>
            </rdfs:Datatype>
        </rdfs:range>
        <rdfs:comment xml:lang="fr">Tension de construction de la ligne électrique en kV (kilo Volts).</rdfs:comment>
        <rdfs:comment xml:lang="en">Voltage of construction of the electric line in kV (kilo volts).</rdfs:comment>
        <rdfs:isDefinedBy rdf:resource="http://data.ign.fr/def/topo"/>
        <rdfs:label xml:lang="en">voltage</rdfs:label>
        <rdfs:label xml:lang="fr">voltage</rdfs:label>
    </owl:DatatypeProperty>
    


    <!-- http://data.ign.fr/def/topo#zFin -->


    <owl:DatatypeProperty rdf:about="http://data.ign.fr/def/topo#zFin">
        <rdfs:domain>
            <owl:Class>
                <owl:intersectionOf rdf:parseType="Collection">
                    <rdf:Description rdf:about="http://data.ign.fr/def/topo#EntiteTopographique"/>
                    <owl:Restriction>
                        <owl:onProperty rdf:resource="http://data.ign.fr/def/geometrie#geometry"/>
                        <owl:someValuesFrom rdf:resource="http://data.ign.fr/def/geometrie#Curve"/>
                    </owl:Restriction>
                </owl:intersectionOf>
            </owl:Class>
        </rdfs:domain>
        <rdfs:range rdf:resource="http://www.w3.org/2001/XMLSchema#double"/>
        <rdfs:comment xml:lang="fr">Altitude du sommet final d&apos;une portion d&apos;élément linéaire d&apos;un réseau.</rdfs:comment>
        <rdfs:comment xml:lang="en">Altitude of the final peak of a linear element portion of a network.</rdfs:comment>
        <rdfs:isDefinedBy rdf:resource="http://data.ign.fr/def/topo"/>
        <rdfs:label xml:lang="en">final z</rdfs:label>
        <rdfs:label xml:lang="fr">z final</rdfs:label>
    </owl:DatatypeProperty>
    


    <!-- http://data.ign.fr/def/topo#zIni -->


    <owl:DatatypeProperty rdf:about="http://data.ign.fr/def/topo#zIni">
        <rdfs:domain>
            <owl:Class>
                <owl:intersectionOf rdf:parseType="Collection">
                    <rdf:Description rdf:about="http://data.ign.fr/def/topo#EntiteTopographique"/>
                    <owl:Restriction>
                        <owl:onProperty rdf:resource="http://data.ign.fr/def/geometrie#geometry"/>
                        <owl:someValuesFrom rdf:resource="http://data.ign.fr/def/geometrie#Curve"/>
                    </owl:Restriction>
                </owl:intersectionOf>
            </owl:Class>
        </rdfs:domain>
        <rdfs:range rdf:resource="http://www.w3.org/2001/XMLSchema#double"/>
        <rdfs:comment xml:lang="fr">Altitude du sommet initial d&apos;une portion d&apos;élément linéaire d&apos;un réseau.</rdfs:comment>
        <rdfs:comment xml:lang="en">Altitude of the initial vertex of a linear element portion of a network.</rdfs:comment>
        <rdfs:isDefinedBy rdf:resource="http://data.ign.fr/def/topo"/>
        <rdfs:label xml:lang="en">initial z</rdfs:label>
        <rdfs:label xml:lang="fr">z initial</rdfs:label>
    </owl:DatatypeProperty>
    


    <!-- http://data.ign.fr/def/topo#zMax -->


    <owl:DatatypeProperty rdf:about="http://data.ign.fr/def/topo#zMax">
        <rdfs:domain rdf:resource="http://data.ign.fr/def/topo#EntiteTopographique"/>
        <rdfs:range rdf:resource="http://www.w3.org/2001/XMLSchema#double"/>
        <rdfs:comment xml:lang="fr">Altitude maximale d’un objet linéaire ou surfacique. Cette information est issue de la saisie photogrammétrique et concerne des objets dont les points initiaux et finaux ne sont pas caractéristiques de l’altitude de l’objet (objets surfaciques, objets linéaires isolés). Pour des objets surfaciques comme les bâtiments ou les réservoirs, il s’agit de l’altitude maximum du pourtour tel qu’il est défini en planimétrie (généralement l’altitude aux gouttières) et non de l’altitude maximum absolue (voir schéma ci-dessus). Dans le cas d’un bâtiment obtenu après intégration du bâti issu du cadastre, Z_MAX correspond à une altitude toit médiane calculée, en prenant en compte les altitudes des contours des bâtiments directement contigus s’ils existent. Dans ce cas Z_MAX et Z_MIN prennent la même valeur. L’attribut peut prendre une valeur conventionnelle (9999) lorsque la géométrie de l’objet n’est pas issue d’une saisie photogrammétrique (ex. objets numérisés sur la carte en service). </rdfs:comment>
        <rdfs:comment xml:lang="en">Maximum altitude of a linear or polygon object. This information comes from the photogrammetric input and concerns objects whose initial and final points are not characteristic of the altitude of the object (surface objects, isolated linear objects). For areal objects such as buildings or reservoirs, this is the maximum altitude of the circumference as it is defined in planimetry (usually the altitude at the gutters) and not the absolute maximum altitude (see diagram below). -above). In the case of a building obtained after integration of the frame from the cadastre, Z_MAX corresponds to a computed median roof altitude, taking into account the altitudes of the outlines of buildings directly adjacent if they exist. In this case Z_MAX and Z_MIN take the same value. The attribute can take a conventional value (9999) when the geometry of the object is not the result of a photogrammetric capture (eg objects scanned on the map in use).</rdfs:comment>
        <rdfs:isDefinedBy rdf:resource="http://data.ign.fr/def/topo"/>
        <rdfs:label xml:lang="en">max z</rdfs:label>
        <rdfs:label xml:lang="fr">z max</rdfs:label>
    </owl:DatatypeProperty>
    


    <!-- http://data.ign.fr/def/topo#zMin -->


    <owl:DatatypeProperty rdf:about="http://data.ign.fr/def/topo#zMin">
        <rdfs:domain rdf:resource="http://data.ign.fr/def/topo#EntiteTopographique"/>
        <rdfs:range rdf:resource="http://www.w3.org/2001/XMLSchema#double"/>
        <rdfs:comment xml:lang="fr">Altitude minimale d’un objet linéaire ou surfacique. Cette information est issue de la saisie photogrammétrique et concerne des objets dont les points initiaux et finaux ne sont pas caractéristiques de l’altitude de l’objet (objets surfaciques, objets linéaires isolés). Pour des objets surfaciques comme les bâtiments ou les réservoirs, il s’agit de l’altitude minimum du pourtour tel qu’il est défini en planimétrie (généralement l’altitude aux gouttières) et non de l’altitude minimum absolue. Dans le cas d’un bâtiment obtenu après intégration du bâti issu du cadastre, Z_MIN correspond à une altitude toit médiane calculée, en prenant en compte les altitudes des contours des bâtiments directement contigus s’ils existent. Dans ce cas Z_MAX et Z_MIN prennent la même valeur. L’attribut peut prendre une valeur conventionnelle (9999) lorsque la géométrie de l’objet n’est pas issue d’une saisie photogrammétrique (ex. objets numérisés sur la carte en service).</rdfs:comment>
        <rdfs:comment xml:lang="en">Minimum altitude of a linear or polygon object. This information comes from the photogrammetric input and concerns objects whose initial and final points are not characteristic of the altitude of the object (surface objects, isolated linear objects). For areal objects such as buildings or reservoirs, this is the minimum altitude of the perimeter as defined in planimetry (usually the elevation at the gutters) and not the absolute minimum altitude. In the case of a building obtained after integration of the frame from the cadastre, Z_MIN corresponds to a computed median roof altitude, taking into account the altitudes of the outlines of buildings directly contiguous if they exist. In this case Z_MAX and Z_MIN take the same value. The attribute can take a conventional value (9999) when the geometry of the object is not the result of a photogrammetric capture (eg objects scanned on the map in use).</rdfs:comment>
        <rdfs:isDefinedBy rdf:resource="http://data.ign.fr/def/topo"/>
        <rdfs:label xml:lang="en">min z</rdfs:label>
        <rdfs:label xml:lang="fr">z min</rdfs:label>
    </owl:DatatypeProperty>
    


    <!-- http://data.ign.fr/def/topo#zMoyen -->


    <owl:DatatypeProperty rdf:about="http://data.ign.fr/def/topo#zMoyen">
        <rdfs:domain rdf:resource="http://data.ign.fr/def/topo#EntiteTopographique"/>
        <rdfs:range rdf:resource="http://www.w3.org/2001/XMLSchema#double"/>
        <rdfs:comment xml:lang="fr">Altitude moyenne des points composants la géométrie de l’objet telle qu’il a été saisi à l’origine lorsqu’il est issu d’une saisie photogrammétrique. L’attribut peut prendre une valeur conventionnelle (9999) lorsque la géométrie de l’objet n’est pas issue d’une saisie photogrammétrique (ex. objets numérisés sur la carte en service).</rdfs:comment>
        <rdfs:comment xml:lang="en">Average altitude of the points that make up the geometry of the object as it was originally entered when it came from a photogrammetric capture. The attribute can take a conventional value (9999) when the geometry of the object is not the result of a photogrammetric capture (eg objects scanned on the map in use).</rdfs:comment>
        <rdfs:isDefinedBy rdf:resource="http://data.ign.fr/def/topo"/>
        <rdfs:label xml:lang="en">average z</rdfs:label>
        <rdfs:label xml:lang="fr">z moyen</rdfs:label>
    </owl:DatatypeProperty>
    


    <!-- 
    ///////////////////////////////////////////////////////////////////////////////////////
    //
    // Classes
    //
    ///////////////////////////////////////////////////////////////////////////////////////
     -->


    


    <!-- http://data.ign.fr/def/geofla#Commune -->


    <owl:Class rdf:about="http://data.ign.fr/def/geofla#Commune">
        <rdfs:isDefinedBy rdf:resource="http://data.ign.fr/def/geofla#"/>
        <rdfs:label xml:lang="en">Commune</rdfs:label>
        <rdfs:label xml:lang="fr">Commune</rdfs:label>
    </owl:Class>
    


    <!-- http://data.ign.fr/def/geometrie#Curve -->


    <owl:Class rdf:about="http://data.ign.fr/def/geometrie#Curve"/>
    


    <!-- http://data.ign.fr/def/topo#AireDePeage -->


    <owl:Class rdf:about="http://data.ign.fr/def/topo#AireDePeage">
        <rdfs:subClassOf rdf:resource="http://data.ign.fr/def/topo#ElementReseauRoutier"/>
        <rdfs:comment xml:lang="fr">Emprise de la chaussée d&apos;une aire de péage.</rdfs:comment>
        <rdfs:comment xml:lang="en">Roadway of a toll area.</rdfs:comment>
        <rdfs:isDefinedBy rdf:resource="http://data.ign.fr/def/topo"/>
        <rdfs:label xml:lang="fr">Aire de péage</rdfs:label>
        <rdfs:label xml:lang="en">Toll-gate area</rdfs:label>
    </owl:Class>
    


    <!-- http://data.ign.fr/def/topo#AireDeTriage -->


    <owl:Class rdf:about="http://data.ign.fr/def/topo#AireDeTriage">
        <rdfs:subClassOf rdf:resource="http://data.ign.fr/def/topo#ElementReseauFerroviaire"/>
        <rdfs:comment xml:lang="en">Area encompassing all sections of tracks, sidings, switches for sorting cars and the composition of trains. Sorting area, beam of tracks.</rdfs:comment>
        <rdfs:comment xml:lang="fr">Surface qui englobe l’ensemble des tronçons de voies, voies de garage, aiguillages permettant le tri des wagons et la composition des trains. Aire de triage, faisceau de voies.</rdfs:comment>
        <rdfs:isDefinedBy rdf:resource="http://data.ign.fr/def/topo"/>
        <rdfs:label xml:lang="fr">Aire de triage</rdfs:label>
        <rdfs:label xml:lang="en">Marshalling yard</rdfs:label>
    </owl:Class>
    


    <!-- http://data.ign.fr/def/topo#Bassin -->


    <owl:Class rdf:about="http://data.ign.fr/def/topo#Bassin">
        <rdfs:subClassOf rdf:resource="http://data.ign.fr/def/topo#EntiteHydrographiqueTerrestre"/>
        <rdfs:comment xml:lang="fr">Construction non couverte destinée à recevoir de l&apos;eau temporairement ou de manière permanente.</rdfs:comment>
        <rdfs:comment xml:lang="en">Uncovered construction intended to receive water temporarily or permanently.</rdfs:comment>
        <rdfs:isDefinedBy rdf:resource="http://data.ign.fr/def/topo"/>
        <rdfs:label xml:lang="en">Basin</rdfs:label>
        <rdfs:label xml:lang="fr">Bassin</rdfs:label>
    </owl:Class>
    


    <!-- http://data.ign.fr/def/topo#Bati -->


    <owl:Class rdf:about="http://data.ign.fr/def/topo#Bati">
        <rdfs:subClassOf rdf:resource="http://data.ign.fr/def/topo#EntiteTopographique"/>
        <rdfs:comment xml:lang="en">Buildings (undifferentiated, industrial and remarkable) and other constructions.</rdfs:comment>
        <rdfs:comment xml:lang="fr">Bâtiments (indifférenciés, industriels et remarquables) et autres constructions.</rdfs:comment>
        <rdfs:isDefinedBy rdf:resource="http://data.ign.fr/def/topo"/>
        <rdfs:label xml:lang="en">Buildings and structures</rdfs:label>
        <rdfs:label xml:lang="fr">Bâti</rdfs:label>
    </owl:Class>
    


    <!-- http://data.ign.fr/def/topo#Batiment -->


    <owl:Class rdf:about="http://data.ign.fr/def/topo#Batiment">
        <rdfs:subClassOf rdf:resource="http://data.ign.fr/def/topo#Bati"/>
        <rdfs:comment xml:lang="fr">Construction d&apos;une certaine importance destinée à abriter des personnes, des choses ou des animaux.</rdfs:comment>
        <rdfs:comment xml:lang="en">Construction of a certain importance intended to shelter people, things or animals.</rdfs:comment>
        <rdfs:isDefinedBy rdf:resource="http://data.ign.fr/def/topo"/>
        <rdfs:label xml:lang="en">Building</rdfs:label>
        <rdfs:label xml:lang="fr">Bâtiment</rdfs:label>
    </owl:Class>
    


    <!-- http://data.ign.fr/def/topo#BornePostale -->


    <owl:Class rdf:about="http://data.ign.fr/def/topo#BornePostale">
        <rdfs:subClassOf rdf:resource="http://data.ign.fr/def/topo#ElementReseauRoutier"/>
        <rdfs:comment xml:lang="fr">Borne postale située à l&apos;extrémité d&apos;un tronçon de route.</rdfs:comment>
        <rdfs:comment xml:lang="en">Postal terminal located at the end of a stretch of road.</rdfs:comment>
        <rdfs:isDefinedBy rdf:resource="http://data.ign.fr/def/topo"/>
        <rdfs:label xml:lang="fr">Borne postale</rdfs:label>
        <rdfs:label xml:lang="en">Civic number marker</rdfs:label>
    </owl:Class>
    


    <!-- http://data.ign.fr/def/topo#CanalisationDEau -->


    <owl:Class rdf:about="http://data.ign.fr/def/topo#CanalisationDEau">
        <rdfs:subClassOf rdf:resource="http://data.ign.fr/def/topo#EntiteHydrographiqueTerrestre"/>
        <rdfs:comment xml:lang="en">Aerial water pipeline.</rdfs:comment>
        <rdfs:comment xml:lang="fr">Canalisation d&apos;eau aérienne.</rdfs:comment>
        <rdfs:isDefinedBy rdf:resource="http://data.ign.fr/def/topo"/>
        <rdfs:label xml:lang="fr">Canalisation d&apos;eau</rdfs:label>
        <rdfs:label xml:lang="en">Water pipe</rdfs:label>
    </owl:Class>
    


    <!-- http://data.ign.fr/def/topo#Cimetiere -->


    <owl:Class rdf:about="http://data.ign.fr/def/topo#Cimetiere">
        <rdfs:subClassOf rdf:resource="http://data.ign.fr/def/topo#Bati"/>
        <rdfs:comment xml:lang="fr">Lieu où l’on enterre les morts.</rdfs:comment>
        <rdfs:comment xml:lang="en">Place where we bury the dead.</rdfs:comment>
        <rdfs:isDefinedBy rdf:resource="http://data.ign.fr/def/topo"/>
        <rdfs:label xml:lang="en">Cemetery</rdfs:label>
        <rdfs:label xml:lang="fr">Cimetière</rdfs:label>
    </owl:Class>
    


    <!-- http://data.ign.fr/def/topo#Conduite -->


    <owl:Class rdf:about="http://data.ign.fr/def/topo#Conduite">
        <rdfs:subClassOf rdf:resource="http://data.ign.fr/def/topo#InfrastructureTransportEnergie"/>
        <rdfs:comment xml:lang="fr">Conduite (autre que canalisation d’eau) ou tapis roulant utilisés pour le transport de matière première (gaz, hydrocarbure, minerai, etc.) ou canalisation de nature inconnue.</rdfs:comment>
        <rdfs:comment xml:lang="en">Driving (other than water piping) or treadmill used for the transportation of raw material (gas, hydrocarbon, ore, etc.) or pipeline of unknown nature.</rdfs:comment>
        <rdfs:isDefinedBy rdf:resource="http://data.ign.fr/def/topo"/>
        <rdfs:label xml:lang="fr">Conduite</rdfs:label>
        <rdfs:label xml:lang="en">Pipeline</rdfs:label>
    </owl:Class>
    


    <!-- http://data.ign.fr/def/topo#Construction -->


    <owl:Class rdf:about="http://data.ign.fr/def/topo#Construction">
        <rdfs:subClassOf rdf:resource="http://data.ign.fr/def/topo#Bati"/>
        <rdfs:comment xml:lang="en">Civil engineering works.</rdfs:comment>
        <rdfs:comment xml:lang="fr">Ouvrage de génie civil.</rdfs:comment>
        <rdfs:isDefinedBy rdf:resource="http://data.ign.fr/def/topo"/>
        <rdfs:label xml:lang="fr">Construction</rdfs:label>
        <rdfs:label xml:lang="en">Structure</rdfs:label>
    </owl:Class>
    


    <!-- http://data.ign.fr/def/topo#CoursDEau -->


    <owl:Class rdf:about="http://data.ign.fr/def/topo#CoursDEau">
        <rdfs:subClassOf rdf:resource="http://data.ign.fr/def/topo#EntiteHydrographiqueTerrestre"/>
        <rdfs:comment xml:lang="fr">Portion de cours d&apos;eau, réel ou fictif, permanent ou temporaire, naturel ou artificiel, homogène pour l&apos;ensemble des attributs qui la concernent, et qui n&apos;inclut pas de confluent.</rdfs:comment>
        <rdfs:comment xml:lang="en">Portion of watercourses, real or fictitious, permanent or temporary, natural or artificial, homogeneous for all the attributes which concern it, and which does not include a confluence.</rdfs:comment>
        <rdfs:isDefinedBy rdf:resource="http://data.ign.fr/def/topo"/>
        <rdfs:label xml:lang="fr">Cours d&apos;eau</rdfs:label>
        <rdfs:label xml:lang="en">Watercourse</rdfs:label>
    </owl:Class>
    


    <!-- http://data.ign.fr/def/topo#ElementDuRelief -->


    <owl:Class rdf:about="http://data.ign.fr/def/topo#ElementDuRelief">
        <rdfs:subClassOf rdf:resource="http://data.ign.fr/def/topo#EntiteTopographique"/>
        <rdfs:comment xml:lang="fr">Entité topographique correspondant à une rupture de pente artificielle, ou à un élément remarquable du relief nommé.</rdfs:comment>
        <rdfs:comment xml:lang="en">Topographic entity corresponding to an artificial slope break, or to a remarkable element of the named relief.</rdfs:comment>
        <rdfs:isDefinedBy rdf:resource="http://data.ign.fr/def/topo"/>
        <rdfs:label xml:lang="en">Relief feature</rdfs:label>
        <rdfs:label xml:lang="fr">Élément du relief</rdfs:label>
    </owl:Class>
    


    <!-- http://data.ign.fr/def/topo#ElementReseauFerroviaire -->


    <owl:Class rdf:about="http://data.ign.fr/def/topo#ElementReseauFerroviaire">
        <rdfs:subClassOf rdf:resource="http://data.ign.fr/def/topo#EntiteTopographique"/>
        <rdfs:comment xml:lang="en">Elements of the rail transportation system: railways and marshalling yards.</rdfs:comment>
        <rdfs:comment xml:lang="fr">Éléments du réseau de transport ferroviaire: voies ferrées et aires de triage.</rdfs:comment>
        <rdfs:isDefinedBy rdf:resource="http://data.ign.fr/def/topo"/>
        <rdfs:label xml:lang="en">Transport by rail feature</rdfs:label>
        <rdfs:label xml:lang="fr">Élément du réseau ferroviaire</rdfs:label>
    </owl:Class>
    


    <!-- http://data.ign.fr/def/topo#ElementReseauRoutier -->


    <owl:Class rdf:about="http://data.ign.fr/def/topo#ElementReseauRoutier">
        <rdfs:subClassOf rdf:resource="http://data.ign.fr/def/topo#EntiteTopographique"/>
        <rdfs:comment xml:lang="en">Elements of the road transport network: paved and unpaved roads, &apos;addressed&apos; network, and a selection of roads and trails.</rdfs:comment>
        <rdfs:comment xml:lang="fr">Éléments du réseau de transport routier: voies de communication revêtues et non revêtues, réseau &apos;adressé&apos;, et une sélection des chemins et sentiers.</rdfs:comment>
        <rdfs:isDefinedBy rdf:resource="http://data.ign.fr/def/topo"/>
        <rdfs:label xml:lang="en">Road transport feature</rdfs:label>
        <rdfs:label xml:lang="fr">Élément du réseau routier</rdfs:label>
    </owl:Class>
    


    <!-- http://data.ign.fr/def/topo#EntiteHydrographiqueTerrestre -->


    <owl:Class rdf:about="http://data.ign.fr/def/topo#EntiteHydrographiqueTerrestre">
        <rdfs:subClassOf rdf:resource="http://data.ign.fr/def/topo#EntiteTopographique"/>
        <rdfs:comment xml:lang="fr">Entité topographique relative au réseau hydrographique terrestre, à la production ou au stockage d&apos;eau.</rdfs:comment>
        <rdfs:comment xml:lang="en">Topographic entity relating to the terrestrial hydrographic network, the production or the storage of water.</rdfs:comment>
        <rdfs:isDefinedBy rdf:resource="http://data.ign.fr/def/topo"/>
        <rdfs:label xml:lang="fr">Entité hydrographique terrestre</rdfs:label>
        <rdfs:label xml:lang="en">Inland hydrographic feature</rdfs:label>
    </owl:Class>
    


    <!-- http://data.ign.fr/def/topo#EntiteTopographique -->


    <owl:Class rdf:about="http://data.ign.fr/def/topo#EntiteTopographique">
        <owl:equivalentClass rdf:resource="http://www.geonames.org/ontology#Feature"/>
        <rdfs:comment xml:lang="en">A real world phenomenon that is associated with a location on earth</rdfs:comment>
        <rdfs:comment xml:lang="fr">Un phénomène du monde réel qui est associé à une localisation sur la terre</rdfs:comment>
        <rdfs:isDefinedBy rdf:resource="http://data.ign.fr/def/topo"/>
        <rdfs:label xml:lang="fr">Entité topographique</rdfs:label>
        <rdfs:label xml:lang="en">Topographic entity</rdfs:label>
    </owl:Class>
    


    <!-- http://data.ign.fr/def/topo#InfrastructureTransportEnergie -->


    <owl:Class rdf:about="http://data.ign.fr/def/topo#InfrastructureTransportEnergie">
        <rdfs:subClassOf rdf:resource="http://data.ign.fr/def/topo#EntiteTopographique"/>
        <rdfs:comment xml:lang="en">Elements of the electricity transmission network at high and very high voltage, and pipes used for the transport of raw material.</rdfs:comment>
        <rdfs:comment xml:lang="fr">Éléments du réseau de transport d&apos;électricité à une haute et très haute tension, et conduites utilisées pour le transport de matière première.</rdfs:comment>
        <rdfs:isDefinedBy rdf:resource="http://data.ign.fr/def/topo"/>
        <rdfs:label xml:lang="en">Energy transport infrastructure</rdfs:label>
        <rdfs:label xml:lang="fr">Infrastructure de transport d&apos;énergie</rdfs:label>
    </owl:Class>
    


    <!-- http://data.ign.fr/def/topo#Laisse -->


    <owl:Class rdf:about="http://data.ign.fr/def/topo#Laisse">
        <rdfs:subClassOf rdf:resource="http://data.ign.fr/def/topo#EntiteHydrographiqueTerrestre"/>
        <rdfs:comment xml:lang="fr">Limite supérieure ou inférieure de l&apos;estran.</rdfs:comment>
        <rdfs:comment xml:lang="en">Upper or lower limit of the foreshore.</rdfs:comment>
        <rdfs:isDefinedBy rdf:resource="http://data.ign.fr/def/topo"/>
        <rdfs:label xml:lang="fr">Laisse</rdfs:label>
        <rdfs:label xml:lang="en">Tide line</rdfs:label>
    </owl:Class>
    


    <!-- http://data.ign.fr/def/topo#LigneElectrique -->


    <owl:Class rdf:about="http://data.ign.fr/def/topo#LigneElectrique">
        <rdfs:subClassOf rdf:resource="http://data.ign.fr/def/topo#InfrastructureTransportEnergie"/>
        <rdfs:comment xml:lang="fr">Portion de ligne électrique homogène pour l&apos;ensemble des attributs qui la concernent.</rdfs:comment>
        <rdfs:comment xml:lang="en">Portion of homogeneous electrical line for all the attributes that concern it.</rdfs:comment>
        <rdfs:isDefinedBy rdf:resource="http://data.ign.fr/def/topo"/>
        <rdfs:label xml:lang="en">Electricity transmission line</rdfs:label>
        <rdfs:label xml:lang="fr">Ligne électrique</rdfs:label>
    </owl:Class>
    


    <!-- http://data.ign.fr/def/topo#LigneTransportCable -->


    <owl:Class rdf:about="http://data.ign.fr/def/topo#LigneTransportCable">
        <rdfs:subClassOf rdf:resource="http://data.ign.fr/def/topo#EntiteTopographique"/>
        <rdfs:comment xml:lang="en">Means of transport consisting of one or more carrying cables.</rdfs:comment>
        <rdfs:comment xml:lang="fr">Moyen de transport constitué d&apos;un ou de plusieurs câbles porteurs.</rdfs:comment>
        <rdfs:isDefinedBy rdf:resource="http://data.ign.fr/def/topo"/>
        <rdfs:label xml:lang="en">Cableway transport line</rdfs:label>
        <rdfs:label xml:lang="fr">Ligne de transport par câble</rdfs:label>
    </owl:Class>
    


    <!-- http://data.ign.fr/def/topo#Parking -->


    <owl:Class rdf:about="http://data.ign.fr/def/topo#Parking">
        <rdfs:subClassOf rdf:resource="http://data.ign.fr/def/topo#ElementReseauRoutier"/>
        <rdfs:comment xml:lang="en">Area developed for the parking of automobiles. Parking uncovered, public or private, parking area of about half a hectare and more.</rdfs:comment>
        <rdfs:comment xml:lang="fr">Zone aménagée pour le parcage des automobiles. Parking non couvert, public ou privé, aire de stationnement d’environ un demi hectare et plus.</rdfs:comment>
        <rdfs:isDefinedBy rdf:resource="http://data.ign.fr/def/topo"/>
        <rdfs:label xml:lang="en">Car park</rdfs:label>
        <rdfs:label xml:lang="fr">Parking</rdfs:label>
    </owl:Class>
    


    <!-- http://data.ign.fr/def/topo#PisteAerodrome -->


    <owl:Class rdf:about="http://data.ign.fr/def/topo#PisteAerodrome">
        <rdfs:subClassOf rdf:resource="http://data.ign.fr/def/topo#Bati"/>
        <rdfs:comment xml:lang="fr">Aire située sur un aérodrome, aménagée afin de servir au roulement des aéronefs, au décollage et à l’atterrissage, en dur ou en herbe.</rdfs:comment>
        <rdfs:comment xml:lang="en">Area located on an aerodrome, designed for use in aircraft rolling, take-off and landing, hard or grass.</rdfs:comment>
        <rdfs:isDefinedBy rdf:resource="http://data.ign.fr/def/topo"/>
        <rdfs:label xml:lang="fr">Piste d&apos;aérodrome</rdfs:label>
        <rdfs:label xml:lang="en">Taxiway</rdfs:label>
    </owl:Class>
    


    <!-- http://data.ign.fr/def/topo#Place -->


    <owl:Class rdf:about="http://data.ign.fr/def/topo#Place">
        <rdfs:subClassOf rdf:resource="http://data.ign.fr/def/topo#ElementReseauRoutier"/>
        <rdfs:comment xml:lang="en">Place or crossroads covered with wide width.</rdfs:comment>
        <rdfs:comment xml:lang="fr">Place ou carrefour revêtu de grande largeur.</rdfs:comment>
        <rdfs:isDefinedBy rdf:resource="http://data.ign.fr/def/topo"/>
        <rdfs:label xml:lang="fr">Place</rdfs:label>
        <rdfs:label xml:lang="en">Square</rdfs:label>
    </owl:Class>
    


    <!-- http://data.ign.fr/def/topo#PointDEau -->


    <owl:Class rdf:about="http://data.ign.fr/def/topo#PointDEau">
        <rdfs:subClassOf rdf:resource="http://data.ign.fr/def/topo#EntiteHydrographiqueTerrestre"/>
        <rdfs:comment xml:lang="en">Source (captured or not), point of water production (pumping, drilling, well, ...) or small water storage point (cistern, waterer, laundry, basin).</rdfs:comment>
        <rdfs:comment xml:lang="fr">Source (captée ou non), point de production d’eau (pompage, forage, puits,...) ou point de stockage d’eau de petite dimension (citerne, abreuvoir, lavoir, bassin).</rdfs:comment>
        <rdfs:isDefinedBy rdf:resource="http://data.ign.fr/def/topo"/>
        <rdfs:label xml:lang="fr">Point d&apos;eau</rdfs:label>
        <rdfs:label xml:lang="en">Waterhole</rdfs:label>
    </owl:Class>
    


    <!-- http://data.ign.fr/def/topo#PosteTransformation -->


    <owl:Class rdf:about="http://data.ign.fr/def/topo#PosteTransformation">
        <rdfs:subClassOf rdf:resource="http://data.ign.fr/def/topo#InfrastructureTransportEnergie"/>
        <rdfs:comment xml:lang="fr">Enceinte à l&apos;intérieur de laquelle le courant transporté par une ligne électrique est transformé.</rdfs:comment>
        <rdfs:comment xml:lang="en">Enclosure inside which the current carried by a power line is transformed.</rdfs:comment>
        <rdfs:isDefinedBy rdf:resource="http://data.ign.fr/def/topo"/>
        <rdfs:label xml:lang="fr">Poste de transformation</rdfs:label>
        <rdfs:label xml:lang="en">Transformation sub-station</rdfs:label>
    </owl:Class>
    


    <!-- http://data.ign.fr/def/topo#Pylone -->


    <owl:Class rdf:about="http://data.ign.fr/def/topo#Pylone">
        <rdfs:subClassOf rdf:resource="http://data.ign.fr/def/topo#InfrastructureTransportEnergie"/>
        <rdfs:comment xml:lang="en">Electric line support. Pylon, portico.</rdfs:comment>
        <rdfs:comment xml:lang="fr">Support de ligne électrique. Pylône, portique.</rdfs:comment>
        <rdfs:isDefinedBy rdf:resource="http://data.ign.fr/def/topo"/>
        <rdfs:label xml:lang="en">Pylon</rdfs:label>
        <rdfs:label xml:lang="fr">Pylône</rdfs:label>
    </owl:Class>
    


    <!-- http://data.ign.fr/def/topo#Reservoir -->


    <owl:Class rdf:about="http://data.ign.fr/def/topo#Reservoir">
        <rdfs:subClassOf rdf:resource="http://data.ign.fr/def/topo#Bati"/>
        <rdfs:comment xml:lang="fr">Réservoir (eau, matières industrielles,...) de plus de 10m de diamètre.</rdfs:comment>
        <rdfs:comment xml:lang="en">Tank (water, industrial materials, ...) more than 10m in diameter.</rdfs:comment>
        <rdfs:isDefinedBy rdf:resource="http://data.ign.fr/def/topo"/>
        <rdfs:label xml:lang="fr">Réservoir</rdfs:label>
        <rdfs:label xml:lang="en">Tank</rdfs:label>
    </owl:Class>
    


    <!-- http://data.ign.fr/def/topo#Route -->


    <owl:Class rdf:about="http://data.ign.fr/def/topo#Route">
        <rdfs:subClassOf rdf:resource="http://data.ign.fr/def/topo#ElementReseauRoutier"/>
        <rdfs:subClassOf>
            <owl:Restriction>
                <owl:onProperty rdf:resource="http://purl.org/dc/terms/isPartOf"/>
                <owl:someValuesFrom rdf:resource="http://data.ign.fr/def/topo#Voie"/>
            </owl:Restriction>
        </rdfs:subClassOf>
        <rdfs:comment xml:lang="fr">Portion de voie de communication destinée aux automobiles, aux piétons, aux cycles ou aux animaux, homogène pour l&apos;ensemble des attributs et des relations qui la concerne. Le tronçon de route peut être revêtu ou non revêtu (pas de revêtement de surface ou revêtement de surface fortement dégradé).</rdfs:comment>
        <rdfs:comment xml:lang="en">Portion of communication channel intended for automobiles, pedestrians, cycles or animals, homogeneous for all the attributes and relations that concern it. The road section may be coated or uncoated (no surface coating or highly degraded surface coating).</rdfs:comment>
        <rdfs:isDefinedBy rdf:resource="http://data.ign.fr/def/topo"/>
        <rdfs:label xml:lang="en">Road</rdfs:label>
        <rdfs:label xml:lang="fr">Route</rdfs:label>
    </owl:Class>
    


    <!-- http://data.ign.fr/def/topo#SurfaceDEau -->


    <owl:Class rdf:about="http://data.ign.fr/def/topo#SurfaceDEau">
        <rdfs:subClassOf rdf:resource="http://data.ign.fr/def/topo#EntiteHydrographiqueTerrestre"/>
        <rdfs:comment xml:lang="en">Non-marine water surface: wide channel, pond, wide river, lake, pond, wide river.</rdfs:comment>
        <rdfs:comment xml:lang="fr">Surface d&apos;eau non marine : large canal, étang, large fleuve, lac, mare, large rivière.</rdfs:comment>
        <rdfs:isDefinedBy rdf:resource="http://data.ign.fr/def/topo"/>
        <rdfs:label xml:lang="fr">Surface d&apos;eau</rdfs:label>
        <rdfs:label xml:lang="en">Water surface</rdfs:label>
    </owl:Class>
    


    <!-- http://data.ign.fr/def/topo#TerrainDeSport -->


    <owl:Class rdf:about="http://data.ign.fr/def/topo#TerrainDeSport">
        <rdfs:subClassOf rdf:resource="http://data.ign.fr/def/topo#Bati"/>
        <rdfs:comment xml:lang="en">Outdoor sports equipment.</rdfs:comment>
        <rdfs:comment xml:lang="fr">Équipement sportif de plein air.</rdfs:comment>
        <rdfs:isDefinedBy rdf:resource="http://data.ign.fr/def/topo"/>
        <rdfs:label xml:lang="en">Sports ground</rdfs:label>
        <rdfs:label xml:lang="fr">Terrain de sport</rdfs:label>
    </owl:Class>
    


    <!-- http://data.ign.fr/def/topo#TypeDeBatiment -->


    <owl:Class rdf:about="http://data.ign.fr/def/topo#TypeDeBatiment">
        <rdfs:subClassOf rdf:resource="http://www.w3.org/2004/02/skos/core#Concept"/>
        <rdfs:comment xml:lang="en">Includes all instances designating building types.</rdfs:comment>
        <rdfs:comment xml:lang="fr">Regroupe l&apos;ensemble des instances désignant des types de bâtiments.</rdfs:comment>
        <rdfs:isDefinedBy rdf:resource="http://data.ign.fr/def/topo"/>
        <rdfs:label xml:lang="fr">Type de bâtiment</rdfs:label>
        <rdfs:label xml:lang="en">Type of building </rdfs:label>
    </owl:Class>
    


    <!-- http://data.ign.fr/def/topo#TypeDeConstruction -->


    <owl:Class rdf:about="http://data.ign.fr/def/topo#TypeDeConstruction">
        <rdfs:subClassOf rdf:resource="http://www.w3.org/2004/02/skos/core#Concept"/>
        <rdfs:comment xml:lang="en">Group together all the instances designating types of constructions.</rdfs:comment>
        <rdfs:comment xml:lang="fr">Regroupe l&apos;ensemble des instances désignant des types de constructions.</rdfs:comment>
        <rdfs:isDefinedBy rdf:resource="http://data.ign.fr/def/topo"/>
        <rdfs:label xml:lang="fr">Type de construction</rdfs:label>
        <rdfs:label xml:lang="en">Type of structure</rdfs:label>
    </owl:Class>
    


    <!-- http://data.ign.fr/def/topo#TypeDeFranchissement -->


    <owl:Class rdf:about="http://data.ign.fr/def/topo#TypeDeFranchissement">
        <rdfs:subClassOf rdf:resource="http://www.w3.org/2004/02/skos/core#Concept"/>
        <rdfs:comment xml:lang="en">Includes all instances designating types of crossing structures.</rdfs:comment>
        <rdfs:comment xml:lang="fr">Regroupe l&apos;ensemble des instances désignant des types d&apos;ouvrages de franchissement.</rdfs:comment>
        <rdfs:isDefinedBy rdf:resource="http://data.ign.fr/def/topo"/>
        <rdfs:label xml:lang="fr">Type de franchissement</rdfs:label>
        <rdfs:label xml:lang="en">Type of crossing</rdfs:label>
    </owl:Class>
    


    <!-- http://data.ign.fr/def/topo#TypeDeLaisse -->


    <owl:Class rdf:about="http://data.ign.fr/def/topo#TypeDeLaisse">
        <rdfs:subClassOf rdf:resource="http://www.w3.org/2004/02/skos/core#Concept"/>
        <rdfs:comment xml:lang="en">Group together all instances designating leash types.</rdfs:comment>
        <rdfs:comment xml:lang="fr">Regroupe l&apos;ensemble des instances désignant des types de laisses.</rdfs:comment>
        <rdfs:isDefinedBy rdf:resource="http://data.ign.fr/def/topo"/>
        <rdfs:label xml:lang="fr">Type de laisse</rdfs:label>
        <rdfs:label xml:lang="en">Type of tide line</rdfs:label>
    </owl:Class>
    


    <!-- http://data.ign.fr/def/topo#TypeDePointDEau -->


    <owl:Class rdf:about="http://data.ign.fr/def/topo#TypeDePointDEau">
        <rdfs:subClassOf rdf:resource="http://www.w3.org/2004/02/skos/core#Concept"/>
        <rdfs:comment xml:lang="en">Gathers all the instances designating types of water points.</rdfs:comment>
        <rdfs:comment xml:lang="fr">Regroupe l&apos;ensemble des instances désignant des types de points d&apos;eau.</rdfs:comment>
        <rdfs:isDefinedBy rdf:resource="http://data.ign.fr/def/topo"/>
        <rdfs:label xml:lang="fr">Type de point d&apos;eau</rdfs:label>
        <rdfs:label xml:lang="en">Type of waterhole</rdfs:label>
    </owl:Class>
    


    <!-- http://data.ign.fr/def/topo#TypeDeRelief -->


    <owl:Class rdf:about="http://data.ign.fr/def/topo#TypeDeRelief">
        <rdfs:subClassOf rdf:resource="http://www.w3.org/2004/02/skos/core#Concept"/>
        <rdfs:comment xml:lang="en">Gathers all the instances designating types of reliefs.</rdfs:comment>
        <rdfs:comment xml:lang="fr">Regroupe l&apos;ensemble des instances désignant des types de reliefs.</rdfs:comment>
        <rdfs:isDefinedBy rdf:resource="http://data.ign.fr/def/topo"/>
        <rdfs:label xml:lang="fr">Type d&apos;élément du relief</rdfs:label>
        <rdfs:label xml:lang="en">Type of relief feature</rdfs:label>
    </owl:Class>
    


    <!-- http://data.ign.fr/def/topo#TypeDeReservoir -->


    <owl:Class rdf:about="http://data.ign.fr/def/topo#TypeDeReservoir">
        <rdfs:subClassOf rdf:resource="http://www.w3.org/2004/02/skos/core#Concept"/>
        <rdfs:comment xml:lang="en">Group together all instances designating types of tanks.</rdfs:comment>
        <rdfs:comment xml:lang="fr">Regroupe l&apos;ensemble des instances désignant des types de réservoirs.</rdfs:comment>
        <rdfs:isDefinedBy rdf:resource="http://data.ign.fr/def/topo"/>
        <rdfs:label xml:lang="fr">Type de réservoir</rdfs:label>
        <rdfs:label xml:lang="en">Type of tank</rdfs:label>
    </owl:Class>
    


    <!-- http://data.ign.fr/def/topo#TypeDeRoute -->


    <owl:Class rdf:about="http://data.ign.fr/def/topo#TypeDeRoute">
        <rdfs:subClassOf rdf:resource="http://www.w3.org/2004/02/skos/core#Concept"/>
        <rdfs:comment xml:lang="en">Group together all instances designating types of routes.</rdfs:comment>
        <rdfs:comment xml:lang="fr">Regroupe l&apos;ensemble des instances désignant des types de routes.</rdfs:comment>
        <rdfs:isDefinedBy rdf:resource="http://data.ign.fr/def/topo"/>
        <rdfs:label xml:lang="fr">Type de route</rdfs:label>
        <rdfs:label xml:lang="en">Type of road</rdfs:label>
    </owl:Class>
    


    <!-- http://data.ign.fr/def/topo#TypeDeTerrainDeSport -->


    <owl:Class rdf:about="http://data.ign.fr/def/topo#TypeDeTerrainDeSport">
        <rdfs:subClassOf rdf:resource="http://www.w3.org/2004/02/skos/core#Concept"/>
        <rdfs:comment xml:lang="en">Includes all instances designating types of sports fields.</rdfs:comment>
        <rdfs:comment xml:lang="fr">Regroupe l&apos;ensemble des instances désignant des types de terrains de sports.</rdfs:comment>
        <rdfs:isDefinedBy rdf:resource="http://data.ign.fr/def/topo"/>
        <rdfs:label xml:lang="fr">Type de terrain de sport</rdfs:label>
        <rdfs:label xml:lang="en">Type of sports ground </rdfs:label>
    </owl:Class>
    


    <!-- http://data.ign.fr/def/topo#TypeDeTransportCable -->


    <owl:Class rdf:about="http://data.ign.fr/def/topo#TypeDeTransportCable">
        <rdfs:subClassOf rdf:resource="http://www.w3.org/2004/02/skos/core#Concept"/>
        <rdfs:comment xml:lang="en">Consists of all instances designating types of cable transport infrastructure.</rdfs:comment>
        <rdfs:comment xml:lang="fr">Regroupe l&apos;ensemble des instances désignant des types d&apos;infrastructures de transport par câble.</rdfs:comment>
        <rdfs:isDefinedBy rdf:resource="http://data.ign.fr/def/topo"/>
        <rdfs:label xml:lang="fr">Type de ligne de transport par câble</rdfs:label>
        <rdfs:label xml:lang="en">Type of cableway transport line</rdfs:label>
    </owl:Class>
    


    <!-- http://data.ign.fr/def/topo#TypeDeVegetation -->


    <owl:Class rdf:about="http://data.ign.fr/def/topo#TypeDeVegetation">
        <rdfs:subClassOf rdf:resource="http://www.w3.org/2004/02/skos/core#Concept"/>
        <rdfs:comment xml:lang="en">Includes all instances designating tree vegetation types.</rdfs:comment>
        <rdfs:comment xml:lang="fr">Regroupe l&apos;ensemble des instances désignant des types de végétation arborée.</rdfs:comment>
        <rdfs:isDefinedBy rdf:resource="http://data.ign.fr/def/topo"/>
        <rdfs:label xml:lang="fr">Type de végétation</rdfs:label>
        <rdfs:label xml:lang="en">Type of vegetation </rdfs:label>
    </owl:Class>
    


    <!-- http://data.ign.fr/def/topo#TypeDeVoieFerree -->


    <owl:Class rdf:about="http://data.ign.fr/def/topo#TypeDeVoieFerree">
        <rdfs:subClassOf rdf:resource="http://www.w3.org/2004/02/skos/core#Concept"/>
        <rdfs:comment xml:lang="en">Includes all instances designating railway types.</rdfs:comment>
        <rdfs:comment xml:lang="fr">Regroupe l&apos;ensemble des instances désignant des types de voies ferrées.</rdfs:comment>
        <rdfs:isDefinedBy rdf:resource="http://data.ign.fr/def/topo"/>
        <rdfs:label xml:lang="fr">Type de voie ferrée</rdfs:label>
        <rdfs:label xml:lang="en">Type of railway track</rdfs:label>
    </owl:Class>
    


    <!-- http://data.ign.fr/def/topo#TypeDeZAI -->


    <owl:Class rdf:about="http://data.ign.fr/def/topo#TypeDeZAI">
        <rdfs:subClassOf rdf:resource="http://www.w3.org/2004/02/skos/core#Concept"/>
        <rdfs:comment xml:lang="en">Includes all instances designating types of activity and interest areas.</rdfs:comment>
        <rdfs:comment xml:lang="fr">Regroupe l&apos;ensemble des instances désignant des types de zones d&apos;activités et d&apos;intérêt.</rdfs:comment>
        <rdfs:isDefinedBy rdf:resource="http://data.ign.fr/def/topo"/>
        <rdfs:label xml:lang="fr">Type de ZAI</rdfs:label>
        <rdfs:label xml:lang="en">Type of Area Of Interest (AOI)</rdfs:label>
    </owl:Class>
    


    <!-- http://data.ign.fr/def/topo#Voie -->


    <owl:Class rdf:about="http://data.ign.fr/def/topo#Voie">
        <rdfs:subClassOf rdf:resource="http://data.ign.fr/def/topo#ElementReseauRoutier"/>
        <rdfs:comment xml:lang="en">A lane is a set of road sections associated with the same name. A path is identified by name in a given commune. The channel name is the one used for addressing.</rdfs:comment>
        <rdfs:comment xml:lang="fr">Une voie est un ensemble de tronçons de route associés à un même nom. Une voie est identifiée par son nom dans une commune donnée. Le nom de voie est celui qui sert à l’adressage.</rdfs:comment>
        <rdfs:isDefinedBy rdf:resource="http://data.ign.fr/def/topo"/>
        <rdfs:label xml:lang="en">Named street</rdfs:label>
        <rdfs:label xml:lang="fr">Voie nommée</rdfs:label>
    </owl:Class>
    


    <!-- http://data.ign.fr/def/topo#VoieFerree -->


    <owl:Class rdf:about="http://data.ign.fr/def/topo#VoieFerree">
        <rdfs:subClassOf rdf:resource="http://data.ign.fr/def/topo#ElementReseauFerroviaire"/>
        <rdfs:comment xml:lang="fr">Portion de voie ferrée homogène pour l&apos;ensemble des attributs qui la concernent. Dans le cas d’une ligne composée de deux à quatre voies parallèles, l’ensemble des voies est modélisé par un seul objet.</rdfs:comment>
        <rdfs:comment xml:lang="en">Portion of homogeneous railway for all the attributes that concern it. In the case of a line composed of two to four parallel tracks, the set of channels is modeled by a single object.</rdfs:comment>
        <rdfs:isDefinedBy rdf:resource="http://data.ign.fr/def/topo"/>
        <rdfs:label xml:lang="en">Railway track</rdfs:label>
        <rdfs:label xml:lang="fr">Voie ferrée</rdfs:label>
    </owl:Class>
    


    <!-- http://data.ign.fr/def/topo#ZoneActiviteInteret -->


    <owl:Class rdf:about="http://data.ign.fr/def/topo#ZoneActiviteInteret">
        <rdfs:subClassOf rdf:resource="http://data.ign.fr/def/topo#EntiteTopographique"/>
        <rdfs:comment xml:lang="en">Building or site with a specific vocation or character (administrative, religious, sports, industrial, etc.).</rdfs:comment>
        <rdfs:comment xml:lang="fr">Bâtiment ou site ayant une vocation ou un caractère particuliers (administratif, religieux, sportif, industriel, etc.).</rdfs:comment>
        <rdfs:isDefinedBy rdf:resource="http://data.ign.fr/def/topo"/>
        <rdfs:label xml:lang="en">Working area or area of interest</rdfs:label>
        <rdfs:label xml:lang="fr">Zone d&apos;activité ou d&apos;intérêt</rdfs:label>
    </owl:Class>
    


    <!-- http://data.ign.fr/def/topo#ZoneDeVegetation -->


    <owl:Class rdf:about="http://data.ign.fr/def/topo#ZoneDeVegetation">
        <rdfs:subClassOf rdf:resource="http://data.ign.fr/def/topo#EntiteTopographique"/>
        <rdfs:comment xml:lang="fr">Espace végétal naturel ou non différencié selon le couvert forestier.</rdfs:comment>
        <rdfs:comment xml:lang="en">Natural space of vegetation or undifferentiated according to the forest cover.</rdfs:comment>
        <rdfs:isDefinedBy rdf:resource="http://data.ign.fr/def/topo"/>
        <rdfs:label xml:lang="en">Vegetation area</rdfs:label>
        <rdfs:label xml:lang="fr">Zone de végétation</rdfs:label>
    </owl:Class>
    


    <!-- http://purl.org/vocommons/voaf#Vocabulary -->


    <owl:Class rdf:about="http://purl.org/vocommons/voaf#Vocabulary"/>
    


    <!-- http://www.geonames.org/ontology#Feature -->


    <owl:Class rdf:about="http://www.geonames.org/ontology#Feature"/>
    


    <!-- http://www.w3.org/2004/02/skos/core#Concept -->


    <owl:Class rdf:about="http://www.w3.org/2004/02/skos/core#Concept"/>
    


    <!-- http://www.w3.org/2004/02/skos/core#ConceptScheme -->


    <owl:Class rdf:about="http://www.w3.org/2004/02/skos/core#ConceptScheme"/>
    


    <!-- http://www.w3.org/2006/time#Instant -->


    <owl:Class rdf:about="http://www.w3.org/2006/time#Instant"/>
    


    <!-- http://www.w3.org/2006/time#Interval -->


    <owl:Class rdf:about="http://www.w3.org/2006/time#Interval"/>
    


    <!-- http://www.w3.org/ns/org#Membership -->


    <owl:Class rdf:about="http://www.w3.org/ns/org#Membership"/>
    


    <!-- http://www.w3.org/ns/org#Role -->


    <owl:Class rdf:about="http://www.w3.org/ns/org#Role"/>
    


    <!-- http://www.w3.org/ns/prov#Entity -->


    <owl:Class rdf:about="http://www.w3.org/ns/prov#Entity"/>
    


    <!-- http://xmlns.com/foaf/0.1/Person -->


    <owl:Class rdf:about="http://xmlns.com/foaf/0.1/Person"/>
    


    <!-- 
    ///////////////////////////////////////////////////////////////////////////////////////
    //
    // Individuals
    //
    ///////////////////////////////////////////////////////////////////////////////////////
     -->


    


    <!-- http://data.ign.fr/def/topo# -->


    <owl:NamedIndividual rdf:about="http://data.ign.fr/def/topo#">
        <rdf:type rdf:resource="http://purl.org/vocommons/voaf#Vocabulary"/>
    </owl:NamedIndividual>
    


    <!-- http://data.ign.fr/id/codes/topo/typedebatiment/Aerogare -->


    <owl:NamedIndividual rdf:about="http://data.ign.fr/id/codes/topo/typedebatiment/Aerogare">
        <rdf:type rdf:resource="http://data.ign.fr/def/topo#TypeDeBatiment"/>
        <rdf:type rdf:resource="http://www.w3.org/2004/02/skos/core#Concept"/>
        <skos:definition xml:lang="fr">Ensemble des bâtiments d&apos;un aéroport réservés aux voyageurs et aux marchandises.</skos:definition>
        <skos:definition xml:lang="en">Set of airport buildings reserved for travelers and goods.</skos:definition>
        <skos:inScheme rdf:resource="http://data.ign.fr/id/codes/topo/typedebatiment/liste"/>
        <skos:prefLabel xml:lang="en">air terminal</skos:prefLabel>
        <skos:prefLabel xml:lang="fr">aérogare</skos:prefLabel>
    </owl:NamedIndividual>
    


    <!-- http://data.ign.fr/id/codes/topo/typedebatiment/ArcDeTriomphe -->


    <owl:NamedIndividual rdf:about="http://data.ign.fr/id/codes/topo/typedebatiment/ArcDeTriomphe">
        <rdf:type rdf:resource="http://data.ign.fr/def/topo#TypeDeBatiment"/>
        <rdf:type rdf:resource="http://www.w3.org/2004/02/skos/core#Concept"/>
        <skos:definition xml:lang="en">Monumental portico: triumphal arch, city gate.</skos:definition>
        <skos:definition xml:lang="fr">Portique monumental : arc de triomphe, porte de ville.</skos:definition>
        <skos:inScheme rdf:resource="http://data.ign.fr/id/codes/topo/typedebatiment/liste"/>
        <skos:prefLabel xml:lang="fr">arc de triomphe</skos:prefLabel>
        <skos:prefLabel xml:lang="en">triumphal arch</skos:prefLabel>
    </owl:NamedIndividual>
    


    <!-- http://data.ign.fr/id/codes/topo/typedebatiment/Arene -->


    <owl:NamedIndividual rdf:about="http://data.ign.fr/id/codes/topo/typedebatiment/Arene">
        <rdf:type rdf:resource="http://data.ign.fr/def/topo#TypeDeBatiment"/>
        <rdf:type rdf:resource="http://www.w3.org/2004/02/skos/core#Concept"/>
        <skos:altLabel xml:lang="en">roman theater</skos:altLabel>
        <skos:altLabel xml:lang="fr">théâtre antique</skos:altLabel>
        <skos:definition xml:lang="en">Large tiered building, partly or totally round or elliptical in shape: amphitheater, arena, antique theater, outdoor theater.</skos:definition>
        <skos:definition xml:lang="fr">Vaste édifice à gradins, de forme en partie ou totalement ronde ou elliptique : amphithéâtre, arène, théâtre antique, théâtre de plein air.</skos:definition>
        <skos:inScheme rdf:resource="http://data.ign.fr/id/codes/topo/typedebatiment/liste"/>
        <skos:prefLabel xml:lang="en">arena</skos:prefLabel>
        <skos:prefLabel xml:lang="fr">arène</skos:prefLabel>
    </owl:NamedIndividual>
    


    <!-- http://data.ign.fr/id/codes/topo/typedebatiment/BatimentAgricole -->


    <owl:NamedIndividual rdf:about="http://data.ign.fr/id/codes/topo/typedebatiment/BatimentAgricole">
        <rdf:type rdf:resource="http://data.ign.fr/def/topo#TypeDeBatiment"/>
        <rdf:type rdf:resource="http://www.w3.org/2004/02/skos/core#Concept"/>
        <skos:definition xml:lang="en">Building reserved for agricultural activities: industrial breeding building, agricultural shed (large), flour mill.</skos:definition>
        <skos:definition xml:lang="fr">Bâtiment réservé à des activités agricoles : bâtiment d&apos;élevage industriel, hangar agricole (grand), minoterie.</skos:definition>
        <skos:inScheme rdf:resource="http://data.ign.fr/id/codes/topo/typedebatiment/liste"/>
        <skos:prefLabel xml:lang="fr">bâtiment agricole</skos:prefLabel>
        <skos:prefLabel xml:lang="en">farm building</skos:prefLabel>
    </owl:NamedIndividual>
    


    <!-- http://data.ign.fr/id/codes/topo/typedebatiment/BatimentCommercial -->


    <owl:NamedIndividual rdf:about="http://data.ign.fr/id/codes/topo/typedebatiment/BatimentCommercial">
        <rdf:type rdf:resource="http://data.ign.fr/def/topo#TypeDeBatiment"/>
        <rdf:type rdf:resource="http://data.ign.fr/def/topo#TypeDeZAI"/>
        <rdf:type rdf:resource="http://www.w3.org/2004/02/skos/core#Concept"/>
        <skos:broader rdf:resource="http://data.ign.fr/id/codes/topo/typedezai/PAIIndustrielCommercial"/>
        <skos:definition xml:lang="en">Building or area of large area reserved for commercial activities: shopping center, hypermarket, store (large, isolated), fairground (building), commercial area.</skos:definition>
        <skos:definition xml:lang="fr">Bâtiment ou zone de grande surface réservé à des activités commerciales : centre commercial, hypermarché, magasin (grand, isolé), parc des expositions (bâtiment), zone à caractère commercial.</skos:definition>
        <skos:inScheme rdf:resource="http://data.ign.fr/id/codes/topo/typedebatiment/liste"/>
        <skos:inScheme rdf:resource="http://data.ign.fr/id/codes/topo/typedezai/liste"/>
        <skos:prefLabel xml:lang="fr">bâtiment ou zone à caractère commercial</skos:prefLabel>
        <skos:prefLabel xml:lang="en">commercial building or area</skos:prefLabel>
    </owl:NamedIndividual>
    


    <!-- http://data.ign.fr/id/codes/topo/typedebatiment/BatimentIndustriel -->


    <owl:NamedIndividual rdf:about="http://data.ign.fr/id/codes/topo/typedebatiment/BatimentIndustriel">
        <rdf:type rdf:resource="http://data.ign.fr/def/topo#TypeDeBatiment"/>
        <rdf:type rdf:resource="http://data.ign.fr/def/topo#TypeDeZAI"/>
        <rdf:type rdf:resource="http://www.w3.org/2004/02/skos/core#Concept"/>
        <skos:broader rdf:resource="http://data.ign.fr/id/codes/topo/typedezai/PAIIndustrielCommercial"/>
        <skos:definition xml:lang="en">Building or area reserved for industrial activities not specifically distinguished: research center, depot, cooperative (winemaking, cereal &apos;), mushroom, poultry farming, stud farm, slaughterhouse, refuse center, workshop (large), station platform awning) , toll canopy, industrial building (large), power station (building), technical construction, warehouse, industrial shed (big), sawmill, factory.</skos:definition>
        <skos:definition xml:lang="fr">Bâtiment ou zone réservé à des activités industrielles non distingué de façon spécifique : centre de recherche, dépôt, coopérative (vinicole, céréaliè&apos;), champignonniè, élevage avicole, haras, abattoir, déchèterie, atelier (grand), auvent de quai de gare), auvent de péage, bâtiment industriel (grand), centrale électrique (bâtiment), construction technique, entrepôt, hangar industriel (grand), scierie, usine.</skos:definition>
        <skos:inScheme rdf:resource="http://data.ign.fr/id/codes/topo/typedebatiment/liste"/>
        <skos:inScheme rdf:resource="http://data.ign.fr/id/codes/topo/typedezai/liste"/>
        <skos:prefLabel xml:lang="fr">bâtiment ou zone à caractère industriel</skos:prefLabel>
        <skos:prefLabel xml:lang="en">industrial building or area</skos:prefLabel>
    </owl:NamedIndividual>
    


    <!-- http://data.ign.fr/id/codes/topo/typedebatiment/BatimentReligieux -->


    <owl:NamedIndividual rdf:about="http://data.ign.fr/id/codes/topo/typedebatiment/BatimentReligieux">
        <rdf:type rdf:resource="http://data.ign.fr/def/topo#TypeDeBatiment"/>
        <rdf:type rdf:resource="http://www.w3.org/2004/02/skos/core#Concept"/>
        <skos:definition xml:lang="en">Building reserved for the exercise of a religious cult, other than a chapel or a church: mosque, synagogue, temple.</skos:definition>
        <skos:definition xml:lang="fr">Bâtiment réservé à l’exercice d’un culte religieux, autre qu’une chapelle ou qu’une église : mosquée, synagogue, temple.</skos:definition>
        <skos:inScheme rdf:resource="http://data.ign.fr/id/codes/topo/typedebatiment/liste"/>
        <skos:prefLabel xml:lang="fr">bâtiment religieux</skos:prefLabel>
        <skos:prefLabel xml:lang="en">religious building</skos:prefLabel>
    </owl:NamedIndividual>
    


    <!-- http://data.ign.fr/id/codes/topo/typedebatiment/BatimentSportif -->


    <owl:NamedIndividual rdf:about="http://data.ign.fr/id/codes/topo/typedebatiment/BatimentSportif">
        <rdf:type rdf:resource="http://data.ign.fr/def/topo#TypeDeBatiment"/>
        <rdf:type rdf:resource="http://www.w3.org/2004/02/skos/core#Concept"/>
        <skos:definition xml:lang="fr">Bâtiment réservé à la pratique sportive : gymnase, piscine couverte, salle de sport, tennis couvert.</skos:definition>
        <skos:definition xml:lang="en">Sports building: gym, indoor pool, gym, indoor tennis.</skos:definition>
        <skos:inScheme rdf:resource="http://data.ign.fr/id/codes/topo/typedebatiment/liste"/>
        <skos:prefLabel xml:lang="fr">bâtiment sportif</skos:prefLabel>
        <skos:prefLabel xml:lang="en">sports building</skos:prefLabel>
    </owl:NamedIndividual>
    


    <!-- http://data.ign.fr/id/codes/topo/typedebatiment/Chapelle -->


    <owl:NamedIndividual rdf:about="http://data.ign.fr/id/codes/topo/typedebatiment/Chapelle">
        <rdf:type rdf:resource="http://data.ign.fr/def/topo#TypeDeBatiment"/>
        <rdf:type rdf:resource="http://www.w3.org/2004/02/skos/core#Concept"/>
        <skos:definition xml:lang="fr">Petit édifice religieux catholique de forme caractéristique.</skos:definition>
        <skos:definition xml:lang="en">Small Catholic religious building of characteristic form.</skos:definition>
        <skos:inScheme rdf:resource="http://data.ign.fr/id/codes/topo/typedebatiment/liste"/>
        <skos:prefLabel xml:lang="en">chapel</skos:prefLabel>
        <skos:prefLabel xml:lang="fr">chapelle</skos:prefLabel>
    </owl:NamedIndividual>
    


    <!-- http://data.ign.fr/id/codes/topo/typedebatiment/Chateau -->


    <owl:NamedIndividual rdf:about="http://data.ign.fr/id/codes/topo/typedebatiment/Chateau">
        <rdf:type rdf:resource="http://data.ign.fr/def/topo#TypeDeBatiment"/>
        <rdf:type rdf:resource="http://data.ign.fr/def/topo#TypeDeZAI"/>
        <rdf:type rdf:resource="http://www.w3.org/2004/02/skos/core#Concept"/>
        <skos:broader rdf:resource="http://data.ign.fr/id/codes/topo/typedezai/PAIZoneHabitation"/>
        <skos:definition xml:lang="en">Habitation or former feudal, royal or seigniorial dwelling: castle, castle, citadel, tower. The locality, still named, may not be inhabited or be inhabited but is not totally in ruins.</skos:definition>
        <skos:definition xml:lang="fr">Habitation ou ancienne habitation féodale, royale ou seigneuriale: château, château fort, citadelle, tour. Le lieu-dit, toujours nommé, peut ne pas être habité ou ne plus être habité mais n&apos;est pas totalement en ruines.</skos:definition>
        <skos:inScheme rdf:resource="http://data.ign.fr/id/codes/topo/typedebatiment/liste"/>
        <skos:inScheme rdf:resource="http://data.ign.fr/id/codes/topo/typedezai/liste"/>
        <skos:prefLabel xml:lang="en">castle</skos:prefLabel>
        <skos:prefLabel xml:lang="fr">château</skos:prefLabel>
    </owl:NamedIndividual>
    


    <!-- http://data.ign.fr/id/codes/topo/typedebatiment/ConstructionLegere -->


    <owl:NamedIndividual rdf:about="http://data.ign.fr/id/codes/topo/typedebatiment/ConstructionLegere">
        <rdf:type rdf:resource="http://data.ign.fr/def/topo#TypeDeBatiment"/>
        <rdf:type rdf:resource="http://www.w3.org/2004/02/skos/core#Concept"/>
        <skos:definition xml:lang="en">Light structure not attached to the ground through foundations (cabins, garden sheds ...) or any building open on at least one side (yards, awnings, stands).</skos:definition>
        <skos:definition xml:lang="fr">Structure légère non attachée au sol par l’intermédiaire de fondations (cabanes, abris de jardins…) ou bâtiment quelconque ouvert sur au moins un côté (préaux, auvents, tribunes).</skos:definition>
        <skos:inScheme rdf:resource="http://data.ign.fr/id/codes/topo/typedebatiment/liste"/>
        <skos:prefLabel xml:lang="fr">construction légère</skos:prefLabel>
        <skos:prefLabel xml:lang="en">light construction</skos:prefLabel>
    </owl:NamedIndividual>
    


    <!-- http://data.ign.fr/id/codes/topo/typedebatiment/Eglise -->


    <owl:NamedIndividual rdf:about="http://data.ign.fr/id/codes/topo/typedebatiment/Eglise">
        <rdf:type rdf:resource="http://data.ign.fr/def/topo#TypeDeBatiment"/>
        <rdf:type rdf:resource="http://www.w3.org/2004/02/skos/core#Concept"/>
        <skos:definition xml:lang="en">Characteristic Catholic religious building: basilica, cathedral, church.</skos:definition>
        <skos:definition xml:lang="fr">Édifice religieux catholique de forme caractéristique : basilique, cathédrale, église.</skos:definition>
        <skos:inScheme rdf:resource="http://data.ign.fr/id/codes/topo/typedebatiment/liste"/>
        <skos:prefLabel xml:lang="en">church</skos:prefLabel>
        <skos:prefLabel xml:lang="fr">église</skos:prefLabel>
    </owl:NamedIndividual>
    


    <!-- http://data.ign.fr/id/codes/topo/typedebatiment/Fort -->


    <owl:NamedIndividual rdf:about="http://data.ign.fr/id/codes/topo/typedebatiment/Fort">
        <rdf:type rdf:resource="http://data.ign.fr/def/topo#TypeDeBatiment"/>
        <rdf:type rdf:resource="http://www.w3.org/2004/02/skos/core#Concept"/>
        <skos:altLabel xml:lang="fr">blockhaus</skos:altLabel>
        <skos:altLabel xml:lang="en">blockhouse</skos:altLabel>
        <skos:altLabel xml:lang="en">casemate</skos:altLabel>
        <skos:altLabel xml:lang="fr">casemate</skos:altLabel>
        <skos:definition xml:lang="en">Military work: blockhouse, casemate, fort, fortified work.</skos:definition>
        <skos:definition xml:lang="fr">Ouvrage militaire : blockhaus, casemate, fort, ouvrage fortifié.</skos:definition>
        <skos:inScheme rdf:resource="http://data.ign.fr/id/codes/topo/typedebatiment/liste"/>
        <skos:prefLabel xml:lang="en">fort</skos:prefLabel>
        <skos:prefLabel xml:lang="fr">fort</skos:prefLabel>
    </owl:NamedIndividual>
    


    <!-- http://data.ign.fr/id/codes/topo/typedebatiment/Gare -->


    <owl:NamedIndividual rdf:about="http://data.ign.fr/id/codes/topo/typedebatiment/Gare">
        <rdf:type rdf:resource="http://data.ign.fr/def/topo#TypeDeBatiment"/>
        <rdf:type rdf:resource="http://www.w3.org/2004/02/skos/core#Concept"/>
        <skos:definition xml:lang="en">Building used for boarding and disembarking passengers by train.</skos:definition>
        <skos:definition xml:lang="fr">Bâtiment servant à l&apos;embarquement et au débarquement des voyageurs en train.</skos:definition>
        <skos:inScheme rdf:resource="http://data.ign.fr/id/codes/topo/typedebatiment/liste"/>
        <skos:prefLabel xml:lang="fr">gare</skos:prefLabel>
        <skos:prefLabel xml:lang="en">station</skos:prefLabel>
    </owl:NamedIndividual>
    


    <!-- http://data.ign.fr/id/codes/topo/typedebatiment/Mairie -->


    <owl:NamedIndividual rdf:about="http://data.ign.fr/id/codes/topo/typedebatiment/Mairie">
        <rdf:type rdf:resource="http://data.ign.fr/def/topo#TypeDeBatiment"/>
        <rdf:type rdf:resource="http://www.w3.org/2004/02/skos/core#Concept"/>
        <skos:altLabel xml:lang="en">city hall</skos:altLabel>
        <skos:altLabel xml:lang="fr">hôtel de ville</skos:altLabel>
        <skos:broader rdf:resource="http://data.ign.fr/id/codes/topo/typedezai/PAIAdministratifOuMilitaire"/>
        <skos:definition xml:lang="en">Building where are the services of the municipal administration, also called city hall.</skos:definition>
        <skos:definition xml:lang="fr">Édifice où se trouvent les services de l&apos;administration municipale, appelé aussi hôtel de ville.</skos:definition>
        <skos:inScheme rdf:resource="http://data.ign.fr/id/codes/topo/typedebatiment/liste"/>
        <skos:inScheme rdf:resource="http://data.ign.fr/id/codes/topo/typedezai/liste"/>
        <skos:prefLabel xml:lang="fr">mairie</skos:prefLabel>
        <skos:prefLabel xml:lang="en">town-hall</skos:prefLabel>
    </owl:NamedIndividual>
    


    <!-- http://data.ign.fr/id/codes/topo/typedebatiment/Monument -->


    <owl:NamedIndividual rdf:about="http://data.ign.fr/id/codes/topo/typedebatiment/Monument">
        <rdf:type rdf:resource="http://data.ign.fr/def/topo#TypeDeBatiment"/>
        <rdf:type rdf:resource="http://www.w3.org/2004/02/skos/core#Concept"/>
        <skos:broader rdf:resource="http://data.ign.fr/id/codes/topo/typedezai/PAICultureLoisirs"/>
        <skos:definition xml:lang="en">Any memorial without particular religious character: monument, statue, stele. The triumphal arches are excluded.</skos:definition>
        <skos:definition xml:lang="fr">Monument commémoratif quelconque, sans caractère religieux particulier : monument, statue, stèle. Les arcs de triomphe sont exclus.</skos:definition>
        <skos:inScheme rdf:resource="http://data.ign.fr/id/codes/topo/typedebatiment/liste"/>
        <skos:inScheme rdf:resource="http://data.ign.fr/id/codes/topo/typedezai/liste"/>
        <skos:prefLabel xml:lang="en">monument</skos:prefLabel>
        <skos:prefLabel xml:lang="fr">monument</skos:prefLabel>
    </owl:NamedIndividual>
    


    <!-- http://data.ign.fr/id/codes/topo/typedebatiment/Peage -->


    <owl:NamedIndividual rdf:about="http://data.ign.fr/id/codes/topo/typedebatiment/Peage">
        <rdf:type rdf:resource="http://data.ign.fr/def/topo#TypeDeBatiment"/>
        <rdf:type rdf:resource="http://www.w3.org/2004/02/skos/core#Concept"/>
        <skos:definition xml:lang="en">Building where are collected the rights of use.</skos:definition>
        <skos:definition xml:lang="fr">Bâtiment où sont perçus les droits d‘usage.</skos:definition>
        <skos:inScheme rdf:resource="http://data.ign.fr/id/codes/topo/typedebatiment/liste"/>
        <skos:prefLabel xml:lang="fr">péage</skos:prefLabel>
        <skos:prefLabel xml:lang="en">toll</skos:prefLabel>
        <skos:relatedMatch rdf:resource="http://data.ign.fr/id/codes/topo/typedezai/Peage"/>
    </owl:NamedIndividual>
    


    <!-- http://data.ign.fr/id/codes/topo/typedebatiment/Prefecture -->


    <owl:NamedIndividual rdf:about="http://data.ign.fr/id/codes/topo/typedebatiment/Prefecture">
        <rdf:type rdf:resource="http://data.ign.fr/def/topo#TypeDeBatiment"/>
        <rdf:type rdf:resource="http://www.w3.org/2004/02/skos/core#Concept"/>
        <skos:broader rdf:resource="http://data.ign.fr/id/codes/topo/typedezai/PAIAdministratifOuMilitaire"/>
        <skos:definition xml:lang="en">Building where prefectural services are installed.</skos:definition>
        <skos:definition xml:lang="fr">Bâtiment où sont installés les services préfectoraux.</skos:definition>
        <skos:inScheme rdf:resource="http://data.ign.fr/id/codes/topo/typedebatiment/liste"/>
        <skos:inScheme rdf:resource="http://data.ign.fr/id/codes/topo/typedezai/liste"/>
        <skos:prefLabel xml:lang="en">prefecture</skos:prefLabel>
        <skos:prefLabel xml:lang="fr">préfecture</skos:prefLabel>
    </owl:NamedIndividual>
    


    <!-- http://data.ign.fr/id/codes/topo/typedebatiment/Serre -->


    <owl:NamedIndividual rdf:about="http://data.ign.fr/id/codes/topo/typedebatiment/Serre">
        <rdf:type rdf:resource="http://data.ign.fr/def/topo#TypeDeBatiment"/>
        <rdf:type rdf:resource="http://www.w3.org/2004/02/skos/core#Concept"/>
        <skos:definition xml:lang="fr">Abri clos à parois translucides destiné à protéger les végétaux du froid : jardinerie, serre.</skos:definition>
        <skos:definition xml:lang="en">Closed shelter with translucent walls intended to protect plants from the cold: gardening, greenhouse.</skos:definition>
        <skos:inScheme rdf:resource="http://data.ign.fr/id/codes/topo/typedebatiment/liste"/>
        <skos:prefLabel xml:lang="en">glass-house</skos:prefLabel>
        <skos:prefLabel xml:lang="fr">serre</skos:prefLabel>
    </owl:NamedIndividual>
    


    <!-- http://data.ign.fr/id/codes/topo/typedebatiment/Silo -->


    <owl:NamedIndividual rdf:about="http://data.ign.fr/id/codes/topo/typedebatiment/Silo">
        <rdf:type rdf:resource="http://data.ign.fr/def/topo#TypeDeBatiment"/>
        <rdf:type rdf:resource="http://www.w3.org/2004/02/skos/core#Concept"/>
        <skos:definition xml:lang="fr">Réservoir, qui chargé par le haut se vide par le bas, et qui sert de dépôt, de magasin, etc. Le silo est exclusivement destiné aux produits agricoles : cuve à vin, silo.</skos:definition>
        <skos:definition xml:lang="en">Tank, which is loaded from the top empties from the bottom, and which serves as a depot, store, etc. The silo is exclusively for agricultural products: wine tank, silo.</skos:definition>
        <skos:inScheme rdf:resource="http://data.ign.fr/id/codes/topo/typedebatiment/liste"/>
        <skos:prefLabel xml:lang="en">silo</skos:prefLabel>
        <skos:prefLabel xml:lang="fr">silo</skos:prefLabel>
    </owl:NamedIndividual>
    


    <!-- http://data.ign.fr/id/codes/topo/typedebatiment/SousPrefecture -->


    <owl:NamedIndividual rdf:about="http://data.ign.fr/id/codes/topo/typedebatiment/SousPrefecture">
        <rdf:type rdf:resource="http://data.ign.fr/def/topo#TypeDeBatiment"/>
        <rdf:type rdf:resource="http://www.w3.org/2004/02/skos/core#Concept"/>
        <skos:broader rdf:resource="http://data.ign.fr/id/codes/topo/typedezai/PAIAdministratifOuMilitaire"/>
        <skos:definition xml:lang="en">Building where are the offices of the sub-prefect: chief town of district.</skos:definition>
        <skos:definition xml:lang="fr">Bâtiment où sont les bureaux du sous-préfet: chef-lieu d’arrondissement.</skos:definition>
        <skos:inScheme rdf:resource="http://data.ign.fr/id/codes/topo/typedebatiment/liste"/>
        <skos:inScheme rdf:resource="http://data.ign.fr/id/codes/topo/typedezai/liste"/>
        <skos:prefLabel xml:lang="fr">sous-préfecture</skos:prefLabel>
        <skos:prefLabel xml:lang="en">subprefecture</skos:prefLabel>
    </owl:NamedIndividual>
    


    <!-- http://data.ign.fr/id/codes/topo/typedebatiment/Tour -->


    <owl:NamedIndividual rdf:about="http://data.ign.fr/id/codes/topo/typedebatiment/Tour">
        <rdf:type rdf:resource="http://data.ign.fr/def/topo#TypeDeBatiment"/>
        <rdf:type rdf:resource="http://www.w3.org/2004/02/skos/core#Concept"/>
        <skos:altLabel xml:lang="en">donjon</skos:altLabel>
        <skos:altLabel xml:lang="fr">donjon</skos:altLabel>
        <skos:altLabel xml:lang="en">mill</skos:altLabel>
        <skos:altLabel xml:lang="fr">moulin</skos:altLabel>
        <skos:definition xml:lang="fr">Bâtiment remarquable dans le paysage par sa forme élevée : donjon, moulin à vent, tour, tour de contrôle.</skos:definition>
        <skos:definition xml:lang="en">Remarkable building in the landscape by its high form: dungeon, windmill, tower, control tower.</skos:definition>
        <skos:inScheme rdf:resource="http://data.ign.fr/id/codes/topo/typedebatiment/liste"/>
        <skos:prefLabel xml:lang="fr">tour</skos:prefLabel>
        <skos:prefLabel xml:lang="en">tower</skos:prefLabel>
    </owl:NamedIndividual>
    


    <!-- http://data.ign.fr/id/codes/topo/typedebatiment/Tribune -->


    <owl:NamedIndividual rdf:about="http://data.ign.fr/id/codes/topo/typedebatiment/Tribune">
        <rdf:type rdf:resource="http://data.ign.fr/def/topo#TypeDeBatiment"/>
        <rdf:type rdf:resource="http://www.w3.org/2004/02/skos/core#Concept"/>
        <skos:definition xml:lang="fr">Tribune de terrain de sport (stade, hippodrome, vélodrome,…).</skos:definition>
        <skos:definition xml:lang="en">Tribune of sports ground (stadium, racecourse, velodrome, ...).</skos:definition>
        <skos:inScheme rdf:resource="http://data.ign.fr/id/codes/topo/typedebatiment/liste"/>
        <skos:prefLabel xml:lang="en">stand</skos:prefLabel>
        <skos:prefLabel xml:lang="fr">tribune</skos:prefLabel>
    </owl:NamedIndividual>
    


    <!-- http://data.ign.fr/id/codes/topo/typedebatiment/liste -->


    <owl:NamedIndividual rdf:about="http://data.ign.fr/id/codes/topo/typedebatiment/liste">
        <rdf:type rdf:resource="http://www.w3.org/2004/02/skos/core#ConceptScheme"/>
        <rdfs:comment xml:lang="en">List of different types of buildings, represented as a hierarchy of SKOS concepts.</rdfs:comment>
        <rdfs:comment xml:lang="fr">Liste des différents types de bâtiments, représentés comme une hiérarchie de concepts SKOS.</rdfs:comment>
        <rdfs:label xml:lang="fr">Type de bâtiment</rdfs:label>
        <rdfs:label xml:lang="en">Type of building</rdfs:label>
    </owl:NamedIndividual>
    


    <!-- http://data.ign.fr/id/codes/topo/typedeconstruction/Antenne -->


    <owl:NamedIndividual rdf:about="http://data.ign.fr/id/codes/topo/typedeconstruction/Antenne">
        <rdf:type rdf:resource="http://data.ign.fr/def/topo#TypeDeConstruction"/>
        <rdf:type rdf:resource="http://www.w3.org/2004/02/skos/core#Concept"/>
        <skos:definition xml:lang="fr">Construction destinée à la réception ou à l&apos;émission d&apos;ondes électromagnétiques : antenne, pylône de télécommunication.</skos:definition>
        <skos:definition xml:lang="en">Construction intended for receiving or emitting electromagnetic waves: antenna, telecommunication tower.</skos:definition>
        <skos:inScheme rdf:resource="http://data.ign.fr/id/codes/topo/typedeconstruction/liste"/>
        <skos:prefLabel xml:lang="en">antenna</skos:prefLabel>
        <skos:prefLabel xml:lang="fr">antenne</skos:prefLabel>
    </owl:NamedIndividual>
    


    <!-- http://data.ign.fr/id/codes/topo/typedeconstruction/Barrage -->


    <owl:NamedIndividual rdf:about="http://data.ign.fr/id/codes/topo/typedeconstruction/Barrage">
        <rdf:type rdf:resource="http://data.ign.fr/def/topo#TypeDeConstruction"/>
        <rdf:type rdf:resource="http://data.ign.fr/def/topo#TypeDeFranchissement"/>
        <rdf:type rdf:resource="http://www.w3.org/2004/02/skos/core#Concept"/>
        <skos:broadMatch rdf:resource="http://data.ign.fr/id/codes/topo/typedezai/Barrage"/>
        <skos:definition xml:lang="fr">Ouvrage établi en travers du lit d’un cours d’eau et créant une dénivellation du plan d’eau entre l’amont et l’aval : barrage, vanne.</skos:definition>
        <skos:definition xml:lang="en">Work established across the bed of a river and creating a difference in level of water between upstream and downstream: dam, valve.</skos:definition>
        <skos:inScheme rdf:resource="http://data.ign.fr/id/codes/topo/typedeconstruction/liste"/>
        <skos:inScheme rdf:resource="http://data.ign.fr/id/codes/topo/typedefranchissement/liste"/>
        <skos:prefLabel xml:lang="fr">barrage</skos:prefLabel>
        <skos:prefLabel xml:lang="en">dam</skos:prefLabel>
    </owl:NamedIndividual>
    


    <!-- http://data.ign.fr/id/codes/topo/typedeconstruction/Cheminee -->


    <owl:NamedIndividual rdf:about="http://data.ign.fr/id/codes/topo/typedeconstruction/Cheminee">
        <rdf:type rdf:resource="http://data.ign.fr/def/topo#TypeDeConstruction"/>
        <rdf:type rdf:resource="http://www.w3.org/2004/02/skos/core#Concept"/>
        <skos:definition xml:lang="fr">Construction destinée à l&apos;émission de fumées ou de gaz.</skos:definition>
        <skos:definition xml:lang="en">Construction intended for the emission of fumes or gas.</skos:definition>
        <skos:inScheme rdf:resource="http://data.ign.fr/id/codes/topo/typedeconstruction/liste"/>
        <skos:prefLabel xml:lang="fr">cheminée</skos:prefLabel>
        <skos:prefLabel xml:lang="en">chimney</skos:prefLabel>
    </owl:NamedIndividual>
    


    <!-- http://data.ign.fr/id/codes/topo/typedeconstruction/DalleDeProtection -->


    <owl:NamedIndividual rdf:about="http://data.ign.fr/id/codes/topo/typedeconstruction/DalleDeProtection">
        <rdf:type rdf:resource="http://data.ign.fr/def/topo#TypeDeConstruction"/>
        <rdf:type rdf:resource="http://www.w3.org/2004/02/skos/core#Concept"/>
        <skos:definition xml:lang="fr">Dalle (ou auvent) horizontale protégeant une voie de communication des chutes de pierres, des coulées de neige, ou protégeant le voisinage du bruit.</skos:definition>
        <skos:definition xml:lang="en">Horizontal slab (or awning) protecting a communication path from falling rocks, snowflows, or protecting the neighborhood from noise.</skos:definition>
        <skos:inScheme rdf:resource="http://data.ign.fr/id/codes/topo/typedeconstruction/liste"/>
        <skos:prefLabel xml:lang="fr">dalle de protection</skos:prefLabel>
        <skos:prefLabel xml:lang="en">protective wall</skos:prefLabel>
    </owl:NamedIndividual>
    


    <!-- http://data.ign.fr/id/codes/topo/typedeconstruction/Ecluse -->


    <owl:NamedIndividual rdf:about="http://data.ign.fr/id/codes/topo/typedeconstruction/Ecluse">
        <rdf:type rdf:resource="http://data.ign.fr/def/topo#TypeDeConstruction"/>
        <rdf:type rdf:resource="http://www.w3.org/2004/02/skos/core#Concept"/>
        <skos:broadMatch rdf:resource="http://data.ign.fr/id/codes/topo/typedezai/Barrage"/>
        <skos:definition xml:lang="en">Hydraulic structure consisting essentially of doors equipped with valves to retain or release water as needed: boat lift, dry dock, lock, refit.</skos:definition>
        <skos:definition xml:lang="fr">Ouvrage hydraulique formé essentiellement de portes munies de vannes destiné à retenir ou à lâcher l’eau selon les besoins : ascenseur à bateaux, cale sèche, écluse, radoub.</skos:definition>
        <skos:inScheme rdf:resource="http://data.ign.fr/id/codes/topo/typedeconstruction/liste"/>
        <skos:prefLabel xml:lang="en">lock</skos:prefLabel>
        <skos:prefLabel xml:lang="fr">écluse</skos:prefLabel>
    </owl:NamedIndividual>
    


    <!-- http://data.ign.fr/id/codes/topo/typedeconstruction/Eolienne -->


    <owl:NamedIndividual rdf:about="http://data.ign.fr/id/codes/topo/typedeconstruction/Eolienne">
        <rdf:type rdf:resource="http://data.ign.fr/def/topo#TypeDeConstruction"/>
        <rdf:type rdf:resource="http://www.w3.org/2004/02/skos/core#Concept"/>
        <skos:definition xml:lang="en">A wind turbine is a device that uses wind energy to produce mechanical energy or electricity.</skos:definition>
        <skos:definition xml:lang="fr">Une éolienne est un dispositif permettant d&apos;utiliser l&apos;énergie éolienne pour produire de l&apos;énergie mécanique ou bien de l&apos;électricité.</skos:definition>
        <skos:inScheme rdf:resource="http://data.ign.fr/id/codes/topo/typedeconstruction/liste"/>
        <skos:prefLabel xml:lang="en">wind pump</skos:prefLabel>
        <skos:prefLabel xml:lang="fr">éolienne</skos:prefLabel>
    </owl:NamedIndividual>
    


    <!-- http://data.ign.fr/id/codes/topo/typedeconstruction/EscalierMonumental -->


    <owl:NamedIndividual rdf:about="http://data.ign.fr/id/codes/topo/typedeconstruction/EscalierMonumental">
        <rdf:type rdf:resource="http://data.ign.fr/def/topo#TypeDeConstruction"/>
        <rdf:type rdf:resource="http://www.w3.org/2004/02/skos/core#Concept"/>
        <skos:definition xml:lang="fr">Escalier monumental.</skos:definition>
        <skos:definition xml:lang="en">Monumental staircase.</skos:definition>
        <skos:inScheme rdf:resource="http://data.ign.fr/id/codes/topo/typedeconstruction/liste"/>
        <skos:prefLabel xml:lang="fr">escalier monumental</skos:prefLabel>
        <skos:prefLabel xml:lang="en">monumental stairs</skos:prefLabel>
    </owl:NamedIndividual>
    


    <!-- http://data.ign.fr/id/codes/topo/typedeconstruction/MurAntiBruit -->


    <owl:NamedIndividual rdf:about="http://data.ign.fr/id/codes/topo/typedeconstruction/MurAntiBruit">
        <rdf:type rdf:resource="http://data.ign.fr/def/topo#TypeDeConstruction"/>
        <rdf:type rdf:resource="http://www.w3.org/2004/02/skos/core#Concept"/>
        <skos:definition xml:lang="fr">Mur destiné à protéger les riverains d’une voie de communication du bruit qu’elle engendre.</skos:definition>
        <skos:definition xml:lang="en">Wall intended to protect residents of a communication channel from the noise it generates.</skos:definition>
        <skos:inScheme rdf:resource="http://data.ign.fr/id/codes/topo/typedeconstruction/liste"/>
        <skos:prefLabel xml:lang="fr">mur anti-bruit</skos:prefLabel>
        <skos:prefLabel xml:lang="en">sound attenuation barrier</skos:prefLabel>
    </owl:NamedIndividual>
    


    <!-- http://data.ign.fr/id/codes/topo/typedeconstruction/Phare -->


    <owl:NamedIndividual rdf:about="http://data.ign.fr/id/codes/topo/typedeconstruction/Phare">
        <rdf:type rdf:resource="http://data.ign.fr/def/topo#TypeDeConstruction"/>
        <rdf:type rdf:resource="http://www.w3.org/2004/02/skos/core#Concept"/>
        <skos:definition xml:lang="en">High tower carrying at the top a more or less powerful focus intended to guide the ships during the night.</skos:definition>
        <skos:definition xml:lang="fr">Tour élevée portant au sommet un foyer plus ou moins puissant destiné à guider les navires pendant la nuit.</skos:definition>
        <skos:inScheme rdf:resource="http://data.ign.fr/id/codes/topo/typedeconstruction/liste"/>
        <skos:prefLabel xml:lang="en">lighthouse</skos:prefLabel>
        <skos:prefLabel xml:lang="fr">phare</skos:prefLabel>
    </owl:NamedIndividual>
    


    <!-- http://data.ign.fr/id/codes/topo/typedeconstruction/Quai -->


    <owl:NamedIndividual rdf:about="http://data.ign.fr/id/codes/topo/typedeconstruction/Quai">
        <rdf:type rdf:resource="http://data.ign.fr/def/topo#TypeDeConstruction"/>
        <rdf:type rdf:resource="http://www.w3.org/2004/02/skos/core#Concept"/>
        <skos:definition xml:lang="fr">Muraille en maçonnerie ou enrochement, élevée le long d’un cours d’eau pour retenir les berges, pour empêcher les débordements. Rivage d’un port aménagé pour l’accostage des bateaux. Ouvrage en maçonnerie s’opposant à l’écoulement des eaux marines ou fluviales.</skos:definition>
        <skos:definition xml:lang="en">Wall in masonry or rip rap, raised along a stream to retain the banks, to prevent overflows. Shoreline of a harbor arranged for the docking of the boats. Masonry structure opposing the flow of marine or fluvial waters.</skos:definition>
        <skos:inScheme rdf:resource="http://data.ign.fr/id/codes/topo/typedeconstruction/liste"/>
        <skos:prefLabel xml:lang="fr">quai</skos:prefLabel>
        <skos:prefLabel xml:lang="en">wharf</skos:prefLabel>
    </owl:NamedIndividual>
    


    <!-- http://data.ign.fr/id/codes/topo/typedeconstruction/Ruines -->


    <owl:NamedIndividual rdf:about="http://data.ign.fr/id/codes/topo/typedeconstruction/Ruines">
        <rdf:type rdf:resource="http://data.ign.fr/def/topo#TypeDeConstruction"/>
        <rdf:type rdf:resource="http://www.w3.org/2004/02/skos/core#Concept"/>
        <skos:broader rdf:resource="http://data.ign.fr/id/codes/topo/typedezai/PAIZoneHabitation"/>
        <skos:definition xml:lang="en">Building or construction in ruins.</skos:definition>
        <skos:definition xml:lang="fr">Bâtiment ou construction en ruines.</skos:definition>
        <skos:inScheme rdf:resource="http://data.ign.fr/id/codes/topo/typedeconstruction/liste"/>
        <skos:inScheme rdf:resource="http://data.ign.fr/id/codes/topo/typedezai/liste"/>
        <skos:prefLabel xml:lang="fr">ruines</skos:prefLabel>
        <skos:prefLabel xml:lang="en">ruins</skos:prefLabel>
    </owl:NamedIndividual>
    


    <!-- http://data.ign.fr/id/codes/topo/typedeconstruction/Torchere -->


    <owl:NamedIndividual rdf:about="http://data.ign.fr/id/codes/topo/typedeconstruction/Torchere">
        <rdf:type rdf:resource="http://data.ign.fr/def/topo#TypeDeConstruction"/>
        <rdf:type rdf:resource="http://www.w3.org/2004/02/skos/core#Concept"/>
        <skos:definition xml:lang="fr">Canalisation verticale par laquelle s&apos;échappent et brûlent les résidus gazeux d&apos;une raffinerie.</skos:definition>
        <skos:definition xml:lang="en">Vertical pipe through which escape and burn the gaseous residues of a refinery.</skos:definition>
        <skos:inScheme rdf:resource="http://data.ign.fr/id/codes/topo/typedeconstruction/liste"/>
        <skos:prefLabel xml:lang="en">flare tower</skos:prefLabel>
        <skos:prefLabel xml:lang="fr">torchère</skos:prefLabel>
    </owl:NamedIndividual>
    


    <!-- http://data.ign.fr/id/codes/topo/typedeconstruction/Transformateur -->


    <owl:NamedIndividual rdf:about="http://data.ign.fr/id/codes/topo/typedeconstruction/Transformateur">
        <rdf:type rdf:resource="http://data.ign.fr/def/topo#TypeDeConstruction"/>
        <rdf:type rdf:resource="http://www.w3.org/2004/02/skos/core#Concept"/>
        <skos:definition xml:lang="fr">Bâtiment technique dont la fonction est de transformer un système de courants variables en un ou plusieurs autres systèmes de courants variables de même fréquence, mais d’intensité ou de tension généralement différentes.</skos:definition>
        <skos:definition xml:lang="en">Technical building whose function is to transform a system of variable currents into one or more other systems of variable currents of the same frequency, but of generally different intensity or voltage.</skos:definition>
        <skos:inScheme rdf:resource="http://data.ign.fr/id/codes/topo/typedeconstruction/liste"/>
        <skos:prefLabel xml:lang="fr">transformateur</skos:prefLabel>
        <skos:prefLabel xml:lang="en">transformer</skos:prefLabel>
    </owl:NamedIndividual>
    


    <!-- http://data.ign.fr/id/codes/topo/typedeconstruction/liste -->


    <owl:NamedIndividual rdf:about="http://data.ign.fr/id/codes/topo/typedeconstruction/liste">
        <rdf:type rdf:resource="http://www.w3.org/2004/02/skos/core#ConceptScheme"/>
        <rdfs:comment xml:lang="en">List of different types of constructions, represented as a hierarchy of SKOS concepts.</rdfs:comment>
        <rdfs:comment xml:lang="fr">Liste des différents types de constructions, représentés comme une hiérarchie de concepts SKOS.</rdfs:comment>
        <rdfs:label xml:lang="fr">Type de construction</rdfs:label>
        <rdfs:label xml:lang="en">Type of structure</rdfs:label>
    </owl:NamedIndividual>
    


    <!-- http://data.ign.fr/id/codes/topo/typedefranchissement/Cascade -->


    <owl:NamedIndividual rdf:about="http://data.ign.fr/id/codes/topo/typedefranchissement/Cascade">
        <rdf:type rdf:resource="http://data.ign.fr/def/topo#TypeDeFranchissement"/>
        <rdf:type rdf:resource="http://data.ign.fr/def/topo#TypeDeZAI"/>
        <rdf:type rdf:resource="http://www.w3.org/2004/02/skos/core#Concept"/>
        <skos:broader rdf:resource="http://data.ign.fr/id/codes/topo/typedezai/PAIHydrographie"/>
        <skos:definition xml:lang="fr">Chute d’eau, cascade.</skos:definition>
        <skos:definition xml:lang="en">Waterfall</skos:definition>
        <skos:inScheme rdf:resource="http://data.ign.fr/id/codes/topo/typedefranchissement/liste"/>
        <skos:inScheme rdf:resource="http://data.ign.fr/id/codes/topo/typedezai/liste"/>
        <skos:prefLabel xml:lang="fr">cascade</skos:prefLabel>
        <skos:prefLabel xml:lang="en">waterfall</skos:prefLabel>
    </owl:NamedIndividual>
    


    <!-- http://data.ign.fr/id/codes/topo/typedefranchissement/Ecluse -->


    <owl:NamedIndividual rdf:about="http://data.ign.fr/id/codes/topo/typedefranchissement/Ecluse">
        <rdf:type rdf:resource="http://data.ign.fr/def/topo#TypeDeFranchissement"/>
        <rdf:type rdf:resource="http://www.w3.org/2004/02/skos/core#Concept"/>
        <skos:definition xml:lang="en">Hydraulic structure consisting essentially of doors equipped with valves to retain or release water as needed: Boat lift, lock.</skos:definition>
        <skos:definition xml:lang="fr">Ouvrage hydraulique formé essentiellement de portes munies de vannes destiné à retenir ou à lâcher l’eau selon les besoins : Ascenseur à bateaux, écluse.</skos:definition>
        <skos:inScheme rdf:resource="http://data.ign.fr/id/codes/topo/typedefranchissement/liste"/>
        <skos:prefLabel xml:lang="en">lock</skos:prefLabel>
        <skos:prefLabel xml:lang="fr">écluse</skos:prefLabel>
    </owl:NamedIndividual>
    


    <!-- http://data.ign.fr/id/codes/topo/typedefranchissement/Gue -->


    <owl:NamedIndividual rdf:about="http://data.ign.fr/id/codes/topo/typedefranchissement/Gue">
        <rdf:type rdf:resource="http://data.ign.fr/def/topo#TypeDeFranchissement"/>
        <rdf:type rdf:resource="http://www.w3.org/2004/02/skos/core#Concept"/>
        <skos:definition xml:lang="en">Passage natural or arranged allowing vehicles to work a watercourse without the use of a bridge or a boat.</skos:definition>
        <skos:definition xml:lang="fr">Passage naturel ou aménagé permettant aux véhicules de travaerser un cours d&apos;eau sans le recours d&apos;un pont ou d&apos;un bateau.</skos:definition>
        <skos:inScheme rdf:resource="http://data.ign.fr/id/codes/topo/typedefranchissement/liste"/>
        <skos:prefLabel xml:lang="en">ford</skos:prefLabel>
        <skos:prefLabel xml:lang="fr">gué</skos:prefLabel>
    </owl:NamedIndividual>
    


    <!-- http://data.ign.fr/id/codes/topo/typedefranchissement/Pont -->


    <owl:NamedIndividual rdf:about="http://data.ign.fr/id/codes/topo/typedefranchissement/Pont">
        <rdf:type rdf:resource="http://data.ign.fr/def/topo#TypeDeFranchissement"/>
        <rdf:type rdf:resource="http://www.w3.org/2004/02/skos/core#Concept"/>
        <skos:broader rdf:resource="http://data.ign.fr/id/codes/topo/typedezai/PAITransport"/>
        <skos:definition xml:lang="en">A work of art likely to span one or more elements of the road, rail or hydrographic network or allowing the crossing of a valley: bridge, footbridge, isolated bridge, moving bridge. Portion of the network located above the ground level.</skos:definition>
        <skos:definition xml:lang="fr">Ouvrage d’art susceptible d’enjamber un ou plusieurs éléments du réseau routier, ferré ou hydrographique ou permettant le franchissement d&apos;une vallée : pont, passerelle, pont isolé, pont mobile. Portion du réseau située au dessus du niveau du sol.</skos:definition>
        <skos:inScheme rdf:resource="http://data.ign.fr/id/codes/topo/typedeconstruction/liste"/>
        <skos:inScheme rdf:resource="http://data.ign.fr/id/codes/topo/typedefranchissement/liste"/>
        <skos:inScheme rdf:resource="http://data.ign.fr/id/codes/topo/typedezai/liste"/>
        <skos:prefLabel xml:lang="en">bridge</skos:prefLabel>
        <skos:prefLabel xml:lang="fr">pont</skos:prefLabel>
    </owl:NamedIndividual>
    


    <!-- http://data.ign.fr/id/codes/topo/typedefranchissement/PontCanal -->


    <owl:NamedIndividual rdf:about="http://data.ign.fr/id/codes/topo/typedefranchissement/PontCanal">
        <rdf:type rdf:resource="http://data.ign.fr/def/topo#TypeDeFranchissement"/>
        <rdf:type rdf:resource="http://www.w3.org/2004/02/skos/core#Concept"/>
        <skos:definition xml:lang="en">Section of artificial watercourses passing over a bridge.</skos:definition>
        <skos:definition xml:lang="fr">Tronçon de cours d’eau artificiel passant sur un pont.</skos:definition>
        <skos:inScheme rdf:resource="http://data.ign.fr/id/codes/topo/typedefranchissement/liste"/>
        <skos:prefLabel xml:lang="en">canal aqueduct</skos:prefLabel>
        <skos:prefLabel xml:lang="fr">pont-canal</skos:prefLabel>
    </owl:NamedIndividual>
    


    <!-- http://data.ign.fr/id/codes/topo/typedefranchissement/Tunnel -->


    <owl:NamedIndividual rdf:about="http://data.ign.fr/id/codes/topo/typedefranchissement/Tunnel">
        <rdf:type rdf:resource="http://data.ign.fr/def/topo#TypeDeFranchissement"/>
        <rdf:type rdf:resource="http://www.w3.org/2004/02/skos/core#Concept"/>
        <skos:broader rdf:resource="http://data.ign.fr/id/codes/topo/typedezai/PAITransport"/>
        <skos:definition xml:lang="fr">Portion souterraine du réseau.</skos:definition>
        <skos:definition xml:lang="en">Underground portion of the network.</skos:definition>
        <skos:inScheme rdf:resource="http://data.ign.fr/id/codes/topo/typedefranchissement/liste"/>
        <skos:inScheme rdf:resource="http://data.ign.fr/id/codes/topo/typedezai/liste"/>
        <skos:prefLabel xml:lang="en">tunnel</skos:prefLabel>
        <skos:prefLabel xml:lang="fr">tunnel</skos:prefLabel>
    </owl:NamedIndividual>
    


    <!-- http://data.ign.fr/id/codes/topo/typedefranchissement/liste -->


    <owl:NamedIndividual rdf:about="http://data.ign.fr/id/codes/topo/typedefranchissement/liste">
        <rdf:type rdf:resource="http://www.w3.org/2004/02/skos/core#ConceptScheme"/>
        <rdfs:comment xml:lang="en">List of the different types of obstacle or infrastructure dedicated to obstacle clearance, represented as a hierarchy of SKOS concepts.</rdfs:comment>
        <rdfs:comment xml:lang="fr">Liste des différents types d&apos;obstacles ou d&apos;infrastructures dédiées au franchissement d&apos;obstacles, représentés comme une hiérarchie de concepts SKOS.</rdfs:comment>
        <rdfs:label xml:lang="fr">Type de franchissement</rdfs:label>
        <rdfs:label xml:lang="en">Type of crossing</rdfs:label>
    </owl:NamedIndividual>
    


    <!-- http://data.ign.fr/id/codes/topo/typedelaisse/BassesMers -->


    <owl:NamedIndividual rdf:about="http://data.ign.fr/id/codes/topo/typedelaisse/BassesMers">
        <rdf:type rdf:resource="http://data.ign.fr/def/topo#TypeDeLaisse"/>
        <rdf:type rdf:resource="http://www.w3.org/2004/02/skos/core#Concept"/>
        <skos:definition xml:lang="fr">Limite inférieure de l&apos;estran. Elle sépare la zone littorale découvrante de la zone toujours envahie par la mer.</skos:definition>
        <skos:definition xml:lang="en">Lower limit of the foreshore. It separates the discovering littoral zone from the zone always invaded by the sea.</skos:definition>
        <skos:inScheme rdf:resource="http://data.ign.fr/id/codes/topo/typedelaisse/liste"/>
        <skos:prefLabel xml:lang="fr">laisse des plus basses mers</skos:prefLabel>
        <skos:prefLabel xml:lang="en">low-tide line</skos:prefLabel>
    </owl:NamedIndividual>
    


    <!-- http://data.ign.fr/id/codes/topo/typedelaisse/HautesMers -->


    <owl:NamedIndividual rdf:about="http://data.ign.fr/id/codes/topo/typedelaisse/HautesMers">
        <rdf:type rdf:resource="http://data.ign.fr/def/topo#TypeDeLaisse"/>
        <rdf:type rdf:resource="http://www.w3.org/2004/02/skos/core#Concept"/>
        <skos:definition xml:lang="fr">Limite supérieure de l&apos;estran. Elle sépare la zone littorale découvrante de la zone jamais envahie par la mer.</skos:definition>
        <skos:definition xml:lang="en">Upper limit of the foreshore. It separates the discovering littoral zone from the zone never invaded by the sea.</skos:definition>
        <skos:inScheme rdf:resource="http://data.ign.fr/id/codes/topo/typedelaisse/liste"/>
        <skos:prefLabel xml:lang="en">high-tide line</skos:prefLabel>
        <skos:prefLabel xml:lang="fr">laisse des plus hautes mers</skos:prefLabel>
    </owl:NamedIndividual>
    


    <!-- http://data.ign.fr/id/codes/topo/typedelaisse/liste -->


    <owl:NamedIndividual rdf:about="http://data.ign.fr/id/codes/topo/typedelaisse/liste">
        <rdf:type rdf:resource="http://www.w3.org/2004/02/skos/core#ConceptScheme"/>
        <rdfs:comment xml:lang="en">List of different types of leashes, represented as a hierarchy of SKOS concepts.</rdfs:comment>
        <rdfs:comment xml:lang="fr">Liste des différents types de laisses, représentés comme une hiérarchie de concepts SKOS.</rdfs:comment>
        <rdfs:label xml:lang="fr">Type de laisse</rdfs:label>
        <rdfs:label xml:lang="en">Type of tide line</rdfs:label>
    </owl:NamedIndividual>
    


    <!-- http://data.ign.fr/id/codes/topo/typedepointdeau/Citerne -->


    <owl:NamedIndividual rdf:about="http://data.ign.fr/id/codes/topo/typedepointdeau/Citerne">
        <rdf:type rdf:resource="http://data.ign.fr/def/topo#TypeDePointDEau"/>
        <rdf:type rdf:resource="http://www.w3.org/2004/02/skos/core#Concept"/>
        <skos:definition xml:lang="fr">Réservoir où l&apos;on recueille et conserve les eaux de pluie.</skos:definition>
        <skos:definition xml:lang="en">Tank where rainwater is collected and stored.</skos:definition>
        <skos:inScheme rdf:resource="http://data.ign.fr/id/codes/topo/typedepointdeau/liste"/>
        <skos:prefLabel xml:lang="en">cistern</skos:prefLabel>
        <skos:prefLabel xml:lang="fr">citerne</skos:prefLabel>
    </owl:NamedIndividual>
    


    <!-- http://data.ign.fr/id/codes/topo/typedepointdeau/Fontaine -->


    <owl:NamedIndividual rdf:about="http://data.ign.fr/id/codes/topo/typedepointdeau/Fontaine">
        <rdf:type rdf:resource="http://data.ign.fr/def/topo#TypeDePointDEau"/>
        <rdf:type rdf:resource="http://www.w3.org/2004/02/skos/core#Concept"/>
        <skos:definition xml:lang="fr">Construction comportant une alimentation en eau et généralement un bassin.</skos:definition>
        <skos:definition xml:lang="en">Construction comprising a water supply and generally a pond.</skos:definition>
        <skos:inScheme rdf:resource="http://data.ign.fr/id/codes/topo/typedepointdeau/liste"/>
        <skos:prefLabel xml:lang="fr">fontaine</skos:prefLabel>
        <skos:prefLabel xml:lang="en">fountain</skos:prefLabel>
    </owl:NamedIndividual>
    


    <!-- http://data.ign.fr/id/codes/topo/typedepointdeau/Source -->


    <owl:NamedIndividual rdf:about="http://data.ign.fr/id/codes/topo/typedepointdeau/Source">
        <rdf:type rdf:resource="http://data.ign.fr/def/topo#TypeDePointDEau"/>
        <rdf:type rdf:resource="http://www.w3.org/2004/02/skos/core#Concept"/>
        <skos:definition xml:lang="fr">Point d&apos;émergence à la surface du sol de l&apos;eau emmagasinée à l&apos;intérieur. Exsurgence, résurgence, source.</skos:definition>
        <skos:definition xml:lang="en">Point of emergence on the soil surface of the water stored inside. Exsurgence, resurgence, source.</skos:definition>
        <skos:inScheme rdf:resource="http://data.ign.fr/id/codes/topo/typedepointdeau/liste"/>
        <skos:prefLabel xml:lang="fr">source</skos:prefLabel>
        <skos:prefLabel xml:lang="en">spring</skos:prefLabel>
    </owl:NamedIndividual>
    


    <!-- http://data.ign.fr/id/codes/topo/typedepointdeau/SourceCaptee -->


    <owl:NamedIndividual rdf:about="http://data.ign.fr/id/codes/topo/typedepointdeau/SourceCaptee">
        <rdf:type rdf:resource="http://data.ign.fr/def/topo#TypeDePointDEau"/>
        <rdf:type rdf:resource="http://www.w3.org/2004/02/skos/core#Concept"/>
        <skos:definition xml:lang="en">Collection installation of a source.</skos:definition>
        <skos:definition xml:lang="fr">Installation de captage d’une source.</skos:definition>
        <skos:inScheme rdf:resource="http://data.ign.fr/id/codes/topo/typedepointdeau/liste"/>
        <skos:prefLabel xml:lang="fr">source captée</skos:prefLabel>
        <skos:prefLabel xml:lang="en">water catchment</skos:prefLabel>
    </owl:NamedIndividual>
    


    <!-- http://data.ign.fr/id/codes/topo/typedepointdeau/StationDePompage -->


    <owl:NamedIndividual rdf:about="http://data.ign.fr/id/codes/topo/typedepointdeau/StationDePompage">
        <rdf:type rdf:resource="http://data.ign.fr/def/topo#TypeDePointDEau"/>
        <rdf:type rdf:resource="http://data.ign.fr/def/topo#TypeDeZAI"/>
        <rdf:type rdf:resource="http://www.w3.org/2004/02/skos/core#Concept"/>
        <skos:broader rdf:resource="http://data.ign.fr/id/codes/topo/typedezai/PAIGestionEaux"/>
        <skos:definition xml:lang="fr">Installation comprenant une pompe destinée à pomper l&apos;eau du sous-sol, d&apos;une rivière, ou à monter de l&apos;eau dans un réservoir ou un château d&apos;eau.</skos:definition>
        <skos:definition xml:lang="en">Installation comprising a pump for pumping water from the basement, a river, or to raise water in a tank or a water tower.</skos:definition>
        <skos:inScheme rdf:resource="http://data.ign.fr/id/codes/topo/typedepointdeau/liste"/>
        <skos:inScheme rdf:resource="http://data.ign.fr/id/codes/topo/typedezai/liste"/>
        <skos:prefLabel xml:lang="en">pumping station</skos:prefLabel>
        <skos:prefLabel xml:lang="fr">station de pompage</skos:prefLabel>
    </owl:NamedIndividual>
    


    <!-- http://data.ign.fr/id/codes/topo/typedepointdeau/liste -->


    <owl:NamedIndividual rdf:about="http://data.ign.fr/id/codes/topo/typedepointdeau/liste">
        <rdf:type rdf:resource="http://www.w3.org/2004/02/skos/core#ConceptScheme"/>
        <rdfs:comment xml:lang="en">List of different types of water points, represented as a hierarchy of SKOS concepts.</rdfs:comment>
        <rdfs:comment xml:lang="fr">Liste des différents types de points d&apos;eau, représentés comme une hiérarchie de concepts SKOS.</rdfs:comment>
        <rdfs:label xml:lang="fr">Type de point d&apos;eau</rdfs:label>
        <rdfs:label xml:lang="en">Type of waterhole</rdfs:label>
    </owl:NamedIndividual>
    


    <!-- http://data.ign.fr/id/codes/topo/typederelief/Cap -->


    <owl:NamedIndividual rdf:about="http://data.ign.fr/id/codes/topo/typederelief/Cap">
        <rdf:type rdf:resource="http://data.ign.fr/def/topo#TypeDeRelief"/>
        <rdf:type rdf:resource="http://www.w3.org/2004/02/skos/core#Concept"/>
        <skos:broader rdf:resource="http://data.ign.fr/id/codes/topo/typedezai/PAIOrographie"/>
        <skos:definition xml:lang="en">Predominance in the outline of a coast: cape, point, promontory.</skos:definition>
        <skos:definition xml:lang="fr">Prédominance dans le contour d&apos;une côte : cap, pointe, promontoire.</skos:definition>
        <skos:inScheme rdf:resource="http://data.ign.fr/id/codes/topo/typederelief/liste"/>
        <skos:inScheme rdf:resource="http://data.ign.fr/id/codes/topo/typedezai/liste"/>
        <skos:prefLabel xml:lang="fr">cap</skos:prefLabel>
        <skos:prefLabel xml:lang="en">cape</skos:prefLabel>
    </owl:NamedIndividual>
    


    <!-- http://data.ign.fr/id/codes/topo/typederelief/Carriere -->


    <owl:NamedIndividual rdf:about="http://data.ign.fr/id/codes/topo/typederelief/Carriere">
        <rdf:type rdf:resource="http://data.ign.fr/def/topo#TypeDeRelief"/>
        <rdf:type rdf:resource="http://www.w3.org/2004/02/skos/core#Concept"/>
        <skos:broader rdf:resource="http://data.ign.fr/id/codes/topo/typedezai/PAIIndustrielCommercial"/>
        <skos:definition xml:lang="fr">Lieu d&apos;où l&apos;on extrait à ciel ouvert des matériaux de construction (pierre, roche) : carrière, sablière, ballastière, gravière. Grand talus marquant le front et la structure principale d’une carrière : gravière (talus), mine à ciel ouvert (talus), talus de carrière.</skos:definition>
        <skos:definition xml:lang="en">Place from where we extract construction materials (stone, rock): quarry, sandpit, ballast tank, gravel pit. Large embankment marking the front and main structure of a quarry: gravel pit (embankment), open pit mine (slope), quarry slope.</skos:definition>
        <skos:inScheme rdf:resource="http://data.ign.fr/id/codes/topo/typederelief/liste"/>
        <skos:inScheme rdf:resource="http://data.ign.fr/id/codes/topo/typedezai/liste"/>
        <skos:prefLabel xml:lang="fr">carrière</skos:prefLabel>
        <skos:prefLabel xml:lang="en">quarry</skos:prefLabel>
    </owl:NamedIndividual>
    


    <!-- http://data.ign.fr/id/codes/topo/typederelief/Cirque -->


    <owl:NamedIndividual rdf:about="http://data.ign.fr/id/codes/topo/typederelief/Cirque">
        <rdf:type rdf:resource="http://data.ign.fr/def/topo#TypeDeRelief"/>
        <rdf:type rdf:resource="http://www.w3.org/2004/02/skos/core#Concept"/>
        <skos:broader rdf:resource="http://data.ign.fr/id/codes/topo/typedezai/PAIOrographie"/>
        <skos:definition xml:lang="fr">Dépression semi-circulaire, à bords raides.</skos:definition>
        <skos:definition xml:lang="en">Semi-circular depression, with steep edges.</skos:definition>
        <skos:inScheme rdf:resource="http://data.ign.fr/id/codes/topo/typederelief/liste"/>
        <skos:inScheme rdf:resource="http://data.ign.fr/id/codes/topo/typedezai/liste"/>
        <skos:prefLabel xml:lang="en">cirque</skos:prefLabel>
        <skos:prefLabel xml:lang="fr">cirque</skos:prefLabel>
    </owl:NamedIndividual>
    


    <!-- http://data.ign.fr/id/codes/topo/typederelief/Col -->


    <owl:NamedIndividual rdf:about="http://data.ign.fr/id/codes/topo/typederelief/Col">
        <rdf:type rdf:resource="http://data.ign.fr/def/topo#TypeDeRelief"/>
        <rdf:type rdf:resource="http://www.w3.org/2004/02/skos/core#Concept"/>
        <skos:broader rdf:resource="http://data.ign.fr/id/codes/topo/typedezai/PAIOrographie"/>
        <skos:definition xml:lang="fr">Point de passage imposé par la configuration du relief : col, passage.</skos:definition>
        <skos:definition xml:lang="en">Point of passage imposed by the relief configuration: pass, passage.</skos:definition>
        <skos:inScheme rdf:resource="http://data.ign.fr/id/codes/topo/typederelief/liste"/>
        <skos:inScheme rdf:resource="http://data.ign.fr/id/codes/topo/typedezai/liste"/>
        <skos:prefLabel xml:lang="fr">col</skos:prefLabel>
        <skos:prefLabel xml:lang="en">mountain pass</skos:prefLabel>
    </owl:NamedIndividual>
    


    <!-- http://data.ign.fr/id/codes/topo/typederelief/Crete -->


    <owl:NamedIndividual rdf:about="http://data.ign.fr/id/codes/topo/typederelief/Crete">
        <rdf:type rdf:resource="http://data.ign.fr/def/topo#TypeDeRelief"/>
        <rdf:type rdf:resource="http://www.w3.org/2004/02/skos/core#Concept"/>
        <skos:broader rdf:resource="http://data.ign.fr/id/codes/topo/typedezai/PAIOrographie"/>
        <skos:definition xml:lang="fr">Ligne de partage des eaux : crête, arête, ligne de faîte.</skos:definition>
        <skos:definition xml:lang="en">Watershed: crest, ridge, ridge line.</skos:definition>
        <skos:inScheme rdf:resource="http://data.ign.fr/id/codes/topo/typederelief/liste"/>
        <skos:inScheme rdf:resource="http://data.ign.fr/id/codes/topo/typedezai/liste"/>
        <skos:prefLabel xml:lang="en">crest</skos:prefLabel>
        <skos:prefLabel xml:lang="fr">crête</skos:prefLabel>
    </owl:NamedIndividual>
    


    <!-- http://data.ign.fr/id/codes/topo/typederelief/Depression -->


    <owl:NamedIndividual rdf:about="http://data.ign.fr/id/codes/topo/typederelief/Depression">
        <rdf:type rdf:resource="http://data.ign.fr/def/topo#TypeDeRelief"/>
        <rdf:type rdf:resource="http://www.w3.org/2004/02/skos/core#Concept"/>
        <skos:broader rdf:resource="http://data.ign.fr/id/codes/topo/typedezai/PAIOrographie"/>
        <skos:definition xml:lang="fr">Dépression naturelle du sol : cuvette, bassin fermé, dépression, doline.</skos:definition>
        <skos:definition xml:lang="en">Natural soil depression: basin, closed basin, depression, sinkhole.</skos:definition>
        <skos:inScheme rdf:resource="http://data.ign.fr/id/codes/topo/typederelief/liste"/>
        <skos:inScheme rdf:resource="http://data.ign.fr/id/codes/topo/typedezai/liste"/>
        <skos:prefLabel xml:lang="en">depression</skos:prefLabel>
        <skos:prefLabel xml:lang="fr">dépression</skos:prefLabel>
    </owl:NamedIndividual>
    


    <!-- http://data.ign.fr/id/codes/topo/typederelief/Dune -->


    <owl:NamedIndividual rdf:about="http://data.ign.fr/id/codes/topo/typederelief/Dune">
        <rdf:type rdf:resource="http://data.ign.fr/def/topo#TypeDeRelief"/>
        <rdf:type rdf:resource="http://www.w3.org/2004/02/skos/core#Concept"/>
        <skos:broader rdf:resource="http://data.ign.fr/id/codes/topo/typedezai/PAIOrographie"/>
        <skos:definition xml:lang="fr">Monticule de sable sur les bords de la mer.</skos:definition>
        <skos:definition xml:lang="en">Sand mound on the shores of the sea.</skos:definition>
        <skos:inScheme rdf:resource="http://data.ign.fr/id/codes/topo/typederelief/liste"/>
        <skos:inScheme rdf:resource="http://data.ign.fr/id/codes/topo/typedezai/liste"/>
        <skos:prefLabel xml:lang="en">dune</skos:prefLabel>
        <skos:prefLabel xml:lang="fr">dune</skos:prefLabel>
    </owl:NamedIndividual>
    


    <!-- http://data.ign.fr/id/codes/topo/typederelief/Escarpement -->


    <owl:NamedIndividual rdf:about="http://data.ign.fr/id/codes/topo/typederelief/Escarpement">
        <rdf:type rdf:resource="http://data.ign.fr/def/topo#TypeDeRelief"/>
        <rdf:type rdf:resource="http://www.w3.org/2004/02/skos/core#Concept"/>
        <skos:broader rdf:resource="http://data.ign.fr/id/codes/topo/typedezai/PAIOrographie"/>
        <skos:definition xml:lang="fr">Escarpement du relief : barre rocheuse, escarpement rocheux, face abrupte, falaise.</skos:definition>
        <skos:definition xml:lang="en">Relief of the relief: rocky ledge, rocky escarpment, abrupt face, cliff.</skos:definition>
        <skos:inScheme rdf:resource="http://data.ign.fr/id/codes/topo/typederelief/liste"/>
        <skos:inScheme rdf:resource="http://data.ign.fr/id/codes/topo/typedezai/liste"/>
        <skos:prefLabel xml:lang="fr">escarpement</skos:prefLabel>
        <skos:prefLabel xml:lang="en">escarpment</skos:prefLabel>
    </owl:NamedIndividual>
    


    <!-- http://data.ign.fr/id/codes/topo/typederelief/Gorge -->


    <owl:NamedIndividual rdf:about="http://data.ign.fr/id/codes/topo/typederelief/Gorge">
        <rdf:type rdf:resource="http://data.ign.fr/def/topo#TypeDeRelief"/>
        <rdf:type rdf:resource="http://www.w3.org/2004/02/skos/core#Concept"/>
        <skos:broader rdf:resource="http://data.ign.fr/id/codes/topo/typedezai/PAIOrographie"/>
        <skos:definition xml:lang="en">Valley narrow and concealed: canyon, cluse, parade, gorge.</skos:definition>
        <skos:definition xml:lang="fr">Vallée étroite et encaissée : canyon, cluse, défilé, gorge.</skos:definition>
        <skos:inScheme rdf:resource="http://data.ign.fr/id/codes/topo/typederelief/liste"/>
        <skos:inScheme rdf:resource="http://data.ign.fr/id/codes/topo/typedezai/liste"/>
        <skos:prefLabel xml:lang="en">gorge</skos:prefLabel>
        <skos:prefLabel xml:lang="fr">gorge</skos:prefLabel>
    </owl:NamedIndividual>
    


    <!-- http://data.ign.fr/id/codes/topo/typederelief/Grotte -->


    <owl:NamedIndividual rdf:about="http://data.ign.fr/id/codes/topo/typederelief/Grotte">
        <rdf:type rdf:resource="http://data.ign.fr/def/topo#TypeDeRelief"/>
        <rdf:type rdf:resource="http://www.w3.org/2004/02/skos/core#Concept"/>
        <skos:broader rdf:resource="http://data.ign.fr/id/codes/topo/typedezai/PAIOrographie"/>
        <skos:definition xml:lang="fr">Grotte naturelle ou excavation : aven, cave, gouffre, grotte.</skos:definition>
        <skos:definition xml:lang="en">Natural cave or excavation: aven, gulf, cave.</skos:definition>
        <skos:inScheme rdf:resource="http://data.ign.fr/id/codes/topo/typederelief/liste"/>
        <skos:inScheme rdf:resource="http://data.ign.fr/id/codes/topo/typedezai/liste"/>
        <skos:prefLabel xml:lang="en">cave</skos:prefLabel>
        <skos:prefLabel xml:lang="fr">grotte</skos:prefLabel>
    </owl:NamedIndividual>
    


    <!-- http://data.ign.fr/id/codes/topo/typederelief/Ile -->


    <owl:NamedIndividual rdf:about="http://data.ign.fr/id/codes/topo/typederelief/Ile">
        <rdf:type rdf:resource="http://data.ign.fr/def/topo#TypeDeRelief"/>
        <rdf:type rdf:resource="http://www.w3.org/2004/02/skos/core#Concept"/>
        <skos:broader rdf:resource="http://data.ign.fr/id/codes/topo/typedezai/PAIOrographie"/>
        <skos:definition xml:lang="en">Island or peninsula.</skos:definition>
        <skos:definition xml:lang="fr">Île, îlot ou presqu&apos;île.</skos:definition>
        <skos:inScheme rdf:resource="http://data.ign.fr/id/codes/topo/typederelief/liste"/>
        <skos:inScheme rdf:resource="http://data.ign.fr/id/codes/topo/typedezai/liste"/>
        <skos:prefLabel xml:lang="en">island</skos:prefLabel>
        <skos:prefLabel xml:lang="fr">île</skos:prefLabel>
    </owl:NamedIndividual>
    


    <!-- http://data.ign.fr/id/codes/topo/typederelief/Isthme -->


    <owl:NamedIndividual rdf:about="http://data.ign.fr/id/codes/topo/typederelief/Isthme">
        <rdf:type rdf:resource="http://data.ign.fr/def/topo#TypeDeRelief"/>
        <rdf:type rdf:resource="http://www.w3.org/2004/02/skos/core#Concept"/>
        <skos:broader rdf:resource="http://data.ign.fr/id/codes/topo/typedezai/PAIOrographie"/>
        <skos:definition xml:lang="en">A narrow strip of land between two seas, uniting two lands: coastal cord, isthmus.</skos:definition>
        <skos:definition xml:lang="fr">Bande de terre étroite entre deux mers, réunissant deux terres : cordon littoral, isthme.</skos:definition>
        <skos:inScheme rdf:resource="http://data.ign.fr/id/codes/topo/typederelief/liste"/>
        <skos:inScheme rdf:resource="http://data.ign.fr/id/codes/topo/typedezai/liste"/>
        <skos:prefLabel xml:lang="fr">isthme</skos:prefLabel>
        <skos:prefLabel xml:lang="en">isthmus</skos:prefLabel>
    </owl:NamedIndividual>
    


    <!-- http://data.ign.fr/id/codes/topo/typederelief/Levee -->


    <owl:NamedIndividual rdf:about="http://data.ign.fr/id/codes/topo/typederelief/Levee">
        <rdf:type rdf:resource="http://data.ign.fr/def/topo#TypeDeRelief"/>
        <rdf:type rdf:resource="http://www.w3.org/2004/02/skos/core#Concept"/>
        <skos:definition xml:lang="fr">Digue en terre (levée de terre) ou en maçonnerie de faible largeur : crassier, levée de terre, digue en terre, remblai, terril.</skos:definition>
        <skos:definition xml:lang="en">Dike in earth (raised earth) or in masonry of small width: slag, raised earth, earth dam, embankment, heap.</skos:definition>
        <skos:inScheme rdf:resource="http://data.ign.fr/id/codes/topo/typederelief/liste"/>
        <skos:prefLabel xml:lang="en">levee</skos:prefLabel>
        <skos:prefLabel xml:lang="fr">levée</skos:prefLabel>
    </owl:NamedIndividual>
    


    <!-- http://data.ign.fr/id/codes/topo/typederelief/Montagne -->


    <owl:NamedIndividual rdf:about="http://data.ign.fr/id/codes/topo/typederelief/Montagne">
        <rdf:type rdf:resource="http://data.ign.fr/def/topo#TypeDeRelief"/>
        <rdf:type rdf:resource="http://www.w3.org/2004/02/skos/core#Concept"/>
        <skos:broader rdf:resource="http://data.ign.fr/id/codes/topo/typedezai/PAIOrographie"/>
        <skos:definition xml:lang="en">Designates a mountain or a massif in a global way and not a particular summit (see summit).</skos:definition>
        <skos:definition xml:lang="fr">Désigne une montagne ou un massif de manière globale et non un sommet en particulier (voir sommet).</skos:definition>
        <skos:inScheme rdf:resource="http://data.ign.fr/id/codes/topo/typederelief/liste"/>
        <skos:inScheme rdf:resource="http://data.ign.fr/id/codes/topo/typedezai/liste"/>
        <skos:prefLabel xml:lang="fr">montagne</skos:prefLabel>
        <skos:prefLabel xml:lang="en">mountain</skos:prefLabel>
    </owl:NamedIndividual>
    


    <!-- http://data.ign.fr/id/codes/topo/typederelief/MurDeSoutenement -->


    <owl:NamedIndividual rdf:about="http://data.ign.fr/id/codes/topo/typederelief/MurDeSoutenement">
        <rdf:type rdf:resource="http://data.ign.fr/def/topo#TypeDeRelief"/>
        <rdf:type rdf:resource="http://www.w3.org/2004/02/skos/core#Concept"/>
        <skos:definition xml:lang="fr">Mur épaulant un remblai, une terrasse.</skos:definition>
        <skos:definition xml:lang="en">Wall supporting an embankment, a terrace.</skos:definition>
        <skos:inScheme rdf:resource="http://data.ign.fr/id/codes/topo/typederelief/liste"/>
        <skos:prefLabel xml:lang="fr">mur de soutènement</skos:prefLabel>
        <skos:prefLabel xml:lang="en">retaining wall</skos:prefLabel>
    </owl:NamedIndividual>
    


    <!-- http://data.ign.fr/id/codes/topo/typederelief/Pic -->


    <owl:NamedIndividual rdf:about="http://data.ign.fr/id/codes/topo/typederelief/Pic">
        <rdf:type rdf:resource="http://data.ign.fr/def/topo#TypeDeRelief"/>
        <rdf:type rdf:resource="http://www.w3.org/2004/02/skos/core#Concept"/>
        <skos:broader rdf:resource="http://data.ign.fr/id/codes/topo/typedezai/PAIOrographie"/>
        <skos:definition xml:lang="en">Sharp summit of a mountain: needle, peak.</skos:definition>
        <skos:definition xml:lang="fr">Sommet pointu d&apos;une montagne : aiguille, pic, piton.</skos:definition>
        <skos:inScheme rdf:resource="http://data.ign.fr/id/codes/topo/typederelief/liste"/>
        <skos:inScheme rdf:resource="http://data.ign.fr/id/codes/topo/typedezai/liste"/>
        <skos:prefLabel xml:lang="en">peak</skos:prefLabel>
        <skos:prefLabel xml:lang="fr">pic</skos:prefLabel>
    </owl:NamedIndividual>
    


    <!-- http://data.ign.fr/id/codes/topo/typederelief/Plage -->


    <owl:NamedIndividual rdf:about="http://data.ign.fr/id/codes/topo/typederelief/Plage">
        <rdf:type rdf:resource="http://data.ign.fr/def/topo#TypeDeRelief"/>
        <rdf:type rdf:resource="http://www.w3.org/2004/02/skos/core#Concept"/>
        <skos:broader rdf:resource="http://data.ign.fr/id/codes/topo/typedezai/PAIOrographie"/>
        <skos:definition xml:lang="en">Coastal zone marked by the ebb and flow of the tides: beach.</skos:definition>
        <skos:definition xml:lang="fr">Zone littorale marquée par le flux et le reflux des marées : grève, plage.</skos:definition>
        <skos:inScheme rdf:resource="http://data.ign.fr/id/codes/topo/typederelief/liste"/>
        <skos:inScheme rdf:resource="http://data.ign.fr/id/codes/topo/typedezai/liste"/>
        <skos:prefLabel xml:lang="en">beach</skos:prefLabel>
        <skos:prefLabel xml:lang="fr">plage</skos:prefLabel>
    </owl:NamedIndividual>
    


    <!-- http://data.ign.fr/id/codes/topo/typederelief/Plaine -->


    <owl:NamedIndividual rdf:about="http://data.ign.fr/id/codes/topo/typederelief/Plaine">
        <rdf:type rdf:resource="http://data.ign.fr/def/topo#TypeDeRelief"/>
        <rdf:type rdf:resource="http://www.w3.org/2004/02/skos/core#Concept"/>
        <skos:broader rdf:resource="http://data.ign.fr/id/codes/topo/typedezai/PAIOrographie"/>
        <skos:definition xml:lang="en">Land surface area characterized by relative flatness: plain, plateau.</skos:definition>
        <skos:definition xml:lang="fr">Zone de surface terrestre caractérisée par une relative planéité : plaine, plateau.</skos:definition>
        <skos:inScheme rdf:resource="http://data.ign.fr/id/codes/topo/typederelief/liste"/>
        <skos:inScheme rdf:resource="http://data.ign.fr/id/codes/topo/typedezai/liste"/>
        <skos:prefLabel xml:lang="en">plain</skos:prefLabel>
        <skos:prefLabel xml:lang="fr">plaine</skos:prefLabel>
    </owl:NamedIndividual>
    


    <!-- http://data.ign.fr/id/codes/topo/typederelief/Recif -->


    <owl:NamedIndividual rdf:about="http://data.ign.fr/id/codes/topo/typederelief/Recif">
        <rdf:type rdf:resource="http://data.ign.fr/def/topo#TypeDeRelief"/>
        <rdf:type rdf:resource="http://www.w3.org/2004/02/skos/core#Concept"/>
        <skos:broader rdf:resource="http://data.ign.fr/id/codes/topo/typedezai/PAIOrographie"/>
        <skos:definition xml:lang="fr">Rocher situé en mer ou dans un fleuve, mais dont une partie, faiblement émergée, peut constituer un obstacle ou un repère : brisant, récif, rocher marin.</skos:definition>
        <skos:definition xml:lang="en">Rock located in the sea or in a river, but part of which, slightly emerged, can constitute an obstacle or a landmark: breaking, reef, marine rock.</skos:definition>
        <skos:inScheme rdf:resource="http://data.ign.fr/id/codes/topo/typederelief/liste"/>
        <skos:inScheme rdf:resource="http://data.ign.fr/id/codes/topo/typedezai/liste"/>
        <skos:prefLabel xml:lang="en">reef</skos:prefLabel>
        <skos:prefLabel xml:lang="fr">récif</skos:prefLabel>
    </owl:NamedIndividual>
    


    <!-- http://data.ign.fr/id/codes/topo/typederelief/Rochers -->


    <owl:NamedIndividual rdf:about="http://data.ign.fr/id/codes/topo/typederelief/Rochers">
        <rdf:type rdf:resource="http://data.ign.fr/def/topo#TypeDeRelief"/>
        <rdf:type rdf:resource="http://www.w3.org/2004/02/skos/core#Concept"/>
        <skos:broader rdf:resource="http://data.ign.fr/id/codes/topo/typedezai/PAIOrographie"/>
        <skos:definition xml:lang="en">Zone or detail characterized by a rocky but not vertical nature: chaos, scree, rock.</skos:definition>
        <skos:definition xml:lang="fr">Zone ou détail caractérisé par une nature rocheuse mais non verticale : chaos, éboulis, pierrier, rocher.</skos:definition>
        <skos:inScheme rdf:resource="http://data.ign.fr/id/codes/topo/typederelief/liste"/>
        <skos:inScheme rdf:resource="http://data.ign.fr/id/codes/topo/typedezai/liste"/>
        <skos:prefLabel xml:lang="fr">rochers</skos:prefLabel>
        <skos:prefLabel xml:lang="en">rocks</skos:prefLabel>
    </owl:NamedIndividual>
    


    <!-- http://data.ign.fr/id/codes/topo/typederelief/Sommet -->


    <owl:NamedIndividual rdf:about="http://data.ign.fr/id/codes/topo/typederelief/Sommet">
        <rdf:type rdf:resource="http://data.ign.fr/def/topo#TypeDeRelief"/>
        <rdf:type rdf:resource="http://www.w3.org/2004/02/skos/core#Concept"/>
        <skos:broader rdf:resource="http://data.ign.fr/id/codes/topo/typedezai/PAIOrographie"/>
        <skos:definition xml:lang="en">High point of the relief not characterized by an abrupt profile (see the nature Pic): hill, nipple, mount, summit.</skos:definition>
        <skos:definition xml:lang="fr">Point haut du relief non caractérisé par un profil abrupt (voir la nature Pic) : colline, mamelon, mont, sommet.</skos:definition>
        <skos:inScheme rdf:resource="http://data.ign.fr/id/codes/topo/typederelief/liste"/>
        <skos:inScheme rdf:resource="http://data.ign.fr/id/codes/topo/typedezai/liste"/>
        <skos:prefLabel xml:lang="fr">sommet</skos:prefLabel>
        <skos:prefLabel xml:lang="en">summit</skos:prefLabel>
    </owl:NamedIndividual>
    


    <!-- http://data.ign.fr/id/codes/topo/typederelief/Talus -->


    <owl:NamedIndividual rdf:about="http://data.ign.fr/id/codes/topo/typederelief/Talus">
        <rdf:type rdf:resource="http://data.ign.fr/def/topo#TypeDeRelief"/>
        <rdf:type rdf:resource="http://www.w3.org/2004/02/skos/core#Concept"/>
        <skos:definition xml:lang="fr">Ligne de rupture de pente : crassier, déblai, remblai, talus.</skos:definition>
        <skos:definition xml:lang="en">Slope breaking line: slag, excavation, embankment, embankment.</skos:definition>
        <skos:inScheme rdf:resource="http://data.ign.fr/id/codes/topo/typederelief/liste"/>
        <skos:prefLabel xml:lang="en">slope</skos:prefLabel>
        <skos:prefLabel xml:lang="fr">talus</skos:prefLabel>
    </owl:NamedIndividual>
    


    <!-- http://data.ign.fr/id/codes/topo/typederelief/Vallee -->


    <owl:NamedIndividual rdf:about="http://data.ign.fr/id/codes/topo/typederelief/Vallee">
        <rdf:type rdf:resource="http://data.ign.fr/def/topo#TypeDeRelief"/>
        <rdf:type rdf:resource="http://www.w3.org/2004/02/skos/core#Concept"/>
        <skos:broader rdf:resource="http://data.ign.fr/id/codes/topo/typedezai/PAIOrographie"/>
        <skos:definition xml:lang="fr">Espace entre deux ou plusieurs montagnes. Forme définie par la convergence des versants et qui est, ou a été parcourue par un cours d&apos;eau : combe, ravin, val, vallée, vallon, thalweg.</skos:definition>
        <skos:definition xml:lang="en">Space between two or more mountains. Form defined by the convergence of slopes and which is, or has been traversed by a river: combe, ravine, val, valley, thalweg.</skos:definition>
        <skos:inScheme rdf:resource="http://data.ign.fr/id/codes/topo/typederelief/liste"/>
        <skos:inScheme rdf:resource="http://data.ign.fr/id/codes/topo/typedezai/liste"/>
        <skos:prefLabel xml:lang="en">valley</skos:prefLabel>
        <skos:prefLabel xml:lang="fr">vallée</skos:prefLabel>
    </owl:NamedIndividual>
    


    <!-- http://data.ign.fr/id/codes/topo/typederelief/Versant -->


    <owl:NamedIndividual rdf:about="http://data.ign.fr/id/codes/topo/typederelief/Versant">
        <rdf:type rdf:resource="http://data.ign.fr/def/topo#TypeDeRelief"/>
        <rdf:type rdf:resource="http://www.w3.org/2004/02/skos/core#Concept"/>
        <skos:broader rdf:resource="http://data.ign.fr/id/codes/topo/typedezai/PAIOrographie"/>
        <skos:definition xml:lang="en">Inclined plane joining a ridge line to a thalweg: hillside, slope.</skos:definition>
        <skos:definition xml:lang="fr">Plan incliné joignant une ligne de crête à un thalweg : coteau, versant.</skos:definition>
        <skos:inScheme rdf:resource="http://data.ign.fr/id/codes/topo/typederelief/liste"/>
        <skos:inScheme rdf:resource="http://data.ign.fr/id/codes/topo/typedezai/liste"/>
        <skos:prefLabel xml:lang="en">slope</skos:prefLabel>
        <skos:prefLabel xml:lang="fr">versant</skos:prefLabel>
    </owl:NamedIndividual>
    


    <!-- http://data.ign.fr/id/codes/topo/typederelief/Volcan -->


    <owl:NamedIndividual rdf:about="http://data.ign.fr/id/codes/topo/typederelief/Volcan">
        <rdf:type rdf:resource="http://data.ign.fr/def/topo#TypeDeRelief"/>
        <rdf:type rdf:resource="http://www.w3.org/2004/02/skos/core#Concept"/>
        <skos:broader rdf:resource="http://data.ign.fr/id/codes/topo/typedezai/PAIOrographie"/>
        <skos:definition xml:lang="en">Any form of relief testifying to volcanic activity: crater, volcano.</skos:definition>
        <skos:definition xml:lang="fr">Toute forme de relief témoignant d&apos;une activité volcanique : cratère, volcan.</skos:definition>
        <skos:inScheme rdf:resource="http://data.ign.fr/id/codes/topo/typederelief/liste"/>
        <skos:inScheme rdf:resource="http://data.ign.fr/id/codes/topo/typedezai/liste"/>
        <skos:prefLabel xml:lang="fr">volcan</skos:prefLabel>
        <skos:prefLabel xml:lang="en">volcano</skos:prefLabel>
    </owl:NamedIndividual>
    


    <!-- http://data.ign.fr/id/codes/topo/typederelief/liste -->


    <owl:NamedIndividual rdf:about="http://data.ign.fr/id/codes/topo/typederelief/liste">
        <rdf:type rdf:resource="http://www.w3.org/2004/02/skos/core#ConceptScheme"/>
        <rdfs:comment xml:lang="en">List of different types of terrain elements, represented as a hierarchy of SKOS concepts.</rdfs:comment>
        <rdfs:comment xml:lang="fr">Liste des différents types d&apos;éléments du relief, représentés comme une hiérarchie de concepts SKOS.</rdfs:comment>
        <rdfs:label xml:lang="fr">Type d&apos;élément du relief</rdfs:label>
        <rdfs:label xml:lang="en">Type of relief feature</rdfs:label>
    </owl:NamedIndividual>
    


    <!-- http://data.ign.fr/id/codes/topo/typedereservoir/ChateauDEau -->


    <owl:NamedIndividual rdf:about="http://data.ign.fr/id/codes/topo/typedereservoir/ChateauDEau">
        <rdf:type rdf:resource="http://data.ign.fr/def/topo#TypeDeReservoir"/>
        <rdf:type rdf:resource="http://www.w3.org/2004/02/skos/core#Concept"/>
        <skos:definition xml:lang="fr">Réservoir d’eau construit en hauteur pour surélever le niveau de l’eau par rapport aux constructions.</skos:definition>
        <skos:definition xml:lang="en">Water tank built in height to raise the level of water compared to buildings.</skos:definition>
        <skos:inScheme rdf:resource="http://data.ign.fr/id/codes/topo/typedereservoir/liste"/>
        <skos:prefLabel xml:lang="fr">château d&apos;eau</skos:prefLabel>
        <skos:prefLabel xml:lang="en">water tower</skos:prefLabel>
    </owl:NamedIndividual>
    


    <!-- http://data.ign.fr/id/codes/topo/typedereservoir/ReservoirDEau -->


    <owl:NamedIndividual rdf:about="http://data.ign.fr/id/codes/topo/typedereservoir/ReservoirDEau">
        <rdf:type rdf:resource="http://data.ign.fr/def/topo#TypeDeReservoir"/>
        <rdf:type rdf:resource="http://www.w3.org/2004/02/skos/core#Concept"/>
        <skos:definition xml:lang="fr">Réservoirs d’eau et châteaux d’eau au sol dans lesquels la réserve d’eau est située au niveau du sol.</skos:definition>
        <skos:definition xml:lang="en">Water tanks and ground water towers in which the water supply is located at ground level.</skos:definition>
        <skos:inScheme rdf:resource="http://data.ign.fr/id/codes/topo/typedereservoir/liste"/>
        <skos:prefLabel xml:lang="fr">réservoir d&apos;eau</skos:prefLabel>
        <skos:prefLabel xml:lang="en">water-tank</skos:prefLabel>
    </owl:NamedIndividual>
    


    <!-- http://data.ign.fr/id/codes/topo/typedereservoir/ReservoirIndustriel -->


    <owl:NamedIndividual rdf:about="http://data.ign.fr/id/codes/topo/typedereservoir/ReservoirIndustriel">
        <rdf:type rdf:resource="http://data.ign.fr/def/topo#TypeDeReservoir"/>
        <rdf:type rdf:resource="http://www.w3.org/2004/02/skos/core#Concept"/>
        <skos:definition xml:lang="en">Industrial raw material tank: gasometer, hydrocarbon tank, building material tank, industrial tank.</skos:definition>
        <skos:definition xml:lang="fr">Réservoir de matière première industrielle : gazomètre, réservoir d’hydrocarbure, réservoir de matériaux de construction, réservoir industriel.</skos:definition>
        <skos:inScheme rdf:resource="http://data.ign.fr/id/codes/topo/typedereservoir/liste"/>
        <skos:prefLabel xml:lang="fr">réservoir industriel</skos:prefLabel>
        <skos:prefLabel xml:lang="en">tank</skos:prefLabel>
    </owl:NamedIndividual>
    


    <!-- http://data.ign.fr/id/codes/topo/typedereservoir/liste -->


    <owl:NamedIndividual rdf:about="http://data.ign.fr/id/codes/topo/typedereservoir/liste">
        <rdf:type rdf:resource="http://www.w3.org/2004/02/skos/core#ConceptScheme"/>
        <rdfs:comment xml:lang="en">List of different types of tanks, represented as a hierarchy of SKOS concepts.</rdfs:comment>
        <rdfs:comment xml:lang="fr">Liste des différents types de réservoirs, représentés comme une hiérarchie de concepts SKOS.</rdfs:comment>
        <rdfs:label xml:lang="fr">Type de réservoirs</rdfs:label>
        <rdfs:label xml:lang="en">Type of tank</rdfs:label>
    </owl:NamedIndividual>
    


    <!-- http://data.ign.fr/id/codes/topo/typederoute/Autoroute -->


    <owl:NamedIndividual rdf:about="http://data.ign.fr/id/codes/topo/typederoute/Autoroute">
        <rdf:type rdf:resource="http://data.ign.fr/def/topo#TypeDeRoute"/>
        <rdf:type rdf:resource="http://www.w3.org/2004/02/skos/core#Concept"/>
        <skos:definition xml:lang="en">Roads without junction, accessible only at designated points for this purpose and reserved for vehicles with mechanical propulsion. The classification in the category of highways is pronounced by decree of the council of state, taken after public inquiry.</skos:definition>
        <skos:definition xml:lang="fr">Routes sans croisement, accessibles seulement en des points aménagés à cet effet et réservées aux véhicules à propulsion mécanique. Le classement dans la catégorie des autoroutes est prononcé par décret du conseil d’état, pris après enquête publique.</skos:definition>
        <skos:inScheme rdf:resource="http://data.ign.fr/id/codes/topo/typederoute/liste"/>
        <skos:prefLabel xml:lang="fr">autoroute</skos:prefLabel>
        <skos:prefLabel xml:lang="en">motorway</skos:prefLabel>
    </owl:NamedIndividual>
    


    <!-- http://data.ign.fr/id/codes/topo/typederoute/BacAuto -->


    <owl:NamedIndividual rdf:about="http://data.ign.fr/id/codes/topo/typederoute/BacAuto">
        <rdf:type rdf:resource="http://data.ign.fr/def/topo#TypeDeRoute"/>
        <rdf:type rdf:resource="http://www.w3.org/2004/02/skos/core#Concept"/>
        <skos:definition xml:lang="en">Routes of the boat used to pass vehicles from one bank to the other of a watercourse or an arm of the sea.</skos:definition>
        <skos:definition xml:lang="fr">Trajets du bateau servant à passer des véhicules d’une rive à l’autre d’un cours d’eau ou d’un bras de mer.</skos:definition>
        <skos:inScheme rdf:resource="http://data.ign.fr/id/codes/topo/typederoute/liste"/>
        <skos:prefLabel xml:lang="fr">bac auto</skos:prefLabel>
        <skos:prefLabel xml:lang="en">car ferry</skos:prefLabel>
    </owl:NamedIndividual>
    


    <!-- http://data.ign.fr/id/codes/topo/typederoute/BacPieton -->


    <owl:NamedIndividual rdf:about="http://data.ign.fr/id/codes/topo/typederoute/BacPieton">
        <rdf:type rdf:resource="http://data.ign.fr/def/topo#TypeDeRoute"/>
        <rdf:type rdf:resource="http://www.w3.org/2004/02/skos/core#Concept"/>
        <skos:definition xml:lang="en">Routes of the boat used to cross pedestrians from one bank to the other of a watercourse or an arm of the sea.</skos:definition>
        <skos:definition xml:lang="fr">Trajets du bateau servant à passer des piétons d’une rive à l’autre d’un cours d’eau ou d’un bras de mer.</skos:definition>
        <skos:inScheme rdf:resource="http://data.ign.fr/id/codes/topo/typederoute/liste"/>
        <skos:prefLabel xml:lang="fr">bac piéton</skos:prefLabel>
        <skos:prefLabel xml:lang="en">passenger ferry</skos:prefLabel>
    </owl:NamedIndividual>
    


    <!-- http://data.ign.fr/id/codes/topo/typederoute/Bretelle -->


    <owl:NamedIndividual rdf:about="http://data.ign.fr/id/codes/topo/typederoute/Bretelle">
        <rdf:type rdf:resource="http://data.ign.fr/def/topo#TypeDeRoute"/>
        <rdf:type rdf:resource="http://www.w3.org/2004/02/skos/core#Concept"/>
        <skos:definition xml:lang="fr">Bretelles de liaison (ou d’échangeur) ou voies d’accès à une aire de service ou de repos.</skos:definition>
        <skos:definition xml:lang="en">Connecting braces (or interchange) or access routes to a service or rest area.</skos:definition>
        <skos:inScheme rdf:resource="http://data.ign.fr/id/codes/topo/typederoute/liste"/>
        <skos:prefLabel xml:lang="fr">bretelle</skos:prefLabel>
        <skos:prefLabel xml:lang="en">ramp</skos:prefLabel>
    </owl:NamedIndividual>
    


    <!-- http://data.ign.fr/id/codes/topo/typederoute/Chemin -->


    <owl:NamedIndividual rdf:about="http://data.ign.fr/id/codes/topo/typederoute/Chemin">
        <rdf:type rdf:resource="http://data.ign.fr/def/topo#TypeDeRoute"/>
        <rdf:type rdf:resource="http://www.w3.org/2004/02/skos/core#Concept"/>
        <skos:definition xml:lang="fr">Les chemins sont prévus pour la circulation de véhicules ou d’engins d’exploitation. Ils ne sont pas forcément carrossables pour tous les véhicules et par tout temps.</skos:definition>
        <skos:definition xml:lang="en">Roads are intended for the circulation of vehicles or machinery. They are not necessarily drivable for all vehicles and in any weather.</skos:definition>
        <skos:inScheme rdf:resource="http://data.ign.fr/id/codes/topo/typederoute/liste"/>
        <skos:prefLabel xml:lang="fr">chemin</skos:prefLabel>
        <skos:prefLabel xml:lang="en">dirt road</skos:prefLabel>
    </owl:NamedIndividual>
    


    <!-- http://data.ign.fr/id/codes/topo/typederoute/Escalier -->


    <owl:NamedIndividual rdf:about="http://data.ign.fr/id/codes/topo/typederoute/Escalier">
        <rdf:type rdf:resource="http://data.ign.fr/def/topo#TypeDeRoute"/>
        <rdf:type rdf:resource="http://www.w3.org/2004/02/skos/core#Concept"/>
        <skos:definition xml:lang="fr">Escaliers directement reliés au réseau routier, assurant la jonction entre deux voies de communication ou entre le réseau routier et un élément adressable.</skos:definition>
        <skos:definition xml:lang="en">Stairs directly connected to the road network, ensuring the junction between two communication channels or between the road network and an addressable element.</skos:definition>
        <skos:inScheme rdf:resource="http://data.ign.fr/id/codes/topo/typederoute/liste"/>
        <skos:prefLabel xml:lang="fr">escalier</skos:prefLabel>
        <skos:prefLabel xml:lang="en">stair way street</skos:prefLabel>
    </owl:NamedIndividual>
    


    <!-- http://data.ign.fr/id/codes/topo/typederoute/PisteCyclable -->


    <owl:NamedIndividual rdf:about="http://data.ign.fr/id/codes/topo/typederoute/PisteCyclable">
        <rdf:type rdf:resource="http://data.ign.fr/def/topo#TypeDeRoute"/>
        <rdf:type rdf:resource="http://www.w3.org/2004/02/skos/core#Concept"/>
        <skos:definition xml:lang="en">Segments of pavement in own site, reserved for bicycles. Bike lanes are excluded.</skos:definition>
        <skos:definition xml:lang="fr">Tronçons de chaussée en site propre, réservés aux cycles. Les bandes cyclables sont exclues.</skos:definition>
        <skos:inScheme rdf:resource="http://data.ign.fr/id/codes/topo/typederoute/liste"/>
        <skos:prefLabel xml:lang="en">bicycle path</skos:prefLabel>
        <skos:prefLabel xml:lang="fr">piste cyclable</skos:prefLabel>
    </owl:NamedIndividual>
    


    <!-- http://data.ign.fr/id/codes/topo/typederoute/QuasiAutoroute -->


    <owl:NamedIndividual rdf:about="http://data.ign.fr/id/codes/topo/typederoute/QuasiAutoroute">
        <rdf:type rdf:resource="http://data.ign.fr/def/topo#TypeDeRoute"/>
        <rdf:type rdf:resource="http://www.w3.org/2004/02/skos/core#Concept"/>
        <skos:definition xml:lang="fr">Routes de même définition que l’autoroute mais non classées officiellement dans cette catégorie. Ce sont des routes à chaussées séparées par un terre-plein central, qui ne possèdent pas de croisement à niveau avec le reste du réseau routier.</skos:definition>
        <skos:definition xml:lang="en">Routes of the same definition as the highway but not officially classified in this category. These are paved roads separated by a median strip, which do not have a level crossing with the rest of the road network.</skos:definition>
        <skos:inScheme rdf:resource="http://data.ign.fr/id/codes/topo/typederoute/liste"/>
        <skos:prefLabel xml:lang="en">non-classified motorway</skos:prefLabel>
        <skos:prefLabel xml:lang="fr">quasi-autoroute</skos:prefLabel>
    </owl:NamedIndividual>
    


    <!-- http://data.ign.fr/id/codes/topo/typederoute/RouteADeuxChaussees -->


    <owl:NamedIndividual rdf:about="http://data.ign.fr/id/codes/topo/typederoute/RouteADeuxChaussees">
        <rdf:type rdf:resource="http://data.ign.fr/def/topo#TypeDeRoute"/>
        <rdf:type rdf:resource="http://www.w3.org/2004/02/skos/core#Concept"/>
        <skos:definition xml:lang="en">Roads with 2 carriageways separated by a physical obstacle possibly open at intersections. They therefore have level crossings, which prevents them from being classified in the highway or near-highway category.</skos:definition>
        <skos:definition xml:lang="fr">Routes comportant 2 chaussées séparées par un obstacle physique éventuellement ouvert aux carrefours. Elles possèdent donc des croisements à niveau, ce qui leur interdit d&apos;être classées dans la catégorie autoroute ou quasi-autoroute.</skos:definition>
        <skos:inScheme rdf:resource="http://data.ign.fr/id/codes/topo/typederoute/liste"/>
        <skos:prefLabel xml:lang="en">dual carriageway road</skos:prefLabel>
        <skos:prefLabel xml:lang="fr">route à deux chaussées</skos:prefLabel>
    </owl:NamedIndividual>
    


    <!-- http://data.ign.fr/id/codes/topo/typederoute/RouteAUneChaussee -->


    <owl:NamedIndividual rdf:about="http://data.ign.fr/id/codes/topo/typederoute/RouteAUneChaussee">
        <rdf:type rdf:resource="http://data.ign.fr/def/topo#TypeDeRoute"/>
        <rdf:type rdf:resource="http://www.w3.org/2004/02/skos/core#Concept"/>
        <skos:definition xml:lang="en">Roads with 1 roadway. All tarmac roads that are not classified as 2-lane Road, Near-highway or Highway are included in this class.</skos:definition>
        <skos:definition xml:lang="fr">Routes comportant 1 chaussée. Toutes les routes goudronnées qui ne sont pas classées en Route à 2 chaussées, Quasi-autoroute ou Autoroute se retrouvent dans cette classe.</skos:definition>
        <skos:inScheme rdf:resource="http://data.ign.fr/id/codes/topo/typederoute/liste"/>
        <skos:prefLabel xml:lang="fr">route à une chaussée</skos:prefLabel>
        <skos:prefLabel xml:lang="en">single carriageway road</skos:prefLabel>
    </owl:NamedIndividual>
    


    <!-- http://data.ign.fr/id/codes/topo/typederoute/RouteDepartementale -->


    <owl:NamedIndividual rdf:about="http://data.ign.fr/id/codes/topo/typederoute/RouteDepartementale">
        <rdf:type rdf:resource="http://data.ign.fr/def/topo#TypeDeRoute"/>
        <rdf:type rdf:resource="http://www.w3.org/2004/02/skos/core#Concept"/>
        <skos:definition xml:lang="en">Road that is part of the public road departmental.</skos:definition>
        <skos:definition xml:lang="fr">Voie qui fait partie du domaine public routier départemental.</skos:definition>
        <skos:inScheme rdf:resource="http://data.ign.fr/id/codes/topo/typederoute/liste"/>
        <skos:prefLabel xml:lang="fr">route départementale</skos:prefLabel>
        <skos:prefLabel xml:lang="en">secondary road</skos:prefLabel>
    </owl:NamedIndividual>
    


    <!-- http://data.ign.fr/id/codes/topo/typederoute/RouteEmpierree -->


    <owl:NamedIndividual rdf:about="http://data.ign.fr/id/codes/topo/typederoute/RouteEmpierree">
        <rdf:type rdf:resource="http://data.ign.fr/def/topo#TypeDeRoute"/>
        <rdf:type rdf:resource="http://www.w3.org/2004/02/skos/core#Concept"/>
        <skos:definition xml:lang="en">Roads lightly surfaced (no surface coating or very degraded coating), but allowing the circulation of passenger cars all the time. All stone roads are included.</skos:definition>
        <skos:definition xml:lang="fr">Routes sommairement revêtues (pas de revêtement de surface ou revêtement très dégradé), mais permettant la circulation de véhicules automobiles de tourisme par tout temps. Toutes les routes empierrées sont incluses.</skos:definition>
        <skos:inScheme rdf:resource="http://data.ign.fr/id/codes/topo/typederoute/liste"/>
        <skos:prefLabel xml:lang="en">gravel road</skos:prefLabel>
        <skos:prefLabel xml:lang="fr">route empierrée</skos:prefLabel>
    </owl:NamedIndividual>
    


    <!-- http://data.ign.fr/id/codes/topo/typederoute/RouteNationale -->


    <owl:NamedIndividual rdf:about="http://data.ign.fr/id/codes/topo/typederoute/RouteNationale">
        <rdf:type rdf:resource="http://data.ign.fr/def/topo#TypeDeRoute"/>
        <rdf:type rdf:resource="http://www.w3.org/2004/02/skos/core#Concept"/>
        <skos:definition xml:lang="en">National public highway roadway other than motorways.</skos:definition>
        <skos:definition xml:lang="fr">Voie du domaine public routier national autre que les autoroutes.</skos:definition>
        <skos:inScheme rdf:resource="http://data.ign.fr/id/codes/topo/typederoute/liste"/>
        <skos:prefLabel xml:lang="en">main road</skos:prefLabel>
        <skos:prefLabel xml:lang="fr">route nationale</skos:prefLabel>
    </owl:NamedIndividual>
    


    <!-- http://data.ign.fr/id/codes/topo/typederoute/Sentier -->


    <owl:NamedIndividual rdf:about="http://data.ign.fr/id/codes/topo/typederoute/Sentier">
        <rdf:type rdf:resource="http://data.ign.fr/def/topo#TypeDeRoute"/>
        <rdf:type rdf:resource="http://www.w3.org/2004/02/skos/core#Concept"/>
        <skos:definition xml:lang="fr">Chemins étroits ne permettant pas le passage de véhicules. Seuls les principaux sentiers sont inclus. Passerelles supportant une allée, directement reliés au réseau routier. Les passerelles ont une position par rapport au sol supérieure à 0.</skos:definition>
        <skos:definition xml:lang="en">Narrow paths that do not allow the passage of vehicles. Only the main trails are included. Bridges supporting an alley, directly connected to the road network. The bridges have a position relative to the ground greater than 0.</skos:definition>
        <skos:inScheme rdf:resource="http://data.ign.fr/id/codes/topo/typederoute/liste"/>
        <skos:prefLabel xml:lang="en">footpath</skos:prefLabel>
        <skos:prefLabel xml:lang="fr">sentier</skos:prefLabel>
    </owl:NamedIndividual>
    


    <!-- http://data.ign.fr/id/codes/topo/typederoute/liste -->


    <owl:NamedIndividual rdf:about="http://data.ign.fr/id/codes/topo/typederoute/liste">
        <rdf:type rdf:resource="http://www.w3.org/2004/02/skos/core#ConceptScheme"/>
        <rdfs:comment xml:lang="en">List of different road types, represented as a hierarchy of SKOS concepts.</rdfs:comment>
        <rdfs:comment xml:lang="fr">Liste des différents types de routes, représentés comme une hiérarchie de concepts SKOS.</rdfs:comment>
        <rdfs:label xml:lang="fr">Type de route</rdfs:label>
        <rdfs:label xml:lang="en">Type of road</rdfs:label>
    </owl:NamedIndividual>
    


    <!-- http://data.ign.fr/id/codes/topo/typedesource/AutreSource -->


    <owl:NamedIndividual rdf:about="http://data.ign.fr/id/codes/topo/typedesource/AutreSource">
        <rdf:type rdf:resource="http://www.w3.org/ns/prov#Entity"/>
        <rdfs:label xml:lang="fr">autre source de données</rdfs:label>
        <rdfs:label xml:lang="en">other data source</rdfs:label>
    </owl:NamedIndividual>
    


    <!-- http://data.ign.fr/id/codes/topo/typedesource/BdCarto -->


    <owl:NamedIndividual rdf:about="http://data.ign.fr/id/codes/topo/typedesource/BdCarto">
        <rdf:type rdf:resource="http://www.w3.org/ns/prov#Entity"/>
        <rdfs:label xml:lang="en">BD CARTO</rdfs:label>
        <rdfs:label xml:lang="fr">BD CARTO</rdfs:label>
        <foaf:homepage rdf:resource="http://professionnels.ign.fr/bdcarto"/>
    </owl:NamedIndividual>
    


    <!-- http://data.ign.fr/id/codes/topo/typedesource/BdNyme -->


    <owl:NamedIndividual rdf:about="http://data.ign.fr/id/codes/topo/typedesource/BdNyme">
        <rdf:type rdf:resource="http://www.w3.org/ns/prov#Entity"/>
        <rdfs:label xml:lang="en">BD NYME</rdfs:label>
        <rdfs:label xml:lang="fr">BD NYME</rdfs:label>
        <foaf:homepage rdf:resource="http://professionnels.ign.fr/bdnyme"/>
    </owl:NamedIndividual>
    


    <!-- http://data.ign.fr/id/codes/topo/typedesource/BdParcellaire -->


    <owl:NamedIndividual rdf:about="http://data.ign.fr/id/codes/topo/typedesource/BdParcellaire">
        <rdf:type rdf:resource="http://www.w3.org/ns/prov#Entity"/>
        <rdfs:label xml:lang="en">BD PARCELLAIRE</rdfs:label>
        <rdfs:label xml:lang="fr">BD PARCELLAIRE</rdfs:label>
        <foaf:homepage rdf:resource="http://professionnels.ign.fr/bdparcellaire"/>
    </owl:NamedIndividual>
    


    <!-- http://data.ign.fr/id/codes/topo/typedesource/BdTopo -->


    <owl:NamedIndividual rdf:about="http://data.ign.fr/id/codes/topo/typedesource/BdTopo">
        <rdf:type rdf:resource="http://www.w3.org/ns/prov#Entity"/>
        <rdfs:label xml:lang="en">BD TOPO</rdfs:label>
        <rdfs:label xml:lang="fr">BD TOPO</rdfs:label>
        <foaf:homepage rdf:resource="http://professionnels.ign.fr/bdtopo"/>
    </owl:NamedIndividual>
    


    <!-- http://data.ign.fr/id/codes/topo/typedesource/Cadastre -->


    <owl:NamedIndividual rdf:about="http://data.ign.fr/id/codes/topo/typedesource/Cadastre">
        <rdf:type rdf:resource="http://www.w3.org/ns/prov#Entity"/>
        <rdfs:label xml:lang="en">cadastre</rdfs:label>
        <rdfs:label xml:lang="fr">cadastre</rdfs:label>
    </owl:NamedIndividual>
    


    <!-- http://data.ign.fr/id/codes/topo/typedesource/Calcul -->


    <owl:NamedIndividual rdf:about="http://data.ign.fr/id/codes/topo/typedesource/Calcul">
        <rdf:type rdf:resource="http://www.w3.org/ns/prov#Entity"/>
        <rdfs:label xml:lang="fr">calcul</rdfs:label>
        <rdfs:label xml:lang="en">computation</rdfs:label>
    </owl:NamedIndividual>
    


    <!-- http://data.ign.fr/id/codes/topo/typedesource/Fichier -->


    <owl:NamedIndividual rdf:about="http://data.ign.fr/id/codes/topo/typedesource/Fichier">
        <rdf:type rdf:resource="http://www.w3.org/ns/prov#Entity"/>
        <rdfs:label xml:lang="fr">fichier</rdfs:label>
        <rdfs:label xml:lang="en">file</rdfs:label>
    </owl:NamedIndividual>
    


    <!-- http://data.ign.fr/id/codes/topo/typedesource/Georoute -->


    <owl:NamedIndividual rdf:about="http://data.ign.fr/id/codes/topo/typedesource/Georoute">
        <rdf:type rdf:resource="http://www.w3.org/ns/prov#Entity"/>
        <rdfs:label xml:lang="en">Georoute</rdfs:label>
        <rdfs:label xml:lang="fr">Géoroute</rdfs:label>
    </owl:NamedIndividual>
    


    <!-- http://data.ign.fr/id/codes/topo/typedesource/Orthophotographie -->


    <owl:NamedIndividual rdf:about="http://data.ign.fr/id/codes/topo/typedesource/Orthophotographie">
        <rdf:type rdf:resource="http://www.w3.org/ns/prov#Entity"/>
        <rdfs:label xml:lang="en">orthophotograph</rdfs:label>
        <rdfs:label xml:lang="fr">orthophotographie</rdfs:label>
    </owl:NamedIndividual>
    


    <!-- http://data.ign.fr/id/codes/topo/typedesource/Plan -->


    <owl:NamedIndividual rdf:about="http://data.ign.fr/id/codes/topo/typedesource/Plan">
        <rdf:type rdf:resource="http://www.w3.org/ns/prov#Entity"/>
        <rdfs:label xml:lang="en">plan</rdfs:label>
        <rdfs:label xml:lang="fr">plan</rdfs:label>
    </owl:NamedIndividual>
    


    <!-- http://data.ign.fr/id/codes/topo/typedesource/Scan25 -->


    <owl:NamedIndividual rdf:about="http://data.ign.fr/id/codes/topo/typedesource/Scan25">
        <rdf:type rdf:resource="http://www.w3.org/ns/prov#Entity"/>
        <rdfs:label xml:lang="en">Scan25</rdfs:label>
        <rdfs:label xml:lang="fr">Scan25</rdfs:label>
        <foaf:homepage rdf:resource="http://professionnels.ign.fr/scan25"/>
    </owl:NamedIndividual>
    


    <!-- http://data.ign.fr/id/codes/topo/typedesource/Terrain -->


    <owl:NamedIndividual rdf:about="http://data.ign.fr/id/codes/topo/typedesource/Terrain">
        <rdf:type rdf:resource="http://www.w3.org/ns/prov#Entity"/>
        <rdfs:label xml:lang="fr">relevé de terrain</rdfs:label>
        <rdfs:label xml:lang="en">topographic survey</rdfs:label>
    </owl:NamedIndividual>
    


    <!-- http://data.ign.fr/id/codes/topo/typedeterraindesport/BassinDeNatation -->


    <owl:NamedIndividual rdf:about="http://data.ign.fr/id/codes/topo/typedeterraindesport/BassinDeNatation">
        <rdf:type rdf:resource="http://data.ign.fr/def/topo#TypeDeTerrainDeSport"/>
        <rdf:type rdf:resource="http://www.w3.org/2004/02/skos/core#Concept"/>
        <skos:broadMatch rdf:resource="http://data.ign.fr/id/codes/topo/typedezai/Piscine"/>
        <skos:definition xml:lang="fr">Bassin de natation d’une piscine découverte : bassin de natation, piscine (découverte).</skos:definition>
        <skos:definition xml:lang="en">Swimming pool of an outdoor swimming pool: swimming pool, swimming pool (discovery).</skos:definition>
        <skos:inScheme rdf:resource="http://data.ign.fr/id/codes/topo/typedeterraindesport/liste"/>
        <skos:prefLabel xml:lang="fr">bassin de natation</skos:prefLabel>
        <skos:prefLabel xml:lang="en">swimming-pool</skos:prefLabel>
    </owl:NamedIndividual>
    


    <!-- http://data.ign.fr/id/codes/topo/typedeterraindesport/PisteDeSport -->


    <owl:NamedIndividual rdf:about="http://data.ign.fr/id/codes/topo/typedeterraindesport/PisteDeSport">
        <rdf:type rdf:resource="http://data.ign.fr/def/topo#TypeDeTerrainDeSport"/>
        <rdf:type rdf:resource="http://www.w3.org/2004/02/skos/core#Concept"/>
        <skos:definition xml:lang="en">Large outdoor track reserved for the race: autodrome (track), automoto circuit (track), track (racetrack), racecourse (track), velodrome (track).</skos:definition>
        <skos:definition xml:lang="fr">Large piste en plein air réservée à la course : autodrome (piste), circuit automoto (piste), cynodrome (piste), hippodrome (piste), vélodrome (piste).</skos:definition>
        <skos:inScheme rdf:resource="http://data.ign.fr/id/codes/topo/typedeterraindesport/liste"/>
        <skos:prefLabel xml:lang="fr">piste de sport</skos:prefLabel>
        <skos:prefLabel xml:lang="en">sports track</skos:prefLabel>
    </owl:NamedIndividual>
    


    <!-- http://data.ign.fr/id/codes/topo/typedeterraindesport/TerrainDeTennis -->


    <owl:NamedIndividual rdf:about="http://data.ign.fr/id/codes/topo/typedeterraindesport/TerrainDeTennis">
        <rdf:type rdf:resource="http://data.ign.fr/def/topo#TypeDeTerrainDeSport"/>
        <rdf:type rdf:resource="http://www.w3.org/2004/02/skos/core#Concept"/>
        <skos:definition xml:lang="en">Specially landscaped grounds for playing tennis.</skos:definition>
        <skos:definition xml:lang="fr">Terrain spécialement aménagé pour la pratique du tennis.</skos:definition>
        <skos:inScheme rdf:resource="http://data.ign.fr/id/codes/topo/typedeterraindesport/liste"/>
        <skos:prefLabel xml:lang="en">tennis court</skos:prefLabel>
        <skos:prefLabel xml:lang="fr">terrain de tennis</skos:prefLabel>
    </owl:NamedIndividual>
    


    <!-- http://data.ign.fr/id/codes/topo/typedeterraindesport/liste -->


    <owl:NamedIndividual rdf:about="http://data.ign.fr/id/codes/topo/typedeterraindesport/liste">
        <rdf:type rdf:resource="http://www.w3.org/2004/02/skos/core#ConceptScheme"/>
        <rdfs:comment xml:lang="en">List of different types of sports fields, represented as a hierarchy of SKOS concepts.</rdfs:comment>
        <rdfs:comment xml:lang="fr">Liste des différents types de terrains de sport, représentés comme une hiérarchie de concepts SKOS.</rdfs:comment>
        <rdfs:label xml:lang="fr">Type de terrain de sport</rdfs:label>
        <rdfs:label xml:lang="en">Type of sports ground</rdfs:label>
    </owl:NamedIndividual>
    


    <!-- http://data.ign.fr/id/codes/topo/typedetransportcable/CableTransporteur -->


    <owl:NamedIndividual rdf:about="http://data.ign.fr/id/codes/topo/typedetransportcable/CableTransporteur">
        <rdf:type rdf:resource="http://data.ign.fr/def/topo#TypeDeTransportCable"/>
        <rdf:type rdf:resource="http://www.w3.org/2004/02/skos/core#Concept"/>
        <skos:definition xml:lang="en">Means of transport consisting of one or more load-bearing cables used to transport equipment.</skos:definition>
        <skos:definition xml:lang="fr">Moyen de transport constitué d&apos;un ou de plusieurs câbles porteurs et servant à assurer le transport de matériel.</skos:definition>
        <skos:inScheme rdf:resource="http://data.ign.fr/id/codes/topo/typedetransportcable/liste"/>
        <skos:prefLabel xml:lang="en">cableway</skos:prefLabel>
        <skos:prefLabel xml:lang="fr">câble transporteur</skos:prefLabel>
    </owl:NamedIndividual>
    


    <!-- http://data.ign.fr/id/codes/topo/typedetransportcable/Telepherique -->


    <owl:NamedIndividual rdf:about="http://data.ign.fr/id/codes/topo/typedetransportcable/Telepherique">
        <rdf:type rdf:resource="http://data.ign.fr/def/topo#TypeDeTransportCable"/>
        <rdf:type rdf:resource="http://data.ign.fr/def/topo#TypeDeZAI"/>
        <rdf:type rdf:resource="http://www.w3.org/2004/02/skos/core#Concept"/>
        <skos:broader rdf:resource="http://data.ign.fr/id/codes/topo/typedezai/PAITransport"/>
        <skos:definition xml:lang="en">Cable cars, including ski lifts, lifts, gondola lifts, ski lifts, telebens, chair lifts.</skos:definition>
        <skos:definition xml:lang="fr">Téléphériques, y compris les remonte-pentes, remontées mécaniques, télécabines, téléskis, télébennes, télésièges.</skos:definition>
        <skos:inScheme rdf:resource="http://data.ign.fr/id/codes/topo/typedetransportcable/liste"/>
        <skos:inScheme rdf:resource="http://data.ign.fr/id/codes/topo/typedezai/liste"/>
        <skos:prefLabel xml:lang="en">aerial ropeway</skos:prefLabel>
        <skos:prefLabel xml:lang="fr">téléphérique</skos:prefLabel>
    </owl:NamedIndividual>
    


    <!-- http://data.ign.fr/id/codes/topo/typedetransportcable/liste -->


    <owl:NamedIndividual rdf:about="http://data.ign.fr/id/codes/topo/typedetransportcable/liste">
        <rdf:type rdf:resource="http://www.w3.org/2004/02/skos/core#ConceptScheme"/>
        <rdfs:comment xml:lang="en">List of different types of cable transport lines, represented as a hierarchy of SKOS concepts.</rdfs:comment>
        <rdfs:comment xml:lang="fr">Liste des différents types lignes de transport par câble, représentés comme une hiérarchie de concepts SKOS.</rdfs:comment>
        <rdfs:label xml:lang="fr">Type de ligne de transport par câble</rdfs:label>
        <rdfs:label xml:lang="en">Type of cableway transport line</rdfs:label>
    </owl:NamedIndividual>
    


    <!-- http://data.ign.fr/id/codes/topo/typedevegetation/Bananeraie -->


    <owl:NamedIndividual rdf:about="http://data.ign.fr/id/codes/topo/typedevegetation/Bananeraie">
        <rdf:type rdf:resource="http://data.ign.fr/def/topo#TypeDeVegetation"/>
        <rdf:type rdf:resource="http://www.w3.org/2004/02/skos/core#Concept"/>
        <skos:broader rdf:resource="http://data.ign.fr/id/codes/topo/typedebatiment/ZoneArboree"/>
        <skos:definition xml:lang="en">Banana plantation.</skos:definition>
        <skos:definition xml:lang="fr">Plantation de bananiers.</skos:definition>
        <skos:inScheme rdf:resource="http://data.ign.fr/id/codes/topo/typedevegetation/liste"/>
        <skos:prefLabel xml:lang="en">banana plantation</skos:prefLabel>
        <skos:prefLabel xml:lang="fr">bananeraie</skos:prefLabel>
    </owl:NamedIndividual>
    


    <!-- http://data.ign.fr/id/codes/topo/typedevegetation/Bois -->


    <owl:NamedIndividual rdf:about="http://data.ign.fr/id/codes/topo/typedevegetation/Bois">
        <rdf:type rdf:resource="http://data.ign.fr/def/topo#TypeDeVegetation"/>
        <rdf:type rdf:resource="http://www.w3.org/2004/02/skos/core#Concept"/>
        <skos:broader rdf:resource="http://data.ign.fr/id/codes/topo/typedebatiment/ZoneArboree"/>
        <skos:broader rdf:resource="http://data.ign.fr/id/codes/topo/typedezai/PAIEspaceNaturel"/>
        <skos:definition xml:lang="en">Area populated by forest trees covering at least 40% of the soil.</skos:definition>
        <skos:definition xml:lang="fr">Espace peuplé d’arbres forestiers couvrant au moins 40% du sol.</skos:definition>
        <skos:inScheme rdf:resource="http://data.ign.fr/id/codes/topo/typedevegetation/liste"/>
        <skos:inScheme rdf:resource="http://data.ign.fr/id/codes/topo/typedezai/liste"/>
        <skos:prefLabel xml:lang="fr">bois</skos:prefLabel>
        <skos:prefLabel xml:lang="en">wood</skos:prefLabel>
    </owl:NamedIndividual>
    


    <!-- http://data.ign.fr/id/codes/topo/typedevegetation/CanneASucre -->


    <owl:NamedIndividual rdf:about="http://data.ign.fr/id/codes/topo/typedevegetation/CanneASucre">
        <rdf:type rdf:resource="http://data.ign.fr/def/topo#TypeDeVegetation"/>
        <rdf:type rdf:resource="http://www.w3.org/2004/02/skos/core#Concept"/>
        <skos:broader rdf:resource="http://data.ign.fr/id/codes/topo/typedebatiment/ZoneArboree"/>
        <skos:definition xml:lang="fr">Plantation de canne à sucre.</skos:definition>
        <skos:definition xml:lang="en">Plantation of sugar cane.</skos:definition>
        <skos:inScheme rdf:resource="http://data.ign.fr/id/codes/topo/typedevegetation/liste"/>
        <skos:prefLabel xml:lang="fr">canne à sucre</skos:prefLabel>
        <skos:prefLabel xml:lang="en">sugarcane plantation</skos:prefLabel>
    </owl:NamedIndividual>
    


    <!-- http://data.ign.fr/id/codes/topo/typedevegetation/ForetFermeeConiferes -->


    <owl:NamedIndividual rdf:about="http://data.ign.fr/id/codes/topo/typedevegetation/ForetFermeeConiferes">
        <rdf:type rdf:resource="http://data.ign.fr/def/topo#TypeDeVegetation"/>
        <rdf:type rdf:resource="http://www.w3.org/2004/02/skos/core#Concept"/>
        <skos:broader rdf:resource="http://data.ign.fr/id/codes/topo/typedebatiment/ZoneArboree"/>
        <skos:definition xml:lang="en">Area populated with forest trees covering at least 40% of the soil and composed mainly of conifers (ie a relative cover rate of more than 75%).</skos:definition>
        <skos:definition xml:lang="fr">Espace peuplé d’arbres forestiers couvrant au moins 40% du sol et composée essentiellement de conifères (soit un taux de couvert relatif de plus de 75%).</skos:definition>
        <skos:inScheme rdf:resource="http://data.ign.fr/id/codes/topo/typedevegetation/liste"/>
        <skos:prefLabel xml:lang="en">closed softwood forest</skos:prefLabel>
        <skos:prefLabel xml:lang="fr">forêt fermée de conifères</skos:prefLabel>
    </owl:NamedIndividual>
    


    <!-- http://data.ign.fr/id/codes/topo/typedevegetation/ForetFermeeFeuillus -->


    <owl:NamedIndividual rdf:about="http://data.ign.fr/id/codes/topo/typedevegetation/ForetFermeeFeuillus">
        <rdf:type rdf:resource="http://data.ign.fr/def/topo#TypeDeVegetation"/>
        <rdf:type rdf:resource="http://www.w3.org/2004/02/skos/core#Concept"/>
        <skos:broader rdf:resource="http://data.ign.fr/id/codes/topo/typedebatiment/ZoneArboree"/>
        <skos:definition xml:lang="en">Area populated with forest trees covering at least 40% of the soil, and composed of more than 75% of hardwoods (relative cover rate).</skos:definition>
        <skos:definition xml:lang="fr">Espace peuplé d’arbres forestiers couvrant au moins 40% du sol, et composée de plus de 75% de feuillus (taux de couvert relatif).</skos:definition>
        <skos:inScheme rdf:resource="http://data.ign.fr/id/codes/topo/typedevegetation/liste"/>
        <skos:prefLabel xml:lang="en">closed hardwood forest</skos:prefLabel>
        <skos:prefLabel xml:lang="fr">forêt fermée de feuillus</skos:prefLabel>
    </owl:NamedIndividual>
    


    <!-- http://data.ign.fr/id/codes/topo/typedevegetation/ForetFermeeMixte -->


    <owl:NamedIndividual rdf:about="http://data.ign.fr/id/codes/topo/typedevegetation/ForetFermeeMixte">
        <rdf:type rdf:resource="http://data.ign.fr/def/topo#TypeDeVegetation"/>
        <rdf:type rdf:resource="http://www.w3.org/2004/02/skos/core#Concept"/>
        <skos:broader rdf:resource="http://data.ign.fr/id/codes/topo/typedebatiment/ZoneArboree"/>
        <skos:definition xml:lang="en">Area populated with forest trees covering at least 40% of the soil, and composed of more than 25% and less than 75% of hardwoods (relative cover rate).</skos:definition>
        <skos:definition xml:lang="fr">Espace peuplé d’arbres forestiers couvrant au moins 40% du sol, et composée de plus de 25% et moins de 75% de feuillus (taux de couvert relatif).</skos:definition>
        <skos:inScheme rdf:resource="http://data.ign.fr/id/codes/topo/typedevegetation/liste"/>
        <skos:prefLabel xml:lang="en">closed mixed forest</skos:prefLabel>
        <skos:prefLabel xml:lang="fr">forêt fermée mixte</skos:prefLabel>
    </owl:NamedIndividual>
    


    <!-- http://data.ign.fr/id/codes/topo/typedevegetation/ForetOuverte -->


    <owl:NamedIndividual rdf:about="http://data.ign.fr/id/codes/topo/typedevegetation/ForetOuverte">
        <rdf:type rdf:resource="http://data.ign.fr/def/topo#TypeDeVegetation"/>
        <rdf:type rdf:resource="http://www.w3.org/2004/02/skos/core#Concept"/>
        <skos:broader rdf:resource="http://data.ign.fr/id/codes/topo/typedebatiment/ZoneArboree"/>
        <skos:definition xml:lang="en">Area populated with forest trees whose absolute cover is between 10% and 40%.</skos:definition>
        <skos:definition xml:lang="fr">Espace peuplé d’arbres forestiers dont le couvert absolu est compris entre 10% et 40%.</skos:definition>
        <skos:inScheme rdf:resource="http://data.ign.fr/id/codes/topo/typedevegetation/liste"/>
        <skos:prefLabel xml:lang="fr">forêt ouverte</skos:prefLabel>
        <skos:prefLabel xml:lang="en">open forest</skos:prefLabel>
    </owl:NamedIndividual>
    


    <!-- http://data.ign.fr/id/codes/topo/typedevegetation/Haie -->


    <owl:NamedIndividual rdf:about="http://data.ign.fr/id/codes/topo/typedevegetation/Haie">
        <rdf:type rdf:resource="http://data.ign.fr/def/topo#TypeDeVegetation"/>
        <rdf:type rdf:resource="http://www.w3.org/2004/02/skos/core#Concept"/>
        <skos:broader rdf:resource="http://data.ign.fr/id/codes/topo/typedebatiment/ZoneArboree"/>
        <skos:definition xml:lang="en">A natural fence made of trees, shrubs, thorns or branches that serves to limit or protect a field. Aligning trees or planting fruit trees less than 25 m wide.</skos:definition>
        <skos:definition xml:lang="fr">Clôture naturelle composée d’arbres, d’arbustes, d’épines ou de branchages et servant à limiter ou à protéger un champ. Alignement d’arbres ou plantation d’arbres fruitiers dont la largeur est inférieure à 25 m.</skos:definition>
        <skos:inScheme rdf:resource="http://data.ign.fr/id/codes/topo/typedevegetation/liste"/>
        <skos:prefLabel xml:lang="fr">haie</skos:prefLabel>
        <skos:prefLabel xml:lang="en">hedge</skos:prefLabel>
    </owl:NamedIndividual>
    


    <!-- http://data.ign.fr/id/codes/topo/typedevegetation/LandeLigneuse -->


    <owl:NamedIndividual rdf:about="http://data.ign.fr/id/codes/topo/typedevegetation/LandeLigneuse">
        <rdf:type rdf:resource="http://data.ign.fr/def/topo#TypeDeVegetation"/>
        <rdf:type rdf:resource="http://www.w3.org/2004/02/skos/core#Concept"/>
        <skos:broader rdf:resource="http://data.ign.fr/id/codes/topo/typedebatiment/ZoneArboree"/>
        <skos:definition xml:lang="en">Spontaneous vegetation that includes a significant proportion of woody plants (heather, broom, gorse, various thorny, etc.) and semi woody (ferns, phragmites ...) whose height does not exceed 5 meters. This woody vegetation has a vegetative cover of at least 25%.</skos:definition>
        <skos:definition xml:lang="fr">Végétation spontanée qui comprend une proportion importante de plantes ligneuses (bruyères, genêts, ajoncs, épineux divers, etc.) et semi ligneuses (fougères, phragmites…) dont la hauteur ne dépasse pas 5 mètres. Cette végétation ligneuse présente un couvert végétal d’au moins 25%.</skos:definition>
        <skos:inScheme rdf:resource="http://data.ign.fr/id/codes/topo/typedevegetation/liste"/>
        <skos:prefLabel xml:lang="fr">lande ligneuse</skos:prefLabel>
        <skos:prefLabel xml:lang="en">woody heath</skos:prefLabel>
    </owl:NamedIndividual>
    


    <!-- http://data.ign.fr/id/codes/topo/typedevegetation/Mangrove -->


    <owl:NamedIndividual rdf:about="http://data.ign.fr/id/codes/topo/typedevegetation/Mangrove">
        <rdf:type rdf:resource="http://data.ign.fr/def/topo#TypeDeVegetation"/>
        <rdf:type rdf:resource="http://www.w3.org/2004/02/skos/core#Concept"/>
        <skos:broader rdf:resource="http://data.ign.fr/id/codes/topo/typedebatiment/ZoneArboree"/>
        <skos:definition xml:lang="fr">Dans les régions côtières intertropicales,formation végétale caractérisée par des forêts impénétrables de palétuviers qui fixent leurs fortes racines dans les baies aux eaux calmes où se déposent boues et limons.</skos:definition>
        <skos:definition xml:lang="en">In the intertropical coastal regions, vegetation formation characterized by impenetrable forests of mangroves that fix their strong roots in the bays with calm waters where sludge and silt are deposited.</skos:definition>
        <skos:inScheme rdf:resource="http://data.ign.fr/id/codes/topo/typedevegetation/liste"/>
        <skos:prefLabel xml:lang="fr">mangrove</skos:prefLabel>
        <skos:prefLabel xml:lang="en">mangrove forest</skos:prefLabel>
    </owl:NamedIndividual>
    


    <!-- http://data.ign.fr/id/codes/topo/typedevegetation/Peupleraie -->


    <owl:NamedIndividual rdf:about="http://data.ign.fr/id/codes/topo/typedevegetation/Peupleraie">
        <rdf:type rdf:resource="http://data.ign.fr/def/topo#TypeDeVegetation"/>
        <rdf:type rdf:resource="http://www.w3.org/2004/02/skos/core#Concept"/>
        <skos:broader rdf:resource="http://data.ign.fr/id/codes/topo/typedebatiment/ZoneArboree"/>
        <skos:definition xml:lang="en">Area planted with poplars.</skos:definition>
        <skos:definition xml:lang="fr">Zone plantée de peupliers.</skos:definition>
        <skos:inScheme rdf:resource="http://data.ign.fr/id/codes/topo/typedevegetation/liste"/>
        <skos:prefLabel xml:lang="fr">peupleraie</skos:prefLabel>
        <skos:prefLabel xml:lang="en">poplar plantation</skos:prefLabel>
    </owl:NamedIndividual>
    


    <!-- http://data.ign.fr/id/codes/topo/typedevegetation/Verger -->


    <owl:NamedIndividual rdf:about="http://data.ign.fr/id/codes/topo/typedevegetation/Verger">
        <rdf:type rdf:resource="http://data.ign.fr/def/topo#TypeDeVegetation"/>
        <rdf:type rdf:resource="http://www.w3.org/2004/02/skos/core#Concept"/>
        <skos:broader rdf:resource="http://data.ign.fr/id/codes/topo/typedebatiment/ZoneArboree"/>
        <skos:definition xml:lang="en">Non-forest stand plantation area.</skos:definition>
        <skos:definition xml:lang="fr">Zone de plantation d’arbres hors peuplement forestier.</skos:definition>
        <skos:inScheme rdf:resource="http://data.ign.fr/id/codes/topo/typedevegetation/liste"/>
        <skos:prefLabel xml:lang="en">orchard</skos:prefLabel>
        <skos:prefLabel xml:lang="fr">verger</skos:prefLabel>
    </owl:NamedIndividual>
    


    <!-- http://data.ign.fr/id/codes/topo/typedevegetation/Vigne -->


    <owl:NamedIndividual rdf:about="http://data.ign.fr/id/codes/topo/typedevegetation/Vigne">
        <rdf:type rdf:resource="http://data.ign.fr/def/topo#TypeDeVegetation"/>
        <rdf:type rdf:resource="http://www.w3.org/2004/02/skos/core#Concept"/>
        <skos:broader rdf:resource="http://data.ign.fr/id/codes/topo/typedebatiment/ZoneArboree"/>
        <skos:definition xml:lang="en">Vineyard area.</skos:definition>
        <skos:definition xml:lang="fr">Zone de vignes.</skos:definition>
        <skos:inScheme rdf:resource="http://data.ign.fr/id/codes/topo/typedevegetation/liste"/>
        <skos:prefLabel xml:lang="fr">vigne</skos:prefLabel>
        <skos:prefLabel xml:lang="en">vineyard</skos:prefLabel>
    </owl:NamedIndividual>
    


    <!-- http://data.ign.fr/id/codes/topo/typedevegetation/ZoneArboree -->


    <owl:NamedIndividual rdf:about="http://data.ign.fr/id/codes/topo/typedevegetation/ZoneArboree">
        <rdf:type rdf:resource="http://data.ign.fr/def/topo#TypeDeVegetation"/>
        <rdf:type rdf:resource="http://www.w3.org/2004/02/skos/core#Concept"/>
        <skos:definition xml:lang="fr">Espace peuplé d’arbres d’essence quelconque.</skos:definition>
        <skos:definition xml:lang="en">Space populated with trees of any kind.</skos:definition>
        <skos:inScheme rdf:resource="http://data.ign.fr/id/codes/topo/typedevegetation/liste"/>
        <skos:prefLabel xml:lang="en">wooded area</skos:prefLabel>
        <skos:prefLabel xml:lang="fr">zone arborée</skos:prefLabel>
    </owl:NamedIndividual>
    


    <!-- http://data.ign.fr/id/codes/topo/typedevegetation/liste -->


    <owl:NamedIndividual rdf:about="http://data.ign.fr/id/codes/topo/typedevegetation/liste">
        <rdf:type rdf:resource="http://www.w3.org/2004/02/skos/core#ConceptScheme"/>
        <rdfs:comment xml:lang="en">List of different types of vegetation, represented as a hierarchy of SKOS concepts.</rdfs:comment>
        <rdfs:comment xml:lang="fr">Liste des différents types de végétation, représentés comme une hiérarchie de concepts SKOS.</rdfs:comment>
        <rdfs:label xml:lang="fr">Type de végétation</rdfs:label>
        <rdfs:label xml:lang="en">Type of vegetation</rdfs:label>
        <skos:hasTopConcept rdf:resource="http://data.ign.fr/id/codes/topo/typedevegetation/ZoneArboree"/>
    </owl:NamedIndividual>
    


    <!-- http://data.ign.fr/id/codes/topo/typedevoieferree/Funiculaire -->


    <owl:NamedIndividual rdf:about="http://data.ign.fr/id/codes/topo/typedevoieferree/Funiculaire">
        <rdf:type rdf:resource="http://data.ign.fr/def/topo#TypeDeVoieFerree"/>
        <rdf:type rdf:resource="http://www.w3.org/2004/02/skos/core#Concept"/>
        <skos:altLabel xml:lang="en">rack-railway</skos:altLabel>
        <skos:altLabel xml:lang="fr">voie ferrée à crémaillère</skos:altLabel>
        <skos:definition xml:lang="fr">Funiculaire ou voie ferrée à crémaillère.</skos:definition>
        <skos:definition xml:lang="en">Funicular or cog railway.</skos:definition>
        <skos:inScheme rdf:resource="http://data.ign.fr/id/codes/topo/typedevoieferree/liste"/>
        <skos:prefLabel xml:lang="fr">Funiculaire</skos:prefLabel>
        <skos:prefLabel xml:lang="en">Funicular railway</skos:prefLabel>
    </owl:NamedIndividual>
    


    <!-- http://data.ign.fr/id/codes/topo/typedevoieferree/LGV -->


    <owl:NamedIndividual rdf:about="http://data.ign.fr/id/codes/topo/typedevoieferree/LGV">
        <rdf:type rdf:resource="http://data.ign.fr/def/topo#TypeDeVoieFerree"/>
        <rdf:type rdf:resource="http://www.w3.org/2004/02/skos/core#Concept"/>
        <skos:definition xml:lang="fr">Ligne ferroviaire réservée aux trains à grande vitesse.</skos:definition>
        <skos:definition xml:lang="en">Railway line reserved for high-speed trains.</skos:definition>
        <skos:inScheme rdf:resource="http://data.ign.fr/id/codes/topo/typedevoieferree/liste"/>
        <skos:prefLabel xml:lang="fr">ligne à grande vitesse</skos:prefLabel>
        <skos:prefLabel xml:lang="en">ultra-high speed railway</skos:prefLabel>
    </owl:NamedIndividual>
    


    <!-- http://data.ign.fr/id/codes/topo/typedevoieferree/VoieDeService -->


    <owl:NamedIndividual rdf:about="http://data.ign.fr/id/codes/topo/typedevoieferree/VoieDeService">
        <rdf:type rdf:resource="http://data.ign.fr/def/topo#TypeDeVoieFerree"/>
        <rdf:type rdf:resource="http://www.w3.org/2004/02/skos/core#Concept"/>
        <skos:definition xml:lang="fr">Les voies de service de moins de 200 m de long sont exclues, ainsi que les voies s’inscrivant dans un faisceau de voies ferrées de plus de 25 m de large (voir &lt;aire de triage&gt;) et les voies de service souterraines.</skos:definition>
        <skos:definition xml:lang="en">Service roads of less than 200 m in length are excluded, as well as tracks within a railway line of more than 25 m wide (see &lt;marshalling yard&gt;) and underground service roads.</skos:definition>
        <skos:inScheme rdf:resource="http://data.ign.fr/id/codes/topo/typedevoieferree/liste"/>
        <skos:prefLabel xml:lang="en">service track</skos:prefLabel>
        <skos:prefLabel xml:lang="fr">voie de service</skos:prefLabel>
    </owl:NamedIndividual>
    


    <!-- http://data.ign.fr/id/codes/topo/typedevoieferree/VoieNonExploitee -->


    <owl:NamedIndividual rdf:about="http://data.ign.fr/id/codes/topo/typedevoieferree/VoieNonExploitee">
        <rdf:type rdf:resource="http://data.ign.fr/def/topo#TypeDeVoieFerree"/>
        <rdf:type rdf:resource="http://www.w3.org/2004/02/skos/core#Concept"/>
        <skos:definition xml:lang="en">Decommissioned railway, railway closed to all traffic, neutralized railway.</skos:definition>
        <skos:definition xml:lang="fr">Voie ferrée déclassée, voie ferrée fermée à tout trafic, voie ferrée neutralisée.</skos:definition>
        <skos:inScheme rdf:resource="http://data.ign.fr/id/codes/topo/typedevoieferree/liste"/>
        <skos:prefLabel xml:lang="en">unused track</skos:prefLabel>
        <skos:prefLabel xml:lang="fr">voie non exploitée</skos:prefLabel>
    </owl:NamedIndividual>
    


    <!-- http://data.ign.fr/id/codes/topo/typedevoieferree/VoiePrincipale -->


    <owl:NamedIndividual rdf:about="http://data.ign.fr/id/codes/topo/typedevoieferree/VoiePrincipale">
        <rdf:type rdf:resource="http://data.ign.fr/def/topo#TypeDeVoieFerree"/>
        <rdf:type rdf:resource="http://www.w3.org/2004/02/skos/core#Concept"/>
        <skos:definition xml:lang="en">Railway line in operation used for the transport of passengers or goods. RER, railway line in operation, tourist railway, special branch line. All operating rail lines providing regular or seasonal service for the transport of passengers or goods. Metro lines and TGV lines are excluded.</skos:definition>
        <skos:definition xml:lang="fr">Voie ferrée en exploitation servant au transport des voyageurs ou des marchandises. RER, voie ferrée en exploitation, voie ferrée touristique, voie-mère d’embranchement particulier. Toutes les voies ferrées en exploitation assurant un service régulier ou saisonnier pour le transport des voyageurs ou des marchandises. Les lignes de métro et les lignes de TGV sont exclues.</skos:definition>
        <skos:inScheme rdf:resource="http://data.ign.fr/id/codes/topo/typedevoieferree/liste"/>
        <skos:prefLabel xml:lang="en">standard gauge railway</skos:prefLabel>
        <skos:prefLabel xml:lang="fr">voie ferrée principale</skos:prefLabel>
    </owl:NamedIndividual>
    


    <!-- http://data.ign.fr/id/codes/topo/typedevoieferree/VoieTransportUrbain -->


    <owl:NamedIndividual rdf:about="http://data.ign.fr/id/codes/topo/typedevoieferree/VoieTransportUrbain">
        <rdf:type rdf:resource="http://data.ign.fr/def/topo#TypeDeVoieFerree"/>
        <rdf:type rdf:resource="http://www.w3.org/2004/02/skos/core#Concept"/>
        <skos:definition xml:lang="en">Aerial metro or tram line.</skos:definition>
        <skos:definition xml:lang="fr">Ligne de métro aérien ou de tramway.</skos:definition>
        <skos:inScheme rdf:resource="http://data.ign.fr/id/codes/topo/typedevoieferree/liste"/>
        <skos:prefLabel xml:lang="en">urban transport railway</skos:prefLabel>
        <skos:prefLabel xml:lang="fr">voie de transport urbain</skos:prefLabel>
    </owl:NamedIndividual>
    


    <!-- http://data.ign.fr/id/codes/topo/typedevoieferree/liste -->


    <owl:NamedIndividual rdf:about="http://data.ign.fr/id/codes/topo/typedevoieferree/liste">
        <rdf:type rdf:resource="http://www.w3.org/2004/02/skos/core#ConceptScheme"/>
        <rdfs:comment xml:lang="en">List of different types of railways, represented as a hierarchy of SKOS concepts.</rdfs:comment>
        <rdfs:comment xml:lang="fr">Liste des différents types de voies ferrées, représentés comme une hiérarchie de concepts SKOS.</rdfs:comment>
        <rdfs:label xml:lang="fr">Type de voie ferrée</rdfs:label>
        <rdfs:label xml:lang="en">Type of railway track</rdfs:label>
    </owl:NamedIndividual>
    


    <!-- http://data.ign.fr/id/codes/topo/typedezai/Aerodrome -->


    <owl:NamedIndividual rdf:about="http://data.ign.fr/id/codes/topo/typedezai/Aerodrome">
        <rdf:type rdf:resource="http://data.ign.fr/def/topo#TypeDeZAI"/>
        <rdf:type rdf:resource="http://www.w3.org/2004/02/skos/core#Concept"/>
        <skos:broader rdf:resource="http://data.ign.fr/id/codes/topo/typedezai/PAITransport"/>
        <skos:definition xml:lang="en">Any land or body of water specially designed for the landing, take-off and maneuvering of aircraft, including ancillary facilities it may include for the purposes of traffic and the service of aircraft: military aerodrome, military heliport. not taken into account the flying clubs, the gliding grounds, the ULM tracks.</skos:definition>
        <skos:definition xml:lang="fr">Tout terrain ou plan d&apos;eau spécialement aménagé pour l&apos;atterrissage, le décollage et les manoeuvres des aéronefs y compris les installations annexes qu&apos;il peut comporter pour les besoins du trafic et le service des aéronefs : aérodrome militaire, héliport militaire.Ne sont pas pris en compte les aéro-clubs, les terrains de vol à voile, les pistes d&apos;ULM.</skos:definition>
        <skos:inScheme rdf:resource="http://data.ign.fr/id/codes/topo/typedezai/liste"/>
        <skos:prefLabel xml:lang="en">aerodrome</skos:prefLabel>
        <skos:prefLabel xml:lang="fr">aérodrome</skos:prefLabel>
    </owl:NamedIndividual>
    


    <!-- http://data.ign.fr/id/codes/topo/typedezai/AeroportInternational -->


    <owl:NamedIndividual rdf:about="http://data.ign.fr/id/codes/topo/typedezai/AeroportInternational">
        <rdf:type rdf:resource="http://data.ign.fr/def/topo#TypeDeZAI"/>
        <rdf:type rdf:resource="http://www.w3.org/2004/02/skos/core#Concept"/>
        <skos:broader rdf:resource="http://data.ign.fr/id/codes/topo/typedezai/PAITransport"/>
        <skos:definition xml:lang="en">Aerodrome of international status on which facilities have been provided for the shelter, maintenance or distribution of aircraft, and for the reception, loading and unloading of passengers, the loading and unloading of merchandise.</skos:definition>
        <skos:definition xml:lang="fr">Aérodrome de statut international sur lequel ont été prévues des installations en vue de l&apos;abri, de l&apos;entretien ou de la répartition des aéronefs, ainsi que pour la réception, l&apos;embarquement et le débarquement des passagers, le chargement et le déchargement des marchandises.</skos:definition>
        <skos:inScheme rdf:resource="http://data.ign.fr/id/codes/topo/typedezai/liste"/>
        <skos:prefLabel xml:lang="fr">aéroport international</skos:prefLabel>
        <skos:prefLabel xml:lang="en">international airport</skos:prefLabel>
    </owl:NamedIndividual>
    


    <!-- http://data.ign.fr/id/codes/topo/typedezai/AeroportQuelconque -->


    <owl:NamedIndividual rdf:about="http://data.ign.fr/id/codes/topo/typedezai/AeroportQuelconque">
        <rdf:type rdf:resource="http://data.ign.fr/def/topo#TypeDeZAI"/>
        <rdf:type rdf:resource="http://www.w3.org/2004/02/skos/core#Concept"/>
        <skos:broader rdf:resource="http://data.ign.fr/id/codes/topo/typedezai/PAITransport"/>
        <skos:definition xml:lang="en">Aerodrome on which facilities have been provided for the purpose of sheltering, maintaining or distributing aircraft, and for receiving, loading and unloading passengers, loading and unloading of goods.</skos:definition>
        <skos:definition xml:lang="fr">Aérodrome sur lequel ont été prévues des installations en vue de l&apos;abri, de l&apos;entretien ou de la répartition des aéronefs, ainsi que pour la réception, l&apos;embarquement et le débarquement des passagers, le chargement et le déchargement des marchandises.</skos:definition>
        <skos:inScheme rdf:resource="http://data.ign.fr/id/codes/topo/typedezai/liste"/>
        <skos:prefLabel xml:lang="en">airport</skos:prefLabel>
        <skos:prefLabel xml:lang="fr">aéroport</skos:prefLabel>
    </owl:NamedIndividual>
    


    <!-- http://data.ign.fr/id/codes/topo/typedezai/AireDeRepos -->


    <owl:NamedIndividual rdf:about="http://data.ign.fr/id/codes/topo/typedezai/AireDeRepos">
        <rdf:type rdf:resource="http://data.ign.fr/def/topo#TypeDeZAI"/>
        <rdf:type rdf:resource="http://www.w3.org/2004/02/skos/core#Concept"/>
        <skos:broader rdf:resource="http://data.ign.fr/id/codes/topo/typedezai/PAITransport"/>
        <skos:definition xml:lang="en">Developed space (presence of a compulsory water point) away from the roadways, especially highways, to allow users to stop and rest.Emprise of the area. The contours of the surface never rest on sections of road that represent the axis of pavements.</skos:definition>
        <skos:definition xml:lang="fr">Espace aménagé (présence d&apos;un point d&apos;eau obligatoire) à l &apos;écart des chaussées, notamment des autoroutes, pour permettre aux usagers de s&apos;arrêter et de se reposer.Emprise de l&apos;aire. Les contours de la surface ne s&apos;appuient jamais sur des tronçons de route qui représentent l&apos;axe des chaussées.</skos:definition>
        <skos:inScheme rdf:resource="http://data.ign.fr/id/codes/topo/typedezai/liste"/>
        <skos:prefLabel xml:lang="fr">aire de repos</skos:prefLabel>
        <skos:prefLabel xml:lang="en">rest area</skos:prefLabel>
    </owl:NamedIndividual>
    


    <!-- http://data.ign.fr/id/codes/topo/typedezai/AireDeService -->


    <owl:NamedIndividual rdf:about="http://data.ign.fr/id/codes/topo/typedezai/AireDeService">
        <rdf:type rdf:resource="http://data.ign.fr/def/topo#TypeDeZAI"/>
        <rdf:type rdf:resource="http://www.w3.org/2004/02/skos/core#Concept"/>
        <skos:broader rdf:resource="http://data.ign.fr/id/codes/topo/typedezai/PAITransport"/>
        <skos:definition xml:lang="fr">Espace aménagé à l&apos;écart des chaussées, notamment des autoroutes, pour permettre aux usagers de se ravitailler en carburant. Emprise de l&apos;aire. Les contours de la surface ne s&apos;appuient jamais sur des tronçons de route (qui représentent l&apos;axe des chaussées).</skos:definition>
        <skos:definition xml:lang="en">Space arranged away from roads, especially highways, to allow users to refuel. Emprise of the area. The contours of the surface never rest on sections of road (which represent the axis of pavements).</skos:definition>
        <skos:inScheme rdf:resource="http://data.ign.fr/id/codes/topo/typedezai/liste"/>
        <skos:prefLabel xml:lang="fr">aire de service</skos:prefLabel>
        <skos:prefLabel xml:lang="en">service area</skos:prefLabel>
    </owl:NamedIndividual>
    


    <!-- http://data.ign.fr/id/codes/topo/typedezai/Amer -->


    <owl:NamedIndividual rdf:about="http://data.ign.fr/id/codes/topo/typedezai/Amer">
        <rdf:type rdf:resource="http://data.ign.fr/def/topo#TypeDeZAI"/>
        <rdf:type rdf:resource="http://www.w3.org/2004/02/skos/core#Concept"/>
        <skos:broader rdf:resource="http://data.ign.fr/id/codes/topo/typedezai/PAIHydrographie"/>
        <skos:definition xml:lang="fr">Point de repère visible de la mer : amer, bouée, balise, phare, feu, tourelle.</skos:definition>
        <skos:definition xml:lang="en">Visible landmark of the sea: bitter, buoy, beacon, lighthouse, fire, turret.</skos:definition>
        <skos:inScheme rdf:resource="http://data.ign.fr/id/codes/topo/typedezai/liste"/>
        <skos:prefLabel xml:lang="fr">amer</skos:prefLabel>
        <skos:prefLabel xml:lang="en">seamark</skos:prefLabel>
    </owl:NamedIndividual>
    


    <!-- http://data.ign.fr/id/codes/topo/typedezai/Aquaculture -->


    <owl:NamedIndividual rdf:about="http://data.ign.fr/id/codes/topo/typedezai/Aquaculture">
        <rdf:type rdf:resource="http://data.ign.fr/def/topo#TypeDeZAI"/>
        <rdf:type rdf:resource="http://www.w3.org/2004/02/skos/core#Concept"/>
        <skos:broader rdf:resource="http://data.ign.fr/id/codes/topo/typedezai/PAIIndustrielCommercial"/>
        <skos:definition xml:lang="fr">Site aménagé pour l&apos;élevage piscicole ou la culture d&apos;espèces animales marines (coques, coquilles Saint-Jacques, huîtres, moules, palourdes,etc.) : bouchot, parc à huîtres, zone conchylicole, zone mytilicole, zone ostréicole. Toutes les zones de plus de 3 ha possédant des installations fixes de pêche et délimitées par des alignements de pieux, les parcs à huîtres, les bassins. Les installations de pêche au carrelet sont exclues.</skos:definition>
        <skos:definition xml:lang="en">Site developed for fish farming or the cultivation of marine animal species (hulls, scallops, oysters, mussels, clams, etc.): bouchot, oyster beds, shellfish growing area, mussel zone, oyster farming area. All areas of more than 3 ha with fixed fishing facilities and defined by pile alignments, oyster beds, ponds. The plaice fishing facilities are excluded.</skos:definition>
        <skos:inScheme rdf:resource="http://data.ign.fr/id/codes/topo/typedezai/liste"/>
        <skos:prefLabel xml:lang="en">aquaculture facilities</skos:prefLabel>
        <skos:prefLabel xml:lang="fr">installation d&apos;aquaculture</skos:prefLabel>
    </owl:NamedIndividual>
    


    <!-- http://data.ign.fr/id/codes/topo/typedezai/Arbre -->


    <owl:NamedIndividual rdf:about="http://data.ign.fr/id/codes/topo/typedezai/Arbre">
        <rdf:type rdf:resource="http://data.ign.fr/def/topo#TypeDeZAI"/>
        <rdf:type rdf:resource="http://www.w3.org/2004/02/skos/core#Concept"/>
        <skos:broader rdf:resource="http://data.ign.fr/id/codes/topo/typedezai/PAIEspaceNaturel"/>
        <skos:definition xml:lang="fr">Arbre nommé isolé, arbre remarquable.</skos:definition>
        <skos:definition xml:lang="en">Isolated named tree, remarkable tree.</skos:definition>
        <skos:inScheme rdf:resource="http://data.ign.fr/id/codes/topo/typedezai/liste"/>
        <skos:prefLabel xml:lang="fr">arbre</skos:prefLabel>
        <skos:prefLabel xml:lang="en">tree</skos:prefLabel>
    </owl:NamedIndividual>
    


    <!-- http://data.ign.fr/id/codes/topo/typedezai/Baie -->


    <owl:NamedIndividual rdf:about="http://data.ign.fr/id/codes/topo/typedezai/Baie">
        <rdf:type rdf:resource="http://data.ign.fr/def/topo#TypeDeZAI"/>
        <rdf:type rdf:resource="http://www.w3.org/2004/02/skos/core#Concept"/>
        <skos:broader rdf:resource="http://data.ign.fr/id/codes/topo/typedezai/PAIHydrographie"/>
        <skos:definition xml:lang="fr">Espace marin pénétrant entre les terres : anse, baie, calanque, crique, golfe.</skos:definition>
        <skos:definition xml:lang="en">Marine space penetrating between the grounds: cove, bay, cove, cove, gulf.</skos:definition>
        <skos:inScheme rdf:resource="http://data.ign.fr/id/codes/topo/typedezai/liste"/>
        <skos:prefLabel xml:lang="fr">baie</skos:prefLabel>
        <skos:prefLabel xml:lang="en">bay</skos:prefLabel>
    </owl:NamedIndividual>
    


    <!-- http://data.ign.fr/id/codes/topo/typedezai/Banc -->


    <owl:NamedIndividual rdf:about="http://data.ign.fr/id/codes/topo/typedezai/Banc">
        <rdf:type rdf:resource="http://data.ign.fr/def/topo#TypeDeZAI"/>
        <rdf:type rdf:resource="http://www.w3.org/2004/02/skos/core#Concept"/>
        <skos:broader rdf:resource="http://data.ign.fr/id/codes/topo/typedezai/PAIHydrographie"/>
        <skos:definition xml:lang="en">At sea or on a river, non-rocky underwater relief representing a potential danger for navigation: benches, shoals.</skos:definition>
        <skos:definition xml:lang="fr">En mer ou sur un fleuve, relief sous-marin non rocheux représentant un danger potentiel pour la navigation: bancs, hauts-fonds.</skos:definition>
        <skos:inScheme rdf:resource="http://data.ign.fr/id/codes/topo/typedezai/liste"/>
        <skos:prefLabel xml:lang="fr">banc</skos:prefLabel>
        <skos:prefLabel xml:lang="en">bank</skos:prefLabel>
    </owl:NamedIndividual>
    


    <!-- http://data.ign.fr/id/codes/topo/typedezai/Barrage -->


    <owl:NamedIndividual rdf:about="http://data.ign.fr/id/codes/topo/typedezai/Barrage">
        <rdf:type rdf:resource="http://data.ign.fr/def/topo#TypeDeZAI"/>
        <rdf:type rdf:resource="http://www.w3.org/2004/02/skos/core#Concept"/>
        <skos:broader rdf:resource="http://data.ign.fr/id/codes/topo/typedezai/PAITransport"/>
        <skos:definition xml:lang="en">Artificial obstacle placed across a watercourse: dam, lock, valve.</skos:definition>
        <skos:definition xml:lang="fr">Obstacle artificiel placé en travers d&apos;un cours d&apos;eau : barrage, écluse, vanne.</skos:definition>
        <skos:inScheme rdf:resource="http://data.ign.fr/id/codes/topo/typedezai/liste"/>
        <skos:narrowMatch rdf:resource="http://data.ign.fr/id/codes/topo/typedebatiment/Barrage"/>
        <skos:narrowMatch rdf:resource="http://data.ign.fr/id/codes/topo/typedebatiment/Ecluse"/>
        <skos:prefLabel xml:lang="en">barrage</skos:prefLabel>
        <skos:prefLabel xml:lang="fr">barrage</skos:prefLabel>
    </owl:NamedIndividual>
    


    <!-- http://data.ign.fr/id/codes/topo/typedezai/BarriereDePeage -->


    <owl:NamedIndividual rdf:about="http://data.ign.fr/id/codes/topo/typedezai/BarriereDePeage">
        <rdf:type rdf:resource="http://data.ign.fr/def/topo#TypeDeZAI"/>
        <rdf:type rdf:resource="http://www.w3.org/2004/02/skos/core#Concept"/>
        <skos:broader rdf:resource="http://data.ign.fr/id/codes/topo/typedezai/PAITransport"/>
        <skos:definition xml:lang="fr">Barrière de péage. Toutes les barrières de péage sont représentées, qu&apos;elles soient ou non accompagnées d&apos;un élargissement de la chaussée ou d&apos;un bâtiment : péage d&apos;autoroute, de pont, de route.</skos:definition>
        <skos:definition xml:lang="en">Toll barrier. All toll barriers are represented, whether or not accompanied by a widening of the roadway or a building: highway toll, bridge, road.</skos:definition>
        <skos:inScheme rdf:resource="http://data.ign.fr/id/codes/topo/typedezai/liste"/>
        <skos:prefLabel xml:lang="fr">barrière de péage</skos:prefLabel>
        <skos:prefLabel xml:lang="en">toll-gate</skos:prefLabel>
        <skos:relatedMatch rdf:resource="http://data.ign.fr/id/codes/topo/typedebatiment/Peage"/>
    </owl:NamedIndividual>
    


    <!-- http://data.ign.fr/id/codes/topo/typedezai/Borne -->


    <owl:NamedIndividual rdf:about="http://data.ign.fr/id/codes/topo/typedezai/Borne">
        <rdf:type rdf:resource="http://data.ign.fr/def/topo#TypeDeZAI"/>
        <rdf:type rdf:resource="http://www.w3.org/2004/02/skos/core#Concept"/>
        <skos:broader rdf:resource="http://data.ign.fr/id/codes/topo/typedezai/PAIAdministratifOuMilitaire"/>
        <skos:definition xml:lang="fr">Borne nommée : borne frontière, point de triangulation, point frontière.</skos:definition>
        <skos:definition xml:lang="en">Named terminal: boundary marker, triangulation point, boundary point.</skos:definition>
        <skos:inScheme rdf:resource="http://data.ign.fr/id/codes/topo/typedezai/liste"/>
        <skos:prefLabel xml:lang="fr">borne</skos:prefLabel>
        <skos:prefLabel xml:lang="en">marker</skos:prefLabel>
    </owl:NamedIndividual>
    


    <!-- http://data.ign.fr/id/codes/topo/typedezai/BureauDePoste -->


    <owl:NamedIndividual rdf:about="http://data.ign.fr/id/codes/topo/typedezai/BureauDePoste">
        <rdf:type rdf:resource="http://data.ign.fr/def/topo#TypeDeZAI"/>
        <rdf:type rdf:resource="http://www.w3.org/2004/02/skos/core#Concept"/>
        <skos:altLabel xml:lang="en">general post office</skos:altLabel>
        <skos:altLabel xml:lang="fr">hôtel des postes</skos:altLabel>
        <skos:broader rdf:resource="http://data.ign.fr/id/codes/topo/typedezai/PAIAdministratifOuMilitaire"/>
        <skos:definition xml:lang="fr">Bureau de poste ouvert au public : Bureau de poste, hôtel des postes. Seuls les bureaux de poste ouverts en permanence sont inclus. En général, dans les agglomérations, seules les postes centrales sont incluses.</skos:definition>
        <skos:definition xml:lang="en">Post Office open to the public: Post Office, Post Office. Only permanently open post offices are included. In general, in the agglomerations, only the central stations are included.</skos:definition>
        <skos:inScheme rdf:resource="http://data.ign.fr/id/codes/topo/typedezai/liste"/>
        <skos:prefLabel xml:lang="fr">bureau de poste</skos:prefLabel>
        <skos:prefLabel xml:lang="en">post office</skos:prefLabel>
    </owl:NamedIndividual>
    


    <!-- http://data.ign.fr/id/codes/topo/typedezai/Camping -->


    <owl:NamedIndividual rdf:about="http://data.ign.fr/id/codes/topo/typedezai/Camping">
        <rdf:type rdf:resource="http://data.ign.fr/def/topo#TypeDeZAI"/>
        <rdf:type rdf:resource="http://www.w3.org/2004/02/skos/core#Concept"/>
        <skos:broader rdf:resource="http://data.ign.fr/id/codes/topo/typedezai/PAICultureLoisirs"/>
        <skos:definition xml:lang="fr">Emplacement aménagé pour la pratique du camping d&apos;une superficie de plus de 2 ha.</skos:definition>
        <skos:definition xml:lang="en">Site arranged for the practice of the camping of an area of more than 2 ha.</skos:definition>
        <skos:inScheme rdf:resource="http://data.ign.fr/id/codes/topo/typedezai/liste"/>
        <skos:prefLabel xml:lang="fr">camping</skos:prefLabel>
        <skos:prefLabel xml:lang="en">camping grounds</skos:prefLabel>
    </owl:NamedIndividual>
    


    <!-- http://data.ign.fr/id/codes/topo/typedezai/Canal -->


    <owl:NamedIndividual rdf:about="http://data.ign.fr/id/codes/topo/typedezai/Canal">
        <rdf:type rdf:resource="http://data.ign.fr/def/topo#TypeDeZAI"/>
        <rdf:type rdf:resource="http://www.w3.org/2004/02/skos/core#Concept"/>
        <skos:broader rdf:resource="http://data.ign.fr/id/codes/topo/typedezai/PAIHydrographie"/>
        <skos:definition xml:lang="en">Artificial water course: old canal, reach, canal, ditch, channel.</skos:definition>
        <skos:definition xml:lang="fr">Cours d&apos;eau artificiel : ancien canal, bief, canal, fossé, rigole.</skos:definition>
        <skos:inScheme rdf:resource="http://data.ign.fr/id/codes/topo/typedezai/liste"/>
        <skos:prefLabel xml:lang="fr">canal</skos:prefLabel>
        <skos:prefLabel xml:lang="en">channel</skos:prefLabel>
    </owl:NamedIndividual>
    


    <!-- http://data.ign.fr/id/codes/topo/typedezai/Carrefour -->


    <owl:NamedIndividual rdf:about="http://data.ign.fr/id/codes/topo/typedezai/Carrefour">
        <rdf:type rdf:resource="http://data.ign.fr/def/topo#TypeDeZAI"/>
        <rdf:type rdf:resource="http://www.w3.org/2004/02/skos/core#Concept"/>
        <skos:broader rdf:resource="http://data.ign.fr/id/codes/topo/typedezai/PAITransport"/>
        <skos:definition xml:lang="en">Node of the road network: road junction, interchange, roundabout.</skos:definition>
        <skos:definition xml:lang="fr">Noeud du réseau routier : carrefour routier, échangeur, rond-point.</skos:definition>
        <skos:inScheme rdf:resource="http://data.ign.fr/id/codes/topo/typedezai/liste"/>
        <skos:prefLabel xml:lang="fr">carrefour</skos:prefLabel>
        <skos:prefLabel xml:lang="en">crossroads</skos:prefLabel>
    </owl:NamedIndividual>
    


    <!-- http://data.ign.fr/id/codes/topo/typedezai/CaserneDePompiers -->


    <owl:NamedIndividual rdf:about="http://data.ign.fr/id/codes/topo/typedezai/CaserneDePompiers">
        <rdf:type rdf:resource="http://data.ign.fr/def/topo#TypeDeZAI"/>
        <rdf:type rdf:resource="http://www.w3.org/2004/02/skos/core#Concept"/>
        <skos:broader rdf:resource="http://data.ign.fr/id/codes/topo/typedezai/PAIAdministratifOuMilitaire"/>
        <skos:definition xml:lang="en">Building with or without an office or a permanence and which is entirely concerned by the activity of the body of the Fire-fighters.</skos:definition>
        <skos:definition xml:lang="fr">Bâtiment ayant ou non un bureau ou une permanence et qui est entièment concerné par l&apos;activité du corps des Sapeurs-Pompiers.</skos:definition>
        <skos:inScheme rdf:resource="http://data.ign.fr/id/codes/topo/typedezai/liste"/>
        <skos:prefLabel xml:lang="fr">caserne de pompiers</skos:prefLabel>
        <skos:prefLabel xml:lang="en">fire station</skos:prefLabel>
    </owl:NamedIndividual>
    


    <!-- http://data.ign.fr/id/codes/topo/typedezai/CentraleElectrique -->


    <owl:NamedIndividual rdf:about="http://data.ign.fr/id/codes/topo/typedezai/CentraleElectrique">
        <rdf:type rdf:resource="http://data.ign.fr/def/topo#TypeDeZAI"/>
        <rdf:type rdf:resource="http://www.w3.org/2004/02/skos/core#Concept"/>
        <skos:broader rdf:resource="http://data.ign.fr/id/codes/topo/typedezai/PAIIndustrielCommercial"/>
        <skos:definition xml:lang="en">Plant where electric power is produced: hydroelectric plant, thermal power station, nuclear power station. Underground power plants are excluded.</skos:definition>
        <skos:definition xml:lang="fr">Usine où l&apos;on produit de l&apos;énergie électrique : centrale hydroélectrique, centrale thermique, centrale nucléaire. Les centrales électriques souterraines sont exclues.</skos:definition>
        <skos:inScheme rdf:resource="http://data.ign.fr/id/codes/topo/typedezai/liste"/>
        <skos:prefLabel xml:lang="fr">centrale électrique</skos:prefLabel>
        <skos:prefLabel xml:lang="en">power station</skos:prefLabel>
    </owl:NamedIndividual>
    


    <!-- http://data.ign.fr/id/codes/topo/typedezai/Chemin -->


    <owl:NamedIndividual rdf:about="http://data.ign.fr/id/codes/topo/typedezai/Chemin">
        <rdf:type rdf:resource="http://data.ign.fr/def/topo#TypeDeZAI"/>
        <rdf:type rdf:resource="http://www.w3.org/2004/02/skos/core#Concept"/>
        <skos:broader rdf:resource="http://data.ign.fr/id/codes/topo/typedezai/PAITransport"/>
        <skos:definition xml:lang="en">Non-road communication path: driveway, path, forest laie, path.</skos:definition>
        <skos:definition xml:lang="fr">Voie de communication non routière : allée, chemin, laie forestière, sentier.</skos:definition>
        <skos:inScheme rdf:resource="http://data.ign.fr/id/codes/topo/typedezai/liste"/>
        <skos:prefLabel xml:lang="fr">chemin</skos:prefLabel>
        <skos:prefLabel xml:lang="en">trail</skos:prefLabel>
    </owl:NamedIndividual>
    


    <!-- http://data.ign.fr/id/codes/topo/typedezai/Construction -->


    <owl:NamedIndividual rdf:about="http://data.ign.fr/id/codes/topo/typedezai/Construction">
        <rdf:type rdf:resource="http://data.ign.fr/def/topo#TypeDeZAI"/>
        <rdf:type rdf:resource="http://www.w3.org/2004/02/skos/core#Concept"/>
        <skos:broader rdf:resource="http://data.ign.fr/id/codes/topo/typedezai/PAICultureLoisirs"/>
        <skos:definition xml:lang="en">Construction named inhabited or associated with a group of houses: various construction, dovecote, windmill.</skos:definition>
        <skos:definition xml:lang="fr">Construction nommée habitée ou associée à un groupe d&apos;habitations : construction diverse, pigeonnier, moulin à vent.</skos:definition>
        <skos:inScheme rdf:resource="http://data.ign.fr/id/codes/topo/typedezai/liste"/>
        <skos:prefLabel xml:lang="fr">construction nommée</skos:prefLabel>
        <skos:prefLabel xml:lang="en">named building</skos:prefLabel>
    </owl:NamedIndividual>
    


    <!-- http://data.ign.fr/id/codes/topo/typedezai/Croix -->


    <owl:NamedIndividual rdf:about="http://data.ign.fr/id/codes/topo/typedezai/Croix">
        <rdf:type rdf:resource="http://data.ign.fr/def/topo#TypeDeZAI"/>
        <rdf:type rdf:resource="http://www.w3.org/2004/02/skos/core#Concept"/>
        <skos:broader rdf:resource="http://data.ign.fr/id/codes/topo/typedezai/PAIReligieux"/>
        <skos:definition xml:lang="fr">Monument religieux : croix, calvaire, vierge, statue religieuse.</skos:definition>
        <skos:definition xml:lang="en">Religious monument: cross, calvary, virgin, religious statue.</skos:definition>
        <skos:inScheme rdf:resource="http://data.ign.fr/id/codes/topo/typedezai/liste"/>
        <skos:prefLabel xml:lang="fr">croix</skos:prefLabel>
        <skos:prefLabel xml:lang="en">cross</skos:prefLabel>
    </owl:NamedIndividual>
    


    <!-- http://data.ign.fr/id/codes/topo/typedezai/CulteCatholiqueOuOrthodoxe -->


    <owl:NamedIndividual rdf:about="http://data.ign.fr/id/codes/topo/typedezai/CulteCatholiqueOuOrthodoxe">
        <rdf:type rdf:resource="http://data.ign.fr/def/topo#TypeDeZAI"/>
        <rdf:type rdf:resource="http://www.w3.org/2004/02/skos/core#Concept"/>
        <skos:broader rdf:resource="http://data.ign.fr/id/codes/topo/typedezai/PAIReligieux"/>
        <skos:definition xml:lang="en">Building reserved for the exercise of Catholic or Orthodox worship: church, cathedral, basilica, chapel, abbey, oratory.</skos:definition>
        <skos:definition xml:lang="fr">Bâtiment réservé à l&apos;exercice du culte catholique ou orthodoxe : église, cathédrale, basilique, chapelle, abbaye, oratoire.</skos:definition>
        <skos:inScheme rdf:resource="http://data.ign.fr/id/codes/topo/typedezai/liste"/>
        <skos:prefLabel xml:lang="en">catholic or orthodox building</skos:prefLabel>
        <skos:prefLabel xml:lang="fr">édifice religieux catholique ou orthodoxe</skos:prefLabel>
    </owl:NamedIndividual>
    


    <!-- http://data.ign.fr/id/codes/topo/typedezai/CulteDivers -->


    <owl:NamedIndividual rdf:about="http://data.ign.fr/id/codes/topo/typedezai/CulteDivers">
        <rdf:type rdf:resource="http://data.ign.fr/def/topo#TypeDeZAI"/>
        <rdf:type rdf:resource="http://www.w3.org/2004/02/skos/core#Concept"/>
        <skos:broader rdf:resource="http://data.ign.fr/id/codes/topo/typedezai/PAIReligieux"/>
        <skos:definition xml:lang="en">Building reserved for religious worship other than Christian, Islamic or Jewish: Buddhist temple, Hindu temple.</skos:definition>
        <skos:definition xml:lang="fr">Bâtiment réservé à l&apos;exercice d&apos;un culte religieux autre que chrétien, islamique ou israélite : temple bouddhiste, temple hindouiste.</skos:definition>
        <skos:inScheme rdf:resource="http://data.ign.fr/id/codes/topo/typedezai/liste"/>
        <skos:prefLabel xml:lang="en">other religious building</skos:prefLabel>
        <skos:prefLabel xml:lang="fr">édifice religieux divers</skos:prefLabel>
    </owl:NamedIndividual>
    


    <!-- http://data.ign.fr/id/codes/topo/typedezai/CulteIslamique -->


    <owl:NamedIndividual rdf:about="http://data.ign.fr/id/codes/topo/typedezai/CulteIslamique">
        <rdf:type rdf:resource="http://data.ign.fr/def/topo#TypeDeZAI"/>
        <rdf:type rdf:resource="http://www.w3.org/2004/02/skos/core#Concept"/>
        <skos:broader rdf:resource="http://data.ign.fr/id/codes/topo/typedezai/PAIReligieux"/>
        <skos:definition xml:lang="en">Building reserved for the exercise of Islamic worship: mosque.</skos:definition>
        <skos:definition xml:lang="fr">Bâtiment réservé à l&apos;exercice du culte islamique : mosquée.</skos:definition>
        <skos:inScheme rdf:resource="http://data.ign.fr/id/codes/topo/typedezai/liste"/>
        <skos:prefLabel xml:lang="en">moslem religious building</skos:prefLabel>
        <skos:prefLabel xml:lang="fr">édifice religieux islamique</skos:prefLabel>
    </owl:NamedIndividual>
    


    <!-- http://data.ign.fr/id/codes/topo/typedezai/CulteIsraelite -->


    <owl:NamedIndividual rdf:about="http://data.ign.fr/id/codes/topo/typedezai/CulteIsraelite">
        <rdf:type rdf:resource="http://data.ign.fr/def/topo#TypeDeZAI"/>
        <rdf:type rdf:resource="http://www.w3.org/2004/02/skos/core#Concept"/>
        <skos:broader rdf:resource="http://data.ign.fr/id/codes/topo/typedezai/PAIReligieux"/>
        <skos:definition xml:lang="en">Building reserved for the exercise of Jewish worship: synagogue.</skos:definition>
        <skos:definition xml:lang="fr">Bâtiment réservé à l&apos;exercice du culte israélite : synagogue.</skos:definition>
        <skos:inScheme rdf:resource="http://data.ign.fr/id/codes/topo/typedezai/liste"/>
        <skos:prefLabel xml:lang="en">jewish religious building</skos:prefLabel>
        <skos:prefLabel xml:lang="fr">édifice religieux israélite</skos:prefLabel>
    </owl:NamedIndividual>
    


    <!-- http://data.ign.fr/id/codes/topo/typedezai/CulteProtestant -->


    <owl:NamedIndividual rdf:about="http://data.ign.fr/id/codes/topo/typedezai/CulteProtestant">
        <rdf:type rdf:resource="http://data.ign.fr/def/topo#TypeDeZAI"/>
        <rdf:type rdf:resource="http://www.w3.org/2004/02/skos/core#Concept"/>
        <skos:broader rdf:resource="http://data.ign.fr/id/codes/topo/typedezai/PAIReligieux"/>
        <skos:definition xml:lang="en">Building reserved for the practice of Protestant worship: temple (Protestant), Reformed church.</skos:definition>
        <skos:definition xml:lang="fr">Bâtiment réservé à l&apos;exercice du culte protestant : temple (protestant), église réformée.</skos:definition>
        <skos:inScheme rdf:resource="http://data.ign.fr/id/codes/topo/typedezai/liste"/>
        <skos:prefLabel xml:lang="en">protestant building</skos:prefLabel>
        <skos:prefLabel xml:lang="fr">édifice religieux protestant</skos:prefLabel>
    </owl:NamedIndividual>
    


    <!-- http://data.ign.fr/id/codes/topo/typedezai/Digue -->


    <owl:NamedIndividual rdf:about="http://data.ign.fr/id/codes/topo/typedezai/Digue">
        <rdf:type rdf:resource="http://data.ign.fr/def/topo#TypeDeZAI"/>
        <rdf:type rdf:resource="http://www.w3.org/2004/02/skos/core#Concept"/>
        <skos:broader rdf:resource="http://data.ign.fr/id/codes/topo/typedezai/PAICultureLoisirs"/>
        <skos:definition xml:lang="fr">Digue, môle, jetée.</skos:definition>
        <skos:definition xml:lang="en">Dike, breakwater, jetty.</skos:definition>
        <skos:inScheme rdf:resource="http://data.ign.fr/id/codes/topo/typedezai/liste"/>
        <skos:prefLabel xml:lang="fr">digue</skos:prefLabel>
        <skos:prefLabel xml:lang="en">dike</skos:prefLabel>
    </owl:NamedIndividual>
    


    <!-- http://data.ign.fr/id/codes/topo/typedezai/Dolmen -->


    <owl:NamedIndividual rdf:about="http://data.ign.fr/id/codes/topo/typedezai/Dolmen">
        <rdf:type rdf:resource="http://data.ign.fr/def/topo#TypeDeZAI"/>
        <rdf:type rdf:resource="http://www.w3.org/2004/02/skos/core#Concept"/>
        <skos:broader rdf:resource="http://data.ign.fr/id/codes/topo/typedezai/PAICultureLoisirs"/>
        <skos:definition xml:lang="en">Megalithic monument formed by a large flat stone resting on other vertically standing stones. Covered walkways are included.</skos:definition>
        <skos:definition xml:lang="fr">Monument mégalithique formé d&apos;une grande pierre plate posée sur d&apos;autres pierres dressées verticalement. Les allées couvertes sont incluses.</skos:definition>
        <skos:inScheme rdf:resource="http://data.ign.fr/id/codes/topo/typedezai/liste"/>
        <skos:prefLabel xml:lang="en">dolmen</skos:prefLabel>
        <skos:prefLabel xml:lang="fr">dolmen</skos:prefLabel>
    </owl:NamedIndividual>
    


    <!-- http://data.ign.fr/id/codes/topo/typedezai/Echangeur -->


    <owl:NamedIndividual rdf:about="http://data.ign.fr/id/codes/topo/typedezai/Echangeur">
        <rdf:type rdf:resource="http://data.ign.fr/def/topo#TypeDeZAI"/>
        <rdf:type rdf:resource="http://www.w3.org/2004/02/skos/core#Concept"/>
        <skos:broader rdf:resource="http://data.ign.fr/id/codes/topo/typedezai/PAITransport"/>
        <skos:definition xml:lang="en">Node of the divided road network. Motorway interchange bearing a name.</skos:definition>
        <skos:definition xml:lang="fr">Noeud du réseau routier à chaussées séparées. Échangeur autoroutier portant un nom.</skos:definition>
        <skos:inScheme rdf:resource="http://data.ign.fr/id/codes/topo/typedezai/liste"/>
        <skos:prefLabel xml:lang="en">interchange</skos:prefLabel>
        <skos:prefLabel xml:lang="fr">échangeur</skos:prefLabel>
    </owl:NamedIndividual>
    


    <!-- http://data.ign.fr/id/codes/topo/typedezai/Embouchure -->


    <owl:NamedIndividual rdf:about="http://data.ign.fr/id/codes/topo/typedezai/Embouchure">
        <rdf:type rdf:resource="http://data.ign.fr/def/topo#TypeDeZAI"/>
        <rdf:type rdf:resource="http://www.w3.org/2004/02/skos/core#Concept"/>
        <skos:broader rdf:resource="http://data.ign.fr/id/codes/topo/typedezai/PAIHydrographie"/>
        <skos:definition xml:lang="fr">Embouchure d&apos;un fleuve : delta, embouchure, estuaire.</skos:definition>
        <skos:definition xml:lang="en">Mouth of a river: delta, mouth, estuary.</skos:definition>
        <skos:inScheme rdf:resource="http://data.ign.fr/id/codes/topo/typedezai/liste"/>
        <skos:prefLabel xml:lang="fr">embouchure</skos:prefLabel>
        <skos:prefLabel xml:lang="en">mouth</skos:prefLabel>
    </owl:NamedIndividual>
    


    <!-- http://data.ign.fr/id/codes/topo/typedezai/EnceinteMilitaire -->


    <owl:NamedIndividual rdf:about="http://data.ign.fr/id/codes/topo/typedezai/EnceinteMilitaire">
        <rdf:type rdf:resource="http://data.ign.fr/def/topo#TypeDeZAI"/>
        <rdf:type rdf:resource="http://www.w3.org/2004/02/skos/core#Concept"/>
        <skos:broader rdf:resource="http://data.ign.fr/id/codes/topo/typedezai/PAIAdministratifOuMilitaire"/>
        <skos:definition xml:lang="en">Area permanently reserved for troop gatherings of all arms, either for maneuvers, exercises (training camp), or for tests, studies: base, camp, barracks, deposit of equipment, permanent ground of training, barracks of CRS, barracks of mobile gendarmes, ... The ranges are excluded as well as the properties of the army which are not indicated in any way on the ground (neither fences, barriers, nor signs,. ..) and not subject to any particular restriction.</skos:definition>
        <skos:definition xml:lang="fr">Zone en permanence réservée pour les rassemblements de troupes de toutes les armes, soit pour des manoeuvres, des exercices (camp d&apos;instruction), soit pour des essais, des études: base, camp, caserne, dépôt de matériels, terrain permanent d&apos;entrainement, caserne de CRS, caserne de gendarmes mobiles, ... Les champs de tir sont exclus ainsi que les propriétés de l&apos;armée qui ne sont indiquées d&apos;aucune manière sur le terrain (ni clôtures, ni barrières, ni pancartes, ...) et ne faisant l&apos;objet d&apos;aucune restriction particulière.</skos:definition>
        <skos:inScheme rdf:resource="http://data.ign.fr/id/codes/topo/typedezai/liste"/>
        <skos:prefLabel xml:lang="fr">enceinte militaire</skos:prefLabel>
        <skos:prefLabel xml:lang="en">military area</skos:prefLabel>
    </owl:NamedIndividual>
    


    <!-- http://data.ign.fr/id/codes/topo/typedezai/EnseignementPrimaire -->


    <owl:NamedIndividual rdf:about="http://data.ign.fr/id/codes/topo/typedezai/EnseignementPrimaire">
        <rdf:type rdf:resource="http://data.ign.fr/def/topo#TypeDeZAI"/>
        <rdf:type rdf:resource="http://www.w3.org/2004/02/skos/core#Concept"/>
        <skos:broader rdf:resource="http://data.ign.fr/id/codes/topo/typedezai/PAIScienceEnseignement"/>
        <skos:definition xml:lang="en">Institution devoted to nursery and primary education: primary school, nursery school, school group, Institut Médico-Pédagogique (I.M.P.). All primary schools, public, religious or private, having a simple contract or association with the State are included. The nurseries are excluded.</skos:definition>
        <skos:definition xml:lang="fr">Établissement consacré à l&apos;enseignement maternel et primaire : école primaire, école maternelle, groupe scolaire, Institut Médico-Pédagogique (I.M.P.). Tous les établissements d&apos;enseignement primaire, publics, confessionnels ou privés, ayant un contrat simple ou d&apos;association avec l&apos;État sont inclus. Les crèches sont exclues.</skos:definition>
        <skos:inScheme rdf:resource="http://data.ign.fr/id/codes/topo/typedezai/liste"/>
        <skos:prefLabel xml:lang="en">nursery or elementary school</skos:prefLabel>
        <skos:prefLabel xml:lang="fr">établissement d&apos;enseignement maternel ou primaire</skos:prefLabel>
    </owl:NamedIndividual>
    


    <!-- http://data.ign.fr/id/codes/topo/typedezai/EnseignementSecondaire -->


    <owl:NamedIndividual rdf:about="http://data.ign.fr/id/codes/topo/typedezai/EnseignementSecondaire">
        <rdf:type rdf:resource="http://data.ign.fr/def/topo#TypeDeZAI"/>
        <rdf:type rdf:resource="http://www.w3.org/2004/02/skos/core#Concept"/>
        <skos:broader rdf:resource="http://data.ign.fr/id/codes/topo/typedezai/PAIScienceEnseignement"/>
        <skos:definition xml:lang="en">Establishment devoted to secondary education: middle school, high school, Center for Help by Work (C.A.T.), Professional Training of Adults (F.P.A.), Medical-Professional Institute (I.M.Pro.). All public, religious or private secondary schools with a simple contract or association with the state are included.</skos:definition>
        <skos:definition xml:lang="fr">Établissement consacré à l&apos;enseignement secondaire : collège, lycée, Centre d&apos;Aide par le Travail (C.A.T.), Formation Professionnelle des Adultes (F.P.A.), Institut Médico-Professionnel (I.M.Pro.). Tous les établissements d&apos;enseignement secondaire publics, confessionnels ou privés, ayant un contrat simple ou d&apos;association avec l&apos;État sont inclus.</skos:definition>
        <skos:inScheme rdf:resource="http://data.ign.fr/id/codes/topo/typedezai/liste"/>
        <skos:prefLabel xml:lang="en">secondary education school</skos:prefLabel>
        <skos:prefLabel xml:lang="fr">établissement d&apos;enseignement secondaire</skos:prefLabel>
    </owl:NamedIndividual>
    


    <!-- http://data.ign.fr/id/codes/topo/typedezai/EnseignementSuperieur -->


    <owl:NamedIndividual rdf:about="http://data.ign.fr/id/codes/topo/typedezai/EnseignementSuperieur">
        <rdf:type rdf:resource="http://data.ign.fr/def/topo#TypeDeZAI"/>
        <rdf:type rdf:resource="http://www.w3.org/2004/02/skos/core#Concept"/>
        <skos:broader rdf:resource="http://data.ign.fr/id/codes/topo/typedezai/PAIScienceEnseignement"/>
        <skos:definition xml:lang="en">Institution devoted to higher education: faculty, university center, institute, grande école, etc. All public, religious or private higher education institutions with a simple contract or association with the state are included. Evening classes, cities and university restaurants are excluded.</skos:definition>
        <skos:definition xml:lang="fr">Établissement consacré à l&apos;enseignement supérieur : faculté, centre universitaire, institut, grande école,etc. Tous les établissements d&apos;enseignement supérieur publics, confessionnels ou privés, ayant un contrat simple ou d&apos;association avec l&apos;État sont inclus. Les cours du soir, les cités et les restaurants universitaires sont exclus.</skos:definition>
        <skos:inScheme rdf:resource="http://data.ign.fr/id/codes/topo/typedezai/liste"/>
        <skos:prefLabel xml:lang="en">postsecondary education school</skos:prefLabel>
        <skos:prefLabel xml:lang="fr">établissement d&apos;enseignement supérieur</skos:prefLabel>
    </owl:NamedIndividual>
    


    <!-- http://data.ign.fr/id/codes/topo/typedezai/EspaceMaritime -->


    <owl:NamedIndividual rdf:about="http://data.ign.fr/id/codes/topo/typedezai/EspaceMaritime">
        <rdf:type rdf:resource="http://data.ign.fr/def/topo#TypeDeZAI"/>
        <rdf:type rdf:resource="http://www.w3.org/2004/02/skos/core#Concept"/>
        <skos:broader rdf:resource="http://data.ign.fr/id/codes/topo/typedezai/PAIHydrographie"/>
        <skos:definition xml:lang="fr">Espace maritime, mer, océan, passe.</skos:definition>
        <skos:definition xml:lang="en">Maritime area, sea, ocean, pass.</skos:definition>
        <skos:inScheme rdf:resource="http://data.ign.fr/id/codes/topo/typedezai/liste"/>
        <skos:prefLabel xml:lang="fr">espace maritime</skos:prefLabel>
        <skos:prefLabel xml:lang="en">maritime feature</skos:prefLabel>
    </owl:NamedIndividual>
    


    <!-- http://data.ign.fr/id/codes/topo/typedezai/EspacePublic -->


    <owl:NamedIndividual rdf:about="http://data.ign.fr/id/codes/topo/typedezai/EspacePublic">
        <rdf:type rdf:resource="http://data.ign.fr/def/topo#TypeDeZAI"/>
        <rdf:type rdf:resource="http://www.w3.org/2004/02/skos/core#Concept"/>
        <skos:broader rdf:resource="http://data.ign.fr/id/codes/topo/typedezai/PAICultureLoisirs"/>
        <skos:definition xml:lang="fr">Large espace découvert urbain désigné par un toponyme où aboutissent plusieurs rues, fermé à la circulation automobile, constituant un lieu remarquable : place, square, jardin, parc, parc communal, parc intercommunal, parc départemental, parc interdépartemental. Seuls les espaces publics possédant un toponyme sont retenus. Les parcs à vocation commerciale sont exclus (voir la valeur &apos;Parc de loisirs&apos;), de même que les parcs naturels (réserves, parcs nationaux, parcs naturels régionaux) qui sont traités en PAI_ESPACE_NATUREL.</skos:definition>
        <skos:definition xml:lang="en">Large open space urban designated by a toponym where end several streets, closed to traffic, constituting a remarkable place: square, square, garden, park, communal park, intercommunal park, departmental park, interdepartmental park. Only public spaces with a toponym are retained. The commercial parks are excluded (see the value &apos;Leisure park&apos;), as well as the natural parks (reserves, national parks, regional natural parks) which are treated in PAI_ESPACE_NATUREL.</skos:definition>
        <skos:inScheme rdf:resource="http://data.ign.fr/id/codes/topo/typedezai/liste"/>
        <skos:prefLabel xml:lang="fr">espace public nommé</skos:prefLabel>
        <skos:prefLabel xml:lang="en">named public area</skos:prefLabel>
    </owl:NamedIndividual>
    


    <!-- http://data.ign.fr/id/codes/topo/typedezai/EtablissementHospitalier -->


    <owl:NamedIndividual rdf:about="http://data.ign.fr/id/codes/topo/typedezai/EtablissementHospitalier">
        <rdf:type rdf:resource="http://data.ign.fr/def/topo#TypeDeZAI"/>
        <rdf:type rdf:resource="http://www.w3.org/2004/02/skos/core#Concept"/>
        <skos:broader rdf:resource="http://data.ign.fr/id/codes/topo/typedezai/PAISante"/>
        <skos:definition xml:lang="en">Public or private institution that receives or deals for a limited time the sick, wounded and women in childbirth: hospital, sanatorium, hospice, health center, dispensary, day hospital, psychiatric hospital, etc. All facilities providing care and accommodation or care only are included. Retirement homes that do not have a health center are excluded.</skos:definition>
        <skos:definition xml:lang="fr">Établissement public ou privé qui reçoit ou traite pendant un temps limité les malades, les blessés et les femmes en couches : hôpital, sanatorium, hospice, centre de soins, dispensaire, hôpital de jour, hôpital psychiatrique, etc. Tous les établissements assurant les soins et l&apos;hébergement ou les soins seulement sont inclus. Les maisons de retraite ne possédant pas de centre de soins sont exclues.</skos:definition>
        <skos:inScheme rdf:resource="http://data.ign.fr/id/codes/topo/typedezai/liste"/>
        <skos:prefLabel xml:lang="en">healthcare facility</skos:prefLabel>
        <skos:prefLabel xml:lang="fr">établissement hospitalier</skos:prefLabel>
    </owl:NamedIndividual>
    


    <!-- http://data.ign.fr/id/codes/topo/typedezai/EtablissementPenitenciaire -->


    <owl:NamedIndividual rdf:about="http://data.ign.fr/id/codes/topo/typedezai/EtablissementPenitenciaire">
        <rdf:type rdf:resource="http://data.ign.fr/def/topo#TypeDeZAI"/>
        <rdf:type rdf:resource="http://www.w3.org/2004/02/skos/core#Concept"/>
        <skos:broader rdf:resource="http://data.ign.fr/id/codes/topo/typedezai/PAIAdministratifOuMilitaire"/>
        <skos:definition xml:lang="en">Enclosed institution equipped to receive offenders sentenced to deprivation of liberty or inmates awaiting trial: prison. The annexes are excluded.</skos:definition>
        <skos:definition xml:lang="fr">Établissement clos aménagé pour recevoir des délinquants condamnés à une peine privative de liberté ou des détenus en instance de jugement: maison d&apos;arrêt, prison. Les annexes sont exclues.</skos:definition>
        <skos:inScheme rdf:resource="http://data.ign.fr/id/codes/topo/typedezai/liste"/>
        <skos:prefLabel xml:lang="en">penitentiary</skos:prefLabel>
        <skos:prefLabel xml:lang="fr">établissement pénitenciaire</skos:prefLabel>
    </owl:NamedIndividual>
    


    <!-- http://data.ign.fr/id/codes/topo/typedezai/EtablissementThermal -->


    <owl:NamedIndividual rdf:about="http://data.ign.fr/id/codes/topo/typedezai/EtablissementThermal">
        <rdf:type rdf:resource="http://data.ign.fr/def/topo#TypeDeZAI"/>
        <rdf:type rdf:resource="http://www.w3.org/2004/02/skos/core#Concept"/>
        <skos:broader rdf:resource="http://data.ign.fr/id/codes/topo/typedezai/PAISante"/>
        <skos:definition xml:lang="en">Establishment where medicinal waters are used (mineral waters, hot or not): thermal establishment, thalassotherapy center. Only establishments approved by the Social Security are included.</skos:definition>
        <skos:definition xml:lang="fr">Établissement où l&apos;on utilise les eaux médicinales (eaux minérales, chaudes ou non) : établissement thermal, centre de thalassothérapie. Seuls sont inclus les établissements agréés par la Sécurité Sociale.</skos:definition>
        <skos:inScheme rdf:resource="http://data.ign.fr/id/codes/topo/typedezai/liste"/>
        <skos:prefLabel xml:lang="en">health resort</skos:prefLabel>
        <skos:prefLabel xml:lang="fr">établissement thermal</skos:prefLabel>
    </owl:NamedIndividual>
    


    <!-- http://data.ign.fr/id/codes/topo/typedezai/GareFretUniquement -->


    <owl:NamedIndividual rdf:about="http://data.ign.fr/id/codes/topo/typedezai/GareFretUniquement">
        <rdf:type rdf:resource="http://data.ign.fr/def/topo#TypeDeZAI"/>
        <rdf:type rdf:resource="http://www.w3.org/2004/02/skos/core#Concept"/>
        <skos:broader rdf:resource="http://data.ign.fr/id/codes/topo/typedezai/PAITransport"/>
        <skos:definition xml:lang="en">Railway establishment providing a commercial merchandise service: freight station, service point. Air or sea freight is excluded.</skos:definition>
        <skos:definition xml:lang="fr">Établissement ferroviaire assurant un service commercial de marchandises : gare de fret, point de desserte. Le fret aérien ou maritime est exclu.</skos:definition>
        <skos:inScheme rdf:resource="http://data.ign.fr/id/codes/topo/typedezai/liste"/>
        <skos:prefLabel xml:lang="fr">gare de fret</skos:prefLabel>
        <skos:prefLabel xml:lang="en">goods station</skos:prefLabel>
    </owl:NamedIndividual>
    


    <!-- http://data.ign.fr/id/codes/topo/typedezai/GareRoutiere -->


    <owl:NamedIndividual rdf:about="http://data.ign.fr/id/codes/topo/typedezai/GareRoutiere">
        <rdf:type rdf:resource="http://data.ign.fr/def/topo#TypeDeZAI"/>
        <rdf:type rdf:resource="http://www.w3.org/2004/02/skos/core#Concept"/>
        <skos:broader rdf:resource="http://data.ign.fr/id/codes/topo/typedezai/PAITransport"/>
        <skos:definition xml:lang="en">All facilities intended for the loading and unloading of passengers by bus or bus at a specific point. The bus stations of city buses, school buses, RATP and bus depots are not included.</skos:definition>
        <skos:definition xml:lang="fr">Ensemble des installations destinées à l&apos;embarquement et au débarquement de voyageurs en car ou en bus en un point déterminé. Ne sont pas retenues les gares routières des bus de ville, des bus scolaires, de la RATP et les dépôts de bus.</skos:definition>
        <skos:inScheme rdf:resource="http://data.ign.fr/id/codes/topo/typedezai/liste"/>
        <skos:prefLabel xml:lang="en">bus station</skos:prefLabel>
        <skos:prefLabel xml:lang="fr">gare routière</skos:prefLabel>
    </owl:NamedIndividual>
    


    <!-- http://data.ign.fr/id/codes/topo/typedezai/GareVoyageursEtFret -->


    <owl:NamedIndividual rdf:about="http://data.ign.fr/id/codes/topo/typedezai/GareVoyageursEtFret">
        <rdf:type rdf:resource="http://data.ign.fr/def/topo#TypeDeZAI"/>
        <rdf:type rdf:resource="http://www.w3.org/2004/02/skos/core#Concept"/>
        <skos:broader rdf:resource="http://data.ign.fr/id/codes/topo/typedezai/PAITransport"/>
        <skos:definition xml:lang="en">Railway establishment providing a commercial service for passengers and goods (Only the main building open to the public)</skos:definition>
        <skos:definition xml:lang="fr">Établissement ferroviaire assurant un service commercial de voyageurs et de marchandises.(Uniquement le bâtiment principal ouvert au public.)</skos:definition>
        <skos:inScheme rdf:resource="http://data.ign.fr/id/codes/topo/typedezai/liste"/>
        <skos:prefLabel xml:lang="fr">gare de voyageurs et fret</skos:prefLabel>
        <skos:prefLabel xml:lang="en">passengers and goods station</skos:prefLabel>
    </owl:NamedIndividual>
    


    <!-- http://data.ign.fr/id/codes/topo/typedezai/GareVoyageursUniquement -->


    <owl:NamedIndividual rdf:about="http://data.ign.fr/id/codes/topo/typedezai/GareVoyageursUniquement">
        <rdf:type rdf:resource="http://data.ign.fr/def/topo#TypeDeZAI"/>
        <rdf:type rdf:resource="http://www.w3.org/2004/02/skos/core#Concept"/>
        <skos:broader rdf:resource="http://data.ign.fr/id/codes/topo/typedezai/PAITransport"/>
        <skos:definition xml:lang="en">Railway or cable transport establishment with or without a commercial passenger service: station, station, stopping point, urban railway station, cable car station. All stations and railway stops in use are included.</skos:definition>
        <skos:definition xml:lang="fr">Établissement ferroviaire ou de transport par câble assurant avec ou sans personnel un service commercial de voyageurs : gare, station, point d&apos;arrêt, station réseau ferré urbain, gare téléphérique. Toutes les gares et arrêts ferroviaires en service sont inclus.</skos:definition>
        <skos:inScheme rdf:resource="http://data.ign.fr/id/codes/topo/typedezai/liste"/>
        <skos:prefLabel xml:lang="fr">gare de voyageurs</skos:prefLabel>
        <skos:prefLabel xml:lang="en">passengers station</skos:prefLabel>
    </owl:NamedIndividual>
    


    <!-- http://data.ign.fr/id/codes/topo/typedezai/Gendarmerie -->


    <owl:NamedIndividual rdf:about="http://data.ign.fr/id/codes/topo/typedezai/Gendarmerie">
        <rdf:type rdf:resource="http://data.ign.fr/def/topo#TypeDeZAI"/>
        <rdf:type rdf:resource="http://www.w3.org/2004/02/skos/core#Concept"/>
        <skos:broader rdf:resource="http://data.ign.fr/id/codes/topo/typedezai/PAIAdministratifOuMilitaire"/>
        <skos:definition xml:lang="en">Barracks where the gendarmes are lodged; offices where they fulfill their administrative functions: gendarmerie, highway police. Definition of the footprint of the site: area of the entire barracks, usually delimited by a fence and including housing and offices.</skos:definition>
        <skos:definition xml:lang="fr">Caserne où les gendarmes sont logés ; bureaux où ils remplissent leurs fonctions administratives : gendarmerie, gendarmerie d&apos;autoroute. Définition de l&apos;emprise du site : surface de l&apos;ensemble de la caserne, généralement délimitée par une clôture et incluant logements et bureaux.</skos:definition>
        <skos:inScheme rdf:resource="http://data.ign.fr/id/codes/topo/typedezai/liste"/>
        <skos:prefLabel xml:lang="en">gendarmerie</skos:prefLabel>
        <skos:prefLabel xml:lang="fr">gendarmerie</skos:prefLabel>
    </owl:NamedIndividual>
    


    <!-- http://data.ign.fr/id/codes/topo/typedezai/Glacier -->


    <owl:NamedIndividual rdf:about="http://data.ign.fr/id/codes/topo/typedezai/Glacier">
        <rdf:type rdf:resource="http://data.ign.fr/def/topo#TypeDeZAI"/>
        <rdf:type rdf:resource="http://www.w3.org/2004/02/skos/core#Concept"/>
        <skos:broader rdf:resource="http://data.ign.fr/id/codes/topo/typedezai/PAIHydrographie"/>
        <skos:definition xml:lang="en">Name of a glacier or a detail related to a glacier: crevasse, glacier, moraine, firn, serac.</skos:definition>
        <skos:definition xml:lang="fr">Nom d&apos;un glacier ou d&apos;un détail relatif à un glacier : crevasse, glacier, moraine, névé, sérac.</skos:definition>
        <skos:inScheme rdf:resource="http://data.ign.fr/id/codes/topo/typedezai/liste"/>
        <skos:prefLabel xml:lang="en">glacier</skos:prefLabel>
        <skos:prefLabel xml:lang="fr">glacier</skos:prefLabel>
    </owl:NamedIndividual>
    


    <!-- http://data.ign.fr/id/codes/topo/typedezai/Golf -->


    <owl:NamedIndividual rdf:about="http://data.ign.fr/id/codes/topo/typedezai/Golf">
        <rdf:type rdf:resource="http://data.ign.fr/def/topo#TypeDeZAI"/>
        <rdf:type rdf:resource="http://www.w3.org/2004/02/skos/core#Concept"/>
        <skos:broader rdf:resource="http://data.ign.fr/id/codes/topo/typedezai/PAISport"/>
        <skos:definition xml:lang="en">Land open to the public and dedicated to the practice of golf. Less than 9 holes and minigolfs are excluded.</skos:definition>
        <skos:definition xml:lang="fr">Terrain ouvert au public et consacré à la pratique du golf. Les terrains de moins de 9 trous et les minigolfs sont exclus.</skos:definition>
        <skos:inScheme rdf:resource="http://data.ign.fr/id/codes/topo/typedezai/liste"/>
        <skos:prefLabel xml:lang="fr">golf</skos:prefLabel>
        <skos:prefLabel xml:lang="en">golf course</skos:prefLabel>
    </owl:NamedIndividual>
    


    <!-- http://data.ign.fr/id/codes/topo/typedezai/Grange -->


    <owl:NamedIndividual rdf:about="http://data.ign.fr/id/codes/topo/typedezai/Grange">
        <rdf:type rdf:resource="http://data.ign.fr/def/topo#TypeDeZAI"/>
        <rdf:type rdf:resource="http://www.w3.org/2004/02/skos/core#Concept"/>
        <skos:broader rdf:resource="http://data.ign.fr/id/codes/topo/typedezai/PAIZoneHabitation"/>
        <skos:definition xml:lang="fr">Construction légère : abri, baraquement, cabane, grange, hangar.</skos:definition>
        <skos:definition xml:lang="en">Light construction: shelter, barracks, hut, barn, shed.</skos:definition>
        <skos:inScheme rdf:resource="http://data.ign.fr/id/codes/topo/typedezai/liste"/>
        <skos:prefLabel xml:lang="en">barn</skos:prefLabel>
        <skos:prefLabel xml:lang="fr">grange</skos:prefLabel>
    </owl:NamedIndividual>
    


    <!-- http://data.ign.fr/id/codes/topo/typedezai/HabitationTroglodytique -->


    <owl:NamedIndividual rdf:about="http://data.ign.fr/id/codes/topo/typedezai/HabitationTroglodytique">
        <rdf:type rdf:resource="http://data.ign.fr/def/topo#TypeDeZAI"/>
        <rdf:type rdf:resource="http://www.w3.org/2004/02/skos/core#Concept"/>
        <skos:broader rdf:resource="http://data.ign.fr/id/codes/topo/typedezai/PAICultureLoisirs"/>
        <skos:definition xml:lang="fr">Excavation naturelle ou creusée dans le roc (caverne, grotte), habitée ou anciennement habitée.</skos:definition>
        <skos:definition xml:lang="en">Natural excavation or excavated in the rock (cavern, cave), inhabited or formerly inhabited.</skos:definition>
        <skos:inScheme rdf:resource="http://data.ign.fr/id/codes/topo/typedezai/liste"/>
        <skos:prefLabel xml:lang="en">cliff dwelling</skos:prefLabel>
        <skos:prefLabel xml:lang="fr">habitation troglodytique</skos:prefLabel>
    </owl:NamedIndividual>
    


    <!-- http://data.ign.fr/id/codes/topo/typedezai/HarasNational -->


    <owl:NamedIndividual rdf:about="http://data.ign.fr/id/codes/topo/typedezai/HarasNational">
        <rdf:type rdf:resource="http://data.ign.fr/def/topo#TypeDeZAI"/>
        <rdf:type rdf:resource="http://www.w3.org/2004/02/skos/core#Concept"/>
        <skos:broader rdf:resource="http://data.ign.fr/id/codes/topo/typedezai/PAIIndustrielCommercial"/>
        <skos:definition xml:lang="fr">Lieu ou établissement destiné à la reproduction de l&apos;espèce chevaline, à l&apos;amélioration des races de chevaux par la sélection des étalons. Tous les haras nationaux sont inclus. L&apos;enceinte comprend l&apos;ensemble des installations (manège, écuries, piste d&apos;entraînement,etc.).</skos:definition>
        <skos:definition xml:lang="en">Place or establishment intended for the reproduction of the horse species, for the improvement of the breeds of horses by the selection of the stallions. All national stud farms are included. The enclosure includes all the facilities (carousel, stables, training track, etc.).</skos:definition>
        <skos:inScheme rdf:resource="http://data.ign.fr/id/codes/topo/typedezai/liste"/>
        <skos:prefLabel xml:lang="fr">haras national</skos:prefLabel>
        <skos:prefLabel xml:lang="en">ranch</skos:prefLabel>
    </owl:NamedIndividual>
    


    <!-- http://data.ign.fr/id/codes/topo/typedezai/Hippodrome -->


    <owl:NamedIndividual rdf:about="http://data.ign.fr/id/codes/topo/typedezai/Hippodrome">
        <rdf:type rdf:resource="http://data.ign.fr/def/topo#TypeDeZAI"/>
        <rdf:type rdf:resource="http://www.w3.org/2004/02/skos/core#Concept"/>
        <skos:broader rdf:resource="http://data.ign.fr/id/codes/topo/typedezai/PAISport"/>
        <skos:definition xml:lang="fr">Lieu ouvert au public et consacré aux courses de chevaux. Seuls les hippodromes possédant des aménagements conséquents (tribunes, bâtiments spécifiques) sont inclus.</skos:definition>
        <skos:definition xml:lang="en">Open to the public and dedicated to horse racing. Only racetracks with significant amenities (stands, specific buildings) are included.</skos:definition>
        <skos:inScheme rdf:resource="http://data.ign.fr/id/codes/topo/typedezai/liste"/>
        <skos:prefLabel xml:lang="fr">hippodrome</skos:prefLabel>
        <skos:prefLabel xml:lang="en">racecourse</skos:prefLabel>
    </owl:NamedIndividual>
    


    <!-- http://data.ign.fr/id/codes/topo/typedezai/Hopital -->


    <owl:NamedIndividual rdf:about="http://data.ign.fr/id/codes/topo/typedezai/Hopital">
        <rdf:type rdf:resource="http://data.ign.fr/def/topo#TypeDeZAI"/>
        <rdf:type rdf:resource="http://www.w3.org/2004/02/skos/core#Concept"/>
        <skos:broader rdf:resource="http://data.ign.fr/id/codes/topo/typedezai/PAISante"/>
        <skos:definition xml:lang="en">Public or private institution, where all the medical and surgical heavy and / or long-term care, as well as deliveries are carried out: hospital, university hospital, military hospital, clinic.</skos:definition>
        <skos:definition xml:lang="fr">Établissement public ou privé, où sont effectués tous les soins médicaux et chirurgicaux lourds et/ou de longue durée, ainsi que les accouchements : hôpital, CHU, hôpital militaire, clinique.</skos:definition>
        <skos:inScheme rdf:resource="http://data.ign.fr/id/codes/topo/typedezai/liste"/>
        <skos:prefLabel xml:lang="en">hospital</skos:prefLabel>
        <skos:prefLabel xml:lang="fr">hôpital</skos:prefLabel>
    </owl:NamedIndividual>
    


    <!-- http://data.ign.fr/id/codes/topo/typedezai/HotelDeDepartement -->


    <owl:NamedIndividual rdf:about="http://data.ign.fr/id/codes/topo/typedezai/HotelDeDepartement">
        <rdf:type rdf:resource="http://data.ign.fr/def/topo#TypeDeZAI"/>
        <rdf:type rdf:resource="http://www.w3.org/2004/02/skos/core#Concept"/>
        <skos:broader rdf:resource="http://data.ign.fr/id/codes/topo/typedezai/PAIAdministratifOuMilitaire"/>
        <skos:definition xml:lang="en">Building where the General Council sits. Only the main building is included. The annexes are not, except possibly an annex located in another agglomeration when it has a function close to that of the headquarters.</skos:definition>
        <skos:definition xml:lang="fr">Bâtiment où siège le conseil général. Seul le bâtiment principal est inclus. Les annexes ne le sont pas, sauf éventuellement une annexe située dans une autre agglomération lorsqu&apos;elle a une fonction proche de celle du siège.</skos:definition>
        <skos:inScheme rdf:resource="http://data.ign.fr/id/codes/topo/typedezai/liste"/>
        <skos:prefLabel xml:lang="en">departmental administration building</skos:prefLabel>
        <skos:prefLabel xml:lang="fr">hôtel de département</skos:prefLabel>
    </owl:NamedIndividual>
    


    <!-- http://data.ign.fr/id/codes/topo/typedezai/HotelDeRegion -->


    <owl:NamedIndividual rdf:about="http://data.ign.fr/id/codes/topo/typedezai/HotelDeRegion">
        <rdf:type rdf:resource="http://data.ign.fr/def/topo#TypeDeZAI"/>
        <rdf:type rdf:resource="http://www.w3.org/2004/02/skos/core#Concept"/>
        <skos:broader rdf:resource="http://data.ign.fr/id/codes/topo/typedezai/PAIAdministratifOuMilitaire"/>
        <skos:definition xml:lang="en">Building where the regional council sits. Only the main building is included. The annexes are not, except possibly an annex located in another agglomeration when it has a function close to that of the headquarters.</skos:definition>
        <skos:definition xml:lang="fr">Bâtiment où siège le conseil régional. Seul le bâtiment principal est inclus. Les annexes ne le sont pas, sauf éventuellement une annexe située dans une autre agglomération lorsqu&apos;elle a une fonction proche de celle du siège.</skos:definition>
        <skos:inScheme rdf:resource="http://data.ign.fr/id/codes/topo/typedezai/liste"/>
        <skos:prefLabel xml:lang="fr">hôtel de région</skos:prefLabel>
        <skos:prefLabel xml:lang="en">regional administration building</skos:prefLabel>
    </owl:NamedIndividual>
    


    <!-- http://data.ign.fr/id/codes/topo/typedezai/InfrastructureRoutiere -->


    <owl:NamedIndividual rdf:about="http://data.ign.fr/id/codes/topo/typedezai/InfrastructureRoutiere">
        <rdf:type rdf:resource="http://data.ign.fr/def/topo#TypeDeZAI"/>
        <rdf:type rdf:resource="http://www.w3.org/2004/02/skos/core#Concept"/>
        <skos:broader rdf:resource="http://data.ign.fr/id/codes/topo/typedezai/PAITransport"/>
        <skos:definition xml:lang="en">A road network element that is neither an attribute of a &apos;road segment&apos; object nor the &apos;crossroad&apos; attribute value: road, toll area, rest area.</skos:definition>
        <skos:definition xml:lang="fr">Élément du réseau routier ne figurant ni en attribut d&apos;un objet &apos;tronçon de route&apos; ni avec la valeur d&apos;attribut &apos;carrefour&apos; : route, aire de péage, aire de repos.</skos:definition>
        <skos:inScheme rdf:resource="http://data.ign.fr/id/codes/topo/typedezai/liste"/>
        <skos:prefLabel xml:lang="fr">infrastructure routière</skos:prefLabel>
        <skos:prefLabel xml:lang="en">road transport infrastructure</skos:prefLabel>
    </owl:NamedIndividual>
    


    <!-- http://data.ign.fr/id/codes/topo/typedezai/Lac -->


    <owl:NamedIndividual rdf:about="http://data.ign.fr/id/codes/topo/typedezai/Lac">
        <rdf:type rdf:resource="http://data.ign.fr/def/topo#TypeDeZAI"/>
        <rdf:type rdf:resource="http://www.w3.org/2004/02/skos/core#Concept"/>
        <skos:broader rdf:resource="http://data.ign.fr/id/codes/topo/typedezai/PAIHydrographie"/>
        <skos:definition xml:lang="en">Body of water: pond, pond, lake, pond.</skos:definition>
        <skos:definition xml:lang="fr">Étendue d&apos;eau terrestre : bassin, étang, lac, mare.</skos:definition>
        <skos:inScheme rdf:resource="http://data.ign.fr/id/codes/topo/typedezai/liste"/>
        <skos:prefLabel xml:lang="fr">lac</skos:prefLabel>
        <skos:prefLabel xml:lang="en">lake</skos:prefLabel>
    </owl:NamedIndividual>
    


    <!-- http://data.ign.fr/id/codes/topo/typedezai/LieuDitHabite -->


    <owl:NamedIndividual rdf:about="http://data.ign.fr/id/codes/topo/typedezai/LieuDitHabite">
        <rdf:type rdf:resource="http://data.ign.fr/def/topo#TypeDeZAI"/>
        <rdf:type rdf:resource="http://www.w3.org/2004/02/skos/core#Concept"/>
        <skos:broader rdf:resource="http://data.ign.fr/id/codes/topo/typedezai/PAIZoneHabitation"/>
        <skos:definition xml:lang="en">Inhabited locality characterized by a name.</skos:definition>
        <skos:definition xml:lang="fr">Lieu-dit habité caractérisé par un nom.</skos:definition>
        <skos:inScheme rdf:resource="http://data.ign.fr/id/codes/topo/typedezai/liste"/>
        <skos:prefLabel xml:lang="en">inhabited local placename</skos:prefLabel>
        <skos:prefLabel xml:lang="fr">lieu-dit habité</skos:prefLabel>
    </owl:NamedIndividual>
    


    <!-- http://data.ign.fr/id/codes/topo/typedezai/LieuDitNonHabite -->


    <owl:NamedIndividual rdf:about="http://data.ign.fr/id/codes/topo/typedezai/LieuDitNonHabite">
        <rdf:type rdf:resource="http://data.ign.fr/def/topo#TypeDeZAI"/>
        <rdf:type rdf:resource="http://www.w3.org/2004/02/skos/core#Concept"/>
        <skos:broader rdf:resource="http://data.ign.fr/id/codes/topo/typedezai/PAIEspaceNaturel"/>
        <skos:definition xml:lang="en">Any locality, whose name is generally attached to land: uninhabited locality, plantation, cultivated area.</skos:definition>
        <skos:definition xml:lang="fr">Lieu-dit quelconque, dont le nom est généralement attaché à des terres : lieu-dit non habité, plantation, espace cultivé.</skos:definition>
        <skos:inScheme rdf:resource="http://data.ign.fr/id/codes/topo/typedezai/liste"/>
        <skos:prefLabel xml:lang="fr">lieu-dit non habité</skos:prefLabel>
        <skos:prefLabel xml:lang="en">non inhabited local placename</skos:prefLabel>
    </owl:NamedIndividual>
    


    <!-- http://data.ign.fr/id/codes/topo/typedezai/MaisonDuParc -->


    <owl:NamedIndividual rdf:about="http://data.ign.fr/id/codes/topo/typedezai/MaisonDuParc">
        <rdf:type rdf:resource="http://data.ign.fr/def/topo#TypeDeZAI"/>
        <rdf:type rdf:resource="http://www.w3.org/2004/02/skos/core#Concept"/>
        <skos:broader rdf:resource="http://data.ign.fr/id/codes/topo/typedezai/PAICultureLoisirs"/>
        <skos:definition xml:lang="en">Building open to the public and managed by a National or Regional Park.</skos:definition>
        <skos:definition xml:lang="fr">Bâtiment ouvert au public et géré par un Parc National ou Régional.</skos:definition>
        <skos:inScheme rdf:resource="http://data.ign.fr/id/codes/topo/typedezai/liste"/>
        <skos:prefLabel xml:lang="fr">maison du parc</skos:prefLabel>
        <skos:prefLabel xml:lang="en">park center</skos:prefLabel>
    </owl:NamedIndividual>
    


    <!-- http://data.ign.fr/id/codes/topo/typedezai/MaisonForestiere -->


    <owl:NamedIndividual rdf:about="http://data.ign.fr/id/codes/topo/typedezai/MaisonForestiere">
        <rdf:type rdf:resource="http://data.ign.fr/def/topo#TypeDeZAI"/>
        <rdf:type rdf:resource="http://www.w3.org/2004/02/skos/core#Concept"/>
        <skos:broader rdf:resource="http://data.ign.fr/id/codes/topo/typedezai/PAIAdministratifOuMilitaire"/>
        <skos:definition xml:lang="en">House managed by the National Forest Office. Guard houses occupied by at least one NFB agent are included. The offices of the NFB, the homes of agents also used as offices, are excluded when they are not located in a forest house.</skos:definition>
        <skos:definition xml:lang="fr">Maison gérée par l&apos;office national des forêts. Les maisons de garde occupées par au moins un agent de l&apos;ONF sont incluses. Les bureaux de l&apos;ONF, les domiciles d&apos;agents servant aussi de bureau, sont exclus lorsqu&apos;ils ne sont pas situés dans une maison forestière.</skos:definition>
        <skos:inScheme rdf:resource="http://data.ign.fr/id/codes/topo/typedezai/liste"/>
        <skos:prefLabel xml:lang="en">forest house</skos:prefLabel>
        <skos:prefLabel xml:lang="fr">maison forestière</skos:prefLabel>
    </owl:NamedIndividual>
    


    <!-- http://data.ign.fr/id/codes/topo/typedezai/Marais -->


    <owl:NamedIndividual rdf:about="http://data.ign.fr/id/codes/topo/typedezai/Marais">
        <rdf:type rdf:resource="http://data.ign.fr/def/topo#TypeDeZAI"/>
        <rdf:type rdf:resource="http://www.w3.org/2004/02/skos/core#Concept"/>
        <skos:broader rdf:resource="http://data.ign.fr/id/codes/topo/typedezai/PAIHydrographie"/>
        <skos:definition xml:lang="en">Wetland: marsh, swamp, saline.</skos:definition>
        <skos:definition xml:lang="fr">Zone humide : marais, marécage, saline.</skos:definition>
        <skos:inScheme rdf:resource="http://data.ign.fr/id/codes/topo/typedezai/liste"/>
        <skos:prefLabel xml:lang="fr">marais</skos:prefLabel>
        <skos:prefLabel xml:lang="en">marsh</skos:prefLabel>
    </owl:NamedIndividual>
    


    <!-- http://data.ign.fr/id/codes/topo/typedezai/MaraisSalants -->


    <owl:NamedIndividual rdf:about="http://data.ign.fr/id/codes/topo/typedezai/MaraisSalants">
        <rdf:type rdf:resource="http://data.ign.fr/def/topo#TypeDeZAI"/>
        <rdf:type rdf:resource="http://www.w3.org/2004/02/skos/core#Concept"/>
        <skos:broader rdf:resource="http://data.ign.fr/id/codes/topo/typedezai/PAIIndustrielCommercial"/>
        <skos:definition xml:lang="en">Area consisting of basins dug near the coasts to extract salt from seawater by evaporation. Areas of salt marshes less than 3 ha are excluded. Old salt marshes that are no longer active are excluded.</skos:definition>
        <skos:definition xml:lang="fr">Zone constituée de bassins creusés à proximité des côtes pour extraire le sel de l&apos;eau de mer par évaporation. Les zones de marais salants de moins de 3 ha sont exclues. Les anciens marais salants qui ne sont plus en activité sont exclus.</skos:definition>
        <skos:inScheme rdf:resource="http://data.ign.fr/id/codes/topo/typedezai/liste"/>
        <skos:prefLabel xml:lang="fr">marais salants</skos:prefLabel>
        <skos:prefLabel xml:lang="en">salt evaporator</skos:prefLabel>
    </owl:NamedIndividual>
    


    <!-- http://data.ign.fr/id/codes/topo/typedezai/Marche -->


    <owl:NamedIndividual rdf:about="http://data.ign.fr/id/codes/topo/typedezai/Marche">
        <rdf:type rdf:resource="http://data.ign.fr/def/topo#TypeDeZAI"/>
        <rdf:type rdf:resource="http://www.w3.org/2004/02/skos/core#Concept"/>
        <skos:broader rdf:resource="http://data.ign.fr/id/codes/topo/typedezai/PAIIndustrielCommercial"/>
        <skos:definition xml:lang="en">Any building built for the purpose of marketing wholesale or retail foodstuffs: covered market, national interest market, regional interest market, hall, fair, permanent exhibition area, covered auction.</skos:definition>
        <skos:definition xml:lang="fr">Tout ensemble construit dont la finalité est la commercialisation de gros ou de détail de denrées alimentaires : marché couvert, marché d&apos;intérêt national, marché d&apos;intérêt régional, halle, foire, zone d&apos;exposition à caractère permanent, criée couverte.</skos:definition>
        <skos:inScheme rdf:resource="http://data.ign.fr/id/codes/topo/typedezai/liste"/>
        <skos:prefLabel xml:lang="fr">marché</skos:prefLabel>
        <skos:prefLabel xml:lang="en">market</skos:prefLabel>
    </owl:NamedIndividual>
    


    <!-- http://data.ign.fr/id/codes/topo/typedezai/Menhir -->


    <owl:NamedIndividual rdf:about="http://data.ign.fr/id/codes/topo/typedezai/Menhir">
        <rdf:type rdf:resource="http://data.ign.fr/def/topo#TypeDeZAI"/>
        <rdf:type rdf:resource="http://www.w3.org/2004/02/skos/core#Concept"/>
        <skos:broader rdf:resource="http://data.ign.fr/id/codes/topo/typedezai/PAICultureLoisirs"/>
        <skos:definition xml:lang="en">Elongated stone, erected vertically. The alignments in cromlech are included.</skos:definition>
        <skos:definition xml:lang="fr">Pierre allongée, dressée verticalement. Les alignements en cromlech sont inclus.</skos:definition>
        <skos:inScheme rdf:resource="http://data.ign.fr/id/codes/topo/typedezai/liste"/>
        <skos:prefLabel xml:lang="en">menhir</skos:prefLabel>
        <skos:prefLabel xml:lang="fr">menhir</skos:prefLabel>
    </owl:NamedIndividual>
    


    <!-- http://data.ign.fr/id/codes/topo/typedezai/Mine -->


    <owl:NamedIndividual rdf:about="http://data.ign.fr/id/codes/topo/typedezai/Mine">
        <rdf:type rdf:resource="http://data.ign.fr/def/topo#TypeDeZAI"/>
        <rdf:type rdf:resource="http://www.w3.org/2004/02/skos/core#Concept"/>
        <skos:broader rdf:resource="http://data.ign.fr/id/codes/topo/typedezai/PAIIndustrielCommercial"/>
        <skos:definition xml:lang="fr">Lieu d&apos;où l&apos;on extrait des minerais : mine de houille, mine de lignite, crassier, entrée de mine, terril. Les mines à ciel ouvert de plus de 10 ha sont incluses. Les mines souterraines sont exclues.</skos:definition>
        <skos:definition xml:lang="en">Location from which minerals are mined: coal mine, lignite mine, slag pit, mine entrance, slag heap. Open pit mines of more than 10 ha are included. Underground mines are excluded.</skos:definition>
        <skos:inScheme rdf:resource="http://data.ign.fr/id/codes/topo/typedezai/liste"/>
        <skos:prefLabel xml:lang="en">mine</skos:prefLabel>
        <skos:prefLabel xml:lang="fr">mine</skos:prefLabel>
    </owl:NamedIndividual>
    


    <!-- http://data.ign.fr/id/codes/topo/typedezai/Moulin -->


    <owl:NamedIndividual rdf:about="http://data.ign.fr/id/codes/topo/typedezai/Moulin">
        <rdf:type rdf:resource="http://data.ign.fr/def/topo#TypeDeZAI"/>
        <rdf:type rdf:resource="http://www.w3.org/2004/02/skos/core#Concept"/>
        <skos:broader rdf:resource="http://data.ign.fr/id/codes/topo/typedezai/PAIZoneHabitation"/>
        <skos:definition xml:lang="en">Mill or old water mill.</skos:definition>
        <skos:definition xml:lang="fr">Moulin ou ancien moulin à eau.</skos:definition>
        <skos:inScheme rdf:resource="http://data.ign.fr/id/codes/topo/typedezai/liste"/>
        <skos:prefLabel xml:lang="en">mill</skos:prefLabel>
        <skos:prefLabel xml:lang="fr">moulin</skos:prefLabel>
    </owl:NamedIndividual>
    


    <!-- http://data.ign.fr/id/codes/topo/typedezai/Musee -->


    <owl:NamedIndividual rdf:about="http://data.ign.fr/id/codes/topo/typedezai/Musee">
        <rdf:type rdf:resource="http://data.ign.fr/def/topo#TypeDeZAI"/>
        <rdf:type rdf:resource="http://www.w3.org/2004/02/skos/core#Concept"/>
        <skos:broader rdf:resource="http://data.ign.fr/id/codes/topo/typedezai/PAICultureLoisirs"/>
        <skos:definition xml:lang="en">Open to the public with a large collection of art and science objects, documents, etc. that can be used in their history. Included: all museums controlled or supervised by the Ministry of Culture (national museums, classified, controlled, etc.), museums under certain technical ministries or public assistance (Army Museum, Navy Museum ), private museums or associations with high notoriety, ecomuseums.</skos:definition>
        <skos:definition xml:lang="fr">Établissement ouvert au public exposant une grande collection d&apos;objets, de documents, etc., relatifs aux arts et aux sciences et pouvant servir à leur histoire. Sont inclus : tous les musées controlés ou supervisés par le ministère de la Culture (musées nationaux, classés, controlés,etc.), les musées relevant de certains ministères techniques ou de l&apos;assistance publique (musée de l&apos;armée, de la marine), les musées privés ou associatifs ayant une grande notoriété, les écomusées.</skos:definition>
        <skos:inScheme rdf:resource="http://data.ign.fr/id/codes/topo/typedezai/liste"/>
        <skos:prefLabel xml:lang="en">museum</skos:prefLabel>
        <skos:prefLabel xml:lang="fr">musée</skos:prefLabel>
    </owl:NamedIndividual>
    


    <!-- http://data.ign.fr/id/codes/topo/typedezai/OuvrageMilitaire -->


    <owl:NamedIndividual rdf:about="http://data.ign.fr/id/codes/topo/typedezai/OuvrageMilitaire">
        <rdf:type rdf:resource="http://data.ign.fr/def/topo#TypeDeZAI"/>
        <rdf:type rdf:resource="http://www.w3.org/2004/02/skos/core#Concept"/>
        <skos:broader rdf:resource="http://data.ign.fr/id/codes/topo/typedezai/PAIAdministratifOuMilitaire"/>
        <skos:definition xml:lang="en">Military works or installations.</skos:definition>
        <skos:definition xml:lang="fr">Ouvrages ou installations militaires.</skos:definition>
        <skos:inScheme rdf:resource="http://data.ign.fr/id/codes/topo/typedezai/liste"/>
        <skos:prefLabel xml:lang="en">defence work</skos:prefLabel>
        <skos:prefLabel xml:lang="fr">ouvrage militaire</skos:prefLabel>
    </owl:NamedIndividual>
    


    <!-- http://data.ign.fr/id/codes/topo/typedezai/PAIAdministratifOuMilitaire -->


    <owl:NamedIndividual rdf:about="http://data.ign.fr/id/codes/topo/typedezai/PAIAdministratifOuMilitaire">
        <rdf:type rdf:resource="http://data.ign.fr/def/topo#TypeDeZAI"/>
        <rdf:type rdf:resource="http://www.w3.org/2004/02/skos/core#Concept"/>
        <skos:definition xml:lang="en">Designation of an establishment, site or area of public, administrative or military character.</skos:definition>
        <skos:definition xml:lang="fr">Désignation d&apos;un établissement, site ou zone ayant un caractère public, administratif ou militaire.</skos:definition>
        <skos:inScheme rdf:resource="http://data.ign.fr/id/codes/topo/typedezai/liste"/>
        <skos:prefLabel xml:lang="fr">PAI administratif ou militaire</skos:prefLabel>
        <skos:prefLabel xml:lang="en">administrative or military POI</skos:prefLabel>
    </owl:NamedIndividual>
    


    <!-- http://data.ign.fr/id/codes/topo/typedezai/PAICultureLoisirs -->


    <owl:NamedIndividual rdf:about="http://data.ign.fr/id/codes/topo/typedezai/PAICultureLoisirs">
        <rdf:type rdf:resource="http://data.ign.fr/def/topo#TypeDeZAI"/>
        <rdf:type rdf:resource="http://www.w3.org/2004/02/skos/core#Concept"/>
        <skos:definition xml:lang="en">Designation of an establishment or place specially equipped for a cultural, tourist or leisure activity.</skos:definition>
        <skos:definition xml:lang="fr">Désignation d&apos;un établissement ou lieu spécialement aménagé pour une activité culturelle, touristique ou de loisirs.</skos:definition>
        <skos:inScheme rdf:resource="http://data.ign.fr/id/codes/topo/typedezai/liste"/>
        <skos:prefLabel xml:lang="fr">PAI culture ou loisirs</skos:prefLabel>
        <skos:prefLabel xml:lang="en">culture or leasure POI</skos:prefLabel>
    </owl:NamedIndividual>
    


    <!-- http://data.ign.fr/id/codes/topo/typedezai/PAIEspaceNaturel -->


    <owl:NamedIndividual rdf:about="http://data.ign.fr/id/codes/topo/typedezai/PAIEspaceNaturel">
        <rdf:type rdf:resource="http://data.ign.fr/def/topo#TypeDeZAI"/>
        <rdf:type rdf:resource="http://www.w3.org/2004/02/skos/core#Concept"/>
        <skos:definition xml:lang="en">Designation of an uninhabited locality whose name does not relate to an orographic detail or a hydrographic detail.</skos:definition>
        <skos:definition xml:lang="fr">Désignation d&apos;un lieu-dit non habité dont le nom ne se rapporte ni à un détail orographique ni à un détail hydrographique.</skos:definition>
        <skos:inScheme rdf:resource="http://data.ign.fr/id/codes/topo/typedezai/liste"/>
        <skos:prefLabel xml:lang="fr">PAI espace naturel</skos:prefLabel>
        <skos:prefLabel xml:lang="en">natural POI</skos:prefLabel>
    </owl:NamedIndividual>
    


    <!-- http://data.ign.fr/id/codes/topo/typedezai/PAIGestionEaux -->


    <owl:NamedIndividual rdf:about="http://data.ign.fr/id/codes/topo/typedezai/PAIGestionEaux">
        <rdf:type rdf:resource="http://data.ign.fr/def/topo#TypeDeZAI"/>
        <rdf:type rdf:resource="http://www.w3.org/2004/02/skos/core#Concept"/>
        <skos:definition xml:lang="en">Designation of a construction or site related to the supply, treatment of water for different needs (agricultural, industrial, consumption) or sewage treatment before release into the wild.</skos:definition>
        <skos:definition xml:lang="fr">Désignation d&apos;une construction ou site liés à l&apos;approvisionnement, au traitement de l&apos;eau pour différents besoins (agricole, industriel, consommation) ou à l&apos;épuration des eaux usées avant rejet dans la nature.</skos:definition>
        <skos:inScheme rdf:resource="http://data.ign.fr/id/codes/topo/typedezai/liste"/>
        <skos:prefLabel xml:lang="fr">PAI gestion des eaux</skos:prefLabel>
        <skos:prefLabel xml:lang="en">water treatment POI</skos:prefLabel>
    </owl:NamedIndividual>
    


    <!-- http://data.ign.fr/id/codes/topo/typedezai/PAIHydrographie -->


    <owl:NamedIndividual rdf:about="http://data.ign.fr/id/codes/topo/typedezai/PAIHydrographie">
        <rdf:type rdf:resource="http://data.ign.fr/def/topo#TypeDeZAI"/>
        <rdf:type rdf:resource="http://www.w3.org/2004/02/skos/core#Concept"/>
        <skos:definition xml:lang="en">Designation relating to a hydrographic detail.</skos:definition>
        <skos:definition xml:lang="fr">Désignation se rapportant à un détail hydrographique.</skos:definition>
        <skos:inScheme rdf:resource="http://data.ign.fr/id/codes/topo/typedezai/liste"/>
        <skos:prefLabel xml:lang="fr">PAI hydrographie</skos:prefLabel>
        <skos:prefLabel xml:lang="en">hydrographic POI</skos:prefLabel>
    </owl:NamedIndividual>
    


    <!-- http://data.ign.fr/id/codes/topo/typedezai/PAIIndustrielCommercial -->


    <owl:NamedIndividual rdf:about="http://data.ign.fr/id/codes/topo/typedezai/PAIIndustrielCommercial">
        <rdf:type rdf:resource="http://data.ign.fr/def/topo#TypeDeZAI"/>
        <rdf:type rdf:resource="http://www.w3.org/2004/02/skos/core#Concept"/>
        <skos:definition xml:lang="en">Designation of a building, site or zone of an industrial or commercial nature.</skos:definition>
        <skos:definition xml:lang="fr">Désignation d&apos;un bâtiment, site ou zone à caractère industriel ou commercial.</skos:definition>
        <skos:inScheme rdf:resource="http://data.ign.fr/id/codes/topo/typedezai/liste"/>
        <skos:prefLabel xml:lang="fr">PAI industriel ou commercial</skos:prefLabel>
        <skos:prefLabel xml:lang="en">industrial or commercial POI</skos:prefLabel>
    </owl:NamedIndividual>
    


    <!-- http://data.ign.fr/id/codes/topo/typedezai/PAIOrographie -->


    <owl:NamedIndividual rdf:about="http://data.ign.fr/id/codes/topo/typedezai/PAIOrographie">
        <rdf:type rdf:resource="http://data.ign.fr/def/topo#TypeDeZAI"/>
        <rdf:type rdf:resource="http://www.w3.org/2004/02/skos/core#Concept"/>
        <skos:definition xml:lang="en">Designation of a relief detail.</skos:definition>
        <skos:definition xml:lang="fr">Désignation d&apos;un détail du relief.</skos:definition>
        <skos:inScheme rdf:resource="http://data.ign.fr/id/codes/topo/typedezai/liste"/>
        <skos:prefLabel xml:lang="fr">PAI orographie</skos:prefLabel>
        <skos:prefLabel xml:lang="en">relief POI</skos:prefLabel>
    </owl:NamedIndividual>
    


    <!-- http://data.ign.fr/id/codes/topo/typedezai/PAIReligieux -->


    <owl:NamedIndividual rdf:about="http://data.ign.fr/id/codes/topo/typedezai/PAIReligieux">
        <rdf:type rdf:resource="http://data.ign.fr/def/topo#TypeDeZAI"/>
        <rdf:type rdf:resource="http://www.w3.org/2004/02/skos/core#Concept"/>
        <skos:definition xml:lang="en">Designation of a building reserved for the practice of a religion.</skos:definition>
        <skos:definition xml:lang="fr">Désignation d&apos;un bâtiment réservé à la pratique d&apos;une religion.</skos:definition>
        <skos:inScheme rdf:resource="http://data.ign.fr/id/codes/topo/typedezai/liste"/>
        <skos:prefLabel xml:lang="fr">PAI religieux</skos:prefLabel>
        <skos:prefLabel xml:lang="en">religious POI</skos:prefLabel>
    </owl:NamedIndividual>
    


    <!-- http://data.ign.fr/id/codes/topo/typedezai/PAISante -->


    <owl:NamedIndividual rdf:about="http://data.ign.fr/id/codes/topo/typedezai/PAISante">
        <rdf:type rdf:resource="http://data.ign.fr/def/topo#TypeDeZAI"/>
        <rdf:type rdf:resource="http://www.w3.org/2004/02/skos/core#Concept"/>
        <skos:definition xml:lang="en">Designation of a thermal or hospital type establishment.</skos:definition>
        <skos:definition xml:lang="fr">Désignation d&apos;un établissement thermal ou de type hospitalier.</skos:definition>
        <skos:inScheme rdf:resource="http://data.ign.fr/id/codes/topo/typedezai/liste"/>
        <skos:prefLabel xml:lang="fr">PAI santé</skos:prefLabel>
        <skos:prefLabel xml:lang="en">healthcare POI</skos:prefLabel>
    </owl:NamedIndividual>
    


    <!-- http://data.ign.fr/id/codes/topo/typedezai/PAIScienceEnseignement -->


    <owl:NamedIndividual rdf:about="http://data.ign.fr/id/codes/topo/typedezai/PAIScienceEnseignement">
        <rdf:type rdf:resource="http://data.ign.fr/def/topo#TypeDeZAI"/>
        <rdf:type rdf:resource="http://www.w3.org/2004/02/skos/core#Concept"/>
        <skos:definition xml:lang="en">Designation of an educational or research institution.</skos:definition>
        <skos:definition xml:lang="fr">Désignation d&apos;un établissement d&apos;enseignement ou de recherche.</skos:definition>
        <skos:inScheme rdf:resource="http://data.ign.fr/id/codes/topo/typedezai/liste"/>
        <skos:prefLabel xml:lang="fr">PAI science ou enseignement</skos:prefLabel>
        <skos:prefLabel xml:lang="en">science or education POI</skos:prefLabel>
    </owl:NamedIndividual>
    


    <!-- http://data.ign.fr/id/codes/topo/typedezai/PAISport -->


    <owl:NamedIndividual rdf:about="http://data.ign.fr/id/codes/topo/typedezai/PAISport">
        <rdf:type rdf:resource="http://data.ign.fr/def/topo#TypeDeZAI"/>
        <rdf:type rdf:resource="http://www.w3.org/2004/02/skos/core#Concept"/>
        <skos:definition xml:lang="fr">Désignation d&apos;un établissement ou lieu spécialement aménagé pour la pratique d&apos;une ou plusieurs activités sportives.</skos:definition>
        <skos:inScheme rdf:resource="http://data.ign.fr/id/codes/topo/typedezai/liste"/>
        <skos:prefLabel xml:lang="fr">PAI sport</skos:prefLabel>
        <skos:prefLabel xml:lang="en">sports POI</skos:prefLabel>
    </owl:NamedIndividual>
    


    <!-- http://data.ign.fr/id/codes/topo/typedezai/PAITransport -->


    <owl:NamedIndividual rdf:about="http://data.ign.fr/id/codes/topo/typedezai/PAITransport">
        <rdf:type rdf:resource="http://data.ign.fr/def/topo#TypeDeZAI"/>
        <rdf:type rdf:resource="http://www.w3.org/2004/02/skos/core#Concept"/>
        <skos:definition xml:lang="en">Designation of an establishment or place specially equipped for the practice of one or more sports activities.</skos:definition>
        <skos:definition xml:lang="fr">Désignation d&apos;un bâtiment ou site lié à une activité de transport routier, ferré ou aérien.</skos:definition>
        <skos:inScheme rdf:resource="http://data.ign.fr/id/codes/topo/typedezai/liste"/>
        <skos:prefLabel xml:lang="fr">PAI transport</skos:prefLabel>
        <skos:prefLabel xml:lang="en">transport POI</skos:prefLabel>
    </owl:NamedIndividual>
    


    <!-- http://data.ign.fr/id/codes/topo/typedezai/PAIZoneHabitation -->


    <owl:NamedIndividual rdf:about="http://data.ign.fr/id/codes/topo/typedezai/PAIZoneHabitation">
        <rdf:type rdf:resource="http://data.ign.fr/def/topo#TypeDeZAI"/>
        <rdf:type rdf:resource="http://www.w3.org/2004/02/skos/core#Concept"/>
        <skos:definition xml:lang="en">Designation of an inhabited locality characterized by a name.</skos:definition>
        <skos:definition xml:lang="fr">Désignation d&apos;un lieu-dit habité caractérisé par un nom.</skos:definition>
        <skos:inScheme rdf:resource="http://data.ign.fr/id/codes/topo/typedezai/liste"/>
        <skos:prefLabel xml:lang="fr">PAI zone d&apos;habitation</skos:prefLabel>
        <skos:prefLabel xml:lang="en">dwellings zone POI</skos:prefLabel>
    </owl:NamedIndividual>
    


    <!-- http://data.ign.fr/id/codes/topo/typedezai/PalaisDeJustice -->


    <owl:NamedIndividual rdf:about="http://data.ign.fr/id/codes/topo/typedezai/PalaisDeJustice">
        <rdf:type rdf:resource="http://data.ign.fr/def/topo#TypeDeZAI"/>
        <rdf:type rdf:resource="http://www.w3.org/2004/02/skos/core#Concept"/>
        <skos:broader rdf:resource="http://data.ign.fr/id/codes/topo/typedezai/PAIAdministratifOuMilitaire"/>
        <skos:definition xml:lang="en">Building where justice is done: courthouse, court. Only criminal justice is treated. Administrative tribunals are excluded.</skos:definition>
        <skos:definition xml:lang="fr">Bâtiment où l&apos;on rend la justice : palais de justice, tribunal. Seule la justice pénale est traitée. Les tribunaux administratifs sont exclus.</skos:definition>
        <skos:inScheme rdf:resource="http://data.ign.fr/id/codes/topo/typedezai/liste"/>
        <skos:prefLabel xml:lang="en">law-courts</skos:prefLabel>
        <skos:prefLabel xml:lang="fr">palais de justice</skos:prefLabel>
    </owl:NamedIndividual>
    


    <!-- http://data.ign.fr/id/codes/topo/typedezai/Parc -->


    <owl:NamedIndividual rdf:about="http://data.ign.fr/id/codes/topo/typedezai/Parc">
        <rdf:type rdf:resource="http://data.ign.fr/def/topo#TypeDeZAI"/>
        <rdf:type rdf:resource="http://www.w3.org/2004/02/skos/core#Concept"/>
        <skos:broader rdf:resource="http://data.ign.fr/id/codes/topo/typedezai/PAIEspaceNaturel"/>
        <skos:definition xml:lang="fr">Espace réglementé, généralement libre d&apos;accès pour le public et où la nature fait l&apos;objet d&apos;une protection spéciale : jardin, parc municipal, parc intercommunal, parc départemental, parc interdépartemental, parc naturel régional, parc national, réserve naturelle, parc marin. Les parcs à vocation commerciale ne sont pas pris en compte.</skos:definition>
        <skos:definition xml:lang="en">Regulated area, generally free for the public and where nature is the subject of special protection: garden, municipal park, intercommunal park, departmental park, interdepartmental park, regional nature park, national park, nature reserve, park marine. Commercial parks are not taken into account.</skos:definition>
        <skos:inScheme rdf:resource="http://data.ign.fr/id/codes/topo/typedezai/liste"/>
        <skos:prefLabel xml:lang="fr">parc</skos:prefLabel>
        <skos:prefLabel xml:lang="en">park</skos:prefLabel>
    </owl:NamedIndividual>
    


    <!-- http://data.ign.fr/id/codes/topo/typedezai/ParcDeLoisirs -->


    <owl:NamedIndividual rdf:about="http://data.ign.fr/id/codes/topo/typedezai/ParcDeLoisirs">
        <rdf:type rdf:resource="http://data.ign.fr/def/topo#TypeDeZAI"/>
        <rdf:type rdf:resource="http://www.w3.org/2004/02/skos/core#Concept"/>
        <skos:broader rdf:resource="http://data.ign.fr/id/codes/topo/typedezai/PAICultureLoisirs"/>
        <skos:definition xml:lang="en">Commercial park specially designed for recreation: permanent games center, amusement park, relaxation park, leisure center. Only parks with an area exceeding 10 ha and equipped with substantial equipment are included. Public parks (gardens, municipal parks, departmental parks) are excluded (see the value &apos;public space&apos;).</skos:definition>
        <skos:definition xml:lang="fr">Parc à caractère commercial spécialement aménagé pour les loisirs : centre permanent de jeux, parc d&apos;attractions, parc de détente, centre de loisirs. Seuls les parcs dont la superficie excède 10 ha et dotés d&apos;équipements conséquents sont inclus. Les parcs publics (jardins, parcs communaux, départementaux) sont exclus (voir la valeur &apos;espace public&apos;).</skos:definition>
        <skos:inScheme rdf:resource="http://data.ign.fr/id/codes/topo/typedezai/liste"/>
        <skos:prefLabel xml:lang="en">leisure park</skos:prefLabel>
        <skos:prefLabel xml:lang="fr">parc de loisirs</skos:prefLabel>
    </owl:NamedIndividual>
    


    <!-- http://data.ign.fr/id/codes/topo/typedezai/ParcDesExpositions -->


    <owl:NamedIndividual rdf:about="http://data.ign.fr/id/codes/topo/typedezai/ParcDesExpositions">
        <rdf:type rdf:resource="http://data.ign.fr/def/topo#TypeDeZAI"/>
        <rdf:type rdf:resource="http://www.w3.org/2004/02/skos/core#Concept"/>
        <skos:broader rdf:resource="http://data.ign.fr/id/codes/topo/typedezai/PAICultureLoisirs"/>
        <skos:definition xml:lang="fr">Lieu d&apos;exposition ou de culture : centre culturel, parc des expositions.</skos:definition>
        <skos:definition xml:lang="en">Place of exhibition or culture: cultural center, exhibition center.</skos:definition>
        <skos:inScheme rdf:resource="http://data.ign.fr/id/codes/topo/typedezai/liste"/>
        <skos:prefLabel xml:lang="en">fairground</skos:prefLabel>
        <skos:prefLabel xml:lang="fr">parc des expositions</skos:prefLabel>
    </owl:NamedIndividual>
    


    <!-- http://data.ign.fr/id/codes/topo/typedezai/ParcZoologique -->


    <owl:NamedIndividual rdf:about="http://data.ign.fr/id/codes/topo/typedezai/ParcZoologique">
        <rdf:type rdf:resource="http://data.ign.fr/def/topo#TypeDeZAI"/>
        <rdf:type rdf:resource="http://www.w3.org/2004/02/skos/core#Concept"/>
        <skos:broader rdf:resource="http://data.ign.fr/id/codes/topo/typedezai/PAICultureLoisirs"/>
        <skos:definition xml:lang="fr">Parc ouvert au public, où il est possible de voir des animaux sauvages vivant en captivité ou en semi-liberté. Tous les parcs ouverts au public sont inclus.</skos:definition>
        <skos:definition xml:lang="en">Park open to the public, where it is possible to see wild animals living in captivity or semi-freedom. All parks open to the public are included.</skos:definition>
        <skos:inScheme rdf:resource="http://data.ign.fr/id/codes/topo/typedezai/liste"/>
        <skos:prefLabel xml:lang="fr">parc zoologique</skos:prefLabel>
        <skos:prefLabel xml:lang="en">zoological park</skos:prefLabel>
    </owl:NamedIndividual>
    


    <!-- http://data.ign.fr/id/codes/topo/typedezai/PareFeu -->


    <owl:NamedIndividual rdf:about="http://data.ign.fr/id/codes/topo/typedezai/PareFeu">
        <rdf:type rdf:resource="http://data.ign.fr/def/topo#TypeDeZAI"/>
        <rdf:type rdf:resource="http://www.w3.org/2004/02/skos/core#Concept"/>
        <skos:broader rdf:resource="http://data.ign.fr/id/codes/topo/typedezai/PAIEspaceNaturel"/>
        <skos:definition xml:lang="en">Device designed to prevent the spread of a fire (usually opening in the endangered forest).</skos:definition>
        <skos:definition xml:lang="fr">Dispositif destiné à empêcher la propagation d&apos;un incendie (généralement, ouverture pratiquée dans le massif forestier menacé).</skos:definition>
        <skos:inScheme rdf:resource="http://data.ign.fr/id/codes/topo/typedezai/liste"/>
        <skos:prefLabel xml:lang="en">fire-break</skos:prefLabel>
        <skos:prefLabel xml:lang="fr">pare-feu</skos:prefLabel>
    </owl:NamedIndividual>
    


    <!-- http://data.ign.fr/id/codes/topo/typedezai/Parking -->


    <owl:NamedIndividual rdf:about="http://data.ign.fr/id/codes/topo/typedezai/Parking">
        <rdf:type rdf:resource="http://data.ign.fr/def/topo#TypeDeZAI"/>
        <rdf:type rdf:resource="http://www.w3.org/2004/02/skos/core#Concept"/>
        <skos:broader rdf:resource="http://data.ign.fr/id/codes/topo/typedezai/PAITransport"/>
        <skos:definition xml:lang="en">A parking area or parking area is a parking area for vehicles: parking, parking, underground parking, parking. All public car parks with more than 25 spaces are included, whether underground or air (eg municipal car parks), Car parks with more than 25 spaces associated with transport services (train stations, airports) are retained even if they do not have a proper name. Parking spaces at rest or service areas are not retained (see &apos;Rest Area&apos; and &apos;Service Area&apos; values). Car parks belonging to purely commercial establishments (eg supermarket car park) are excluded (for these, see also the &apos;Road surface&apos; class). Parking is a one-off object located in the center of the parking area, or at the entrance for underground car parks. It is generally associated with a surface area for car parks over 5 ha.</skos:definition>
        <skos:definition xml:lang="fr">Une aire de stationnement ou parking est une zone aménagée pour le stationnement des véhicules : aire de stationnement, parking, parking souterrain, parking à étages. Tous les parkings publics nommés de plus de 25 places sont inclus qu&apos;ils soient souterrains ou aériens (ex. parkings municipaux), Les parkings de plus de 25 places associés à des services de transport (gares, aéroports) sont retenus même s&apos;ils n&apos;ont pas de nom propre. Les parkings d&apos;aires de repos ou de service ne sont pas retenus (voir les valeur &apos;Aire de repos&apos; et &apos;Aire de service&apos;). Le parkings appartenant à des établissements purement commerciaux (ex. parking de supermarché) sont exclus (pour ces derniers, voir aussi la classe &apos;Surface de route&apos;). Un Parking est un objet ponctuel situé au centre de l&apos;aire de stationnement, ou à l&apos;entrée pour les parkings souterrains. Il est généralement associé à une surface pour des parkings aériens de plus de 5 ha.</skos:definition>
        <skos:inScheme rdf:resource="http://data.ign.fr/id/codes/topo/typedezai/liste"/>
        <skos:prefLabel xml:lang="en">car park</skos:prefLabel>
        <skos:prefLabel xml:lang="fr">parking</skos:prefLabel>
    </owl:NamedIndividual>
    


    <!-- http://data.ign.fr/id/codes/topo/typedezai/Pecherie -->


    <owl:NamedIndividual rdf:about="http://data.ign.fr/id/codes/topo/typedezai/Pecherie">
        <rdf:type rdf:resource="http://data.ign.fr/def/topo#TypeDeZAI"/>
        <rdf:type rdf:resource="http://www.w3.org/2004/02/skos/core#Concept"/>
        <skos:broader rdf:resource="http://data.ign.fr/id/codes/topo/typedezai/PAIHydrographie"/>
        <skos:definition xml:lang="en">Aquaculture activity area: bouchot, oyster farm, fishery.</skos:definition>
        <skos:definition xml:lang="fr">Zone d&apos;activité aquacole : bouchot, parc à huîtres, pêcherie.</skos:definition>
        <skos:inScheme rdf:resource="http://data.ign.fr/id/codes/topo/typedezai/liste"/>
        <skos:prefLabel xml:lang="en">aquaculture area</skos:prefLabel>
        <skos:prefLabel xml:lang="fr">pêcherie</skos:prefLabel>
    </owl:NamedIndividual>
    


    <!-- http://data.ign.fr/id/codes/topo/typedezai/Perte -->


    <owl:NamedIndividual rdf:about="http://data.ign.fr/id/codes/topo/typedezai/Perte">
        <rdf:type rdf:resource="http://data.ign.fr/def/topo#TypeDeZAI"/>
        <rdf:type rdf:resource="http://www.w3.org/2004/02/skos/core#Concept"/>
        <skos:broader rdf:resource="http://data.ign.fr/id/codes/topo/typedezai/PAIHydrographie"/>
        <skos:definition xml:lang="fr">Lieu où disparaît, où se perd un cours d&apos;eau, qui réapparaît ensuite, en formant une résurgence, après avoir effectué un trajet souterrain.</skos:definition>
        <skos:definition xml:lang="en">Place where disappears, where a stream is lost, which reappears then, forming a resurgence, after having made an underground trip.</skos:definition>
        <skos:inScheme rdf:resource="http://data.ign.fr/id/codes/topo/typedezai/liste"/>
        <skos:prefLabel xml:lang="en">loss</skos:prefLabel>
        <skos:prefLabel xml:lang="fr">perte</skos:prefLabel>
    </owl:NamedIndividual>
    


    <!-- http://data.ign.fr/id/codes/topo/typedezai/Piscine -->


    <owl:NamedIndividual rdf:about="http://data.ign.fr/id/codes/topo/typedezai/Piscine">
        <rdf:type rdf:resource="http://data.ign.fr/def/topo#TypeDeZAI"/>
        <rdf:type rdf:resource="http://www.w3.org/2004/02/skos/core#Concept"/>
        <skos:broader rdf:resource="http://data.ign.fr/id/codes/topo/typedezai/PAISport"/>
        <skos:definition xml:lang="fr">Grand bassin de natation, et ensemble des installations qui l&apos;entourent : piscine couverte, piscine découverte. Toutes les piscines ouvertes au public et ayant un bassin au moins de 25 m ou plus sont incluses. Les piscines des centres de vacances ou des hôtels sont exclues (voir la classe TERRAIN_SPORT).</skos:definition>
        <skos:definition xml:lang="en">Large swimming pool, and all the facilities that surround it: indoor pool, outdoor pool. All pools open to the public and having a pool of at least 25 m or more are included. Pools at holiday centers or hotels are excluded (see the TERRAIN_SPORT class).</skos:definition>
        <skos:inScheme rdf:resource="http://data.ign.fr/id/codes/topo/typedezai/liste"/>
        <skos:narrowMatch rdf:resource="http://data.ign.fr/id/codes/topo/typedebatiment/BassinDeNatation"/>
        <skos:prefLabel xml:lang="fr">piscine</skos:prefLabel>
        <skos:prefLabel xml:lang="en">swimming-pool</skos:prefLabel>
    </owl:NamedIndividual>
    


    <!-- http://data.ign.fr/id/codes/topo/typedezai/PointDEau -->


    <owl:NamedIndividual rdf:about="http://data.ign.fr/id/codes/topo/typedezai/PointDEau">
        <rdf:type rdf:resource="http://data.ign.fr/def/topo#TypeDeZAI"/>
        <rdf:type rdf:resource="http://www.w3.org/2004/02/skos/core#Concept"/>
        <skos:broader rdf:resource="http://data.ign.fr/id/codes/topo/typedezai/PAIHydrographie"/>
        <skos:definition xml:lang="en">Any natural or artificial water point: catchment, cistern, fountain, well, resurgence, source.</skos:definition>
        <skos:definition xml:lang="fr">Tout point d&apos;eau naturel ou artificiel : captage, citerne, fontaine, puits, résurgence, source.</skos:definition>
        <skos:inScheme rdf:resource="http://data.ign.fr/id/codes/topo/typedezai/liste"/>
        <skos:prefLabel xml:lang="fr">point d&apos;eau</skos:prefLabel>
        <skos:prefLabel xml:lang="en">waterhole</skos:prefLabel>
    </owl:NamedIndividual>
    


    <!-- http://data.ign.fr/id/codes/topo/typedezai/PointDeVue -->


    <owl:NamedIndividual rdf:about="http://data.ign.fr/id/codes/topo/typedezai/PointDeVue">
        <rdf:type rdf:resource="http://data.ign.fr/def/topo#TypeDeZAI"/>
        <rdf:type rdf:resource="http://www.w3.org/2004/02/skos/core#Concept"/>
        <skos:broader rdf:resource="http://data.ign.fr/id/codes/topo/typedezai/PAIEspaceNaturel"/>
        <skos:definition xml:lang="fr">Endroit d&apos;où l&apos;on jouit d&apos;une vue pittoresque : point de vue, table d&apos;orientation, belvédè. Seuls les points de vue aménagés (table d&apos;orientation, bancs,etc.) sont inclus.</skos:definition>
        <skos:definition xml:lang="en">Place from where one enjoys a picturesque sight: point of view, orientation table, belvede. Only the points of view (orientation table, benches, etc.) are included.</skos:definition>
        <skos:inScheme rdf:resource="http://data.ign.fr/id/codes/topo/typedezai/liste"/>
        <skos:prefLabel xml:lang="fr">point de vue</skos:prefLabel>
        <skos:prefLabel xml:lang="en">viewpoint</skos:prefLabel>
    </owl:NamedIndividual>
    


    <!-- http://data.ign.fr/id/codes/topo/typedezai/Port -->


    <owl:NamedIndividual rdf:about="http://data.ign.fr/id/codes/topo/typedezai/Port">
        <rdf:type rdf:resource="http://data.ign.fr/def/topo#TypeDeZAI"/>
        <rdf:type rdf:resource="http://www.w3.org/2004/02/skos/core#Concept"/>
        <skos:broader rdf:resource="http://data.ign.fr/id/codes/topo/typedezai/PAITransport"/>
        <skos:definition xml:lang="fr">Abri naturel ou artificiel aménagé pour recevoir les navires, pour l&apos;embarquement et le débarquement de leur chargement : port de plaisance, port de pêche, port national, port privé, port international, port militaire.</skos:definition>
        <skos:definition xml:lang="en">Natural or artificial shelter fitted out to receive the ships, for loading and unloading of their load: marina, fishing port, national port, private port, international port, military port.</skos:definition>
        <skos:inScheme rdf:resource="http://data.ign.fr/id/codes/topo/typedezai/liste"/>
        <skos:prefLabel xml:lang="en">harbor</skos:prefLabel>
        <skos:prefLabel xml:lang="fr">port</skos:prefLabel>
    </owl:NamedIndividual>
    


    <!-- http://data.ign.fr/id/codes/topo/typedezai/PosteDePolice -->


    <owl:NamedIndividual rdf:about="http://data.ign.fr/id/codes/topo/typedezai/PosteDePolice">
        <rdf:type rdf:resource="http://data.ign.fr/def/topo#TypeDeZAI"/>
        <rdf:type rdf:resource="http://www.w3.org/2004/02/skos/core#Concept"/>
        <skos:altLabel xml:lang="fr">hôtel de police</skos:altLabel>
        <skos:altLabel xml:lang="en">police station</skos:altLabel>
        <skos:broader rdf:resource="http://data.ign.fr/id/codes/topo/typedezai/PAIAdministratifOuMilitaire"/>
        <skos:definition xml:lang="en">Establishment occupied by a police commissioner (judicial police officer responsible for enforcing police regulations and ensuring the maintenance of public peace): national police station, police station, highway, port or airport CRS. Buildings housing only the municipal police are excluded. The barracks of CRS and mobile gendarmes take the value &apos;military enclosure&apos; and the gendarmeries the value &apos;gendarmerie&apos;.</skos:definition>
        <skos:definition xml:lang="fr">Établissement occupé par un commissaire de police (officier de police judiciaire chargé de faire observer les règlements de police et de veiller au maintien de la paix publique) : hôtel de police nationale, commissariat, CRS d&apos;autoroute, de port ou d&apos;aéroport. Les bâtiments hébergeant uniquement la police municipale sont exclus. Les casernes de CRS et de gendarmes mobiles prennent la valeur &apos;enceinte militaire&apos; et les gendarmeries la valeur &apos;gendarmerie&apos;.</skos:definition>
        <skos:inScheme rdf:resource="http://data.ign.fr/id/codes/topo/typedezai/liste"/>
        <skos:prefLabel xml:lang="en">police post</skos:prefLabel>
        <skos:prefLabel xml:lang="fr">poste de police</skos:prefLabel>
    </owl:NamedIndividual>
    


    <!-- http://data.ign.fr/id/codes/topo/typedezai/PrefectureDeRegion -->


    <owl:NamedIndividual rdf:about="http://data.ign.fr/id/codes/topo/typedezai/PrefectureDeRegion">
        <rdf:type rdf:resource="http://data.ign.fr/def/topo#TypeDeZAI"/>
        <rdf:type rdf:resource="http://www.w3.org/2004/02/skos/core#Concept"/>
        <skos:broader rdf:resource="http://data.ign.fr/id/codes/topo/typedezai/PAIAdministratifOuMilitaire"/>
        <skos:definition xml:lang="en">Establishment which houses the headquarters of the civil administration of the region. The annexes are excluded.</skos:definition>
        <skos:definition xml:lang="fr">Établissement qui abrite le siège de l&apos;administration civile de la région. Les annexes sont exclues.</skos:definition>
        <skos:inScheme rdf:resource="http://data.ign.fr/id/codes/topo/typedezai/liste"/>
        <skos:prefLabel xml:lang="fr">préfecture de région</skos:prefLabel>
        <skos:prefLabel xml:lang="en">regional prefecture</skos:prefLabel>
    </owl:NamedIndividual>
    


    <!-- http://data.ign.fr/id/codes/topo/typedezai/Quartier -->


    <owl:NamedIndividual rdf:about="http://data.ign.fr/id/codes/topo/typedezai/Quartier">
        <rdf:type rdf:resource="http://data.ign.fr/def/topo#TypeDeZAI"/>
        <rdf:type rdf:resource="http://www.w3.org/2004/02/skos/core#Concept"/>
        <skos:broader rdf:resource="http://data.ign.fr/id/codes/topo/typedezai/PAIZoneHabitation"/>
        <skos:definition xml:lang="en">Neighborhood named: city, suburb, housing estate.</skos:definition>
        <skos:definition xml:lang="fr">Quartier nommé : cité, faubourg, lotissement.</skos:definition>
        <skos:inScheme rdf:resource="http://data.ign.fr/id/codes/topo/typedezai/liste"/>
        <skos:prefLabel xml:lang="en">district</skos:prefLabel>
        <skos:prefLabel xml:lang="fr">quartier</skos:prefLabel>
    </owl:NamedIndividual>
    


    <!-- http://data.ign.fr/id/codes/topo/typedezai/Refuge -->


    <owl:NamedIndividual rdf:about="http://data.ign.fr/id/codes/topo/typedezai/Refuge">
        <rdf:type rdf:resource="http://data.ign.fr/def/topo#TypeDeZAI"/>
        <rdf:type rdf:resource="http://www.w3.org/2004/02/skos/core#Concept"/>
        <skos:broader rdf:resource="http://data.ign.fr/id/codes/topo/typedezai/PAICultureLoisirs"/>
        <skos:definition xml:lang="fr">Refuge, refuge gardé, abri de montagne nommé.</skos:definition>
        <skos:definition xml:lang="en">Refuge, sheltered refuge, named mountain shelter.</skos:definition>
        <skos:inScheme rdf:resource="http://data.ign.fr/id/codes/topo/typedezai/liste"/>
        <skos:prefLabel xml:lang="fr">refuge</skos:prefLabel>
        <skos:prefLabel xml:lang="en">shelter</skos:prefLabel>
    </owl:NamedIndividual>
    


    <!-- http://data.ign.fr/id/codes/topo/typedezai/Riviere -->


    <owl:NamedIndividual rdf:about="http://data.ign.fr/id/codes/topo/typedezai/Riviere">
        <rdf:type rdf:resource="http://data.ign.fr/def/topo#TypeDeZAI"/>
        <rdf:type rdf:resource="http://www.w3.org/2004/02/skos/core#Concept"/>
        <skos:broader rdf:resource="http://data.ign.fr/id/codes/topo/typedezai/PAIHydrographie"/>
        <skos:definition xml:lang="fr">Cours d&apos;eau: fleuve, rivière, ruisseau, torrent.</skos:definition>
        <skos:definition xml:lang="en">Stream: river, stream.</skos:definition>
        <skos:inScheme rdf:resource="http://data.ign.fr/id/codes/topo/typedezai/liste"/>
        <skos:prefLabel xml:lang="en">river</skos:prefLabel>
        <skos:prefLabel xml:lang="fr">rivière</skos:prefLabel>
    </owl:NamedIndividual>
    


    <!-- http://data.ign.fr/id/codes/topo/typedezai/RondPoint -->


    <owl:NamedIndividual rdf:about="http://data.ign.fr/id/codes/topo/typedezai/RondPoint">
        <rdf:type rdf:resource="http://data.ign.fr/def/topo#TypeDeZAI"/>
        <rdf:type rdf:resource="http://www.w3.org/2004/02/skos/core#Concept"/>
        <skos:broader rdf:resource="http://data.ign.fr/id/codes/topo/typedezai/PAITransport"/>
        <skos:definition xml:lang="fr">Rond-point, place de forme circulaire, ovale ou semi-circulaire, ou carrefour giratoire. Un giratoire est formé d&apos;un anneau central qui permet aux usagers de prendre n&apos;importe quelle direction, y compris de faire un demi-tour. Seuls les ronds-points nommés sont retenus.</skos:definition>
        <skos:definition xml:lang="en">Roundabout, circular, oval or semicircular square, or roundabout. A roundabout consists of a central ring that allows users to take any direction, including making a U-turn. Only the roundabouts named are retained.</skos:definition>
        <skos:inScheme rdf:resource="http://data.ign.fr/id/codes/topo/typedezai/liste"/>
        <skos:prefLabel xml:lang="fr">rond-point</skos:prefLabel>
        <skos:prefLabel xml:lang="en">roundabout</skos:prefLabel>
    </owl:NamedIndividual>
    


    <!-- http://data.ign.fr/id/codes/topo/typedezai/Science -->


    <owl:NamedIndividual rdf:about="http://data.ign.fr/id/codes/topo/typedezai/Science">
        <rdf:type rdf:resource="http://data.ign.fr/def/topo#TypeDeZAI"/>
        <rdf:type rdf:resource="http://www.w3.org/2004/02/skos/core#Concept"/>
        <skos:broader rdf:resource="http://data.ign.fr/id/codes/topo/typedezai/PAIScienceEnseignement"/>
        <skos:definition xml:lang="en">Scientific or technical institution named: research center, laboratory, observatory, scientific station.</skos:definition>
        <skos:definition xml:lang="fr">Établissement scientifique ou technique nommé: centre de recherche, laboratoire, observatoire, station scientifique.</skos:definition>
        <skos:inScheme rdf:resource="http://data.ign.fr/id/codes/topo/typedezai/liste"/>
        <skos:prefLabel xml:lang="en">scientific or technological center</skos:prefLabel>
        <skos:prefLabel xml:lang="fr">établissement scientifique ou technique</skos:prefLabel>
    </owl:NamedIndividual>
    


    <!-- http://data.ign.fr/id/codes/topo/typedezai/Stade -->


    <owl:NamedIndividual rdf:about="http://data.ign.fr/id/codes/topo/typedezai/Stade">
        <rdf:type rdf:resource="http://data.ign.fr/def/topo#TypeDeZAI"/>
        <rdf:type rdf:resource="http://www.w3.org/2004/02/skos/core#Concept"/>
        <skos:broader rdf:resource="http://data.ign.fr/id/codes/topo/typedezai/PAISport"/>
        <skos:definition xml:lang="fr">Grande enceinte, terrain aménagé pour la pratique des sports, et le plus souvent entouré de gradins, de tribunes : stade, terrain de sports, vélodrome découvert, circuit auto-moto, complexe sportif pluridisciplinaire. Seules les enceintes incluant des aménagements conséquents (piste &apos;construite&apos;, tribunes,etc.) sont incluses. Les terrains d&apos;entraînement incluant seulement 2 ou 3 terrains de football et de petits vestiaires sont exclus (voir aussi la classe TERRAIN_SPORT).</skos:definition>
        <skos:definition xml:lang="en">Large enclosure, ground arranged for the practice of the sports, and most often surrounded by bleachers, tribunes: stadium, ground of sports, velodrome discovered, circuit auto-moto, sport complex multidisciplinary. Only enclosures including substantial amenities (track &apos;built&apos;, stands, etc.) are included. Training grounds with only 2 or 3 football pitches and locker rooms are excluded (see also TERRAIN_SPORT class).</skos:definition>
        <skos:inScheme rdf:resource="http://data.ign.fr/id/codes/topo/typedezai/liste"/>
        <skos:prefLabel xml:lang="fr">stade</skos:prefLabel>
        <skos:prefLabel xml:lang="en">stadium</skos:prefLabel>
    </owl:NamedIndividual>
    


    <!-- http://data.ign.fr/id/codes/topo/typedezai/StationDeMetro -->


    <owl:NamedIndividual rdf:about="http://data.ign.fr/id/codes/topo/typedezai/StationDeMetro">
        <rdf:type rdf:resource="http://data.ign.fr/def/topo#TypeDeZAI"/>
        <rdf:type rdf:resource="http://www.w3.org/2004/02/skos/core#Concept"/>
        <skos:broader rdf:resource="http://data.ign.fr/id/codes/topo/typedezai/PAITransport"/>
        <skos:definition xml:lang="fr">Station où il est possible d&apos;accéder au réseau du métro. On saisit un seul objet &apos;Station de métro&apos; même s&apos;il y a plusieurs entrées distinctes, éventuellement plusieurs ponctuels &apos;Station de métro&apos; pour les correspondances importantes (ex : Bastille) mais un seul ponctuel pour une station de métro qui n&apos;est pas une correspondance.</skos:definition>
        <skos:definition xml:lang="en">Station where it is possible to access the metro network. One seize only one object &apos;Metro Station&apos; even if there are several separate entrances, possibly several punctual &apos;Metro Station&apos; for important connections (eg Bastille) but only one punctual for a metro station that is not not a match.</skos:definition>
        <skos:inScheme rdf:resource="http://data.ign.fr/id/codes/topo/typedezai/liste"/>
        <skos:prefLabel xml:lang="fr">station de métro</skos:prefLabel>
        <skos:prefLabel xml:lang="en">underground station</skos:prefLabel>
    </owl:NamedIndividual>
    


    <!-- http://data.ign.fr/id/codes/topo/typedezai/Tombeau -->


    <owl:NamedIndividual rdf:about="http://data.ign.fr/id/codes/topo/typedezai/Tombeau">
        <rdf:type rdf:resource="http://data.ign.fr/def/topo#TypeDeZAI"/>
        <rdf:type rdf:resource="http://www.w3.org/2004/02/skos/core#Concept"/>
        <skos:broader rdf:resource="http://data.ign.fr/id/codes/topo/typedezai/PAIReligieux"/>
        <skos:definition xml:lang="en">Cemetery, grave or tomb named: cemetery, tomb, tomb, ossuary, funeral parlor.</skos:definition>
        <skos:definition xml:lang="fr">Cimetière, tombe ou tombeau nommé : cimetière, tombe, tombeau, ossuaire, funérarium.</skos:definition>
        <skos:inScheme rdf:resource="http://data.ign.fr/id/codes/topo/typedezai/liste"/>
        <skos:prefLabel xml:lang="en">tomb</skos:prefLabel>
        <skos:prefLabel xml:lang="fr">tombeau</skos:prefLabel>
    </owl:NamedIndividual>
    


    <!-- http://data.ign.fr/id/codes/topo/typedezai/Usine -->


    <owl:NamedIndividual rdf:about="http://data.ign.fr/id/codes/topo/typedezai/Usine">
        <rdf:type rdf:resource="http://data.ign.fr/def/topo#TypeDeZAI"/>
        <rdf:type rdf:resource="http://www.w3.org/2004/02/skos/core#Concept"/>
        <skos:broader rdf:resource="http://data.ign.fr/id/codes/topo/typedezai/PAIIndustrielCommercial"/>
        <skos:definition xml:lang="en">Establishment dominated by an industrial activity (manufacture of objects or products, transformation or conservation of raw materials): workshop, factory, manufacture, mine with built infrastructure, factory, sawmill. Sites with an area of less than 5 ha are generally excluded.</skos:definition>
        <skos:definition xml:lang="fr">Établissement dominé par une activité industrielle (fabrication d&apos;objets ou de produits, transformation ou conservation de matières premières) : atelier, fabrique, manufacture, mine avec infrastructure bâtie, usine, scierie. Les sites dont la superficie est inférieure à 5 ha sont généralement exclus.</skos:definition>
        <skos:inScheme rdf:resource="http://data.ign.fr/id/codes/topo/typedezai/liste"/>
        <skos:prefLabel xml:lang="en">factory</skos:prefLabel>
        <skos:prefLabel xml:lang="fr">usine</skos:prefLabel>
    </owl:NamedIndividual>
    


    <!-- http://data.ign.fr/id/codes/topo/typedezai/UsineDeTraitementDesEaux -->


    <owl:NamedIndividual rdf:about="http://data.ign.fr/id/codes/topo/typedezai/UsineDeTraitementDesEaux">
        <rdf:type rdf:resource="http://data.ign.fr/def/topo#TypeDeZAI"/>
        <rdf:type rdf:resource="http://www.w3.org/2004/02/skos/core#Concept"/>
        <skos:broader rdf:resource="http://data.ign.fr/id/codes/topo/typedezai/PAIGestionEaux"/>
        <skos:definition xml:lang="en">Establishment with facilities to make water clean for consumption (water treatment plant) or to purify wastewater before discharge into the natural environment (sewage treatment plants, lagooning plants): water treatment plant, station purification plant, lagooning station. Treatment and lagooning plants are included. Stations treating water to make it fit for consumption are included when they include significant facilities (factories including basins, filtering, mechanical treatments). Stations are excluded when it concerns only a secondary chemical treatment carried out at the level of a catchment or a reservoir. Bearing stations are also excluded.</skos:definition>
        <skos:definition xml:lang="fr">Établissement comprenant des installations destinées à rendre l&apos;eau propre à la consommation (usine de traitement des eaux) ou à épurer des eaux usées avant leur rejet dans la nature (stations d&apos;épuration, de lagunage) : usine de traitement des eaux, station d&apos;épuration, station de lagunage. Les stations d&apos;épuration et de lagunage sont incluses. Les stations traitant l&apos;eau afin de la rendre propre à la consommation sont incluses lorsqu&apos;elles comprennent des installations conséquentes (usines comprenant bassins, filtrages, traitements mécaniques). Sont exclues les stations lorsqu&apos;il s&apos;agit uniquement d&apos;un traitement chimique d&apos;appoint effectué au niveau d&apos;un captage ou d&apos;un réservoir. Les stations de relèvement sont également exclues.</skos:definition>
        <skos:inScheme rdf:resource="http://data.ign.fr/id/codes/topo/typedezai/liste"/>
        <skos:prefLabel xml:lang="fr">usine de traitement des eaux</skos:prefLabel>
        <skos:prefLabel xml:lang="en">water treatment plant</skos:prefLabel>
    </owl:NamedIndividual>
    


    <!-- http://data.ign.fr/id/codes/topo/typedezai/Vestiges -->


    <owl:NamedIndividual rdf:about="http://data.ign.fr/id/codes/topo/typedezai/Vestiges">
        <rdf:type rdf:resource="http://data.ign.fr/def/topo#TypeDeZAI"/>
        <rdf:type rdf:resource="http://www.w3.org/2004/02/skos/core#Concept"/>
        <skos:broader rdf:resource="http://data.ign.fr/id/codes/topo/typedezai/PAICultureLoisirs"/>
        <skos:definition xml:lang="en">Archaeological remains, excavations, burial mounds, oppidum.</skos:definition>
        <skos:definition xml:lang="fr">Vestiges archéologiques, fouilles, tumulus, oppidum.</skos:definition>
        <skos:inScheme rdf:resource="http://data.ign.fr/id/codes/topo/typedezai/liste"/>
        <skos:prefLabel xml:lang="en">archeological ruins</skos:prefLabel>
        <skos:prefLabel xml:lang="fr">vestiges archéologiques</skos:prefLabel>
    </owl:NamedIndividual>
    


    <!-- http://data.ign.fr/id/codes/topo/typedezai/VillageDeVacances -->


    <owl:NamedIndividual rdf:about="http://data.ign.fr/id/codes/topo/typedezai/VillageDeVacances">
        <rdf:type rdf:resource="http://data.ign.fr/def/topo#TypeDeZAI"/>
        <rdf:type rdf:resource="http://www.w3.org/2004/02/skos/core#Concept"/>
        <skos:broader rdf:resource="http://data.ign.fr/id/codes/topo/typedezai/PAICultureLoisirs"/>
        <skos:definition xml:lang="en">Establishment of holidays including sports facilities or substantial relaxation of which the manager is private or public: village of vacanaces, colony of holidays. Hotels and &apos;holiday camps&apos; are excluded, as well as establishments with a carrying capacity of less than 300 people.</skos:definition>
        <skos:definition xml:lang="fr">Établissement de vacances comprenant des équipements sportifs ou de détente conséquents dont le gestionnaire est privé ou public: village de vacanaces, colonie de vacances. Les hôtels et les &apos;camps de vacances&apos; sont exclus, ainsi que les établissements dont la capacité de rpise en charge est inférieure à 300 personnes.</skos:definition>
        <skos:inScheme rdf:resource="http://data.ign.fr/id/codes/topo/typedezai/liste"/>
        <skos:prefLabel xml:lang="en">holiday village</skos:prefLabel>
        <skos:prefLabel xml:lang="fr">village de vacances</skos:prefLabel>
    </owl:NamedIndividual>
    


    <!-- http://data.ign.fr/id/codes/topo/typedezai/VoieFerree -->


    <owl:NamedIndividual rdf:about="http://data.ign.fr/id/codes/topo/typedezai/VoieFerree">
        <rdf:type rdf:resource="http://data.ign.fr/def/topo#TypeDeZAI"/>
        <rdf:type rdf:resource="http://www.w3.org/2004/02/skos/core#Concept"/>
        <skos:broader rdf:resource="http://data.ign.fr/id/codes/topo/typedezai/PAITransport"/>
        <skos:definition xml:lang="en">Railroad name</skos:definition>
        <skos:definition xml:lang="fr">Voie ferrée nommée</skos:definition>
        <skos:inScheme rdf:resource="http://data.ign.fr/id/codes/topo/typedezai/liste"/>
        <skos:prefLabel xml:lang="en">railway line</skos:prefLabel>
        <skos:prefLabel xml:lang="fr">voie ferrée</skos:prefLabel>
    </owl:NamedIndividual>
    


    <!-- http://data.ign.fr/id/codes/topo/typedezai/ZoneIndustrielle -->


    <owl:NamedIndividual rdf:about="http://data.ign.fr/id/codes/topo/typedezai/ZoneIndustrielle">
        <rdf:type rdf:resource="http://data.ign.fr/def/topo#TypeDeZAI"/>
        <rdf:type rdf:resource="http://www.w3.org/2004/02/skos/core#Concept"/>
        <skos:broader rdf:resource="http://data.ign.fr/id/codes/topo/typedezai/PAIIndustrielCommercial"/>
        <skos:definition xml:lang="en">Grouping of production activities on the initiative of local authorities or parastatals (chambers of commerce and industry) and bearing a name: artisanal zone, industrial zone. Sites with an area of less than 5 ha are generally excluded.</skos:definition>
        <skos:definition xml:lang="fr">Regroupement d&apos;activités de production sur l&apos;initiative des collectivités locales ou d&apos;organismes parapublics (chambres de commerce et d&apos;industrie) et portant un nom : zone artisanale, zone industrielle. Les sites dont la superficie est inférieure à 5 ha sont généralement exclus.</skos:definition>
        <skos:inScheme rdf:resource="http://data.ign.fr/id/codes/topo/typedezai/liste"/>
        <skos:prefLabel xml:lang="en">industrial area</skos:prefLabel>
        <skos:prefLabel xml:lang="fr">zone industrielle</skos:prefLabel>
    </owl:NamedIndividual>
    


    <!-- http://data.ign.fr/id/codes/topo/typedezai/liste -->


    <owl:NamedIndividual rdf:about="http://data.ign.fr/id/codes/topo/typedezai/liste">
        <rdf:type rdf:resource="http://www.w3.org/2004/02/skos/core#ConceptScheme"/>
        <rdfs:comment xml:lang="en">List of different types of activity areas and interests, represented as a hierarchy of SKOS concepts.</rdfs:comment>
        <rdfs:comment xml:lang="fr">Liste des différents types de zones d&apos;activité et d&apos;intérêt, représentés comme une hiérarchie de concepts SKOS.</rdfs:comment>
        <rdfs:label xml:lang="fr">Type de ZAI</rdfs:label>
        <rdfs:label xml:lang="en">Type of AOI</rdfs:label>
        <skos:hasTopConcept rdf:resource="http://data.ign.fr/id/codes/topo/typedezai/PAIAdministratifOuMilitaire"/>
        <skos:hasTopConcept rdf:resource="http://data.ign.fr/id/codes/topo/typedezai/PAICultureLoisirs"/>
        <skos:hasTopConcept rdf:resource="http://data.ign.fr/id/codes/topo/typedezai/PAIEspaceNaturel"/>
        <skos:hasTopConcept rdf:resource="http://data.ign.fr/id/codes/topo/typedezai/PAIGestionEaux"/>
        <skos:hasTopConcept rdf:resource="http://data.ign.fr/id/codes/topo/typedezai/PAIHydrographie"/>
        <skos:hasTopConcept rdf:resource="http://data.ign.fr/id/codes/topo/typedezai/PAIIndustrielCommercial"/>
        <skos:hasTopConcept rdf:resource="http://data.ign.fr/id/codes/topo/typedezai/PAIOrographie"/>
        <skos:hasTopConcept rdf:resource="http://data.ign.fr/id/codes/topo/typedezai/PAIReligieux"/>
        <skos:hasTopConcept rdf:resource="http://data.ign.fr/id/codes/topo/typedezai/PAISante"/>
        <skos:hasTopConcept rdf:resource="http://data.ign.fr/id/codes/topo/typedezai/PAIScienceEnseignement"/>
        <skos:hasTopConcept rdf:resource="http://data.ign.fr/id/codes/topo/typedezai/PAISport"/>
        <skos:hasTopConcept rdf:resource="http://data.ign.fr/id/codes/topo/typedezai/PAITransport"/>
        <skos:hasTopConcept rdf:resource="http://data.ign.fr/id/codes/topo/typedezai/PAIZoneHabitation"/>
    </owl:NamedIndividual>
    


    <!-- http://www.eurecom.fr/~atemezin/ -->


    <owl:NamedIndividual rdf:about="http://www.eurecom.fr/~atemezin/">
        <rdf:type rdf:resource="http://xmlns.com/foaf/0.1/Person"/>
    </owl:NamedIndividual>
    <rdf:Description rdf:nodeID="genid82">
        <rdf:type rdf:resource="http://xmlns.com/foaf/0.1/Person"/>
        <org:hasMembership>
            <rdf:Description rdf:nodeID="genid83">
                <rdf:type rdf:resource="http://www.w3.org/ns/org#Membership"/>
                <org:memberDuring>
                    <rdf:Description rdf:nodeID="genid84">
                        <rdf:type rdf:resource="http://www.w3.org/2006/time#Interval"/>
                        <time:hasBeginning>
                            <rdf:Description rdf:nodeID="genid85">
                                <rdf:type rdf:resource="http://www.w3.org/2006/time#Instant"/>
                                <time:inXSDDateTimeStamp rdf:datatype="http://www.w3.org/2001/XMLSchema#dateTimeStamp">2005-09-09</time:inXSDDateTimeStamp>
                            </rdf:Description>
                        </time:hasBeginning>
                    </rdf:Description>
                </org:memberDuring>
                <org:organization rdf:resource="http://recherche.ign.fr/"/>
                <org:organization rdf:resource="http://www.ign.fr/"/>
                <org:role>
                    <rdf:Description rdf:nodeID="genid86">
                        <rdf:type rdf:resource="http://www.w3.org/ns/org#Role"/>
                        <rdfs:label xml:lang="fr">Chargée de recherche</rdfs:label>
                        <rdfs:label xml:lang="en">Survey engineer and Scientist</rdfs:label>
                    </rdf:Description>
                </org:role>
            </rdf:Description>
        </org:hasMembership>
        <foaf:family_name>Abadie</foaf:family_name>
        <foaf:firstName>Nathalie</foaf:firstName>
        <foaf:mbox rdf:resource="mailto:nathalie-f.abadie@ign.fr"/>
        <foaf:name>Nathalie Abadie</foaf:name>
        <foaf:workInfoHomepage rdf:resource="http://recherche.ign.fr/labos/cogit/cv.php?prenom=Nathalie&amp;nom=Abadie"/>
    </rdf:Description>
    <rdf:Description rdf:nodeID="genid87">
        <rdf:type rdf:resource="http://xmlns.com/foaf/0.1/Person"/>
        <org:hasMembership>
            <rdf:Description rdf:nodeID="genid88">
                <rdf:type rdf:resource="http://www.w3.org/ns/org#Membership"/>
                <org:memberDuring>
                    <rdf:Description rdf:nodeID="genid89">
                        <rdf:type rdf:resource="http://www.w3.org/2006/time#Interval"/>
                        <time:hasBeginning>
                            <rdf:Description rdf:nodeID="genid90">
                                <rdf:type rdf:resource="http://www.w3.org/2006/time#Instant"/>
                                <time:inXSDDateTimeStamp rdf:datatype="http://www.w3.org/2001/XMLSchema#dateTimeStamp">2014-04-01T00:00:00+08:00</time:inXSDDateTimeStamp>
                            </rdf:Description>
                        </time:hasBeginning>
                    </rdf:Description>
                </org:memberDuring>
                <org:organization rdf:resource="http://dbpedia.org/resource/JPL"/>
                <org:organization rdf:resource="https://www.jpl.nasa.gov"/>
                <org:role>
                    <rdf:Description rdf:nodeID="genid91">
                        <rdf:type rdf:resource="http://www.w3.org/ns/org#Role"/>
                        <rdfs:label>Data Scientist</rdfs:label>
                    </rdf:Description>
                </org:role>
            </rdf:Description>
        </org:hasMembership>
        <foaf:family_name>McGibbney</foaf:family_name>
        <foaf:firstName>Lewis J</foaf:firstName>
        <foaf:mbox rdf:resource="mailto:lewis.j.mcgibbney@jpl.nasa.gov"/>
        <foaf:name>Lewis John McGibbney</foaf:name>
    </rdf:Description>
</rdf:RDF>



<!-- Generated by the OWL API (version 5.1.9) https://github.com/owlcs/owlapi/ -->


